PREFIX dcterms: <http://purl.org/dc/terms/>
PREFIX prov: <http://www.w3.org/ns/prov#>
PREFIX schema: <https://schema.org/>
PREFIX skos: <http://www.w3.org/2004/02/skos/core#>
PREFIX xsd: <http://www.w3.org/2001/XMLSchema#>

<http://example.com/digComp/135ca7d8-bf57-44e8-ba27-0016a0871dda>
    a skos:Concept ;
    dcterms:created "2025-02-25T23:24:36.838000+00:00"^^xsd:dateTime ;
    dcterms:creator <https://ror.org/04j5wtv36> ;
    dcterms:modified "2025-03-03T05:46:47.340000+00:00"^^xsd:dateTime ;
    dcterms:source "https://joint-research-centre.ec.europa.eu/scientific-activities-z/education-and-training/digital-transformation-education/digital-competence-framework-citizens-digcomp_en"^^xsd:anyURI ;
    skos:broader <http://example.com/digComp/ded05862-dc66-4564-9223-890481316a44> ;
    skos:definition "To create and manage one or multiple digital identities, to be able to protect one's own reputation, to deal with the data that one produces through several digital tools, environments and services."@en ;
    skos:inScheme <http://example.com/digComp> ;
    skos:notation "2.6" ;
    skos:prefLabel "Managing digital identity"@en ;
.

<http://example.com/digComp/22191328-30b0-4b90-8ddb-c49d38a44cd2>
    a skos:Concept ;
    dcterms:created "2025-02-25T23:24:06.313000+00:00"^^xsd:dateTime ;
    dcterms:creator <https://ror.org/04j5wtv36> ;
    dcterms:modified "2025-03-03T05:46:42.515000+00:00"^^xsd:dateTime ;
    dcterms:source "https://joint-research-centre.ec.europa.eu/scientific-activities-z/education-and-training/digital-transformation-education/digital-competence-framework-citizens-digcomp_en"^^xsd:anyURI ;
    skos:broader <http://example.com/digComp/ded05862-dc66-4564-9223-890481316a44> ;
    skos:definition "To participate in society through the use of public and private digital services. To seek opportunities for self-empowerment and for participatory citizenship through appropriate digital technologies."@en ;
    skos:inScheme <http://example.com/digComp> ;
    skos:notation "2.3" ;
    skos:prefLabel "Engaging in citizenship through digital technologies"@en ;
.

<http://example.com/digComp/3be27c3d-fc74-46c3-933c-a5c3a2dc18e9>
    a skos:Concept ;
    dcterms:created "2025-02-25T23:30:42.508000+00:00"^^xsd:dateTime ;
    dcterms:creator <https://ror.org/04j5wtv36> ;
    dcterms:modified "2025-03-03T05:47:24.323000+00:00"^^xsd:dateTime ;
    dcterms:source "https://joint-research-centre.ec.europa.eu/scientific-activities-z/education-and-training/digital-transformation-education/digital-competence-framework-citizens-digcomp_en"^^xsd:anyURI ;
    skos:broader <http://example.com/digComp/7b36b6e6-e9c6-43fa-a874-8c1bc09e46cf> ;
    skos:definition "To understand where one’s own digital competence needs to be improved or updated. To be able to support others with their digital competence development. To seek opportunities for self-development and to keep up-to-date with the digital evolution."@en ;
    skos:inScheme <http://example.com/digComp> ;
    skos:notation "5.4" ;
    skos:prefLabel "Identifying digital competence gaps"@en ;
.

<http://example.com/digComp/43d68b7a-6bcf-4e2f-bc14-4f601bb73fb0>
    a skos:Concept ;
    dcterms:created "2025-02-25T23:24:25.906000+00:00"^^xsd:dateTime ;
    dcterms:creator <https://ror.org/04j5wtv36> ;
    dcterms:modified "2025-03-03T05:46:49.530000+00:00"^^xsd:dateTime ;
    dcterms:source "https://joint-research-centre.ec.europa.eu/scientific-activities-z/education-and-training/digital-transformation-education/digital-competence-framework-citizens-digcomp_en"^^xsd:anyURI ;
    skos:broader <http://example.com/digComp/ded05862-dc66-4564-9223-890481316a44> ;
    skos:definition "To be aware of behavioural norms and know-how while using digital technologies and interacting in digital environments. To adapt communication strategies to the specific audience and to be aware of cultural and generational diversity in digital environments."@en ;
    skos:inScheme <http://example.com/digComp> ;
    skos:notation "2.5" ;
    skos:prefLabel "Netiquette"@en ;
.

<http://example.com/digComp/4a0b2c9c-9a1a-4530-95bb-607321707d1d>
    a skos:Concept ;
    dcterms:created "2025-02-25T23:26:58.910000+00:00"^^xsd:dateTime ;
    dcterms:creator <https://ror.org/04j5wtv36> ;
    dcterms:modified "2025-03-03T05:46:57.811000+00:00"^^xsd:dateTime ;
    dcterms:source "https://joint-research-centre.ec.europa.eu/scientific-activities-z/education-and-training/digital-transformation-education/digital-competence-framework-citizens-digcomp_en"^^xsd:anyURI ;
    skos:broader <http://example.com/digComp/6e024199-248f-40cb-84c3-c0ae3dd36e06> ;
    skos:definition "To understand how copyright and licences apply to data, information and digital content."@en ;
    skos:inScheme <http://example.com/digComp> ;
    skos:notation "3.3" ;
    skos:prefLabel "Copyright and licenses"@en ;
.

<http://example.com/digComp/4b7ad738-5959-422c-aacf-0ce9c4073e77>
    a skos:Concept ;
    dcterms:created "2025-02-25T23:23:47.973000+00:00"^^xsd:dateTime ;
    dcterms:creator <https://ror.org/04j5wtv36> ;
    dcterms:modified "2025-03-03T05:46:51.648000+00:00"^^xsd:dateTime ;
    dcterms:source "https://joint-research-centre.ec.europa.eu/scientific-activities-z/education-and-training/digital-transformation-education/digital-competence-framework-citizens-digcomp_en"^^xsd:anyURI ;
    skos:broader <http://example.com/digComp/ded05862-dc66-4564-9223-890481316a44> ;
    skos:definition "To share data, information and digital content with others through appropriate digital technologies. To act as an intermediary, to know about referencing and attribution practices."@en ;
    skos:inScheme <http://example.com/digComp> ;
    skos:notation "2.2" ;
    skos:prefLabel "Sharing information and content thro"@en ;
.

<http://example.com/digComp/5aed599f-7889-4a73-8e74-90e592c38467>
    a skos:Concept ;
    dcterms:created "2025-02-25T23:28:17.277000+00:00"^^xsd:dateTime ;
    dcterms:creator <https://ror.org/04j5wtv36> ;
    dcterms:modified "2025-03-03T05:47:40.728000+00:00"^^xsd:dateTime ;
    dcterms:source "https://joint-research-centre.ec.europa.eu/scientific-activities-z/education-and-training/digital-transformation-education/digital-competence-framework-citizens-digcomp_en"^^xsd:anyURI ;
    skos:broader <http://example.com/digComp/a4f9a0b6-3415-471d-8eb1-72fcbbf0800b> ;
    skos:definition "To protect personal data and privacy in digital environments. To understand how to use and share personally identifiable information while being able to protect oneself and others from damages. To understand that digital services use a “Privacy policy” to inform how personal data is used."@en ;
    skos:inScheme <http://example.com/digComp> ;
    skos:notation "4.2" ;
    skos:prefLabel "Protecting personal data and privacy"@en ;
.

<http://example.com/digComp/5ee39c36-4d89-4bfb-97bc-d1b904386960>
    a skos:Concept ;
    dcterms:created "2025-02-25T23:18:04.291000+00:00"^^xsd:dateTime ;
    dcterms:creator <https://ror.org/04j5wtv36> ;
    dcterms:modified "2025-03-03T05:47:12.460000+00:00"^^xsd:dateTime ;
    dcterms:source "https://joint-research-centre.ec.europa.eu/scientific-activities-z/education-and-training/digital-transformation-education/digital-competence-framework-citizens-digcomp_en"^^xsd:anyURI ;
    skos:broader <http://example.com/digComp/6a85adb3-9529-4630-85d2-8831f5be8ee6> ;
    skos:definition "To articulate information needs , to search for data, information and content in digital environments, to access them and to navigate between them. To create and update personal search strategies."@en ;
    skos:inScheme <http://example.com/digComp> ;
    skos:notation "1.1" ;
    skos:prefLabel "Browsing, searching and filtering data, information and digital content"@en ;
.

<http://example.com/digComp/63d748e7-ff24-4392-82ae-47d780c0cbee>
    a skos:Concept ;
    dcterms:created "2025-02-25T23:27:05.058000+00:00"^^xsd:dateTime ;
    dcterms:creator <https://ror.org/04j5wtv36> ;
    dcterms:modified "2025-03-03T05:47:06.906000+00:00"^^xsd:dateTime ;
    dcterms:source "https://joint-research-centre.ec.europa.eu/scientific-activities-z/education-and-training/digital-transformation-education/digital-competence-framework-citizens-digcomp_en"^^xsd:anyURI ;
    skos:broader <http://example.com/digComp/6e024199-248f-40cb-84c3-c0ae3dd36e06> ;
    skos:definition "To plan and develop a sequence of understandable instructions for a computing system to solve a given problem or perform a specific task."@en ;
    skos:inScheme <http://example.com/digComp> ;
    skos:notation "3.4" ;
    skos:prefLabel "Programming"@en ;
.

<http://example.com/digComp/776fb14b-1793-4412-a666-9629f28f7048>
    a skos:Concept ;
    dcterms:created "2025-02-25T23:28:06.406000+00:00"^^xsd:dateTime ;
    dcterms:creator <https://ror.org/04j5wtv36> ;
    dcterms:modified "2025-03-03T05:47:36.433000+00:00"^^xsd:dateTime ;
    dcterms:source "https://joint-research-centre.ec.europa.eu/scientific-activities-z/education-and-training/digital-transformation-education/digital-competence-framework-citizens-digcomp_en"^^xsd:anyURI ;
    skos:broader <http://example.com/digComp/a4f9a0b6-3415-471d-8eb1-72fcbbf0800b> ;
    skos:definition "To protect devices and digital content, and to understand risks and threats in digital environments. To know about safety and security measures and to have due regard to reliability and privacy."@en ;
    skos:inScheme <http://example.com/digComp> ;
    skos:notation "4.1" ;
    skos:prefLabel "Protecting devices"@en ;
.

<http://example.com/digComp/8ab59992-805e-42ce-8de1-bb5da0d8c32a>
    a skos:Concept ;
    dcterms:created "2025-02-25T23:28:28.850000+00:00"^^xsd:dateTime ;
    dcterms:creator <https://ror.org/04j5wtv36> ;
    dcterms:modified "2025-03-03T05:47:38.791000+00:00"^^xsd:dateTime ;
    dcterms:source "https://joint-research-centre.ec.europa.eu/scientific-activities-z/education-and-training/digital-transformation-education/digital-competence-framework-citizens-digcomp_en"^^xsd:anyURI ;
    skos:broader <http://example.com/digComp/a4f9a0b6-3415-471d-8eb1-72fcbbf0800b> ;
    skos:definition "To be able to avoid health-risks and threats to physical and psychological well-being while using digital technologies. To be able to protect oneself and others from possible dangers in digital environments (e.g. cyber bullying). To be aware of digital technologies for social well-being and social inclusion."@en ;
    skos:inScheme <http://example.com/digComp> ;
    skos:notation "4.3" ;
    skos:prefLabel "Protecting health and well-being"@en ;
.

<http://example.com/digComp/9ef843e5-a771-4fed-896c-27070a8173bb>
    a skos:Concept ;
    dcterms:created "2025-02-25T23:18:23.925000+00:00"^^xsd:dateTime ;
    dcterms:creator <https://ror.org/04j5wtv36> ;
    dcterms:modified "2025-03-03T05:47:14.565000+00:00"^^xsd:dateTime ;
    dcterms:source "https://joint-research-centre.ec.europa.eu/scientific-activities-z/education-and-training/digital-transformation-education/digital-competence-framework-citizens-digcomp_en"^^xsd:anyURI ;
    skos:broader <http://example.com/digComp/6a85adb3-9529-4630-85d2-8831f5be8ee6> ;
    skos:definition "To analyse, compare and critically evaluate the credibility and reliability of sources of data, information and digital content. To analyse, interpret and critically evaluate the data, information and digital content."@en ;
    skos:inScheme <http://example.com/digComp> ;
    skos:notation "1.2" ;
    skos:prefLabel "Evaluating data, information and digital content"@en ;
.

<http://example.com/digComp/ad231929-18d3-4001-b955-df68b1b0e305>
    a skos:Concept ;
    dcterms:created "2025-02-25T23:30:01.344000+00:00"^^xsd:dateTime ;
    dcterms:creator <https://ror.org/04j5wtv36> ;
    dcterms:modified "2025-03-03T05:47:26.509000+00:00"^^xsd:dateTime ;
    dcterms:source "https://joint-research-centre.ec.europa.eu/scientific-activities-z/education-and-training/digital-transformation-education/digital-competence-framework-citizens-digcomp_en"^^xsd:anyURI ;
    skos:broader <http://example.com/digComp/7b36b6e6-e9c6-43fa-a874-8c1bc09e46cf> ;
    skos:definition "To assess needs and to identify, evaluate, select and use digital tools and possible technological responses to solve them. To adjust and customise digital environments to personal needs (e.g. accessibility)."@en ;
    skos:inScheme <http://example.com/digComp> ;
    skos:notation "5.2" ;
    skos:prefLabel "Identifying needs and technologial responses"@en ;
.

<http://example.com/digComp/b0d88c6e-42da-44ab-a156-51e0b14f0180>
    a skos:Concept ;
    dcterms:created "2025-02-25T23:23:34.086000+00:00"^^xsd:dateTime ;
    dcterms:creator <https://ror.org/04j5wtv36> ;
    dcterms:modified "2025-03-03T05:46:44.689000+00:00"^^xsd:dateTime ;
    dcterms:source "https://joint-research-centre.ec.europa.eu/scientific-activities-z/education-and-training/digital-transformation-education/digital-competence-framework-citizens-digcomp_en"^^xsd:anyURI ;
    skos:broader <http://example.com/digComp/ded05862-dc66-4564-9223-890481316a44> ;
    skos:definition "To interact through a variety of digital technologies and to understand appropriate digital communication means for a given context."@en ;
    skos:inScheme <http://example.com/digComp> ;
    skos:notation "2.1" ;
    skos:prefLabel "Interacting through digital technologies"@en ;
.

<http://example.com/digComp/c31c4623-ece5-4c15-be4e-f6d5bde77e71>
    a skos:Concept ;
    dcterms:created "2025-02-25T23:26:47.952000+00:00"^^xsd:dateTime ;
    dcterms:creator <https://ror.org/04j5wtv36> ;
    dcterms:modified "2025-03-03T05:47:02.328000+00:00"^^xsd:dateTime ;
    dcterms:source "https://joint-research-centre.ec.europa.eu/scientific-activities-z/education-and-training/digital-transformation-education/digital-competence-framework-citizens-digcomp_en"^^xsd:anyURI ;
    skos:broader <http://example.com/digComp/6e024199-248f-40cb-84c3-c0ae3dd36e06> ;
    skos:definition "To modify, refine, improve and integrate information and content into an existing body of knowledge to create new, original and relevant content and knowledge."@en ;
    skos:inScheme <http://example.com/digComp> ;
    skos:notation "3.2" ;
    skos:prefLabel "Integrating and re-elaborating digital content"@en ;
.

<http://example.com/digComp/ccd20172-7e9c-4d36-9aba-3a0986081c65>
    a skos:Concept ;
    dcterms:created "2025-02-25T23:18:36.527000+00:00"^^xsd:dateTime ;
    dcterms:creator <https://ror.org/04j5wtv36> ;
    dcterms:modified "2025-03-03T05:47:16.662000+00:00"^^xsd:dateTime ;
    dcterms:source "https://joint-research-centre.ec.europa.eu/scientific-activities-z/education-and-training/digital-transformation-education/digital-competence-framework-citizens-digcomp_en"^^xsd:anyURI ;
    skos:broader <http://example.com/digComp/6a85adb3-9529-4630-85d2-8831f5be8ee6> ;
    skos:definition "To organise, store and retrieve data, information and content in digital environments. To organise and process them in a structured environment."@en ;
    skos:inScheme <http://example.com/digComp> ;
    skos:notation "1.3" ;
    skos:prefLabel "Managing data, information and digital content"@en ;
.

<http://example.com/digComp/d1aec613-7e6c-4e8a-bb49-f7273fc4c5fe>
    a skos:Concept ;
    dcterms:created "2025-02-25T23:28:38.066000+00:00"^^xsd:dateTime ;
    dcterms:creator <https://ror.org/04j5wtv36> ;
    dcterms:modified "2025-03-03T05:47:43.781000+00:00"^^xsd:dateTime ;
    dcterms:source "https://joint-research-centre.ec.europa.eu/scientific-activities-z/education-and-training/digital-transformation-education/digital-competence-framework-citizens-digcomp_en"^^xsd:anyURI ;
    skos:broader <http://example.com/digComp/a4f9a0b6-3415-471d-8eb1-72fcbbf0800b> ;
    skos:definition "To be aware of the environmental impact of digital technologies and their use."@en ;
    skos:inScheme <http://example.com/digComp> ;
    skos:notation "4.4" ;
    skos:prefLabel "Protecting the environment"@en ;
.

<http://example.com/digComp/d6bb5cf7-1480-402a-9eb3-a511eb4cb945>
    a skos:Concept ;
    dcterms:created "2025-02-25T23:24:18.416000+00:00"^^xsd:dateTime ;
    dcterms:creator <https://ror.org/04j5wtv36> ;
    dcterms:modified "2025-03-03T05:46:40.470000+00:00"^^xsd:dateTime ;
    dcterms:source "https://joint-research-centre.ec.europa.eu/scientific-activities-z/education-and-training/digital-transformation-education/digital-competence-framework-citizens-digcomp_en"^^xsd:anyURI ;
    skos:broader <http://example.com/digComp/ded05862-dc66-4564-9223-890481316a44> ;
    skos:definition "To use digital tools and technologies for collaborative processes, and for co-construction and co-creation of resources and knowledge."@en ;
    skos:inScheme <http://example.com/digComp> ;
    skos:notation "2.4" ;
    skos:prefLabel "Collaborating through digital technologies"@en ;
.

<http://example.com/digComp/e3c81318-0964-4d71-ba5f-b85c099d4bf9>
    a skos:Concept ;
    dcterms:created "2025-02-25T23:26:32.363000+00:00"^^xsd:dateTime ;
    dcterms:creator <https://ror.org/04j5wtv36> ;
    dcterms:modified "2025-03-03T05:47:00.468000+00:00"^^xsd:dateTime ;
    dcterms:source "https://joint-research-centre.ec.europa.eu/scientific-activities-z/education-and-training/digital-transformation-education/digital-competence-framework-citizens-digcomp_en"^^xsd:anyURI ;
    skos:broader <http://example.com/digComp/6e024199-248f-40cb-84c3-c0ae3dd36e06> ;
    skos:definition "To create and edit digital content in different formats, to express oneself through digital means."@en ;
    skos:inScheme <http://example.com/digComp> ;
    skos:notation "3.1" ;
    skos:prefLabel "Developing digital content"@en ;
.

<http://example.com/digComp/e89ea019-00b8-40ee-8f36-4c67ee247fc9>
    a skos:Concept ;
    dcterms:created "2025-02-25T23:30:24.792000+00:00"^^xsd:dateTime ;
    dcterms:creator <https://ror.org/04j5wtv36> ;
    dcterms:modified "2025-03-03T05:47:22.111000+00:00"^^xsd:dateTime ;
    dcterms:source "https://joint-research-centre.ec.europa.eu/scientific-activities-z/education-and-training/digital-transformation-education/digital-competence-framework-citizens-digcomp_en"^^xsd:anyURI ;
    skos:broader <http://example.com/digComp/7b36b6e6-e9c6-43fa-a874-8c1bc09e46cf> ;
    skos:definition "To use digital tools and technologies to create knowledge and to innovate processes and products. To engage individually and collectively in cognitive processing to understand and resolve conceptual problems and problem situations in digital environments."@en ;
    skos:inScheme <http://example.com/digComp> ;
    skos:notation "5.3" ;
    skos:prefLabel "Creatively using digital technologies"@en ;
.

<http://example.com/digComp/effcbb68-404b-4093-b9df-66f98a46c50f>
    a skos:Concept ;
    dcterms:created "2025-02-25T23:29:41.155000+00:00"^^xsd:dateTime ;
    dcterms:creator <https://ror.org/04j5wtv36> ;
    dcterms:modified "2025-03-03T05:47:28.629000+00:00"^^xsd:dateTime ;
    dcterms:source "https://joint-research-centre.ec.europa.eu/scientific-activities-z/education-and-training/digital-transformation-education/digital-competence-framework-citizens-digcomp_en"^^xsd:anyURI ;
    skos:broader <http://example.com/digComp/7b36b6e6-e9c6-43fa-a874-8c1bc09e46cf> ;
    skos:definition "To identify technical problems when operating devices and using digital environments, and to solve them (from trouble-shooting to solving more complex problems)."@en ;
    skos:inScheme <http://example.com/digComp> ;
    skos:notation "5.1" ;
    skos:prefLabel "Solving technical problems"@en ;
.

<http://example.com/digComp/6a85adb3-9529-4630-85d2-8831f5be8ee6>
    a skos:Concept ;
    dcterms:created "2025-02-25T23:15:39.154000+00:00"^^xsd:dateTime ;
    dcterms:creator <https://ror.org/04j5wtv36> ;
    dcterms:modified "2025-03-03T05:46:29.564000+00:00"^^xsd:dateTime ;
    dcterms:source "https://joint-research-centre.ec.europa.eu/scientific-activities-z/education-and-training/digital-transformation-education/digital-competence-framework-citizens-digcomp_en"^^xsd:anyURI ;
    skos:definition "To articulate information needs, to locate and retrieve digital data, information and content. To judge the relevance of the source and its content. To store, manage, and organise digital data, information and content."@en ;
    skos:inScheme <http://example.com/digComp> ;
    skos:narrower
        <http://example.com/digComp/5ee39c36-4d89-4bfb-97bc-d1b904386960> ,
        <http://example.com/digComp/9ef843e5-a771-4fed-896c-27070a8173bb> ,
        <http://example.com/digComp/ccd20172-7e9c-4d36-9aba-3a0986081c65> ;
    skos:notation "1" ;
    skos:prefLabel "Information and data literacy"@en ;
    skos:topConceptOf <http://example.com/digComp> ;
.

<http://example.com/digComp/6e024199-248f-40cb-84c3-c0ae3dd36e06>
    a skos:Concept ;
    dcterms:created "2025-02-25T23:16:08.407000+00:00"^^xsd:dateTime ;
    dcterms:creator <https://ror.org/04j5wtv36> ;
    dcterms:modified "2025-03-03T05:46:23.883000+00:00"^^xsd:dateTime ;
    dcterms:source "https://joint-research-centre.ec.europa.eu/scientific-activities-z/education-and-training/digital-transformation-education/digital-competence-framework-citizens-digcomp_en"^^xsd:anyURI ;
    skos:definition "To create and edit digital content. To improve and integrate information and content into an existing body of knowledge while understanding how copyright and licences are to be applied. To know how to give understandable instructions for a computer system."@en ;
    skos:inScheme <http://example.com/digComp> ;
    skos:narrower
        <http://example.com/digComp/4a0b2c9c-9a1a-4530-95bb-607321707d1d> ,
        <http://example.com/digComp/63d748e7-ff24-4392-82ae-47d780c0cbee> ,
        <http://example.com/digComp/c31c4623-ece5-4c15-be4e-f6d5bde77e71> ,
        <http://example.com/digComp/e3c81318-0964-4d71-ba5f-b85c099d4bf9> ;
    skos:notation "3" ;
    skos:prefLabel "Digital content creation"@en ;
    skos:topConceptOf <http://example.com/digComp> ;
.

<http://example.com/digComp/7b36b6e6-e9c6-43fa-a874-8c1bc09e46cf>
    a skos:Concept ;
    dcterms:created "2025-02-25T23:16:24.835000+00:00"^^xsd:dateTime ;
    dcterms:creator <https://ror.org/04j5wtv36> ;
    dcterms:modified "2025-03-03T05:46:33.432000+00:00"^^xsd:dateTime ;
    dcterms:source "https://joint-research-centre.ec.europa.eu/scientific-activities-z/education-and-training/digital-transformation-education/digital-competence-framework-citizens-digcomp_en"^^xsd:anyURI ;
    skos:definition "To identify needs and problems, and to resolve conceptual problems and problem situations in digital environments. To use digital tools to innovate processes and products. To keep up-to-date with the digital evolution."@en ;
    skos:inScheme <http://example.com/digComp> ;
    skos:narrower
        <http://example.com/digComp/3be27c3d-fc74-46c3-933c-a5c3a2dc18e9> ,
        <http://example.com/digComp/ad231929-18d3-4001-b955-df68b1b0e305> ,
        <http://example.com/digComp/e89ea019-00b8-40ee-8f36-4c67ee247fc9> ,
        <http://example.com/digComp/effcbb68-404b-4093-b9df-66f98a46c50f> ;
    skos:notation "5" ;
    skos:prefLabel "Problem solving"@en ;
    skos:topConceptOf <http://example.com/digComp> ;
.

<http://example.com/digComp/a4f9a0b6-3415-471d-8eb1-72fcbbf0800b>
    a skos:Concept ;
    dcterms:created "2025-02-25T23:16:14.179000+00:00"^^xsd:dateTime ;
    dcterms:creator <https://ror.org/04j5wtv36> ;
    dcterms:modified "2025-03-03T05:46:35.666000+00:00"^^xsd:dateTime ;
    dcterms:source "https://joint-research-centre.ec.europa.eu/scientific-activities-z/education-and-training/digital-transformation-education/digital-competence-framework-citizens-digcomp_en"^^xsd:anyURI ;
    skos:definition "To protect devices, content, personal data and privacy in digital environments. To protect physical and psychological health, and to be aware of digital technologies for social well-being and social inclusion. To be aware of the environmental impact of digital technologies and their use."@en ;
    skos:inScheme <http://example.com/digComp> ;
    skos:narrower
        <http://example.com/digComp/5aed599f-7889-4a73-8e74-90e592c38467> ,
        <http://example.com/digComp/776fb14b-1793-4412-a666-9629f28f7048> ,
        <http://example.com/digComp/8ab59992-805e-42ce-8de1-bb5da0d8c32a> ,
        <http://example.com/digComp/d1aec613-7e6c-4e8a-bb49-f7273fc4c5fe> ;
    skos:notation "4" ;
    skos:prefLabel "Safety"@en ;
    skos:topConceptOf <http://example.com/digComp> ;
.

<http://example.com/digComp/ded05862-dc66-4564-9223-890481316a44>
    a skos:Concept ;
    dcterms:created "2025-02-25T23:15:54.223000+00:00"^^xsd:dateTime ;
    dcterms:creator <https://ror.org/04j5wtv36> ;
    dcterms:modified "2025-03-07T03:29:33.221000+00:00"^^xsd:dateTime ;
    dcterms:source "https://joint-research-centre.ec.europa.eu/scientific-activities-z/education-and-training/digital-transformation-education/digital-competence-framework-citizens-digcomp_en"^^xsd:anyURI ;
    skos:definition "To interact, communicate and collaborate through digital technologies while being aware of cultural and generational diversity. To participate in society through public and private digital services and participatory citizenship. To manage one’s digital presence, identity and reputation."@en ;
    skos:inScheme <http://example.com/digComp> ;
    skos:narrower
        <http://example.com/digComp/135ca7d8-bf57-44e8-ba27-0016a0871dda> ,
        <http://example.com/digComp/22191328-30b0-4b90-8ddb-c49d38a44cd2> ,
        <http://example.com/digComp/43d68b7a-6bcf-4e2f-bc14-4f601bb73fb0> ,
        <http://example.com/digComp/4b7ad738-5959-422c-aacf-0ce9c4073e77> ,
        <http://example.com/digComp/b0d88c6e-42da-44ab-a156-51e0b14f0180> ,
        <http://example.com/digComp/d6bb5cf7-1480-402a-9eb3-a511eb4cb945> ;
    skos:notation "2" ;
    skos:prefLabel "Communication and collaboration"@en ;
    skos:topConceptOf <http://example.com/digComp> ;
.

<https://ror.org/04j5wtv36>
    a prov:Organization ;
    schema:name "Directorate-General Joint Research Centre" ;
    schema:url "https://ec.europa.eu/info/departments/joint-research-centre_en"^^xsd:anyURI ;
.

<http://example.com/digComp>
    a skos:ConceptScheme ;
    dcterms:created "2025-02-25T23:14:57.743000+00:00"^^xsd:dateTime ;
    dcterms:creator <https://ror.org/04j5wtv36> ;
    dcterms:description "Jobs and Skills Australia RDF presentation of the Digital competency framework for citizens"@en ;
    dcterms:modified "2025-02-25T23:30:42.528000+00:00"^^xsd:dateTime ;
    dcterms:publisher <https://linked.data.gov.au/org/jsa> ;
    dcterms:subject "Skills"@en ;
    dcterms:title "DigComp"@en ;
    skos:definition "Jobs and Skills Australia RDF presentation of the Digital competency framework for citizens"@en ;
    skos:hasTopConcept
        <http://example.com/digComp/6a85adb3-9529-4630-85d2-8831f5be8ee6> ,
        <http://example.com/digComp/6e024199-248f-40cb-84c3-c0ae3dd36e06> ,
        <http://example.com/digComp/7b36b6e6-e9c6-43fa-a874-8c1bc09e46cf> ,
        <http://example.com/digComp/a4f9a0b6-3415-471d-8eb1-72fcbbf0800b> ,
        <http://example.com/digComp/ded05862-dc66-4564-9223-890481316a44> ;
    skos:prefLabel "DigComp"@en ;
    schema:citation "https://joint-research-centre.ec.europa.eu/scientific-activities-z/education-and-training/digital-transformation-education/digital-competence-framework-citizens-digcomp_en"^^xsd:anyURI ;
    schema:version "3" ;
.
