@prefix rdf: <http://www.w3.org/1999/02/22-rdf-syntax-ns#> .
@prefix rdfs: <http://www.w3.org/2000/01/rdf-schema#> .
@prefix skos: <http://www.w3.org/2004/02/skos/core#> .
@prefix skosxl: <http://www.w3.org/2008/05/skos-xl#> .
@prefix owl: <http://www.w3.org/2002/07/owl#> .
@prefix dcterms: <http://purl.org/dc/terms/> .
@prefix xsd: <http://www.w3.org/2001/XMLSchema#> .
@prefix tags: <http://www.holygoat.co.uk/owl/redwood/0.1/tags/> .
@prefix dbpedia: <http://dbpedia.org/resource/> .
@prefix schema: <https://schema.org/> .
@prefix prov: <http://www.w3.org/ns/prov#> .

<http://example.com/WEFGST>
  a skos:ConceptScheme;
  dcterms:creator <https://ror.org/05wm3vw64> ;
  dcterms:publisher <https://linked.data.gov.au/org/jsa> ;
  dcterms:title "WEF Global Skills Taxonomy"@en;
  dcterms:created "2025-03-06T02:28:59.763Z"^^xsd:dateTime;
  skos:prefLabel "WEF Global Skills Taxonomy"@en;
  skos:definition "The Global Skills Taxonomy is a comprehensive, structured framework developed by the World Economic Forum and its network of partners to define, categorize, and organize the essential skills required in today’s workforce. It serves as a common language for employers, educators, and policymakers by providing standardized definitions and classifications, fostering alignment and a shared understanding of labour market trends and skill demands."@en ;
  skos:historyNote "The WEF Global Skills Taxonomy is presented here in RDF by Jobs and Skills Australia"@en ;
  dcterms:subject "Skills"@en;
  dcterms:modified "2025-03-07T04:07:12.514Z"^^xsd:dateTime;
  skos:hasTopConcept <http://example.com/WEFGST/0a9ac146-77e9-4ad3-94d5-ab9f62c8cd02> .

<https://ror.org/05wm3vw64>
a prov:Organization ;
schema:name "World Economic Forum"@en ;
schema:url "https://www.weforum.org/"^^xsd:anyURI
.

<https://linked.data.gov.au/org/jsa> 
a prov:Organization ;
schema:name "Jobs and Skills Australia"@en ;
schema:url "https://jobsandskills.gov.au"^^xsd:anyURI 
.

<http://example.com/WEFGST/0a9ac146-77e9-4ad3-94d5-ab9f62c8cd02>
  a skos:Concept;
  dcterms:created "2025-03-06T02:34:20.432Z"^^xsd:dateTime;
  dcterms:source "https://www1.reskillingrevolution2030.org/skills-taxonomy"^^xsd:anyURI ;
  skos:inScheme <http://example.com/WEFGST> ;
  skos:topConceptOf <http://example.com/WEFGST> ;
  skos:prefLabel "Skills, Knowledge and abilities"@en;
  skos:narrower <http://example.com/WEFGST/67bac4bd-6131-4b95-a6f1-a8e0eb45df9e>,
    <http://example.com/WEFGST/2b9f062d-41b8-4108-9cdf-40cc1efaf5e4>,
    <http://example.com/WEFGST/e634918b-4f3e-467b-ab1c-66aecad6fc8d>,
    <http://example.com/WEFGST/b804fbe2-e09d-4fd1-9e03-9cb5758f8b43>,
    <http://example.com/WEFGST/e8cdd6ea-4ef1-426b-9f24-e37b563559d5>;
  dcterms:modified "2025-03-07T04:07:09.592Z"^^xsd:dateTime .

<http://example.com/WEFGST/2b9f062d-41b8-4108-9cdf-40cc1efaf5e4>
  a skos:Concept;
  dcterms:created "2025-03-06T02:34:20.719Z"^^xsd:dateTime;
  dcterms:source "https://www1.reskillingrevolution2030.org/skills-taxonomy"^^xsd:anyURI ;
  skos:inScheme <http://example.com/WEFGST> ;
  skos:prefLabel "Cognitive skills"@en;
  skos:narrower <http://example.com/WEFGST/e83c6ddd-7648-4ddb-9f26-bc015304bfc7>,
    <http://example.com/WEFGST/214bf93c-d300-42cd-81e5-9c7e3ca8d481>,
    <http://example.com/WEFGST/37b553e3-7c65-413f-b6b0-7cc1a0303558>;
  dcterms:modified "2025-03-07T04:07:09.671Z"^^xsd:dateTime;
  skos:broader <http://example.com/WEFGST/0a9ac146-77e9-4ad3-94d5-ab9f62c8cd02> .

<http://example.com/WEFGST/e83c6ddd-7648-4ddb-9f26-bc015304bfc7>
  a skos:Concept;
  dcterms:created "2025-03-06T02:34:20.748Z"^^xsd:dateTime;
  dcterms:source "https://www1.reskillingrevolution2030.org/skills-taxonomy"^^xsd:anyURI ;
  skos:inScheme <http://example.com/WEFGST> ;
  skos:prefLabel "Creativity and problem solving"@en;
  skos:narrower <http://example.com/WEFGST/e5611029-38b5-4df6-9702-10f70470d6e8>,
    <http://example.com/WEFGST/9fc90204-8eb8-4e8c-9a7e-af340d766c7f>,
    <http://example.com/WEFGST/0e93e4d0-70b7-413b-8675-38655a9a3216>;
  dcterms:modified "2025-03-07T04:07:09.901Z"^^xsd:dateTime;
  skos:broader <http://example.com/WEFGST/2b9f062d-41b8-4108-9cdf-40cc1efaf5e4> .

<http://example.com/WEFGST/9fc90204-8eb8-4e8c-9a7e-af340d766c7f>
  a skos:Concept;
  dcterms:created "2025-03-06T02:34:20.809Z"^^xsd:dateTime;
  dcterms:source "https://www1.reskillingrevolution2030.org/skills-taxonomy"^^xsd:anyURI ;
  skos:definition "Capacity to break down concepts and complex ideas into basic or fundamental principles. Includes critical thinking, whereby judgements are made by analysing and interpreting facts and information."@en;
  skos:inScheme <http://example.com/WEFGST> ;
  skos:prefLabel "Analytical thinking"@en;
  dcterms:modified "2025-03-07T04:07:10.830Z"^^xsd:dateTime;
  skos:broader <http://example.com/WEFGST/e83c6ddd-7648-4ddb-9f26-bc015304bfc7> .

<http://example.com/WEFGST/e5611029-38b5-4df6-9702-10f70470d6e8>
  a skos:Concept;
  dcterms:created "2025-03-06T02:34:20.773Z"^^xsd:dateTime;
  dcterms:source "https://www1.reskillingrevolution2030.org/skills-taxonomy"^^xsd:anyURI ;
  skos:definition "Capacity to bring a new idea or concept into existence through imagination and to imagine something that does not exist."@en;
  skos:inScheme <http://example.com/WEFGST> ;
  skos:prefLabel "Creative thinking"@en;
  dcterms:modified "2025-03-07T04:07:10.784Z"^^xsd:dateTime;
  skos:broader <http://example.com/WEFGST/e83c6ddd-7648-4ddb-9f26-bc015304bfc7> .

<http://example.com/WEFGST/0e93e4d0-70b7-413b-8675-38655a9a3216>
  a skos:Concept;
  dcterms:created "2025-03-06T02:34:20.859Z"^^xsd:dateTime;
  dcterms:source "https://www1.reskillingrevolution2030.org/skills-taxonomy"^^xsd:anyURI ;
  skos:definition "Capacity to understand how concepts work together, embrace a multidisciplinary approach, and identify patterns over time."@en;
  skos:inScheme <http://example.com/WEFGST> ;
  skos:prefLabel "Systems thinking"@en;
  dcterms:modified "2025-03-07T04:07:10.875Z"^^xsd:dateTime;
  skos:broader <http://example.com/WEFGST/e83c6ddd-7648-4ddb-9f26-bc015304bfc7> .

<http://example.com/WEFGST/214bf93c-d300-42cd-81e5-9c7e3ca8d481>
  a skos:Concept;
  dcterms:created "2025-03-06T02:34:20.926Z"^^xsd:dateTime;
  dcterms:source "https://www1.reskillingrevolution2030.org/skills-taxonomy"^^xsd:anyURI ;
  skos:inScheme <http://example.com/WEFGST> ;
  skos:prefLabel "Mathematical and statistical thinking"@en;
  skos:narrower <http://example.com/WEFGST/be1fcf9a-62e4-4113-80b1-4631cf2f739a>,
    <http://example.com/WEFGST/d3dfd17d-0342-4ede-b276-b265c254719a>,
    <http://example.com/WEFGST/769a56e3-0441-4e94-8486-b507f029775d>,
    <http://example.com/WEFGST/bac12539-a0a6-4f1a-8f27-cdb635c5dc7f>;
  dcterms:modified "2025-03-07T04:07:09.941Z"^^xsd:dateTime;
  skos:broader <http://example.com/WEFGST/2b9f062d-41b8-4108-9cdf-40cc1efaf5e4> .

<http://example.com/WEFGST/769a56e3-0441-4e94-8486-b507f029775d>
  a skos:Concept;
  dcterms:created "2025-03-06T02:34:21.464Z"^^xsd:dateTime;
  dcterms:source "https://www1.reskillingrevolution2030.org/skills-taxonomy"^^xsd:anyURI ;
  skos:definition "Solving equations and using advanced mathematical techniques."@en;
  skos:inScheme <http://example.com/WEFGST> ;
  skos:prefLabel "Algebraic facility"@en;
  dcterms:modified "2025-03-07T04:07:10.995Z"^^xsd:dateTime;
  skos:broader <http://example.com/WEFGST/214bf93c-d300-42cd-81e5-9c7e3ca8d481> .

<http://example.com/WEFGST/d3dfd17d-0342-4ede-b276-b265c254719a>
  a skos:Concept;
  dcterms:created "2025-03-06T02:34:21.442Z"^^xsd:dateTime;
  dcterms:source "https://www1.reskillingrevolution2030.org/skills-taxonomy"^^xsd:anyURI ;
  skos:definition "The ability to synthesise quantitative information into pertinent calculations or estimates given precise or approximate information."@en;
  skos:inScheme <http://example.com/WEFGST> ;
  skos:prefLabel "Calculating and estimating"@en;
  dcterms:modified "2025-03-07T04:07:10.954Z"^^xsd:dateTime;
  skos:broader <http://example.com/WEFGST/214bf93c-d300-42cd-81e5-9c7e3ca8d481> .

<http://example.com/WEFGST/bac12539-a0a6-4f1a-8f27-cdb635c5dc7f>
  a skos:Concept;
  dcterms:created "2025-03-06T02:34:21.486Z"^^xsd:dateTime;
  dcterms:source "https://www1.reskillingrevolution2030.org/skills-taxonomy"^^xsd:anyURI ;
  skos:definition "Making statistical inferences from data and using statistical techniques to determine the properties of complex systems."@en;
  skos:inScheme <http://example.com/WEFGST> ;
  skos:prefLabel "Data analysis and mathematical modelling"@en;
  dcterms:modified "2025-03-07T04:07:11.038Z"^^xsd:dateTime;
  skos:broader <http://example.com/WEFGST/214bf93c-d300-42cd-81e5-9c7e3ca8d481> .

<http://example.com/WEFGST/be1fcf9a-62e4-4113-80b1-4631cf2f739a>
  a skos:Concept;
  dcterms:created "2025-03-06T02:34:21.422Z"^^xsd:dateTime;
  dcterms:source "https://www1.reskillingrevolution2030.org/skills-taxonomy"^^xsd:anyURI ;
  skos:definition "The ability to rapidly and accurately add, subtract, multiply and divide."@en;
  skos:inScheme <http://example.com/WEFGST> ;
  skos:prefLabel "Number facility"@en;
  dcterms:modified "2025-03-07T04:07:10.914Z"^^xsd:dateTime;
  skos:broader <http://example.com/WEFGST/214bf93c-d300-42cd-81e5-9c7e3ca8d481> .

<http://example.com/WEFGST/37b553e3-7c65-413f-b6b0-7cc1a0303558>
  a skos:Concept;
  dcterms:created "2025-03-06T02:34:21.506Z"^^xsd:dateTime;
  dcterms:source "https://www1.reskillingrevolution2030.org/skills-taxonomy"^^xsd:anyURI ;
  skos:inScheme <http://example.com/WEFGST> ;
  skos:prefLabel "Speaking, writing and languages"@en;
  skos:narrower <http://example.com/WEFGST/cb1c2879-c53c-4c2c-9f07-d612e18708e8>,
    <http://example.com/WEFGST/0708e1fd-8fe3-43e7-80e1-40cd9b0bbfcd>,
    <http://example.com/WEFGST/cf8eae15-d451-4446-97ba-3449435cc3c4>,
    <http://example.com/WEFGST/fa59733b-a8fe-4f80-b499-f2d959541ecd>,
    <http://example.com/WEFGST/994dd3d5-ca81-44a0-bbcb-4ed2cec95a86>;
  dcterms:modified "2025-03-07T04:07:09.981Z"^^xsd:dateTime;
  skos:broader <http://example.com/WEFGST/2b9f062d-41b8-4108-9cdf-40cc1efaf5e4> .

<http://example.com/WEFGST/cb1c2879-c53c-4c2c-9f07-d612e18708e8>
  a skos:Concept;
  dcterms:created "2025-03-06T02:34:21.526Z"^^xsd:dateTime;
  dcterms:source "https://www1.reskillingrevolution2030.org/skills-taxonomy"^^xsd:anyURI ;
  skos:definition "Understanding written sentences and paragraphs in work-related documents."@en;
  skos:inScheme <http://example.com/WEFGST> ;
  skos:prefLabel "Reading"@en;
  dcterms:modified "2025-03-07T04:07:11.077Z"^^xsd:dateTime;
  skos:broader <http://example.com/WEFGST/37b553e3-7c65-413f-b6b0-7cc1a0303558> .

<http://example.com/WEFGST/0708e1fd-8fe3-43e7-80e1-40cd9b0bbfcd>
  a skos:Concept;
  dcterms:created "2025-03-06T02:34:21.547Z"^^xsd:dateTime;
  dcterms:source "https://www1.reskillingrevolution2030.org/skills-taxonomy"^^xsd:anyURI ;
  skos:definition "Talking to others to convey information effectively."@en;
  skos:inScheme <http://example.com/WEFGST> ;
  skos:prefLabel "Speaking"@en;
  dcterms:modified "2025-03-07T04:07:11.117Z"^^xsd:dateTime;
  skos:broader <http://example.com/WEFGST/37b553e3-7c65-413f-b6b0-7cc1a0303558> .

<http://example.com/WEFGST/fa59733b-a8fe-4f80-b499-f2d959541ecd>
  a skos:Concept;
  dcterms:created "2025-03-06T02:34:21.594Z"^^xsd:dateTime;
  dcterms:source "https://www1.reskillingrevolution2030.org/skills-taxonomy"^^xsd:anyURI ;
  skos:definition "Synthesising text resources into a coherent narrative with a specified style or for a target audience."@en;
  skos:inScheme <http://example.com/WEFGST> ;
  skos:prefLabel "Editing"@en;
  dcterms:modified "2025-03-07T04:07:11.194Z"^^xsd:dateTime;
  skos:broader <http://example.com/WEFGST/37b553e3-7c65-413f-b6b0-7cc1a0303558> .

<http://example.com/WEFGST/994dd3d5-ca81-44a0-bbcb-4ed2cec95a86>
  a skos:Concept;
  dcterms:created "2025-03-06T02:34:21.620Z"^^xsd:dateTime;
  dcterms:source "https://www1.reskillingrevolution2030.org/skills-taxonomy"^^xsd:anyURI ;
  skos:definition "Communicating through reading, writing, speaking and listening in foreign languages."@en;
  skos:inScheme <http://example.com/WEFGST> ;
  skos:prefLabel "Multi-lingualism"@en;
  dcterms:modified "2025-03-07T04:07:11.234Z"^^xsd:dateTime;
  skos:broader <http://example.com/WEFGST/37b553e3-7c65-413f-b6b0-7cc1a0303558> .

<http://example.com/WEFGST/cf8eae15-d451-4446-97ba-3449435cc3c4>
  a skos:Concept;
  dcterms:created "2025-03-06T02:34:21.569Z"^^xsd:dateTime;
  dcterms:source "https://www1.reskillingrevolution2030.org/skills-taxonomy"^^xsd:anyURI ;
  skos:definition "Communicating effectively in writing as appropriate for the needs of the audience."@en;
  skos:inScheme <http://example.com/WEFGST> ;
  skos:prefLabel "Writing"@en;
  dcterms:modified "2025-03-07T04:07:11.155Z"^^xsd:dateTime;
  skos:broader <http://example.com/WEFGST/37b553e3-7c65-413f-b6b0-7cc1a0303558> .

<http://example.com/WEFGST/67bac4bd-6131-4b95-a6f1-a8e0eb45df9e>
  a skos:Concept;
  dcterms:created "2025-03-06T02:34:20.454Z"^^xsd:dateTime;
  dcterms:source "https://www1.reskillingrevolution2030.org/skills-taxonomy"^^xsd:anyURI ;
  skos:inScheme <http://example.com/WEFGST> ;
  skos:prefLabel "Physical abilities"@en;
  skos:narrower <http://example.com/WEFGST/898b7810-2ecc-46c6-a1b3-e452d07af9c8>,
    <http://example.com/WEFGST/595b98f9-24b7-4696-9eb0-e6d7e63a796a>;
  dcterms:modified "2025-03-07T04:07:09.632Z"^^xsd:dateTime;
  skos:broader <http://example.com/WEFGST/0a9ac146-77e9-4ad3-94d5-ab9f62c8cd02> .

<http://example.com/WEFGST/595b98f9-24b7-4696-9eb0-e6d7e63a796a>
  a skos:Concept;
  dcterms:created "2025-03-06T02:34:20.579Z"^^xsd:dateTime;
  dcterms:source "https://www1.reskillingrevolution2030.org/skills-taxonomy"^^xsd:anyURI ;
  skos:inScheme <http://example.com/WEFGST> ;
  skos:prefLabel "Sensory processing abilities"@en;
  skos:narrower <http://example.com/WEFGST/b20f5f85-838c-420d-8466-b7dfef7116e6>,
    <http://example.com/WEFGST/6c3f828a-790d-4312-87f0-bcff30548f93>,
    <http://example.com/WEFGST/8411e4ca-00f0-4245-9dff-4549f0828bad>,
    <http://example.com/WEFGST/f8b49cc1-ad8e-4d00-8d19-b669e2b265d5>;
  dcterms:modified "2025-03-14T03:29:13.890Z"^^xsd:dateTime;
  skos:broader <http://example.com/WEFGST/67bac4bd-6131-4b95-a6f1-a8e0eb45df9e> .

<http://example.com/WEFGST/8411e4ca-00f0-4245-9dff-4549f0828bad>
  a skos:Concept;
  dcterms:created "2025-03-06T02:34:20.650Z"^^xsd:dateTime;
  dcterms:source "https://www1.reskillingrevolution2030.org/skills-taxonomy"^^xsd:anyURI ;
  skos:definition "The ability to remember and organise information, identify patterns and differences, concentrate, and shift attention between sources of information."@en;
  skos:inScheme <http://example.com/WEFGST> ;
  skos:prefLabel "Information-processing abilities"@en;
  dcterms:modified "2025-03-07T04:07:10.701Z"^^xsd:dateTime;
  skos:broader <http://example.com/WEFGST/595b98f9-24b7-4696-9eb0-e6d7e63a796a> .

<http://example.com/WEFGST/b20f5f85-838c-420d-8466-b7dfef7116e6>
  a skos:Concept;
  dcterms:created "2025-03-06T02:34:20.604Z"^^xsd:dateTime;
  dcterms:source "https://www1.reskillingrevolution2030.org/skills-taxonomy"^^xsd:anyURI ;
  skos:definition "Abilities relating to resolving details, perceiving depth, differentiating colours and intensities, and seeing in low light, at oblique angles and in bright lighting."@en;
  skos:inScheme <http://example.com/WEFGST> ;
  skos:prefLabel "Visual abilities"@en;
  dcterms:modified "2025-03-07T04:07:10.617Z"^^xsd:dateTime;
  skos:broader <http://example.com/WEFGST/595b98f9-24b7-4696-9eb0-e6d7e63a796a> .

<http://example.com/WEFGST/f8b49cc1-ad8e-4d00-8d19-b669e2b265d5>
  a skos:Concept;
  dcterms:created "2025-03-06T02:34:20.681Z"^^xsd:dateTime;
  dcterms:source "https://www1.reskillingrevolution2030.org/skills-taxonomy"^^xsd:anyURI ;
  skos:definition "The ability to mentally manipulate objects and perceive locations relative to an environment."@en;
  skos:inScheme <http://example.com/WEFGST> ;
  skos:prefLabel "Spatial abilities"@en;
  dcterms:modified "2025-03-07T04:07:10.741Z"^^xsd:dateTime;
  skos:broader <http://example.com/WEFGST/595b98f9-24b7-4696-9eb0-e6d7e63a796a> .

<http://example.com/WEFGST/6c3f828a-790d-4312-87f0-bcff30548f93>
  a skos:Concept;
  dcterms:created "2025-03-06T02:34:20.626Z"^^xsd:dateTime;
  dcterms:source "https://www1.reskillingrevolution2030.org/skills-taxonomy"^^xsd:anyURI ;
  skos:definition "Abilities relating to distinguishing and isolating sounds, interpreting speech and speaking clearly."@en;
  skos:inScheme <http://example.com/WEFGST> ;
  skos:prefLabel "Auditory abilities"@en;
  dcterms:modified "2025-03-07T04:07:10.659Z"^^xsd:dateTime;
  skos:broader <http://example.com/WEFGST/595b98f9-24b7-4696-9eb0-e6d7e63a796a> .

<http://example.com/WEFGST/898b7810-2ecc-46c6-a1b3-e452d07af9c8>
  a skos:Concept;
  dcterms:created "2025-03-06T02:34:20.478Z"^^xsd:dateTime;
  dcterms:source "https://www1.reskillingrevolution2030.org/skills-taxonomy"^^xsd:anyURI ;
  skos:inScheme <http://example.com/WEFGST> ;
  skos:prefLabel "Manual dexterity, endurance and precision"@en;
  skos:narrower <http://example.com/WEFGST/fc93602c-d50f-4669-95d1-55691b5b5220>,
    <http://example.com/WEFGST/40f1f49c-6ed0-4b37-ba31-070a729831aa>,
    <http://example.com/WEFGST/b989a522-5be3-43fd-9986-557eb8d4c0cc>;
  dcterms:modified "2025-03-07T04:07:09.823Z"^^xsd:dateTime;
  skos:broader <http://example.com/WEFGST/67bac4bd-6131-4b95-a6f1-a8e0eb45df9e> .

<http://example.com/WEFGST/40f1f49c-6ed0-4b37-ba31-070a729831aa>
  a skos:Concept;
  dcterms:created "2025-03-06T02:34:20.528Z"^^xsd:dateTime;
  dcterms:source "https://www1.reskillingrevolution2030.org/skills-taxonomy"^^xsd:anyURI ;
  skos:definition "The ability to exert muscle force in short bursts or over long periods with endurance to fatigue."@en;
  skos:inScheme <http://example.com/WEFGST> ;
  skos:prefLabel "Strength and stamina"@en;
  dcterms:modified "2025-03-07T04:07:10.533Z"^^xsd:dateTime;
  skos:broader <http://example.com/WEFGST/898b7810-2ecc-46c6-a1b3-e452d07af9c8> .

<http://example.com/WEFGST/fc93602c-d50f-4669-95d1-55691b5b5220>
  a skos:Concept;
  dcterms:created "2025-03-06T02:34:20.504Z"^^xsd:dateTime;
  dcterms:source "https://www1.reskillingrevolution2030.org/skills-taxonomy"^^xsd:anyURI ;
  skos:definition "The ability to steadily, precisely and responsively grasp, manipulate, and assemble objects or adjust the controls of a machine."@en;
  skos:inScheme <http://example.com/WEFGST> ;
  skos:prefLabel "Dexterity"@en;
  dcterms:modified "2025-03-07T04:07:10.491Z"^^xsd:dateTime;
  skos:broader <http://example.com/WEFGST/898b7810-2ecc-46c6-a1b3-e452d07af9c8> .

<http://example.com/WEFGST/b989a522-5be3-43fd-9986-557eb8d4c0cc>
  a skos:Concept;
  dcterms:created "2025-03-06T02:34:20.552Z"^^xsd:dateTime;
  dcterms:source "https://www1.reskillingrevolution2030.org/skills-taxonomy"^^xsd:anyURI ;
  skos:definition "The ability to bend, stretch, twist, and reach, and coordinate these movements when the whole body is in motion, while maintaining balance and stability"@en;
  skos:inScheme <http://example.com/WEFGST> ;
  skos:prefLabel "Flexibility and coordination"@en;
  dcterms:modified "2025-03-07T04:07:10.576Z"^^xsd:dateTime;
  skos:broader <http://example.com/WEFGST/898b7810-2ecc-46c6-a1b3-e452d07af9c8> .

<http://example.com/WEFGST/b804fbe2-e09d-4fd1-9e03-9cb5758f8b43>
  a skos:Concept;
  dcterms:created "2025-03-06T02:34:21.942Z"^^xsd:dateTime;
  dcterms:source "https://www1.reskillingrevolution2030.org/skills-taxonomy"^^xsd:anyURI ;
  skos:inScheme <http://example.com/WEFGST> ;
  skos:prefLabel "Engagement skills"@en;
  skos:narrower <http://example.com/WEFGST/7f60d3b5-07d7-4bca-9ca0-78eed9298d44>,
    <http://example.com/WEFGST/89234341-1235-476f-a6c8-3cb662bfa53f>;
  dcterms:modified "2025-03-07T04:07:09.747Z"^^xsd:dateTime;
  skos:broader <http://example.com/WEFGST/0a9ac146-77e9-4ad3-94d5-ab9f62c8cd02> .

<http://example.com/WEFGST/7f60d3b5-07d7-4bca-9ca0-78eed9298d44>
  a skos:Concept;
  dcterms:created "2025-03-06T02:34:21.962Z"^^xsd:dateTime;
  dcterms:source "https://www1.reskillingrevolution2030.org/skills-taxonomy"^^xsd:anyURI ;
  skos:inScheme <http://example.com/WEFGST> ;
  skos:prefLabel "Marketing and media"@en;
  skos:narrower <http://example.com/WEFGST/dfe2bfeb-97fe-43cb-b479-b60d1c8a79b1>,
    <http://example.com/WEFGST/085e1895-ca1c-4ee3-a84a-abdd947623fd>;
  dcterms:modified "2025-03-07T04:07:10.177Z"^^xsd:dateTime;
  skos:broader <http://example.com/WEFGST/b804fbe2-e09d-4fd1-9e03-9cb5758f8b43> .

<http://example.com/WEFGST/dfe2bfeb-97fe-43cb-b479-b60d1c8a79b1>
  a skos:Concept;
  dcterms:created "2025-03-06T02:34:21.984Z"^^xsd:dateTime;
  dcterms:source "https://www1.reskillingrevolution2030.org/skills-taxonomy"^^xsd:anyURI ;
  skos:definition "Capacity to identify and shape effective value propositions for products and services, as well as to sell products on that basis."@en;
  skos:inScheme <http://example.com/WEFGST> ;
  skos:prefLabel "Sales, communication and marketing of products and services"@en;
  dcterms:modified "2025-03-07T04:07:11.683Z"^^xsd:dateTime;
  skos:broader <http://example.com/WEFGST/7f60d3b5-07d7-4bca-9ca0-78eed9298d44> .

<http://example.com/WEFGST/085e1895-ca1c-4ee3-a84a-abdd947623fd>
  a skos:Concept;
  dcterms:created "2025-03-06T02:34:22.005Z"^^xsd:dateTime;
  dcterms:source "https://www1.reskillingrevolution2030.org/skills-taxonomy"^^xsd:anyURI ;
  skos:definition "Using the internet, mobile devices, social media, search engines and other online channels to reach consumers."@en;
  skos:inScheme <http://example.com/WEFGST> ;
  skos:prefLabel "Digital marketing"@en;
  dcterms:modified "2025-03-07T04:07:11.725Z"^^xsd:dateTime;
  skos:broader <http://example.com/WEFGST/7f60d3b5-07d7-4bca-9ca0-78eed9298d44> .

<http://example.com/WEFGST/89234341-1235-476f-a6c8-3cb662bfa53f>
  a skos:Concept;
  dcterms:created "2025-03-06T02:34:22.026Z"^^xsd:dateTime;
  dcterms:source "https://www1.reskillingrevolution2030.org/skills-taxonomy"^^xsd:anyURI ;
  skos:inScheme <http://example.com/WEFGST> ;
  skos:prefLabel "Customer experience"@en;
  skos:narrower <http://example.com/WEFGST/56e6080a-bd82-44de-ac34-38f5edc397ed>,
    <http://example.com/WEFGST/7359d07f-9dae-487e-be45-b9c62ac8c5a9>;
  dcterms:modified "2025-03-07T04:07:10.217Z"^^xsd:dateTime;
  skos:broader <http://example.com/WEFGST/b804fbe2-e09d-4fd1-9e03-9cb5758f8b43> .

<http://example.com/WEFGST/56e6080a-bd82-44de-ac34-38f5edc397ed>
  a skos:Concept;
  dcterms:created "2025-03-06T02:34:22.048Z"^^xsd:dateTime;
  dcterms:source "https://www1.reskillingrevolution2030.org/skills-taxonomy"^^xsd:anyURI ;
  skos:definition "Responding to customer enquiries in a manner that balances speed and quality, and represents brand values."@en;
  skos:inScheme <http://example.com/WEFGST> ;
  skos:prefLabel "Customer service"@en;
  dcterms:modified "2025-03-07T04:07:11.768Z"^^xsd:dateTime;
  skos:broader <http://example.com/WEFGST/89234341-1235-476f-a6c8-3cb662bfa53f> .

<http://example.com/WEFGST/7359d07f-9dae-487e-be45-b9c62ac8c5a9>
  a skos:Concept;
  dcterms:created "2025-03-06T02:34:22.070Z"^^xsd:dateTime;
  dcterms:source "https://www1.reskillingrevolution2030.org/skills-taxonomy"^^xsd:anyURI ;
  skos:definition "Managing and developing a portfolio of client relationships over extended periods to accomplish an operational strategy."@en;
  skos:inScheme <http://example.com/WEFGST> ;
  skos:prefLabel "Customer relationship management"@en;
  dcterms:modified "2025-03-07T04:07:11.808Z"^^xsd:dateTime;
  skos:broader <http://example.com/WEFGST/89234341-1235-476f-a6c8-3cb662bfa53f> .

<http://example.com/WEFGST/e634918b-4f3e-467b-ab1c-66aecad6fc8d>
  a skos:Concept;
  dcterms:created "2025-03-06T02:34:21.645Z"^^xsd:dateTime;
  dcterms:source "https://www1.reskillingrevolution2030.org/skills-taxonomy"^^xsd:anyURI ;
  skos:inScheme <http://example.com/WEFGST> ;
  skos:prefLabel "Management skills"@en;
  skos:narrower <http://example.com/WEFGST/ccf12791-3881-4f93-a8a7-de5e3b27837d>,
    <http://example.com/WEFGST/545565f7-2069-436e-8243-efe39197353b>,
    <http://example.com/WEFGST/7c2d58fd-fed0-40e0-8a90-0c9b81764805>,
    <http://example.com/WEFGST/b69be616-3e77-4a9f-bf49-96af4a792bf6>;
  dcterms:modified "2025-03-07T04:07:09.709Z"^^xsd:dateTime;
  skos:broader <http://example.com/WEFGST/0a9ac146-77e9-4ad3-94d5-ab9f62c8cd02> .

<http://example.com/WEFGST/7c2d58fd-fed0-40e0-8a90-0c9b81764805>
  a skos:Concept;
  dcterms:created "2025-03-06T02:34:21.810Z"^^xsd:dateTime;
  dcterms:source "https://www1.reskillingrevolution2030.org/skills-taxonomy"^^xsd:anyURI ;
  skos:inScheme <http://example.com/WEFGST> ;
  skos:prefLabel "Financial management"@en;
  skos:narrower <http://example.com/WEFGST/6fffa062-7536-451b-b3f9-1e95eb6f2720>,
    <http://example.com/WEFGST/67991569-80d2-4fbd-84ff-01293124c747>;
  dcterms:modified "2025-03-07T04:07:10.097Z"^^xsd:dateTime;
  skos:broader <http://example.com/WEFGST/e634918b-4f3e-467b-ab1c-66aecad6fc8d> .

<http://example.com/WEFGST/6fffa062-7536-451b-b3f9-1e95eb6f2720>
  a skos:Concept;
  dcterms:created "2025-03-06T02:34:21.828Z"^^xsd:dateTime;
  dcterms:source "https://www1.reskillingrevolution2030.org/skills-taxonomy"^^xsd:anyURI ;
  skos:definition "Tracking the flow of money that has been spent."@en;
  skos:inScheme <http://example.com/WEFGST> ;
  skos:prefLabel "Accounting"@en;
  dcterms:modified "2025-03-07T04:07:11.467Z"^^xsd:dateTime;
  skos:broader <http://example.com/WEFGST/7c2d58fd-fed0-40e0-8a90-0c9b81764805> .

<http://example.com/WEFGST/67991569-80d2-4fbd-84ff-01293124c747>
  a skos:Concept;
  dcterms:created "2025-03-06T02:34:21.846Z"^^xsd:dateTime;
  dcterms:source "https://www1.reskillingrevolution2030.org/skills-taxonomy"^^xsd:anyURI ;
  skos:definition "Budgeting money that will be spent, managing financial portfolios, and tracking economic trends which affect business performance."@en;
  skos:inScheme <http://example.com/WEFGST> ;
  skos:prefLabel "Finance"@en;
  dcterms:modified "2025-03-07T04:07:11.510Z"^^xsd:dateTime;
  skos:broader <http://example.com/WEFGST/7c2d58fd-fed0-40e0-8a90-0c9b81764805> .

<http://example.com/WEFGST/545565f7-2069-436e-8243-efe39197353b>
  a skos:Concept;
  dcterms:created "2025-03-06T02:34:21.727Z"^^xsd:dateTime;
  dcterms:source "https://www1.reskillingrevolution2030.org/skills-taxonomy"^^xsd:anyURI ;
  skos:inScheme <http://example.com/WEFGST> ;
  skos:prefLabel "Operations and logistics"@en;
  skos:narrower <http://example.com/WEFGST/b19f0e4d-51c1-4648-a8a2-680aa7ba6b52>,
    <http://example.com/WEFGST/734b9f53-d194-4df5-8db9-469ebabb338d>,
    <http://example.com/WEFGST/bcfc8caf-06ea-475b-9b2c-0c6b6833eda6>;
  dcterms:modified "2025-03-07T04:07:10.059Z"^^xsd:dateTime;
  skos:broader <http://example.com/WEFGST/e634918b-4f3e-467b-ab1c-66aecad6fc8d> .

<http://example.com/WEFGST/b19f0e4d-51c1-4648-a8a2-680aa7ba6b52>
  a skos:Concept;
  dcterms:created "2025-03-06T02:34:21.748Z"^^xsd:dateTime;
  dcterms:source "https://www1.reskillingrevolution2030.org/skills-taxonomy"^^xsd:anyURI ;
  skos:definition "Capacity to coordinate time-sensitive schedules in cooperation with others."@en;
  skos:inScheme <http://example.com/WEFGST> ;
  skos:prefLabel "Coordination and time management"@en;
  dcterms:modified "2025-03-07T04:07:11.350Z"^^xsd:dateTime;
  skos:broader <http://example.com/WEFGST/545565f7-2069-436e-8243-efe39197353b> .

<http://example.com/WEFGST/bcfc8caf-06ea-475b-9b2c-0c6b6833eda6>
  a skos:Concept;
  dcterms:created "2025-03-06T02:34:21.790Z"^^xsd:dateTime;
  dcterms:source "https://www1.reskillingrevolution2030.org/skills-taxonomy"^^xsd:anyURI ;
  skos:definition "Optimising the flow of the goods and services which are required to realise a product or goal."@en;
  skos:inScheme <http://example.com/WEFGST> ;
  skos:prefLabel "Supply-chain management"@en;
  dcterms:modified "2025-03-07T04:07:11.427Z"^^xsd:dateTime;
  skos:broader <http://example.com/WEFGST/545565f7-2069-436e-8243-efe39197353b> .

<http://example.com/WEFGST/734b9f53-d194-4df5-8db9-469ebabb338d>
  a skos:Concept;
  dcterms:created "2025-03-06T02:34:21.769Z"^^xsd:dateTime;
  dcterms:source "https://www1.reskillingrevolution2030.org/skills-taxonomy"^^xsd:anyURI ;
  skos:definition "Capacity to lead the work of a team to identify, select and implement the appropriate changes, tools, and improvements to achieve and deliver a defined goal."@en;
  skos:inScheme <http://example.com/WEFGST> ;
  skos:prefLabel "Project management"@en;
  dcterms:modified "2025-03-07T04:07:11.389Z"^^xsd:dateTime;
  skos:broader <http://example.com/WEFGST/545565f7-2069-436e-8243-efe39197353b> .

<http://example.com/WEFGST/ccf12791-3881-4f93-a8a7-de5e3b27837d>
  a skos:Concept;
  dcterms:created "2025-03-06T02:34:21.665Z"^^xsd:dateTime;
  dcterms:source "https://www1.reskillingrevolution2030.org/skills-taxonomy"^^xsd:anyURI ;
  skos:inScheme <http://example.com/WEFGST> ;
  skos:prefLabel "Talent management"@en;
  skos:narrower <http://example.com/WEFGST/074133e1-31eb-4a10-baa5-6fb773457d6f>,
    <http://example.com/WEFGST/a6930331-6da9-435c-a729-042179879b65>;
  dcterms:modified "2025-03-07T04:07:10.019Z"^^xsd:dateTime;
  skos:broader <http://example.com/WEFGST/e634918b-4f3e-467b-ab1c-66aecad6fc8d> .

<http://example.com/WEFGST/074133e1-31eb-4a10-baa5-6fb773457d6f>
  a skos:Concept;
  dcterms:created "2025-03-06T02:34:21.686Z"^^xsd:dateTime;
  dcterms:source "https://www1.reskillingrevolution2030.org/skills-taxonomy"^^xsd:anyURI ;
  skos:definition "Accurately evaluating a candidate or colleague’s proficiencies and characteristics over their full profile of skills, knowledge, abilities and attitudes."@en;
  skos:inScheme <http://example.com/WEFGST> ;
  skos:prefLabel "Skill evaluation"@en;
  dcterms:modified "2025-03-07T04:07:11.273Z"^^xsd:dateTime;
  skos:broader <http://example.com/WEFGST/ccf12791-3881-4f93-a8a7-de5e3b27837d> .

<http://example.com/WEFGST/a6930331-6da9-435c-a729-042179879b65>
  a skos:Concept;
  dcterms:created "2025-03-06T02:34:21.707Z"^^xsd:dateTime;
  dcterms:source "https://www1.reskillingrevolution2030.org/skills-taxonomy"^^xsd:anyURI ;
  skos:definition "Identifying developmental or hiring solutions to bridge a team’s skills gaps and ensuring knowledge transfer when team members transition to new roles."@en;
  skos:inScheme <http://example.com/WEFGST> ;
  skos:prefLabel "Talent planning and development"@en;
  dcterms:modified "2025-03-07T04:07:11.311Z"^^xsd:dateTime;
  skos:broader <http://example.com/WEFGST/ccf12791-3881-4f93-a8a7-de5e3b27837d> .

<http://example.com/WEFGST/b69be616-3e77-4a9f-bf49-96af4a792bf6>
  a skos:Concept;
  dcterms:created "2025-03-06T02:34:21.865Z"^^xsd:dateTime;
  dcterms:source "https://www1.reskillingrevolution2030.org/skills-taxonomy"^^xsd:anyURI ;
  skos:inScheme <http://example.com/WEFGST> ;
  skos:prefLabel "Quality management"@en;
  skos:narrower <http://example.com/WEFGST/bedf28b5-96ff-4a8e-8771-4d518e0877dc>,
    <http://example.com/WEFGST/f5145733-89b7-40f8-8794-0e23efe91ada>,
    <http://example.com/WEFGST/659da579-61cf-427a-889d-8be1c8ba6172>;
  dcterms:modified "2025-03-07T04:07:10.134Z"^^xsd:dateTime;
  skos:broader <http://example.com/WEFGST/e634918b-4f3e-467b-ab1c-66aecad6fc8d> .

<http://example.com/WEFGST/659da579-61cf-427a-889d-8be1c8ba6172>
  a skos:Concept;
  dcterms:created "2025-03-06T02:34:21.924Z"^^xsd:dateTime;
  dcterms:source "https://www1.reskillingrevolution2030.org/skills-taxonomy"^^xsd:anyURI ;
  skos:definition "Assessing, prioritising and mitigating the effect of uncertainty on objectives, to enhance institutional resilience."@en;
  skos:inScheme <http://example.com/WEFGST> ;
  skos:prefLabel "Risk management"@en;
  dcterms:modified "2025-03-07T04:07:11.641Z"^^xsd:dateTime;
  skos:broader <http://example.com/WEFGST/b69be616-3e77-4a9f-bf49-96af4a792bf6> .

<http://example.com/WEFGST/f5145733-89b7-40f8-8794-0e23efe91ada>
  a skos:Concept;
  dcterms:created "2025-03-06T02:34:21.905Z"^^xsd:dateTime;
  dcterms:source "https://www1.reskillingrevolution2030.org/skills-taxonomy"^^xsd:anyURI ;
  skos:definition "Inspecting products to ensure they fulfil quality requirements."@en;
  skos:inScheme <http://example.com/WEFGST> ;
  skos:prefLabel "Quality control"@en;
  dcterms:modified "2025-03-07T04:07:11.596Z"^^xsd:dateTime;
  skos:broader <http://example.com/WEFGST/b69be616-3e77-4a9f-bf49-96af4a792bf6> .

<http://example.com/WEFGST/bedf28b5-96ff-4a8e-8771-4d518e0877dc>
  a skos:Concept;
  dcterms:created "2025-03-06T02:34:21.885Z"^^xsd:dateTime;
  dcterms:source "https://www1.reskillingrevolution2030.org/skills-taxonomy"^^xsd:anyURI ;
  skos:definition "Setting quality objectives, specifying operational processes to achieve them, providing confidence they will be effective, and improving them based on experience."@en;
  skos:inScheme <http://example.com/WEFGST> ;
  skos:prefLabel "Quality assurance"@en;
  dcterms:modified "2025-03-07T04:07:11.552Z"^^xsd:dateTime;
  skos:broader <http://example.com/WEFGST/b69be616-3e77-4a9f-bf49-96af4a792bf6> .

<http://example.com/WEFGST/e8cdd6ea-4ef1-426b-9f24-e37b563559d5>
  a skos:Concept;
  dcterms:created "2025-03-06T02:34:22.093Z"^^xsd:dateTime;
  dcterms:source "https://www1.reskillingrevolution2030.org/skills-taxonomy"^^xsd:anyURI ;
  skos:inScheme <http://example.com/WEFGST> ;
  skos:prefLabel "Technology skills"@en;
  skos:narrower <http://example.com/WEFGST/a82a2b20-328b-4f55-bc4f-2557918b2446>,
    <http://example.com/WEFGST/db95361d-6956-42ed-b0dc-f810359234bb>,
    <http://example.com/WEFGST/b30fc93c-99c3-4005-b4c8-33442f7a76e2>,
    <http://example.com/WEFGST/a2336259-d93d-4d3e-bf98-0bbdf1b1cf5e>,
    <http://example.com/WEFGST/c1e1b25e-619e-4e1a-a92b-739f242ce82a>;
  dcterms:modified "2025-03-07T04:07:09.785Z"^^xsd:dateTime;
  skos:broader <http://example.com/WEFGST/0a9ac146-77e9-4ad3-94d5-ab9f62c8cd02> .

<http://example.com/WEFGST/a82a2b20-328b-4f55-bc4f-2557918b2446>
  a skos:Concept;
  dcterms:created "2025-03-06T02:34:22.114Z"^^xsd:dateTime;
  dcterms:source "https://www1.reskillingrevolution2030.org/skills-taxonomy"^^xsd:anyURI ;
  skos:inScheme <http://example.com/WEFGST> ;
  skos:prefLabel "Technology literacy"@en;
  skos:narrower <http://example.com/WEFGST/69c24bb3-08d0-425d-923c-b50e5045a020>,
    <http://example.com/WEFGST/4fda7259-b144-495e-965b-a31f207a1eaf>,
    <http://example.com/WEFGST/bebc1c85-9544-4779-a73f-43e420b28906>;
  dcterms:modified "2025-03-07T04:07:10.270Z"^^xsd:dateTime;
  skos:broader <http://example.com/WEFGST/e8cdd6ea-4ef1-426b-9f24-e37b563559d5> .

<http://example.com/WEFGST/69c24bb3-08d0-425d-923c-b50e5045a020>
  a skos:Concept;
  dcterms:created "2025-03-06T02:34:22.135Z"^^xsd:dateTime;
  dcterms:source "https://www1.reskillingrevolution2030.org/skills-taxonomy"^^xsd:anyURI ;
  skos:definition "Using software designed to help get work done faster and more efficiently."@en;
  skos:inScheme <http://example.com/WEFGST> ;
  skos:prefLabel "Collaboration and productivity software"@en;
  dcterms:modified "2025-03-07T04:07:11.854Z"^^xsd:dateTime;
  skos:broader <http://example.com/WEFGST/a82a2b20-328b-4f55-bc4f-2557918b2446> .

<http://example.com/WEFGST/4fda7259-b144-495e-965b-a31f207a1eaf>
  a skos:Concept;
  dcterms:created "2025-03-06T02:34:22.156Z"^^xsd:dateTime;
  dcterms:source "https://www1.reskillingrevolution2030.org/skills-taxonomy"^^xsd:anyURI ;
  skos:definition "Using technologies that assist in industrial production and manufacturing processes."@en;
  skos:inScheme <http://example.com/WEFGST> ;
  skos:prefLabel "Manufacturing technologies"@en;
  dcterms:modified "2025-03-07T04:07:11.898Z"^^xsd:dateTime;
  skos:broader <http://example.com/WEFGST/a82a2b20-328b-4f55-bc4f-2557918b2446> .

<http://example.com/WEFGST/bebc1c85-9544-4779-a73f-43e420b28906>
  a skos:Concept;
  dcterms:created "2025-03-06T02:34:22.177Z"^^xsd:dateTime;
  dcterms:source "https://www1.reskillingrevolution2030.org/skills-taxonomy"^^xsd:anyURI ;
  skos:definition "Installing equipment, machines, wiring or programs to meet specifications."@en;
  skos:inScheme <http://example.com/WEFGST> ;
  skos:prefLabel "Installation"@en;
  dcterms:modified "2025-03-07T04:07:11.940Z"^^xsd:dateTime;
  skos:broader <http://example.com/WEFGST/a82a2b20-328b-4f55-bc4f-2557918b2446> .

<http://example.com/WEFGST/a2336259-d93d-4d3e-bf98-0bbdf1b1cf5e>
  a skos:Concept;
  dcterms:created "2025-03-06T02:34:22.379Z"^^xsd:dateTime;
  dcterms:source "https://www1.reskillingrevolution2030.org/skills-taxonomy"^^xsd:anyURI ;
  skos:inScheme <http://example.com/WEFGST> ;
  skos:prefLabel "Networks and cybersecurity"@en;
  skos:narrower <http://example.com/WEFGST/6028a6d1-298e-476b-892d-fa63c13f55b1>,
    <http://example.com/WEFGST/3658a3d6-886f-4255-a31f-979b0b0b4397>,
    <http://example.com/WEFGST/60574e00-f499-47fc-983c-4dfa3cbc7b49>;
  dcterms:modified "2025-03-07T04:07:10.409Z"^^xsd:dateTime;
  skos:broader <http://example.com/WEFGST/e8cdd6ea-4ef1-426b-9f24-e37b563559d5> .

<http://example.com/WEFGST/6028a6d1-298e-476b-892d-fa63c13f55b1>
  a skos:Concept;
  dcterms:created "2025-03-06T02:34:22.405Z"^^xsd:dateTime;
  dcterms:source "https://www1.reskillingrevolution2030.org/skills-taxonomy"^^xsd:anyURI ;
  skos:definition "Setting up a connected network of computing devices, such as laptops, desktops, servers, smartphones, tablets and internet-of-things devices that communicate with one another."@en;
  skos:inScheme <http://example.com/WEFGST> ;
  skos:prefLabel "Computer hardware and networking"@en;
  dcterms:modified "2025-03-07T04:07:12.282Z"^^xsd:dateTime;
  skos:broader <http://example.com/WEFGST/a2336259-d93d-4d3e-bf98-0bbdf1b1cf5e> .

<http://example.com/WEFGST/60574e00-f499-47fc-983c-4dfa3cbc7b49>
  a skos:Concept;
  dcterms:created "2025-03-06T02:34:22.451Z"^^xsd:dateTime;
  dcterms:source "https://www1.reskillingrevolution2030.org/skills-taxonomy"^^xsd:anyURI ;
  skos:definition "Delivering computing services over the internet."@en;
  skos:inScheme <http://example.com/WEFGST> ;
  skos:prefLabel "Cloud computing"@en;
  dcterms:modified "2025-03-07T04:07:12.377Z"^^xsd:dateTime;
  skos:broader <http://example.com/WEFGST/a2336259-d93d-4d3e-bf98-0bbdf1b1cf5e> .

<http://example.com/WEFGST/3658a3d6-886f-4255-a31f-979b0b0b4397>
  a skos:Concept;
  dcterms:created "2025-03-06T02:34:22.430Z"^^xsd:dateTime;
  dcterms:source "https://www1.reskillingrevolution2030.org/skills-taxonomy"^^xsd:anyURI ;
  skos:definition "Using technologies, processes and practices to protect computers, networks, programs and data from unauthorised access or attacks that are aimed for exploitation."@en;
  skos:inScheme <http://example.com/WEFGST> ;
  skos:prefLabel "Cybersecurity and application security"@en;
  dcterms:modified "2025-03-07T04:07:12.329Z"^^xsd:dateTime;
  skos:broader <http://example.com/WEFGST/a2336259-d93d-4d3e-bf98-0bbdf1b1cf5e> .

<http://example.com/WEFGST/b30fc93c-99c3-4005-b4c8-33442f7a76e2>
  a skos:Concept;
  dcterms:created "2025-03-06T02:34:22.282Z"^^xsd:dateTime;
  dcterms:source "https://www1.reskillingrevolution2030.org/skills-taxonomy"^^xsd:anyURI ;
  skos:inScheme <http://example.com/WEFGST> ;
  skos:prefLabel "Design and user experience"@en;
  skos:narrower <http://example.com/WEFGST/6aba2110-d2c1-4ad0-9f52-b3699b87eb3e>,
    <http://example.com/WEFGST/67c59734-2e7a-4edb-a911-dcefc6af9e34>,
    <http://example.com/WEFGST/688f51b4-1e2b-4789-b12e-834043d9273f>;
  dcterms:modified "2025-03-07T04:07:10.366Z"^^xsd:dateTime;
  skos:broader <http://example.com/WEFGST/e8cdd6ea-4ef1-426b-9f24-e37b563559d5> .

<http://example.com/WEFGST/688f51b4-1e2b-4789-b12e-834043d9273f>
  a skos:Concept;
  dcterms:created "2025-03-06T02:34:22.355Z"^^xsd:dateTime;
  dcterms:source "https://www1.reskillingrevolution2030.org/skills-taxonomy"^^xsd:anyURI ;
  skos:definition "Building and maintaining websites."@en;
  skos:inScheme <http://example.com/WEFGST> ;
  skos:prefLabel "Web development"@en;
  dcterms:modified "2025-03-07T04:07:12.231Z"^^xsd:dateTime;
  skos:broader <http://example.com/WEFGST/b30fc93c-99c3-4005-b4c8-33442f7a76e2> .

<http://example.com/WEFGST/6aba2110-d2c1-4ad0-9f52-b3699b87eb3e>
  a skos:Concept;
  dcterms:created "2025-03-06T02:34:22.307Z"^^xsd:dateTime;
  dcterms:source "https://www1.reskillingrevolution2030.org/skills-taxonomy"^^xsd:anyURI ;
  skos:definition "Designing technology from a user's perspective by balancing considerations such as practical usability, ergonomics, perception, cognition, social psychology, consumer behaviour and environmental impact."@en;
  skos:inScheme <http://example.com/WEFGST> ;
  skos:prefLabel "Human-technology interaction"@en;
  dcterms:modified "2025-03-07T04:07:12.119Z"^^xsd:dateTime;
  skos:broader <http://example.com/WEFGST/b30fc93c-99c3-4005-b4c8-33442f7a76e2> .

<http://example.com/WEFGST/67c59734-2e7a-4edb-a911-dcefc6af9e34>
  a skos:Concept;
  dcterms:created "2025-03-06T02:34:22.333Z"^^xsd:dateTime;
  dcterms:source "https://www1.reskillingrevolution2030.org/skills-taxonomy"^^xsd:anyURI ;
  skos:definition "Developing applications for mobile devices."@en;
  skos:inScheme <http://example.com/WEFGST> ;
  skos:prefLabel "Mobile development"@en;
  dcterms:modified "2025-03-07T04:07:12.167Z"^^xsd:dateTime;
  skos:broader <http://example.com/WEFGST/b30fc93c-99c3-4005-b4c8-33442f7a76e2> .

<http://example.com/WEFGST/db95361d-6956-42ed-b0dc-f810359234bb>
  a skos:Concept;
  dcterms:created "2025-03-06T02:34:22.200Z"^^xsd:dateTime;
  dcterms:source "https://www1.reskillingrevolution2030.org/skills-taxonomy"^^xsd:anyURI ;
  skos:inScheme <http://example.com/WEFGST> ;
  skos:prefLabel "Programming"@en;
  skos:narrower <http://example.com/WEFGST/c1656813-25e4-4235-bb27-9b1e2c799937>,
    <http://example.com/WEFGST/5f469463-0d4b-4b36-9299-db64d200cd6a>,
    <http://example.com/WEFGST/6fa4d4fa-96f5-4fca-a56c-60c18fa57fd2>;
  dcterms:modified "2025-03-07T04:07:10.319Z"^^xsd:dateTime;
  skos:broader <http://example.com/WEFGST/e8cdd6ea-4ef1-426b-9f24-e37b563559d5> .

<http://example.com/WEFGST/c1656813-25e4-4235-bb27-9b1e2c799937>
  a skos:Concept;
  dcterms:created "2025-03-06T02:34:22.221Z"^^xsd:dateTime;
  dcterms:source "https://www1.reskillingrevolution2030.org/skills-taxonomy"^^xsd:anyURI ;
  skos:definition "Writing simple programs using calls to subroutines."@en;
  skos:inScheme <http://example.com/WEFGST> ;
  skos:prefLabel "Functional programming"@en;
  dcterms:modified "2025-03-07T04:07:11.983Z"^^xsd:dateTime;
  skos:broader <http://example.com/WEFGST/db95361d-6956-42ed-b0dc-f810359234bb> .

<http://example.com/WEFGST/5f469463-0d4b-4b36-9299-db64d200cd6a>
  a skos:Concept;
  dcterms:created "2025-03-06T02:34:22.241Z"^^xsd:dateTime;
  dcterms:source "https://www1.reskillingrevolution2030.org/skills-taxonomy"^^xsd:anyURI ;
  skos:definition "Using data encapsulation and inheritance to develop well designed programming projects, often as part of a team."@en;
  skos:inScheme <http://example.com/WEFGST> ;
  skos:prefLabel "Object-oriented programming"@en;
  dcterms:modified "2025-03-07T04:07:12.025Z"^^xsd:dateTime;
  skos:broader <http://example.com/WEFGST/db95361d-6956-42ed-b0dc-f810359234bb> .

<http://example.com/WEFGST/6fa4d4fa-96f5-4fca-a56c-60c18fa57fd2>
  a skos:Concept;
  dcterms:created "2025-03-06T02:34:22.261Z"^^xsd:dateTime;
  dcterms:source "https://www1.reskillingrevolution2030.org/skills-taxonomy"^^xsd:anyURI ;
  skos:definition "Looking at real-world scenarios and creating models that can be processed by a computer."@en;
  skos:inScheme <http://example.com/WEFGST> ;
  skos:prefLabel "Computational thinking"@en;
  dcterms:modified "2025-03-07T04:07:12.071Z"^^xsd:dateTime;
  skos:broader <http://example.com/WEFGST/db95361d-6956-42ed-b0dc-f810359234bb> .

<http://example.com/WEFGST/c1e1b25e-619e-4e1a-a92b-739f242ce82a>
  a skos:Concept;
  dcterms:created "2025-03-06T02:34:22.472Z"^^xsd:dateTime;
  dcterms:source "https://www1.reskillingrevolution2030.org/skills-taxonomy"^^xsd:anyURI ;
  skos:inScheme <http://example.com/WEFGST> ;
  skos:prefLabel "Artificial intelligence and big data"@en;
  skos:narrower <http://example.com/WEFGST/1469466d-bcb6-43ab-bda0-65da29dbda81>,
    <http://example.com/WEFGST/b0f98594-dbf5-488b-aef4-2a09ab4e182e>,
    <http://example.com/WEFGST/d61cec92-04fb-4515-accf-021c11e5888e>;
  dcterms:modified "2025-03-07T04:07:10.448Z"^^xsd:dateTime;
  skos:broader <http://example.com/WEFGST/e8cdd6ea-4ef1-426b-9f24-e37b563559d5> .

<http://example.com/WEFGST/b0f98594-dbf5-488b-aef4-2a09ab4e182e>
  a skos:Concept;
  dcterms:created "2025-03-06T02:34:22.511Z"^^xsd:dateTime;
  dcterms:source "https://www1.reskillingrevolution2030.org/skills-taxonomy"^^xsd:anyURI ;
  skos:definition "Designing neural networks which can be trained to reliably make decisions based on example data."@en;
  skos:inScheme <http://example.com/WEFGST> ;
  skos:prefLabel "Supervised learning"@en;
  dcterms:modified "2025-03-07T04:07:12.470Z"^^xsd:dateTime;
  skos:broader <http://example.com/WEFGST/c1e1b25e-619e-4e1a-a92b-739f242ce82a> .

<http://example.com/WEFGST/d61cec92-04fb-4515-accf-021c11e5888e>
  a skos:Concept;
  dcterms:created "2025-03-06T02:34:22.530Z"^^xsd:dateTime;
  dcterms:source "https://www1.reskillingrevolution2030.org/skills-taxonomy"^^xsd:anyURI ;
  skos:definition "Designing neural networks which can detect clusters and patterns in large and complex data sets without human guidance."@en;
  skos:inScheme <http://example.com/WEFGST> ;
  skos:prefLabel "Unsupervised learning"@en;
  dcterms:modified "2025-03-07T04:07:12.514Z"^^xsd:dateTime;
  skos:broader <http://example.com/WEFGST/c1e1b25e-619e-4e1a-a92b-739f242ce82a> .

<http://example.com/WEFGST/1469466d-bcb6-43ab-bda0-65da29dbda81>
  a skos:Concept;
  dcterms:created "2025-03-06T02:34:22.491Z"^^xsd:dateTime;
  dcterms:source "https://www1.reskillingrevolution2030.org/skills-taxonomy"^^xsd:anyURI ;
  skos:definition "Accessing, cleaning and sorting large data sets, and using software tools to visualise the results."@en;
  skos:inScheme <http://example.com/WEFGST> ;
  skos:prefLabel "Data mining"@en;
  dcterms:modified "2025-03-07T04:07:12.425Z"^^xsd:dateTime;
  skos:broader <http://example.com/WEFGST/c1e1b25e-619e-4e1a-a92b-739f242ce82a> .
