PREFIX skillcat:    <https://data.jobsandskills.gov.au/def/skillcat/>
PREFIX skillcatcs:  <https://data.jobsandskills.gov.au/def/skillcat>
PREFIX dcterms:     <http://purl.org/dc/terms/>
PREFIX dewr:        <https://linked.data.gov.au/org/dewr>
PREFIX jsa:         <https://linked.data.gov.au/org/jsa>
PREFIX nst:         <https://test.linked.data.gov.au/def/nst/>
PREFIX owl:         <http://www.w3.org/2002/07/owl#>
PREFIX rdfs:        <http://www.w3.org/2000/01/rdf-schema#>
PREFIX ror:         <https://ror.org/>
PREFIX schema:      <https://schema.org/>
PREFIX skos:        <http://www.w3.org/2004/02/skos/core#>
PREFIX xsd:         <http://www.w3.org/2001/XMLSchema#>

dewr:
a schema:Organization ;
schema:name "Jobs and Skills Australia"@en ;
schema:alternateName "JSA"@en ;
schema:url "https://www.jobsandskills.gov.au"^^xsd:anyURI
.

jsa:
a schema:Organization ;
schema:name "Jobs and Skills Australia"@en ;
schema:alternateName "JSA"@en ;
schema:url "https://www.jobsandskills.gov.au"^^xsd:anyURI
.

skillcatcs: a skos:ConceptScheme ;
dcterms:creator jsa: ;
dcterms:publisher dewr: ;
skos:prefLabel "Skill categroy"@en ;
skos:definition "Indicates the Skill category: Cognitive; Domain knowledge; Interpersonal; Technical"@en ;
skos:hasTopConcept skillcat:cognitive , skillcat:domainKnowledge , skillcat:interpersonal , skillcat:technical
.

skillcat:cognitive a skos:Concept ;
skos:prefLabel "Cognitive"@en ;
skos:altLabel "Thinking skills"@en , "Analysis skills"@en ;
skos:definition: "Skills focused on mental processes, analysis, problem-solving, and decision-making"@en ;
skos:inScheme skillcatcs: ;
skos:topConceptOf skillcatcs: 
.

skillcat:domainKnowledge a skos:Concept ; 
skos:prefLabel "Domain knowledge"@en ;
skos:altLabel "Subject matter expertise"@en ;
skos:definition: "Core knowledge, principles, regulations, and theoretical understanding specific to a field"@en ;
skos:inScheme skillcatcs: ;
skos:topConceptOf skillcatcs: 
.

skillcat:interpersonal a skos:Concept; 
skos:prefLabel "Interpersonal"@en ;
skos:altLabel "Communication skills"@en , "Relationship skills"@en ;
skos:definition "Skills related to communication, collaboration, leadership, and working with others"@en ;
skos:inScheme skillcatcs: ;
skos:topConceptOf skillcatcs: 
.

skillcat:technical  a skos:Concept; 
skos:prefLabel "Technical"@en ;
skos:altLabel
   "Tool skills"@en , "Technology skills"@en , "System skills"@en ;
skos:definition "Skills requiring specific technical tools, programming, systems, or hands-on implementation"@en ;
skos:inScheme skillcatcs: ;
skos:topConceptOf skillcatcs: 
.