PREFIX aqflvl:     <https://training.gov.au/aqfLevel/>
PREFIX aqflvlcs:   <https://training.gov.au/aqfLevel>
PREFIX aqftype:    <https://training.gov.au/aqfType/>
PREFIX aqftypecs:  <https://training.gov.au/aqfType>
PREFIX asn:        <http://purl.org/ASN/schema/core/>
PREFIX attributes: <https://rdf.sfia-online.org/9/attributes/>
PREFIX dcterms:    <http://purl.org/dc/terms/>
PREFIX jsa:        <https://linked.data.gov.au/org/jsa>
PREFIX ror:        <https://ror.org/>
PREFIX rdf:        <http://www.w3.org/1999/02/22-rdf-syntax-ns#>
PREFIX schema:     <https://schema.org/>
PREFIX sfia:       <https://rdf.sfia-online.org/9/ontology/>
PREFIX skos:       <http://www.w3.org/2004/02/skos/core#>
PREFIX xsd:        <http://www.w3.org/2001/XMLSchema#>

ror:03z942k20
a schema:Orgainzation ;
schema:name "Department of Education" ;
schema:url "https://www.education.gov.au"^^xsd:anyURI
.

jsa:
a schema:Organization ;
schema:name "Jobs and Skills Australia"@en ;
schema:alternateName "JSA"@en ;
schema:url "https://www.jobsandskills.gov.au"^^xsd:anyURI
.

    aqftypecs: a skos:ConceptScheme;
    dcterms:creator     ror:03z942k20 ;
    dcterms:publisher   jsa: ;
    dcterms:modified    "2025-08-01T00:03:52.116Z"^^xsd:dateTime;
    dcterms:title       "AQF Qualification Types"@en;
    skos:prefLabel      "AQF Qualification Types"@en;
    skos:definition     "Qualification type refers to the broad discipline-free nomenclature used in the AQF to describe each category of AQF qualification, for example, Senior Secondary Certificate of Education, Certificate III, Bachelor Degree."@en ;
    schema:citation     "https://www.aqf.edu.au/framework/aqf-qualifications"^^xsd:anyURI ;
    skos:hasTopConcept  aqftype:524 , aqftype:521 , aqftype:514 , aqftype:511 , aqftype:421 , aqftype:411 , aqftype:211 , aqftype:221 , aqftype:UC , aqftype:BHD , aqftype:MD , aqftype:DD
	. 

    aqftype:524 a skos:Concept ;
    skos:prefLabel "Certificate I"@en ;
    skos:definition "The purpose of the Certificate I qualification type is to qualify individuals with basic functional knowledge and skills to undertake work, further learning and community involvement. Certificate I qualifications are located at level 1 of the Australian Qualifications Framework. Certificate I qualifications must be designed and accredited to enable graduates to demonstrate the learning outcomes expressed as knowledge, skills and the application of knowledge and skills specified in the level 1 criteria and the Certificate I descriptor."@en ;
    skos:notation "1" ;
    sfia:level aqflvl:1 ;
    skos:inScheme aqftypecs: ;
    skos:topConceptOf aqftypecs:
    .

    aqftype:521 a skos:Concept ;
    skos:prefLabel "Certificate II"@en ;
    skos:definition "The purpose of the Certificate II qualification type is to qualify individuals to undertake mainly routine work and as a pathway to further learning. Certificate II qualifications are located at level 2 of the Australian Qualifications Framework. Certificate II qualifications must be designed and accredited to enable graduates to demonstrate the learning outcomes expressed as knowledge, skills and the application of knowledge and skills Specified in the level 2 criteria and the Certificate II descriptor."@en ;
    skos:notation "2" ;
    sfia:level aqflvl:2 ;
    skos:inScheme aqftypecs: ;
    skos:topConceptOf aqftypecs:
    .

    aqftype:514 a skos:Concept ;
    skos:prefLabel "Certificate III"@en ;
    skos:definition "The purpose of the Certificate III qualification type is to qualify individuals who apply a broad range of knowledge and skills in varied contexts to undertake skilled work and as a pathway for further learning. Certificate III qualifications are located at level 3 of the Australian Qualifications Framework. Certificate III qualifications must be designed and accredited to enable graduates to demonstrate the learning outcomes expressed as knowledge, skills and the application of knowledge and skills specified in the level 3 criteria and the Certificate III descriptor."@en ;
    skos:notation "3" ;
    sfia:level aqflvl:3 ;
    skos:inScheme aqftypecs: ;
    skos:topConceptOf aqftypecs:
    .

    aqftype:511 a skos:Concept ;
    skos:prefLabel "Certificate IV"@en;
    skos:definition "The purpose of the Certificate IV qualification type is to qualify individuals who apply a broad range of specialised knowledge and skills in varied contexts to undertake skilled work and as a pathway for further learning. Certificate IV qualifications are located at level 4 of the Australian Qualifications Framework. Certificate IV qualifications must be designed and accredited to enable graduates to demonstrate the learning outcomes expressed as knowledge, skills and the application of knowledge and skills specified in the level 4 criteria and the Certificate IV descriptor."@en ;
    skos:notation "4" ;
    sfia:level aqflvl:4 ;
    skos:inScheme aqftypecs: ;
    skos:topConceptOf aqftypecs:
    .

    aqftype:421 a skos:Concept ;
    skos:prefLabel "Diploma"@en ;
    skos:definition "The purpose of the Diploma qualification type is to qualify individuals who apply integrated technical and theoretical concepts in a broad range of contexts to undertake advanced skilled or paraprofessional work and as a pathway for further learning. Diploma qualifications are located at level 5 of the Australian Qualifications Framework. Diploma qualifications must be designed and accredited to enable graduates to demonstrate the learning outcomes expressed as knowledge, skills and the application of knowledge and skills specified in the level 5 criteria and the Diploma descriptor. Diploma qualifications are available for accreditation and issuance in both higher education and vocational education and training."@en ;
    skos:notation "5" ;
    sfia:level aqflvl:5 ;
    skos:inScheme aqftypecs: ;
    skos:topConceptOf aqftypecs:
    .

    aqftype:411 a skos:Concept ;
    skos:prefLabel "Advanced Diploma"@en ;
    skos:definition "AQF Level 6 criteria for the Advanced Diploma: The purpose of the Advanced Diploma qualification type is to qualify individuals who apply specialised knowledge in a range of contexts to undertake advanced skilled or paraprofessional work and as a pathway for further learning. Advanced Diploma qualifications are located at level 6 of the Australian Qualifications Framework. Advanced Diploma qualifications must be designed and accredited to enable graduates to demonstrate the learning outcomes expressed as knowledge, skills and the application of knowledge and skills specified in the level 6 criteria and the Advanced Diploma descriptor. Advanced Diploma qualifications are available for accreditation and issuance in both higher education and vocational education and training. Full qualification type specification."@en ;
    skos:notation "6" ;
    sfia:level aqflvl:6 ;
    skos:inScheme aqftypecs: ;
    skos:topConceptOf aqftypecs:
    .

    aqftype:221 a skos:Concept ;
    skos:prefLabel "Graduate Certificate"@en ;
    skos:definition "The purpose of the Graduate Certificate qualification type is to qualify individuals who apply a body of knowledge in a range of contexts to undertake professional or highly skilled work and as a pathway for further learning. Graduate Certificate qualifications are located at level 8 of the Australian Qualifications Framework. Graduate Certificate qualifications must be designed and accredited to enable graduates to demonstrate the learning outcomes expressed as knowledge, skills and the application of knowledge and skills specified in the level 8 criteria and the Graduate Certificate descriptor. Graduate Certificate qualifications are available for accreditation and issuance in both higher education and vocational education and training. Full qualification type specification."@en ;
    skos:notation "8" ;
    sfia:level aqflvl:8 ;
    skos:inScheme aqftypecs: ;
    skos:topConceptOf aqftypecs:
    .

    aqftype:211 a skos:Concept ;
    skos:prefLabel "Graduate Diploma"@en ;
    skos:definition "The purpose of the Graduate Diploma qualification type is to qualify individuals who apply a body of knowledge in a range of contexts to undertake professional or highly skilled work and as a pathway for further learning. Graduate Diploma qualifications are located at level 8 of the Australian Qualifications Framework. Graduate Diploma qualifications must be designed and accredited to enable graduates to demonstrate the learning outcomes expressed as knowledge, skills and the application of knowledge and skills specified in the level 8 criteria and the Graduate Diploma descriptor. Graduate Diploma qualifications are available for accreditation and issuance in both higher education and vocational education and training."@en ;
    skos:notation "8" ;
    sfia:level aqflvl:8 ;
    skos:inScheme aqftypecs: ;
    skos:topConceptOf aqftypecs:
    .

    aqftype:UC a skos:Concept ;
	skos:prefLabel "Undergraduate Certificate"@en ;
    skos:definition "The Undergraduate Certificate has been developed in response to community and industry need based on the AQF review and as a result of the COVID-19 crisis. The Undergraduate Certificate is a higher education qualification of six months duration that may be used to articulate into an existing qualification at AQF levels 5, 6, or 7. It qualifies individuals with knowledge and skills for further study, professional upskilling, employment and participation in lifelong learning. Undergraduate Certificate qualifications are not located at a particular level in the Australian Qualifications Framework, however they cover AQF levels 5, 6, or 7. Undergraduate Certificate qualifications must be designed and accredited to enable graduates to demonstrate the learning outcomes expressed as knowledge, skills and the application of knowledge and skills specified in the Undergraduate Certificate descriptor."@en ;
    sfia:level aqflvl:5 , aqflvl:6 , aqflvl:7 ; 
    skos:inScheme aqftypecs: ;
    skos:topConceptOf aqftypecs:
    .

    aqftype:BHD a skos:Concept ;
	skos:prefLabel "Bachelor Honours Degree"@en ;
    skos:definition "The purpose of the Bachelor Honours Degree qualification type is to qualify individuals who apply a body of knowledge in a specific context to undertake professional work and as a pathway for research and further learning. Bachelor Honours Degree qualifications are located at level 8 of the Australian Qualifications Framework. Bachelor Honours Degree qualifications must be designed and accredited to enable graduates to demonstrate the learning outcomes expressed as knowledge, skills and the application of knowledge and skills specified in the level 8 criteria and the Bachelor Degree descriptor. Full qualification type specification"@en ;
    skos:notation "8" ;
    sfia:level aqflvl:8 ;
    skos:inScheme aqftypecs: ;
    skos:topConceptOf aqftypecs:
    .

    aqftype:MD a skos:Concept ;
	skos:prefLabel "Masters Degree"@en ;
    skos:definition "There are three main forms of Masters Degrees within the Masters Degree qualification type: the Masters Degree (Research), the Masters Degree (Coursework) and the Masters Degree (Extended). The purpose of the Masters Degree (Research) is to qualify individuals who apply an advanced body of knowledge in a range of contexts for research and scholarship and as a pathway for further learning. The purpose of the Masters Degree (Coursework) is to qualify individuals who apply an advanced body of knowledge in a range of contexts for professional practice or scholarship and as a pathway for further learning. The purpose of the Masters Degree (Extended) is to qualify individuals who apply an advanced body of knowledge in a range of contexts for professional practice and as a pathway for further learning. Masters Degree qualifications are located at level 9 of the Australian Qualifications Framework. Masters Degree qualifications must be designed and accredited to enable graduates to demonstrate the learning outcomes specified in the level 9 criteria and either the Masters Degree (Research) descriptor, the Masters Degree (Coursework) descriptor or the Masters Degree (Extended) descriptor."@en ;
    skos:notation "9" ;
    sfia:level aqflvl:9 ;
    skos:inScheme aqftypecs: ;
    skos:topConceptOf aqftypecs:
    .

    aqftype:DD a skos:Concept ;
	skos:prefLabel "Doctoral Degree"@en ;
    skos:definition "The purpose of the Doctoral Degree is to qualify individuals who apply a substantial body of knowledge to research, investigate and develop new knowledge, in one or more fields of investigation, scholarship or professional practice. Doctoral Degree qualifications are located at level 10 of the Australian Qualifications Framework. There are two forms of Doctoral Degree with the same descriptor within the Doctoral Degree qualification type: the Doctoral Degree (Research) and the Doctoral Degree (Professional). Research is the defining characteristic of all Doctoral Degree qualifications. The research Doctoral Degree (typically referred to as a Doctor of Philosophy) makes a significant and original contribution to knowledge; the professional Doctoral Degree (typically titled Doctor of [field of study]) makes a significant and original contribution to knowledge in the context of professional practice. The emphasis in the learning outcomes and research may differ between the different forms of Doctoral Degree qualifications but all graduates will demonstrate knowledge, skills and the application of the knowledge and skills at AQF level 10. Doctoral Degree qualifications must be designed and accredited to enable graduates to demonstrate the learning outcomes specified in the level 10 criteria and the Doctoral Degree."@en ;
    skos:notation "10" ;
    sfia:level aqflvl:10 ;
    skos:inScheme aqftypecs: ;
    skos:topConceptOf aqftypecs:
    .


aqflvlcs: a skos:ConceptScheme ;
skos:prefLabel "AQF Levels"@en ;
skos:definition "AQF levels and the AQF levels criteria are an indication of the relative complexity and/or depth of achievement and the autonomy required to demonstrate that achievement. AQF level 1 has the lowest complexity and AQF level 10 has the highest complexity. The AQF level summaries are statements of the typical achievement of graduates who have been awarded a qualification at a certain level in the AQF."@en ;
schema:citation "https://www.aqf.edu.au/framework/aqf-levels"^^xsd:anyURI ;
skos:hasTopConcept aqflvl:1 , aqflvl:2 , aqflvl:3 , aqflvl:4 , aqflvl:5 , aqflvl:6 , aqflvl:7 , aqflvl:8 , aqflvl:9 , aqflvl:10
.

aqflvl:1 a skos:Concept ;
skos:prefLabel "AQF level 1 criteria"@en ;
skos:inScheme aqflvlcs: ;
skos:topConceptOf aqflvlcs: ;
dcterms:description "Graduates at this level will have knowledge and skills for initial work, community involvement and/or further learning."@en ;
asn:skillEmbodied "Graduates at this level will have foundational cognitive, technical and communication skills to: undertake defined routine activities; identify and report simple issues and problems"@en ;
attributes:KNGE "Graduates at this level will have foundational knowledge for everyday life, further learning and preparation for initial work."@en ;
sfia:levelEssence "Graduates at this level will apply knowledge and skills to demonstrate autonomy in highly structured and stable contexts and within narrow parameters"@en
.

aqflvl:2 a skos:Concept ;
skos:prefLabel "AQF level 2 criteria"@en ;
skos:inScheme aqflvlcs: ;
skos:topConceptOf aqflvlcs: ;
dcterms:description "Graduates at this level will have knowledge and skills for work in a defined context and/or further learning."@en ;
asn:skillEmbodied "Graduates at this level will have basic cognitive, technical and communication skills to apply appropriate methods, tools, materials and readily available information to: undertake defined activities; provide solutions to a limited range of predictable problems"@en ; 
attributes:KNGE "Graduates at this level will have basic factual, technical and procedural knowledge of a defined area of work and learning."@en ;
sfia:levelEssence "Graduates at this level will apply knowledge and skills to demonstrate autonomy and limited judgement in structured and stable contexts and within narrow parameters."@en
.

aqflvl:3 a skos:Concept ;
skos:prefLabel "AQF level 3 criteria"@en ;
skos:inScheme aqflvlcs: ;
skos:topConceptOf aqflvlcs: ;
dcterms:description "Graduates at this level will have theoretical and practical knowledge and skills for work and/or further learning."@en ;
asn:skillEmbodied "Graduates at this level will have a range of cognitive, technical and communication skills to select and apply a specialised range of methods, tools, materials and information to: complete routine activities; provide and transmit solutions to predictable and sometimes unpredictable problems"@en ;
attributes:KNGE "Graduates at this level will have factual, technical, procedural and some theoretical knowledge of a specific area of work and learning."@en ;
sfia:levelEssence "Graduates at this level will apply knowledge and skills to demonstrate autonomy and judgement and to take limited responsibility in known and stable contexts within established parameters."@en
.

aqflvl:4 a skos:Concept ;
skos:prefLabel "AQF level 4 criteria"@en ;
skos:inScheme aqflvlcs: ;
skos:topConceptOf aqflvlcs: ;
dcterms:description "Graduates at this level will have theoretical and practical knowledge and skills for specialised and/or skilled work and/or further learning."@en ;
asn:skillEmbodied "Graduates at this level will have a broad range of cognitive, technical and communication skills to select and apply a range of methods, tools, materials and information to: complete routine and non-routine activities; provide and transmit solutions to a variety of predictable and sometimes unpredictable problems"@en ; 
attributes:KNGE "Graduates at this level will have broad factual, technical and some theoretical knowledge of a specific area or a broad field of work and learning."@en ;
sfia:levelEssence "Graduates at this level will apply knowledge and skills to demonstrate autonomy, judgement and limited responsibility in known or changing contexts and within established parameters."@en
.

aqflvl:5 a skos:Concept ;
skos:prefLabel "AQF level 5 criteria"@en ;
skos:inScheme aqflvlcs: ;
skos:topConceptOf aqflvlcs: ;
dcterms:description "Graduates at this level will have specialised knowledge and skills for skilled/paraprofessional work and/or further learning."@en ;
asn:skillEmbodied "Graduates at this level will have a broad range of cognitive, technical and communication skills to select and apply methods and technologies to: analyse information to complete a range of activities; provide and transmit solutions to sometimes complex problems; transmit information and skills to others"@en ; 
attributes:KNGE "Graduates at this level will have technical and theoretical knowledge in a specific area or a broad field of work and learning."@en ;
sfia:levelEssence "Graduates at this level will apply knowledge and skills to demonstrate autonomy, judgement and defined responsibility in known or changing contexts and within broad but established parameters."@en
.

aqflvl:6 a skos:Concept ;
skos:prefLabel "AQF level 6 criteria"@en ;
skos:inScheme aqflvlcs: ;
skos:topConceptOf aqflvlcs: ;
dcterms:description "Graduates at this level will have broad knowledge and skills for paraprofessional/highly skilled work and/or further learning."@en ;
asn:skillEmbodied "Graduates at this level will have a broad range of cognitive, technical and communication skills to select and apply methods and technologies to: analyse information to complete a range of activities; interpret and transmit solutions to unpredictable and sometimes complex problems; transmit information and skills to others"@en ;
attributes:KNGE "Graduates at this level will have broad theoretical and technical knowledge of a specific area or a broad field of work and learning."@en ;
sfia:levelEssence "Graduates at this level will apply knowledge and skills to demonstrate autonomy, judgement and defined responsibility: in contexts that are subject to change; within broad parameters to provide specialist advice and functions"@en
.

aqflvl:7 a skos:Concept ;
skos:prefLabel "AQF level 7 criteria"@en ;
skos:inScheme aqflvlcs: ;
skos:topConceptOf aqflvlcs: ;
dcterms:description "Graduates at this level will have broad and coherent knowledge and skills for professional work and/or further learning."@en ;
asn:skillEmbodied "Graduates at this level will have well-developed cognitive, technical and communication skills to select and apply methods and technologies to: analyse and evaluate information to complete a range of activities; analyse, generate and transmit solutions to unpredictable and sometimes complex problems; transmit knowledge, skills and ideas to others"@en ; 
attributes:KNGE "Graduates at this level will have broad and coherent theoretical and technical knowledge with depth in one or more disciplines or areas of practice."@en ;
sfia:levelEssence "Graduates at this level will apply knowledge and skills to demonstrate autonomy, well-developed judgement and responsibility: in contexts that require self-directed work and learning; within broad parameters to provide specialist advice and functions"@en
.

aqflvl:8 a skos:Concept ;
skos:prefLabel "AQF level 8 criteria"@en ;
skos:inScheme aqflvlcs: ;
skos:topConceptOf aqflvlcs: ;
dcterms:description "Graduates at this level will have advanced knowledge and skills for professional or highly skilled work and/or further learning."@en ;
asn:skillEmbodied "Graduates at this level will have advanced cognitive, technical and communication skills to select and apply methods and technologies to: analyse critically, evaluate and transform information to complete a range of activities; analyse, generate and transmit solutions to complex problems; transmit knowledge, skills and ideas to others"@en ; 
attributes:KNGE "Graduates at this level will have advanced theoretical and technical knowledge in one or more disciplines or areas of practice"@en ;
sfia:levelEssence "Graduates at this level will apply knowledge and skills to demonstrate autonomy, well-developed judgement, adaptability and responsibility as a practitioner or learner."@en
.

aqflvl:9 a skos:Concept ;
skos:prefLabel "AQF level 9 criteria"@en ;
skos:inScheme aqflvlcs: ;
skos:topConceptOf aqflvlcs: ;
dcterms:description "Graduates at this level will have specialised knowledge and skills for research, and/or professional practice and/or further learning."@en ;
asn:skillEmbodied "Graduates at this level will have expert, specialised cognitive and technical skills in a body of knowledge or practice to independently: analyse critically, reflect on and synthesise complex information, problems, concepts and theories; research and apply established theories to a body of knowledge or practice; interpret and transmit knowledge, skills and ideas to specialist and non-specialist audiences"@en ; 
attributes:KNGE "Graduates at this level will have advanced and integrated understanding of a complex body of knowledge in one or more disciplines or areas of practice."@en ;
sfia:levelEssence "Graduates at this level will apply knowledge and skills to demonstrate autonomy, expert judgement, adaptability and responsibility as a practitioner or learner."@en
.

aqflvl:10 a skos:Concept ;
skos:prefLabel "AQF level 10 criteria"@en ;
skos:inScheme aqflvlcs: ;
skos:topConceptOf aqflvlcs: ;
dcterms:description "Graduates at this level will have systematic and critical understanding of a complex field of learning and specialised research skills for the advancement of learning and/or for professional practice."@en ;
asn:skillEmbodied "Graduates at this level will have expert, specialised cognitive, technical and research skills in a discipline area to independently and systematically: engage in critical reflection, synthesis and evaluation; develop, adapt and implement research methodologies to extend and redefine existing knowledge or professional practice; disseminate and promote new insights to peers and the community; generate original knowledge and understanding to make a substantial contribution to a discipline or area of professional practice"@en ; 
attributes:KNGE "Graduates at this level will have systemic and critical understanding of a substantial and complex body of knowledge at the frontier of a discipline or area of professional practice."@en ;
sfia:levelEssence "Graduates at this level will apply knowledge and skills to demonstrate autonomy, authoritative judgement, adaptability and responsibility as an expert and leading practitioner or scholar."@en 
.
