PREFIX abs: <https://linked.data.gov.au/org/abs>
PREFIX asced: <https://abs.gov.au/classifications/ASCED/>
PREFIX ascedcs: <https://abs.gov.au/classifications/ASCED>
PREFIX dcterms: <http://purl.org/dc/terms/>
PREFIX dewr: <https://linked.data.gov.au/org/dewr>
PREFIX jsa: <https://linked.data.gov.au/org/jsa>
PREFIX schema: <https://schema.org/>
PREFIX skos: <http://www.w3.org/2004/02/skos/core#>
PREFIX xsd: <http://www.w3.org/2001/XMLSchema#>

abs: a schema:Organization ;
    schema:alternateName "ABS"@en ;
    schema:name "Australian Bureau of Statistics"@en ;
    schema:url "https://www.abs.gov.au"^^xsd:anyURI .

dewr: a schema:Organization ;
    schema:alternateName "Department of Education and Workplace Relations"@en ;
    schema:name "DEWR"@en ;
    schema:url "https://www.jobsandskills.gov.au"^^xsd:anyURI .

jsa: a schema:Organization ;
    schema:alternateName "JSA"@en ;
    schema:name "Jobs and Skills Australia"@en ;
    schema:url "https://www.jobsandskills.gov.au"^^xsd:anyURI .

asced:010101 a skos:Concept,
        skos:Concpet ;
    dcterms:created "2025-08-01T01:49:07.899000+00:00"^^xsd:dateTime ;
    dcterms:modified "2025-08-05T22:47:55.381000+00:00"^^xsd:dateTime ;
    skos:broader asced:0101 ;
    skos:definition "Mathematics is the study of deductive systems, including algebra, arithmetic, geometry, analysis and applied mathematics." ;
    skos:example "calculus, numerical analysis, combinatorics, optimisation, topology, trigonometry" ;
    skos:inScheme ascedcs: ;
    skos:notation "010101" ;
    skos:prefLabel "Mathematics"@en .

asced:010103 a skos:Concept ;
    dcterms:created "2025-08-01T01:49:07.901000+00:00"^^xsd:dateTime ;
    dcterms:modified "2025-08-05T22:47:55.438000+00:00"^^xsd:dateTime ;
    skos:broader asced:0101 ;
    skos:definition "Statistics is the study of collecting, describing, arranging and analysing numerical data." ;
    skos:example "biometrics, linear and multivariate models, probability estimations, statistical significance tests, stochastic processes, time series analysis" ;
    skos:inScheme ascedcs: ;
    skos:notation "010103" ;
    skos:prefLabel "Statistics"@en ;
    skos:scopeNote "Exclusions: Econometrics. This is included in Detailed Field 091903 Econometrics." .

asced:010199 a skos:Concept ;
    dcterms:created "2025-08-01T01:49:07.902000+00:00"^^xsd:dateTime ;
    dcterms:modified "2025-08-05T22:47:55.494000+00:00"^^xsd:dateTime ;
    skos:broader asced:0101 ;
    skos:definition "This detailed field includes all Mathematical Sciences not elsewhere classified." ;
    skos:inScheme ascedcs: ;
    skos:notation "010199" ;
    skos:prefLabel "Mathematical Sciences, n.e.c."@en .

asced:010301 a skos:Concept ;
    dcterms:created "2025-08-01T01:49:07.904000+00:00"^^xsd:dateTime ;
    dcterms:modified "2025-08-05T22:47:55.549000+00:00"^^xsd:dateTime ;
    skos:broader asced:0103 ;
    skos:definition "Physics is the study of the laws governing states and properties of matter and energy." ;
    skos:example "acoustics, gravitation, .solid and liquid states, geometric optics, quantum mechanics, thermodynamics" ;
    skos:inScheme ascedcs: ;
    skos:notation "010301" ;
    skos:prefLabel "Physics"@en .

asced:010303 a skos:Concept ;
    dcterms:created "2025-08-01T01:49:07.905000+00:00"^^xsd:dateTime ;
    dcterms:modified "2025-08-05T22:47:55.601000+00:00"^^xsd:dateTime ;
    skos:broader asced:0103 ;
    skos:definition "Astronomy is the study of celestial bodies, their positions, motions, distances and physical conditions, and their origins and evolution." ;
    skos:example "astrophysics, celestial mechanics, cosmology" ;
    skos:inScheme ascedcs: ;
    skos:notation "010303" ;
    skos:prefLabel "Astronomy"@en .

asced:010501 a skos:Concept ;
    dcterms:created "2025-08-01T01:49:07.908000+00:00"^^xsd:dateTime ;
    dcterms:modified "2025-08-05T22:47:55.653000+00:00"^^xsd:dateTime ;
    skos:broader asced:0105 ;
    skos:definition "Organic Chemistry is the study of the description, properties, reactions and preparations of carbon compounds." ;
    skos:example "aromatic compounds, carbon-carbon bond formation, free radicals, hydrocarbons, isomerism, organic synthesis" ;
    skos:inScheme ascedcs: ;
    skos:notation "010501" ;
    skos:prefLabel "Organic Chemistry"@en ;
    skos:scopeNote "Exclusions: Biochemistry. This is included in Detailed Field 010901 Biochemistry and Cell Biology." .

asced:010503 a skos:Concept ;
    dcterms:created "2025-08-01T01:49:07.909000+00:00"^^xsd:dateTime ;
    dcterms:modified "2025-08-05T22:47:55.707000+00:00"^^xsd:dateTime ;
    skos:broader asced:0105 ;
    skos:definition "Inorganic Chemistry is the study of the description, properties, reactions, and preparation of all the elements and their compounds, with the exception of carbon compounds." ;
    skos:example "crystallography, main group metal chemistry, non-metal chemistry, structural basis of inorganic solids" ;
    skos:inScheme ascedcs: ;
    skos:notation "010503" ;
    skos:prefLabel "Inorganic Chemistry"@en .

asced:010599 a skos:Concept ;
    dcterms:created "2025-08-01T01:49:07.910000+00:00"^^xsd:dateTime ;
    dcterms:modified "2025-08-05T22:47:55.762000+00:00"^^xsd:dateTime ;
    skos:broader asced:0105 ;
    skos:definition "This detailed field includes all Chemical Sciences not elsewhere classified." ;
    skos:example "analytical chemistry, colloid science, environmental chemistry, theoretical chemistry, physical chemistry" ;
    skos:inScheme ascedcs: ;
    skos:notation "010599" ;
    skos:prefLabel "Chemical Sciences, n.e.c."@en ;
    skos:scopeNote "Exclusions: Geochemistry. This is included in Detailed Field 010707 Geochemistry." .

asced:010701 a skos:Concept ;
    dcterms:created "2025-08-01T01:49:07.912000+00:00"^^xsd:dateTime ;
    dcterms:modified "2025-08-05T22:47:55.813000+00:00"^^xsd:dateTime ;
    skos:broader asced:0107 ;
    skos:definition "Atmospheric Sciences is the study of the composition and structure of the earth's atmosphere and climate." ;
    skos:example "atmospheric stability, moisture and motion, climatology, meteorology" ;
    skos:inScheme ascedcs: ;
    skos:notation "010701" ;
    skos:prefLabel "Atmospheric Sciences"@en .

asced:010703 a skos:Concept ;
    dcterms:created "2025-08-01T01:49:07.914000+00:00"^^xsd:dateTime ;
    dcterms:modified "2025-08-05T22:47:55.865000+00:00"^^xsd:dateTime ;
    skos:broader asced:0107 ;
    skos:definition "Geology is the study of origin, composition and structure of the earth." ;
    skos:example "coastal and marine geoscience, sedimentology, mineralogy, petrology, tectonics, volcanology" ;
    skos:inScheme ascedcs: ;
    skos:notation "010703" ;
    skos:prefLabel "Geology"@en ;
    skos:scopeNote "Exclusions: Palaeontology. This is included in Detailed Field 019999 Natural and Physical Sciences, n.e.c." .

asced:010705 a skos:Concept ;
    dcterms:created "2025-08-01T01:49:07.915000+00:00"^^xsd:dateTime ;
    dcterms:modified "2025-08-05T22:47:55.919000+00:00"^^xsd:dateTime ;
    skos:broader asced:0107 ;
    skos:definition "Geophysics is the study of the physical properties of the Earth through collecting and interpreting gravitational, magnetic, seismic and electrical data." ;
    skos:example "electrical properties of rocks and minerals, geomagnetism, petrophysics, seismology" ;
    skos:inScheme ascedcs: ;
    skos:notation "010705" ;
    skos:prefLabel "Geophysics"@en .

asced:010707 a skos:Concept ;
    dcterms:created "2025-08-01T01:49:07.916000+00:00"^^xsd:dateTime ;
    dcterms:modified "2025-08-05T22:47:55.974000+00:00"^^xsd:dateTime ;
    skos:broader asced:0107 ;
    skos:definition "Geochemistry is the study of the quantities and distribution of the chemical elements in minerals, ores, rocks, soils, water, and the atmosphere." ;
    skos:example "hydrogeochemistry, sediment geochemistry" ;
    skos:inScheme ascedcs: ;
    skos:notation "010707" ;
    skos:prefLabel "Geochemistry"@en .

asced:010709 a skos:Concept ;
    dcterms:created "2025-08-01T01:49:07.917000+00:00"^^xsd:dateTime ;
    dcterms:modified "2025-08-05T22:47:56.026000+00:00"^^xsd:dateTime ;
    skos:broader asced:0107 ;
    skos:definition "Soil Science is the study of the origins, composition, structure and classification of soils." ;
    skos:example "soil nutrient and water supply, soils in the landscape, the soil environment, soil mineralogy" ;
    skos:inScheme ascedcs: ;
    skos:notation "010709" ;
    skos:prefLabel "Soil Science"@en .

asced:010711 a skos:Concept ;
    dcterms:created "2025-08-01T01:49:07.918000+00:00"^^xsd:dateTime ;
    dcterms:modified "2025-08-05T22:47:56.082000+00:00"^^xsd:dateTime ;
    skos:broader asced:0107 ;
    skos:definition "Hydrology is the study of the location and movement of inland water, both frozen and liquid, above and below ground." ;
    skos:example "flood estimation models and procedures, groundwater modelling, water catchments, water resources" ;
    skos:inScheme ascedcs: ;
    skos:notation "010711" ;
    skos:prefLabel "Hydrology"@en .

asced:010713 a skos:Concept ;
    dcterms:created "2025-08-01T01:49:07.919000+00:00"^^xsd:dateTime ;
    dcterms:modified "2025-08-05T22:47:56.134000+00:00"^^xsd:dateTime ;
    skos:broader asced:0107 ;
    skos:definition "Oceanography is the study of the origins, composition, structure and history of the oceans and the ocean floor." ;
    skos:example "chemical and physical properties of seawater, currents, waves and tides, ocean floor topography" ;
    skos:inScheme ascedcs: ;
    skos:notation "010713" ;
    skos:prefLabel "Oceanography"@en .

asced:010799 a skos:Concept ;
    dcterms:created "2025-08-01T01:49:07.920000+00:00"^^xsd:dateTime ;
    dcterms:modified "2025-08-05T22:47:56.186000+00:00"^^xsd:dateTime ;
    skos:broader asced:0107 ;
    skos:definition "This detailed field includes all Earth Sciences not elsewhere classified." ;
    skos:example "physical geography" ;
    skos:inScheme ascedcs: ;
    skos:notation "010799" ;
    skos:prefLabel "Earth Sciences, n.e.c."@en .

asced:010901 a skos:Concept ;
    dcterms:created "2025-08-01T01:49:07.922000+00:00"^^xsd:dateTime ;
    dcterms:modified "2025-08-05T22:47:56.240000+00:00"^^xsd:dateTime ;
    skos:broader asced:0109 ;
    skos:definition "Biochemistry and Cell Biology is the study of the chemistry of living organisms and the structure and function of cells." ;
    skos:example "biosynthesis, cellular regulation, cytology, molecular biology, metabolism" ;
    skos:inScheme ascedcs: ;
    skos:notation "010901" ;
    skos:prefLabel "Biochemistry and Cell Biology"@en ;
    skos:scopeNote "Exclusions: Medical biochemistry. This is included in Detailed Field 019901 Medical Science." .

asced:010903 a skos:Concept ;
    dcterms:created "2025-08-01T01:49:07.923000+00:00"^^xsd:dateTime ;
    dcterms:modified "2025-08-05T22:47:56.299000+00:00"^^xsd:dateTime ;
    skos:broader asced:0109 ;
    skos:definition "Botany is the study of plants." ;
    skos:example "plant anatomy, plant histology, plant morphology, plant physiology, plant taxonomy" ;
    skos:inScheme ascedcs: ;
    skos:notation "010903" ;
    skos:prefLabel "Botany"@en ;
    skos:scopeNote "Exclusions: Palaeobotany. This is included in Detailed Field 019999 Natural and Physical Sciences, n.e.c. Horticulture. This is included in Detailed Field 050301 Horticulture." .

asced:010905 a skos:Concept ;
    dcterms:created "2025-08-01T01:49:07.924000+00:00"^^xsd:dateTime ;
    dcterms:modified "2025-08-05T22:47:56.357000+00:00"^^xsd:dateTime ;
    skos:broader asced:0109 ;
    skos:definition "Ecology and Evolution is the study of interactions between organisms and their environment, and the processes of biological change in organisms." ;
    skos:example "autecology, biodiversity, ecosystems, habitats, organic population studies, synecology" ;
    skos:inScheme ascedcs: ;
    skos:notation "010905" ;
    skos:prefLabel "Ecology and Evolution"@en ;
    skos:scopeNote "Exclusions: Human and primate evolution. These are included in Detailed Field 010913 Human Biology." .

asced:010907 a skos:Concept ;
    dcterms:created "2025-08-01T01:49:07.925000+00:00"^^xsd:dateTime ;
    dcterms:modified "2025-08-05T22:47:56.407000+00:00"^^xsd:dateTime ;
    skos:broader asced:0109 ;
    skos:definition "Marine Science is the study of marine and estuarine plants and wildlife. It includes freshwater science." ;
    skos:example "marine, estuarine and freshwater biology, marine, estuarine and freshwater ecology" ;
    skos:inScheme ascedcs: ;
    skos:notation "010907" ;
    skos:prefLabel "Marine Science"@en .

asced:010909 a skos:Concept ;
    dcterms:created "2025-08-01T01:49:07.926000+00:00"^^xsd:dateTime ;
    dcterms:modified "2025-08-05T22:47:56.461000+00:00"^^xsd:dateTime ;
    skos:broader asced:0109 ;
    skos:definition "Genetics is the study of heredity and the units of biological inheritance." ;
    skos:example "cytogenetics, genotypes, microbial genetics, gene expression, molecular genetics, monohybrids, phenotypes" ;
    skos:inScheme ascedcs: ;
    skos:notation "010909" ;
    skos:prefLabel "Genetics"@en ;
    skos:scopeNote "Exclusions: Recombinant DNA technology. This is included in Detailed Field 019905 Food Science and Biotechnology." .

asced:010911 a skos:Concept ;
    dcterms:created "2025-08-01T01:49:07.927000+00:00"^^xsd:dateTime ;
    dcterms:modified "2025-08-05T22:47:56.518000+00:00"^^xsd:dateTime ;
    skos:broader asced:0109 ;
    skos:definition "Microbiology is the study of microscopic forms of life such as bacteria, viruses and protozoa." ;
    skos:example "microbial ecology, microbial physiology, microbial taxonomy, virology" ;
    skos:inScheme ascedcs: ;
    skos:notation "010911" ;
    skos:prefLabel "Microbiology"@en ;
    skos:scopeNote "Exclusions: Medical microbiology. This is included in Detailed Field 019901 Medical Science." .

asced:010913 a skos:Concept ;
    dcterms:created "2025-08-01T01:49:07.928000+00:00"^^xsd:dateTime ;
    dcterms:modified "2025-08-05T22:47:56.573000+00:00"^^xsd:dateTime ;
    skos:broader asced:0109 ;
    skos:definition "Human Biology is the study of human and primate anatomy, physiology, evolution and biosocial interactions." ;
    skos:example "biological anthropology, human histology, human evolution and variation, human growth, development and reproduction, primatology" ;
    skos:inScheme ascedcs: ;
    skos:notation "010913" ;
    skos:prefLabel "Human Biology"@en .

asced:010915 a skos:Concept ;
    dcterms:created "2025-08-01T01:49:07.929000+00:00"^^xsd:dateTime ;
    dcterms:modified "2025-08-05T22:47:56.616000+00:00"^^xsd:dateTime ;
    skos:broader asced:0109 ;
    skos:definition "Zoology is the study of animals and insects." ;
    skos:example "animal anatomy, animal behaviour, animal embryology, animal physiology, animal taxonomy, entomology" ;
    skos:inScheme ascedcs: ;
    skos:notation "010915" ;
    skos:prefLabel "Zoology"@en .

asced:010999 a skos:Concept ;
    dcterms:created "2025-08-01T01:49:07.930000+00:00"^^xsd:dateTime ;
    dcterms:modified "2025-08-05T22:47:56.662000+00:00"^^xsd:dateTime ;
    skos:broader asced:0109 ;
    skos:definition "This detailed field includes all Biological Sciences not elsewhere classified." ;
    skos:example "biogeography, bioinformatics, biophysics, mycology, neuroscience, parasitology" ;
    skos:inScheme ascedcs: ;
    skos:notation "010999" ;
    skos:prefLabel "Biological Sciences, n.e.c."@en .

asced:019901 a skos:Concept ;
    dcterms:created "2025-08-01T01:49:07.932000+00:00"^^xsd:dateTime ;
    dcterms:modified "2025-08-05T22:47:56.724000+00:00"^^xsd:dateTime ;
    skos:broader asced:0199 ;
    skos:definition "Medical Science is the study of the application of physics, biology and chemistry to medicine." ;
    skos:example "biomedical science, clinical and medical biochemistry, medical biotechnology, clinical and medical microbiology, medical physics" ;
    skos:inScheme ascedcs: ;
    skos:notation "019901" ;
    skos:prefLabel "Medical Science"@en ;
    skos:scopeNote "Exclusions: Biomedical engineering. This is included in Detailed Field 039903 Biomedical Engineering. Pathology and histopathology. These are included in Detailed Field 060113 Pathology. Radiology. This is included in Detailed Field 060115 Radiology." .

asced:019903 a skos:Concept ;
    dcterms:created "2025-08-01T01:49:07.933000+00:00"^^xsd:dateTime ;
    dcterms:modified "2025-08-05T22:47:56.779000+00:00"^^xsd:dateTime ;
    skos:broader asced:0199 ;
    skos:definition "Forensic Science is the study of the application of scientific techniques to criminal investigations." ;
    skos:example "ballistics, blood splash pattern analysis, crime scene investigation, fingerprint enhancement and identification, trace evidence, fire and explosion investigation" ;
    skos:inScheme ascedcs: ;
    skos:notation "019903" ;
    skos:prefLabel "Forensic Science"@en .

asced:019905 a skos:Concept ;
    dcterms:created "2025-08-01T01:49:07.934000+00:00"^^xsd:dateTime ;
    dcterms:modified "2025-08-05T22:47:56.837000+00:00"^^xsd:dateTime ;
    skos:broader asced:0199 ;
    skos:definition "Food Science and Biotechnology is the study of the physical and chemical properties of food, and the industrial use of living organisms to produce food, pharmaceuticals and other products." ;
    skos:example "fermentation, food analogues, food preservation: heating, chilling, freezing, dehydration, salt, sugar, acids, and chemical preservatives, oenology, protein technology, recombinant DNA technology" ;
    skos:inScheme ascedcs: ;
    skos:notation "019905" ;
    skos:prefLabel "Food Science and Biotechnology"@en ;
    skos:scopeNote "Exclusions: Food microbiology. This is included in Detailed Field 010911 Microbiology." .

asced:019907 a skos:Concept ;
    dcterms:created "2025-08-01T01:49:07.935000+00:00"^^xsd:dateTime ;
    dcterms:modified "2025-08-05T22:47:56.878000+00:00"^^xsd:dateTime ;
    skos:broader asced:0199 ;
    skos:definition "Pharmacology is the study of the development, uses and effects of drugs." ;
    skos:example "clinical drug trials, drug analysis, pharmacodynamics, pharmacokinetics, toxicology" ;
    skos:inScheme ascedcs: ;
    skos:notation "019907" ;
    skos:prefLabel "Pharmacology"@en .

asced:019909 a skos:Concept ;
    dcterms:created "2025-08-01T01:49:07.936000+00:00"^^xsd:dateTime ;
    dcterms:modified "2025-08-05T22:47:56.926000+00:00"^^xsd:dateTime ;
    skos:broader asced:0199 ;
    skos:definition "Laboratory Technology is the study of the procedures, techniques and equipment used in biological, chemical, medical and other laboratories." ;
    skos:example "chromatography, laboratory safety, microscopy, spectroscopy, sample preparation and handling" ;
    skos:inScheme ascedcs: ;
    skos:notation "019909" ;
    skos:prefLabel "Laboratory Technology"@en ;
    skos:scopeNote "Exclusions: Radiology. This is included in Detailed Field 060115 Radiology." .

asced:019999 a skos:Concept ;
    dcterms:created "2025-08-01T01:49:07.937000+00:00"^^xsd:dateTime ;
    dcterms:modified "2025-08-05T22:47:56.970000+00:00"^^xsd:dateTime ;
    skos:broader asced:0199 ;
    skos:definition "This detailed field includes all Natural and Physical Sciences not elsewhere classified." ;
    skos:example "palaeobotany, palaeontology" ;
    skos:inScheme ascedcs: ;
    skos:notation "019999" ;
    skos:prefLabel "Natural and Physical Sciences, n.e.c."@en .

asced:020101 a skos:Concept ;
    dcterms:created "2025-08-01T01:49:07.940000+00:00"^^xsd:dateTime ;
    dcterms:modified "2025-08-05T22:47:57.196000+00:00"^^xsd:dateTime ;
    skos:broader asced:0201 ;
    skos:definition "Formal Language Theory is the study of automated formal languages and the algorithms used to recognise them." ;
    skos:example "finite automata, formal grammars, language limitations, recognition and representation, rational languages, syntax analysis and specification" ;
    skos:inScheme ascedcs: ;
    skos:notation "020101" ;
    skos:prefLabel "Formal Language Theory"@en .

asced:020103 a skos:Concept ;
    dcterms:created "2025-08-01T01:49:07.941000+00:00"^^xsd:dateTime ;
    dcterms:modified "2025-08-05T22:47:57.237000+00:00"^^xsd:dateTime ;
    skos:broader asced:0201 ;
    skos:definition "Programming is the study of writing coded instructions for computers to perform particular tasks." ;
    skos:example "imperative, functional, logic and object programming paradigms, iterative and recursive processes, program development, software engineering, specific language written machine codes" ;
    skos:inScheme ascedcs: ;
    skos:notation "020103" ;
    skos:prefLabel "Programming"@en .

asced:020105 a skos:Concept ;
    dcterms:created "2025-08-01T01:49:07.942000+00:00"^^xsd:dateTime ;
    dcterms:modified "2025-08-05T22:47:57.283000+00:00"^^xsd:dateTime ;
    skos:broader asced:0201 ;
    skos:definition "Computational Theory is the study of problems that can be solved using efficient algorithms and the identification of problems that are unsolvable." ;
    skos:example "problem solving" ;
    skos:inScheme ascedcs: ;
    skos:notation "020105" ;
    skos:prefLabel "Computational Theory"@en ;
    skos:scopeNote "Exclusions: Numerical analysis. This is included in Detailed Field 010101 Mathematics." .

asced:020107 a skos:Concept ;
    dcterms:created "2025-08-01T01:49:07.943000+00:00"^^xsd:dateTime ;
    dcterms:modified "2025-08-05T22:47:57.324000+00:00"^^xsd:dateTime ;
    skos:broader asced:0201 ;
    skos:definition "Compiler Construction is the study of the theories and techniques for translating instructions between high and low level languages." ;
    skos:example "automated syntax error correction, code generation, object programs, source programs" ;
    skos:inScheme ascedcs: ;
    skos:notation "020107" ;
    skos:prefLabel "Compiler Construction"@en .

asced:020109 a skos:Concept ;
    dcterms:created "2025-08-01T01:49:07.944000+00:00"^^xsd:dateTime ;
    dcterms:modified "2025-08-05T22:47:57.375000+00:00"^^xsd:dateTime ;
    skos:broader asced:0201 ;
    skos:definition "Algorithms is the study of the processes and rules that describe the logical sequence of operations to be performed by a program." ;
    skos:example "algorithm analysis, algorithm application, algorithm design" ;
    skos:inScheme ascedcs: ;
    skos:notation "020109" ;
    skos:prefLabel "Algorithms"@en .

asced:020111 a skos:Concept ;
    dcterms:created "2025-08-01T01:49:07.945000+00:00"^^xsd:dateTime ;
    dcterms:modified "2025-08-05T22:47:57.415000+00:00"^^xsd:dateTime ;
    skos:broader asced:0201 ;
    skos:definition "Data Structures is the study of the system of relationships between items of data which permit efficient manipulation through reducing complexity." ;
    skos:example "adjacency matrix, hash, linked list, queue, table, tree structures" ;
    skos:inScheme ascedcs: ;
    skos:notation "020111" ;
    skos:prefLabel "Data Structures"@en .

asced:020113 a skos:Concept ;
    dcterms:created "2025-08-01T01:49:07.946000+00:00"^^xsd:dateTime ;
    dcterms:modified "2025-08-05T22:47:57.460000+00:00"^^xsd:dateTime ;
    skos:broader asced:0201 ;
    skos:definition "Networks and Communications is the study of linking computers for information exchange and distribution." ;
    skos:example "distributive systems, local area networks, network architectures, network organisation, network protocol" ;
    skos:inScheme ascedcs: ;
    skos:notation "020113" ;
    skos:prefLabel "Networks and Communications"@en .

asced:020115 a skos:Concept ;
    dcterms:created "2025-08-01T01:49:07.947000+00:00"^^xsd:dateTime ;
    dcterms:modified "2025-08-05T22:47:57.511000+00:00"^^xsd:dateTime ;
    skos:broader asced:0201 ;
    skos:definition "Computer Graphics is the study of developing and programming graphical output devices to generate pictures." ;
    skos:example "2D and 3D graphics systems, computer animation, ray tracing, scan conversion, shading and texturing, vector and bit-mapped graphics" ;
    skos:inScheme ascedcs: ;
    skos:notation "020115" ;
    skos:prefLabel "Computer Graphics"@en ;
    skos:scopeNote "Exclusions: Animation using computers. This is included in Detailed Field 100399 Visual Arts and Crafts, n.e.c." .

asced:020117 a skos:Concept ;
    dcterms:created "2025-08-01T01:49:07.948000+00:00"^^xsd:dateTime ;
    dcterms:modified "2025-08-05T22:47:57.560000+00:00"^^xsd:dateTime ;
    skos:broader asced:0201 ;
    skos:definition "Operating Systems is the study of designing and constructing systems to control processes and process scheduling." ;
    skos:example "concurrency and synchronisation, file systems, memory management, multi-tasking systems" ;
    skos:inScheme ascedcs: ;
    skos:notation "020117" ;
    skos:prefLabel "Operating Systems"@en .

asced:020119 a skos:Concept ;
    dcterms:created "2025-08-01T01:49:07.949000+00:00"^^xsd:dateTime ;
    dcterms:modified "2025-08-05T22:47:57.611000+00:00"^^xsd:dateTime ;
    skos:broader asced:0201 ;
    skos:definition "Artificial Intelligence is the study of creating computer programs which demonstrate some of the attributes associated with human intelligence." ;
    skos:example "automated problem solving, automated reasoning and theorem proving, expert systems, game playing, machine learning, searching" ;
    skos:inScheme ascedcs: ;
    skos:notation "020119" ;
    skos:prefLabel "Artificial Intelligence"@en .

asced:020199 a skos:Concept ;
    dcterms:created "2025-08-01T01:49:07.950000+00:00"^^xsd:dateTime ;
    dcterms:modified "2025-08-05T22:47:57.657000+00:00"^^xsd:dateTime ;
    skos:broader asced:0201 ;
    skos:definition "This detailed field includes all Computer Science not elsewhere classified." ;
    skos:inScheme ascedcs: ;
    skos:notation "020199" ;
    skos:prefLabel "Computer Science, n.e.c."@en .

asced:020301 a skos:Concept ;
    dcterms:created "2025-08-01T01:49:07.952000+00:00"^^xsd:dateTime ;
    dcterms:modified "2025-08-05T22:47:57.717000+00:00"^^xsd:dateTime ;
    skos:broader asced:0203 ;
    skos:definition "Conceptual Modelling is the study of representing the structure, type, and relationships of data elements within a system used to support system design." ;
    skos:example "entity relationship modelling" ;
    skos:inScheme ascedcs: ;
    skos:notation "020301" ;
    skos:prefLabel "Conceptual Modelling"@en .

asced:020303 a skos:Concept ;
    dcterms:created "2025-08-01T01:49:07.953000+00:00"^^xsd:dateTime ;
    dcterms:modified "2025-08-05T22:47:57.781000+00:00"^^xsd:dateTime ;
    skos:broader asced:0203 ;
    skos:definition "Database Management is the study of programs which create and maintain databases." ;
    skos:example "database independence, distributed databases, logic based databases, object oriented databases, relational databases" ;
    skos:inScheme ascedcs: ;
    skos:notation "020303" ;
    skos:prefLabel "Database Management"@en .

asced:020305 a skos:Concept ;
    dcterms:created "2025-08-01T01:49:07.954000+00:00"^^xsd:dateTime ;
    dcterms:modified "2025-08-05T22:47:57.831000+00:00"^^xsd:dateTime ;
    skos:broader asced:0203 ;
    skos:definition "Systems Analysis and Design is the study of analysing the information needs of the user and designing or modifying a system to meet these needs." ;
    skos:example "data and process modelling, identifying system components, general systems theory, systems software engineering, systems design, systems development lifecycle" ;
    skos:inScheme ascedcs: ;
    skos:notation "020305" ;
    skos:prefLabel "Systems Analysis and Design"@en .

asced:020307 a skos:Concept ;
    dcterms:created "2025-08-01T01:49:07.955000+00:00"^^xsd:dateTime ;
    dcterms:modified "2025-08-05T22:47:57.877000+00:00"^^xsd:dateTime ;
    skos:broader asced:0203 ;
    skos:definition "Decision Support Systems is the study of designing information systems based on statistical and mathematical models to support management decisions." ;
    skos:example "linear and dynamic decision making approaches, multicriteria design decision making, optimisation and simulation models, utilisation of appropriate models" ;
    skos:inScheme ascedcs: ;
    skos:notation "020307" ;
    skos:prefLabel "Decision Support Systems"@en ;
    skos:scopeNote "Exclusions: Expert systems. This is included in Detailed Field 020119 Artificial Intelligence." .

asced:020399 a skos:Concept ;
    dcterms:created "2025-08-01T01:49:07.956000+00:00"^^xsd:dateTime ;
    dcterms:modified "2025-08-05T22:47:57.938000+00:00"^^xsd:dateTime ;
    skos:broader asced:0203 ;
    skos:definition "This detailed field includes all Information Systems not elsewhere classified." ;
    skos:inScheme ascedcs: ;
    skos:notation "020399" ;
    skos:prefLabel "Information Systems, n.e.c."@en .

asced:029901 a skos:Concept ;
    dcterms:created "2025-08-01T01:49:07.959000+00:00"^^xsd:dateTime ;
    dcterms:modified "2025-08-05T22:47:57.989000+00:00"^^xsd:dateTime ;
    skos:broader asced:0299 ;
    skos:definition "Security Science is the study of securing electronic information and preventing unauthorised access to data and programs." ;
    skos:example "computer viruses, cryptology, digital signatures, secure multi-party computation, smart cards, system security" ;
    skos:inScheme ascedcs: ;
    skos:notation "029901" ;
    skos:prefLabel "Security Science"@en .

asced:029999 a skos:Concept ;
    dcterms:created "2025-08-01T01:49:07.960000+00:00"^^xsd:dateTime ;
    dcterms:modified "2025-08-05T22:47:58.038000+00:00"^^xsd:dateTime ;
    skos:broader asced:0299 ;
    skos:definition "This detailed field includes all Information Technology not elsewhere classified." ;
    skos:example "human computer interaction, network administration, systems administration" ;
    skos:inScheme ascedcs: ;
    skos:notation "029999" ;
    skos:prefLabel "Information Technology, n.e.c."@en .

asced:030101 a skos:Concept ;
    dcterms:created "2025-08-01T01:49:07.962000+00:00"^^xsd:dateTime ;
    dcterms:modified "2025-08-05T22:47:58.658000+00:00"^^xsd:dateTime ;
    skos:broader asced:0301 ;
    skos:definition "Manufacturing Engineering is the study of designing, developing and organising safe and flexible manufacturing processes, systems and facilities." ;
    skos:example "automation, computer-aided manufacture, flexible manufacturing systems, general and specialised machinery, mechanised assembly and specialised joining processes, mechatronics" ;
    skos:inScheme ascedcs: ;
    skos:notation "030101" ;
    skos:prefLabel "Manufacturing Engineering"@en .

asced:030103 a skos:Concept ;
    dcterms:created "2025-08-01T01:49:07.963000+00:00"^^xsd:dateTime ;
    dcterms:modified "2025-08-05T22:47:58.717000+00:00"^^xsd:dateTime ;
    skos:broader asced:0301 ;
    skos:definition "Printing is the study of reproducing texts and pictorial works onto any media from original plates and masters, and producing finished publications. It includes electronic (desktop) publishing." ;
    skos:example "binding and finishing techniques, design, composition and layout, operating printing machinery, printing techniques" ;
    skos:inScheme ascedcs: ;
    skos:notation "030103" ;
    skos:prefLabel "Printing"@en .

asced:030105 a skos:Concept ;
    dcterms:created "2025-08-01T01:49:07.966000+00:00"^^xsd:dateTime ;
    dcterms:modified "2025-08-05T22:47:58.769000+00:00"^^xsd:dateTime ;
    skos:broader asced:0301 ;
    skos:definition "Textile Making is the study of the commercial production of textiles, yarns and fabrics." ;
    skos:example "dye and colouration techniques, fibre technology, textile technology, weaving and tufting, yarn manufacture" ;
    skos:inScheme ascedcs: ;
    skos:notation "030105" ;
    skos:prefLabel "Textile Making"@en .

asced:030107 a skos:Concept ;
    dcterms:created "2025-08-01T01:49:07.967000+00:00"^^xsd:dateTime ;
    dcterms:modified "2025-08-05T22:47:58.821000+00:00"^^xsd:dateTime ;
    skos:broader asced:0301 ;
    skos:definition "Garment Making is the study of the commercial production of clothing and other apparel." ;
    skos:example "fabric spreading, garment assembly, marking and cutting, pattern construction and apparel fitting principles" ;
    skos:inScheme ascedcs: ;
    skos:notation "030107" ;
    skos:prefLabel "Garment Making"@en .

asced:030109 a skos:Concept ;
    dcterms:created "2025-08-01T01:49:07.968000+00:00"^^xsd:dateTime ;
    dcterms:modified "2025-08-05T22:47:58.867000+00:00"^^xsd:dateTime ;
    skos:broader asced:0301 ;
    skos:definition "Footwear Making is the study of designing, making and repairing shoes, boots and other footwear." ;
    skos:example "clicking, measurement and fitting, footwear pattern design and cutting, shoe repairing" ;
    skos:inScheme ascedcs: ;
    skos:notation "030109" ;
    skos:prefLabel "Footwear Making"@en ;
    skos:scopeNote "Exclusions: Footwear design. This is included in Detailed Field 100599 Graphic and Design, n.e.c." .

asced:030111 a skos:Concept ;
    dcterms:created "2025-08-01T01:49:07.968000+00:00"^^xsd:dateTime ;
    dcterms:modified "2025-08-05T22:47:58.918000+00:00"^^xsd:dateTime ;
    skos:broader asced:0301 ;
    skos:definition "Wood Machining and Turning is the study of shaping wood using various machines." ;
    skos:example "lathe, saw, plane and router maintenance and operation, template and jig design and construction, sawing, planing, shaping, carving and machining wood" ;
    skos:inScheme ascedcs: ;
    skos:notation "030111" ;
    skos:prefLabel "Wood Machining and Turning"@en .

asced:030113 a skos:Concept ;
    dcterms:created "2025-08-01T01:49:07.969000+00:00"^^xsd:dateTime ;
    dcterms:modified "2025-08-05T22:47:58.961000+00:00"^^xsd:dateTime ;
    skos:broader asced:0301 ;
    skos:definition "Cabinet Making is the study of making and repairing furniture and interior fittings for buildings." ;
    skos:example "custom-built furniture, interior fittings and fixtures, furniture, interior fittings and cabinet reparation, furniture and interior fittings material selection" ;
    skos:inScheme ascedcs: ;
    skos:notation "030113" ;
    skos:prefLabel "Cabinet Making"@en .

asced:030115 a skos:Concept ;
    dcterms:created "2025-08-01T01:49:07.970000+00:00"^^xsd:dateTime ;
    dcterms:modified "2025-08-05T22:47:59.016000+00:00"^^xsd:dateTime ;
    skos:broader asced:0301 ;
    skos:definition "Furniture Upholstery and Renovation is the study of designing, making and repairing the soft furnishings of chairs, beds and other furniture." ;
    skos:example "padding and furniture coverings, upholstery machining, decorative upholstery accessories" ;
    skos:inScheme ascedcs: ;
    skos:notation "030115" ;
    skos:prefLabel "Furniture Upholstery and Renovation"@en ;
    skos:scopeNote "Exclusions: Vehicle upholstery and trimming. This is included in Detailed Field 030513 Upholstery and Vehicle Trimming." .

asced:030117 a skos:Concept ;
    dcterms:created "2025-08-01T01:49:07.971000+00:00"^^xsd:dateTime ;
    dcterms:modified "2025-08-05T22:47:59.068000+00:00"^^xsd:dateTime ;
    skos:broader asced:0301 ;
    skos:definition "Furniture Polishing is the study of preparing and polishing different timber furniture surfaces." ;
    skos:example "French polishing, furniture stripping and mechanical buffing, wood staining, lacquering and bleaching" ;
    skos:inScheme ascedcs: ;
    skos:notation "030117" ;
    skos:prefLabel "Furniture Polishing"@en .

asced:030199 a skos:Concept ;
    dcterms:created "2025-08-01T01:49:07.972000+00:00"^^xsd:dateTime ;
    dcterms:modified "2025-08-05T22:47:59.117000+00:00"^^xsd:dateTime ;
    skos:broader asced:0301 ;
    skos:definition "This detailed field includes all Manufacturing Engineering and Technology not elsewhere classified." ;
    skos:example "coopering, leatherwork, furriery, picture framing, curtain and blind making" ;
    skos:inScheme ascedcs: ;
    skos:notation "030199" ;
    skos:prefLabel "Manufacturing Engineering and Technology, n.e.c."@en .

asced:030301 a skos:Concept ;
    dcterms:created "2025-08-01T01:49:07.974000+00:00"^^xsd:dateTime ;
    dcterms:modified "2025-08-05T22:47:59.164000+00:00"^^xsd:dateTime ;
    skos:broader asced:0303 ;
    skos:definition "Chemical Engineering is the study of planning, designing and developing products and processes where chemical and physical changes occur." ;
    skos:example "process control optimisation and simulation, laws of physical chemistry in chemical engineering, biochemical engineering, process plant design, petrochemical product development, petroleum refining" ;
    skos:inScheme ascedcs: ;
    skos:notation "030301" ;
    skos:prefLabel "Chemical Engineering"@en .

asced:030303 a skos:Concept ;
    dcterms:created "2025-08-01T01:49:07.975000+00:00"^^xsd:dateTime ;
    dcterms:modified "2025-08-05T22:47:59.203000+00:00"^^xsd:dateTime ;
    skos:broader asced:0303 ;
    skos:definition "Mining Engineering is the study of planning, developing, assessing, directing and managing the extraction of minerals, oil and gas from the earth." ;
    skos:example "economic feasibility of mining mineral deposits, mine design and construction, gas and oil extraction methods, mine safety" ;
    skos:inScheme ascedcs: ;
    skos:notation "030303" ;
    skos:prefLabel "Mining Engineering"@en ;
    skos:scopeNote "Exclusions: Mining surveying. This is included in Detailed Field 031101 Surveying." .

asced:030305 a skos:Concept ;
    dcterms:created "2025-08-01T01:49:07.975000+00:00"^^xsd:dateTime ;
    dcterms:modified "2025-08-05T22:47:59.261000+00:00"^^xsd:dateTime ;
    skos:broader asced:0303 ;
    skos:definition "Materials Engineering is the study of assaying, producing and refining materials, including metals, alloys, ceramics and polymers, timber, pulp and paper." ;
    skos:example "composite materials analysis, papermaking technology, materials production and processing techniques, drying, treating and grading timber, materials testing, metallurgy" ;
    skos:inScheme ascedcs: ;
    skos:notation "030305" ;
    skos:prefLabel "Materials Engineering"@en .

asced:030307 a skos:Concept ;
    dcterms:created "2025-08-01T01:49:07.976000+00:00"^^xsd:dateTime ;
    dcterms:modified "2025-08-05T22:47:59.308000+00:00"^^xsd:dateTime ;
    skos:broader asced:0303 ;
    skos:definition "Food Processing Technology is the study of the industrial processing, packaging and handling of food." ;
    skos:example "smallgoods manufacturing, fruit and vegetables, sugars and cereal product processing, food packaging and storage principles, dairy products manufacturing, seafood processing, meat inspection" ;
    skos:inScheme ascedcs: ;
    skos:notation "030307" ;
    skos:prefLabel "Food Processing Technology"@en ;
    skos:scopeNote "Exclusions: Butchery. This is included in Detailed Field 110105 Butchery. Food science. This is included in Detailed Field 019905 Food Science and Biotechnology. Wine making. This is included in Detailed Field 019905 Food Science and Biotechnology." .

asced:030399 a skos:Concept ;
    dcterms:created "2025-08-01T01:49:07.977000+00:00"^^xsd:dateTime ;
    dcterms:modified "2025-08-05T22:47:59.363000+00:00"^^xsd:dateTime ;
    skos:broader asced:0303 ;
    skos:definition "This detailed field includes all Process and Resources Engineering not elsewhere classified." ;
    skos:example "fuel technology, pharmaceutical manufacturing" ;
    skos:inScheme ascedcs: ;
    skos:notation "030399" ;
    skos:prefLabel "Process and Resources Engineering, n.e.c."@en .

asced:030501 a skos:Concept ;
    dcterms:created "2025-08-01T01:49:07.979000+00:00"^^xsd:dateTime ;
    dcterms:modified "2025-08-05T22:47:59.409000+00:00"^^xsd:dateTime ;
    skos:broader asced:0305 ;
    skos:definition "Automotive Engineering is the study of designing, developing and testing motor vehicles, earth moving equipment, small engines and their components." ;
    skos:example "engineering mathematics and science in automotive practices, motor vehicle components and design standards, vehicle performance and safety testing and evaluation" ;
    skos:inScheme ascedcs: ;
    skos:notation "030501" ;
    skos:prefLabel "Automotive Engineering"@en .

asced:030503 a skos:Concept ;
    dcterms:created "2025-08-01T01:49:07.980000+00:00"^^xsd:dateTime ;
    dcterms:modified "2025-08-05T22:47:59.456000+00:00"^^xsd:dateTime ;
    skos:broader asced:0305 ;
    skos:definition "Vehicle Mechanics is the study of maintaining, diagnosing faults in, repairing and servicing motor vehicles and their components and small engines in boats, motorcycles, lawnmowers, generators and related equipment." ;
    skos:example "automotive fitting and turning, exhaust emission control systems, tuning engines, automotive air conditioning, suspension, steering and brake systems, tyre fitting and wheel alignments" ;
    skos:inScheme ascedcs: ;
    skos:notation "030503" ;
    skos:prefLabel "Vehicle Mechanics"@en .

asced:030505 a skos:Concept ;
    dcterms:created "2025-08-01T01:49:07.981000+00:00"^^xsd:dateTime ;
    dcterms:modified "2025-08-05T22:47:59.506000+00:00"^^xsd:dateTime ;
    skos:broader asced:0305 ;
    skos:definition "Automotive Electrics and Electronics is the study of installing, maintaining and repairing electrical wiring and electronic components in motor vehicles, boats and earth moving equipment." ;
    skos:example "engine control systems and timing adjustment, electrical and electronic equipment installation and repair, automotive security systems and other electronic accessories, electrical and electronic malfunction detection techniques, batteries and charging principles, vehicle lighting systems" ;
    skos:inScheme ascedcs: ;
    skos:notation "030505" ;
    skos:prefLabel "Automotive Electrics and Electronics"@en .

asced:030507 a skos:Concept ;
    dcterms:created "2025-08-01T01:49:07.982000+00:00"^^xsd:dateTime ;
    dcterms:modified "2025-08-05T22:47:59.554000+00:00"^^xsd:dateTime ;
    skos:broader asced:0305 ;
    skos:definition "Automotive Vehicle Refinishing is the study of preparing vehicle surfaces, mixing and matching paint colours, spray painting and detailing motor vehicles and aircraft." ;
    skos:example "metallic and non-metallic paint technology, protective mouldings, transfers and stet, anti-corrosion treatment, painted and unpainted surface preparation, spraying techniques, spot repairs (major and minor)" ;
    skos:inScheme ascedcs: ;
    skos:notation "030507" ;
    skos:prefLabel "Automotive Vehicle Refinishing"@en .

asced:030509 a skos:Concept ;
    dcterms:created "2025-08-01T01:49:07.982000+00:00"^^xsd:dateTime ;
    dcterms:modified "2025-08-05T22:47:59.600000+00:00"^^xsd:dateTime ;
    skos:broader asced:0305 ;
    skos:definition "Automotive Body Construction is the study of building bodies for motor vehicles, trailers, buses, and railway rolling stock." ;
    skos:example "body structure, framework construction techniques, attaching panels to frameworks" ;
    skos:inScheme ascedcs: ;
    skos:notation "030509" ;
    skos:prefLabel "Automotive Body Construction"@en ;
    skos:scopeNote "Exclusions: Aircraft body construction. This is included in Detailed Field 031503 Aircraft Maintenance Engineering." .

asced:030511 a skos:Concept ;
    dcterms:created "2025-08-01T01:49:07.983000+00:00"^^xsd:dateTime ;
    dcterms:modified "2025-08-05T22:47:59.654000+00:00"^^xsd:dateTime ;
    skos:broader asced:0305 ;
    skos:definition "Panel Beating is the study of repairing damaged motor vehicle bodies and replacing panels." ;
    skos:example "damage and cost assessment, panelbeating equipment, panel section replacement, forming custom panels" ;
    skos:inScheme ascedcs: ;
    skos:notation "030511" ;
    skos:prefLabel "Panel Beating"@en ;
    skos:scopeNote "Exclusions: Windscreen glazing. This is included in Detailed Field 040323 Glazing." .

asced:030513 a skos:Concept ;
    dcterms:created "2025-08-01T01:49:07.984000+00:00"^^xsd:dateTime ;
    dcterms:modified "2025-08-05T22:47:59.712000+00:00"^^xsd:dateTime ;
    skos:broader asced:0305 ;
    skos:definition "Upholstery and Vehicle Trimming is the study of making, installing, repairing and replacing the interior trimmings and upholstery of motor vehicles, boats, aircraft and railway carriages." ;
    skos:example "vehicle trimming principles, seat cover repairs and manufacture, canopy, tonneau covers, seat and squab production" ;
    skos:inScheme ascedcs: ;
    skos:notation "030513" ;
    skos:prefLabel "Upholstery and Vehicle Trimming"@en .

asced:030515 a skos:Concept ;
    dcterms:created "2025-08-01T01:49:07.985000+00:00"^^xsd:dateTime ;
    dcterms:modified "2025-08-05T22:47:59.768000+00:00"^^xsd:dateTime ;
    skos:broader asced:0305 ;
    skos:definition "Automotive Vehicle Operations is the study of driving motor vehicles including motor cycles, trucks and buses." ;
    skos:example "advanced driver training, motor vehicle handling, road rules and defensive driving techniques" ;
    skos:inScheme ascedcs: ;
    skos:notation "030515" ;
    skos:prefLabel "Automotive Vehicle Operations"@en ;
    skos:scopeNote "Exclusions: Driving instructor training. This is included in Detailed Field 079999 Education, n.e.c." .

asced:030599 a skos:Concept ;
    dcterms:created "2025-08-01T01:49:07.986000+00:00"^^xsd:dateTime ;
    dcterms:modified "2025-08-05T22:47:59.821000+00:00"^^xsd:dateTime ;
    skos:broader asced:0305 ;
    skos:definition "This detailed field includes all Automotive Engineering and Technology not elsewhere classified." ;
    skos:example "manufacturing and repairing bicycles, automotive parts interpreting" ;
    skos:inScheme ascedcs: ;
    skos:notation "030599" ;
    skos:prefLabel "Automotive Engineering and Technology, n.e.c."@en .

asced:030701 a skos:Concept ;
    dcterms:created "2025-08-01T01:49:07.988000+00:00"^^xsd:dateTime ;
    dcterms:modified "2025-08-05T22:47:59.864000+00:00"^^xsd:dateTime ;
    skos:broader asced:0307 ;
    skos:definition "Mechanical Engineering is the study of planning, designing and developing machines, mechanical plant and systems." ;
    skos:example "machinery, plant and equipment stress and strain analysis, mechanical systems and component design, maintenance of mechanical systems, lubrication, friction and wear" ;
    skos:inScheme ascedcs: ;
    skos:notation "030701" ;
    skos:prefLabel "Mechanical Engineering"@en .

asced:030703 a skos:Concept ;
    dcterms:created "2025-08-01T01:49:07.988000+00:00"^^xsd:dateTime ;
    dcterms:modified "2025-08-05T22:47:59.907000+00:00"^^xsd:dateTime ;
    skos:broader asced:0307 ;
    skos:definition "Industrial Engineering is the study of planning, designing, organising and operating industrial facilities and processes for the economic, safe and effective use of physical and human resources." ;
    skos:example "control system design, industrial plant design, methods engineering" ;
    skos:inScheme ascedcs: ;
    skos:notation "030703" ;
    skos:prefLabel "Industrial Engineering"@en .

asced:030705 a skos:Concept ;
    dcterms:created "2025-08-01T01:49:07.989000+00:00"^^xsd:dateTime ;
    dcterms:modified "2025-08-05T22:47:59.952000+00:00"^^xsd:dateTime ;
    skos:broader asced:0307 ;
    skos:definition "Toolmaking is the study of making and repairing tools, dies, jigs, fixtures and other precision parts and equipment." ;
    skos:example "precision toolmaking tools operation, tool dimensions and tolerances, metals, alloys and plastics in toolmaking" ;
    skos:inScheme ascedcs: ;
    skos:notation "030705" ;
    skos:prefLabel "Toolmaking"@en .

asced:030707 a skos:Concept ;
    dcterms:created "2025-08-01T01:49:07.990000+00:00"^^xsd:dateTime ;
    dcterms:modified "2025-08-05T22:47:59.995000+00:00"^^xsd:dateTime ;
    skos:broader asced:0307 ;
    skos:definition "Metal Fitting, Turning and Machining is the study of setting up machining tools, production machines and textile machines, operating machining tools and machines to shape metal stock and castings, and fitting and assembling the fabricated metal parts into products." ;
    skos:example "fabricated metal parts fitting and assembling, turning, gearcutting, milling and computer controlled machining, shaping metal stocks" ;
    skos:inScheme ascedcs: ;
    skos:notation "030707" ;
    skos:prefLabel "Metal Fitting, Turning and Machining"@en .

asced:030709 a skos:Concept ;
    dcterms:created "2025-08-01T01:49:07.991000+00:00"^^xsd:dateTime ;
    dcterms:modified "2025-08-05T22:48:00.039000+00:00"^^xsd:dateTime ;
    skos:broader asced:0307 ;
    skos:definition "Sheetmetal Working is the study of cutting, shaping and joining sheetmetal and other materials, and using hand tools, power tools and machines to make products and components." ;
    skos:example "sheetmetal products construction, stock marking techniques, metal spinning" ;
    skos:inScheme ascedcs: ;
    skos:notation "030709" ;
    skos:prefLabel "Sheetmetal Working"@en .

asced:030711 a skos:Concept ;
    dcterms:created "2025-08-01T01:49:07.991000+00:00"^^xsd:dateTime ;
    dcterms:modified "2025-08-05T22:48:00.083000+00:00"^^xsd:dateTime ;
    skos:broader asced:0307 ;
    skos:definition "Boilermaking and Welding is the study of marking out, cutting, shaping and joining metals, and constructing and repairing steelwork structures and pressure vessels including boilers, piping systems and ships." ;
    skos:example "welding and thermal cutting, weld smoothing, weld testing, metal welding techniques, metal section and pipe shaping" ;
    skos:inScheme ascedcs: ;
    skos:notation "030711" ;
    skos:prefLabel "Boilermaking and Welding"@en .

asced:030713 a skos:Concept ;
    dcterms:created "2025-08-01T01:49:07.992000+00:00"^^xsd:dateTime ;
    dcterms:modified "2025-08-05T22:48:00.125000+00:00"^^xsd:dateTime ;
    skos:broader asced:0307 ;
    skos:definition "Metal Casting and Patternmaking is the study of planning and fabricating mould patterns and cores for the production of metal castings." ;
    skos:example "metallic and non-metallic pattern, mould and core design and fabrication, metal moulding and casting techniques, ferrous and non-ferrous alloy moulding, coremaking and casting" ;
    skos:inScheme ascedcs: ;
    skos:notation "030713" ;
    skos:prefLabel "Metal Casting and Patternmaking"@en .

asced:030715 a skos:Concept ;
    dcterms:created "2025-08-01T01:49:07.993000+00:00"^^xsd:dateTime ;
    dcterms:modified "2025-08-05T22:48:00.166000+00:00"^^xsd:dateTime ;
    skos:broader asced:0307 ;
    skos:definition "Precision Metalworking is the study of designing, fabricating, assembling, maintaining and repairing precision instruments such as locks, timepieces and firearms." ;
    skos:example "precision instrument assembly, dismantling and repair, calibration, fine metal work and ornamental inscription engraving, saw blade construction and repair" ;
    skos:inScheme ascedcs: ;
    skos:notation "030715" ;
    skos:prefLabel "Precision Metalworking"@en .

asced:030717 a skos:Concept ;
    dcterms:created "2025-08-01T01:49:07.995000+00:00"^^xsd:dateTime ;
    dcterms:modified "2025-08-05T22:48:00.209000+00:00"^^xsd:dateTime ;
    skos:broader asced:0307 ;
    skos:definition "Plant and Machine Operations is the study of setting up, controlling and monitoring mobile and stationary plant, equipment and machinery either directly or by remote control." ;
    skos:example "equipment cleaning, lubricating and maintenance, forklift, tractor, front-end loader and crane operation, equipment safety and efficiency monitoring, pre-start-up inspection" ;
    skos:inScheme ascedcs: ;
    skos:notation "030717" ;
    skos:prefLabel "Plant and Machine Operations"@en .

asced:030799 a skos:Concept ;
    dcterms:created "2025-08-01T01:49:07.995000+00:00"^^xsd:dateTime ;
    dcterms:modified "2025-08-05T22:48:00.250000+00:00"^^xsd:dateTime ;
    skos:broader asced:0307 ;
    skos:definition "This detailed field includes all Mechanical and Industrial Engineering and Technology not elsewhere classified." ;
    skos:example "farriery, armament fitting, blacksmithing" ;
    skos:inScheme ascedcs: ;
    skos:notation "030799" ;
    skos:prefLabel "Mechanical and Industrial Engineering and Technology, n.e.c."@en .

asced:030901 a skos:Concept ;
    dcterms:created "2025-08-01T01:49:07.997000+00:00"^^xsd:dateTime ;
    dcterms:modified "2025-08-05T22:48:00.291000+00:00"^^xsd:dateTime ;
    skos:broader asced:0309 ;
    skos:definition "Construction Engineering is the study of designing and developing infrastructure such as buildings, roads, bridges, tunnels and quarries." ;
    skos:example "airport engineering, roads and bridges, underground construction and tunnelling" ;
    skos:inScheme ascedcs: ;
    skos:notation "030901" ;
    skos:prefLabel "Construction Engineering"@en ;
    skos:scopeNote "Exclusions: Mine construction. This is included in Detailed Field 030303 Mining Engineering." .

asced:030903 a skos:Concept ;
    dcterms:created "2025-08-01T01:49:07.998000+00:00"^^xsd:dateTime ;
    dcterms:modified "2025-08-05T22:48:00.329000+00:00"^^xsd:dateTime ;
    skos:broader asced:0309 ;
    skos:definition "Structural Engineering is the study of the statical properties of structures and the behaviour and durability of materials used for erecting structures." ;
    skos:example "structural systems strength, serviceability and durability, material behaviour, solid mechanics, structural erection techniques, structural loading" ;
    skos:inScheme ascedcs: ;
    skos:notation "030903" ;
    skos:prefLabel "Structural Engineering"@en .

asced:030905 a skos:Concept ;
    dcterms:created "2025-08-01T01:49:07.998000+00:00"^^xsd:dateTime ;
    dcterms:modified "2025-08-05T22:48:00.373000+00:00"^^xsd:dateTime ;
    skos:broader asced:0309 ;
    skos:definition "Building Services Engineering is the study of designing and developing infrastructure aimed at enhancing human comfort through controlling heat, light and sound in built environments." ;
    skos:example "secure access systems, building fire detection and suppression systems, thermal, visual and acoustical environment in buildings, building mechanical services, building electrical services, energy efficient buildings" ;
    skos:inScheme ascedcs: ;
    skos:notation "030905" ;
    skos:prefLabel "Building Services Engineering"@en ;
    skos:scopeNote "Exclusions: Refrigeration and air-conditioning repair. This is included in Detailed Field 031315 Refrigeration and Air Conditioning Mechanics." .

asced:030907 a skos:Concept ;
    dcterms:created "2025-08-01T01:49:07.999000+00:00"^^xsd:dateTime ;
    dcterms:modified "2025-08-05T22:48:00.415000+00:00"^^xsd:dateTime ;
    skos:broader asced:0309 ;
    skos:definition "Water and Sanitary Engineering is the study of designing and developing water storage and distribution systems, and sludge, effluent and waste water treatment systems." ;
    skos:example "on-site waste water treatment, pond and lagoon systems, primary, secondary and tertiary municipal waste water treatments" ;
    skos:inScheme ascedcs: ;
    skos:notation "030907" ;
    skos:prefLabel "Water and Sanitary Engineering"@en .

asced:030909 a skos:Concept ;
    dcterms:created "2025-08-01T01:49:08.001000+00:00"^^xsd:dateTime ;
    dcterms:modified "2025-08-05T22:48:00.455000+00:00"^^xsd:dateTime ;
    skos:broader asced:0309 ;
    skos:definition "Transport Engineering is the study of planning and developing efficient transport systems." ;
    skos:example "transport network systems evaluation, transport facilities planning, design and operation, public transport systems, traffic operations and control, traffic studies" ;
    skos:inScheme ascedcs: ;
    skos:notation "030909" ;
    skos:prefLabel "Transport Engineering"@en ;
    skos:scopeNote "Exclusions: Air traffic control. This is included in Detailed Field 031507 Air Traffic Control." .

asced:030911 a skos:Concept ;
    dcterms:created "2025-08-01T01:49:08.002000+00:00"^^xsd:dateTime ;
    dcterms:modified "2025-08-05T22:48:00.498000+00:00"^^xsd:dateTime ;
    skos:broader asced:0309 ;
    skos:definition "Geotechnical Engineering is the study of analysing foundations, slopes and soil mechanics, and designing foundations." ;
    skos:example "earth and rock slope analysis, failure in soil, geotechnical investigations and orientation, geotechnical practical skills, managing earth pressure in engineering projects" ;
    skos:inScheme ascedcs: ;
    skos:notation "030911" ;
    skos:prefLabel "Geotechnical Engineering"@en .

asced:030913 a skos:Concept ;
    dcterms:created "2025-08-01T01:49:08.002000+00:00"^^xsd:dateTime ;
    dcterms:modified "2025-08-05T22:48:00.541000+00:00"^^xsd:dateTime ;
    skos:broader asced:0309 ;
    skos:definition "Ocean Engineering is the study of designing, constructing and maintaining coastal and ocean related projects and facilities, and designing floating, fixed and sub-sea offshore systems." ;
    skos:example "buoy engineering, coastal engineering, floating and compliant platforms, semi-submersibles" ;
    skos:inScheme ascedcs: ;
    skos:notation "030913" ;
    skos:prefLabel "Ocean Engineering"@en .

asced:030999 a skos:Concept ;
    dcterms:created "2025-08-01T01:49:08.003000+00:00"^^xsd:dateTime ;
    dcterms:modified "2025-08-05T22:48:00.582000+00:00"^^xsd:dateTime ;
    skos:broader asced:0309 ;
    skos:definition "This detailed field includes all Civil Engineering not elsewhere classified." ;
    skos:example "hydraulic engineering" ;
    skos:inScheme ascedcs: ;
    skos:notation "030999" ;
    skos:prefLabel "Civil Engineering, n.e.c."@en .

asced:031101 a skos:Concept ;
    dcterms:created "2025-08-01T01:49:08.004000+00:00"^^xsd:dateTime ;
    dcterms:modified "2025-08-05T22:48:00.628000+00:00"^^xsd:dateTime ;
    skos:broader asced:0311 ;
    skos:definition "Surveying is the study of measuring and representing the shape, contours, locations and dimensions of the constructed and natural features of the earth, in the form of reports and plans." ;
    skos:example "survey plans preparation, survey statistics and adjustments, land information plans and reports, surveying mines, geodesy, survey data presentation" ;
    skos:inScheme ascedcs: ;
    skos:notation "031101" ;
    skos:prefLabel "Surveying"@en ;
    skos:scopeNote "Exclusions: Surveying of mineral deposits. This is included in Detailed Field 010705 Geophysics. Building surveying. This is included in Detailed Field 040305 Building Surveying. Quantity surveying. This is included in Detailed Field 040307 Building Construction Economics." .

asced:031103 a skos:Concept ;
    dcterms:created "2025-08-01T01:49:08.007000+00:00"^^xsd:dateTime ;
    dcterms:modified "2025-08-05T22:48:00.669000+00:00"^^xsd:dateTime ;
    skos:broader asced:0311 ;
    skos:definition "Mapping Science is the study of graphically representing the constructed and natural features of the earth in the form of maps." ;
    skos:example "graphic communication techniques in map production, cartography, hydrography, map and chart development and revision" ;
    skos:inScheme ascedcs: ;
    skos:notation "031103" ;
    skos:prefLabel "Mapping Science"@en .

asced:031199 a skos:Concept ;
    dcterms:created "2025-08-01T01:49:08.007000+00:00"^^xsd:dateTime ;
    dcterms:modified "2025-08-05T22:48:00.707000+00:00"^^xsd:dateTime ;
    skos:broader asced:0311 ;
    skos:definition "This detailed field includes all Geomatic Engineering not elsewhere classified." ;
    skos:example "geographical information systems (GIS), land information systems (LIS), photogrammetry, remote sensing, spatial information systems (SIS)" ;
    skos:inScheme ascedcs: ;
    skos:notation "031199" ;
    skos:prefLabel "Geomatic Engineering, n.e.c."@en .

asced:031301 a skos:Concept ;
    dcterms:created "2025-08-01T01:49:08.009000+00:00"^^xsd:dateTime ;
    dcterms:modified "2025-08-05T22:48:00.744000+00:00"^^xsd:dateTime ;
    skos:broader asced:0313 ;
    skos:definition "Electrical Engineering is the study of planning, designing, developing and maintaining electrical equipment, circuits and systems." ;
    skos:example "analogue systems, electronic components and systems design, operational amplifiers, integrated circuit design" ;
    skos:inScheme ascedcs: ;
    skos:notation "031301" ;
    skos:prefLabel "Electrical Engineering"@en ;
    skos:scopeNote "Electronic Engineering is the study of planning, designing, developing and maintaining electronic equipment, machinery and systems." .

asced:031303 a skos:Concept ;
    dcterms:created "2025-08-01T01:49:08.010000+00:00"^^xsd:dateTime ;
    dcterms:modified "2025-08-05T22:48:00.838000+00:00"^^xsd:dateTime ;
    skos:broader asced:0313 ;
    skos:inScheme ascedcs: ;
    skos:notation "031303" ;
    skos:prefLabel "Electronic Engineering"@en .

asced:031305 a skos:Concept ;
    dcterms:created "2025-08-01T01:49:08.011000+00:00"^^xsd:dateTime ;
    dcterms:modified "2025-08-05T22:48:00.894000+00:00"^^xsd:dateTime ;
    skos:broader asced:0313 ;
    skos:definition "Computer Engineering is the study of designing and constructing digital data processing hardware." ;
    skos:example "arithmetic and logic structures, computer architecture, computer hardware design and construction, computer systems engineering, input, output and data devices, logic design" ;
    skos:inScheme ascedcs: ;
    skos:notation "031305" ;
    skos:prefLabel "Computer Engineering"@en .

asced:031307 a skos:Concept ;
    dcterms:created "2025-08-01T01:49:08.011000+00:00"^^xsd:dateTime ;
    dcterms:modified "2025-08-05T22:48:00.946000+00:00"^^xsd:dateTime ;
    skos:broader asced:0313 ;
    skos:definition "Communications Technologies is the study of communication transmission and signal systems." ;
    skos:example "antenna technology, broadband network technology, digital and microwave communication systems, fibre optic and photonic communication systems, modem technology, satellite communication systems" ;
    skos:inScheme ascedcs: ;
    skos:notation "031307" ;
    skos:prefLabel "Communications Technologies"@en .

asced:031309 a skos:Concept ;
    dcterms:created "2025-08-01T01:49:08.012000+00:00"^^xsd:dateTime ;
    dcterms:modified "2025-08-05T22:48:00.994000+00:00"^^xsd:dateTime ;
    skos:broader asced:0313 ;
    skos:definition "Communications Equipment Installation and Maintenance is the study of installing, maintaining, operating, diagnosing and repairing faults in telecommunications equipment, appliances, instruments and systems." ;
    skos:example "telephone, radio and computer transmission equipment, underground communications cabling, broadcast station equipment operation, fibre-optic cable jointing" ;
    skos:inScheme ascedcs: ;
    skos:notation "031309" ;
    skos:prefLabel "Communications Equipment Installation and Maintenance"@en .

asced:031311 a skos:Concept ;
    dcterms:created "2025-08-01T01:49:08.013000+00:00"^^xsd:dateTime ;
    dcterms:modified "2025-08-05T22:48:01.043000+00:00"^^xsd:dateTime ;
    skos:broader asced:0313 ;
    skos:definition "Powerline Installation and Maintenance is the study of installing, repairing, maintaining and monitoring overhead and underground electrical power distribution networks." ;
    skos:example "overhead and underground electric powerlines and aerial equipment, powerline fault finding, powerline quality and performance testing, powerline insulation" ;
    skos:inScheme ascedcs: ;
    skos:notation "031311" ;
    skos:prefLabel "Powerline Installation and Maintenance"@en .

asced:031313 a skos:Concept ;
    dcterms:created "2025-08-01T01:49:08.013000+00:00"^^xsd:dateTime ;
    dcterms:modified "2025-08-05T22:48:01.099000+00:00"^^xsd:dateTime ;
    skos:broader asced:0313 ;
    skos:definition "Electrical Fitting, Electrical Mechanics is the study of installing, maintaining, diagnosing faults in and repairing electrical wiring and equipment in domestic, commercial and industrial establishments, ships and trains." ;
    skos:example "electrical wiring installations, electrical units fault finding and repair, electrical circuits compatibility and safety testing, electrical drawing interpretation" ;
    skos:inScheme ascedcs: ;
    skos:notation "031313" ;
    skos:prefLabel "Electrical Fitting, Electrical Mechanics"@en .

asced:031315 a skos:Concept ;
    dcterms:created "2025-08-01T01:49:08.014000+00:00"^^xsd:dateTime ;
    dcterms:modified "2025-08-05T22:48:01.148000+00:00"^^xsd:dateTime ;
    skos:broader asced:0313 ;
    skos:definition "Refrigeration and Air Conditioning Mechanics is the study of installing, maintaining, diagnosing faults in and repairing domestic, commercial and industrial refrigeration, air conditioning and heating equipment." ;
    skos:example "refrigerants, refrigeration, air conditioning and heating equipment repair, refrigeration systems analysis, ventilation" ;
    skos:inScheme ascedcs: ;
    skos:notation "031315" ;
    skos:prefLabel "Refrigeration and Air Conditioning Mechanics"@en ;
    skos:scopeNote "Exclusions: Air conditioning and heating system design. This is included in Detailed Field 030905 Building Services Engineering. Automotive air conditioning. This is included in Detailed Field 030503 Vehicle Mechanics." .

asced:031317 a skos:Concept ;
    dcterms:created "2025-08-01T01:49:08.015000+00:00"^^xsd:dateTime ;
    dcterms:modified "2025-08-05T22:48:01.197000+00:00"^^xsd:dateTime ;
    skos:broader asced:0313 ;
    skos:definition "Electronic Equipment Servicing is the study of maintaining, diagnosing faults in and repairing computers, radio and television receivers, audio, video, and other electronic business and domestic equipment." ;
    skos:example "electronic wiring and equipment testing, electronic equipment installation, electronic mechanics, cromiance and luminance, filters and resonance, PC configuration" ;
    skos:inScheme ascedcs: ;
    skos:notation "031317" ;
    skos:prefLabel "Electronic Equipment Servicing"@en .

asced:031399 a skos:Concept ;
    dcterms:created "2025-08-01T01:49:08.016000+00:00"^^xsd:dateTime ;
    dcterms:modified "2025-08-05T22:48:01.239000+00:00"^^xsd:dateTime ;
    skos:broader asced:0313 ;
    skos:definition "This detailed field includes all Electrical and Electronic Engineering and Technology not elsewhere classified." ;
    skos:example "renewable energy technology" ;
    skos:inScheme ascedcs: ;
    skos:notation "031399" ;
    skos:prefLabel "Electrical and Electronic Engineering and Technology, n.e.c."@en .

asced:031501 a skos:Concept ;
    dcterms:created "2025-08-01T01:49:08.017000+00:00"^^xsd:dateTime ;
    dcterms:modified "2025-08-05T22:48:01.283000+00:00"^^xsd:dateTime ;
    skos:broader asced:0315 ;
    skos:definition "Aerospace Engineering is the study of designing, developing and modifying aircraft." ;
    skos:example "aerodynamics, airframes engineering, missile design, propulsion, satellite design, spacecraft design" ;
    skos:inScheme ascedcs: ;
    skos:notation "031501" ;
    skos:prefLabel "Aerospace Engineering"@en .

asced:031503 a skos:Concept ;
    dcterms:created "2025-08-01T01:49:08.019000+00:00"^^xsd:dateTime ;
    dcterms:modified "2025-08-05T22:48:01.345000+00:00"^^xsd:dateTime ;
    skos:broader asced:0315 ;
    skos:definition "Aircraft Maintenance Engineering is the study of assembling, maintaining and repairing aircraft structures, and avionic and mechanical systems." ;
    skos:example "aircraft auxiliary systems, propellers and propeller systems, aircraft instrument systems, aircraft fabrication techniques, aerodynamics and structural repairs" ;
    skos:inScheme ascedcs: ;
    skos:notation "031503" ;
    skos:prefLabel "Aircraft Maintenance Engineering"@en .

asced:031505 a skos:Concept ;
    dcterms:created "2025-08-01T01:49:08.019000+00:00"^^xsd:dateTime ;
    dcterms:modified "2025-08-05T22:48:01.407000+00:00"^^xsd:dateTime ;
    skos:broader asced:0315 ;
    skos:definition "Aircraft Operation is the study of piloting and navigating aircraft." ;
    skos:example "aircraft ground control, take-off and landing procedures, aircraft navigation, aircraft operation and flight procedures, aircraft safety, flight plans preparation" ;
    skos:inScheme ascedcs: ;
    skos:notation "031505" ;
    skos:prefLabel "Aircraft Operation"@en .

asced:031507 a skos:Concept ;
    dcterms:created "2025-08-01T01:49:08.020000+00:00"^^xsd:dateTime ;
    dcterms:modified "2025-08-05T22:48:01.456000+00:00"^^xsd:dateTime ;
    skos:broader asced:0315 ;
    skos:definition "Air Traffic Control is the study of monitoring and directing ground and air aircraft movements." ;
    skos:example "ground control systems, air traffic communications, pilot weather briefing, aircraft plotting, flight and operation recording, flight plans clearance, navigational aids and airports" ;
    skos:inScheme ascedcs: ;
    skos:notation "031507" ;
    skos:prefLabel "Air Traffic Control"@en .

asced:031599 a skos:Concept ;
    dcterms:created "2025-08-01T01:49:08.021000+00:00"^^xsd:dateTime ;
    dcterms:modified "2025-08-05T22:48:01.499000+00:00"^^xsd:dateTime ;
    skos:broader asced:0315 ;
    skos:definition "This detailed field includes all Aerospace Engineering and Technology not elsewhere classified." ;
    skos:inScheme ascedcs: ;
    skos:notation "031599" ;
    skos:prefLabel "Aerospace Engineering and Technology, n.e.c."@en .

asced:031701 a skos:Concept ;
    dcterms:created "2025-08-01T01:49:08.023000+00:00"^^xsd:dateTime ;
    dcterms:modified "2025-08-05T22:48:01.538000+00:00"^^xsd:dateTime ;
    skos:broader asced:0317 ;
    skos:definition "Maritime Engineering is the study of maintaining and operating shipboard machinery and systems." ;
    skos:example "marine machinery and control systems, ship machinery and equipment inspection, marine engineering systems maintenance and operation, marine mechanics, marine auxiliary equipment and systems" ;
    skos:inScheme ascedcs: ;
    skos:notation "031701" ;
    skos:prefLabel "Maritime Engineering"@en .

asced:031703 a skos:Concept ;
    dcterms:created "2025-08-01T01:49:08.024000+00:00"^^xsd:dateTime ;
    dcterms:modified "2025-08-05T22:48:01.581000+00:00"^^xsd:dateTime ;
    skos:broader asced:0317 ;
    skos:definition "Marine Construction is the study of fabricating, fitting out and repairing marine vessels and their structural components." ;
    skos:example "hull form and performance, lofting procedures, masts, frames, decking and fittings installation, slipway operations" ;
    skos:inScheme ascedcs: ;
    skos:notation "031703" ;
    skos:prefLabel "Marine Construction"@en .

asced:031705 a skos:Concept ;
    dcterms:created "2025-08-01T01:49:08.024000+00:00"^^xsd:dateTime ;
    dcterms:modified "2025-08-05T22:48:01.627000+00:00"^^xsd:dateTime ;
    skos:broader asced:0317 ;
    skos:definition "Marine Craft Operation is the study of operating ships and other marine craft and their navigation and communication systems." ;
    skos:example "marine radio communication, navigation and navigational aids, vessel maneuvering, handling and stability, seamanship, shipboard safety, fishing operations" ;
    skos:inScheme ascedcs: ;
    skos:notation "031705" ;
    skos:prefLabel "Marine Craft Operation"@en .

asced:031799 a skos:Concept ;
    dcterms:created "2025-08-01T01:49:08.025000+00:00"^^xsd:dateTime ;
    dcterms:modified "2025-08-05T22:48:01.667000+00:00"^^xsd:dateTime ;
    skos:broader asced:0317 ;
    skos:definition "This detailed field includes all Maritime Engineering and Technology not elsewhere classified." ;
    skos:example "naval architecture" ;
    skos:inScheme ascedcs: ;
    skos:notation "031799" ;
    skos:prefLabel "Maritime Engineering and Technology, n.e.c."@en .

asced:039901 a skos:Concept ;
    dcterms:created "2025-08-01T01:49:08.026000+00:00"^^xsd:dateTime ;
    dcterms:modified "2025-08-05T22:48:01.708000+00:00"^^xsd:dateTime ;
    skos:broader asced:0399 ;
    skos:definition "Environmental Engineering is the study of technology concerned with the mitigation of pollution, contamination and deterioration of the environment." ;
    skos:example "cleaner production, erosion control and land rehabilitation technology, noise control mechanisms in engineering projects, waste minimisation, waste management" ;
    skos:inScheme ascedcs: ;
    skos:notation "039901" ;
    skos:prefLabel "Environmental Engineering"@en ;
    skos:scopeNote "Exclusions: Environmental impact assessment. This is included in Detailed Field 050999 Environmental Studies, n.e.c. Environmental management. This is included in Detailed Field 050901 Lands, Parks and Wildlife Management." .

asced:039903 a skos:Concept ;
    dcterms:created "2025-08-01T01:49:08.027000+00:00"^^xsd:dateTime ;
    dcterms:modified "2025-08-05T22:48:01.753000+00:00"^^xsd:dateTime ;
    skos:broader asced:0399 ;
    skos:definition "Biomedical Engineering is the study of designing and manufacturing medical devices and equipment to assist in overcoming physical disabilities." ;
    skos:example "biocompatibility of intracorporeal and extracorporeal systems, biomaterials, designing imaging systems, human rehabilitation engineering" ;
    skos:inScheme ascedcs: ;
    skos:notation "039903" ;
    skos:prefLabel "Biomedical Engineering"@en ;
    skos:scopeNote "Exclusions: Dental prosthetics. This is included in Detailed Field 060705 Dental Technology. Orthotic and prosthetic patient assessment and prescription of orthoses and prostheses. These are included in Detailed Field 061799 Rehabilitation Therapies, n.e.c." .

asced:039905 a skos:Concept ;
    dcterms:created "2025-08-01T01:49:08.027000+00:00"^^xsd:dateTime ;
    dcterms:modified "2025-08-05T22:48:01.816000+00:00"^^xsd:dateTime ;
    skos:broader asced:0399 ;
    skos:definition "Fire Technology is the study of fire detection, suppression and prevention methods and equipment." ;
    skos:example "fire detection, suppression and prevention, fire fighting equipment and techniques, fire hazards, fire behaviour" ;
    skos:inScheme ascedcs: ;
    skos:notation "039905" ;
    skos:prefLabel "Fire Technology"@en .

asced:039907 a skos:Concept ;
    dcterms:created "2025-08-01T01:49:08.029000+00:00"^^xsd:dateTime ;
    dcterms:modified "2025-08-05T22:48:01.869000+00:00"^^xsd:dateTime ;
    skos:broader asced:0399 ;
    skos:definition "Rail Operations is the study of driving, shunting and marshalling trains." ;
    skos:example "train station operation, track safety, train examination, principles of train management, railway yard operation" ;
    skos:inScheme ascedcs: ;
    skos:notation "039907" ;
    skos:prefLabel "Rail Operations"@en .

asced:039909 a skos:Concept ;
    dcterms:created "2025-08-01T01:49:08.029000+00:00"^^xsd:dateTime ;
    dcterms:modified "2025-08-05T22:48:01.920000+00:00"^^xsd:dateTime ;
    skos:broader asced:0399 ;
    skos:definition "Cleaning is the study of removing dirt and stains from, and maintaining and restoring clothing and fabrics, and domestic, industrial and commercial assets." ;
    skos:example "dry-cleaning, dust reduction, domestic cleaning, laundry machine operation, stains, spillages and grime removal techniques, floor, glass and ceiling wet and dry cleaning" ;
    skos:inScheme ascedcs: ;
    skos:notation "039909" ;
    skos:prefLabel "Cleaning"@en ;
    skos:scopeNote "Exclusions: Education primarily related to occupational health and safety. This is included in Detailed Field 061301 Occupational Health and Safety." .

asced:039999 a skos:Concept ;
    dcterms:created "2025-08-01T01:49:08.030000+00:00"^^xsd:dateTime ;
    dcterms:modified "2025-08-05T22:48:01.970000+00:00"^^xsd:dateTime ;
    skos:broader asced:0399 ;
    skos:definition "This detailed field includes all Engineering and Related Technologies not elsewhere classified." ;
    skos:example "nuclear engineering, railway engineering" ;
    skos:inScheme ascedcs: ;
    skos:notation "039999" ;
    skos:prefLabel "Engineering and Related Technologies, n.e.c."@en .

asced:040101 a skos:Concept ;
    dcterms:created "2025-08-01T01:49:08.032000+00:00"^^xsd:dateTime ;
    dcterms:modified "2025-08-05T22:48:02.151000+00:00"^^xsd:dateTime ;
    skos:broader asced:0401 ;
    skos:definition "Architecture is the study of the art, science and techniques of building design. It includes utilitarian ends, such as the soundness of the structure, the functional and economic efficiency of the building, and aesthetic considerations." ;
    skos:example "architectural construction and structures, architectural rendering techniques, architectural history and theory, architectural design and practice" ;
    skos:inScheme ascedcs: ;
    skos:notation "040101" ;
    skos:prefLabel "Architecture"@en .

asced:040103 a skos:Concept ;
    dcterms:created "2025-08-01T01:49:08.032000+00:00"^^xsd:dateTime ;
    dcterms:modified "2025-08-05T22:48:02.203000+00:00"^^xsd:dateTime ;
    skos:broader asced:0401 ;
    skos:definition "Urban Design and Regional Planning is the study of designing and planning towns and rural communities to meet the needs of the population." ;
    skos:example "community planning, urban and regional planning principles, urban design, land use planning, urban land development, social impact assessment" ;
    skos:inScheme ascedcs: ;
    skos:notation "040103" ;
    skos:prefLabel "Urban Design and Regional Planning"@en .

asced:040105 a skos:Concept ;
    dcterms:created "2025-08-01T01:49:08.033000+00:00"^^xsd:dateTime ;
    dcterms:modified "2025-08-05T22:48:02.252000+00:00"^^xsd:dateTime ;
    skos:broader asced:0401 ;
    skos:definition "Landscape Architecture is the study of planning, designing and installing exterior environments with concern for functionality, practicality and human needs and requirements. It includes the design of parks and gardens integrated with the built environment." ;
    skos:example "landscape design, landscape planning, landscape structures, planting design, urban landscapes" ;
    skos:inScheme ascedcs: ;
    skos:notation "040105" ;
    skos:prefLabel "Landscape Architecture"@en .

asced:040107 a skos:Concept ;
    dcterms:created "2025-08-01T01:49:08.034000+00:00"^^xsd:dateTime ;
    dcterms:modified "2025-08-05T22:48:02.302000+00:00"^^xsd:dateTime ;
    skos:broader asced:0401 ;
    skos:definition "Interior and Environmental Design is the study of planning and designing interior environments of homes, offices, factories and other buildings with concern for functionality, practicality and human needs and requirements." ;
    skos:example "interior building design concepts, user centred design, interior design material technologies" ;
    skos:inScheme ascedcs: ;
    skos:notation "040107" ;
    skos:prefLabel "Interior and Environmental Design"@en ;
    skos:scopeNote "Exclusions: Ergonomics. This is included in Detailed Field 061301 Occupational Health and Safety. Heat, light and sound control. These are included in Detailed Field 030905 Building Services." .

asced:040199 a skos:Concept ;
    dcterms:created "2025-08-01T01:49:08.035000+00:00"^^xsd:dateTime ;
    dcterms:modified "2025-08-05T22:48:02.351000+00:00"^^xsd:dateTime ;
    skos:broader asced:0401 ;
    skos:definition "This detailed field includes all Architecture and Urban Environment not elsewhere classified." ;
    skos:example "building conservation" ;
    skos:inScheme ascedcs: ;
    skos:notation "040199" ;
    skos:prefLabel "Architecture and Urban Environment, n.e.c."@en .

asced:040301 a skos:Concept ;
    dcterms:created "2025-08-01T01:49:08.036000+00:00"^^xsd:dateTime ;
    dcterms:modified "2025-08-05T22:48:02.394000+00:00"^^xsd:dateTime ;
    skos:broader asced:0403 ;
    skos:definition "Building Science and Technology is the study of the theories and techniques required to construct and maintain structures." ;
    skos:example "builders working drawings, building maintenance and refurbishment, facades and partitions" ;
    skos:inScheme ascedcs: ;
    skos:notation "040301" ;
    skos:prefLabel "Building Science and Technology"@en .

asced:040303 a skos:Concept ;
    dcterms:created "2025-08-01T01:49:08.037000+00:00"^^xsd:dateTime ;
    dcterms:modified "2025-08-05T22:48:02.439000+00:00"^^xsd:dateTime ;
    skos:broader asced:0403 ;
    skos:definition "Building Construction Management is the study of planning and controlling building projects." ;
    skos:example "construction planning, construction project control, building site management" ;
    skos:inScheme ascedcs: ;
    skos:notation "040303" ;
    skos:prefLabel "Building Construction Management"@en .

asced:040305 a skos:Concept ;
    dcterms:created "2025-08-01T01:49:08.037000+00:00"^^xsd:dateTime ;
    dcterms:modified "2025-08-05T22:48:02.488000+00:00"^^xsd:dateTime ;
    skos:broader asced:0403 ;
    skos:definition "Building Surveying is the study of assessing the condition of buildings to ensure compliance with plans, specification and regulations and that proper techniques and materials have been used." ;
    skos:example "building assessment, building codes and standards, certification codes and practice" ;
    skos:inScheme ascedcs: ;
    skos:notation "040305" ;
    skos:prefLabel "Building Surveying"@en .

asced:040307 a skos:Concept ;
    dcterms:created "2025-08-01T01:49:08.038000+00:00"^^xsd:dateTime ;
    dcterms:modified "2025-08-05T22:48:02.529000+00:00"^^xsd:dateTime ;
    skos:broader asced:0403 ;
    skos:definition "Building Construction Economics is the study of estimating quantities of materials and total costs involved in building and construction." ;
    skos:example "building project feasibility, building cost estimation, contractual arrangements costings, .quantity surveying" ;
    skos:inScheme ascedcs: ;
    skos:notation "040307" ;
    skos:prefLabel "Building Construction Economics"@en .

asced:040309 a skos:Concept ;
    dcterms:created "2025-08-01T01:49:08.039000+00:00"^^xsd:dateTime ;
    dcterms:modified "2025-08-05T22:48:02.580000+00:00"^^xsd:dateTime ;
    skos:broader asced:0403 ;
    skos:definition "Bricklaying and Stonemasonry is the study of cutting, shaping, laying and joining bricks, stone and building blocks to construct and repair all types of masonry structures." ;
    skos:example "arch construction, bricklaying techniques, glass block construction, stone inscription methods, stone restoration and renovation, stone veneer construction" ;
    skos:inScheme ascedcs: ;
    skos:notation "040309" ;
    skos:prefLabel "Bricklaying and Stonemasonry"@en ;
    skos:scopeNote "Exclusions: Brick paving. This is included in Detailed Field 040399 Building, n.e.c." .

asced:040311 a skos:Concept ;
    dcterms:created "2025-08-01T01:49:08.039000+00:00"^^xsd:dateTime ;
    dcterms:modified "2025-08-05T22:48:02.629000+00:00"^^xsd:dateTime ;
    skos:broader asced:0403 ;
    skos:definition "Carpentry and Joinery is the study of fabricating, assembling, installing, renovating and repairing doors, frames, formwork and other fittings in buildings." ;
    skos:example "formwork, framework and trusses, stair construction, window and door joinery" ;
    skos:inScheme ascedcs: ;
    skos:notation "040311" ;
    skos:prefLabel "Carpentry and Joinery"@en ;
    skos:scopeNote "Exclusions: Furniture construction. This is included in Detailed Field 030113 Cabinet Making." .

asced:040313 a skos:Concept ;
    dcterms:created "2025-08-01T01:49:08.040000+00:00"^^xsd:dateTime ;
    dcterms:modified "2025-08-05T22:48:02.680000+00:00"^^xsd:dateTime ;
    skos:broader asced:0403 ;
    skos:definition "Ceiling, Wall and Floor Fixing is the study of fixing tiles and lining materials to ceilings, walls and floors. It includes fixing cladding materials to external surfaces." ;
    skos:example "tile cutting, tiling wet areas, wall cladding and lining" ;
    skos:inScheme ascedcs: ;
    skos:notation "040313" ;
    skos:prefLabel "Ceiling, Wall and Floor Fixing"@en ;
    skos:scopeNote "Exclusions: Fixing fibrous sheets and applying plaster. These are included in Detailed Field 040317 Plastering. Timber flooring. This is included in Detailed Field 040321 Floor Coverings." .

asced:040315 a skos:Concept ;
    dcterms:created "2025-08-01T01:49:08.041000+00:00"^^xsd:dateTime ;
    dcterms:modified "2025-08-05T22:48:02.730000+00:00"^^xsd:dateTime ;
    skos:broader asced:0403 ;
    skos:definition "Roof Fixing is the study of covering structures with roof tiles, shingles and other materials to form a waterproof surface." ;
    skos:example "roofing claddings, slate, shingle, concrete and metal roof tiles, roof tiling and slating procedures" ;
    skos:inScheme ascedcs: ;
    skos:notation "040315" ;
    skos:prefLabel "Roof Fixing"@en .

asced:040317 a skos:Concept ;
    dcterms:created "2025-08-01T01:49:08.042000+00:00"^^xsd:dateTime ;
    dcterms:modified "2025-08-05T22:48:02.784000+00:00"^^xsd:dateTime ;
    skos:broader asced:0403 ;
    skos:definition "Plastering is the study of fixing fibrous sheets and applying plaster, cement-based and similar materials to ceilings, interior and exterior walls of buildings and the study of making plasterboard and plaster mouldings." ;
    skos:example "decorative plaster finishes, fibrous plasterwork, rendering and moulding" ;
    skos:inScheme ascedcs: ;
    skos:notation "040317" ;
    skos:prefLabel "Plastering"@en .

asced:040319 a skos:Concept ;
    dcterms:created "2025-08-01T01:49:08.042000+00:00"^^xsd:dateTime ;
    dcterms:modified "2025-08-05T22:48:02.832000+00:00"^^xsd:dateTime ;
    skos:broader asced:0403 ;
    skos:definition "Furnishing Installation is the study of measuring and installing curtains, blinds, awnings and other soft furnishings." ;
    skos:example "curtain fitting, awning installation techniques, blinds measurement" ;
    skos:inScheme ascedcs: ;
    skos:notation "040319" ;
    skos:prefLabel "Furnishing Installation"@en .

asced:040321 a skos:Concept ;
    dcterms:created "2025-08-01T01:49:08.043000+00:00"^^xsd:dateTime ;
    dcterms:modified "2025-08-05T22:48:02.885000+00:00"^^xsd:dateTime ;
    skos:broader asced:0403 ;
    skos:definition "Floor Coverings is the study of measuring and laying parquetry, carpet, cork, linoleum, vinyl and other resilient floor coverings." ;
    skos:example "floor covering techniques, carpet layout measuring and marking, parquetry and timber floor surfacing" ;
    skos:inScheme ascedcs: ;
    skos:notation "040321" ;
    skos:prefLabel "Floor Coverings"@en .

asced:040323 a skos:Concept ;
    dcterms:created "2025-08-01T01:49:08.044000+00:00"^^xsd:dateTime ;
    dcterms:modified "2025-08-05T22:48:02.933000+00:00"^^xsd:dateTime ;
    skos:broader asced:0403 ;
    skos:definition "Glazing is the study of installing and maintaining glass panes, mirrors and windscreens." ;
    skos:example "decorative glass finishes, leadlighting and stained glass, silvering, windscreen glazing" ;
    skos:inScheme ascedcs: ;
    skos:notation "040323" ;
    skos:prefLabel "Glazing"@en .

asced:040325 a skos:Concept ;
    dcterms:created "2025-08-01T01:49:08.044000+00:00"^^xsd:dateTime ;
    dcterms:modified "2025-08-05T22:48:02.972000+00:00"^^xsd:dateTime ;
    skos:broader asced:0403 ;
    skos:definition "Painting, Decorating and Sign Writing is the study of applying paint, varnish and paper finishes to decorate and protect interior and exterior surfaces. It includes the study of designing and painting signs." ;
    skos:example "painting and decorating techniques, paint and wallpaper application, sign writing techniques" ;
    skos:inScheme ascedcs: ;
    skos:notation "040325" ;
    skos:prefLabel "Painting, Decorating and Sign Writing"@en ;
    skos:scopeNote "Exclusions: Painting motor vehicles. This is included in Detailed Field 030507 Automotive Vehicle Refinishing." .

asced:040327 a skos:Concept ;
    dcterms:created "2025-08-01T01:49:08.045000+00:00"^^xsd:dateTime ;
    dcterms:modified "2025-08-05T22:48:03.016000+00:00"^^xsd:dateTime ;
    skos:broader asced:0403 ;
    skos:definition "Plumbing is the study of designing, installing, maintaining and repairing pipelines, fixtures, fittings and related equipment for water, steam, gas, sewage and other liquids in residential, public commercial and industrial establishments." ;
    skos:example "gas fitting, fire sprinkler systems, pipe joint techniques and fittings, roof plumbing" ;
    skos:inScheme ascedcs: ;
    skos:notation "040327" ;
    skos:prefLabel "Plumbing"@en .

asced:040329 a skos:Concept ;
    dcterms:created "2025-08-01T01:49:08.046000+00:00"^^xsd:dateTime ;
    dcterms:modified "2025-08-05T22:48:03.058000+00:00"^^xsd:dateTime ;
    skos:broader asced:0403 ;
    skos:definition "Scaffolding and Rigging is the study of erecting and dismantling modular scaffolding and rigging." ;
    skos:example "mast climbers, safety nets and static lines, suspended scaffolds, flying foxes and cableways, natural and synthetic ropes" ;
    skos:inScheme ascedcs: ;
    skos:notation "040329" ;
    skos:prefLabel "Scaffolding and Rigging"@en .

asced:040399 a skos:Concept ;
    dcterms:created "2025-08-01T01:49:08.047000+00:00"^^xsd:dateTime ;
    dcterms:modified "2025-08-05T22:48:03.094000+00:00"^^xsd:dateTime ;
    skos:broader asced:0403 ;
    skos:definition "This detailed field includes all Building not elsewhere classified." ;
    skos:example "dogging, steel fixing, brick paving" ;
    skos:inScheme ascedcs: ;
    skos:notation "040399" ;
    skos:prefLabel "Building, n.e.c."@en .

asced:050101 a skos:Concept ;
    dcterms:created "2025-08-01T01:49:08.049000+00:00"^^xsd:dateTime ;
    dcterms:modified "2025-08-05T22:48:03.461000+00:00"^^xsd:dateTime ;
    skos:broader asced:0501 ;
    skos:definition "Agricultural Science is the study of the non-intensive farming of animals and plants." ;
    skos:example "broadacre production, cropping and grazing systems, dairying, dryland farming systems" ;
    skos:inScheme ascedcs: ;
    skos:notation "050101" ;
    skos:prefLabel "Agricultural Science"@en ;
    skos:scopeNote "Exclusions: Vegetable gardening. This is included in Detailed Field 050301 Horticulture." .

asced:050103 a skos:Concept ;
    dcterms:created "2025-08-01T01:49:08.049000+00:00"^^xsd:dateTime ;
    dcterms:modified "2025-08-05T22:48:03.523000+00:00"^^xsd:dateTime ;
    skos:broader asced:0501 ;
    skos:definition "Wool Science is the study of producing, handling and classing wool and other fleece." ;
    skos:example "fleece characteristics, fleece producing animals, wool identification, classification and handling, greasy wool impurities, shearing" ;
    skos:inScheme ascedcs: ;
    skos:notation "050103" ;
    skos:prefLabel "Wool Science"@en .

asced:050105 a skos:Concept ;
    dcterms:created "2025-08-01T01:49:08.050000+00:00"^^xsd:dateTime ;
    dcterms:modified "2025-08-05T22:48:03.571000+00:00"^^xsd:dateTime ;
    skos:broader asced:0501 ;
    skos:definition "Animal Husbandry is the study of the intensive management of animals, their training, handling, care, breeding and rearing." ;
    skos:example "animal grooming, artificial insemination and other breeding techniques, beekeeping, animal hygiene and nutrition, zookeeping, equine management" ;
    skos:inScheme ascedcs: ;
    skos:notation "050105" ;
    skos:prefLabel "Animal Husbandry"@en .

asced:050199 a skos:Concept ;
    dcterms:created "2025-08-01T01:49:08.051000+00:00"^^xsd:dateTime ;
    dcterms:modified "2025-08-05T22:48:03.619000+00:00"^^xsd:dateTime ;
    skos:broader asced:0501 ;
    skos:definition "This detailed field includes all Agriculture not elsewhere classified." ;
    skos:example "agricultural extension" ;
    skos:inScheme ascedcs: ;
    skos:notation "050199" ;
    skos:prefLabel "Agriculture, n.e.c."@en .

asced:050301 a skos:Concept ;
    dcterms:created "2025-08-01T01:49:08.052000+00:00"^^xsd:dateTime ;
    dcterms:modified "2025-08-05T22:48:03.661000+00:00"^^xsd:dateTime ;
    skos:broader asced:0503 ;
    skos:definition "Horticulture is the study of cultivating, propagating and producing intensively managed crops such as fruits (except grapes), vegetables, flowers, foliage, trees, shrubs and plants." ;
    skos:example "arboriculture, greenkeeping, plant culture and garden maintenance, horticultural nursery practice, plant propagation" ;
    skos:inScheme ascedcs: ;
    skos:notation "050301" ;
    skos:prefLabel "Horticulture"@en ;
    skos:scopeNote "Exclusions: Garden design. This is included in Detailed Field 040105 Landscape Architecture. Viticulture. This is included in Detailed Field 050303 Viticulture." .

asced:050303 a skos:Concept ;
    dcterms:created "2025-08-01T01:49:08.053000+00:00"^^xsd:dateTime ;
    dcterms:modified "2025-08-05T22:48:03.703000+00:00"^^xsd:dateTime ;
    skos:broader asced:0503 ;
    skos:definition "Viticulture is the study of cultivating and managing grapevines." ;
    skos:example "grapevine canopy management, grapevine pruning systems, vineyard establishment, grapevine identification and selection, wine and table grape production" ;
    skos:inScheme ascedcs: ;
    skos:notation "050303" ;
    skos:prefLabel "Viticulture"@en ;
    skos:scopeNote "Exclusions: Wine science. This is included in Detailed Field 019905 Food Science and Biotechnology." .

asced:050501 a skos:Concept ;
    dcterms:created "2025-08-01T01:49:08.054000+00:00"^^xsd:dateTime ;
    dcterms:modified "2025-08-05T22:48:03.748000+00:00"^^xsd:dateTime ;
    skos:broader asced:0505 ;
    skos:definition "Forestry Studies is the study of establishing, cultivating, harvesting and managing forests." ;
    skos:example "forest cultivation and maintenance, forest management, forest mensuration and inventory, timber harvesting" ;
    skos:inScheme ascedcs: ;
    skos:notation "050501" ;
    skos:prefLabel "Forestry Studies"@en .

asced:050701 a skos:Concept ;
    dcterms:created "2025-08-01T01:49:08.055000+00:00"^^xsd:dateTime ;
    dcterms:modified "2025-08-05T22:48:03.788000+00:00"^^xsd:dateTime ;
    skos:broader asced:0507 ;
    skos:definition "Aquaculture is the study of breeding, rearing, harvesting, handling and processing fish and other aquatic resources." ;
    skos:example "feeding and maintaining aquatic stock, principles of aquaculture production, stocking and sampling fisheries" ;
    skos:inScheme ascedcs: ;
    skos:notation "050701" ;
    skos:prefLabel "Aquaculture"@en .

asced:050799 a skos:Concept ;
    dcterms:created "2025-08-01T01:49:08.056000+00:00"^^xsd:dateTime ;
    dcterms:modified "2025-08-05T22:48:03.831000+00:00"^^xsd:dateTime ;
    skos:broader asced:0507 ;
    skos:definition "This detailed field includes all Fisheries Studies not elsewhere classified." ;
    skos:example "fisheries compliance" ;
    skos:inScheme ascedcs: ;
    skos:notation "050799" ;
    skos:prefLabel "Fisheries Studies, n.e.c."@en .

asced:050901 a skos:Concept ;
    dcterms:created "2025-08-01T01:49:08.058000+00:00"^^xsd:dateTime ;
    dcterms:modified "2025-08-05T22:48:03.876000+00:00"^^xsd:dateTime ;
    skos:broader asced:0509 ;
    skos:definition "Land, Parks and Wildlife Management is the study of managing land, parkland, marine and coastal zone parks, and wildlife." ;
    skos:example "flora and fauna management, land and water management, land rehabilitation, natural resource inventory and appraisal" ;
    skos:inScheme ascedcs: ;
    skos:notation "050901" ;
    skos:prefLabel "Land, Parks and Wildlife Management"@en .

asced:050999 a skos:Concept ;
    dcterms:created "2025-08-01T01:49:08.059000+00:00"^^xsd:dateTime ;
    dcterms:modified "2025-08-05T22:48:03.916000+00:00"^^xsd:dateTime ;
    skos:broader asced:0509 ;
    skos:definition "This detailed field includes all Environmental Studies not elsewhere classified." ;
    skos:example "environmental impact assessment, environmental science, land conservation, soil conservation" ;
    skos:inScheme ascedcs: ;
    skos:notation "050999" ;
    skos:prefLabel "Environmental Studies, n.e.c."@en .

asced:059901 a skos:Concept ;
    dcterms:created "2025-08-01T01:49:08.060000+00:00"^^xsd:dateTime ;
    dcterms:modified "2025-08-05T22:48:03.958000+00:00"^^xsd:dateTime ;
    skos:broader asced:0599 ;
    skos:definition "Pest and Weed Control is the study of controlling noxious plants, animals, insects and fungi." ;
    skos:example "fumigation techniques, integrated pest and weed control, pest and weed identification, plant disease control, plant protection programmes" ;
    skos:inScheme ascedcs: ;
    skos:notation "059901" ;
    skos:prefLabel "Pest and Weed Control"@en .

asced:059999 a skos:Concept ;
    dcterms:created "2025-08-01T01:49:08.061000+00:00"^^xsd:dateTime ;
    dcterms:modified "2025-08-05T22:48:03.997000+00:00"^^xsd:dateTime ;
    skos:broader asced:0599 ;
    skos:definition "This detailed field includes all Agriculture, Environmental and Related Studies not elsewhere classified." ;
    skos:example "irrigation" ;
    skos:inScheme ascedcs: ;
    skos:notation "059999" ;
    skos:prefLabel "Agriculture, Environmental and Related Studies, n.e.c."@en .

asced:060101 a skos:Concept ;
    dcterms:created "2025-08-01T01:49:08.063000+00:00"^^xsd:dateTime ;
    dcterms:modified "2025-08-05T22:48:04.576000+00:00"^^xsd:dateTime ;
    skos:broader asced:0601 ;
    skos:definition "General Medicine is the study of the clinical presentation and treatment of diseases." ;
    skos:example "clinical diagnosis, diseases affecting humans" ;
    skos:inScheme ascedcs: ;
    skos:notation "060101" ;
    skos:prefLabel "General Medicine"@en .

asced:060103 a skos:Concept ;
    dcterms:created "2025-08-01T01:49:08.064000+00:00"^^xsd:dateTime ;
    dcterms:modified "2025-08-05T22:48:04.617000+00:00"^^xsd:dateTime ;
    skos:broader asced:0601 ;
    skos:definition "Surgery is the study of the medical specialisation concerned with principles and practices for treating diseases, injuries, defects and deformities by manual operation and manipulation, and by using instruments and appliances." ;
    skos:example "post-operative patient progress monitoring, surgical diagnosis, surgical procedures and techniques" ;
    skos:inScheme ascedcs: ;
    skos:notation "060103" ;
    skos:prefLabel "Surgery"@en ;
    skos:scopeNote "Exclusions: Oral surgery. This is included in Detailed Field 060701 Dentistry. Veterinary surgery. This is included in Detailed Field 061101 Veterinary Science." .

asced:060105 a skos:Concept ;
    dcterms:created "2025-08-01T01:49:08.064000+00:00"^^xsd:dateTime ;
    dcterms:modified "2025-08-05T22:48:04.655000+00:00"^^xsd:dateTime ;
    skos:broader asced:0601 ;
    skos:definition "Psychiatry is the study of the medical specialisation concerned with diagnosing, preventing and treating diseases and disorders of the mind." ;
    skos:example "patient's psychiatric state assessment, child psychiatry, developmental psychiatry, psychiatric syndromes and phenomena" ;
    skos:inScheme ascedcs: ;
    skos:notation "060105" ;
    skos:prefLabel "Psychiatry"@en .

asced:060107 a skos:Concept ;
    dcterms:created "2025-08-01T01:49:08.065000+00:00"^^xsd:dateTime ;
    dcterms:modified "2025-08-05T22:48:04.696000+00:00"^^xsd:dateTime ;
    skos:broader asced:0601 ;
    skos:definition "Obstetrics and Gynaecology is the study of the medical specialisation concerned with the care of women during pregnancy, labour and after childbirth, and the prevention, diagnosis and treatment of diseases of the female reproductive system." ;
    skos:example "foetal development, gynaecological and obstetric conditions treatment, female reproductive system diseases" ;
    skos:inScheme ascedcs: ;
    skos:notation "060107" ;
    skos:prefLabel "Obstetrics and Gynaecology"@en .

asced:060109 a skos:Concept ;
    dcterms:created "2025-08-01T01:49:08.066000+00:00"^^xsd:dateTime ;
    dcterms:modified "2025-08-05T22:48:04.744000+00:00"^^xsd:dateTime ;
    skos:broader asced:0601 ;
    skos:definition "Paediatrics is the study of the medical specialisation concerned with normal physical growth and development from birth through to late adolescence. It includes preventing, diagnosing and treating diseases and uncommon disorders in children and adolescents." ;
    skos:example "physical growth and development of children, child and adolescent diseases, neonatology" ;
    skos:inScheme ascedcs: ;
    skos:notation "060109" ;
    skos:prefLabel "Paediatrics"@en .

asced:060111 a skos:Concept ;
    dcterms:created "2025-08-01T01:49:08.067000+00:00"^^xsd:dateTime ;
    dcterms:modified "2025-08-05T22:48:04.786000+00:00"^^xsd:dateTime ;
    skos:broader asced:0601 ;
    skos:definition "Anaesthesiology is the study of the medical specialisation concerned with administering drugs and other substances to achieve lack of sensation with or without loss of consciousness." ;
    skos:example "administering anaesthetics, regional analgesia, anaesthetic reactions" ;
    skos:inScheme ascedcs: ;
    skos:notation "060111" ;
    skos:prefLabel "Anaesthesiology"@en .

asced:060113 a skos:Concept ;
    dcterms:created "2025-08-01T01:49:08.068000+00:00"^^xsd:dateTime ;
    dcterms:modified "2025-08-05T22:48:04.826000+00:00"^^xsd:dateTime ;
    skos:broader asced:0601 ;
    skos:definition "Pathology is the study of the medical specialisation concerned with the causes and effects of diseases, including the structural and functional changes of body organs, tissues and fluids, and the systematic methods of detecting these changes." ;
    skos:example "disease origin, nature and course, histopathology, pathology tests interpretation and evaluation, post-mortem examination" ;
    skos:inScheme ascedcs: ;
    skos:notation "060113" ;
    skos:prefLabel "Pathology"@en .

asced:060115 a skos:Concept ;
    dcterms:created "2025-08-01T01:49:08.068000+00:00"^^xsd:dateTime ;
    dcterms:modified "2025-08-05T22:48:04.867000+00:00"^^xsd:dateTime ;
    skos:broader asced:0601 ;
    skos:definition "Radiology is the study of the medical specialisation concerned with using radioactive substances, X-rays and other ionising radiation to diagnose, treat and follow the course of disease and its response to treatment." ;
    skos:example "medical images interpretation and evaluation, nuclear medicine, tumour radiation treatment" ;
    skos:inScheme ascedcs: ;
    skos:notation "060115" ;
    skos:prefLabel "Radiology"@en .

asced:060117 a skos:Concept ;
    dcterms:created "2025-08-01T01:49:08.069000+00:00"^^xsd:dateTime ;
    dcterms:modified "2025-08-05T22:48:04.909000+00:00"^^xsd:dateTime ;
    skos:broader asced:0601 ;
    skos:definition "Internal Medicine is the study of the medical specialisation concerned with the diagnosis and non-surgical treatment of diseases and disorders of specific bodily structures and functions." ;
    skos:example "endocrinological medicine, gastroenterological medicine, thoracic medicine, clinical immunology, clinical haematology" ;
    skos:inScheme ascedcs: ;
    skos:notation "060117" ;
    skos:prefLabel "Internal Medicine"@en .

asced:060119 a skos:Concept ;
    dcterms:created "2025-08-01T01:49:08.070000+00:00"^^xsd:dateTime ;
    dcterms:modified "2025-08-05T22:48:04.951000+00:00"^^xsd:dateTime ;
    skos:broader asced:0601 ;
    skos:definition "General Practice is the study of providing primary and continuing medical care to patients in a community setting. It is particularly concerned with providing family and community oriented health care." ;
    skos:example "early diagnosis, medication prescription and administration, primary, personal and continuing medical care" ;
    skos:inScheme ascedcs: ;
    skos:notation "060119" ;
    skos:prefLabel "General Practice"@en .

asced:060199 a skos:Concept ;
    dcterms:created "2025-08-01T01:49:08.071000+00:00"^^xsd:dateTime ;
    dcterms:modified "2025-08-05T22:48:04.997000+00:00"^^xsd:dateTime ;
    skos:broader asced:0601 ;
    skos:definition "This detailed field includes all Medical Studies not elsewhere classified." ;
    skos:example "dermatology, oncology, ophthalmology" ;
    skos:inScheme ascedcs: ;
    skos:notation "060199" ;
    skos:prefLabel "Medical Studies, n.e.c."@en .

asced:060301 a skos:Concept ;
    dcterms:created "2025-08-01T01:49:08.072000+00:00"^^xsd:dateTime ;
    dcterms:modified "2025-08-05T22:48:05.044000+00:00"^^xsd:dateTime ;
    skos:broader asced:0603 ;
    skos:definition "General Nursing is the study of the principles and practices of providing preventative, curative and rehabilitative care to individuals and groups." ;
    skos:example "health status analysis and interpretation, nursing care in a variety of settings, nursing practice" ;
    skos:inScheme ascedcs: ;
    skos:notation "060301" ;
    skos:prefLabel "General Nursing"@en .

asced:060303 a skos:Concept ;
    dcterms:created "2025-08-01T01:49:08.072000+00:00"^^xsd:dateTime ;
    dcterms:modified "2025-08-05T22:48:05.087000+00:00"^^xsd:dateTime ;
    skos:broader asced:0603 ;
    skos:definition "Midwifery is the study of the principles and practices of providing care for women during pregnancy, birthing and after childbirth and for caring for the new-born. It includes assisting parents and families during childbearing." ;
    skos:example "pregnancy and post-natal period parent education and counselling, breastfeeding education, professional aspects of midwifery" ;
    skos:inScheme ascedcs: ;
    skos:notation "060303" ;
    skos:prefLabel "Midwifery"@en .

asced:060305 a skos:Concept ;
    dcterms:created "2025-08-01T01:49:08.073000+00:00"^^xsd:dateTime ;
    dcterms:modified "2025-08-05T22:48:05.123000+00:00"^^xsd:dateTime ;
    skos:broader asced:0603 ;
    skos:definition "Mental Health Nursing is the study of the nursing specialisation concerned with caring for persons with mental health problems." ;
    skos:example "acute and chronic mental disorder patient care, post acute phase patient rehabilitation, primary health care for mental health, mental health nursing practice" ;
    skos:inScheme ascedcs: ;
    skos:notation "060305" ;
    skos:prefLabel "Mental Health Nursing"@en .

asced:060307 a skos:Concept ;
    dcterms:created "2025-08-01T01:49:08.074000+00:00"^^xsd:dateTime ;
    dcterms:modified "2025-08-05T22:48:05.168000+00:00"^^xsd:dateTime ;
    skos:broader asced:0603 ;
    skos:definition "Community Nursing is the study of the nursing specialisation concerned with caring for individuals and groups in the community." ;
    skos:example "community nursing assessment, community nursing programme development" ;
    skos:inScheme ascedcs: ;
    skos:notation "060307" ;
    skos:prefLabel "Community Nursing"@en .

asced:060309 a skos:Concept ;
    dcterms:created "2025-08-01T01:49:08.074000+00:00"^^xsd:dateTime ;
    dcterms:modified "2025-08-05T22:48:05.205000+00:00"^^xsd:dateTime ;
    skos:broader asced:0603 ;
    skos:definition "Critical Care Nursing is the study of the nursing specialisation concerned with the theory and practice of caring for patients requiring intensive therapy." ;
    skos:example "post-operative advanced life support, intensive care nursing, neonatal intensive care nursing" ;
    skos:inScheme ascedcs: ;
    skos:notation "060309" ;
    skos:prefLabel "Critical Care Nursing"@en .

asced:060311 a skos:Concept ;
    dcterms:created "2025-08-01T01:49:08.075000+00:00"^^xsd:dateTime ;
    dcterms:modified "2025-08-05T22:48:05.240000+00:00"^^xsd:dateTime ;
    skos:broader asced:0603 ;
    skos:definition "Aged Care Nursing is the study of the nursing specialisation concerned with the theory and practice of caring for elderly patients." ;
    skos:example "health problems of the ageing patient, nursing elderly patients, gerontic nursing practices" ;
    skos:inScheme ascedcs: ;
    skos:notation "060311" ;
    skos:prefLabel "Aged Care Nursing"@en .

asced:060313 a skos:Concept ;
    dcterms:created "2025-08-01T01:49:08.076000+00:00"^^xsd:dateTime ;
    dcterms:modified "2025-08-05T22:48:05.284000+00:00"^^xsd:dateTime ;
    skos:broader asced:0603 ;
    skos:definition "Palliative Care Nursing is the study of the nursing specialisation concerned with caring for the terminally ill and their families." ;
    skos:example "pain and symptom control in the terminally ill, respite care" ;
    skos:inScheme ascedcs: ;
    skos:notation "060313" ;
    skos:prefLabel "Palliative Care Nursing"@en .

asced:060315 a skos:Concept ;
    dcterms:created "2025-08-01T01:49:08.076000+00:00"^^xsd:dateTime ;
    dcterms:modified "2025-08-05T22:48:05.328000+00:00"^^xsd:dateTime ;
    skos:broader asced:0603 ;
    skos:definition "Mothercraft Nursing and Family and Child Health Nursing is the study of the nursing specialisation concerned with the theory and practice of caring for young children and their families." ;
    skos:example "nursing care of infants and young children, paediatric nursing practice" ;
    skos:inScheme ascedcs: ;
    skos:notation "060315" ;
    skos:prefLabel "Mothercraft Nursing and Family and Child Health Nursing"@en .

asced:060399 a skos:Concept ;
    dcterms:created "2025-08-01T01:49:08.077000+00:00"^^xsd:dateTime ;
    dcterms:modified "2025-08-05T22:48:05.372000+00:00"^^xsd:dateTime ;
    skos:broader asced:0603 ;
    skos:definition "This detailed field includes all Nursing not elsewhere classified." ;
    skos:example "breast care nursing, cancer nursing" ;
    skos:inScheme ascedcs: ;
    skos:notation "060399" ;
    skos:prefLabel "Nursing, n.e.c."@en .

asced:060501 a skos:Concept ;
    dcterms:created "2025-08-01T01:49:08.078000+00:00"^^xsd:dateTime ;
    dcterms:modified "2025-08-05T22:48:05.416000+00:00"^^xsd:dateTime ;
    skos:broader asced:0605 ;
    skos:definition "Pharmacy is the study of the preparation and dispensing of drugs." ;
    skos:example "dosage, pharmaceutical calculations, pharmacy administration and practice, pharmaceutics" ;
    skos:inScheme ascedcs: ;
    skos:notation "060501" ;
    skos:prefLabel "Pharmacy"@en .

asced:060701 a skos:Concept ;
    dcterms:created "2025-08-01T01:49:08.079000+00:00"^^xsd:dateTime ;
    dcterms:modified "2025-08-05T22:48:05.458000+00:00"^^xsd:dateTime ;
    skos:broader asced:0607 ;
    skos:definition "Dentistry is the study of diagnosing, treating and preventing diseases of the teeth and adjacent tissues. It includes correcting malocclusion and restoring and replacing missing dental and oral structures." ;
    skos:example "orthodontic appliance fitting, inlays and artificial crowns, cavity detection and filling, teeth extraction, denture fitting, dental instruments and equipment, oral surgery" ;
    skos:inScheme ascedcs: ;
    skos:notation "060701" ;
    skos:prefLabel "Dentistry"@en .

asced:060703 a skos:Concept ;
    dcterms:created "2025-08-01T01:49:08.080000+00:00"^^xsd:dateTime ;
    dcterms:modified "2025-08-05T22:48:05.501000+00:00"^^xsd:dateTime ;
    skos:broader asced:0607 ;
    skos:definition "Dental Assisting is the study of providing assistance to dentists in clinical settings." ;
    skos:example "basic dental procedure assistance, dental materials and equipment care, dental records handling" ;
    skos:inScheme ascedcs: ;
    skos:notation "060703" ;
    skos:prefLabel "Dental Assisting"@en .

asced:060705 a skos:Concept ;
    dcterms:created "2025-08-01T01:49:08.081000+00:00"^^xsd:dateTime ;
    dcterms:modified "2025-08-05T22:48:05.550000+00:00"^^xsd:dateTime ;
    skos:broader asced:0607 ;
    skos:definition "Dental Technology is the study of designing, making and repairing dental prostheses and orthodontic appliances." ;
    skos:example "dental laboratory methodology, dental repairs and relines, dental materials science" ;
    skos:inScheme ascedcs: ;
    skos:notation "060705" ;
    skos:prefLabel "Dental Technology"@en .

asced:060799 a skos:Concept ;
    dcterms:created "2025-08-01T01:49:08.081000+00:00"^^xsd:dateTime ;
    dcterms:modified "2025-08-05T22:48:05.599000+00:00"^^xsd:dateTime ;
    skos:broader asced:0607 ;
    skos:definition "This detailed field includes all Dental Studies not elsewhere classified." ;
    skos:example "dental hygiene, dental radiography" ;
    skos:inScheme ascedcs: ;
    skos:notation "060799" ;
    skos:prefLabel "Dental Studies, n.e.c."@en .

asced:060901 a skos:Concept ;
    dcterms:created "2025-08-01T01:49:08.083000+00:00"^^xsd:dateTime ;
    dcterms:modified "2025-08-05T22:48:05.653000+00:00"^^xsd:dateTime ;
    skos:broader asced:0609 ;
    skos:definition "Optometry is the study of measuring and assessing vision, and prescribing lenses for visual correction." ;
    skos:example "vision testing apparatus operation, ocular diseases and treatment, vision testing, visual aids prescription" ;
    skos:inScheme ascedcs: ;
    skos:notation "060901" ;
    skos:prefLabel "Optometry"@en ;
    skos:scopeNote "Exclusions: Orthoptics. This is included in Detailed Field 061799 Rehabilitation Therapies, n.e.c." .

asced:060903 a skos:Concept ;
    dcterms:created "2025-08-01T01:49:08.083000+00:00"^^xsd:dateTime ;
    dcterms:modified "2025-08-05T22:48:05.716000+00:00"^^xsd:dateTime ;
    skos:broader asced:0609 ;
    skos:definition "Optical Technology is the study of preparing and dispensing corrective lenses according to prescription." ;
    skos:example "lens design, lens surfacing, multifocal lenses" ;
    skos:inScheme ascedcs: ;
    skos:notation "060903" ;
    skos:prefLabel "Optical Technology"@en .

asced:060999 a skos:Concept ;
    dcterms:created "2025-08-01T01:49:08.084000+00:00"^^xsd:dateTime ;
    dcterms:modified "2025-08-05T22:48:05.797000+00:00"^^xsd:dateTime ;
    skos:broader asced:0609 ;
    skos:definition "This detailed field includes all Optical Science not elsewhere classified." ;
    skos:inScheme ascedcs: ;
    skos:notation "060999" ;
    skos:prefLabel "Optical Science, n.e.c."@en .

asced:061101 a skos:Concept ;
    dcterms:created "2025-08-01T01:49:08.085000+00:00"^^xsd:dateTime ;
    dcterms:modified "2025-08-05T22:48:05.844000+00:00"^^xsd:dateTime ;
    skos:broader asced:0611 ;
    skos:definition "Veterinary Science is the study of diagnosing and treating animal diseases, ailments and injuries, and preventing and containing the spread of animal diseases." ;
    skos:example "veterinary pathology, animal health, medical and surgical procedures on animals" ;
    skos:inScheme ascedcs: ;
    skos:notation "061101" ;
    skos:prefLabel "Veterinary Science"@en .

asced:061103 a skos:Concept ;
    dcterms:created "2025-08-01T01:49:08.087000+00:00"^^xsd:dateTime ;
    dcterms:modified "2025-08-05T22:48:05.892000+00:00"^^xsd:dateTime ;
    skos:broader asced:0611 ;
    skos:definition "Veterinary Assisting is the study of caring for sick, injured and infirm animals undergoing treatment in veterinary clinics." ;
    skos:example "animal care and treatment assistance, veterinary surgery preparation, post-operative animal care and monitoring, veterinary nursing practical skills" ;
    skos:inScheme ascedcs: ;
    skos:notation "061103" ;
    skos:prefLabel "Veterinary Assisting"@en .

asced:061199 a skos:Concept ;
    dcterms:created "2025-08-01T01:49:08.088000+00:00"^^xsd:dateTime ;
    dcterms:modified "2025-08-05T22:48:05.941000+00:00"^^xsd:dateTime ;
    skos:broader asced:0611 ;
    skos:definition "This detailed field includes all Veterinary Studies not elsewhere classified." ;
    skos:inScheme ascedcs: ;
    skos:notation "061199" ;
    skos:prefLabel "Veterinary Studies, n.e.c."@en .

asced:061301 a skos:Concept ;
    dcterms:created "2025-08-01T01:49:08.089000+00:00"^^xsd:dateTime ;
    dcterms:modified "2025-08-05T22:48:05.983000+00:00"^^xsd:dateTime ;
    skos:broader asced:0613 ;
    skos:definition "Occupational Health and Safety is the study of recognising, evaluating and controlling environmental factors associated with the interaction of individuals and the workplace." ;
    skos:example "principles of health and safety in the workplace, national occupational health and safety standards, workplace health and safety programmes, hazard management, ergonomics" ;
    skos:inScheme ascedcs: ;
    skos:notation "061301" ;
    skos:prefLabel "Occupational Health and Safety"@en .

asced:061303 a skos:Concept ;
    dcterms:created "2025-08-01T01:49:08.089000+00:00"^^xsd:dateTime ;
    dcterms:modified "2025-08-05T22:48:06.026000+00:00"^^xsd:dateTime ;
    skos:broader asced:0613 ;
    skos:definition "Environmental Health is the study of recognising, evaluating and controlling environmental factors affecting public health." ;
    skos:example "environmental pollution effects on health, communicable disease management systems, food-borne disease prevention techniques, public hygiene" ;
    skos:inScheme ascedcs: ;
    skos:notation "061303" ;
    skos:prefLabel "Environmental Health"@en .

asced:061305 a skos:Concept ;
    dcterms:created "2025-08-01T01:49:08.090000+00:00"^^xsd:dateTime ;
    dcterms:modified "2025-08-05T22:48:06.070000+00:00"^^xsd:dateTime ;
    skos:broader asced:0613 ;
    skos:definition "Indigenous Health is the study of the health of the indigenous population within the broader context of socio-economic development of Aboriginal and Torres Strait Islander communities." ;
    skos:example "indigenous health care delivery approaches, indigenous caring and healing practices, indigenous child health, indigenous community health, indigenous primary health care" ;
    skos:inScheme ascedcs: ;
    skos:notation "061305" ;
    skos:prefLabel "Indigenous Health"@en .

asced:061307 a skos:Concept ;
    dcterms:created "2025-08-01T01:49:08.090000+00:00"^^xsd:dateTime ;
    dcterms:modified "2025-08-05T22:48:06.111000+00:00"^^xsd:dateTime ;
    skos:broader asced:0613 ;
    skos:definition "Health Promotion is the study of promoting a healthy lifestyle and influencing behaviour to improve health." ;
    skos:example "health promotion programme planning, health promotion principles, goals and concepts, social perspectives of health, health promotion strategies and evaluation" ;
    skos:inScheme ascedcs: ;
    skos:notation "061307" ;
    skos:prefLabel "Health Promotion"@en .

asced:061309 a skos:Concept ;
    dcterms:created "2025-08-01T01:49:08.091000+00:00"^^xsd:dateTime ;
    dcterms:modified "2025-08-05T22:48:06.157000+00:00"^^xsd:dateTime ;
    skos:broader asced:0613 ;
    skos:definition "Community Health is the study of health practices in the community which support and assist the management of disabilities and illness." ;
    skos:example "current issues in Australian community health, disabilities and illnesses as community issues" ;
    skos:inScheme ascedcs: ;
    skos:notation "061309" ;
    skos:prefLabel "Community Health"@en .

asced:061311 a skos:Concept ;
    dcterms:created "2025-08-01T01:49:08.093000+00:00"^^xsd:dateTime ;
    dcterms:modified "2025-08-05T22:48:06.202000+00:00"^^xsd:dateTime ;
    skos:broader asced:0613 ;
    skos:definition "Epidemiology is the study of the incidence, distribution and possible control of infectious and chronic diseases as they effect groups of people." ;
    skos:example "disease and injury evaluation and surveillance, infectious and chronic disease prevention" ;
    skos:inScheme ascedcs: ;
    skos:notation "061311" ;
    skos:prefLabel "Epidemiology"@en .

asced:061399 a skos:Concept ;
    dcterms:created "2025-08-01T01:49:08.093000+00:00"^^xsd:dateTime ;
    dcterms:modified "2025-08-05T22:48:06.240000+00:00"^^xsd:dateTime ;
    skos:broader asced:0613 ;
    skos:definition "This detailed field includes all Public Health not elsewhere classified." ;
    skos:example "social health, tropical medicine, infection control" ;
    skos:inScheme ascedcs: ;
    skos:notation "061399" ;
    skos:prefLabel "Public Health, n.e.c."@en .

asced:061501 a skos:Concept ;
    dcterms:created "2025-08-01T01:49:08.094000+00:00"^^xsd:dateTime ;
    dcterms:modified "2025-08-05T22:48:06.281000+00:00"^^xsd:dateTime ;
    skos:broader asced:0615 ;
    skos:definition "Radiography is the study of technologies which use ionising and non-ionising (e.g. ultrasound) radiation for producing diagnostic images and administering radiation therapy." ;
    skos:example "medical imaging equipment operation, radioactive materials preparation, radiation exposure factors, radiographic examination methods, radiological dosimetry" ;
    skos:inScheme ascedcs: ;
    skos:notation "061501" ;
    skos:prefLabel "Radiography"@en ;
    skos:scopeNote "Exclusions: Developing diagnostic imaging systems. This is included in Detailed Field 039903 Biomedical Engineering. Radiology. This is included in Detailed Field 060115 Radiology. Dental radiography. This is included in Detailed Field 060799 Dental Studies, n.e.c." .

asced:061701 a skos:Concept ;
    dcterms:created "2025-08-01T01:49:08.095000+00:00"^^xsd:dateTime ;
    dcterms:modified "2025-08-05T22:48:06.323000+00:00"^^xsd:dateTime ;
    skos:broader asced:0617 ;
    skos:definition "Physiotherapy is the study of assessing people with temporary and longer term physical injuries and movement disorders, and restoring maximum movement and functional ability." ;
    skos:example "electrotherapy and electrophysical agents, movement training and rehabilitation, normal and abnormal musculoskeletal function" ;
    skos:inScheme ascedcs: ;
    skos:notation "061701" ;
    skos:prefLabel "Physiotherapy"@en .

asced:061703 a skos:Concept ;
    dcterms:created "2025-08-01T01:49:08.096000+00:00"^^xsd:dateTime ;
    dcterms:modified "2025-08-05T22:48:06.368000+00:00"^^xsd:dateTime ;
    skos:broader asced:0617 ;
    skos:definition "Occupational Therapy is the study of treating physical, cognitive and psychiatric conditions through activities in order to optimise functioning and independence in daily life." ;
    skos:example "patient's independence level assessment, tailoring treatment programmes, occupational rehabilitation, occupational role development" ;
    skos:inScheme ascedcs: ;
    skos:notation "061703" ;
    skos:prefLabel "Occupational Therapy"@en .

asced:061705 a skos:Concept ;
    dcterms:created "2025-08-01T01:49:08.096000+00:00"^^xsd:dateTime ;
    dcterms:modified "2025-08-05T22:48:06.412000+00:00"^^xsd:dateTime ;
    skos:broader asced:0617 ;
    skos:definition "Chiropractic and Osteopathy is the study of assessing and relieving disorders of the body through manipulating and treating the musculoskeletal system." ;
    skos:example "posture, and preventative and corrective exercises, manipulation and adjustment" ;
    skos:inScheme ascedcs: ;
    skos:notation "061705" ;
    skos:prefLabel "Chiropractic and Osteopathy"@en .

asced:061707 a skos:Concept ;
    dcterms:created "2025-08-01T01:49:08.097000+00:00"^^xsd:dateTime ;
    dcterms:modified "2025-08-05T22:48:06.459000+00:00"^^xsd:dateTime ;
    skos:broader asced:0617 ;
    skos:definition "Speech Pathology is the study of assessing and treating speech and language disorders." ;
    skos:example "communicative functioning assessment and evaluation, stuttering, abnormal articulation and other verbal disorders remedial exercise programmes, language and voice disorders" ;
    skos:inScheme ascedcs: ;
    skos:notation "061707" ;
    skos:prefLabel "Speech Pathology"@en .

asced:061709 a skos:Concept ;
    dcterms:created "2025-08-01T01:49:08.100000+00:00"^^xsd:dateTime ;
    dcterms:modified "2025-08-05T22:48:06.512000+00:00"^^xsd:dateTime ;
    skos:broader asced:0617 ;
    skos:definition "Audiology is the study of assessing and treating hearing disorders." ;
    skos:example "audiometry, fitting hearing aids, testing for hearing loss" ;
    skos:inScheme ascedcs: ;
    skos:notation "061709" ;
    skos:prefLabel "Audiology"@en .

asced:061711 a skos:Concept ;
    dcterms:created "2025-08-01T01:49:08.101000+00:00"^^xsd:dateTime ;
    dcterms:modified "2025-08-05T22:48:06.553000+00:00"^^xsd:dateTime ;
    skos:broader asced:0617 ;
    skos:definition "Massage Therapy is the study of treating disorders through massage of the soft tissue." ;
    skos:example "reflexology, postural massage techniques, deep tissue techniques" ;
    skos:inScheme ascedcs: ;
    skos:notation "061711" ;
    skos:prefLabel "Massage Therapy"@en .

asced:061713 a skos:Concept ;
    dcterms:created "2025-08-01T01:49:08.101000+00:00"^^xsd:dateTime ;
    dcterms:modified "2025-08-05T22:48:06.593000+00:00"^^xsd:dateTime ;
    skos:broader asced:0617 ;
    skos:definition "Podiatry is the study of assessing and treating physical ailments of the human foot and lower limb." ;
    skos:example "foot and lower limb abnormalities, podiatric appliances, foot and gait disorders" ;
    skos:inScheme ascedcs: ;
    skos:notation "061713" ;
    skos:prefLabel "Podiatry"@en .

asced:061799 a skos:Concept ;
    dcterms:created "2025-08-01T01:49:08.102000+00:00"^^xsd:dateTime ;
    dcterms:modified "2025-08-05T22:48:06.640000+00:00"^^xsd:dateTime ;
    skos:broader asced:0617 ;
    skos:definition "This detailed field includes all Rehabilitation Therapies not elsewhere classified." ;
    skos:example "diversional therapy, orthoptics, exercise rehabilitation, orthotics and prosthetics" ;
    skos:inScheme ascedcs: ;
    skos:notation "061799" ;
    skos:prefLabel "Rehabilitation Therapies, n.e.c."@en .

asced:061901 a skos:Concept ;
    dcterms:created "2025-08-01T01:49:08.103000+00:00"^^xsd:dateTime ;
    dcterms:modified "2025-08-05T22:48:06.685000+00:00"^^xsd:dateTime ;
    skos:broader asced:0619 ;
    skos:definition "Naturopathy is the study of treating diseases using natural therapies." ;
    skos:example "pharmocognosy, herbal medicine, phytotherapy, naturopathic diagnosis" ;
    skos:inScheme ascedcs: ;
    skos:notation "061901" ;
    skos:prefLabel "Naturopathy"@en .

asced:061903 a skos:Concept ;
    dcterms:created "2025-08-01T01:49:08.103000+00:00"^^xsd:dateTime ;
    dcterms:modified "2025-08-05T22:48:06.727000+00:00"^^xsd:dateTime ;
    skos:broader asced:0619 ;
    skos:definition "Acupuncture is the study of treating diseases through influencing points on meridians using fine needles." ;
    skos:example "acupuncture therapy, channels and points, identification of acupuncture sites, acupressure" ;
    skos:inScheme ascedcs: ;
    skos:notation "061903" ;
    skos:prefLabel "Acupuncture"@en .

asced:061905 a skos:Concept ;
    dcterms:created "2025-08-01T01:49:08.105000+00:00"^^xsd:dateTime ;
    dcterms:modified "2025-08-05T22:48:06.770000+00:00"^^xsd:dateTime ;
    skos:broader asced:0619 ;
    skos:definition "Traditional Chinese Medicine is the study of treating diseases through traditional Chinese therapies." ;
    skos:example "Chinese herbal medicine, Chinese therapies, moxibustion, patterns of disharmony, pharmocognosy of Chinese herbs" ;
    skos:inScheme ascedcs: ;
    skos:notation "061905" ;
    skos:prefLabel "Traditional Chinese Medicine"@en .

asced:061999 a skos:Concept ;
    dcterms:created "2025-08-01T01:49:08.108000+00:00"^^xsd:dateTime ;
    dcterms:modified "2025-08-05T22:48:06.815000+00:00"^^xsd:dateTime ;
    skos:broader asced:0619 ;
    skos:definition "This detailed field includes all Complementary Therapies not elsewhere classified." ;
    skos:example "aromatherapy, homeopathy, iridology, kinesiology" ;
    skos:inScheme ascedcs: ;
    skos:notation "061999" ;
    skos:prefLabel "Complementary Therapies, n.e.c."@en .

asced:069901 a skos:Concept ;
    dcterms:created "2025-08-01T01:49:08.109000+00:00"^^xsd:dateTime ;
    dcterms:modified "2025-08-05T22:48:06.859000+00:00"^^xsd:dateTime ;
    skos:broader asced:0699 ;
    skos:definition "Nutrition and Dietetics is the study of the nutritional and dietary needs of humans." ;
    skos:example "nutritional assessment and evaluation, food intake measurement, nutrients and metabolism" ;
    skos:inScheme ascedcs: ;
    skos:notation "069901" ;
    skos:prefLabel "Nutrition and Dietetics"@en .

asced:069903 a skos:Concept ;
    dcterms:created "2025-08-01T01:49:08.109000+00:00"^^xsd:dateTime ;
    dcterms:modified "2025-08-05T22:48:06.917000+00:00"^^xsd:dateTime ;
    skos:broader asced:0699 ;
    skos:definition "Human Movement is the study of the nature, cause and control of movement. It includes posture and balance, and the science of human performance." ;
    skos:example "biomechanical basis of movement, motor control and learning, injury prevention and management, sports and exercise science" ;
    skos:inScheme ascedcs: ;
    skos:notation "069903" ;
    skos:prefLabel "Human Movement"@en .

asced:069905 a skos:Concept ;
    dcterms:created "2025-08-01T01:49:08.110000+00:00"^^xsd:dateTime ;
    dcterms:modified "2025-08-05T22:48:06.957000+00:00"^^xsd:dateTime ;
    skos:broader asced:0699 ;
    skos:definition "Paramedical Studies is the study of the emergency treatment of the sick and injured prior to and during transfer to a hospital or medical facility." ;
    skos:example "ambulance principles and practice, fundamentals of paramedicine, pre-hospital health service delivery issues, out of hospital practice, patient transport attendance, specialist life support equipment" ;
    skos:inScheme ascedcs: ;
    skos:notation "069905" ;
    skos:prefLabel "Paramedical Studies"@en .

asced:069907 a skos:Concept ;
    dcterms:created "2025-08-01T01:49:08.110000+00:00"^^xsd:dateTime ;
    dcterms:modified "2025-08-05T22:48:06.997000+00:00"^^xsd:dateTime ;
    skos:broader asced:0699 ;
    skos:definition "First Aid is the study of skills necessary to aid the ill and injured until medical aid arrives." ;
    skos:example "casualty assessment, first aid treatment, resuscitation" ;
    skos:inScheme ascedcs: ;
    skos:notation "069907" ;
    skos:prefLabel "First Aid"@en .

asced:069999 a skos:Concept ;
    dcterms:created "2025-08-01T01:49:08.111000+00:00"^^xsd:dateTime ;
    dcterms:modified "2025-08-05T22:48:07.042000+00:00"^^xsd:dateTime ;
    skos:broader asced:0699 ;
    skos:definition "This detailed field includes all Health not elsewhere classified." ;
    skos:example "pain management, respiratory science" ;
    skos:inScheme ascedcs: ;
    skos:notation "069999" ;
    skos:prefLabel "Health, n.e.c."@en .

asced:070101 a skos:Concept ;
    dcterms:created "2025-08-01T01:49:08.113000+00:00"^^xsd:dateTime ;
    dcterms:modified "2025-08-05T22:48:07.254000+00:00"^^xsd:dateTime ;
    skos:broader asced:0701 ;
    skos:definition "Teacher Education: Early Childhood is the study of the theories, methods and practice of teaching children from birth to 8 years of age within formal education settings." ;
    skos:example "early childhood learning, early childhood development and pedagogy, theory and practice of play" ;
    skos:inScheme ascedcs: ;
    skos:notation "070101" ;
    skos:prefLabel "Teacher Education: Early Childhood"@en .

asced:070103 a skos:Concept ;
    dcterms:created "2025-08-01T01:49:08.114000+00:00"^^xsd:dateTime ;
    dcterms:modified "2025-08-05T22:48:07.290000+00:00"^^xsd:dateTime ;
    skos:broader asced:0701 ;
    skos:definition "Teacher Education: Primary is the study of the theories, methods and practice of teaching children between the ages of 5 and 12 within formal school settings." ;
    skos:example "information technology in primary teaching practices, children's literature in the classroom, communication in a primary educational setting" ;
    skos:inScheme ascedcs: ;
    skos:notation "070103" ;
    skos:prefLabel "Teacher Education: Primary"@en .

asced:070105 a skos:Concept ;
    dcterms:created "2025-08-01T01:49:08.115000+00:00"^^xsd:dateTime ;
    dcterms:modified "2025-08-05T22:48:07.326000+00:00"^^xsd:dateTime ;
    skos:broader asced:0701 ;
    skos:definition "Teacher Education: Secondary is the study of the theories, methods and practice of teaching secondary school students between the ages of 12 and 18 within formal school and college settings." ;
    skos:example "facilitating adolescent learning, communication in a secondary educational setting, information technology in secondary teaching practices" ;
    skos:inScheme ascedcs: ;
    skos:notation "070105" ;
    skos:prefLabel "Teacher Education: Secondary"@en .

asced:070107 a skos:Concept ;
    dcterms:created "2025-08-01T01:49:08.115000+00:00"^^xsd:dateTime ;
    dcterms:modified "2025-08-05T22:48:07.362000+00:00"^^xsd:dateTime ;
    skos:broader asced:0701 ;
    skos:definition "Teacher-Librarianship is the study of the theories, methods and practice of teaching relating to the integration of library and information resources in schools and colleges." ;
    skos:example "resources for learning, educational information sources and services, library technology, school library integration into total school curriculum" ;
    skos:inScheme ascedcs: ;
    skos:notation "070107" ;
    skos:prefLabel "Teacher-Librarianship"@en .

asced:070109 a skos:Concept ;
    dcterms:created "2025-08-01T01:49:08.116000+00:00"^^xsd:dateTime ;
    dcterms:modified "2025-08-05T22:48:07.402000+00:00"^^xsd:dateTime ;
    skos:broader asced:0701 ;
    skos:definition "Teacher Education: Vocational Education and Training is the study of the theories, methods and practice of teaching trade and other vocational subjects." ;
    skos:example "VET training methods, foundations of adult education, post school education and training in Australia" ;
    skos:inScheme ascedcs: ;
    skos:notation "070109" ;
    skos:prefLabel "Teacher Education: Vocational Education and Training"@en .

asced:070111 a skos:Concept ;
    dcterms:created "2025-08-01T01:49:08.116000+00:00"^^xsd:dateTime ;
    dcterms:modified "2025-08-05T22:48:07.443000+00:00"^^xsd:dateTime ;
    skos:broader asced:0701 ;
    skos:definition "Teacher Education: Higher Education is the study of the theories, methods and practice of teaching in higher educational institutions." ;
    skos:example "teaching for learning in higher education, facilitating higher education student learning, information technology for higher education learning and teaching" ;
    skos:inScheme ascedcs: ;
    skos:notation "070111" ;
    skos:prefLabel "Teacher Education: Higher Education"@en .

asced:070113 a skos:Concept ;
    dcterms:created "2025-08-01T01:49:08.117000+00:00"^^xsd:dateTime ;
    dcterms:modified "2025-08-05T22:48:07.488000+00:00"^^xsd:dateTime ;
    skos:broader asced:0701 ;
    skos:definition "Teacher Education: Special Education is the study of the theories, methods and practice of teaching children with special learning needs, including children with physical and mental disabilities and impairments, and gifted children. Special Education may be conducted in special schools or by providing support for teachers in primary and secondary schools." ;
    skos:example "early intervention and children with special needs, gifted children and their needs, teaching methods in special education, learning support" ;
    skos:inScheme ascedcs: ;
    skos:notation "070113" ;
    skos:prefLabel "Teacher Education: Special Education"@en .

asced:070115 a skos:Concept ;
    dcterms:created "2025-08-01T01:49:08.117000+00:00"^^xsd:dateTime ;
    dcterms:modified "2025-08-05T22:48:07.531000+00:00"^^xsd:dateTime ;
    skos:broader asced:0701 ;
    skos:definition "English as a Second Language Teaching is the study of theories, methods and practice of teaching English to those whose first language is other than English, including teaching children in school settings and teaching adults and children in other settings." ;
    skos:example "second language teaching methodologies, managing cross-cultural classes, principles of teaching English as a second language, issues in second language theory and practice" ;
    skos:inScheme ascedcs: ;
    skos:notation "070115" ;
    skos:prefLabel "English as a Second Language Teaching"@en .

asced:070117 a skos:Concept ;
    dcterms:created "2025-08-01T01:49:08.119000+00:00"^^xsd:dateTime ;
    dcterms:modified "2025-08-05T22:48:07.572000+00:00"^^xsd:dateTime ;
    skos:broader asced:0701 ;
    skos:definition "Nursing Education Teacher Training is the study of the theories, methods and practice of teaching nurses in tertiary educational institutions and hospital-based settings." ;
    skos:example "teaching in nurse education, contemporary issues in nurse education" ;
    skos:inScheme ascedcs: ;
    skos:notation "070117" ;
    skos:prefLabel "Nursing Education Teacher Training"@en .

asced:070199 a skos:Concept ;
    dcterms:created "2025-08-01T01:49:08.119000+00:00"^^xsd:dateTime ;
    dcterms:modified "2025-08-05T22:48:07.614000+00:00"^^xsd:dateTime ;
    skos:broader asced:0701 ;
    skos:definition "This detailed field includes all Teacher Education not elsewhere classified." ;
    skos:example "firearms instructor training, indigenous education teacher training, physical education teacher training, drama education, train the trainer" ;
    skos:inScheme ascedcs: ;
    skos:notation "070199" ;
    skos:prefLabel "Teacher Education, n.e.c."@en .

asced:070301 a skos:Concept ;
    dcterms:created "2025-08-01T01:49:08.120000+00:00"^^xsd:dateTime ;
    dcterms:modified "2025-08-05T22:48:07.651000+00:00"^^xsd:dateTime ;
    skos:broader asced:0703 ;
    skos:definition "Curriculum Studies is the study of developing and evaluating appropriate curricula for different Key Learning Areas and subjects to teach to particular groups of children and adults." ;
    skos:example "concepts of curricula, evaluation of curricula, principles of curriculum development, system based and school based curricula" ;
    skos:inScheme ascedcs: ;
    skos:notation "070301" ;
    skos:prefLabel "Curriculum Studies"@en .

asced:070303 a skos:Concept ;
    dcterms:created "2025-08-01T01:49:08.120000+00:00"^^xsd:dateTime ;
    dcterms:modified "2025-08-05T22:48:07.695000+00:00"^^xsd:dateTime ;
    skos:broader asced:0703 ;
    skos:definition "Education Studies is the study of the theoretical background of traditional and current teaching practices." ;
    skos:example "social factors influencing education, comparative education, analysis of educational philosophies, pedagogic theory, theory of educational assessment" ;
    skos:inScheme ascedcs: ;
    skos:notation "070303" ;
    skos:prefLabel "Education Studies"@en .

asced:079999 a skos:Concept ;
    dcterms:created "2025-08-01T01:49:08.121000+00:00"^^xsd:dateTime ;
    dcterms:modified "2025-08-05T22:48:07.730000+00:00"^^xsd:dateTime ;
    skos:broader asced:0799 ;
    skos:definition "This detailed field includes all Education not elsewhere classified." ;
    skos:example "home tutoring, teacher assisting" ;
    skos:inScheme ascedcs: ;
    skos:notation "079999" ;
    skos:prefLabel "Education, n.e.c."@en .

asced:080101 a skos:Concept ;
    dcterms:created "2025-08-01T01:49:08.124000+00:00"^^xsd:dateTime ;
    dcterms:modified "2025-08-05T22:48:08.095000+00:00"^^xsd:dateTime ;
    skos:broader asced:0801 ;
    skos:definition "Accounting is the study of the theory and practice of developing, maintaining, auditing and analysing financial records." ;
    skos:example "auditing and taxation, bookkeeping, financial systems design and operation, financial report writing, general purpose accounting statements" ;
    skos:inScheme ascedcs: ;
    skos:notation "080101" ;
    skos:prefLabel "Accounting"@en ;
    skos:scopeNote "Exclusions: Taxation law. This is included in Detailed Field 090911 Taxation Law." .

asced:080301 a skos:Concept ;
    dcterms:created "2025-08-01T01:49:08.124000+00:00"^^xsd:dateTime ;
    dcterms:modified "2025-08-05T22:48:08.135000+00:00"^^xsd:dateTime ;
    skos:broader asced:0803 ;
    skos:definition "Business Management is the study of planning and directing the activities of commercial enterprises. It includes the study of the nature, operation and role of business, and the resolution of management and administrative problems." ;
    skos:example "business managerial policies, business plan administration, business and the economic, legal, social, political and ethical environment" ;
    skos:inScheme ascedcs: ;
    skos:notation "080301" ;
    skos:prefLabel "Business Management"@en .

asced:080303 a skos:Concept ;
    dcterms:created "2025-08-01T01:49:08.125000+00:00"^^xsd:dateTime ;
    dcterms:modified "2025-08-05T22:48:08.176000+00:00"^^xsd:dateTime ;
    skos:broader asced:0803 ;
    skos:definition "Human Resource Management is the study of staffing policy, practice and management within an organisation." ;
    skos:example "training needs assessment, performance management, personnel management, recruiting and job analysis and design, staff development and training co-ordination, staff supervision" ;
    skos:inScheme ascedcs: ;
    skos:notation "080303" ;
    skos:prefLabel "Human Resource Management"@en .

asced:080305 a skos:Concept ;
    dcterms:created "2025-08-01T01:49:08.126000+00:00"^^xsd:dateTime ;
    dcterms:modified "2025-08-05T22:48:08.213000+00:00"^^xsd:dateTime ;
    skos:broader asced:0803 ;
    skos:definition "Personal Management Training is the study of self-improvement techniques." ;
    skos:example "personal creativity, personal effectiveness, personal motivation, self-esteem, stress management, time management" ;
    skos:inScheme ascedcs: ;
    skos:notation "080305" ;
    skos:prefLabel "Personal Management Training"@en .

asced:080307 a skos:Concept ;
    dcterms:created "2025-08-01T01:49:08.126000+00:00"^^xsd:dateTime ;
    dcterms:modified "2025-08-05T22:48:08.247000+00:00"^^xsd:dateTime ;
    skos:broader asced:0803 ;
    skos:definition "Organisation Management is the study of organisational structure and change." ;
    skos:example "change management, organisational change and leadership, organisational context of human resource management, organisational politics and culture, organisational behaviour" ;
    skos:inScheme ascedcs: ;
    skos:notation "080307" ;
    skos:prefLabel "Organisation Management"@en .

asced:080309 a skos:Concept ;
    dcterms:created "2025-08-01T01:49:08.126000+00:00"^^xsd:dateTime ;
    dcterms:modified "2025-08-05T22:48:08.283000+00:00"^^xsd:dateTime ;
    skos:broader asced:0803 ;
    skos:definition "Industrial Relations is the study of the relationship between employers and employees, and the application of such relations to workplace issues." ;
    skos:example "advocacy and negotiation, employee relations, industrial conflict, workplace issues" ;
    skos:inScheme ascedcs: ;
    skos:notation "080309" ;
    skos:prefLabel "Industrial Relations"@en .

asced:080311 a skos:Concept ;
    dcterms:created "2025-08-01T01:49:08.128000+00:00"^^xsd:dateTime ;
    dcterms:modified "2025-08-05T22:48:08.318000+00:00"^^xsd:dateTime ;
    skos:broader asced:0803 ;
    skos:definition "International Business is the study of international trade, import and export processes and regulations and customs procedures and regulations." ;
    skos:example "customs practices, permit issuing authorities, international and multinational trade, tariffs" ;
    skos:inScheme ascedcs: ;
    skos:notation "080311" ;
    skos:prefLabel "International Business"@en ;
    skos:scopeNote "Exclusions: International trade law. This is included in Detailed Field 090909 International Law." .

asced:080313 a skos:Concept ;
    dcterms:created "2025-08-01T01:49:08.128000+00:00"^^xsd:dateTime ;
    dcterms:modified "2025-08-05T22:48:08.355000+00:00"^^xsd:dateTime ;
    skos:broader asced:0803 ;
    skos:definition "Public and Health Care Administration is the study of planning and directing the functions and operations of organisations whose primary objective is the provision of services for the public good." ;
    skos:example "Australian health system, public sector guidelines and procedures, public organisations and their role, health planning, policy and programme evaluation" ;
    skos:inScheme ascedcs: ;
    skos:notation "080313" ;
    skos:prefLabel "Public and Health Care Administration"@en .

asced:080315 a skos:Concept ;
    dcterms:created "2025-08-01T01:49:08.128000+00:00"^^xsd:dateTime ;
    dcterms:modified "2025-08-05T22:48:08.392000+00:00"^^xsd:dateTime ;
    skos:broader asced:0803 ;
    skos:definition "Project Management is the study of planning and managing a total project process." ;
    skos:example "design management, project life cycles, project management, project planning" ;
    skos:inScheme ascedcs: ;
    skos:notation "080315" ;
    skos:prefLabel "Project Management"@en .

asced:080317 a skos:Concept ;
    dcterms:created "2025-08-01T01:49:08.129000+00:00"^^xsd:dateTime ;
    dcterms:modified "2025-08-05T22:48:08.430000+00:00"^^xsd:dateTime ;
    skos:broader asced:0803 ;
    skos:definition "Quality Management is the study of initiating and implementing quality assurance techniques and procedures to meet standards of best practice." ;
    skos:example "benchmarking, continuous improvement, organisation performance evaluation" ;
    skos:inScheme ascedcs: ;
    skos:notation "080317" ;
    skos:prefLabel "Quality Management"@en .

asced:080319 a skos:Concept ;
    dcterms:created "2025-08-01T01:49:08.129000+00:00"^^xsd:dateTime ;
    dcterms:modified "2025-08-05T22:48:08.466000+00:00"^^xsd:dateTime ;
    skos:broader asced:0803 ;
    skos:definition "Hospitality Management is the study of managing the operations of organisations which provide hospitality services. It includes conference and special events management." ;
    skos:example "equipment and facilities planning, hospitality purchasing, rooms division management, strategic planning in hospitality" ;
    skos:inScheme ascedcs: ;
    skos:notation "080319" ;
    skos:prefLabel "Hospitality Management"@en .

asced:080321 a skos:Concept ;
    dcterms:created "2025-08-01T01:49:08.130000+00:00"^^xsd:dateTime ;
    dcterms:modified "2025-08-05T22:48:08.501000+00:00"^^xsd:dateTime ;
    skos:broader asced:0803 ;
    skos:definition "Farm Management and Agribusiness is the study of managing farming and agricultural business enterprises." ;
    skos:example "farm and agribusiness planning models, farm cash, credit, debt and taxation management, rural credit market" ;
    skos:inScheme ascedcs: ;
    skos:notation "080321" ;
    skos:prefLabel "Farm Management and Agribusiness"@en .

asced:080323 a skos:Concept ;
    dcterms:created "2025-08-01T01:49:08.130000+00:00"^^xsd:dateTime ;
    dcterms:modified "2025-08-05T22:48:08.536000+00:00"^^xsd:dateTime ;
    skos:broader asced:0803 ;
    skos:definition "Tourism Management is the study of planning and managing the activities of tourism focused enterprises." ;
    skos:example "cultural and social aspects of tourism management, tourist behaviour, tourism planning and development" ;
    skos:inScheme ascedcs: ;
    skos:notation "080323" ;
    skos:prefLabel "Tourism Management"@en ;
    skos:scopeNote "Exclusions: Tourism. This is included in Detailed Field 080701 Tourism." .

asced:080399 a skos:Concept ;
    dcterms:created "2025-08-01T01:49:08.131000+00:00"^^xsd:dateTime ;
    dcterms:modified "2025-08-05T22:48:08.571000+00:00"^^xsd:dateTime ;
    skos:broader asced:0803 ;
    skos:definition "This detailed field includes all Business and Management not elsewhere classified." ;
    skos:example "facilities management, recreation management, electronic commerce (e-commerce), business and financial risk management, transport management, emergency management" ;
    skos:inScheme ascedcs: ;
    skos:notation "080399" ;
    skos:prefLabel "Business and Management, n.e.c."@en .

asced:080501 a skos:Concept ;
    dcterms:created "2025-08-01T01:49:08.133000+00:00"^^xsd:dateTime ;
    dcterms:modified "2025-08-05T22:48:08.608000+00:00"^^xsd:dateTime ;
    skos:broader asced:0805 ;
    skos:definition "Sales is the study of buying and selling goods and services." ;
    skos:example "consumer behaviour, sales systems and procedures, selling techniques, stock management, wholesaling" ;
    skos:inScheme ascedcs: ;
    skos:notation "080501" ;
    skos:prefLabel "Sales"@en .

asced:080503 a skos:Concept ;
    dcterms:created "2025-08-01T01:49:08.133000+00:00"^^xsd:dateTime ;
    dcterms:modified "2025-08-05T22:48:08.657000+00:00"^^xsd:dateTime ;
    skos:broader asced:0805 ;
    skos:definition "Real Estate is the study of developing, purchasing, leasing and selling buildings, businesses and properties." ;
    skos:example "property appraisal, commercial and industrial leasing, strata management, residential tenancies, property management" ;
    skos:inScheme ascedcs: ;
    skos:notation "080503" ;
    skos:prefLabel "Real Estate"@en ;
    skos:scopeNote "Exclusions: Real estate valuation. This is included in Detailed Field 089903 Valuation. Real estate law. This is included in Detailed Field 090901 Business and Commercial Law." .

asced:080505 a skos:Concept ;
    dcterms:created "2025-08-01T01:49:08.134000+00:00"^^xsd:dateTime ;
    dcterms:modified "2025-08-05T22:48:08.695000+00:00"^^xsd:dateTime ;
    skos:broader asced:0805 ;
    skos:definition "Marketing is the study of identifying market opportunities and developing and implementing strategies for pricing and promoting products and services." ;
    skos:example "direct marketing, product innovation, sponsorship, market segmentation, consumer and organisational buyer behaviour" ;
    skos:inScheme ascedcs: ;
    skos:notation "080505" ;
    skos:prefLabel "Marketing"@en .

asced:080507 a skos:Concept ;
    dcterms:created "2025-08-01T01:49:08.134000+00:00"^^xsd:dateTime ;
    dcterms:modified "2025-08-05T22:48:08.730000+00:00"^^xsd:dateTime ;
    skos:broader asced:0805 ;
    skos:definition "Advertising is the study of informing potential customers of the nature of products and services and their merits." ;
    skos:example "advertising media, advertising regulations, ethical and operational principles in advertising, advertising strategies, planning and executing advertising campaigns" ;
    skos:inScheme ascedcs: ;
    skos:notation "080507" ;
    skos:prefLabel "Advertising"@en ;
    skos:scopeNote "Exclusions: Copywriting. This is included in Detailed Field 100705 Written Communication." .

asced:080509 a skos:Concept ;
    dcterms:created "2025-08-01T01:49:08.135000+00:00"^^xsd:dateTime ;
    dcterms:modified "2025-08-05T22:48:08.776000+00:00"^^xsd:dateTime ;
    skos:broader asced:0805 ;
    skos:definition "Public Relations is the study of creating and maintaining an understanding and a favourable view of an organisation and its products, services and role." ;
    skos:example "public relations campaign planning, international public relations, media relations, role of organisations' spokespersons" ;
    skos:inScheme ascedcs: ;
    skos:notation "080509" ;
    skos:prefLabel "Public Relations"@en .

asced:080599 a skos:Concept ;
    dcterms:created "2025-08-01T01:49:08.136000+00:00"^^xsd:dateTime ;
    dcterms:modified "2025-08-05T22:48:08.819000+00:00"^^xsd:dateTime ;
    skos:broader asced:0805 ;
    skos:definition "This detailed field includes all Sales and Marketing not elsewhere classified." ;
    skos:example "visual merchandising (window dressing), auctioneering" ;
    skos:inScheme ascedcs: ;
    skos:notation "080599" ;
    skos:prefLabel "Sales and Marketing, n.e.c."@en .

asced:080701 a skos:Concept ;
    dcterms:created "2025-08-01T01:49:08.137000+00:00"^^xsd:dateTime ;
    dcterms:modified "2025-08-05T22:48:08.865000+00:00"^^xsd:dateTime ;
    skos:broader asced:0807 ;
    skos:definition "Tourism is the study of the structure and operations of the tourism industry, tour guiding, and ticketing and reservation practices." ;
    skos:example "accommodation and travel reservations, ecotourism, fares and ticketing, tourist attractions and itinerary preparation, travel agency procedures, charter tours" ;
    skos:inScheme ascedcs: ;
    skos:notation "080701" ;
    skos:prefLabel "Tourism"@en .

asced:080901 a skos:Concept ;
    dcterms:created "2025-08-01T01:49:08.139000+00:00"^^xsd:dateTime ;
    dcterms:modified "2025-08-05T22:48:08.922000+00:00"^^xsd:dateTime ;
    skos:broader asced:0809 ;
    skos:definition "Secretarial and Clerical Studies is the study of shorthand, record keeping, correspondence and general office procedures." ;
    skos:example "business correspondence, filing, office equipment operation, performing general office procedures, shorthand, telephone operation" ;
    skos:inScheme ascedcs: ;
    skos:notation "080901" ;
    skos:prefLabel "Secretarial and Clerical Studies"@en .

asced:080903 a skos:Concept ;
    dcterms:created "2025-08-01T01:49:08.139000+00:00"^^xsd:dateTime ;
    dcterms:modified "2025-08-05T22:48:08.972000+00:00"^^xsd:dateTime ;
    skos:broader asced:0809 ;
    skos:definition "Keyboard Skills is the study of typing and data entry." ;
    skos:example "court reporting, data entry, keyboard operations and techniques, keyboard speed and accuracy" ;
    skos:inScheme ascedcs: ;
    skos:notation "080903" ;
    skos:prefLabel "Keyboard Skills"@en .

asced:080905 a skos:Concept ;
    dcterms:created "2025-08-01T01:49:08.140000+00:00"^^xsd:dateTime ;
    dcterms:modified "2025-08-05T22:48:09.018000+00:00"^^xsd:dateTime ;
    skos:broader asced:0809 ;
    skos:definition "Practical Computing Skills is the study of basic computer operation and using software packages." ;
    skos:example "financial management and planning software, introduction to the web, presentation packages, relational database software, spreadsheet packages, word processing packages" ;
    skos:inScheme ascedcs: ;
    skos:notation "080905" ;
    skos:prefLabel "Practical Computing Skills"@en .

asced:080999 a skos:Concept ;
    dcterms:created "2025-08-01T01:49:08.140000+00:00"^^xsd:dateTime ;
    dcterms:modified "2025-08-05T22:48:09.061000+00:00"^^xsd:dateTime ;
    skos:broader asced:0809 ;
    skos:definition "This detailed field includes all Office Studies not elsewhere classified." ;
    skos:example "reception protocol" ;
    skos:inScheme ascedcs: ;
    skos:notation "080999" ;
    skos:prefLabel "Office Studies, n.e.c."@en .

asced:081101 a skos:Concept ;
    dcterms:created "2025-08-01T01:49:08.141000+00:00"^^xsd:dateTime ;
    dcterms:modified "2025-08-05T22:48:09.144000+00:00"^^xsd:dateTime ;
    skos:broader asced:0811 ;
    skos:definition "Banking and Finance is the study of directing, planning and providing financial institution services in relation to savings and loans." ;
    skos:example "banking and lending practices, basic financial services, bank and financial institutions daily operations, finance theories, national and international financial markets regulations" ;
    skos:inScheme ascedcs: ;
    skos:notation "081101" ;
    skos:prefLabel "Banking and Finance"@en ;
    skos:scopeNote "Exclusions: Banking and financial law. This is included in Detailed Field 090901 Business and Commercial Law." .

asced:081103 a skos:Concept ;
    dcterms:created "2025-08-01T01:49:08.142000+00:00"^^xsd:dateTime ;
    dcterms:modified "2025-08-05T22:48:09.207000+00:00"^^xsd:dateTime ;
    skos:broader asced:0811 ;
    skos:definition "Insurance and Actuarial Studies is the study of directing, planning and providing insurance services, and applying mathematical and statistical analysis to financial planning problems." ;
    skos:example "principles of risk and insurance, insurance portfolio management, developing appropriate insurance packages for clients, actuarial principles" ;
    skos:inScheme ascedcs: ;
    skos:notation "081103" ;
    skos:prefLabel "Insurance and Actuarial Studies"@en .

asced:081105 a skos:Concept ;
    dcterms:created "2025-08-01T01:49:08.143000+00:00"^^xsd:dateTime ;
    dcterms:modified "2025-08-05T22:48:09.264000+00:00"^^xsd:dateTime ;
    skos:broader asced:0811 ;
    skos:definition "Investment and Securities is the study of directing, planning and providing investment and securities services." ;
    skos:example "tailoring individual investment portfolios, investments and financial markets regulations, superannuation and retirement planning" ;
    skos:inScheme ascedcs: ;
    skos:notation "081105" ;
    skos:prefLabel "Investment and Securities"@en .

asced:081199 a skos:Concept ;
    dcterms:created "2025-08-01T01:49:08.143000+00:00"^^xsd:dateTime ;
    dcterms:modified "2025-08-05T22:48:09.316000+00:00"^^xsd:dateTime ;
    skos:broader asced:0811 ;
    skos:definition "This detailed field includes all Banking, Finance and Related Fields not elsewhere classified." ;
    skos:example "financial management" ;
    skos:inScheme ascedcs: ;
    skos:notation "081199" ;
    skos:prefLabel "Banking, Finance and Related Fields, n.e.c."@en .

asced:089901 a skos:Concept ;
    dcterms:created "2025-08-01T01:49:08.144000+00:00"^^xsd:dateTime ;
    dcterms:modified "2025-08-05T22:48:09.369000+00:00"^^xsd:dateTime ;
    skos:broader asced:0899 ;
    skos:definition "Purchasing, Warehousing and Distribution is the study of purchasing, supplying, storing and despatching goods and other materials." ;
    skos:example "materials handling and management, inventory control, staged procurement, logistics management, transport and distribution systems, warehouse storage systems, furniture removal" ;
    skos:inScheme ascedcs: ;
    skos:notation "089901" ;
    skos:prefLabel "Purchasing, Warehousing and Distribution"@en .

asced:089903 a skos:Concept ;
    dcterms:created "2025-08-01T01:49:08.145000+00:00"^^xsd:dateTime ;
    dcterms:modified "2025-08-05T22:48:09.422000+00:00"^^xsd:dateTime ;
    skos:broader asced:0899 ;
    skos:definition "Valuation is the study of valuing land, buildings, businesses, properties, machinery, art and personal items." ;
    skos:example "plant and equipment valuation, land economics, specialist valuation, valuation for rating and taxing" ;
    skos:inScheme ascedcs: ;
    skos:notation "089903" ;
    skos:prefLabel "Valuation"@en .

asced:089999 a skos:Concept ;
    dcterms:created "2025-08-01T01:49:08.145000+00:00"^^xsd:dateTime ;
    dcterms:modified "2025-08-05T22:48:09.471000+00:00"^^xsd:dateTime ;
    skos:broader asced:0899 ;
    skos:definition "This detailed field includes all Management and Commerce not elsewhere classified." ;
    skos:example "laboratory administration, wool commerce" ;
    skos:inScheme ascedcs: ;
    skos:notation "089999" ;
    skos:prefLabel "Management and Commerce, n.e.c."@en .

asced:090101 a skos:Concept ;
    dcterms:created "2025-08-01T01:49:08.147000+00:00"^^xsd:dateTime ;
    dcterms:modified "2025-08-05T22:48:10.181000+00:00"^^xsd:dateTime ;
    skos:broader asced:0901 ;
    skos:definition "Political Science is the study of political ideas, processes, institutions and behaviour, and how they influence public decisions within and among communities." ;
    skos:example "business-government relations, comparative political systems, electoral behaviour, international relations, political ideologies" ;
    skos:inScheme ascedcs: ;
    skos:notation "090101" ;
    skos:prefLabel "Political Science"@en .

asced:090103 a skos:Concept ;
    dcterms:created "2025-08-01T01:49:08.148000+00:00"^^xsd:dateTime ;
    dcterms:modified "2025-08-05T22:48:10.229000+00:00"^^xsd:dateTime ;
    skos:broader asced:0901 ;
    skos:definition "Policy Studies is the study of analysing and developing policies to achieve societal and corporate goals." ;
    skos:example "Australian foreign policy, socio-environmental policy, public policy development, regional development policy, social policy analysis" ;
    skos:inScheme ascedcs: ;
    skos:notation "090103" ;
    skos:prefLabel "Policy Studies"@en .

asced:090301 a skos:Concept ;
    dcterms:created "2025-08-01T01:49:08.149000+00:00"^^xsd:dateTime ;
    dcterms:modified "2025-08-05T22:48:10.277000+00:00"^^xsd:dateTime ;
    skos:broader asced:0903 ;
    skos:definition "Sociology is the study of the origin, development, organisation and functioning of human society, including the study of the patterns of social relations." ;
    skos:example "social control, social inequalities, social interaction, sociological theory, sociology of education, social structure" ;
    skos:inScheme ascedcs: ;
    skos:notation "090301" ;
    skos:prefLabel "Sociology"@en .

asced:090303 a skos:Concept ;
    dcterms:created "2025-08-01T01:49:08.149000+00:00"^^xsd:dateTime ;
    dcterms:modified "2025-08-05T22:48:10.318000+00:00"^^xsd:dateTime ;
    skos:broader asced:0903 ;
    skos:definition "Anthropology is the study of the diversity of human cultural practices and beliefs by participant observation and comparison." ;
    skos:example "anthropology of development, cultural studies, ethnography, ethnology, evolution of human culture, kinship, transformation of traditional societies" ;
    skos:inScheme ascedcs: ;
    skos:notation "090303" ;
    skos:prefLabel "Anthropology"@en .

asced:090305 a skos:Concept ;
    dcterms:created "2025-08-01T01:49:08.150000+00:00"^^xsd:dateTime ;
    dcterms:modified "2025-08-05T22:48:10.360000+00:00"^^xsd:dateTime ;
    skos:broader asced:0903 ;
    skos:definition "History is the study of past cultures, events and ideas using written documents and other evidence." ;
    skos:example "perspectives on the past, film and history, history through monuments, contemporary world history" ;
    skos:inScheme ascedcs: ;
    skos:notation "090305" ;
    skos:prefLabel "History"@en .

asced:090307 a skos:Concept ;
    dcterms:created "2025-08-01T01:49:08.150000+00:00"^^xsd:dateTime ;
    dcterms:modified "2025-08-05T22:48:10.400000+00:00"^^xsd:dateTime ;
    skos:broader asced:0903 ;
    skos:definition "Archaeology is the study of human history and prehistory through the excavation of sites and the analysis of artefacts and other physical remains." ;
    skos:example "archaeological data, archaeological methods and techniques, archaeological theories" ;
    skos:inScheme ascedcs: ;
    skos:notation "090307" ;
    skos:prefLabel "Archaeology"@en .

asced:090309 a skos:Concept ;
    dcterms:created "2025-08-01T01:49:08.151000+00:00"^^xsd:dateTime ;
    dcterms:modified "2025-08-05T22:48:10.442000+00:00"^^xsd:dateTime ;
    skos:broader asced:0903 ;
    skos:definition "Human Geography is the study of spatial variations between human populations and the interactions between people and their environment." ;
    skos:example "human activity and environmental change, demography, human community development theory and practice, globalisation" ;
    skos:inScheme ascedcs: ;
    skos:notation "090309" ;
    skos:prefLabel "Human Geography"@en .

asced:090311 a skos:Concept ;
    dcterms:created "2025-08-01T01:49:08.152000+00:00"^^xsd:dateTime ;
    dcterms:modified "2025-08-05T22:48:10.485000+00:00"^^xsd:dateTime ;
    skos:broader asced:0903 ;
    skos:definition "Indigenous Studies is the study of indigenous culture and societies and their relationship to the broader society of a particular country." ;
    skos:example "comparative indigenous studies, contemporary indigenous studies, indigenous cultures" ;
    skos:inScheme ascedcs: ;
    skos:notation "090311" ;
    skos:prefLabel "Indigenous Studies"@en .

asced:090313 a skos:Concept ;
    dcterms:created "2025-08-01T01:49:08.153000+00:00"^^xsd:dateTime ;
    dcterms:modified "2025-08-05T22:48:10.528000+00:00"^^xsd:dateTime ;
    skos:broader asced:0903 ;
    skos:definition "Gender Specific Studies is the study of the ways that people and society develop various ideas and beliefs concerning the roles and functions of a specific gender and the way that this gender relates to society." ;
    skos:example "feminist theory, gender and power, gender issues, historical perspectives on gender issues, women's studies" ;
    skos:inScheme ascedcs: ;
    skos:notation "090313" ;
    skos:prefLabel "Gender Specific Studies"@en .

asced:090399 a skos:Concept ;
    dcterms:created "2025-08-01T01:49:08.153000+00:00"^^xsd:dateTime ;
    dcterms:modified "2025-08-05T22:48:10.572000+00:00"^^xsd:dateTime ;
    skos:broader asced:0903 ;
    skos:definition "This detailed field includes all Studies in Human Society not elsewhere classified." ;
    skos:example "peace studies, multicultural studies, modern studies" ;
    skos:inScheme ascedcs: ;
    skos:notation "090399" ;
    skos:prefLabel "Studies in Human Society, n.e.c."@en .

asced:090501 a skos:Concept ;
    dcterms:created "2025-08-01T01:49:08.154000+00:00"^^xsd:dateTime ;
    dcterms:modified "2025-08-05T22:48:10.619000+00:00"^^xsd:dateTime ;
    skos:broader asced:0905 ;
    skos:definition "Social Work is the study of promoting, restoring, maintaining and enhancing the functioning of individuals, families, social groups, organisations and communities by the utilisation of resources within individuals and the social environment in order to alleviate social problems." ;
    skos:example "agency intervention, crisis intervention, social work analysis, social work theory" ;
    skos:inScheme ascedcs: ;
    skos:notation "090501" ;
    skos:prefLabel "Social Work"@en .

asced:090503 a skos:Concept ;
    dcterms:created "2025-08-01T01:49:08.155000+00:00"^^xsd:dateTime ;
    dcterms:modified "2025-08-05T22:48:10.688000+00:00"^^xsd:dateTime ;
    skos:broader asced:0905 ;
    skos:definition "Children's Services is the study of the care and development of children." ;
    skos:example "storytelling, infant and child care and development, early childhood research, understanding and guiding children's behaviour, play and learning environment" ;
    skos:inScheme ascedcs: ;
    skos:notation "090503" ;
    skos:prefLabel "Children's Services"@en .

asced:090505 a skos:Concept ;
    dcterms:created "2025-08-01T01:49:08.155000+00:00"^^xsd:dateTime ;
    dcterms:modified "2025-08-05T22:48:10.731000+00:00"^^xsd:dateTime ;
    skos:broader asced:0905 ;
    skos:definition "Youth Work is the study of the development and support of youth." ;
    skos:example "homeless youth, working with adolescents, perspectives on youth" ;
    skos:inScheme ascedcs: ;
    skos:notation "090505" ;
    skos:prefLabel "Youth Work"@en .

asced:090507 a skos:Concept ;
    dcterms:created "2025-08-01T01:49:08.156000+00:00"^^xsd:dateTime ;
    dcterms:modified "2025-08-05T22:48:10.774000+00:00"^^xsd:dateTime ;
    skos:broader asced:0905 ;
    skos:definition "Care for the Aged is the study of caring for elderly people in various social support services associated with families and groups in the community." ;
    skos:example "research techniques in gerontology, quality of life and welfare of the well and frail aged, working with dementia" ;
    skos:inScheme ascedcs: ;
    skos:notation "090507" ;
    skos:prefLabel "Care for the Aged"@en .

asced:090509 a skos:Concept ;
    dcterms:created "2025-08-01T01:49:08.156000+00:00"^^xsd:dateTime ;
    dcterms:modified "2025-08-05T22:48:10.815000+00:00"^^xsd:dateTime ;
    skos:broader asced:0905 ;
    skos:definition "Care for the Disabled is the study of caring for disabled people in various social support services associated with families and groups in the community." ;
    skos:example "augmentative communication systems, disability and development, supporting people with disability" ;
    skos:inScheme ascedcs: ;
    skos:notation "090509" ;
    skos:prefLabel "Care for the Disabled"@en .

asced:090511 a skos:Concept ;
    dcterms:created "2025-08-01T01:49:08.157000+00:00"^^xsd:dateTime ;
    dcterms:modified "2025-08-05T22:48:10.856000+00:00"^^xsd:dateTime ;
    skos:broader asced:0905 ;
    skos:definition "Residential Client Care is the study of caring for people living in a variety of welfare and residential settings." ;
    skos:example "principles and practices of residential client care service provision, residential and community services theory" ;
    skos:inScheme ascedcs: ;
    skos:notation "090511" ;
    skos:prefLabel "Residential Client Care"@en .

asced:090513 a skos:Concept ;
    dcterms:created "2025-08-01T01:49:08.158000+00:00"^^xsd:dateTime ;
    dcterms:modified "2025-08-05T22:48:10.894000+00:00"^^xsd:dateTime ;
    skos:broader asced:0905 ;
    skos:definition "Counselling is the study of the practice and skills required to provide guidance on personal, social and psychological problems." ;
    skos:example "conflict resolution skills, developmental counselling models, theories of counselling, career guidance" ;
    skos:inScheme ascedcs: ;
    skos:notation "090513" ;
    skos:prefLabel "Counselling"@en .

asced:090515 a skos:Concept ;
    dcterms:created "2025-08-01T01:49:08.158000+00:00"^^xsd:dateTime ;
    dcterms:modified "2025-08-05T22:48:10.942000+00:00"^^xsd:dateTime ;
    skos:broader asced:0905 ;
    skos:definition "Welfare Studies is the study of providing personal services to individuals and family groups who are socially disadvantaged or otherwise in need." ;
    skos:example "community and welfare studies, community resource identification and use, human service organisation, interaction of welfare services and law, paradigms of welfare practice" ;
    skos:inScheme ascedcs: ;
    skos:notation "090515" ;
    skos:prefLabel "Welfare Studies"@en .

asced:090599 a skos:Concept ;
    dcterms:created "2025-08-01T01:49:08.159000+00:00"^^xsd:dateTime ;
    dcterms:modified "2025-08-05T22:48:10.980000+00:00"^^xsd:dateTime ;
    skos:broader asced:0905 ;
    skos:definition "This detailed field includes all Human Welfare Studies and Services not elsewhere classified." ;
    skos:example "drug dependence studies, community care, family support, community development" ;
    skos:inScheme ascedcs: ;
    skos:notation "090599" ;
    skos:prefLabel "Human Welfare Studies and Services, n.e.c."@en .

asced:090701 a skos:Concept ;
    dcterms:created "2025-08-01T01:49:08.160000+00:00"^^xsd:dateTime ;
    dcterms:modified "2025-08-05T22:48:11.020000+00:00"^^xsd:dateTime ;
    skos:broader asced:0907 ;
    skos:definition "Psychology is the study of the science of human nature and of mental states and processes. It includes the study of human and animal nature." ;
    skos:example "research methods in psychology, behaviourism, personality theory and assessment, psychotherapy" ;
    skos:inScheme ascedcs: ;
    skos:notation "090701" ;
    skos:prefLabel "Psychology"@en .

asced:090799 a skos:Concept ;
    dcterms:created "2025-08-01T01:49:08.160000+00:00"^^xsd:dateTime ;
    dcterms:modified "2025-08-05T22:48:11.064000+00:00"^^xsd:dateTime ;
    skos:broader asced:0907 ;
    skos:definition "This detailed field includes all Behavioural Science not elsewhere classified." ;
    skos:example "cognitive science, behavioural health studies, neuro-linguistic programming" ;
    skos:inScheme ascedcs: ;
    skos:notation "090799" ;
    skos:prefLabel "Behavioural Science, n.e.c."@en .

asced:090901 a skos:Concept ;
    dcterms:created "2025-08-01T01:49:08.161000+00:00"^^xsd:dateTime ;
    dcterms:modified "2025-08-05T22:48:11.103000+00:00"^^xsd:dateTime ;
    skos:broader asced:0909 ;
    skos:definition "Business and Commercial Law is the study of the principles and regulations governing business and commercial practices." ;
    skos:example "company law, consumer legislation, corporate solvency, conveyancing, regulation of securities" ;
    skos:inScheme ascedcs: ;
    skos:notation "090901" ;
    skos:prefLabel "Business and Commercial Law"@en .

asced:090903 a skos:Concept ;
    dcterms:created "2025-08-01T01:49:08.162000+00:00"^^xsd:dateTime ;
    dcterms:modified "2025-08-05T22:48:11.141000+00:00"^^xsd:dateTime ;
    skos:broader asced:0909 ;
    skos:definition "Constitutional Law is the study of the principles and regulations in relation to the constitution and the respective powers of the federal and state governments." ;
    skos:example "constitutional interpretation, constitutional development, amendments and reform, legislative powers, federalism" ;
    skos:inScheme ascedcs: ;
    skos:notation "090903" ;
    skos:prefLabel "Constitutional Law"@en .

asced:090905 a skos:Concept ;
    dcterms:created "2025-08-01T01:49:08.163000+00:00"^^xsd:dateTime ;
    dcterms:modified "2025-08-05T22:48:11.179000+00:00"^^xsd:dateTime ;
    skos:broader asced:0909 ;
    skos:definition "Criminal Law is the study of the principles and practices associated with the body of law which deals with criminal offences." ;
    skos:example "criminal defences, standards of proof, criminal liability, mens rea and actus reus" ;
    skos:inScheme ascedcs: ;
    skos:notation "090905" ;
    skos:prefLabel "Criminal Law"@en .

asced:090907 a skos:Concept ;
    dcterms:created "2025-08-01T01:49:08.163000+00:00"^^xsd:dateTime ;
    dcterms:modified "2025-08-05T22:48:11.222000+00:00"^^xsd:dateTime ;
    skos:broader asced:0909 ;
    skos:definition "Family Law is the study of the principles and regulations in relation to the family." ;
    skos:example "legal regulation of family formation and breakdown, legal regulation of de facto relationships, rights of children, adoption" ;
    skos:inScheme ascedcs: ;
    skos:notation "090907" ;
    skos:prefLabel "Family Law"@en .

asced:090909 a skos:Concept ;
    dcterms:created "2025-08-01T01:49:08.164000+00:00"^^xsd:dateTime ;
    dcterms:modified "2025-08-05T22:48:11.258000+00:00"^^xsd:dateTime ;
    skos:broader asced:0909 ;
    skos:definition "International Law is the study of the system of rules governing the conduct of international relations, and the relationship between Australian laws and the laws of other countries." ;
    skos:example "domestic and international law, international trade law, public and private international law, international dispute resolution, treaties" ;
    skos:inScheme ascedcs: ;
    skos:notation "090909" ;
    skos:prefLabel "International Law"@en .

asced:090911 a skos:Concept ;
    dcterms:created "2025-08-01T01:49:08.164000+00:00"^^xsd:dateTime ;
    dcterms:modified "2025-08-05T22:48:11.294000+00:00"^^xsd:dateTime ;
    skos:broader asced:0909 ;
    skos:definition "Taxation Law is the study of principles and regulations related to government collection of revenues from corporate and individual tax payers." ;
    skos:example "Australian taxation system, revenue collection mechanisms, income taxation regulations" ;
    skos:inScheme ascedcs: ;
    skos:notation "090911" ;
    skos:prefLabel "Taxation Law"@en .

asced:090913 a skos:Concept ;
    dcterms:created "2025-08-01T01:49:08.165000+00:00"^^xsd:dateTime ;
    dcterms:modified "2025-08-05T22:48:11.329000+00:00"^^xsd:dateTime ;
    skos:broader asced:0909 ;
    skos:definition "Legal Practice is the study of the issues associated with practising law. It includes the methods and principles involved in advising and representing clients on matters relating to law." ;
    skos:example "professional code of practice, rules and etiquette of professional practice" ;
    skos:inScheme ascedcs: ;
    skos:notation "090913" ;
    skos:prefLabel "Legal Practice"@en .

asced:090999 a skos:Concept ;
    dcterms:created "2025-08-01T01:49:08.165000+00:00"^^xsd:dateTime ;
    dcterms:modified "2025-08-05T22:48:11.366000+00:00"^^xsd:dateTime ;
    skos:broader asced:0909 ;
    skos:definition "This detailed field includes all Law not elsewhere classified." ;
    skos:example "administrative law" ;
    skos:inScheme ascedcs: ;
    skos:notation "090999" ;
    skos:prefLabel "Law, n.e.c."@en .

asced:091101 a skos:Concept ;
    dcterms:created "2025-08-01T01:49:08.167000+00:00"^^xsd:dateTime ;
    dcterms:modified "2025-08-05T22:48:11.401000+00:00"^^xsd:dateTime ;
    skos:broader asced:0911 ;
    skos:definition "Justice Administration is the study of the theory and practice of the administrative processes in the justice system." ;
    skos:example "confessional evidence, criminal justice, court operation" ;
    skos:inScheme ascedcs: ;
    skos:notation "091101" ;
    skos:prefLabel "Justice Administration"@en .

asced:091103 a skos:Concept ;
    dcterms:created "2025-08-01T01:49:08.167000+00:00"^^xsd:dateTime ;
    dcterms:modified "2025-08-05T22:48:11.440000+00:00"^^xsd:dateTime ;
    skos:broader asced:0911 ;
    skos:definition "Legal Studies is the study of the administrative and legal skills required to assist in legal practice." ;
    skos:example "basic principles of law, legal documentation, legal library operations and utilisation, legal records" ;
    skos:inScheme ascedcs: ;
    skos:notation "091103" ;
    skos:prefLabel "Legal Studies"@en ;
    skos:scopeNote "Exclusions: Legal secretarial studies. This is included in Detailed Field 080901 Secretarial and Clerical Studies." .

asced:091105 a skos:Concept ;
    dcterms:created "2025-08-01T01:49:08.168000+00:00"^^xsd:dateTime ;
    dcterms:modified "2025-08-05T22:48:11.482000+00:00"^^xsd:dateTime ;
    skos:broader asced:0911 ;
    skos:definition "Police Studies is the study of the maintenance of law and order, and crime detection and prevention." ;
    skos:example "police administration, police investigation techniques, police regulations, police supervision techniques" ;
    skos:inScheme ascedcs: ;
    skos:notation "091105" ;
    skos:prefLabel "Police Studies"@en .

asced:091199 a skos:Concept ;
    dcterms:created "2025-08-01T01:49:08.168000+00:00"^^xsd:dateTime ;
    dcterms:modified "2025-08-05T22:48:11.520000+00:00"^^xsd:dateTime ;
    skos:broader asced:0911 ;
    skos:definition "This detailed field includes all Justice and Law Enforcement not elsewhere classified." ;
    skos:example "correctional studies" ;
    skos:inScheme ascedcs: ;
    skos:notation "091199" ;
    skos:prefLabel "Justice and Law Enforcement, n.e.c."@en .

asced:091301 a skos:Concept ;
    dcterms:created "2025-08-01T01:49:08.169000+00:00"^^xsd:dateTime ;
    dcterms:modified "2025-08-05T22:48:11.556000+00:00"^^xsd:dateTime ;
    skos:broader asced:0913 ;
    skos:definition "Librarianship and Information Management is the study of selecting, acquiring, organising and storing collections of information, and facilitating the use of information." ;
    skos:example "archival studies, cataloguing and classifications, collection management, information retrieval and dissemination, library administration, records management" ;
    skos:inScheme ascedcs: ;
    skos:notation "091301" ;
    skos:prefLabel "Librarianship and Information Management"@en .

asced:091303 a skos:Concept ;
    dcterms:created "2025-08-01T01:49:08.170000+00:00"^^xsd:dateTime ;
    dcterms:modified "2025-08-05T22:48:11.592000+00:00"^^xsd:dateTime ;
    skos:broader asced:0913 ;
    skos:definition "Curatorial Studies is the study of locating, identifying and assessing cultural heritage resources." ;
    skos:example "conservation of objects, exhibition planning, museography, museology" ;
    skos:inScheme ascedcs: ;
    skos:notation "091303" ;
    skos:prefLabel "Curatorial Studies"@en .

asced:091501 a skos:Concept ;
    dcterms:created "2025-08-01T01:49:08.171000+00:00"^^xsd:dateTime ;
    dcterms:modified "2025-08-05T22:48:11.628000+00:00"^^xsd:dateTime ;
    skos:broader asced:0915 ;
    skos:definition "English Language is the study of reading, writing and speaking the English language." ;
    skos:example "English, English as a second language" ;
    skos:inScheme ascedcs: ;
    skos:notation "091501" ;
    skos:prefLabel "English Language"@en .

asced:091503 a skos:Concept ;
    dcterms:created "2025-08-01T01:49:08.172000+00:00"^^xsd:dateTime ;
    dcterms:modified "2025-08-05T22:48:11.667000+00:00"^^xsd:dateTime ;
    skos:broader asced:0915 ;
    skos:definition "Northern European Languages is the study of reading, writing and speaking the languages of Northern Europe." ;
    skos:example "Gaelic, Danish, Dutch, German, Norwegian, Swedish" ;
    skos:inScheme ascedcs: ;
    skos:notation "091503" ;
    skos:prefLabel "Northern European Languages"@en .

asced:091505 a skos:Concept ;
    dcterms:created "2025-08-01T01:49:08.172000+00:00"^^xsd:dateTime ;
    dcterms:modified "2025-08-05T22:48:11.703000+00:00"^^xsd:dateTime ;
    skos:broader asced:0915 ;
    skos:definition "Southern European Languages is the study of reading, writing and speaking the languages of Southern Europe." ;
    skos:example "French, Greek, Italian, Latin, Portuguese, Spanish" ;
    skos:inScheme ascedcs: ;
    skos:notation "091505" ;
    skos:prefLabel "Southern European Languages"@en .

asced:091507 a skos:Concept ;
    dcterms:created "2025-08-01T01:49:08.172000+00:00"^^xsd:dateTime ;
    dcterms:modified "2025-08-05T22:48:11.739000+00:00"^^xsd:dateTime ;
    skos:broader asced:0915 ;
    skos:definition "Eastern European Languages is the study of the reading, writing and speaking the languages of Eastern Europe." ;
    skos:example "Croatian, Finnish, Hungarian, Lithuanian, Russian, Serbian, Ukrainian" ;
    skos:inScheme ascedcs: ;
    skos:notation "091507" ;
    skos:prefLabel "Eastern European Languages"@en .

asced:091509 a skos:Concept ;
    dcterms:created "2025-08-01T01:49:08.173000+00:00"^^xsd:dateTime ;
    dcterms:modified "2025-08-05T22:48:11.781000+00:00"^^xsd:dateTime ;
    skos:broader asced:0915 ;
    skos:definition "Southwest Asian and North African Languages is the study of reading, writing and speaking the languages of Southwest Asia and North Africa." ;
    skos:example "Arabic, Persian, Hebrew, Kurdish, Iranian, Turkish" ;
    skos:inScheme ascedcs: ;
    skos:notation "091509" ;
    skos:prefLabel "Southwest Asian and North African Languages"@en .

asced:091511 a skos:Concept ;
    dcterms:created "2025-08-01T01:49:08.174000+00:00"^^xsd:dateTime ;
    dcterms:modified "2025-08-05T22:48:11.827000+00:00"^^xsd:dateTime ;
    skos:broader asced:0915 ;
    skos:definition "Southern Asian Languages is the study of reading, writing and speaking the languages of Southern Asia." ;
    skos:example "Bengali, Hindi, Nepali, Punjabi, Sinhalese, Tamil" ;
    skos:inScheme ascedcs: ;
    skos:notation "091511" ;
    skos:prefLabel "Southern Asian Languages"@en .

asced:091513 a skos:Concept ;
    dcterms:created "2025-08-01T01:49:08.174000+00:00"^^xsd:dateTime ;
    dcterms:modified "2025-08-05T22:48:11.873000+00:00"^^xsd:dateTime ;
    skos:broader asced:0915 ;
    skos:definition "Southeast Asian Languages is the study of reading, writing and speaking the languages of Southeast Asia." ;
    skos:example "Indonesian, Khmer, Lao, Malay, Thai, Vietnamese" ;
    skos:inScheme ascedcs: ;
    skos:notation "091513" ;
    skos:prefLabel "Southeast Asian Languages"@en .

asced:091515 a skos:Concept ;
    dcterms:created "2025-08-01T01:49:08.175000+00:00"^^xsd:dateTime ;
    dcterms:modified "2025-08-05T22:48:11.914000+00:00"^^xsd:dateTime ;
    skos:broader asced:0915 ;
    skos:definition "Eastern Asian Languages is the study of reading, writing and speaking the languages of Eastern Asia." ;
    skos:example "Cantonese, Japanese, Korean, Mandarin" ;
    skos:inScheme ascedcs: ;
    skos:notation "091515" ;
    skos:prefLabel "Eastern Asian Languages"@en .

asced:091517 a skos:Concept ;
    dcterms:created "2025-08-01T01:49:08.175000+00:00"^^xsd:dateTime ;
    dcterms:modified "2025-08-05T22:48:11.955000+00:00"^^xsd:dateTime ;
    skos:broader asced:0915 ;
    skos:definition "Australian Indigenous Languages is the study of reading, writing and speaking the languages of the Australian indigenous people." ;
    skos:example "Anindilyakwa, Anmatyerr (Anmatyirra), Arrernte (Aranda), Yindjibarndi, Meryam Mir, Pitjantjatjara" ;
    skos:inScheme ascedcs: ;
    skos:notation "091517" ;
    skos:prefLabel "Australian Indigenous Languages"@en .

asced:091519 a skos:Concept ;
    dcterms:created "2025-08-01T01:49:08.176000+00:00"^^xsd:dateTime ;
    dcterms:modified "2025-08-05T22:48:11.997000+00:00"^^xsd:dateTime ;
    skos:broader asced:0915 ;
    skos:definition "Translating and Interpreting is the study of translating and interpreting foreign languages into the mother tongue and vice versa." ;
    skos:example "interpreting, translating" ;
    skos:inScheme ascedcs: ;
    skos:notation "091519" ;
    skos:prefLabel "Translating and Interpreting"@en .

asced:091521 a skos:Concept ;
    dcterms:created "2025-08-01T01:49:08.176000+00:00"^^xsd:dateTime ;
    dcterms:modified "2025-08-05T22:48:12.034000+00:00"^^xsd:dateTime ;
    skos:broader asced:0915 ;
    skos:definition "Linguistics is the study of the structure and composition of language." ;
    skos:example "phonemics, phonetics, sociolinguistics, syntax" ;
    skos:inScheme ascedcs: ;
    skos:notation "091521" ;
    skos:prefLabel "Linguistics"@en .

asced:091523 a skos:Concept ;
    dcterms:created "2025-08-01T01:49:08.177000+00:00"^^xsd:dateTime ;
    dcterms:modified "2025-08-05T22:48:12.080000+00:00"^^xsd:dateTime ;
    skos:broader asced:0915 ;
    skos:definition "Literature is the study of written works valued for form of writing or expression." ;
    skos:example "dramatic scripts, fiction, non-fiction prose, poetry" ;
    skos:inScheme ascedcs: ;
    skos:notation "091523" ;
    skos:prefLabel "Literature"@en .

asced:091599 a skos:Concept ;
    dcterms:created "2025-08-01T01:49:08.177000+00:00"^^xsd:dateTime ;
    dcterms:modified "2025-08-05T22:48:12.124000+00:00"^^xsd:dateTime ;
    skos:broader asced:0915 ;
    skos:definition "This detailed field includes all Language and Literature not elsewhere classified." ;
    skos:example "deaf studies, AUSLAN" ;
    skos:inScheme ascedcs: ;
    skos:notation "091599" ;
    skos:prefLabel "Language and Literature, n.e.c."@en .

asced:091701 a skos:Concept ;
    dcterms:created "2025-08-01T01:49:08.178000+00:00"^^xsd:dateTime ;
    dcterms:modified "2025-08-05T22:48:12.171000+00:00"^^xsd:dateTime ;
    skos:broader asced:0917 ;
    skos:definition "Philosophy is the study of the fundamental nature of knowledge, reality and existence." ;
    skos:example "empiricism and rationalism, epistemology, ethics, formal logic, metaphysics, ontology" ;
    skos:inScheme ascedcs: ;
    skos:notation "091701" ;
    skos:prefLabel "Philosophy"@en .

asced:091703 a skos:Concept ;
    dcterms:created "2025-08-01T01:49:08.179000+00:00"^^xsd:dateTime ;
    dcterms:modified "2025-08-05T22:48:12.221000+00:00"^^xsd:dateTime ;
    skos:broader asced:0917 ;
    skos:definition "Religious Studies is the study of a set of beliefs and practices, usually involving acknowledgement of a divine or higher being or power, by which people order the conduct of their lives both practically and in a moral sense." ;
    skos:example "biblical studies, comparative religion, spirituality, theology" ;
    skos:inScheme ascedcs: ;
    skos:notation "091703" ;
    skos:prefLabel "Religious Studies"@en .

asced:091901 a skos:Concept ;
    dcterms:created "2025-08-01T01:49:08.181000+00:00"^^xsd:dateTime ;
    dcterms:modified "2025-08-05T22:48:12.273000+00:00"^^xsd:dateTime ;
    skos:broader asced:0919 ;
    skos:definition "Economics is the study of the production, consumption and transfer of wealth." ;
    skos:example "economic change and development, macroeconomic theory, microeconomic theory" ;
    skos:inScheme ascedcs: ;
    skos:notation "091901" ;
    skos:prefLabel "Economics"@en .

asced:091903 a skos:Concept ;
    dcterms:created "2025-08-01T01:49:08.181000+00:00"^^xsd:dateTime ;
    dcterms:modified "2025-08-05T22:48:12.319000+00:00"^^xsd:dateTime ;
    skos:broader asced:0919 ;
    skos:definition "Econometrics is the study of analysing and describing economic data using mathematical and statistical methods." ;
    skos:example "cross-sectional analysis, economic models and forecasting, financial econometrics" ;
    skos:inScheme ascedcs: ;
    skos:notation "091903" ;
    skos:prefLabel "Econometrics"@en .

asced:092101 a skos:Concept ;
    dcterms:created "2025-08-01T01:49:08.182000+00:00"^^xsd:dateTime ;
    dcterms:modified "2025-08-05T22:48:12.364000+00:00"^^xsd:dateTime ;
    skos:broader asced:0921 ;
    skos:definition "Sport and Recreation Activities is the study of the theory and practice of participating in various sporting and recreational activities." ;
    skos:example "individual sports, outdoor recreation and adventure based activities, team sports" ;
    skos:inScheme ascedcs: ;
    skos:notation "092101" ;
    skos:prefLabel "Sport and Recreation Activities"@en .

asced:092103 a skos:Concept ;
    dcterms:created "2025-08-01T01:49:08.183000+00:00"^^xsd:dateTime ;
    dcterms:modified "2025-08-05T22:48:12.409000+00:00"^^xsd:dateTime ;
    skos:broader asced:0921 ;
    skos:definition "Sports Coaching, Officiating and Instruction is the study of the techniques for coaching and instructing individuals and teams in various sporting activities. It includes studying the techniques of officiating at various sporting events." ;
    skos:example "fitness programme development, fitness training, recreation leadership, sport rules and regulations, coaching techniques and strategies" ;
    skos:inScheme ascedcs: ;
    skos:notation "092103" ;
    skos:prefLabel "Sports Coaching, Officiating and Instruction"@en ;
    skos:scopeNote "Exclusions: Sport psychology. This is included in Detailed Field 090701 Psychology." .

asced:092199 a skos:Concept ;
    dcterms:created "2025-08-01T01:49:08.183000+00:00"^^xsd:dateTime ;
    dcterms:modified "2025-08-05T22:48:12.456000+00:00"^^xsd:dateTime ;
    skos:broader asced:0921 ;
    skos:definition "This detailed field includes all Sport and Recreation not elsewhere classified." ;
    skos:example "recreation and leisure programme development" ;
    skos:inScheme ascedcs: ;
    skos:notation "092199" ;
    skos:prefLabel "Sport and Recreation, n.e.c."@en .

asced:099901 a skos:Concept ;
    dcterms:created "2025-08-01T01:49:08.184000+00:00"^^xsd:dateTime ;
    dcterms:modified "2025-08-05T22:48:12.497000+00:00"^^xsd:dateTime ;
    skos:broader asced:0999 ;
    skos:definition "Family and Consumer Studies is the study of the wellbeing of individuals and families and the way that they manage resources to achieve their goals." ;
    skos:example "consumer advocacy, consumer science, family economic wellbeing, home economics, technological impacts on consumers" ;
    skos:inScheme ascedcs: ;
    skos:notation "099901" ;
    skos:prefLabel "Family and Consumer Studies"@en .

asced:099903 a skos:Concept ;
    dcterms:created "2025-08-01T01:49:08.184000+00:00"^^xsd:dateTime ;
    dcterms:modified "2025-08-05T22:48:12.545000+00:00"^^xsd:dateTime ;
    skos:broader asced:0999 ;
    skos:definition "Criminology is the study of crime and issues related to offenders and victims." ;
    skos:example "corporate crime, crime prevention, criminal profiling, theories of criminal behaviour" ;
    skos:inScheme ascedcs: ;
    skos:notation "099903" ;
    skos:prefLabel "Criminology"@en ;
    skos:scopeNote "Exclusions: Forensic science. This is included in Detailed Field 019903 Forensic Science." .

asced:099905 a skos:Concept ;
    dcterms:created "2025-08-01T01:49:08.186000+00:00"^^xsd:dateTime ;
    dcterms:modified "2025-08-05T22:48:12.595000+00:00"^^xsd:dateTime ;
    skos:broader asced:0999 ;
    skos:definition "Security Services is the study of protecting properties, premises and people against intruders and damage." ;
    skos:example "crowd control, escorting and carrying valuables, personal protective services, premises and property securing systems, security dog handling, security risk management" ;
    skos:inScheme ascedcs: ;
    skos:notation "099905" ;
    skos:prefLabel "Security Services"@en ;
    skos:scopeNote "Exclusions: Security of computer data and systems. This is included in Detailed Field 029901 Security Science." .

asced:099999 a skos:Concept ;
    dcterms:created "2025-08-01T01:49:08.186000+00:00"^^xsd:dateTime ;
    dcterms:modified "2025-08-05T22:48:12.645000+00:00"^^xsd:dateTime ;
    skos:broader asced:0999 ;
    skos:definition "This detailed field includes all Society and Culture not elsewhere classified." ;
    skos:example "private investigation, road safety" ;
    skos:inScheme ascedcs: ;
    skos:notation "099999" ;
    skos:prefLabel "Society and Culture, n.e.c."@en .

asced:100101 a skos:Concept ;
    dcterms:created "2025-08-01T01:49:08.188000+00:00"^^xsd:dateTime ;
    dcterms:modified "2025-08-05T22:48:12.955000+00:00"^^xsd:dateTime ;
    skos:broader asced:1001 ;
    skos:definition "Music is the study of the history, theory, creation and performance of music." ;
    skos:example "music arranging, transcribing and conducting, composition and song writing, musicology, individual and group voice and instrumental performance" ;
    skos:inScheme ascedcs: ;
    skos:notation "100101" ;
    skos:prefLabel "Music"@en .

asced:100103 a skos:Concept ;
    dcterms:created "2025-08-01T01:49:08.189000+00:00"^^xsd:dateTime ;
    dcterms:modified "2025-08-05T22:48:12.993000+00:00"^^xsd:dateTime ;
    skos:broader asced:1001 ;
    skos:definition "Drama and Theatre Studies is the study of the history, theory, creation and performance of dramatic works. It includes speech, movement, mime, characterisation, improvisation and stage craft." ;
    skos:example "acting, voice and movement, costumes and props, scriptwriting, interpreting stories and themes, stage production directing, stage management" ;
    skos:inScheme ascedcs: ;
    skos:notation "100103" ;
    skos:prefLabel "Drama and Theatre Studies"@en .

asced:100105 a skos:Concept ;
    dcterms:created "2025-08-01T01:49:08.190000+00:00"^^xsd:dateTime ;
    dcterms:modified "2025-08-05T22:48:13.035000+00:00"^^xsd:dateTime ;
    skos:broader asced:1001 ;
    skos:definition "Dance is the study of the history, theory, creation and performance of works of dance." ;
    skos:example "choreography, dance improvisation, dance technique, dance notation and analysis" ;
    skos:inScheme ascedcs: ;
    skos:notation "100105" ;
    skos:prefLabel "Dance"@en .

asced:100199 a skos:Concept ;
    dcterms:created "2025-08-01T01:49:08.190000+00:00"^^xsd:dateTime ;
    dcterms:modified "2025-08-05T22:48:13.076000+00:00"^^xsd:dateTime ;
    skos:broader asced:1001 ;
    skos:definition "This detailed field includes all Performing Arts not elsewhere classified." ;
    skos:example "animateuring" ;
    skos:inScheme ascedcs: ;
    skos:notation "100199" ;
    skos:prefLabel "Performing Arts, n.e.c."@en .

asced:100301 a skos:Concept ;
    dcterms:created "2025-08-01T01:49:08.192000+00:00"^^xsd:dateTime ;
    dcterms:modified "2025-08-05T22:48:13.124000+00:00"^^xsd:dateTime ;
    skos:broader asced:1003 ;
    skos:definition "Fine Arts is the study of non-literary visual forms of creative expression for artistic and aesthetic purposes, and the methods of creating those forms." ;
    skos:example "art appreciation, calligraphy, drawing, painting, sculpture" ;
    skos:inScheme ascedcs: ;
    skos:notation "100301" ;
    skos:prefLabel "Fine Arts"@en ;
    skos:scopeNote "Exclusions: Art history. This is included in Detailed Field 090305 History." .

asced:100303 a skos:Concept ;
    dcterms:created "2025-08-01T01:49:08.192000+00:00"^^xsd:dateTime ;
    dcterms:modified "2025-08-05T22:48:13.167000+00:00"^^xsd:dateTime ;
    skos:broader asced:1003 ;
    skos:definition "Photography is the study of composing, taking, developing, printing, enlarging and presenting photographs for creative and practical purposes." ;
    skos:example "photographic development, view camera control and manipulation, photo equipment technology, photographic theory, photographic lighting techniques" ;
    skos:inScheme ascedcs: ;
    skos:notation "100303" ;
    skos:prefLabel "Photography"@en .

asced:100305 a skos:Concept ;
    dcterms:created "2025-08-01T01:49:08.193000+00:00"^^xsd:dateTime ;
    dcterms:modified "2025-08-05T22:48:13.203000+00:00"^^xsd:dateTime ;
    skos:broader asced:1003 ;
    skos:definition "Crafts is the study of fashioning individual objects for decorative, ornamental and functional purpose." ;
    skos:example "batik, ceramics, embroidery, tapestry, woodcraft" ;
    skos:inScheme ascedcs: ;
    skos:notation "100305" ;
    skos:prefLabel "Crafts"@en .

asced:100307 a skos:Concept ;
    dcterms:created "2025-08-01T01:49:08.194000+00:00"^^xsd:dateTime ;
    dcterms:modified "2025-08-05T22:48:13.244000+00:00"^^xsd:dateTime ;
    skos:broader asced:1003 ;
    skos:definition "Jewellery Making is the study of designing, producing and repairing ornaments for personal adornment." ;
    skos:example "lapidary, gem settings, jewellery design, precious and non-precious metal working" ;
    skos:inScheme ascedcs: ;
    skos:notation "100307" ;
    skos:prefLabel "Jewellery Making"@en .

asced:100309 a skos:Concept ;
    dcterms:created "2025-08-01T01:49:08.194000+00:00"^^xsd:dateTime ;
    dcterms:modified "2025-08-05T22:48:13.291000+00:00"^^xsd:dateTime ;
    skos:broader asced:1003 ;
    skos:definition "Floristry is the study of designing and displaying floral arrangements." ;
    skos:example "cut flower presentation, floral design and colour, floristry equipment, floristry plant materials" ;
    skos:inScheme ascedcs: ;
    skos:notation "100309" ;
    skos:prefLabel "Floristry"@en .

asced:100399 a skos:Concept ;
    dcterms:created "2025-08-01T01:49:08.194000+00:00"^^xsd:dateTime ;
    dcterms:modified "2025-08-05T22:48:13.335000+00:00"^^xsd:dateTime ;
    skos:broader asced:1003 ;
    skos:definition "This detailed field includes all Visual Arts and Crafts not elsewhere classified." ;
    skos:example "animation, fashion consultancy" ;
    skos:inScheme ascedcs: ;
    skos:notation "100399" ;
    skos:prefLabel "Visual Arts and Crafts, n.e.c."@en .

asced:100501 a skos:Concept ;
    dcterms:created "2025-08-01T01:49:08.196000+00:00"^^xsd:dateTime ;
    dcterms:modified "2025-08-05T22:48:13.377000+00:00"^^xsd:dateTime ;
    skos:broader asced:1005 ;
    skos:definition "Graphic Arts and Design Studies is the study of designing and producing visual representations of concepts and information." ;
    skos:example "three-dimensional design, design theory, design in context, design drawing and illustration, industrial arts" ;
    skos:inScheme ascedcs: ;
    skos:notation "100501" ;
    skos:prefLabel "Graphic Arts and Design Studies"@en .

asced:100503 a skos:Concept ;
    dcterms:created "2025-08-01T01:49:08.197000+00:00"^^xsd:dateTime ;
    dcterms:modified "2025-08-05T22:48:13.414000+00:00"^^xsd:dateTime ;
    skos:broader asced:1005 ;
    skos:definition "Textile Design is the study of designing and producing textiles." ;
    skos:example "computer-aided textile design, science of textiles, woven tapestry and experimental textiles" ;
    skos:inScheme ascedcs: ;
    skos:notation "100503" ;
    skos:prefLabel "Textile Design"@en .

asced:100505 a skos:Concept ;
    dcterms:created "2025-08-01T01:49:08.197000+00:00"^^xsd:dateTime ;
    dcterms:modified "2025-08-05T22:48:13.452000+00:00"^^xsd:dateTime ;
    skos:broader asced:1005 ;
    skos:definition "Fashion Design is the study of creatively combining line, form and fabric in designing and constructing fashion garments." ;
    skos:example "history and theory of fashion, fashion drawing and illustration, garment pattern development, fashion design concepts" ;
    skos:inScheme ascedcs: ;
    skos:notation "100505" ;
    skos:prefLabel "Fashion Design"@en .

asced:100599 a skos:Concept ;
    dcterms:created "2025-08-01T01:49:08.198000+00:00"^^xsd:dateTime ;
    dcterms:modified "2025-08-05T22:48:13.495000+00:00"^^xsd:dateTime ;
    skos:broader asced:1005 ;
    skos:definition "This detailed field includes all Graphic and Design Studies not elsewhere classified." ;
    skos:example "furniture design, wood design, footwear design" ;
    skos:inScheme ascedcs: ;
    skos:notation "100599" ;
    skos:prefLabel "Graphic and Design Studies, n.e.c."@en .

asced:100701 a skos:Concept ;
    dcterms:created "2025-08-01T01:49:08.198000+00:00"^^xsd:dateTime ;
    dcterms:modified "2025-08-05T22:48:13.537000+00:00"^^xsd:dateTime ;
    skos:broader asced:1007 ;
    skos:definition "Audio Visual Studies is the study of producing films and videos, and television and radio programmes." ;
    skos:example "audio visual equipment operation, cinema studies, film and video editing, film theory, radio programme production, sound production" ;
    skos:inScheme ascedcs: ;
    skos:notation "100701" ;
    skos:prefLabel "Audio Visual Studies"@en .

asced:100703 a skos:Concept ;
    dcterms:created "2025-08-01T01:49:08.199000+00:00"^^xsd:dateTime ;
    dcterms:modified "2025-08-05T22:48:13.576000+00:00"^^xsd:dateTime ;
    skos:broader asced:1007 ;
    skos:definition "Journalism is the study of researching current affairs and events and other matters of interests and reporting them." ;
    skos:example "newspaper layout, news gathering techniques, television and radio news scripting, reporting and writing for the media" ;
    skos:inScheme ascedcs: ;
    skos:notation "100703" ;
    skos:prefLabel "Journalism"@en .

asced:100705 a skos:Concept ;
    dcterms:created "2025-08-01T01:49:08.199000+00:00"^^xsd:dateTime ;
    dcterms:modified "2025-08-05T22:48:13.623000+00:00"^^xsd:dateTime ;
    skos:broader asced:1007 ;
    skos:definition "Written Communication is the study of developing effective written communication skills." ;
    skos:example "copy writing, letter writing, poetry writing, story writing, technical writing" ;
    skos:inScheme ascedcs: ;
    skos:notation "100705" ;
    skos:prefLabel "Written Communication"@en .

asced:100707 a skos:Concept ;
    dcterms:created "2025-08-01T01:49:08.200000+00:00"^^xsd:dateTime ;
    dcterms:modified "2025-08-05T22:48:13.663000+00:00"^^xsd:dateTime ;
    skos:broader asced:1007 ;
    skos:definition "Verbal Communication is the study of developing effective verbal communication skills." ;
    skos:example "debating, public speaking" ;
    skos:inScheme ascedcs: ;
    skos:notation "100707" ;
    skos:prefLabel "Verbal Communication"@en .

asced:100799 a skos:Concept ;
    dcterms:created "2025-08-01T01:49:08.201000+00:00"^^xsd:dateTime ;
    dcterms:modified "2025-08-05T22:48:13.710000+00:00"^^xsd:dateTime ;
    skos:broader asced:1007 ;
    skos:definition "This detailed field includes all Communication and Media Studies not elsewhere classified." ;
    skos:example "multimedia, photomedia" ;
    skos:inScheme ascedcs: ;
    skos:notation "100799" ;
    skos:prefLabel "Communication and Media Studies, n.e.c."@en .

asced:109999 a skos:Concept ;
    dcterms:created "2025-08-01T01:49:08.202000+00:00"^^xsd:dateTime ;
    dcterms:modified "2025-08-05T22:48:13.755000+00:00"^^xsd:dateTime ;
    skos:broader asced:1099 ;
    skos:definition "This detailed field includes all Creative Arts not elsewhere classified." ;
    skos:example "art criticism" ;
    skos:inScheme ascedcs: ;
    skos:notation "109999" ;
    skos:prefLabel "Creative Arts, n.e.c."@en .

asced:110101 a skos:Concept ;
    dcterms:created "2025-08-01T01:49:08.203000+00:00"^^xsd:dateTime ;
    dcterms:modified "2025-08-05T22:48:13.927000+00:00"^^xsd:dateTime ;
    skos:broader asced:1101 ;
    skos:definition "Hospitality is the study of providing reception, accommodation, entertainment, food, beverages and related services to patrons at hotels, motels, clubs, restaurants, caravan parks, etc." ;
    skos:example "front office operations, guest relations, club and gaming operations, catering operations" ;
    skos:inScheme ascedcs: ;
    skos:notation "110101" ;
    skos:prefLabel "Hospitality"@en .

asced:110103 a skos:Concept ;
    dcterms:created "2025-08-01T01:49:08.204000+00:00"^^xsd:dateTime ;
    dcterms:modified "2025-08-05T22:48:13.968000+00:00"^^xsd:dateTime ;
    skos:broader asced:1101 ;
    skos:definition "Food and Beverage Service is the study of serving and presenting food and beverages." ;
    skos:example "cellar operations, drink preparation, silver service, table setting, taking and serving meal orders" ;
    skos:inScheme ascedcs: ;
    skos:notation "110103" ;
    skos:prefLabel "Food and Beverage Service"@en .

asced:110105 a skos:Concept ;
    dcterms:created "2025-08-01T01:49:08.204000+00:00"^^xsd:dateTime ;
    dcterms:modified "2025-08-05T22:48:14.010000+00:00"^^xsd:dateTime ;
    skos:broader asced:1101 ;
    skos:definition "Butchery is the study of cutting and preparing meat. It includes small-scale sausage and smallgoods making." ;
    skos:example "boning, livestock slaughtering techniques, minced meat product preparation, seasoning, pickling and curing meats, shaping and tying roasts and poultry, cuts of meat" ;
    skos:inScheme ascedcs: ;
    skos:notation "110105" ;
    skos:prefLabel "Butchery"@en ;
    skos:scopeNote "Exclusions: Smallgoods manufacture. This is included in Detailed Field 030307 Food Processing Techniques." .

asced:110107 a skos:Concept ;
    dcterms:created "2025-08-01T01:49:08.205000+00:00"^^xsd:dateTime ;
    dcterms:modified "2025-08-05T22:48:14.051000+00:00"^^xsd:dateTime ;
    skos:broader asced:1101 ;
    skos:definition "Baking and Pastrymaking is the study of making and presenting breads, pastries, buns and cakes." ;
    skos:example "cake and spongemaking, cake decoration, fundamentals of breadmaking, fundamentals of pastry cooking, rye breads, sweet yeast products" ;
    skos:inScheme ascedcs: ;
    skos:notation "110107" ;
    skos:prefLabel "Baking and Pastrymaking"@en .

asced:110109 a skos:Concept ;
    dcterms:created "2025-08-01T01:49:08.206000+00:00"^^xsd:dateTime ;
    dcterms:modified "2025-08-05T22:48:14.096000+00:00"^^xsd:dateTime ;
    skos:broader asced:1101 ;
    skos:definition "Cookery is the study of preparing food. It includes the development of recipes." ;
    skos:example "a la carte and table d'hte operations, appetisers, salads, sandwiches and desserts, kitchen management, mise-en-place and food preparation, meat, poultry and seafood, stocks, sauces and soups" ;
    skos:inScheme ascedcs: ;
    skos:notation "110109" ;
    skos:prefLabel "Cookery"@en .

asced:110111 a skos:Concept ;
    dcterms:created "2025-08-01T01:49:08.206000+00:00"^^xsd:dateTime ;
    dcterms:modified "2025-08-05T22:48:14.142000+00:00"^^xsd:dateTime ;
    skos:broader asced:1101 ;
    skos:definition "Food Hygiene is the study of the principles and regulations of food safe handling and preparation." ;
    skos:example "food safety procedures, hygienic food handling procedures, hazard analysis critical control points (HACCP), food contamination, food storage and temperature control" ;
    skos:inScheme ascedcs: ;
    skos:notation "110111" ;
    skos:prefLabel "Food Hygiene"@en .

asced:110199 a skos:Concept ;
    dcterms:created "2025-08-01T01:49:08.206000+00:00"^^xsd:dateTime ;
    dcterms:modified "2025-08-05T22:48:14.181000+00:00"^^xsd:dateTime ;
    skos:broader asced:1101 ;
    skos:definition "This detailed field includes all Food and Hospitality not elsewhere classified." ;
    skos:example "gaming inspection, housekeeping" ;
    skos:inScheme ascedcs: ;
    skos:notation "110199" ;
    skos:prefLabel "Food and Hospitality, n.e.c."@en .

asced:110301 a skos:Concept ;
    dcterms:created "2025-08-01T01:49:08.207000+00:00"^^xsd:dateTime ;
    dcterms:modified "2025-08-05T22:48:14.221000+00:00"^^xsd:dateTime ;
    skos:broader asced:1103 ;
    skos:definition "Beauty Therapy is the study of maintaining and beautifying the face and body." ;
    skos:example "electrolysis, make-up artistry, nail technology, piercing, skin treatments, tattooing" ;
    skos:inScheme ascedcs: ;
    skos:notation "110301" ;
    skos:prefLabel "Beauty Therapy"@en .

asced:110303 a skos:Concept ;
    dcterms:created "2025-08-01T01:49:08.208000+00:00"^^xsd:dateTime ;
    dcterms:modified "2025-08-05T22:48:14.261000+00:00"^^xsd:dateTime ;
    skos:broader asced:1103 ;
    skos:definition "Hairdressing is the study of cutting, colouring and styling scalp and facial hair." ;
    skos:example "beard trimming, colouring techniques, classic and fashion cutting techniques, hair extensions, perming techniques" ;
    skos:inScheme ascedcs: ;
    skos:notation "110303" ;
    skos:prefLabel "Hairdressing"@en .

asced:110399 a skos:Concept ;
    dcterms:created "2025-08-01T01:49:08.208000+00:00"^^xsd:dateTime ;
    dcterms:modified "2025-08-05T22:48:14.296000+00:00"^^xsd:dateTime ;
    skos:broader asced:1103 ;
    skos:definition "This detailed field includes all Personal Services not elsewhere classified." ;
    skos:example "embalming, funeral services" ;
    skos:inScheme ascedcs: ;
    skos:notation "110399" ;
    skos:prefLabel "Personal Services, n.e.c."@en .

asced:120101 a skos:Concept ;
    dcterms:created "2025-08-01T01:49:08.210000+00:00"^^xsd:dateTime ;
    dcterms:modified "2025-08-05T22:48:14.546000+00:00"^^xsd:dateTime ;
    skos:broader asced:1201 ;
    skos:definition "General Primary and Secondary Education Programmes develop general knowledge and skills through school education programmes. It includes secondary education programmes run in TAFEs and other similar institutions." ;
    skos:example "mathematics skills, reading and writing, general studies in history, geography, natural science, social science, art and music" ;
    skos:inScheme ascedcs: ;
    skos:notation "120101" ;
    skos:prefLabel "General Primary and Secondary Education Programmes"@en .

asced:120103 a skos:Concept ;
    dcterms:created "2025-08-01T01:49:08.211000+00:00"^^xsd:dateTime ;
    dcterms:modified "2025-08-05T22:48:14.588000+00:00"^^xsd:dateTime ;
    skos:broader asced:1201 ;
    skos:definition "Literacy and Numeracy Programmes develop basic reading, writing and numeracy skills." ;
    skos:example "general language skills, basic reading and writing, basic numeracy skills, spelling and grammar" ;
    skos:inScheme ascedcs: ;
    skos:notation "120103" ;
    skos:prefLabel "Literacy and Numeracy Programmes"@en ;
    skos:scopeNote "Exclusions: English as a second language. This is included in Detailed Field 091501 English Language." .

asced:120105 a skos:Concept ;
    dcterms:created "2025-08-01T01:49:08.211000+00:00"^^xsd:dateTime ;
    dcterms:modified "2025-08-05T22:48:14.633000+00:00"^^xsd:dateTime ;
    skos:broader asced:1201 ;
    skos:definition "Learning Skills Programmes develop skills for study, such as research and analysis skills." ;
    skos:example "analysing techniques, general report writing, how to research a topic" ;
    skos:inScheme ascedcs: ;
    skos:notation "120105" ;
    skos:prefLabel "Learning Skills Programmes"@en .

asced:120199 a skos:Concept ;
    dcterms:created "2025-08-01T01:49:08.211000+00:00"^^xsd:dateTime ;
    dcterms:modified "2025-08-05T22:48:14.686000+00:00"^^xsd:dateTime ;
    skos:broader asced:1201 ;
    skos:definition "This detailed field includes all General Education Programmes not elsewhere classified." ;
    skos:example "tertiary preparation, general studies" ;
    skos:inScheme ascedcs: ;
    skos:notation "120199" ;
    skos:prefLabel "General Education Programmes, n.e.c."@en .

asced:120301 a skos:Concept ;
    dcterms:created "2025-08-01T01:49:08.212000+00:00"^^xsd:dateTime ;
    dcterms:modified "2025-08-05T22:48:14.730000+00:00"^^xsd:dateTime ;
    skos:broader asced:1203 ;
    skos:definition "Social and Interpersonal Skills Programmes develop skills for interacting with family and people in the wider community." ;
    skos:example "personal and social relationships, social etiquette, interpersonal communication" ;
    skos:inScheme ascedcs: ;
    skos:notation "120301" ;
    skos:prefLabel "Social and Interpersonal Skills Programmes"@en ;
    skos:scopeNote "Exclusions: Personal management training. This is included in Detailed Field 080305 Personal Management Training." .

asced:120303 a skos:Concept ;
    dcterms:created "2025-08-01T01:49:08.213000+00:00"^^xsd:dateTime ;
    dcterms:modified "2025-08-05T22:48:14.770000+00:00"^^xsd:dateTime ;
    skos:broader asced:1203 ;
    skos:definition "Survival Skills Programmes develop skills for managing a household." ;
    skos:example "basic home economics, banking and buying" ;
    skos:inScheme ascedcs: ;
    skos:notation "120303" ;
    skos:prefLabel "Survival Skills Programmes"@en .

asced:120305 a skos:Concept ;
    dcterms:created "2025-08-01T01:49:08.214000+00:00"^^xsd:dateTime ;
    dcterms:modified "2025-08-05T22:48:14.806000+00:00"^^xsd:dateTime ;
    skos:broader asced:1203 ;
    skos:definition "Parental Education Programmes develop skills for parenting." ;
    skos:example "providing for children, dealing with conflict, resolving values problems, setting boundaries" ;
    skos:inScheme ascedcs: ;
    skos:notation "120305" ;
    skos:prefLabel "Parental Education Programmes"@en .

asced:120399 a skos:Concept ;
    dcterms:created "2025-08-01T01:49:08.214000+00:00"^^xsd:dateTime ;
    dcterms:modified "2025-08-05T22:48:14.846000+00:00"^^xsd:dateTime ;
    skos:broader asced:1203 ;
    skos:definition "This detailed field includes all Social Skills Programmes not elsewhere classified." ;
    skos:inScheme ascedcs: ;
    skos:notation "120399" ;
    skos:prefLabel "Social Skills Programmes, n.e.c."@en .

asced:120501 a skos:Concept ;
    dcterms:created "2025-08-01T01:49:08.215000+00:00"^^xsd:dateTime ;
    dcterms:modified "2025-08-05T22:48:14.886000+00:00"^^xsd:dateTime ;
    skos:broader asced:1205 ;
    skos:definition "Career Development Programmes provide guidance and counselling for career development." ;
    skos:example "vocational exploration, choosing a career, career planning" ;
    skos:inScheme ascedcs: ;
    skos:notation "120501" ;
    skos:prefLabel "Career Development Programmes"@en .

asced:120503 a skos:Concept ;
    dcterms:created "2025-08-01T01:49:08.216000+00:00"^^xsd:dateTime ;
    dcterms:modified "2025-08-05T22:48:14.928000+00:00"^^xsd:dateTime ;
    skos:broader asced:1205 ;
    skos:definition "Job Search Skills Programmes develop skills for finding a job." ;
    skos:example "resume writing, interview skills and presentation, prospecting and general job seeking" ;
    skos:inScheme ascedcs: ;
    skos:notation "120503" ;
    skos:prefLabel "Job Search Skills Programmes"@en .

asced:120505 a skos:Concept ;
    dcterms:created "2025-08-01T01:49:08.216000+00:00"^^xsd:dateTime ;
    dcterms:modified "2025-08-05T22:48:14.984000+00:00"^^xsd:dateTime ;
    skos:broader asced:1205 ;
    skos:definition "Work Practices Programmes develop skills for functioning effectively in the workplace." ;
    skos:example "communicating in the workplace, working with others, participating in teams" ;
    skos:inScheme ascedcs: ;
    skos:notation "120505" ;
    skos:prefLabel "Work Practices Programmes"@en .

asced:120599 a skos:Concept ;
    dcterms:created "2025-08-01T01:49:08.216000+00:00"^^xsd:dateTime ;
    dcterms:modified "2025-08-05T22:48:15.030000+00:00"^^xsd:dateTime ;
    skos:broader asced:1205 ;
    skos:definition "This detailed field includes all Employment Skills Programmes not elsewhere classified." ;
    skos:example "returning to the workforce, industrial skills" ;
    skos:inScheme ascedcs: ;
    skos:notation "120599" ;
    skos:prefLabel "Employment Skills Programmes, n.e.c."@en .

asced:129999 a skos:Concept ;
    dcterms:created "2025-08-01T01:49:08.218000+00:00"^^xsd:dateTime ;
    dcterms:modified "2025-08-05T22:48:15.069000+00:00"^^xsd:dateTime ;
    skos:broader asced:1299 ;
    skos:definition "This detailed field includes all Mixed Field Programmes not elsewhere classified." ;
    skos:inScheme ascedcs: ;
    skos:notation "129999" ;
    skos:prefLabel "Mixed Field Programmes, n.e.c."@en .

asced:0505 a skos:Concept ;
    dcterms:created "2025-08-01T01:49:08.054000+00:00"^^xsd:dateTime ;
    dcterms:modified "2025-08-05T22:48:03.282000+00:00"^^xsd:dateTime ;
    skos:broader asced:05 ;
    skos:definition "Forestry Studies disciplines covering key subfields such as . Emphasises theory, practice, and industry-relevant applications." ;
    skos:inScheme ascedcs: ;
    skos:narrower asced:050501 ;
    skos:notation "0505" ;
    skos:prefLabel "Forestry Studies"@en .

asced:0605 a skos:Concept ;
    dcterms:created "2025-08-01T01:49:08.077000+00:00"^^xsd:dateTime ;
    dcterms:modified "2025-08-05T22:48:04.180000+00:00"^^xsd:dateTime ;
    skos:broader asced:06 ;
    skos:definition "Pharmacy disciplines covering key subfields such as . Emphasises theory, practice, and industry-relevant applications." ;
    skos:inScheme ascedcs: ;
    skos:narrower asced:060501 ;
    skos:notation "0605" ;
    skos:prefLabel "Pharmacy"@en .

asced:0615 a skos:Concept ;
    dcterms:created "2025-08-01T01:49:08.094000+00:00"^^xsd:dateTime ;
    dcterms:modified "2025-08-05T22:48:04.399000+00:00"^^xsd:dateTime ;
    skos:broader asced:06 ;
    skos:definition "Radiography disciplines covering key subfields such as . Emphasises theory, practice, and industry-relevant applications." ;
    skos:inScheme ascedcs: ;
    skos:narrower asced:061501 ;
    skos:notation "0615" ;
    skos:prefLabel "Radiography"@en .

asced:0799 a skos:Concept ;
    dcterms:created "2025-08-01T01:49:08.121000+00:00"^^xsd:dateTime ;
    dcterms:modified "2025-08-05T22:48:07.211000+00:00"^^xsd:dateTime ;
    skos:broader asced:07 ;
    skos:definition "Other Education disciplines spanning core studies and related applied fields." ;
    skos:inScheme ascedcs: ;
    skos:narrower asced:079999 ;
    skos:notation "0799" ;
    skos:prefLabel "Other Education"@en .

asced:0801 a skos:Concept ;
    dcterms:created "2025-08-01T01:49:08.123000+00:00"^^xsd:dateTime ;
    dcterms:modified "2025-08-05T22:48:07.815000+00:00"^^xsd:dateTime ;
    skos:broader asced:08 ;
    skos:definition "Accounting disciplines covering key subfields such as . Emphasises theory, practice, and industry-relevant applications." ;
    skos:inScheme ascedcs: ;
    skos:narrower asced:080101 ;
    skos:notation "0801" ;
    skos:prefLabel "Accounting"@en .

asced:0807 a skos:Concept ;
    dcterms:created "2025-08-01T01:49:08.137000+00:00"^^xsd:dateTime ;
    dcterms:modified "2025-08-05T22:48:07.930000+00:00"^^xsd:dateTime ;
    skos:broader asced:08 ;
    skos:definition "Tourism disciplines covering key subfields such as . Emphasises theory, practice, and industry-relevant applications." ;
    skos:inScheme ascedcs: ;
    skos:narrower asced:080701 ;
    skos:notation "0807" ;
    skos:prefLabel "Tourism"@en .

asced:1099 a skos:Concept ;
    dcterms:created "2025-08-01T01:49:08.202000+00:00"^^xsd:dateTime ;
    dcterms:modified "2025-08-05T22:48:12.911000+00:00"^^xsd:dateTime ;
    skos:broader asced:10 ;
    skos:definition "Other Creative Arts disciplines spanning core studies and related applied fields." ;
    skos:inScheme ascedcs: ;
    skos:narrower asced:109999 ;
    skos:notation "1099" ;
    skos:prefLabel "Other Creative Arts"@en .

asced:1299 a skos:Concept ;
    dcterms:created "2025-08-01T01:49:08.217000+00:00"^^xsd:dateTime ;
    dcterms:modified "2025-08-05T22:48:14.507000+00:00"^^xsd:dateTime ;
    skos:broader asced:12 ;
    skos:definition "Other Mixed Field Programmes disciplines spanning core studies and related applied fields." ;
    skos:inScheme ascedcs: ;
    skos:narrower asced:129999 ;
    skos:notation "1299" ;
    skos:prefLabel "Other Mixed Field Programmes"@en .

asced:0103 a skos:Concept ;
    dcterms:created "2025-08-01T01:49:07.903000+00:00"^^xsd:dateTime ;
    dcterms:modified "2025-08-05T22:47:55.094000+00:00"^^xsd:dateTime ;
    skos:broader asced:01 ;
    skos:definition "Physics and Astronomy disciplines covering key subfields such as Astronomy, and Physics." ;
    skos:inScheme ascedcs: ;
    skos:narrower asced:010301,
        asced:010303 ;
    skos:notation "0103" ;
    skos:prefLabel "Physics and Astronomy"@en .

asced:0299 a skos:Concept ;
    dcterms:created "2025-08-01T01:49:07.958000+00:00"^^xsd:dateTime ;
    dcterms:modified "2025-08-05T22:47:57.145000+00:00"^^xsd:dateTime ;
    skos:broader asced:02 ;
    skos:definition "Other Information Technology disciplines covering key subfields such as ." ;
    skos:inScheme ascedcs: ;
    skos:narrower asced:029901,
        asced:029999 ;
    skos:notation "0299" ;
    skos:prefLabel "Other Information Technology"@en .

asced:04 a skos:Concept ;
    dcterms:created "2025-08-01T01:49:08.030000+00:00"^^xsd:dateTime ;
    dcterms:modified "2025-08-05T22:48:02.015000+00:00"^^xsd:dateTime ;
    skos:inScheme ascedcs: ;
    skos:narrower asced:0401,
        asced:0403 ;
    skos:notation "04" ;
    skos:prefLabel "ARCHITECTURE AND BUILDING"@en ;
    skos:topConceptOf ascedcs: .

asced:0503 a skos:Concept ;
    dcterms:created "2025-08-01T01:49:08.052000+00:00"^^xsd:dateTime ;
    dcterms:modified "2025-08-05T22:48:03.235000+00:00"^^xsd:dateTime ;
    skos:broader asced:05 ;
    skos:definition "Horticulture and Viticulture disciplines covering key subfields such as Horticulture, and Viticulture." ;
    skos:inScheme ascedcs: ;
    skos:narrower asced:050301,
        asced:050303 ;
    skos:notation "0503" ;
    skos:prefLabel "Horticulture and Viticulture"@en .

asced:0507 a skos:Concept ;
    dcterms:created "2025-08-01T01:49:08.055000+00:00"^^xsd:dateTime ;
    dcterms:modified "2025-08-05T22:48:03.320000+00:00"^^xsd:dateTime ;
    skos:broader asced:05 ;
    skos:definition "Fisheries Studies disciplines covering key subfields such as . Emphasises theory, practice, and industry-relevant applications." ;
    skos:inScheme ascedcs: ;
    skos:narrower asced:050701,
        asced:050799 ;
    skos:notation "0507" ;
    skos:prefLabel "Fisheries Studies"@en .

asced:0509 a skos:Concept ;
    dcterms:created "2025-08-01T01:49:08.057000+00:00"^^xsd:dateTime ;
    dcterms:modified "2025-08-05T22:48:03.363000+00:00"^^xsd:dateTime ;
    skos:broader asced:05 ;
    skos:definition "Environmental Studies disciplines covering key subfields such as . Emphasises theory, practice, and industry-relevant applications." ;
    skos:inScheme ascedcs: ;
    skos:narrower asced:050901,
        asced:050999 ;
    skos:notation "0509" ;
    skos:prefLabel "Environmental Studies"@en .

asced:0599 a skos:Concept ;
    dcterms:created "2025-08-01T01:49:08.060000+00:00"^^xsd:dateTime ;
    dcterms:modified "2025-08-05T22:48:03.415000+00:00"^^xsd:dateTime ;
    skos:broader asced:05 ;
    skos:definition "Other Agriculture, Environmental and Related Studies disciplines covering key subfields such as ." ;
    skos:inScheme ascedcs: ;
    skos:narrower asced:059901,
        asced:059999 ;
    skos:notation "0599" ;
    skos:prefLabel "Other Agriculture, Environmental and Related Studies"@en .

asced:0703 a skos:Concept ;
    dcterms:created "2025-08-01T01:49:08.120000+00:00"^^xsd:dateTime ;
    dcterms:modified "2025-08-05T22:48:07.172000+00:00"^^xsd:dateTime ;
    skos:broader asced:07 ;
    skos:definition "Curriculum and Education Studies disciplines covering key subfields such as Curriculum Studies, and Education Studies." ;
    skos:inScheme ascedcs: ;
    skos:narrower asced:070301,
        asced:070303 ;
    skos:notation "0703" ;
    skos:prefLabel "Curriculum and Education Studies"@en .

asced:0901 a skos:Concept ;
    dcterms:created "2025-08-01T01:49:08.146000+00:00"^^xsd:dateTime ;
    dcterms:modified "2025-08-05T22:48:09.581000+00:00"^^xsd:dateTime ;
    skos:broader asced:09 ;
    skos:definition "Political Science and Policy Studies disciplines covering key subfields such as Policy Studies, and Political Science." ;
    skos:inScheme ascedcs: ;
    skos:narrower asced:090101,
        asced:090103 ;
    skos:notation "0901" ;
    skos:prefLabel "Political Science and Policy Studies"@en .

asced:0907 a skos:Concept ;
    dcterms:created "2025-08-01T01:49:08.159000+00:00"^^xsd:dateTime ;
    dcterms:modified "2025-08-05T22:48:09.730000+00:00"^^xsd:dateTime ;
    skos:broader asced:09 ;
    skos:definition "Behavioural Science disciplines covering key subfields such as . Emphasises theory, practice, and industry-relevant applications." ;
    skos:inScheme ascedcs: ;
    skos:narrower asced:090701,
        asced:090799 ;
    skos:notation "0907" ;
    skos:prefLabel "Behavioural Science"@en .

asced:0913 a skos:Concept ;
    dcterms:created "2025-08-01T01:49:08.169000+00:00"^^xsd:dateTime ;
    dcterms:modified "2025-08-05T22:48:09.884000+00:00"^^xsd:dateTime ;
    skos:broader asced:09 ;
    skos:definition "Librarianship, Information Management and Curatorial Studies disciplines covering key subfields such as Curatorial Studies, and Librarianship and Information Management." ;
    skos:inScheme ascedcs: ;
    skos:narrower asced:091301,
        asced:091303 ;
    skos:notation "0913" ;
    skos:prefLabel "Librarianship, Information Management and Curatorial Studies"@en .

asced:0917 a skos:Concept ;
    dcterms:created "2025-08-01T01:49:08.178000+00:00"^^xsd:dateTime ;
    dcterms:modified "2025-08-05T22:48:09.988000+00:00"^^xsd:dateTime ;
    skos:broader asced:09 ;
    skos:definition "Philosophy and Religious Studies disciplines covering key subfields such as Philosophy, and Religious Studies." ;
    skos:inScheme ascedcs: ;
    skos:narrower asced:091701,
        asced:091703 ;
    skos:notation "0917" ;
    skos:prefLabel "Philosophy and Religious Studies"@en .

asced:0919 a skos:Concept ;
    dcterms:created "2025-08-01T01:49:08.179000+00:00"^^xsd:dateTime ;
    dcterms:modified "2025-08-05T22:48:10.043000+00:00"^^xsd:dateTime ;
    skos:broader asced:09 ;
    skos:definition "Economics and Econometrics disciplines covering key subfields such as Econometrics, and Economics." ;
    skos:inScheme ascedcs: ;
    skos:narrower asced:091901,
        asced:091903 ;
    skos:notation "0919" ;
    skos:prefLabel "Economics and Econometrics"@en .

asced:11 a skos:Concept ;
    dcterms:created "2025-08-01T01:49:08.202000+00:00"^^xsd:dateTime ;
    dcterms:modified "2025-08-05T22:48:13.803000+00:00"^^xsd:dateTime ;
    skos:inScheme ascedcs: ;
    skos:narrower asced:1101,
        asced:1103 ;
    skos:notation "11" ;
    skos:prefLabel "FOOD, HOSPITALITY AND PERSONAL SERVICES"@en ;
    skos:topConceptOf ascedcs: .

asced:0101 a skos:Concept ;
    dcterms:created "2025-08-01T01:49:07.898000+00:00"^^xsd:dateTime ;
    dcterms:modified "2025-08-05T22:47:55.043000+00:00"^^xsd:dateTime ;
    skos:broader asced:01 ;
    skos:definition "Mathematical Sciences disciplines covering key subfields such as Mathematics, and Statistics." ;
    skos:inScheme ascedcs: ;
    skos:narrower asced:010101,
        asced:010103,
        asced:010199 ;
    skos:notation "0101" ;
    skos:prefLabel "Mathematical Sciences"@en .

asced:0105 a skos:Concept ;
    dcterms:created "2025-08-01T01:49:07.907000+00:00"^^xsd:dateTime ;
    dcterms:modified "2025-08-05T22:47:55.148000+00:00"^^xsd:dateTime ;
    skos:broader asced:01 ;
    skos:definition "Chemical Sciences disciplines covering key subfields such as Inorganic Chemistry, and Organic Chemistry." ;
    skos:inScheme ascedcs: ;
    skos:narrower asced:010501,
        asced:010503,
        asced:010599 ;
    skos:notation "0105" ;
    skos:prefLabel "Chemical Sciences"@en .

asced:02 a skos:Concept ;
    dcterms:created "2025-08-01T01:49:07.938000+00:00"^^xsd:dateTime ;
    dcterms:modified "2025-08-05T22:47:57.009000+00:00"^^xsd:dateTime ;
    skos:inScheme ascedcs: ;
    skos:narrower asced:0201,
        asced:0203,
        asced:0299 ;
    skos:notation "02" ;
    skos:prefLabel "INFORMATION TECHNOLOGY"@en ;
	skos:closeMatch <https://linked.data.gov.au/def/anzsrc-for/2020/46> ;
    skos:topConceptOf ascedcs: .

asced:0311 a skos:Concept ;
    dcterms:created "2025-08-01T01:49:08.004000+00:00"^^xsd:dateTime ;
    dcterms:modified "2025-08-05T22:47:58.409000+00:00"^^xsd:dateTime ;
    skos:broader asced:03 ;
    skos:definition "Geomatic Engineering disciplines covering key subfields such as Mapping Science, and Surveying." ;
    skos:inScheme ascedcs: ;
    skos:narrower asced:031101,
        asced:031103,
        asced:031199 ;
    skos:notation "0311" ;
    skos:prefLabel "Geomatic Engineering"@en .

asced:0609 a skos:Concept ;
    dcterms:created "2025-08-01T01:49:08.082000+00:00"^^xsd:dateTime ;
    dcterms:modified "2025-08-05T22:48:04.261000+00:00"^^xsd:dateTime ;
    skos:broader asced:06 ;
    skos:definition "Optical Science disciplines covering key subfields such as Optical Technology, and Optometry." ;
    skos:inScheme ascedcs: ;
    skos:narrower asced:060901,
        asced:060903,
        asced:060999 ;
    skos:notation "0609" ;
    skos:prefLabel "Optical Science"@en .

asced:0611 a skos:Concept ;
    dcterms:created "2025-08-01T01:49:08.084000+00:00"^^xsd:dateTime ;
    dcterms:modified "2025-08-05T22:48:04.308000+00:00"^^xsd:dateTime ;
    skos:broader asced:06 ;
    skos:definition "Veterinary Studies disciplines covering key subfields such as Veterinary Assisting, and Veterinary Science." ;
    skos:inScheme ascedcs: ;
    skos:narrower asced:061101,
        asced:061103,
        asced:061199 ;
    skos:notation "0611" ;
    skos:prefLabel "Veterinary Studies"@en .

asced:07 a skos:Concept ;
    dcterms:created "2025-08-01T01:49:08.111000+00:00"^^xsd:dateTime ;
    dcterms:modified "2025-08-05T22:48:07.089000+00:00"^^xsd:dateTime ;
    skos:inScheme ascedcs: ;
    skos:narrower asced:0701,
        asced:0703,
        asced:0799 ;
    skos:notation "07" ;
    skos:prefLabel "EDUCATION"@en ;
    skos:topConceptOf ascedcs: .

asced:0899 a skos:Concept ;
    dcterms:created "2025-08-01T01:49:08.144000+00:00"^^xsd:dateTime ;
    dcterms:modified "2025-08-05T22:48:08.055000+00:00"^^xsd:dateTime ;
    skos:broader asced:08 ;
    skos:definition "Other Management and Commerce disciplines covering key subfields such as Purchasing, Warehousing and Distribution, and Valuation." ;
    skos:inScheme ascedcs: ;
    skos:narrower asced:089901,
        asced:089903,
        asced:089999 ;
    skos:notation "0899" ;
    skos:prefLabel "Other Management and Commerce"@en .

asced:0921 a skos:Concept ;
    dcterms:created "2025-08-01T01:49:08.182000+00:00"^^xsd:dateTime ;
    dcterms:modified "2025-08-05T22:48:10.093000+00:00"^^xsd:dateTime ;
    skos:broader asced:09 ;
    skos:definition "Sport and Recreation disciplines covering key subfields such as Sport and Recreation Activities, and Sports Coaching, Officiating and Instruction." ;
    skos:inScheme ascedcs: ;
    skos:narrower asced:092101,
        asced:092103,
        asced:092199 ;
    skos:notation "0921" ;
    skos:prefLabel "Sport and Recreation"@en .

asced:1103 a skos:Concept ;
    dcterms:created "2025-08-01T01:49:08.207000+00:00"^^xsd:dateTime ;
    dcterms:modified "2025-08-05T22:48:13.885000+00:00"^^xsd:dateTime ;
    skos:broader asced:11 ;
    skos:definition "Personal Services disciplines covering key subfields such as Beauty Therapy, and Hairdressing." ;
    skos:inScheme ascedcs: ;
    skos:narrower asced:110301,
        asced:110303,
        asced:110399 ;
    skos:notation "1103" ;
    skos:prefLabel "Personal Services"@en .

asced:0317 a skos:Concept ;
    dcterms:created "2025-08-01T01:49:08.022000+00:00"^^xsd:dateTime ;
    dcterms:modified "2025-08-05T22:47:58.560000+00:00"^^xsd:dateTime ;
    skos:broader asced:03 ;
    skos:definition "Maritime Engineering and Technology disciplines covering key subfields such as Marine Construction, Marine Craft Operation, and Maritime Engineering." ;
    skos:inScheme ascedcs: ;
    skos:narrower asced:031701,
        asced:031703,
        asced:031705,
        asced:031799 ;
    skos:notation "0317" ;
    skos:prefLabel "Maritime Engineering and Technology"@en .

asced:0501 a skos:Concept ;
    dcterms:created "2025-08-01T01:49:08.048000+00:00"^^xsd:dateTime ;
    dcterms:modified "2025-08-05T22:48:03.188000+00:00"^^xsd:dateTime ;
    skos:broader asced:05 ;
    skos:definition "Agriculture disciplines covering key subfields such as Agricultural Science, Animal Husbandry, and Wool Science." ;
    skos:inScheme ascedcs: ;
    skos:narrower asced:050101,
        asced:050103,
        asced:050105,
        asced:050199 ;
    skos:notation "0501" ;
    skos:prefLabel "Agriculture"@en .

asced:0607 a skos:Concept ;
    dcterms:created "2025-08-01T01:49:08.079000+00:00"^^xsd:dateTime ;
    dcterms:modified "2025-08-05T22:48:04.219000+00:00"^^xsd:dateTime ;
    skos:broader asced:06 ;
    skos:definition "Dental Studies disciplines covering key subfields such as Dental Assisting, Dental Technology, and Dentistry." ;
    skos:inScheme ascedcs: ;
    skos:narrower asced:060701,
        asced:060703,
        asced:060705,
        asced:060799 ;
    skos:notation "0607" ;
    skos:prefLabel "Dental Studies"@en .

asced:0619 a skos:Concept ;
    dcterms:created "2025-08-01T01:49:08.102000+00:00"^^xsd:dateTime ;
    dcterms:modified "2025-08-05T22:48:04.487000+00:00"^^xsd:dateTime ;
    skos:broader asced:06 ;
    skos:definition "Complementary Therapies disciplines covering key subfields such as Acupuncture, Naturopathy, and Traditional Chinese Medicine." ;
    skos:inScheme ascedcs: ;
    skos:narrower asced:061901,
        asced:061903,
        asced:061905,
        asced:061999 ;
    skos:notation "0619" ;
    skos:prefLabel "Complementary Therapies"@en .

asced:0809 a skos:Concept ;
    dcterms:created "2025-08-01T01:49:08.138000+00:00"^^xsd:dateTime ;
    dcterms:modified "2025-08-05T22:48:07.969000+00:00"^^xsd:dateTime ;
    skos:broader asced:08 ;
    skos:definition "Office Studies disciplines covering key subfields such as Keyboard Skills, Practical Computing Skills, and Secretarial and Clerical Studies." ;
    skos:inScheme ascedcs: ;
    skos:narrower asced:080901,
        asced:080903,
        asced:080905,
        asced:080999 ;
    skos:notation "0809" ;
    skos:prefLabel "Office Studies"@en .

asced:0811 a skos:Concept ;
    dcterms:created "2025-08-01T01:49:08.141000+00:00"^^xsd:dateTime ;
    dcterms:modified "2025-08-05T22:48:08.012000+00:00"^^xsd:dateTime ;
    skos:broader asced:08 ;
    skos:definition "Banking, Finance and Related Fields disciplines covering key subfields such as Banking and Finance and Insurance and Actuarial Studies." ;
    skos:inScheme ascedcs: ;
    skos:narrower asced:081101,
        asced:081103,
        asced:081105,
        asced:081199 ;
    skos:notation "0811" ;
    skos:prefLabel "Banking, Finance and Related Fields"@en .

asced:0911 a skos:Concept ;
    dcterms:created "2025-08-01T01:49:08.166000+00:00"^^xsd:dateTime ;
    dcterms:modified "2025-08-05T22:48:09.835000+00:00"^^xsd:dateTime ;
    skos:broader asced:09 ;
    skos:definition "Justice and Law Enforcement disciplines covering key subfields such as Justice Administration, Legal Studies, and Police Studies." ;
    skos:inScheme ascedcs: ;
    skos:narrower asced:091101,
        asced:091103,
        asced:091105,
        asced:091199 ;
    skos:notation "0911" ;
    skos:prefLabel "Justice and Law Enforcement"@en .

asced:0999 a skos:Concept ;
    dcterms:created "2025-08-01T01:49:08.183000+00:00"^^xsd:dateTime ;
    dcterms:modified "2025-08-05T22:48:10.137000+00:00"^^xsd:dateTime ;
    skos:broader asced:09 ;
    skos:definition "Other Society and Culture disciplines covering key subfields such as Criminology, Family and Consumer Studies, and Security Services." ;
    skos:inScheme ascedcs: ;
    skos:narrower asced:099901,
        asced:099903,
        asced:099905,
        asced:099999 ;
    skos:notation "0999" ;
    skos:prefLabel "Other Society and Culture"@en .

asced:1001 a skos:Concept ;
    dcterms:created "2025-08-01T01:49:08.187000+00:00"^^xsd:dateTime ;
    dcterms:modified "2025-08-05T22:48:12.743000+00:00"^^xsd:dateTime ;
    skos:broader asced:10 ;
    skos:definition "Performing Arts disciplines covering key subfields such as Dance, Drama and Theatre Studies, and Music." ;
    skos:inScheme ascedcs: ;
    skos:narrower asced:100101,
        asced:100103,
        asced:100105,
        asced:100199 ;
    skos:notation "1001" ;
    skos:prefLabel "Performing Arts"@en .

asced:1005 a skos:Concept ;
    dcterms:created "2025-08-01T01:49:08.195000+00:00"^^xsd:dateTime ;
    dcterms:modified "2025-08-05T22:48:12.834000+00:00"^^xsd:dateTime ;
    skos:broader asced:10 ;
    skos:definition "Graphic and Design Studies disciplines covering key subfields such as Fashion Design, Graphic Arts and Design Studies, and Textile Design." ;
    skos:inScheme ascedcs: ;
    skos:narrower asced:100501,
        asced:100503,
        asced:100505,
        asced:100599 ;
    skos:notation "1005" ;
    skos:prefLabel "Graphic and Design Studies"@en .

asced:12 a skos:Concept ;
    dcterms:created "2025-08-01T01:49:08.209000+00:00"^^xsd:dateTime ;
    dcterms:modified "2025-08-05T22:48:14.331000+00:00"^^xsd:dateTime ;
    skos:inScheme ascedcs: ;
    skos:narrower asced:1201,
        asced:1203,
        asced:1205,
        asced:1299 ;
    skos:notation "12" ;
    skos:prefLabel "MIXED FIELD PROGRAMMES"@en ;
    skos:topConceptOf ascedcs: .

asced:1201 a skos:Concept ;
    dcterms:created "2025-08-01T01:49:08.210000+00:00"^^xsd:dateTime ;
    dcterms:modified "2025-08-05T22:48:14.369000+00:00"^^xsd:dateTime ;
    skos:broader asced:12 ;
    skos:definition "General Education Programmes disciplines covering key subfields such as General Primary and Secondary Education Programmes and Learning Skills Programmes." ;
    skos:inScheme ascedcs: ;
    skos:narrower asced:120101,
        asced:120103,
        asced:120105,
        asced:120199 ;
    skos:notation "1201" ;
    skos:prefLabel "General Education Programmes"@en .

asced:1203 a skos:Concept ;
    dcterms:created "2025-08-01T01:49:08.212000+00:00"^^xsd:dateTime ;
    dcterms:modified "2025-08-05T22:48:14.412000+00:00"^^xsd:dateTime ;
    skos:broader asced:12 ;
    skos:definition "Social Skills Programmes disciplines covering key subfields such as Parental Education Programmes and Social and Interpersonal Skills Programmes." ;
    skos:inScheme ascedcs: ;
    skos:narrower asced:120301,
        asced:120303,
        asced:120305,
        asced:120399 ;
    skos:notation "1203" ;
    skos:prefLabel "Social Skills Programmes"@en .

asced:1205 a skos:Concept ;
    dcterms:created "2025-08-01T01:49:08.215000+00:00"^^xsd:dateTime ;
    dcterms:modified "2025-08-05T22:48:14.460000+00:00"^^xsd:dateTime ;
    skos:broader asced:12 ;
    skos:definition "Employment Skills Programmes disciplines covering key subfields such as Career Development Programmes, Job Search Skills Programmes, and Work Practices Programmes." ;
    skos:inScheme ascedcs: ;
    skos:narrower asced:120501,
        asced:120503,
        asced:120505,
        asced:120599 ;
    skos:notation "1205" ;
    skos:prefLabel "Employment Skills Programmes"@en .

asced:0203 a skos:Concept ;
    dcterms:created "2025-08-01T01:49:07.951000+00:00"^^xsd:dateTime ;
    dcterms:modified "2025-08-05T22:47:57.101000+00:00"^^xsd:dateTime ;
    skos:broader asced:02 ;
    skos:definition "Information Systems disciplines covering key subfields such as Conceptual Modelling, Database Management, and Decision Support Systems." ;
    skos:inScheme ascedcs: ;
    skos:narrower asced:020301,
        asced:020303,
        asced:020305,
        asced:020307,
        asced:020399 ;
    skos:notation "0203" ;
    skos:prefLabel "Information Systems"@en .

asced:0303 a skos:Concept ;
    dcterms:created "2025-08-01T01:49:07.973000+00:00"^^xsd:dateTime ;
    dcterms:modified "2025-08-05T22:47:58.196000+00:00"^^xsd:dateTime ;
    skos:broader asced:03 ;
    skos:definition "Process and Resources Engineering disciplines covering key subfields such as Chemical Engineering, Food Processing Technology, and Materials Engineering." ;
    skos:inScheme ascedcs: ;
    skos:narrower asced:030301,
        asced:030303,
        asced:030305,
        asced:030307,
        asced:030399 ;
    skos:notation "0303" ;
    skos:prefLabel "Process and Resources Engineering"@en .

asced:0315 a skos:Concept ;
    dcterms:created "2025-08-01T01:49:08.017000+00:00"^^xsd:dateTime ;
    dcterms:modified "2025-08-05T22:47:58.511000+00:00"^^xsd:dateTime ;
    skos:broader asced:03 ;
    skos:definition "Aerospace Engineering and Technology disciplines covering key subfields such as Aerospace Engineering, Air Traffic Control, and Aircraft Maintenance Engineering." ;
    skos:inScheme ascedcs: ;
    skos:narrower asced:031501,
        asced:031503,
        asced:031505,
        asced:031507,
        asced:031599 ;
    skos:notation "0315" ;
    skos:prefLabel "Aerospace Engineering and Technology"@en .

asced:0401 a skos:Concept ;
    dcterms:created "2025-08-01T01:49:08.031000+00:00"^^xsd:dateTime ;
    dcterms:modified "2025-08-05T22:48:02.059000+00:00"^^xsd:dateTime ;
    skos:broader asced:04 ;
    skos:definition "Architecture and Urban Environment disciplines covering key subfields such as Architecture, Interior and Environmental Design, and Landscape Architecture." ;
    skos:inScheme ascedcs: ;
    skos:narrower asced:040101,
        asced:040103,
        asced:040105,
        asced:040107,
        asced:040199 ;
    skos:notation "0401" ;
    skos:prefLabel "Architecture and Urban Environment"@en .

asced:0699 a skos:Concept ;
    dcterms:created "2025-08-01T01:49:08.108000+00:00"^^xsd:dateTime ;
    dcterms:modified "2025-08-05T22:48:04.528000+00:00"^^xsd:dateTime ;
    skos:broader asced:06 ;
    skos:definition "Other Health disciplines covering key subfields such as First Aid, Human Movement, and Nutrition and Dietetics." ;
    skos:inScheme ascedcs: ;
    skos:narrower asced:069901,
        asced:069903,
        asced:069905,
        asced:069907,
        asced:069999 ;
    skos:notation "0699" ;
    skos:prefLabel "Other Health"@en .

asced:10 a skos:Concept ;
    dcterms:created "2025-08-01T01:49:08.187000+00:00"^^xsd:dateTime ;
    dcterms:modified "2025-08-05T22:48:12.693000+00:00"^^xsd:dateTime ;
    skos:inScheme ascedcs: ;
    skos:narrower asced:1001,
        asced:1003,
        asced:1005,
        asced:1007,
        asced:1099 ;
    skos:notation "10" ;
    skos:prefLabel "CREATIVE ARTS"@en ;
    skos:topConceptOf ascedcs: .

asced:1007 a skos:Concept ;
    dcterms:created "2025-08-01T01:49:08.198000+00:00"^^xsd:dateTime ;
    dcterms:modified "2025-08-05T22:48:12.873000+00:00"^^xsd:dateTime ;
    skos:broader asced:10 ;
    skos:definition "Communication and Media Studies disciplines covering key subfields such as Audio Visual Studies, Journalism, and Verbal Communication." ;
    skos:inScheme ascedcs: ;
    skos:narrower asced:100701,
        asced:100703,
        asced:100705,
        asced:100707,
        asced:100799 ;
    skos:notation "1007" ;
    skos:prefLabel "Communication and Media Studies"@en .

asced:01 a skos:Concept ;
    dcterms:created "2025-08-01T01:49:07.897000+00:00"^^xsd:dateTime ;
    dcterms:modified "2025-08-05T22:47:54.907000+00:00"^^xsd:dateTime ;
    skos:inScheme ascedcs: ;
    skos:narrower asced:0101,
        asced:0103,
        asced:0105,
        asced:0107,
        asced:0109,
        asced:0199 ;
    skos:notation "01" ;
    skos:prefLabel "NATURAL AND PHYSICAL SCIENCES"@en ;
	skos:closeMatch <https://linked.data.gov.au/def/anzsrc-for/2020/31> , <https://linked.data.gov.au/def/anzsrc-for/2020/37> , <https://linked.data.gov.au/def/anzsrc-for/2020/51> ;
    skos:topConceptOf ascedcs: .

asced:0199 a skos:Concept ;
    dcterms:created "2025-08-01T01:49:07.931000+00:00"^^xsd:dateTime ;
    dcterms:modified "2025-08-05T22:47:55.323000+00:00"^^xsd:dateTime ;
    skos:broader asced:01 ;
    skos:definition "Other Natural and Physical Sciences disciplines covering key subfields such as Food Science and Biotechnology, Forensic Science, and Laboratory Technology." ;
    skos:inScheme ascedcs: ;
    skos:narrower asced:019901,
        asced:019903,
        asced:019905,
        asced:019907,
        asced:019909,
        asced:019999 ;
    skos:notation "0199" ;
    skos:prefLabel "Other Natural and Physical Sciences"@en .

asced:0399 a skos:Concept ;
    dcterms:created "2025-08-01T01:49:08.025000+00:00"^^xsd:dateTime ;
    dcterms:modified "2025-08-05T22:47:58.612000+00:00"^^xsd:dateTime ;
    skos:broader asced:03 ;
    skos:definition "Other Engineering and Related Technologies disciplines covering key subfields such as Biomedical Engineering, Cleaning, and Environmental Engineering." ;
    skos:inScheme ascedcs: ;
    skos:narrower asced:039901,
        asced:039903,
        asced:039905,
        asced:039907,
        asced:039909,
        asced:039999 ;
    skos:notation "0399" ;
    skos:prefLabel "Other Engineering and Related Technologies"@en .

asced:05 a skos:Concept ;
    dcterms:created "2025-08-01T01:49:08.048000+00:00"^^xsd:dateTime ;
    dcterms:modified "2025-08-05T22:48:03.137000+00:00"^^xsd:dateTime ;
    skos:inScheme ascedcs: ;
    skos:narrower asced:0501,
        asced:0503,
        asced:0505,
        asced:0507,
        asced:0509,
        asced:0599 ;
    skos:notation "05" ;
    skos:prefLabel "AGRICULTURE, ENVIRONMENTAL AND RELATED STUDIES"@en ;
    skos:topConceptOf ascedcs: .

asced:0805 a skos:Concept ;
    dcterms:created "2025-08-01T01:49:08.132000+00:00"^^xsd:dateTime ;
    dcterms:modified "2025-08-05T22:48:07.894000+00:00"^^xsd:dateTime ;
    skos:broader asced:08 ;
    skos:definition "Sales and Marketing disciplines covering key subfields such as Advertising, Marketing, and Public Relations." ;
    skos:inScheme ascedcs: ;
    skos:narrower asced:080501,
        asced:080503,
        asced:080505,
        asced:080507,
        asced:080509,
        asced:080599 ;
    skos:notation "0805" ;
    skos:prefLabel "Sales and Marketing"@en .

asced:1003 a skos:Concept ;
    dcterms:created "2025-08-01T01:49:08.191000+00:00"^^xsd:dateTime ;
    dcterms:modified "2025-08-05T22:48:12.791000+00:00"^^xsd:dateTime ;
    skos:broader asced:10 ;
    skos:definition "Visual Arts and Crafts disciplines covering key subfields such as Crafts, Fine Arts, and Floristry." ;
    skos:inScheme ascedcs: ;
    skos:narrower asced:100301,
        asced:100303,
        asced:100305,
        asced:100307,
        asced:100309,
        asced:100399 ;
    skos:notation "1003" ;
    skos:prefLabel "Visual Arts and Crafts"@en .

asced:0613 a skos:Concept ;
    dcterms:created "2025-08-01T01:49:08.088000+00:00"^^xsd:dateTime ;
    dcterms:modified "2025-08-05T22:48:04.356000+00:00"^^xsd:dateTime ;
    skos:broader asced:06 ;
    skos:definition "Public Health disciplines covering key subfields such as Community Health, Environmental Health, and Epidemiology." ;
    skos:inScheme ascedcs: ;
    skos:narrower asced:061301,
        asced:061303,
        asced:061305,
        asced:061307,
        asced:061309,
        asced:061311,
        asced:061399 ;
    skos:notation "0613" ;
    skos:prefLabel "Public Health"@en .

asced:08 a skos:Concept ;
    dcterms:created "2025-08-01T01:49:08.122000+00:00"^^xsd:dateTime ;
    dcterms:modified "2025-08-05T22:48:07.771000+00:00"^^xsd:dateTime ;
    skos:inScheme ascedcs: ;
    skos:narrower asced:0801,
        asced:0803,
        asced:0805,
        asced:0807,
        asced:0809,
        asced:0811,
        asced:0899 ;
    skos:notation "08" ;
    skos:prefLabel "MANAGEMENT AND COMMERCE"@en ;
    skos:topConceptOf ascedcs: .

asced:1101 a skos:Concept ;
    dcterms:created "2025-08-01T01:49:08.203000+00:00"^^xsd:dateTime ;
    dcterms:modified "2025-08-05T22:48:13.845000+00:00"^^xsd:dateTime ;
    skos:broader asced:11 ;
    skos:definition "Food and Hospitality disciplines covering key subfields such as Baking and Pastrymaking, Butchery, and Cookery." ;
    skos:inScheme ascedcs: ;
    skos:narrower asced:110101,
        asced:110103,
        asced:110105,
        asced:110107,
        asced:110109,
        asced:110111,
        asced:110199 ;
    skos:notation "1101" ;
    skos:prefLabel "Food and Hospitality"@en .

asced:0107 a skos:Concept ;
    dcterms:created "2025-08-01T01:49:07.911000+00:00"^^xsd:dateTime ;
    dcterms:modified "2025-08-05T22:47:55.208000+00:00"^^xsd:dateTime ;
    skos:broader asced:01 ;
    skos:definition "Earth Sciences disciplines covering key subfields such as Atmospheric Sciences, Geochemistry, and Geology." ;
    skos:inScheme ascedcs: ;
    skos:narrower asced:010701,
        asced:010703,
        asced:010705,
        asced:010707,
        asced:010709,
        asced:010711,
        asced:010713,
        asced:010799 ;
    skos:notation "0107" ;
    skos:prefLabel "Earth Sciences"@en .

asced:0309 a skos:Concept ;
    dcterms:created "2025-08-01T01:49:07.996000+00:00"^^xsd:dateTime ;
    dcterms:modified "2025-08-05T22:47:58.353000+00:00"^^xsd:dateTime ;
    skos:broader asced:03 ;
    skos:definition "Civil Engineering disciplines covering key subfields such as Building Services Engineering, Construction Engineering, and Geotechnical Engineering." ;
    skos:inScheme ascedcs: ;
    skos:narrower asced:030901,
        asced:030903,
        asced:030905,
        asced:030907,
        asced:030909,
        asced:030911,
        asced:030913,
        asced:030999 ;
    skos:notation "0309" ;
    skos:prefLabel "Civil Engineering"@en .

asced:0617 a skos:Concept ;
    dcterms:created "2025-08-01T01:49:08.095000+00:00"^^xsd:dateTime ;
    dcterms:modified "2025-08-05T22:48:04.446000+00:00"^^xsd:dateTime ;
    skos:broader asced:06 ;
    skos:definition "Rehabilitation Therapies disciplines covering key subfields such as Audiology, Chiropractic and Osteopathy, and Massage Therapy." ;
    skos:inScheme ascedcs: ;
    skos:narrower asced:061701,
        asced:061703,
        asced:061705,
        asced:061707,
        asced:061709,
        asced:061711,
        asced:061713,
        asced:061799 ;
    skos:notation "0617" ;
    skos:prefLabel "Rehabilitation Therapies"@en .

asced:0903 a skos:Concept ;
    dcterms:created "2025-08-01T01:49:08.148000+00:00"^^xsd:dateTime ;
    dcterms:modified "2025-08-05T22:48:09.631000+00:00"^^xsd:dateTime ;
    skos:broader asced:09 ;
    skos:definition "Studies in Human Society disciplines covering key subfields such as Anthropology, Archaeology, and Gender Specific Studies." ;
    skos:inScheme ascedcs: ;
    skos:narrower asced:090301,
        asced:090303,
        asced:090305,
        asced:090307,
        asced:090309,
        asced:090311,
        asced:090313,
        asced:090399 ;
    skos:notation "0903" ;
    skos:prefLabel "Studies in Human Society"@en .

asced:0909 a skos:Concept ;
    dcterms:created "2025-08-01T01:49:08.161000+00:00"^^xsd:dateTime ;
    dcterms:modified "2025-08-05T22:48:09.784000+00:00"^^xsd:dateTime ;
    skos:broader asced:09 ;
    skos:definition "Law disciplines covering key subfields such as Business and Commercial Law, Constitutional Law, and Criminal Law." ;
    skos:inScheme ascedcs: ;
    skos:narrower asced:090901,
        asced:090903,
        asced:090905,
        asced:090907,
        asced:090909,
        asced:090911,
        asced:090913,
        asced:090999 ;
    skos:notation "0909" ;
    skos:prefLabel "Law"@en .

asced:0109 a skos:Concept ;
    dcterms:created "2025-08-01T01:49:07.921000+00:00"^^xsd:dateTime ;
    dcterms:modified "2025-08-05T22:47:55.268000+00:00"^^xsd:dateTime ;
    skos:broader asced:01 ;
    skos:definition "Biological Sciences disciplines covering key subfields such as Biochemistry and Cell Biology, Botany, and Ecology and Evolution." ;
    skos:inScheme ascedcs: ;
    skos:narrower asced:010901,
        asced:010903,
        asced:010905,
        asced:010907,
        asced:010909,
        asced:010911,
        asced:010913,
        asced:010915,
        asced:010999 ;
    skos:notation "0109" ;
    skos:prefLabel "Biological Sciences"@en .

asced:0305 a skos:Concept ;
    dcterms:created "2025-08-01T01:49:07.978000+00:00"^^xsd:dateTime ;
    dcterms:modified "2025-08-05T22:47:58.248000+00:00"^^xsd:dateTime ;
    skos:broader asced:03 ;
    skos:definition "Automotive Engineering and Technology disciplines covering key subfields such as Automotive Body Construction, Automotive Electrics and Electronics, and Automotive Engineering." ;
    skos:inScheme ascedcs: ;
    skos:narrower asced:030501,
        asced:030503,
        asced:030505,
        asced:030507,
        asced:030509,
        asced:030511,
        asced:030513,
        asced:030515,
        asced:030599 ;
    skos:notation "0305" ;
    skos:prefLabel "Automotive Engineering and Technology"@en .

asced:0603 a skos:Concept ;
    dcterms:created "2025-08-01T01:49:08.071000+00:00"^^xsd:dateTime ;
    dcterms:modified "2025-08-05T22:48:04.137000+00:00"^^xsd:dateTime ;
    skos:broader asced:06 ;
    skos:definition "Nursing disciplines covering key subfields such as Aged Care Nursing, Community Nursing, and Critical Care Nursing." ;
    skos:inScheme ascedcs: ;
    skos:narrower asced:060301,
        asced:060303,
        asced:060305,
        asced:060307,
        asced:060309,
        asced:060311,
        asced:060313,
        asced:060315,
        asced:060399 ;
    skos:notation "0603" ;
    skos:prefLabel "Nursing"@en .

asced:0905 a skos:Concept ;
    dcterms:created "2025-08-01T01:49:08.154000+00:00"^^xsd:dateTime ;
    dcterms:modified "2025-08-05T22:48:09.680000+00:00"^^xsd:dateTime ;
    skos:broader asced:09 ;
    skos:definition "Human Welfare Studies and Services disciplines covering key subfields such as Care for the Aged and Care for the Disabled." ;
    skos:inScheme ascedcs: ;
    skos:narrower asced:090501,
        asced:090503,
        asced:090505,
        asced:090507,
        asced:090509,
        asced:090511,
        asced:090513,
        asced:090515,
        asced:090599 ;
    skos:notation "0905" ;
    skos:prefLabel "Human Welfare Studies and Services"@en .

asced:03 a skos:Concept ;
    dcterms:created "2025-08-01T01:49:07.961000+00:00"^^xsd:dateTime ;
    dcterms:modified "2025-08-05T22:47:58.089000+00:00"^^xsd:dateTime ;
    skos:inScheme ascedcs: ;
    skos:narrower asced:0301,
        asced:0303,
        asced:0305,
        asced:0307,
        asced:0309,
        asced:0311,
        asced:0313,
        asced:0315,
        asced:0317,
        asced:0399 ;
    skos:notation "03" ;
    skos:prefLabel "ENGINEERING AND RELATED TECHNOLOGIES"@en ;
	skos:closeMatch <https://linked.data.gov.au/def/anzsrc-for/2020/40> ;
    skos:topConceptOf ascedcs: .

asced:0301 a skos:Concept ;
    dcterms:created "2025-08-01T01:49:07.962000+00:00"^^xsd:dateTime ;
    dcterms:modified "2025-08-05T22:47:58.142000+00:00"^^xsd:dateTime ;
    skos:broader asced:03 ;
    skos:definition "Manufacturing Engineering and Technology disciplines covering key subfields such as Cabinet Making, Footwear Making, and Furniture Polishing." ;
    skos:inScheme ascedcs: ;
    skos:narrower asced:030101,
        asced:030103,
        asced:030105,
        asced:030107,
        asced:030109,
        asced:030111,
        asced:030113,
        asced:030115,
        asced:030117,
        asced:030199 ;
    skos:notation "0301" ;
    skos:prefLabel "Manufacturing Engineering and Technology"@en .

asced:0307 a skos:Concept ;
    dcterms:created "2025-08-01T01:49:07.987000+00:00"^^xsd:dateTime ;
    dcterms:modified "2025-08-05T22:47:58.300000+00:00"^^xsd:dateTime ;
    skos:broader asced:03 ;
    skos:definition "Mechanical and Industrial Engineering and Technology disciplines covering key subfields such as Boilermaking and Welding, Industrial Engineering, and Mechanical Engineering." ;
    skos:inScheme ascedcs: ;
    skos:narrower asced:030701,
        asced:030703,
        asced:030705,
        asced:030707,
        asced:030709,
        asced:030711,
        asced:030713,
        asced:030715,
        asced:030717,
        asced:030799 ;
    skos:notation "0307" ;
    skos:prefLabel "Mechanical and Industrial Engineering and Technology"@en .

asced:0313 a skos:Concept ;
    dcterms:created "2025-08-01T01:49:08.008000+00:00"^^xsd:dateTime ;
    dcterms:modified "2025-08-05T22:47:58.456000+00:00"^^xsd:dateTime ;
    skos:broader asced:03 ;
    skos:definition "Electrical and Electronic Engineering and Technology disciplines covering key subfields such as Communications Equipment Installation and Maintenance and Communications Technologies." ;
    skos:inScheme ascedcs: ;
    skos:narrower asced:031301,
        asced:031303,
        asced:031305,
        asced:031307,
        asced:031309,
        asced:031311,
        asced:031313,
        asced:031315,
        asced:031317,
        asced:031399 ;
    skos:notation "0313" ;
    skos:prefLabel "Electrical and Electronic Engineering and Technology"@en .

asced:0701 a skos:Concept ;
    dcterms:created "2025-08-01T01:49:08.112000+00:00"^^xsd:dateTime ;
    dcterms:modified "2025-08-05T22:48:07.130000+00:00"^^xsd:dateTime ;
    skos:broader asced:07 ;
    skos:definition "Teacher Education disciplines covering key subfields such as English as a Second Language Teaching and Nursing Education Teacher Training." ;
    skos:inScheme ascedcs: ;
    skos:narrower asced:070101,
        asced:070103,
        asced:070105,
        asced:070107,
        asced:070109,
        asced:070111,
        asced:070113,
        asced:070115,
        asced:070117,
        asced:070199 ;
    skos:notation "0701" ;
    skos:prefLabel "Teacher Education"@en .

asced:0201 a skos:Concept ;
    dcterms:created "2025-08-01T01:49:07.940000+00:00"^^xsd:dateTime ;
    dcterms:modified "2025-08-05T22:47:57.052000+00:00"^^xsd:dateTime ;
    skos:broader asced:02 ;
    skos:definition "Computer Science disciplines covering key subfields such as Algorithms, Artificial Intelligence, and Compiler Construction." ;
    skos:inScheme ascedcs: ;
    skos:narrower asced:020101,
        asced:020103,
        asced:020105,
        asced:020107,
        asced:020109,
        asced:020111,
        asced:020113,
        asced:020115,
        asced:020117,
        asced:020119,
        asced:020199 ;
    skos:notation "0201" ;
    skos:prefLabel "Computer Science"@en .

asced:06 a skos:Concept ;
    dcterms:created "2025-08-01T01:49:08.061000+00:00"^^xsd:dateTime ;
    dcterms:modified "2025-08-05T22:48:04.044000+00:00"^^xsd:dateTime ;
    skos:inScheme ascedcs: ;
    skos:narrower asced:0601,
        asced:0603,
        asced:0605,
        asced:0607,
        asced:0609,
        asced:0611,
        asced:0613,
        asced:0615,
        asced:0617,
        asced:0619,
        asced:0699 ;
    skos:notation "06" ;
    skos:prefLabel "HEALTH"@en ;
    skos:topConceptOf ascedcs: .

asced:0601 a skos:Concept ;
    dcterms:created "2025-08-01T01:49:08.062000+00:00"^^xsd:dateTime ;
    dcterms:modified "2025-08-05T22:48:04.091000+00:00"^^xsd:dateTime ;
    skos:broader asced:06 ;
    skos:definition "Medical Studies disciplines covering key subfields such as Anaesthesiology, General Medicine, and General Practice." ;
    skos:inScheme ascedcs: ;
    skos:narrower asced:060101,
        asced:060103,
        asced:060105,
        asced:060107,
        asced:060109,
        asced:060111,
        asced:060113,
        asced:060115,
        asced:060117,
        asced:060119,
        asced:060199 ;
    skos:notation "0601" ;
    skos:prefLabel "Medical Studies"@en .

asced:09 a skos:Concept ;
    dcterms:created "2025-08-01T01:49:08.146000+00:00"^^xsd:dateTime ;
    dcterms:modified "2025-08-05T22:48:09.527000+00:00"^^xsd:dateTime ;
    skos:inScheme ascedcs: ;
    skos:narrower asced:0901,
        asced:0903,
        asced:0905,
        asced:0907,
        asced:0909,
        asced:0911,
        asced:0913,
        asced:0915,
        asced:0917,
        asced:0919,
        asced:0921,
        asced:0999 ;
    skos:notation "09" ;
    skos:prefLabel "SOCIETY AND CULTURE"@en ;
    skos:topConceptOf ascedcs: .

asced:0803 a skos:Concept ;
    dcterms:created "2025-08-01T01:49:08.124000+00:00"^^xsd:dateTime ;
    dcterms:modified "2025-08-05T22:48:07.850000+00:00"^^xsd:dateTime ;
    skos:broader asced:08 ;
    skos:definition "Business and Management disciplines covering key subfields such as Business Management, Farm Management and Agribusiness, and Hospitality Management." ;
    skos:inScheme ascedcs: ;
    skos:narrower asced:080301,
        asced:080303,
        asced:080305,
        asced:080307,
        asced:080309,
        asced:080311,
        asced:080313,
        asced:080315,
        asced:080317,
        asced:080319,
        asced:080321,
        asced:080323,
        asced:080399 ;
    skos:notation "0803" ;
    skos:prefLabel "Business and Management"@en .

asced:0915 a skos:Concept ;
    dcterms:created "2025-08-01T01:49:08.170000+00:00"^^xsd:dateTime ;
    dcterms:modified "2025-08-05T22:48:09.938000+00:00"^^xsd:dateTime ;
    skos:broader asced:09 ;
    skos:definition "Language and Literature disciplines covering key subfields such as Australian Indigenous Languages, Eastern Asian Languages, and Eastern European Languages." ;
    skos:inScheme ascedcs: ;
    skos:narrower asced:091501,
        asced:091503,
        asced:091505,
        asced:091507,
        asced:091509,
        asced:091511,
        asced:091513,
        asced:091515,
        asced:091517,
        asced:091519,
        asced:091521,
        asced:091523,
        asced:091599 ;
    skos:notation "0915" ;
    skos:prefLabel "Language and Literature"@en .

asced:0403 a skos:Concept ;
    dcterms:created "2025-08-01T01:49:08.036000+00:00"^^xsd:dateTime ;
    dcterms:modified "2025-08-05T22:48:02.100000+00:00"^^xsd:dateTime ;
    skos:broader asced:04 ;
    skos:definition "Building disciplines covering key subfields such as Bricklaying and Stonemasonry, Building Construction Economics, and Building Construction Management." ;
    skos:inScheme ascedcs: ;
    skos:narrower asced:040301,
        asced:040303,
        asced:040305,
        asced:040307,
        asced:040309,
        asced:040311,
        asced:040313,
        asced:040315,
        asced:040317,
        asced:040319,
        asced:040321,
        asced:040323,
        asced:040325,
        asced:040327,
        asced:040329,
        asced:040399 ;
    skos:notation "0403" ;
    skos:prefLabel "Building"@en .

ascedcs: a skos:ConceptScheme ;
    dcterms:created "2001-08-22"^^xsd:date ;
    dcterms:creator abs: ;
    dcterms:publisher dewr: ;
    dcterms:title "ASCED"@en ;
    skos:altLabel "Australian Standard Classification of Education"@en ;
    skos:definition "The Australian Bureau of Statistics (ABS) has developed the Australian Standard Classification of Education (ASCED) for use in the collection, storage and dissemination of statistical and administrative data relating to educational activity undertaken in Australia."@en ;
    skos:hasTopConcept asced:01,
        asced:02,
        asced:03,
        asced:04,
        asced:05,
        asced:06,
        asced:07,
        asced:08,
        asced:09,
        asced:10,
        asced:11,
        asced:12 ;
    skos:historyNote "Presented here for the first time in RDF by Jobs and Skills Australia"@en ;
    skos:prefLabel "ASCED"@en ;
    schema:citation "https://www.abs.gov.au/statistics/classifications/australian-standard-classification-education-asced"^^xsd:anyURI,
        "https://www.abs.gov.au/statistics/classifications/australian-standard-classification-education-asced/2001"^^xsd:anyURI .

