@prefix attributes: <https://rdf.sfia-online.org/9/attributes/> .
@prefix categories: <https://rdf.sfia-online.org/9/categories/> .
@prefix dcterms: <http://purl.org/dc/terms/> .
@prefix esco: <http://data.europa.eu/esco/model#> .
@prefix jsa: <https://linked.data.gov.au/org/jsa> .
@prefix lor: <https://rdf.sfia-online.org/9/lor/> .
@prefix lorcs: <https://rdf.sfia-online.org/9/lor> .
@prefix owl: <http://www.w3.org/2002/07/owl#> .
@prefix rdfs: <http://www.w3.org/2000/01/rdf-schema#> .
@prefix schema: <https://schema.org/> .
@prefix sfia: <https://rdf.sfia-online.org/9/ontology/> .
@prefix sfialevels: <https://rdf.sfia-online.org/9/skilllevels/> .
@prefix skills: <https://rdf.sfia-online.org/9/skills/> .
@prefix skillcs: <http://example.com/skillcs> .
@prefix skos: <http://www.w3.org/2004/02/skos/core#> .
@prefix xsd: <http://www.w3.org/2001/XMLSchema#> .
@prefix sfiaorg: <https://sfia-online.org> .

sfiaorg: a schema:Organization ;
schema:name "SFIA Foundation" ;
schema:url "https://sfia-online.org"^^xsd:anyURI
.

jsa:
a schema:Organization ;
schema:name "Jobs and Skills Australia"@en ;
schema:alternateName "JSA"@en ;
schema:url "https://www.jobsandskills.gov.au"^^xsd:anyURI
.

skillcs: a skos:ConceptScheme ;
skos:prefLabel "SFIA skills concept scheme"@en ;
skos:definition "SFIA skills concept scheme" ;
skos:historyNote "This concept scheme is added to the sfia RDF for conformance with SKOS"@en ;
dcterms:created "2025-10-17"^^xsd:gYear ;
dcterms:creator sfiaorg: ;
dcterms:publisher jsa:
.

attributes:ADAP a owl:AnnotationProperty ;
    rdfs:label "Adaptability"@en ;
    rdfs:comment "Adjusting to change and persisting through challenges at personal, team and organisational levels."@en ;
    skos:notation "ADAP" ;
    sfia:attributeGuidanceNotes """Adaptability and resilience in SFIA represent a progression from personal flexibility to shaping organisational agility. It involves:

being open to change and new ways of working
adjusting to different team dynamics and work requirements
adopting new methods and technologies proactively
enabling others to adapt to challenges
leading teams through transitions
driving significant organisational changes
embedding adaptability into organisational culture.

Effective adaptability and resilience encompass openness to change, proactive learning and the ability to maintain focus on objectives during transitions. It also involves supporting others through change and creating an environment where innovation and flexibility thrive.
As professionals advance, their ability to drive and manage change increasingly shapes organisational resilience and long-term success in dynamic environments."""@en ;
    sfia:attributeType "Business skills/Behavioural factors"@en ;
dcterms:source "https://sfia-online.org/en/shortcode/9/ADAP"^^xsd:anyURI .

attributes:AUTO a owl:AnnotationProperty ;
    rdfs:label "Autonomy"@en ;
    rdfs:comment "The level of independence, discretion and accountability for results in your role."@en ;
    skos:notation "AUTO" ;
    sfia:attributeGuidanceNotes """Autonomy in SFIA represents a progression from following instructions to setting organisational strategy. It involves:

working under varying levels of direction and supervision
making independent decisions in line with responsibility
taking accountability for actions and their outcomes
delegating tasks and responsibilities appropriately
setting personal, team, or organisational goals.

Effective autonomy encompasses decision-making skills, self-management and the ability to balance independence with organisational goals. Autonomy is closely linked with skills such as decision-making, leadership, and planning.
As professionals advance, their level of autonomy increasingly shapes their ability to drive change, innovate and contribute to organisational success. As professionals advance, their autonomy enables them to lead initiatives and drive strategic outcomes.  At higher levels, individuals shape their role and make decisions that have a wider organisational impact, with minimal supervision."""@en ;
    sfia:attributeType "Attributes"@en ;
dcterms:source "https://sfia-online.org/en/shortcode/9/AUTO"^^xsd:anyURI .

attributes:COLL a owl:AnnotationProperty ;
    rdfs:label "Collaboration"@en ;
    rdfs:comment "Working effectively with others, sharing resources and coordinating efforts to achieve shared objectives."@en ;
    skos:notation "COLL" ;
    sfia:attributeGuidanceNotes """Collaboration in SFIA represents a progression from basic team interaction to strategic partnerships and stakeholder management. It involves:

working cooperatively within immediate teams
sharing information and resources effectively
coordinating efforts to achieve common goals
facilitating cross-functional teamwork
building influential relationships across the organisation
establishing and managing strategic partnerships.

Effective collaboration encompasses communication, perspective-taking, and the ability to align diverse viewpoints towards common objectives. It also involves creating an environment that encourages knowledge sharing and collective problem-solving.
As professionals advance, their collaborative skills evolve from supporting team goals to shaping organisational culture, driving innovation, and enhancing the organisation's ability to navigate complex challenges. At higher levels, collaboration extends to influencing industry-wide cooperation and partnerships."""@en ;
    sfia:attributeType "Business skills/Behavioural factors"@en ;
dcterms:source "https://sfia-online.org/en/shortcode/9/COLL"^^xsd:anyURI .

attributes:COMM a owl:AnnotationProperty ;
    rdfs:label "Communication"@en ;
    rdfs:comment "Exchanging information, ideas and insights clearly to enable mutual understanding and cooperation."@en ;
    skos:notation "COMM" ;
    sfia:attributeGuidanceNotes """Communication in SFIA represents a progression from basic team interaction to complex, organisation-wide influence and external engagement. It involves:

communicating within immediate teams
exchanging information and ideas clearly
verbal and written skills, active listening, and the ability to use communication tools and platforms appropriately
adapting communication style to diverse audiences, both technical and non-technical
articulating complex concepts in a way that enables informed decision-making
influencing strategy through effective dialogue with senior stakeholders.

As professionals advance, their communication skills evolve from simple information sharing within teams to influencing decisions at the highest levels of an organisation. This progression involves adapting communication to different audiences, including senior stakeholders and external partners, and shaping strategic outcomes through effective dialogue. At higher levels, professionals take on the responsibility of using communication to drive organisational direction and engage with industry leaders to achieve business objectives."""@en ;
    sfia:attributeType "Business skills/Behavioural factors"@en ;
dcterms:source "https://sfia-online.org/en/shortcode/9/COMM"^^xsd:anyURI .

attributes:COMP a owl:AnnotationProperty ;
    rdfs:label "Complexity"@en ;
    rdfs:comment "The range and intricacy of tasks and responsibilities that come with your role."@en ;
    skos:notation "COMP" ;
    sfia:attributeGuidanceNotes """Complexity in SFIA represents a progression from routine tasks to strategic leadership delivering business value. It involves:

handling increasingly varied and unpredictable work environments
addressing a growing range of technical or professional activities
solving progressively complex problems
managing diverse stakeholders
contributing to policy and strategy
leveraging emerging technologies for business value.

Effective management of complexity encompasses skills in problem solving, decision making and planning alongside technical or professional expertise.  This attribute reflects the range and intricacy of tasks and responsibilities in a role, progressing from routine activities to extensive strategic leadership. It can be measured by the level of problem-solving required, the nature and number of stakeholders involved, and the impact of decisions made.
As professionals advance, their ability to navigate and leverage complexity increasingly contributes to organisational innovation, efficiency and competitive advantage."""@en ;
    sfia:attributeType "Attributes"@en ;
dcterms:source "https://sfia-online.org/en/shortcode/9/COMP"^^xsd:anyURI .

attributes:CRTY a owl:AnnotationProperty ;
    rdfs:label "Creativity"@en ;
    rdfs:comment "Generating and applying innovative ideas to enhance processes, solve problems and drive organisational success."@en ;
    skos:notation "CRTY" ;
    sfia:attributeGuidanceNotes """Creativity in SFIA represents a progression from basic idea generation to driving strategic innovation. It involves:

generating novel ideas and solutions
applying innovative thinking to improve processes
solving complex problems creatively
encouraging and facilitating creative thinking in others
developing a culture of innovation
aligning creative initiatives with organisational strategy.

Effective creativity encompasses imaginative thinking, problem-solving skills and challenging conventional approaches. It thrives in environments that encourage calculated risk-taking and value innovative ideas.
As professionals advance, their role shifts from contributing to creative processes to inspiring and leading innovation at a strategic level. This evolution underscores the growing importance of creative thinking in driving organisational success and navigating complex challenges across various disciplines."""@en ;
    sfia:attributeType "Business skills/Behavioural factors"@en ;
dcterms:source "https://sfia-online.org/en/shortcode/9/CRTY"^^xsd:anyURI .

attributes:DECM a owl:AnnotationProperty ;
    rdfs:label "Decision-making"@en ;
    rdfs:comment "Applying critical thinking to evaluate options, assess risks and select the most appropriate course of action."@en ;
    skos:notation "DECM" ;
    sfia:attributeGuidanceNotes """Decision making in SFIA represents a progression from routine choices to strategic, high-impact decisions. It involves:

evaluating information and assessing risks
balancing intuition and logic
understanding organisational context
determining the best course of action
taking accountability for outcomes.

Effective decision making encompasses analytical and critical thinking skills, the ability to assess risks and consequences, and a comprehensive understanding of business context. It also involves knowing when to escalate issues and how to balance competing priorities.
As professionals advance, their decision-making evolves from addressing routine issues to shaping strategic directions. Early on, decisions focus on managing tasks or small projects. Over time, decision-making becomes more complex, requiring greater judgement, risk assessment, and accountability for high-impact outcomes. At higher levels, professionals are responsible for making critical decisions that influence organisational strategy and success."""@en ;
    sfia:attributeType "Business skills/Behavioural factors"@en ;
dcterms:source "https://sfia-online.org/en/shortcode/9/DECM"^^xsd:anyURI .

attributes:DIGI a owl:AnnotationProperty ;
    rdfs:label "Digital mindset"@en ;
    rdfs:comment "Embracing and effectively using digital tools and technologies to enhance performance and productivity."@en ;
    skos:notation "DIGI" ;
    sfia:attributeGuidanceNotes """Having a digital mindset in SFIA represents a progression from basic digital literacy to driving organisational digital strategy. It involves:

understanding and applying digital technologies
adapting to rapidly evolving digital landscapes
using digital tools, AI and data to enhance work processes
driving digital innovation and transformation
understanding the implications of emerging technologies, including AI, and their potential to drive organisational change
ensuring digital governance and compliance.

An effective digital mindset encompasses continuous learning, adaptability and the ability to see how digital technologies can transform business models and strategies. It also involves understanding the implications of emerging technologies and their potential to drive organisational change.
As professionals advance, their digital mindset evolves from simply using digital tools to shaping and leading organisational digital strategies. Early in their careers, they focus on applying digital skills to their roles, but as they progress, they begin driving innovation and using emerging technologies to transform work processes. At higher levels, professionals are responsible for leading digital transformation, ensuring compliance with digital governance, and embedding a digital culture across the organisation."""@en ;
    sfia:attributeType "Business skills/Behavioural factors"@en ;
dcterms:source "https://sfia-online.org/en/shortcode/9/DIGI"^^xsd:anyURI .

attributes:IMPM a owl:AnnotationProperty ;
    rdfs:label "Improvement mindset"@en ;
    rdfs:comment "Continuously identifying opportunities to refine work practices, processes, products, or services for greater efficiency and impact."@en ;
    skos:notation "IMPM" ;
    sfia:attributeGuidanceNotes """Having an improvement mindset in SFIA represents a progression from recognising opportunities for enhancement to driving a culture of ongoing optimisation. It involves:

identifying areas for improvement in processes, products, or services
implementing changes to enhance efficiency and effectiveness
assessing the impact of improvements and refining approaches
encouraging and supporting a mindset of continuous improvement in others
aligning improvement initiatives with organisational objectives
cultivating a culture of ongoing enhancement and optimisation

An improvement mindset involves proactively seeking opportunities to refine and optimise work practices, processes, products, and services. This reflects the growing responsibility to identify, implement, and lead improvements across increasing scopes of influence.As professionals advance, their focus shifts from identifying opportunities for improvement in their own tasks to leading improvement initiatives across teams and the organisation. This progression includes enhancing practices at a personal level, supporting others in promoting a culture of continuous optimisation, and ensuring improvement efforts align with broader organisational goals. At higher levels, professionals take responsibility for embedding ongoing improvement strategies throughout the organisation, driving long-term impact."""@en ;
    sfia:attributeType "Business skills/Behavioural factors"@en ;
dcterms:source "https://sfia-online.org/en/shortcode/9/IMPM"^^xsd:anyURI .

attributes:INFL a owl:AnnotationProperty ;
    rdfs:label "Influence"@en ;
    rdfs:comment "The reach and impact of your decisions and actions, both within and outside the organisation."@en ;
    skos:notation "INFL" ;
    sfia:attributeGuidanceNotes """Influence in SFIA reflects a progression from impacting immediate colleagues to shaping organisational direction. It involves:

expanding the sphere of interaction and impact
progressing from transactional to strategic interactions
engaging with stakeholders, both internal and external, at increasing levels of seniority
shaping decisions with growing organisational impact
contributing to team, departmental and organisational direction.

Influence is closely linked with other attributes such as, communication and leadership. Effective influence develops through experience and interaction with more senior levels of the organisation and industry. This attribute reflects the reach and impact of decisions and actions, both within and outside the organisation. 
As professionals advance, their influence extends beyond their team, contributing to strategic decisions and helping shape the organisation's direction. It progresses from awareness of how one's work supports others to directing strategy at an organisational level. The extent of influence is often reflected in the nature of interactions, the level of contacts and the impact of decisions on organisational direction."""@en ;
    sfia:attributeType "Attributes"@en ;
dcterms:source "https://sfia-online.org/en/shortcode/9/INFL"^^xsd:anyURI .

attributes:KNGE a owl:AnnotationProperty ;
    rdfs:label "Knowledge"@en ;
    rdfs:comment "The depth and breadth of understanding required to perform and influence work effectively."@en ;
    skos:notation "KNGE" ;
    sfia:attributeGuidanceNotes """Knowledge in SFIA represents a progression from applying basic role-specific information to leveraging broad, strategic understanding that shapes organisational direction and industry trends. It involves:

applying role-specific knowledge to perform routine tasks
integrating general, role-specific, and industry knowledge
using understanding of technologies, methods, and processes to achieve results
applying in-depth expertise to solve complex problems
leveraging broad knowledge to influence strategic decisions
shaping organisational knowledge management practices.

Effective knowledge application develops through practical experience, formal education, professional training, continuous learning, and mentorship. It encompasses the ability to apply understanding in real-world scenarios, adapt to emerging challenges, and create value for the organisation.
As professionals advance, their application of knowledge evolves significantly from basic, role-specific tasks to strategic organisational leadership. This progression involves supporting team activities, applying practices within business contexts, integrating knowledge for complex tasks, offering authoritative advice, and enabling cross-domain decision-making. At higher levels, professionals apply broad business and strategic knowledge to shape organisational strategy and anticipate industry trends."""@en ;
    sfia:attributeType "Attributes"@en ;
dcterms:source "https://sfia-online.org/en/shortcode/9/KNGE"^^xsd:anyURI .

attributes:LADV a owl:AnnotationProperty ;
    rdfs:label "Learning and development"@en ;
    rdfs:comment "Continuously acquiring new knowledge and skills to enhance personal and organisational performance."@en ;
    skos:notation "LADV" ;
    sfia:attributeGuidanceNotes """Learning and professional development in SFIA represents a progression from personal skill enhancement to shaping organisational learning culture. It involves:

acquiring and applying new knowledge
identifying and addressing skill gaps
sharing learnings with colleagues
driving personal and team development
promoting knowledge application for strategic goals
inspiring a learning culture aligned with business objectives.

Effective learning and professional development encompass formal education, experiential learning, self-directed study and the ability to critically assess and apply new information. It also involves maintaining awareness of emerging practices and industry trends, and aligning learning initiatives with strategic business objectives.As professionals advance, their approach to learning and development evolves from focusing on personal skill enhancement to driving team and organisational development. Over time, they move from applying new knowledge to leading efforts that shape a culture of learning, aligning development initiatives with strategic goals. At senior levels, professionals not only inspire a learning culture but also ensure that the organisation has the necessary skills and capabilities to navigate industry changes and take advantage of opportunities."""@en ;
    sfia:attributeType "Business skills/Behavioural factors"@en ;
dcterms:source "https://sfia-online.org/en/shortcode/9/LADV"^^xsd:anyURI .

attributes:LEAD a owl:AnnotationProperty ;
    rdfs:label "Leadership"@en ;
    rdfs:comment "Guiding and influencing individuals or teams to align actions with strategic goals and drive positive outcomes."@en ;
    skos:notation "LEAD" ;
    sfia:attributeGuidanceNotes """Leadership in SFIA represents a progression from self-management to shaping organisational strategy. It involves:

demonstrating personal responsibility
taking ownership of work and development
guiding and influencing others
contributing to team capabilities
aligning actions with organisational objectives
inspiring and driving positive change.

Effective leadership encompasses self-awareness, influence, understanding and inspiring and motivating others. It also involves strategic thinking, risk management and the capacity to align actions with long-term objectives.
As professionals advance, their leadership evolves from managing personal responsibilities to guiding teams and eventually shaping organisational strategy. Over time, they move beyond influencing teams to driving strategic outcomes, aligning policies with organisational goals, and managing risks on a broader scale. At higher levels, leadership plays a critical role in shaping organisational culture, driving innovation, and enhancing the organisation's ability to navigate complex challenges and seize opportunities."""@en ;
    sfia:attributeType "Business skills/Behavioural factors"@en ;
dcterms:source "https://sfia-online.org/en/shortcode/9/LEAD"^^xsd:anyURI .

attributes:PLAN a owl:AnnotationProperty ;
    rdfs:label "Planning"@en ;
    rdfs:comment "Taking a systematic approach to organising tasks, resources and timelines to meet defined goals."@en ;
    skos:notation "PLAN" ;
    sfia:attributeGuidanceNotes """Planning in SFIA represents a progression from organising individual work to leading strategic planning across an organisation. It involves: 

setting objectives and determining timelines
organising tasks and allocating resources
aligning activities with larger goals
adapting plans to changing circumstances
monitoring progress and evaluating outcomes
initiating and influencing strategic objectives.

Effective planning encompasses analytical skills, foresight and the ability to balance multiple priorities. It also involves adaptability to respond to changing circumstances, and the capacity to align operational plans with strategic goals. As professionals advance, their planning skills increasingly shape organisational direction and performance.
As professionals advance, their planning responsibilities grow from managing personal or team tasks to driving organisational planning efforts. Over time, they progress from organising their own work to setting strategic objectives that shape the direction of the organisation. At higher levels, professionals take the lead in planning complex initiatives, ensuring alignment with strategic goals, and guiding organisational performance."""@en ;
    sfia:attributeType "Business skills/Behavioural factors"@en ;
dcterms:source "https://sfia-online.org/en/shortcode/9/PLAN"^^xsd:anyURI .

attributes:PROB a owl:AnnotationProperty ;
    rdfs:label "Problem-solving"@en ;
    rdfs:comment "Analysing challenges, applying logical methods and developing effective solutions to overcome obstacles."@en ;
    skos:notation "PROB" ;
    sfia:attributeGuidanceNotes """Problem solving in SFIA represents a progression from addressing routine issues to managing strategic challenges. It involves:

recognising and understanding problems
analysing potential solutions
implementing effective resolutions
evaluating outcomes and learning from experiences
anticipating and addressing potential issues proactively
aligning problem solving with organisational objectives.

Effective problem solving encompasses analytical thinking, creativity and the ability to make informed decisions. It also involves collaboration with experts from various disciplines, particularly at senior levels.
As professionals advance, their problem-solving responsibilities grow from resolving routine issues to tackling complex, strategic challenges. Initially, they focus on methodical approaches to everyday problems, but over time, they develop the capacity to anticipate issues, evaluate a range of solutions, and address challenges that impact broader organisational objectives. At higher levels, professionals lead problem-solving efforts, ensuring that complex challenges are managed in alignment with long-term goals."""@en ;
    sfia:attributeType "Business skills/Behavioural factors"@en ;
dcterms:source "https://sfia-online.org/en/shortcode/9/PROB"^^xsd:anyURI .

attributes:SCPE a owl:AnnotationProperty ;
    rdfs:label "Security, privacy and ethics"@en ;
    rdfs:comment "Ensuring the protection of sensitive information, upholding privacy of data and individuals, and demonstrating ethical conduct within and outside the organisation."@en ;
    skos:notation "SCPE" ;
    sfia:attributeGuidanceNotes """Security, privacy and ethics in SFIA represent a progression from basic awareness to strategic leadership. It involves:

applying professional working practices and adhering to organisational rules
implementing standards and best practices
promoting a culture of security, privacy and ethical conduct
addressing ethical challenges, including those introduced by emerging technologies, such as AI
ensuring compliance with relevant laws and regulations
leading initiatives that embed security, privacy, and ethics into organisational culture and operations.

Effective management of security, privacy and ethics encompasses technical knowledge, ethical decision-making skills and the ability to balance competing priorities. It also involves creating an environment where these principles are embedded in all aspects of work.
As professionals advance, they are expected to take an active role in promoting ethical behaviour and securing sensitive information across all areas of work. At higher levels, individuals are responsible for developing strategies that balance operational needs with ethical considerations, ensuring long-term sustainability and trust."""@en ;
    sfia:attributeType "Business skills/Behavioural factors"@en ;
dcterms:source "https://sfia-online.org/en/shortcode/9/SCPE"^^xsd:anyURI .

sfia:attributeGuidanceNotes a owl:AnnotationProperty ;
    rdfs:label "has guidance notes"@en ;
    rdfs:domain owl:AnnotationProperty .

sfia:attributeType a owl:AnnotationProperty ;
    rdfs:label "has attribute type"@en ;
    rdfs:domain owl:AnnotationProperty .

sfia:definedAtLevel a owl:ObjectProperty ;
    rdfs:label "defined at level"@en ;
    rdfs:domain sfia:Skill ;
    rdfs:range sfia:SkillLevel .

sfia:level a owl:ObjectProperty ;
    rdfs:label "has level"@en ;
    rdfs:domain sfia:SkillLevel ;
    rdfs:range sfia:Level .

sfia:levelEssence a owl:AnnotationProperty ;
    rdfs:label "essence of the level"@en ;
    rdfs:domain owl:Level .

sfia:levelGuidingPhrase a owl:AnnotationProperty ;
    rdfs:label "has guiding phrase"@en ;
    rdfs:domain owl:Level .

sfia:skillCategory a owl:ObjectProperty ;
    rdfs:label "has category"@en ;
    rdfs:domain sfia:Skill ;
    rdfs:range sfia:Category .

 sfia:skillDescription a owl:AnnotationProperty ;
    rdfs:label "has overall description"@en ;
    rdfs:domain sfia:Skill .

sfia:skillLevelDescription a owl:AnnotationProperty ;
    rdfs:label "has skill-level description"@en ;
    rdfs:domain sfia:SkillLevel .

skos:scopeNote a owl:AnnotationProperty ;
    rdfs:label "notes"@en ;
    rdfs:domain sfia:Skill .

skills:ACIN a sfia:Skill , skos:Concept ;
skos:inScheme skillcs: ;
    skos:prefLabel "Accessibility and inclusion"@en ;
    skos:notation "ACIN" ;
    sfia:definedAtLevel sfialevels:ACIN_2,
        sfialevels:ACIN_3,
        sfialevels:ACIN_4,
        sfialevels:ACIN_5,
        sfialevels:ACIN_6 ;
    sfia:skillCategory categories:user_centred_design ;
     skos:definition "Driving accessibility and inclusion in services and products."@en ;
    skos:scopeNote """Activities may include, but are not limited to:

providing expert advice and guidance on accessibility and inclusion 
defining policies, standards and guidelines for accessible design, development, user research, auditing and testing
conducting accessibility impact assessments and audits to identify potential barriers and areas for improvement
keeping up-to-date with the latest industry trends, regulatory developments and established practices related to accessibility
collaborating with subject matter experts in areas such as usability, user experience, content design, assistive technology and disability rights
advising teams on budgeting appropriately for accessibility activities throughout the service or product development lifecycle
promoting a culture of shared responsibility for accessibility by embedding it into the roles and responsibilities of others, such, as designers, developers, researchers and managers."""@en ;
dcterms:source "https://sfia-online.org/en/skillcode/9/ACIN"^^xsd:anyURI .

skills:ADEV a sfia:Skill , skos:Concept ; 
 skos:inScheme skillcs: ;
    skos:prefLabel "Animation development"@en ;
    skos:notation "ADEV" ;
    sfia:definedAtLevel sfialevels:ADEV_2,
        sfialevels:ADEV_3,
        sfialevels:ADEV_4,
        sfialevels:ADEV_5,
        sfialevels:ADEV_6 ;
    sfia:skillCategory categories:systems_development ;
     skos:definition "Designing and developing animated and interactive systems such as games, simulations and virtual environments."@en ;
    skos:scopeNote """Animation development enables the creation of visually engaging and interactive experiences for various industries, such as gaming, training, scientific research and engineering, as well as virtual reality and augmented reality applications.
Components of animation systems include game engine or framework, visual assets (3D models, 2D artwork, animations), audio assets, user interface and user experience components, game logic, data and configuration files, tools and pipelines, documentation and design documents
Activities may include, but are not limited to:

employing animation techniques, including keyframe animation, motion capture, procedural animation and skeletal animation
using specialised software for rigging, skinning and animation editing
creating and integrating animations into interactive systems
ensuring integration of animations with game logic, physics and artificial intelligence systems
optimising animations for performance and adhering to consistency and quality standards."""@en ;
dcterms:source "https://sfia-online.org/en/skillcode/9/ADEV"^^xsd:anyURI .

skills:ADMN a sfia:Skill , skos:Concept ; 
 skos:inScheme skillcs: ;
    skos:prefLabel "Business administration"@en ;
    skos:notation "ADMN" ;
    sfia:definedAtLevel sfialevels:ADMN_1,
        sfialevels:ADMN_2,
        sfialevels:ADMN_3,
        sfialevels:ADMN_4,
        sfialevels:ADMN_5,
        sfialevels:ADMN_6 ;
    sfia:skillCategory categories:stakeholder_management ;
     skos:definition "Managing and performing administrative services and tasks to enable individuals, teams and organisations to succeed in their objectives."@en ;
    skos:scopeNote """The application of this skill varies widely depending on role and organisation context.
Business administration tasks may include: communication management, information organisation, scheduling and coordination with internal and external stakeholders using various digital tools and platforms.
Management-level business administration tasks focus on planning, managing and coordinating the activities of individuals and teams to enable them to achieve their objectives efficiently and effectively.
Activities may include, but are not limited to:

managing calendars and scheduling meetings
organising and maintaining filing systems (physical and digital)
preparing reports, presentations and correspondence
coordinating travel arrangements and expense management
managing office supplies and equipment
facilitating internal and external communications
supporting project management activities
assisting with budget preparation and monitoring
implementing and maintaining administrative processes and procedures."""@en ;
dcterms:source "https://sfia-online.org/en/skillcode/9/ADMN"^^xsd:anyURI .

skills:AIDE a sfia:Skill , skos:Concept ; 
 skos:inScheme skillcs: ; 
    skos:prefLabel "Artificial intelligence (AI) and data ethics"@en ;
    skos:notation "AIDE" ;
    sfia:definedAtLevel sfialevels:AIDE_3,
        sfialevels:AIDE_4,
        sfialevels:AIDE_5,
        sfialevels:AIDE_6 ;
    sfia:skillCategory categories:governance__risk_and_compliance ;
     skos:definition "Implementing and promoting ethical practices in the design, development, deployment and use of AI and data technologies."@en ;
    skos:scopeNote """Includes principles such as fairness, accountability, transparency and privacy. Ethical considerations encompass issues like bias in algorithms, data privacy, the impact of automation on employment and the societal implications of emerging technologies.
Activities may include, but are not limited to:

providing expert advice on ethical policies, procedures and governance
designing AI and data systems that embed ethical considerations
conducting ethical impact assessments to identify risks and ensure responsible use of technology
responding to ethical dilemmas and incidents
keeping up to date with ethical standards, regulations and recommended practices
creating ethical risk models and frameworks
collaborating with experts in fields such as legal, public relations, data science and AI
promoting a culture of ethical awareness and responsibility within the organisation."""@en ;
dcterms:source "https://sfia-online.org/en/skillcode/9/AIDE"^^xsd:anyURI .

skills:ANCC a sfia:Skill , skos:Concept ; 
 skos:inScheme skillcs: ;
    skos:prefLabel "Analytical classification and coding"@en ;
    skos:notation "ANCC" ;
    sfia:definedAtLevel sfialevels:ANCC_2,
        sfialevels:ANCC_3,
        sfialevels:ANCC_4,
        sfialevels:ANCC_5,
        sfialevels:ANCC_6 ;
    sfia:skillCategory categories:data_and_records_operations ;
     skos:definition "Interpreting information and assigning classifications or labels based on domain-specific knowledge, standards and guidelines to enable data analysis and use."@en ;
    skos:scopeNote """This skill is applied in contexts where consistent categorisation of information is required to enable the data to be used reliably and effectively. This may include, but is not limited to, clinical coding, data labelling for machine learning, legal coding/indexing and market research coding.
Activities may include, but are not limited to:

analysing and interpreting information based on domain-specific knowledge
assigning codes, labels or categories based on specific standards, guidelines or frameworks
ensuring accuracy and consistency of coding/labelling through quality assurance activities
collaborating with subject matter experts to clarify ambiguous cases and improve coding/labelling guidelines
providing guidance and training to others on coding/labelling practices
contributing to the development and improvement of coding/labelling systems, guidelines and processes."""@en ;
dcterms:source "https://sfia-online.org/en/skillcode/9/ANCC"^^xsd:anyURI .

skills:ARCH a sfia:Skill , skos:Concept ; 
 skos:inScheme skillcs: ;
    skos:prefLabel "Solution architecture"@en ;
    skos:notation "ARCH" ;
    sfia:definedAtLevel sfialevels:ARCH_4,
        sfialevels:ARCH_5,
        sfialevels:ARCH_6 ;
    sfia:skillCategory categories:strategy_and_planning ;
     skos:definition "Developing and communicating a multi-dimensional solution architecture to deliver agreed business outcomes."@en ;
    skos:scopeNote """Activities may include, but are not limited to:

defining the planned operation and maintenance of the solution within a production environment, including changes to services, processes, organisation and operating models as well as technology 
ensuring existing and planned solution components are compatible with relevant architectures, strategies, policies, standards and practices 
considering requirements for security, privacy and testing of solutions
taking account of relevant architectures, strategies, policies, standards and practices 
identifying appropriate cloud services, evaluating their cost implications and optimising for cost-efficiency
developing roadmaps to migrate components to cloud services
developing and communicating an implementation roadmap 
providing guidance and risk-based governance to support solution implementation including managing requests for changes and deviations from specifications."""@en ;
dcterms:source "https://sfia-online.org/en/skillcode/9/ARCH"^^xsd:anyURI .

skills:ASMG a sfia:Skill , skos:Concept ; 
 skos:inScheme skillcs: ;
    skos:prefLabel "Asset management"@en ;
    skos:notation "ASMG" ;
    sfia:definedAtLevel sfialevels:ASMG_2,
        sfialevels:ASMG_3,
        sfialevels:ASMG_4,
        sfialevels:ASMG_5,
        sfialevels:ASMG_6 ;
    sfia:skillCategory categories:service_management ;
     skos:definition "Managing the full lifecycle of assets from acquisition, operation, maintenance to disposal."@en ;
    skos:scopeNote """Assets include hardware, software, data, networks, cloud services, devices, IP, licences, agreements and warranties.
The full lifecycle includes: acquisition, storage, distribution, movement and disposal of assets.
Asset management involves financial, legal and technical considerations.
Activities may include, but are not limited to:

advising on value optimisation, cost control, risk management, decision support and regulatory or contractual compliance
managing hardware, software licences, intellectual property and contractual obligations
using international standards for asset management
integrating with security, change and configuration management
resolving issues and risks with unauthorised assets such as: unlicensed copies of software, cloud services, devices."""@en ;
dcterms:source "https://sfia-online.org/en/skillcode/9/ASMG"^^xsd:anyURI .

skills:ASUP a sfia:Skill , skos:Concept ; 
 skos:inScheme skillcs: ;
    skos:prefLabel "Application support"@en ;
    skos:notation "ASUP" ;
    sfia:definedAtLevel sfialevels:ASUP_2,
        sfialevels:ASUP_3,
        sfialevels:ASUP_4,
        sfialevels:ASUP_5 ;
    sfia:skillCategory categories:technology_management ;
     skos:definition "Delivering management, technical and administrative services to support and maintain live applications."@en ;
    skos:scopeNote """Activities may include, but are not limited to:

investigating and resolving issues
implementing working practices to support iterative/agile development and/or cloud-based applications
monitoring performance and maintaining the security of applications
providing guidance or training to users, including enhanced levels of support following new/updated software releases
devising permanent or temporary corrections, workarounds for faults, and applying patches when necessary
adhering to established safety, security and quality standards
capturing user feedback for subsequent analysis to inform future application development
implementing general or site-specific modifications
updating documentation
maintaining application data
defining enhancements.

Support typically involves close collaboration with application developers and other specialist areas. Application maintenance and support services may be delivered directly to users of the systems or to service delivery functions."""@en ;
dcterms:source "https://sfia-online.org/en/skillcode/9/ASUP"^^xsd:anyURI .

skills:AUDT a sfia:Skill , skos:Concept ; 
 skos:inScheme skillcs: ;
    skos:prefLabel "Audit"@en ;
    skos:notation "AUDT" ;
    sfia:definedAtLevel sfialevels:AUDT_2,
        sfialevels:AUDT_3,
        sfialevels:AUDT_4,
        sfialevels:AUDT_5,
        sfialevels:AUDT_6,
        sfialevels:AUDT_7 ;
    sfia:skillCategory categories:governance__risk_and_compliance ;
     skos:definition "Delivering independent, risk-based assessments of the effectiveness of processes, the controls and the compliance environment of an organisation."@en ;
    skos:scopeNote """Audit activity is conducted with appropriate independence from the organisation's management and may be conducted internally or for a third-party client organisation.
Activities may include, but are not limited to:

planning and conducting risk-based assessments
evaluating the effectiveness of controls and compliance measures
documenting and reporting audit findings and recommendations
providing assurance on the integrity of processes and systems
collaborating with management to develop corrective action plans
conducting follow-up reviews to ensure implementation of recommendations
staying current with relevant regulations and industry standards."""@en ;
dcterms:source "https://sfia-online.org/en/skillcode/9/AUDT"^^xsd:anyURI .

skills:AVMT a sfia:Skill , skos:Concept ; 
 skos:inScheme skillcs: ;
    skos:prefLabel "Availability management"@en ;
    skos:notation "AVMT" ;
    sfia:definedAtLevel sfialevels:AVMT_3,
        sfialevels:AVMT_4,
        sfialevels:AVMT_5,
        sfialevels:AVMT_6 ;
    sfia:skillCategory categories:service_management ;
     skos:definition "Ensuring services deliver agreed levels of availability to meet the current and future needs of the business."@en ;
    skos:scopeNote """Activities may include, but are not limited to:

defining and agreeing availability targets
disaster recovery planning and testing
ensuring services can collect data required to measure availability
monitoring, analysing and reporting on service availability
implementing availability management practices, including those for cloud-based services
maintaining and improving the availability of services
controlling and managing service availability to deliver agreed levels of availability in a cost-effective manner."""@en ;
dcterms:source "https://sfia-online.org/en/skillcode/9/AVMT"^^xsd:anyURI .

skills:BENM a sfia:Skill , skos:Concept ; 
 skos:inScheme skillcs: ;
    skos:prefLabel "Benefits management"@en ;
    skos:notation "BENM" ;
    sfia:definedAtLevel sfialevels:BENM_3,
        sfialevels:BENM_4,
        sfialevels:BENM_5,
        sfialevels:BENM_6 ;
    sfia:skillCategory categories:financial_and_value_management ;
     skos:definition "Forecasting, planning and monitoring the emergence and effective realisation of anticipated benefits from projects and programmes."@en ;
    skos:scopeNote """Activities may include, but are not limited to:

implementing a benefits management framework and approach
identifying and implementing the actions needed to optimise the business impact of individual and combined benefits
confirming the achievement of expected benefits
adapting benefits management practices for agile projects
using data-driven analysis for benefits identification, tracking and reporting
engaging stakeholders to embed a value-driven culture."""@en ;
dcterms:source "https://sfia-online.org/en/skillcode/9/BENM"^^xsd:anyURI .

skills:BIDM a sfia:Skill , skos:Concept ; 
 skos:inScheme skillcs: ;
    skos:prefLabel "Bid/proposal management"@en ;
    skos:notation "BIDM" ;
    sfia:definedAtLevel sfialevels:BIDM_3,
        sfialevels:BIDM_4,
        sfialevels:BIDM_5,
        sfialevels:BIDM_6 ;
    sfia:skillCategory categories:sales_and_bid_management ;
     skos:definition "Managing preparation and submission of bids and proposals for contracts, grants, projects, or services."@en ;
    skos:scopeNote """Activities may include, but are not limited to:

assessing requirements, conditions and customer needs relevant to the proposal or bid
developing and implementing bid and proposal strategies, including competitive positioning
leading multidisciplinary teams in crafting detailed, high-quality and persuasive proposal documents
managing bid and proposal teams, resources, risks and issues throughout the proposal lifecycle
overseeing compliance with legal, accessibility, customer and organisational requirements
coordinating stakeholder engagement, communication and proposal reviews/approvals
advocating for effective practices and innovative approaches in proposal development
negotiating and closing deals with customers and stakeholders.

This skill is applicable in diverse contexts, such as commercial organisations bidding for contracts and public sector entities seeking funding. In commercial settings, it emphasises competitive positioning and market strategies. In the public sector, it focuses on aligning with policy objectives and demonstrating public value. The core activities are consistent across different environments."""@en ;
dcterms:source "https://sfia-online.org/en/skillcode/9/BIDM"^^xsd:anyURI .

skills:BINT a sfia:Skill , skos:Concept ; 
 skos:inScheme skillcs: ;
    skos:prefLabel "Business intelligence"@en ;
    skos:notation "BINT" ;
    sfia:definedAtLevel sfialevels:BINT_2,
        sfialevels:BINT_3,
        sfialevels:BINT_4,
        sfialevels:BINT_5 ;
    sfia:skillCategory categories:data_and_analytics ;
     skos:definition "Developing, producing and delivering regular and one-off management information to provide insights and aid decision-making."@en ;
    skos:scopeNote """Typically applied in supporting operational needs through management and governance processes. May be one-off or regular activities aligned with the organisation's planning and reporting cycles.
Activities may include, but are not limited to:

understanding business needs and objectives
identifying and validating internal and external data sets generated from a diverse range of business and operational processes
transforming the results of analysis into information that can be communicated to stakeholders using dashboards and reports
interpreting and analysing data, comparative analysis, benchmarking, trend analysis
bringing data together to communicate clear themes and trends
focusing on data quality to provide confidence for making decisions on a single version of the truth."""@en ;
dcterms:source "https://sfia-online.org/en/skillcode/9/BINT"^^xsd:anyURI .

skills:BPRE a sfia:Skill , skos:Concept ; 
 skos:inScheme skillcs: ;
    skos:prefLabel "Business process improvement"@en ;
    skos:notation "BPRE" ;
    sfia:definedAtLevel sfialevels:BPRE_2,
        sfialevels:BPRE_3,
        sfialevels:BPRE_4,
        sfialevels:BPRE_5,
        sfialevels:BPRE_6,
        sfialevels:BPRE_7 ;
    sfia:skillCategory categories:change_planning ;
     skos:definition "Creating new and potentially disruptive approaches to performing business activities."@en ;
    skos:scopeNote """Activities may include, but are not limited to:

analysing and designing business processes to improve business performance, create business opportunities, deliver new or improved products/services, or improve product/service value chains. Including the adoption and exploitation of data, information, new or existing technologies and cloud-based services
using process mapping, value stream mapping, process mining and analytics, root cause analysis and visual modelling 
identifying and implementing improvements to business models, business operations and services with improved processes
exploiting technologies, such as robotic process automation, artificial intelligence and machine learning
assessing the costs and potential benefits of new approaches to the organisation and all stakeholders
developing enterprise business process management capabilities to increase organisational agility and responsiveness to change."""@en ;
dcterms:source "https://sfia-online.org/en/skillcode/9/BPRE"^^xsd:anyURI .

skills:BPTS a sfia:Skill , skos:Concept ; 
 skos:inScheme skillcs: ;
    skos:prefLabel "User acceptance testing"@en ;
    skos:notation "BPTS" ;
    sfia:definedAtLevel sfialevels:BPTS_2,
        sfialevels:BPTS_3,
        sfialevels:BPTS_4,
        sfialevels:BPTS_5,
        sfialevels:BPTS_6 ;
    sfia:skillCategory categories:change_analysis ;
     skos:definition "Validating systems, products, business processes or services to determine whether the acceptance criteria have been satisfied."@en ;
    skos:scopeNote """Activities include, but are not limited to:

setting and applying standards for user acceptance testing (UAT)
planning, identifying, designing, managing, executing and reporting on the outcomes of acceptance tests
collaborating with a range of relevant stakeholders
defining clear entry and exit criteria for UAT
requesting and enabling formal acceptance of systems, products or services
creating measurable acceptance criteria related to functional and non-functional requirements, features, business processes, user stories and business rules
devising test cases and scenarios from acceptance criteria
enabling exploratory testing to discover unexpected behaviours
deploying model office testing to simulate real-world usage
ensuring appropriate training for users involved in UAT
providing input on UAT resource requirements, including necessary skills and availability.

The acceptance testing approach will be based on the context of the work and may be selected from predictive (plan-driven) or adaptive (iterative/agile) approaches."""@en ;
dcterms:source "https://sfia-online.org/en/skillcode/9/BPTS"^^xsd:anyURI .

skills:BRMG a sfia:Skill , skos:Concept ; 
 skos:inScheme skillcs: ;
    skos:prefLabel "Brand management"@en ;
    skos:notation "BRMG" ;
    sfia:definedAtLevel sfialevels:BRMG_4,
        sfialevels:BRMG_5,
        sfialevels:BRMG_6 ;
    sfia:skillCategory categories:marketing ;
     skos:definition "Managing brand strategy to establish and enhance brand identity and value aligned with organisational goals."@en ;
    skos:scopeNote """Activities may include, but are not limited to:

conducting brand research and analysis to inform brand strategy development
defining brand positioning, values, personality and value proposition
creating and managing brand identity elements, such as logos, colour palettes and typography
developing brand guidelines and ensuring consistent application across all touchpoints
managing brand portfolios, architecture and extensions
monitoring and analysing brand performance metrics and consumer perceptions
collaborating with internal stakeholders to align brand strategy with overall business objectives
partnering with external agencies and vendors to execute brand initiatives and campaigns
using creative strategies to differentiate the brand and drive commercial success
protecting and enhancing brand value to contribute to overall commercial outcomes
continuously refining and adapting brand strategy based on market trends and insights."""@en ;
dcterms:source "https://sfia-online.org/en/skillcode/9/BRMG"^^xsd:anyURI .

skills:BSMO a sfia:Skill , skos:Concept ; 
 skos:inScheme skillcs: ;
    skos:prefLabel "Business modelling"@en ;
    skos:notation "BSMO" ;
    sfia:definedAtLevel sfialevels:BSMO_2,
        sfialevels:BSMO_3,
        sfialevels:BSMO_4,
        sfialevels:BSMO_5,
        sfialevels:BSMO_6 ;
    sfia:skillCategory categories:change_analysis ;
     skos:definition "Creating abstract or distilled models of business scenarios, representing processes, data and roles to support decision-making and analysis."@en ;
    skos:scopeNote """Predominantly focused on the representation of processes, roles, data, organisation and time. Models may be used to represent a subject at varying levels of detail and decomposition.
Business models are typically created to communicate and provide insights into existing, conceptual or proposed scenarios. As such, they are likely to be working models that allow comparisons of alternative outcomes based on changing inputs and parameters.
Activities may include, but are not limited to:

gathering and analysing business requirements
creating visual representations of business workflows, processes and structures
developing and testing simulation models
facilitating workshops to validate and refine models
presenting models to stakeholders and explaining their implications.

This skill shouldn't be applied to the creation of all diagrams related to describing and explaining business concepts. Refer to other SFIA skills, including, but not limited to: Business situation analysis, Business process improvement, Data design and modelling, Enterprise and business architecture, Organisation design."""@en ;
dcterms:source "https://sfia-online.org/en/skillcode/9/BSMO"^^xsd:anyURI .

skills:BUDF a sfia:Skill , skos:Concept ; 
 skos:inScheme skillcs: ;
    skos:prefLabel "Budgeting and forecasting"@en ;
    skos:notation "BUDF" ;
    sfia:definedAtLevel sfialevels:BUDF_2,
        sfialevels:BUDF_3,
        sfialevels:BUDF_4,
        sfialevels:BUDF_5,
        sfialevels:BUDF_6 ;
    sfia:skillCategory categories:financial_and_value_management ;
     skos:definition "Developing and managing financial budgets and forecasts to enable effective decision-making and resource allocation."@en ;
    skos:scopeNote """Activities may include, but are not limited to:

gathering and analysing financial data to prepare budgets and forecasts
selecting and applying appropriate budgeting and forecasting methodologies and tools
incorporating scenario planning, sensitivity analysis and risk assessment into the budgeting and forecasting process
presenting budget and forecast information to stakeholders and facilitating data-driven decision-making
developing and implementing budgeting and forecasting strategies, policies and processes aligned with organisational objectives
driving the adoption of good practices 
providing strategic insights and recommendations based on budget and forecast analysis
ensuring compliance with accounting standards, governance, legal and regulatory requirements
applying budgeting and forecasting to cloud computing and FinOps contexts, such as consumption-based pricing, rapid scalability, and the need for real-time cost-visibility and optimisation."""@en ;
dcterms:source "https://sfia-online.org/en/skillcode/9/BUDF"^^xsd:anyURI .

skills:BURM a sfia:Skill , skos:Concept ; 
 skos:inScheme skillcs: ;
    skos:prefLabel "Risk management"@en ;
    skos:notation "BURM" ;
    sfia:definedAtLevel sfialevels:BURM_2,
        sfialevels:BURM_3,
        sfialevels:BURM_4,
        sfialevels:BURM_5,
        sfialevels:BURM_6,
        sfialevels:BURM_7 ;
    sfia:skillCategory categories:governance__risk_and_compliance ;
     skos:definition "Planning and implementing processes for managing risk across the enterprise, aligned with organisational strategy and governance frameworks."@en ;
    skos:scopeNote """Risk management can be applied to many enterprise functions as well as technical and engineering specialisms, such as, but not limited to, information and technology systems, operations, environmental, information and cyber-security, safety, energy supply. Risk is also explicitly referenced in many SFIA skills. 
Activities may include, but are not limited to:

identifying, classifying and prioritising risks based on impact and probability and required mitigation
developing and implementing risk management strategies that align with organisational goals and governance frameworks
integrating risk management into decision-making processes to ensure alignment with the organisation's risk appetite
developing and implementing organisational goals and governance frameworks
communicating and reporting on risks and mitigation actions to key stakeholders, ensuring transparency and informed decision-making
adapting risk management practices to reflect changes in the organisational and external environment."""@en ;
dcterms:source "https://sfia-online.org/en/skillcode/9/BURM"^^xsd:anyURI .

skills:BUSA a sfia:Skill , skos:Concept ; 
 skos:inScheme skillcs: ;
    skos:prefLabel "Business situation analysis"@en ;
    skos:notation "BUSA" ;
    sfia:definedAtLevel sfialevels:BUSA_2,
        sfialevels:BUSA_3,
        sfialevels:BUSA_4,
        sfialevels:BUSA_5,
        sfialevels:BUSA_6 ;
    sfia:skillCategory categories:change_analysis ;
     skos:definition "Investigating business situations to define recommendations for improvement action."@en ;
    skos:scopeNote """Activities may include, but are not limited to:

planning for business situation analysis
establishing the investigative approach 
engaging with relevant stakeholders
reviewing the strategic context, including the organisation's vision, mission, objectives, strategy and tactics and external business environment
defining problems and analysing root causes
identifying potential changes to address problems or to take advantage of opportunities
gaining agreement to conclusions and recommendations."""@en ;
dcterms:source "https://sfia-online.org/en/skillcode/9/BUSA"^^xsd:anyURI .

skills:CELO a sfia:Skill , skos:Concept ; 
 skos:inScheme skillcs: ;
    skos:prefLabel "Customer engagement and loyalty"@en ;
    skos:notation "CELO" ;
    sfia:definedAtLevel sfialevels:CELO_3,
        sfialevels:CELO_4,
        sfialevels:CELO_5,
        sfialevels:CELO_6 ;
    sfia:skillCategory categories:marketing ;
     skos:definition "Developing and executing strategies to attract, engage and retain customers through targeted communications and loyalty initiatives."@en ;
    skos:scopeNote """Activities may include, but are not limited to:

developing customer engagement and loyalty strategies
establishing customer lifecycle communication strategies
creating and managing customer loyalty programmes and initiatives
managing customer data acquisition and profile augmentation
analysing customer data to inform personalised communications and experiences
developing customer journeys and segmentation strategies
assessing and using marketing technology tools for customer engagement
measuring and reporting on customer engagement and loyalty metrics
collaborating with cross-functional teams to improve customer retention and satisfaction."""@en ;
dcterms:source "https://sfia-online.org/en/skillcode/9/CELO"^^xsd:anyURI .

skills:CEXP a sfia:Skill , skos:Concept ; 
 skos:inScheme skillcs: ;
    skos:prefLabel "Customer experience"@en ;
    skos:notation "CEXP" ;
    sfia:definedAtLevel sfialevels:CEXP_2,
        sfialevels:CEXP_3,
        sfialevels:CEXP_4,
        sfialevels:CEXP_5,
        sfialevels:CEXP_6 ;
    sfia:skillCategory categories:user_centred_design ;
     skos:definition "Ensuring the delivery of high-quality interactions and experiences that meet customer expectations across all touchpoints and channels."@en ;
    skos:scopeNote """Activities may include, but are not limited to:

engaging with customers through various research methods to understand needs, preferences and expectations
creating and optimising customer journeys to enhance satisfaction, loyalty and overall experience
developing and implementing data-driven customer experience strategies aligned with business goals
continuously monitoring, measuring and acting upon customer feedback using appropriate metrics and systems
applying market research and segmentation insights to personalise customer experiences
leading cross-functional initiatives to ensure consistent, integrated experiences across all channels and touchpoints
evaluating and leveraging appropriate technologies to enhance and innovate customer experiences
ensuring compliance with relevant standards, regulations and policies in customer experience practices."""@en ;
dcterms:source "https://sfia-online.org/en/skillcode/9/CEXP"^^xsd:anyURI .

skills:CFMG a sfia:Skill , skos:Concept ; 
 skos:inScheme skillcs: ;
    skos:prefLabel "Configuration management"@en ;
    skos:notation "CFMG" ;
    sfia:definedAtLevel sfialevels:CFMG_2,
        sfialevels:CFMG_3,
        sfialevels:CFMG_4,
        sfialevels:CFMG_5,
        sfialevels:CFMG_6 ;
    sfia:skillCategory categories:technology_management ;
     skos:definition "Planning, identifying, controlling, accounting for and auditing of configuration items (CIs) and their interrelationships."@en ;
    skos:scopeNote """Configuration items (CIs) can include a wide variety of components (objects) such as, but not limited to, source code, software, products, systems, hardware, networks, buildings, suppliers, process definitions and documents. A coherent set of CIs forms a configuration.
Activities may include, but are not limited to:

identifying and documenting the functional and physical characteristics of CIs
identifying the relationships and maintain coherence between CIs for specific configurations
identifying the associated configuration(s), status, version and other characteristics of CIs at distinct points in time
controlling changes to CI characteristics, recording and reporting change processing and implementation status
systematically controlling changes to a configuration and maintaining the integrity, coherence and traceability of that configuration throughout the project, system and/or service lifecycle
adhering to established safety, security and quality standards
verifying and auditing CI records for data quality and compliance with specified internal and external requirements."""@en ;
dcterms:source "https://sfia-online.org/en/skillcode/9/CFMG"^^xsd:anyURI .

skills:CHMG a sfia:Skill , skos:Concept ; 
 skos:inScheme skillcs: ;
    skos:prefLabel "Change control"@en ;
    skos:notation "CHMG" ;
    sfia:definedAtLevel sfialevels:CHMG_2,
        sfialevels:CHMG_3,
        sfialevels:CHMG_4,
        sfialevels:CHMG_5,
        sfialevels:CHMG_6 ;
    sfia:skillCategory categories:service_management ;
     skos:definition "Assessing risks associated with proposed changes and ensuring changes to products, services or systems are controlled and coordinated."@en ;
    skos:scopeNote """Change control is applied to all elements impacting live products, services or systems. This includes: applications, infrastructure, documentation, processes, configuration items and suppliers.
Activities may include, but are not limited to:

managing the change request lifecycle: registering, assessing, authorising, planning and deploying
assessing risks and reducing risks to the availability, performance, security and compliance of the products and services impacted by the change
developing processes for standard, normal or emergency changes
developing methods and tools to automate change control processes to enable continuous integration."""@en ;
dcterms:source "https://sfia-online.org/en/skillcode/9/CHMG"^^xsd:anyURI .

skills:CIPM a sfia:Skill , skos:Concept ; 
 skos:inScheme skillcs: ;
    skos:prefLabel "Organisational change management"@en ;
    skos:notation "CIPM" ;
    sfia:definedAtLevel sfialevels:CIPM_2,
        sfialevels:CIPM_3,
        sfialevels:CIPM_4,
        sfialevels:CIPM_5,
        sfialevels:CIPM_6 ;
    sfia:skillCategory categories:change_planning ;
     skos:definition "Planning, designing and implementing activities to transition the organisation and people to the required future state."@en ;
    skos:scopeNote """Organisational change management focuses on the structured, procedural aspects of transitioning an organisation to a desired future state. It involves planning, designing and implementing change initiatives that are aligned with organisational goals. This skill is responsible for the technical and process-driven components of change, including stakeholder communication focused on procedural updates and assessing readiness from a structured change implementation perspective.
Activities may include, but are not limited to:

developing a business change implementation plan to identify required changes to processes, procedures, systems, structures and ways of working
using a structured process and set of tools for managing the people side of change 
assessing readiness and capacity to change, aligning with business cycles and project timelines
creating and executing communication plans that focus on procedural updates and logistics
monitoring the impact of change management efforts and sustaining the change
assessing and developing change management capabilities 
coaching change sponsors and aligning their roles with structured change processes."""@en ;
dcterms:source "https://sfia-online.org/en/skillcode/9/CIPM"^^xsd:anyURI .

skills:CNSL a sfia:Skill , skos:Concept ; 
 skos:inScheme skillcs: ;
    skos:prefLabel "Consultancy"@en ;
    skos:notation "CNSL" ;
    sfia:definedAtLevel sfialevels:CNSL_4,
        sfialevels:CNSL_5,
        sfialevels:CNSL_6,
        sfialevels:CNSL_7 ;
    sfia:skillCategory categories:advice_and_guidance ;
     skos:definition "Providing advice and recommendations, based on expertise and experience, to address client needs."@en ;
    skos:scopeNote """Consultancy may focus on a specific subject area, or encompass a wide range of strategic business issues. It may also include support for the implementation of agreed solutions.
Activities include, but are not limited to:

leading and managing a consultancy practice
leading and managing consultancy teams and/or consultancy assignments
delivering consultancy assignments
engaging with clients and maintaining client relationships
establishing and managing consultancy agreements or contracts
overseeing the growth and development of a consultancy practice
managing proposals, sales and account management within a consultancy practice.

The Consultancy skill defined in SFIA applies to the delivery of consultancy as part of formal or informal consultancy agreements. 
General advice, guidance, or problem-solving related to an individual's responsibilities is covered by the SFIA generic attributes and by specific SFIA professional skill descriptions that include providing advice and guidance."""@en ;
dcterms:source "https://sfia-online.org/en/skillcode/9/CNSL"^^xsd:anyURI .

skills:COMG a sfia:Skill , skos:Concept ; 
 skos:inScheme skillcs: ;
    skos:prefLabel "Cost management"@en ;
    skos:notation "COMG" ;
    sfia:definedAtLevel sfialevels:COMG_2,
        sfialevels:COMG_3,
        sfialevels:COMG_4,
        sfialevels:COMG_5,
        sfialevels:COMG_6 ;
    sfia:skillCategory categories:financial_and_value_management ;
     skos:definition "Planning, controlling and analysing costs to enable the effective use of financial resources."@en ;
    skos:scopeNote """Activities may include, but are not limited to:

developing and implementing cost management strategies, policies and procedures
analysing costs, identifying trends, and recommending corrective actions
conducting cost-benefit analyses and supporting stakeholder collaboration in the cost management process
overseeing the development of complex cost models and reporting frameworks
presenting cost management insights to stakeholders and facilitating data-driven decision-making
promoting a culture of cost awareness and ongoing improvement throughout the organisation
implementing cost management processes and tools to support cloud computing and FinOps in areas such as consumption-based pricing, rapid scalability, and real-time cost visibility and optimisation."""@en ;
dcterms:source "https://sfia-online.org/en/skillcode/9/COMG"^^xsd:anyURI .

skills:COPL a sfia:Skill , skos:Concept ; 
 skos:inScheme skillcs: ;
    skos:prefLabel "Continuity management"@en ;
    skos:notation "COPL" ;
    sfia:definedAtLevel sfialevels:COPL_2,
        sfialevels:COPL_3,
        sfialevels:COPL_4,
        sfialevels:COPL_5,
        sfialevels:COPL_6 ;
    sfia:skillCategory categories:service_management ;
     skos:definition "Developing, implementing and testing a business continuity framework."@en ;
    skos:scopeNote """Activities may include, but are not limited to:

identifying potential threats and assessing their business impact
developing plans and procedures to respond to an incident
ensuring critical business functions can continue with a planned level of disruption
ensuring an acceptable level of service can be restored after a disruption
developing organisational resilience
assuring that continuity is being designed into systems, processes and ways of working
implementing continuity management practices for cloud-based services
enabling continuous delivery, deployment and integration of applications and infrastructure without adverse impact or disruption to service
collaborating with external partners and suppliers to ensure continuity across the supply chain
using technologies and tools for enhanced risk assessment, monitoring and decision-making
regularly communicating and training staff on their roles and responsibilities during disruptive events.

Incidents have a variety of causes, including, but not limited to: cyber-attacks, data breaches, organised crime, fires, floods, natural disasters, pandemics, health emergencies and supply chain failure."""@en ;
dcterms:source "https://sfia-online.org/en/skillcode/9/COPL"^^xsd:anyURI .

skills:CPMG a sfia:Skill , skos:Concept ; 
 skos:inScheme skillcs: ;
    skos:prefLabel "Capacity management"@en ;
    skos:notation "CPMG" ;
    sfia:definedAtLevel sfialevels:CPMG_2,
        sfialevels:CPMG_3,
        sfialevels:CPMG_4,
        sfialevels:CPMG_5,
        sfialevels:CPMG_6 ;
    sfia:skillCategory categories:service_management ;
     skos:definition "Ensuring service components have the capacity and performance to meet current and planned business needs."@en ;
    skos:scopeNote """Service components include, but are not limited to, hardware, software, network resources and software/infrastructure as a service.
Activities may include, but are not limited to:

planning, design and management of the capability, performance, functionality and sustainability of service components to meet business needs
applying data-driven insights to model long-term changes and short-term variations in the level of capacity required to execute the service 
implementing capacity management practices to support cloud-based services and ensure flexible and scalable capacity
deploying techniques to control the demand and add/reduce capacity in a cost-effective, timely manner to meet changes in demand
collaborating closely with other processes and teams to ensure a holistic approach to capacity management
considering external factors, such as regulatory requirements and market trends, when planning and managing capacity
continuously monitoring and optimising resource utilisation to identify cost-saving opportunities and ensure efficient use of resources"""@en ;
dcterms:source "https://sfia-online.org/en/skillcode/9/CPMG"^^xsd:anyURI .

skills:CRIM a sfia:Skill , skos:Concept ; 
 skos:inScheme skillcs: ;
    skos:prefLabel "Cybercrime investigation"@en ;
    skos:notation "CRIM" ;
    sfia:definedAtLevel sfialevels:CRIM_2,
        sfialevels:CRIM_3,
        sfialevels:CRIM_4,
        sfialevels:CRIM_5,
        sfialevels:CRIM_6 ;
    sfia:skillCategory categories:security_services ;
     skos:definition "Investigates cybercrimes, collects evidence, determines incident impacts and collaborates with legal teams to protect digital assets."@en ;
    skos:scopeNote """Cybercrime investigation focuses on identifying, tracking, and building cases against those engaged in criminal activities in cyber/digital environments.
This involves using investigative techniques to uncover criminal patterns, assess cybercrime impacts, and support prosecution efforts.
Activities may include, but are not limited to:

investigating suspicious activities and alleged cyber/digital crimes
collecting evidence from public networks, private systems, and hard-to-access environments like the deep and dark web
gathering and analysing data from systems, networks and devices
collecting and examining physical evidence such as documents, hardware devices and signs of physical interference
identifying clues indicating unauthorised access and evaluating target vulnerabilities
conducting victim and witness interviews and suspect interrogations to gather information
assessing the credibility and authenticity of evidence, and collaborating with legal teams to identify incidents requiring legal action and ensure evidence admissibility
documenting findings and preparing detailed investigative reports for stakeholders
coordinating responses to significant cybercrime incidents
analysing cybercrime trends and developing strategies to combat emerging threats and participating in cybercrime task forces and information sharing initiatives."""@en ;
dcterms:source "https://sfia-online.org/en/skillcode/9/CRIM"^^xsd:anyURI .

skills:CSMG a sfia:Skill , skos:Concept ; 
 skos:inScheme skillcs: ;
    skos:prefLabel "Customer service support"@en ;
    skos:notation "CSMG" ;
    sfia:definedAtLevel sfialevels:CSMG_1,
        sfialevels:CSMG_2,
        sfialevels:CSMG_3,
        sfialevels:CSMG_4,
        sfialevels:CSMG_5,
        sfialevels:CSMG_6 ;
    sfia:skillCategory categories:stakeholder_management ;
     skos:definition "Managing and operating customer service or service desk functions."@en ;
    skos:scopeNote """Customer service support can be managed and delivered across a variety of environments, such as physical contact centres, distributed or virtual teams, and through automated systems like chatbots or self-service portals. These functions may be applied in any customer-facing context, including but not limited to contact centres, service desks, and digital customer interaction channels.
Activities may include, but are not limited to:

managing customer service functions and teams
acting as a point of contact for customers and clients
responding to inquiries and issues
handling requests for information or assistance
managing access to products, services, or systems
processing and fulfilling service requests
maintaining customer satisfaction."""@en ;
dcterms:source "https://sfia-online.org/en/skillcode/9/CSMG"^^xsd:anyURI .

skills:CSOP a sfia:Skill , skos:Concept ; 
 skos:inScheme skillcs: ;
    skos:prefLabel "Certification scheme operation"@en ;
    skos:notation "CSOP" ;
    sfia:definedAtLevel sfialevels:CSOP_2,
        sfialevels:CSOP_3,
        sfialevels:CSOP_4,
        sfialevels:CSOP_5,
        sfialevels:CSOP_6 ;
    sfia:skillCategory categories:skills_management ;
     skos:definition "Designing, developing and operating certification schemes, accreditations and credentials, including digital credentials or badges."@en ;
    skos:scopeNote """The overall purpose of certification for individuals is to recognise their competence to perform a specific task or job, or to determine whether they have met certain knowledge criteria.
Knowledge and competence are distinct and the two terms should not be confused. A certification body is responsible for ensuring that only individuals who demonstrate competence are awarded certification.Certification of individuals provides value by building public confidence and trust. This confidence relies on a valid assessment of competence by a third party, which is reconfirmed at defined intervals. The certification body must act responsibly to provide confidence to interested parties in its competence, impartiality and integrity.
Activities may include, but are not limited to:

verifying, upon request, whether an individual holds a valid certificate and the scope of that certification, except where legal restrictions apply
documenting security policies and procedures, including non-disclosure agreements or other measures to prevent the release of confidential examination materials or involvement in fraudulent practices
implementing procedures for certified individuals to inform the certification body of any changes that could affect their ability to continue meeting certification requirements."""@en ;
dcterms:source "https://sfia-online.org/en/skillcode/9/CSOP"^^xsd:anyURI .

skills:DAAN a sfia:Skill , skos:Concept ; 
 skos:inScheme skillcs: ;
    skos:prefLabel "Data analytics"@en ;
    skos:notation "DAAN" ;
    sfia:definedAtLevel sfialevels:DAAN_2,
        sfialevels:DAAN_3,
        sfialevels:DAAN_4,
        sfialevels:DAAN_5,
        sfialevels:DAAN_6,
        sfialevels:DAAN_7 ;
    sfia:skillCategory categories:data_and_analytics ;
     skos:definition "Enabling data-driven decision making by extracting, analysing and communicating insights from structured and unstructured data."@en ;
    skos:scopeNote """Data analytics focuses on delivering actionable insights from data to drive better decision making. 
Activities may include, but are not limited to:

collecting, processing and analysing data from various sources
ensuring the validity and integrity of data being processed and analysed
identifying trends, patterns and insights using a range of analytical and statistical techniques
developing and validating predictive models
communicating findings to stakeholders
ensuring data quality, integrity and governance
collaborating with teams to align analytics initiatives with business objectives
designing and implementing data analytics solutions and processes
providing actionable recommendations based on domain expertise
staying current with emerging trends and techniques in data analytics
strategic leadership for data analytics and related disciplines such as data science
contributing to data governance policies, standards and good practices.

Data analytics has diverse applications across industries, including customer segmentation, sales forecasting, fraud detection, supply chain optimisation, predictive maintenance, healthcare analytics, financial risk management, HR analytics, social media analytics and public sector analytics."""@en ;
dcterms:source "https://sfia-online.org/en/skillcode/9/DAAN"^^xsd:anyURI .

skills:DATM a sfia:Skill , skos:Concept ; 
 skos:inScheme skillcs: ;
    skos:prefLabel "Data management"@en ;
    skos:notation "DATM" ;
    sfia:definedAtLevel sfialevels:DATM_2,
        sfialevels:DATM_3,
        sfialevels:DATM_4,
        sfialevels:DATM_5,
        sfialevels:DATM_6 ;
    sfia:skillCategory categories:data_and_analytics ;
     skos:definition "Developing and implementing plans, policies and practices that control, protect and optimise the value and governance of data assets."@en ;
    skos:scopeNote """Activities may include, but are not limited to:

developing and enforcing data governance policies to ensure data quality, compliance and ethical usage
developing plans, policies and practices related to areas including, but not limited to, classification, storage, security, quality, sharing, availability, retrieval, retention and publishing
managing data in all its forms, ensuring alignment with business objectives and regulatory requirements
analysing information structures, including logical analysis of taxonomies, ontologies, data, metadata and industry reference data
ensuring data is appropriately stored and archived, in line with relevant legislation
implementing data management practices for cloud-based services
applying ethical principles when handling data.
developing innovative ways to manage data assets
integrating data from multiple sources to support data pipelines and enable additional operations on the data."""@en ;
dcterms:source "https://sfia-online.org/en/skillcode/9/DATM"^^xsd:anyURI .

skills:DATS a sfia:Skill , skos:Concept ; 
 skos:inScheme skillcs: ;
    skos:prefLabel "Data science"@en ;
    skos:notation "DATS" ;
    sfia:definedAtLevel sfialevels:DATS_2,
        sfialevels:DATS_3,
        sfialevels:DATS_4,
        sfialevels:DATS_5,
        sfialevels:DATS_6 ;
    sfia:skillCategory categories:data_and_analytics ;
     skos:definition "Applying mathematics, statistics, data mining and predictive modelling techniques to gain insights, predict behaviours and generate value from data."@en ;
    skos:scopeNote """Data science is typically used for analysing high volume, high velocity and high variety data (numbers, symbols, text, sound and image).
Activities may include, but are not limited to:

integrating methods from mathematics, statistics and probability modelling using specialised programming languages, tools and techniques
sourcing and preparing data for analysis
identifying, validating and exploiting internal and external data sets generated from a diverse range of processes
developing forward-looking, predictive, real-time, model-based insights to create value and drive effective decision-making
finding, selecting, acquiring and ingesting data sources
integrating and cleansing data to make it fit for purpose
developing hypotheses and exploring data using models and analytics sandboxes
refining requirements, validating, training and evolving models over time to discover deeper insights, make predictions or generate recommendations
using advanced analytic techniques including, but not limited to: data/text mining, machine learning, pattern matching, forecasting, visualisation, semantic analysis, sentiment analysis, network and cluster analysis, multivariate statistics, graph analysis, simulation, complex event processing and neural networks."""@en ;
dcterms:source "https://sfia-online.org/en/skillcode/9/DATS"^^xsd:anyURI .

skills:DBAD a sfia:Skill , skos:Concept ; 
 skos:inScheme skillcs: ;
    skos:prefLabel "Database administration"@en ;
    skos:notation "DBAD" ;
    sfia:definedAtLevel sfialevels:DBAD_2,
        sfialevels:DBAD_3,
        sfialevels:DBAD_4,
        sfialevels:DBAD_5 ;
    sfia:skillCategory categories:data_and_records_operations ;
     skos:definition "Installing, configuring, monitoring, maintaining databases and data stores, ensuring performance and security and adapting to evolving technologies."@en ;
    skos:scopeNote """Database administration involves managing operational databases in production environments as well as supporting databases for development, testing and iterative improvements. The focus is on ensuring database availability, integrity, security and performance across a variety of database types, including relational, NoSQL and cloud-based databases.
Activities may include, but are not limited to:

identifying and acting on automation opportunities to improve performance and value from databases, data stores and data pipelines
using database management system software and tools including both cloud-based and on-premises solutions
applying knowledge of the logical database schema
ensuring compliance with data privacy laws and regulations
designing and implementing disaster recovery, backup strategies, and security monitoring protocols
integrating and managing databases across hybrid environments, combining on-premises and cloud-based solutions
monitoring emerging database technologies and trends, including security features and vulnerabilities."""@en ;
dcterms:source "https://sfia-online.org/en/skillcode/9/DBAD"^^xsd:anyURI .

skills:DBDS a sfia:Skill , skos:Concept ; 
 skos:inScheme skillcs: ;
    skos:prefLabel "Database design"@en ;
    skos:notation "DBDS" ;
    sfia:definedAtLevel sfialevels:DBDS_2,
        sfialevels:DBDS_3,
        sfialevels:DBDS_4,
        sfialevels:DBDS_5 ;
    sfia:skillCategory categories:data_and_analytics ;
     skos:definition "Specifying, designing and maintaining mechanisms for storing and accessing data across various environments and platforms."@en ;
    skos:scopeNote """Activities may include, but are not limited to:

designing operational databases, data warehouses, data lakes, or data stores for on-premise, cloud-based, or hybrid environments
defining physical or virtual structures required to support applications, analytics, machine learning, business intelligence or other data-driven services
designing operational data stores to integrate data from multiple sources to support data pipelines and enable additional operations on the data
aligning designs with data architectures, enterprise architectures, standards, policies and regulations
considering scalability, performance, availability, recovery and other operational requirements."""@en ;
dcterms:source "https://sfia-online.org/en/skillcode/9/DBDS"^^xsd:anyURI .

skills:DCMA a sfia:Skill , skos:Concept ; 
 skos:inScheme skillcs: ;
    skos:prefLabel "Facilities management"@en ;
    skos:notation "DCMA" ;
    sfia:definedAtLevel sfialevels:DCMA_2,
        sfialevels:DCMA_3,
        sfialevels:DCMA_4,
        sfialevels:DCMA_5,
        sfialevels:DCMA_6 ;
    sfia:skillCategory categories:technology_management ;
     skos:definition "Planning, designing and managing the buildings, space and facilities which, collectively, make up the IT estate."@en ;
    skos:scopeNote """Activities may include, but are not limited to:

implementing and overseeing data centre management tools
provisioning and managing the physical environment, including power, space and cooling
ensuring adherence to established safety, security and quality standards
ensuring compliance with mandatory health and safety regulations in the workplace
developing and enforcing electrical safety policies
developing and enforcing physical access control policies
analysing environmental data and energy usage statistics to inform decision-making
formulating sustainability strategies for it infrastructure
evaluating and integrating emerging good practices in data centre management"""@en ;
dcterms:source "https://sfia-online.org/en/skillcode/9/DCMA"^^xsd:anyURI .

skills:DEMG a sfia:Skill , skos:Concept ; 
 skos:inScheme skillcs: ;
    skos:prefLabel "Delivery management"@en ;
    skos:notation "DEMG" ;
    sfia:definedAtLevel sfialevels:DEMG_3,
        sfialevels:DEMG_4,
        sfialevels:DEMG_5,
        sfialevels:DEMG_6 ;
    sfia:skillCategory categories:change_implementation ;
     skos:definition "Ensuring successful delivery of new or updated products and services through effective leadership and collaboration within defined delivery cycles."@en ;
    skos:scopeNote """Activities may include, but are not limited to:

selecting, tailoring and guiding teams in the use of delivery approaches
establishing and managing collaborative delivery teams, ensuring they have the necessary resources and skills
maintaining delivery momentum through effective processes, including change control and risk management
conducting reviews, facilitating continuous improvement and monitoring quality and performance
communicating with technical and non-technical stakeholders, using visual techniques for tracking and reporting progress
managing and prioritising work items, planning deliveries and coordinating with stakeholders to align deliverables and milestones
ensuring closure and transition of delivered products/services."""@en ;
dcterms:source "https://sfia-online.org/en/skillcode/9/DEMG"^^xsd:anyURI .

skills:DEMM a sfia:Skill , skos:Concept ; 
 skos:inScheme skillcs: ;
    skos:prefLabel "Demand management"@en ;
    skos:notation "DEMM" ;
    sfia:definedAtLevel sfialevels:DEMM_4,
        sfialevels:DEMM_5,
        sfialevels:DEMM_6 ;
    sfia:skillCategory categories:financial_and_value_management ;
     skos:definition "Analysing and proactively managing business demand for new services or modifications to existing service features or volumes."@en ;
    skos:scopeNote """Activities may include, but are not limited to:

collaborating with the business to prioritise demand to improve business value
developing and communicating insights into patterns of demand
performing what-if analyses and scenario planning to develop insights and proposals to improve business value
proposing responses to meet both short-term and long-term demand and facilitating decision-making and planning
integrating demand analysis and planning with complementary strategic, operational and change planning processes."""@en ;
dcterms:source "https://sfia-online.org/en/skillcode/9/DEMM"^^xsd:anyURI .

skills:DENG a sfia:Skill , skos:Concept ; 
 skos:inScheme skillcs: ;
    skos:prefLabel "Data engineering"@en ;
    skos:notation "DENG" ;
    sfia:definedAtLevel sfialevels:DENG_2,
        sfialevels:DENG_3,
        sfialevels:DENG_4,
        sfialevels:DENG_5,
        sfialevels:DENG_6 ;
    sfia:skillCategory categories:data_and_analytics ;
     skos:definition "Designing, building, operationalising, securing and monitoring data pipelines, stores and real-time processing systems for scalable and reliable data management."@en ;
    skos:scopeNote """Activities may include, but are not limited to:

identifying data sources, data processing concepts and methods
evaluating, designing and implementing on-premise, cloud-based and hybrid data engineering solutions
structuring and storing data for analytics, machine learning, data mining and sharing with applications and organisations
harvesting structured and unstructured data
integrating, consolidating and cleansing data
implementing real-time and batch data processing pipelines
ensuring compliance with data governance, security and privacy standards, including encryption and secure multi-tenancy
managing continuous integration, deployment and monitoring of data pipelines (DataOps)
migrating and converting data
applying ethical principles in handling data
ensuring data storage aligns with relevant legislation
building in security, compliance, scalability, efficiency, reliability, fidelity, flexibility and portability to data engineering solutions."""@en ;
dcterms:source "https://sfia-online.org/en/skillcode/9/DENG"^^xsd:anyURI .

skills:DEPL a sfia:Skill , skos:Concept ; 
 skos:inScheme skillcs: ;
    skos:prefLabel "Deployment"@en ;
    skos:notation "DEPL" ;
    sfia:definedAtLevel sfialevels:DEPL_2,
        sfialevels:DEPL_3,
        sfialevels:DEPL_4,
        sfialevels:DEPL_5,
        sfialevels:DEPL_6 ;
    sfia:skillCategory categories:technology_management ;
     skos:definition "Transitioning software from development to live usage, managing risks and ensuring it works as intended."@en ;
    skos:scopeNote """Activities may include, but are not limited to:

moving new or changed components to testing, staging and live environments
managing deployments using suitable approaches, such as phased rollouts or continuous delivery
maintaining secure locations for components awaiting deployment 
using deployment tools and techniques to ensure consistent and repeatable deployments, supporting governance, audit and change management
monitoring and troubleshooting deployment processes
rolling back deployments in case of issues or failures
ensuring the availability, performance and security of deployed components
collaborating with release management and other teams 
considering supplier-controlled deployments and their impact on the organisation's environment."""@en ;
dcterms:source "https://sfia-online.org/en/skillcode/9/DEPL"^^xsd:anyURI .

skills:DESN a sfia:Skill , skos:Concept ; 
 skos:inScheme skillcs: ;
    skos:prefLabel "Systems design"@en ;
    skos:notation "DESN" ;
    sfia:definedAtLevel sfialevels:DESN_2,
        sfialevels:DESN_3,
        sfialevels:DESN_4,
        sfialevels:DESN_5,
        sfialevels:DESN_6 ;
    sfia:skillCategory categories:systems_development ;
     skos:definition "Designing systems to meet specified requirements and agreed systems architectures."@en ;
    skos:scopeNote """A system is a structured arrangement of components, both physical and digital, designed to work together to meet specific requirements, considering factors such as scalability, security, human interaction and adherence to organisational and regulatory standards.
Systems design activities may include, but are not limited to:

using design concepts to develop a systems design and provide the basis for systems construction and verification
designing or selecting system components
designing systems compatible with contemporary computing architectures and selection of components such as cloud computing service models and edge computing
designing cyber-physical systems that integrate computational and physical components
considering human factors and socio-technical aspects when designing systems that involve significant human interaction
developing a complete set of detailed models, properties and/or characteristics described in a form suitable for implementation
adopting and adapting of system design lifecycle models based on the context of the work using predictive (plan-driven) approaches or adaptive (iterative/agile) approaches for system design
adhering to regulatory requirements and organisational standards including security."""@en ;
dcterms:source "https://sfia-online.org/en/skillcode/9/DESN"^^xsd:anyURI .

skills:DGFS a sfia:Skill , skos:Concept ; 
 skos:inScheme skillcs: ;
    skos:prefLabel "Digital forensics"@en ;
    skos:notation "DGFS" ;
    sfia:definedAtLevel sfialevels:DGFS_2,
        sfialevels:DGFS_3,
        sfialevels:DGFS_4,
        sfialevels:DGFS_5,
        sfialevels:DGFS_6 ;
    sfia:skillCategory categories:security_services ;
     skos:definition "Recovering and investigating material found in digital devices."@en ;
    skos:scopeNote """Digital forensics involves the recovery, analysis, and investigation of material found in digital devices. This skill focuses on extracting and preserving digital evidence to support various types of investigations and legal proceedings.
Activities may include, but are not limited to:

collecting, processing, and analysing digital evidence from computers and other data storage devices
applying specialised forensic tools and techniques to recover and examine digital material
maintaining the integrity and chain of custody for all digital evidence
reconstructing digital events and timelines to support investigative efforts
documenting findings in comprehensive, legally defensible forensic reports
presenting forensic evidence and testifying as an expert witness in legal proceedings
collaborating with cybercrime investigators and legal teams to interpret technical evidence
developing and implementing forensic methodologies for emerging technologies
ensuring compliance with legal and ethical standards in digital evidence handling
supporting various types of investigations, including security vulnerability assessments, criminal cases, fraud inquiries, and counterintelligence efforts."""@en ;
dcterms:source "https://sfia-online.org/en/skillcode/9/DGFS"^^xsd:anyURI .

skills:DIGM a sfia:Skill , skos:Concept ; 
 skos:inScheme skillcs: ;
    skos:prefLabel "Digital marketing"@en ;
    skos:notation "DIGM" ;
    sfia:definedAtLevel sfialevels:DIGM_2,
        sfialevels:DIGM_3,
        sfialevels:DIGM_4,
        sfialevels:DIGM_5 ;
    sfia:skillCategory categories:marketing ;
     skos:definition "Planning and executing activities to promote products, services and brands through digital channels and technologies."@en ;
    skos:scopeNote """Activities may include, but are not limited to:

planning and executing digital marketing activities aligned with overall business objectives
creating and optimising content for various digital platforms including websites, social media, email
managing paid digital advertising campaigns across search, social and display networks
implementing and optimising search engine optimisation (SEO) practices
using marketing automation tools to personalise and streamline marketing efforts
analysing digital marketing metrics and using insights to guide decision-making and tactics
conducting A/B and multivariate testing to optimise digital marketing performance
managing relationships with digital marketing vendors, agencies and platform representatives
staying informed about emerging digital marketing trends, technologies and recognised good practices
ensuring digital marketing activities comply with relevant regulations and platform policies
collaborating with cross-functional teams to align digital marketing efforts with other business initiatives."""@en ;
dcterms:source "https://sfia-online.org/en/skillcode/9/DIGM"^^xsd:anyURI .

skills:DLMG a sfia:Skill , skos:Concept ; 
 skos:inScheme skillcs: ;
    skos:prefLabel "Systems development management"@en ;
    skos:notation "DLMG" ;
    sfia:definedAtLevel sfialevels:DLMG_4,
        sfialevels:DLMG_5,
        sfialevels:DLMG_6,
        sfialevels:DLMG_7 ;
    sfia:skillCategory categories:systems_development ;
     skos:definition "Planning, estimating and executing systems development work to time, budget and quality targets."@en ;
    skos:scopeNote """Systems development include the delivery of projects, initiatives, enhancement requests and the maintenance of existing systems.
Activities may include, but are not limited to:

planning and estimating work
adopting and adapting systems development lifecycle models based on the context of the work and selecting appropriately from predictive (plan-driven) approaches or adaptive (iterative/agile) approaches
collaboration and open communication with stakeholders with a focus on delivering value from systems development
managing risks and allowing for timely adjustment of plans and deliverables to continue to meet customer requirements and deliver value
ensuring systems development work meets the required quality standards
aligning systems development activity and deliverables with architectures and standards and ensuring quality, security and privacy are built in
developing roadmaps to communicate systems development plans
identifying, allocating and managing resources (including staff, equipment and budgets) and how demand will be met with a supply capacity
continuous improvement to refine and optimise systems development processes."""@en ;
dcterms:source "https://sfia-online.org/en/skillcode/9/DLMG"^^xsd:anyURI .

skills:DTAN a sfia:Skill , skos:Concept ; 
 skos:inScheme skillcs: ;
    skos:prefLabel "Data modelling and design"@en ;
    skos:notation "DTAN" ;
    sfia:definedAtLevel sfialevels:DTAN_2,
        sfialevels:DTAN_3,
        sfialevels:DTAN_4,
        sfialevels:DTAN_5 ;
    sfia:skillCategory categories:data_and_analytics ;
     skos:definition "Developing models and diagrams to represent, communicate and manage data requirements and data assets."@en ;
    skos:scopeNote """Data modelling supports activities such as, but not limited to:

helping organisations understand their data assets, develop software systems and map relationships between real-world entities
engaging with stakeholders to gather requirements and ensure data models align with business objectives
facilitating data engineering, integration and interoperability
enhancing data retrieval
supporting data governance and master data management
incorporating industry reference data standards to ensure consistency, interoperability and compliance.

Data models typically include components such as entities, relationships, attributes and domains. There are various types of data models, including relational, object-oriented, NoSQL and time-based.
Data models communicate different levels of detail, including conceptual, logical and physical."""@en ;
dcterms:source "https://sfia-online.org/en/skillcode/9/DTAN"^^xsd:anyURI .

skills:EEXP a sfia:Skill , skos:Concept ; 
 skos:inScheme skillcs: ;
    skos:prefLabel "Employee experience"@en ;
    skos:notation "EEXP" ;
    sfia:definedAtLevel sfialevels:EEXP_4,
        sfialevels:EEXP_5,
        sfialevels:EEXP_6 ;
    sfia:skillCategory categories:people_management ;
     skos:definition "Enhancing employee engagement and ways of working, empowering employees and supporting their health and wellbeing."@en ;
    skos:scopeNote """Activities may include, but are not limited to:

providing opportunities for personal growth and learning
providing sufficient personal freedom to decide how to achieve work objectives, with support available when needed
supporting different views, working styles and behaviours within the work environment
providing a safe and secure working environment with the resources needed to do the job
providing transparent communications and building trust in leadership
providing a holistic approach in support of mental and physical wellbeing.

Note that the term employee is not limited to specific terms of employment. Depending on the employer it may include temporary and contract staff as well as salaried employees."""@en ;
dcterms:source "https://sfia-online.org/en/skillcode/9/EEXP"^^xsd:anyURI .

skills:EMRG a sfia:Skill , skos:Concept ; 
 skos:inScheme skillcs: ;
    skos:prefLabel "Emerging technology monitoring"@en ;
    skos:notation "EMRG" ;
    sfia:definedAtLevel sfialevels:EMRG_4,
        sfialevels:EMRG_5,
        sfialevels:EMRG_6 ;
    sfia:skillCategory categories:strategy_and_planning ;
     skos:definition "Identifying and assessing new and emerging technologies, products, services, methods and techniques."@en ;
    skos:scopeNote """This skill involves systematically tracking, assessing and reporting on emerging technologies and their potential impact on the organisation.
Activities may include, but are not limited to:

conducting regular technology landscape scans
evaluating potential benefits and risks of new technologies
preparing reports and briefings for stakeholders on emerging trends
recommending pilot projects or proofs of concept for promising technologies
collaborating with research and development (R&D) teams to explore innovative applications
attending industry conferences and engaging with technology vendors
developing frameworks for assessing technology readiness and organisational fit
advising on the strategic implications of adopting emerging technologies."""@en ;
dcterms:source "https://sfia-online.org/en/skillcode/9/EMRG"^^xsd:anyURI .

skills:ETDL a sfia:Skill , skos:Concept ; 
 skos:inScheme skillcs: ;
    skos:prefLabel "Learning delivery"@en ;
    skos:notation "ETDL" ;
    sfia:definedAtLevel sfialevels:ETDL_2,
        sfialevels:ETDL_3,
        sfialevels:ETDL_4,
        sfialevels:ETDL_5 ;
    sfia:skillCategory categories:skills_management ;
     skos:definition "Transferring knowledge, developing skills and changing behaviours using a range of techniques, resources and media."@en ;
    skos:scopeNote """Learning delivery uses a variety of techniques, resources and media including: face-to-face learning, e-learning, online virtual environments, fieldwork and projects, self-assessment, peer-assisted learning and simulation. 
Typically, a blend of techniques will be used which can incorporate both formal and informal learning activities.
Activities may include, but are not limited to:

delivering learning content across various formats and platforms
facilitating interactive learning sessions and workshops
assessing learner progress and providing constructive feedback
adapting delivery methods to suit different learning styles and needs
incorporating new technologies and innovative approaches in learning delivery
evaluating the effectiveness of learning delivery methods
promoting a positive learning environment and encouraging learner engagement
collaborating with subject matter experts and instructional designers."""@en ;
dcterms:source "https://sfia-online.org/en/skillcode/9/ETDL"^^xsd:anyURI .

skills:ETMG a sfia:Skill , skos:Concept ; 
 skos:inScheme skillcs: ;
    skos:prefLabel "Learning and development management"@en ;
    skos:notation "ETMG" ;
    sfia:definedAtLevel sfialevels:ETMG_2,
        sfialevels:ETMG_3,
        sfialevels:ETMG_4,
        sfialevels:ETMG_5,
        sfialevels:ETMG_6,
        sfialevels:ETMG_7 ;
    sfia:skillCategory categories:skills_management ;
     skos:definition "Delivering management, advisory and administrative services to support the development of knowledge, skills and competencies."@en ;
    skos:scopeNote """Activities may include, but are not limited to:

developing the full range of professional, business or technical capabilities required by the organisation
developing learning and development strategies and policies
identifying appropriate learning and development solutions, accreditations and qualifications
selecting, tailoring and adopting skills and competency frameworks
selecting and operating learning management systems
administering, documenting, tracking and reporting on learning and development activities."""@en ;
dcterms:source "https://sfia-online.org/en/skillcode/9/ETMG"^^xsd:anyURI .

skills:FEAS a sfia:Skill , skos:Concept ; 
 skos:inScheme skillcs: ;
    skos:prefLabel "Feasibility assessment"@en ;
    skos:notation "FEAS" ;
    sfia:definedAtLevel sfialevels:FEAS_2,
        sfialevels:FEAS_3,
        sfialevels:FEAS_4,
        sfialevels:FEAS_5,
        sfialevels:FEAS_6 ;
    sfia:skillCategory categories:change_analysis ;
     skos:definition "Defining, evaluating and describing business change options for financial, technical and business feasibility and strategic alignment."@en ;
    skos:scopeNote """Activities may include, but are not limited to:

generating and defining options
ensuring options align with the organisation's vision, mission, objectives, strategy and tactics
engaging with relevant stakeholders and specialists
evaluating options for financial, technical and business feasibility.

Feasibility assessment is multi-dimensional. Options for change must be evaluated from several dimensions including, but not limited to: financial, technical, organisational capability and culture, strategic context, economic and/or commercial environment.
Feasibility assessment typically results in a documented business case used to support organisational decision-making about proposed investments. This skill is focused on the generation, analysis and documentation of investment options."""@en ;
dcterms:source "https://sfia-online.org/en/skillcode/9/FEAS"^^xsd:anyURI .

skills:FIAN a sfia:Skill , skos:Concept ; 
 skos:inScheme skillcs: ;
    skos:prefLabel "Financial analysis"@en ;
    skos:notation "FIAN" ;
    sfia:definedAtLevel sfialevels:FIAN_2,
        sfialevels:FIAN_3,
        sfialevels:FIAN_4,
        sfialevels:FIAN_5,
        sfialevels:FIAN_6 ;
    sfia:skillCategory categories:financial_and_value_management ;
     skos:definition "Conducting in-depth analysis of financial data to derive insights and support decision-making."@en ;
    skos:scopeNote """Activities may include, but are not limited to:

preparing financial insights, dashboards and visualisations to support decision-making
developing and maintaining financial models for scenario planning and sensitivity analysis
providing authoritative advice on financial analysis practices and techniques
presenting findings to stakeholders
defining the organisation's approach to financial analysis, aligning it with objectives
implementing financial analysis policies, standards and processes
developing a culture of data-driven decision-making and continuous improvement
providing strategic insights based on comprehensive financial analysis
evaluating investments, projects and services using financial analysis techniques
applying financial analysis to cloud computing, such as consumption-based pricing and cost optimisation."""@en ;
dcterms:source "https://sfia-online.org/en/skillcode/9/FIAN"^^xsd:anyURI .

skills:FMIT a sfia:Skill , skos:Concept ; 
 skos:inScheme skillcs: ;
    skos:prefLabel "Financial management"@en ;
    skos:notation "FMIT" ;
    sfia:definedAtLevel sfialevels:FMIT_4,
        sfialevels:FMIT_5,
        sfialevels:FMIT_6 ;
    sfia:skillCategory categories:financial_and_value_management ;
     skos:definition "Managing the effective use and control of financial resources to support business strategies, compliance and risk mitigation."@en ;
    skos:scopeNote """This skill typically applies to dedicated financial management roles, not to managers of operational or project budgets.
Financial management should align with business strategies and practices in areas such as governance, risk management, portfolio, programme and project management, and asset management.
Activities may include, but are not limited to:

managing financial control and stewardship of assets and resources
supporting strategic financial decision-making and business unit collaboration
aligning budgeting, forecasting and accounting practices with organisational goals
guiding financial management for consumption-based costs like cloud services
promoting financial practices to support iterative/agile working across the organisation
overseeing development of service, project and component cost models to meet strategic objectives
defining and overseeing charging models for service provision
ensuring compliance with accounting standards, policies and regulatory requirements
providing proactive risk management and mitigation strategies
monitoring business unit performance against financial targets and KPIs, offering insights and recommendations."""@en ;
dcterms:source "https://sfia-online.org/en/skillcode/9/FMIT"^^xsd:anyURI .

skills:GOVN a sfia:Skill , skos:Concept ; 
 skos:inScheme skillcs: ;
    skos:prefLabel "Governance"@en ;
    skos:notation "GOVN" ;
    sfia:definedAtLevel sfialevels:GOVN_6,
        sfialevels:GOVN_7 ;
    sfia:skillCategory categories:governance__risk_and_compliance ;
     skos:definition "Defining and operating frameworks for decision-making, risk management, stakeholder relationships and compliance with organisational and regulatory obligations."@en ;
    skos:scopeNote """Governance can be applied to specific activities or may be a single integrated framework across an organisation.
Specialisms include, but are not limited to, security, information, technology, architectures, enterprise IT and service management.
An organisation's obligations may be external or internal including, but not limited to: legislative, regulatory, contractual and adherence to agreed standards/policies or ethical frameworks. 
Activities may include, but are not limited to:

defining and operating the system of rules, practices and processes by which an organisation makes decisions, manages stakeholders' relationships and identifies legitimate authority
integrating risk management into governance frameworks to support informed decision-making
determining how to direct, evaluate and monitor an organisation's activities
developing and operating strategic and operational frameworks, policies, decision-making, business processes and plans to meet stakeholder requirements
ensuring alignment between governance practices and organisational strategy
establishing and maintaining governance committees and reporting structures.

Governance is explicitly referenced in many SFIA skills. Professionals may contribute specialist knowledge to governance processes, reviews and developments, but that does not imply they need the SFIA skill of Governance."""@en ;
dcterms:source "https://sfia-online.org/en/skillcode/9/GOVN"^^xsd:anyURI .

skills:GRDN a sfia:Skill , skos:Concept ; 
 skos:inScheme skillcs: ;
    skos:prefLabel "Graphic design"@en ;
    skos:notation "GRDN" ;
    sfia:definedAtLevel sfialevels:GRDN_1,
        sfialevels:GRDN_2,
        sfialevels:GRDN_3,
        sfialevels:GRDN_4,
        sfialevels:GRDN_5 ;
    sfia:skillCategory categories:content_management ;
     skos:definition "Creating and applying visual concepts to communicate ideas, enhance aesthetics and improve user experience across digital and print media."@en ;
    skos:scopeNote """Graphic design encompasses a broad range of activities including typography, colour theory, layout and visual storytelling.
Activities may include, but are not limited to:

creating visual elements and layouts for digital and print media
interpreting and applying research findings to inform design decisions
applying design principles to ensure visual consistency and effectiveness and that content is accessible and inclusive to all users
developing and iterating design prototypes based on feedback and research findings
ensuring designs adhere to brand guidelines and assignment specifications
collaborating with stakeholders to understand and meet design requirements
maintaining and organising design assets and libraries
developing and implementing design processes and guidelines
creating high-quality graphics and visual elements using design software
producing design mock-ups and interactive prototypes
using specialised hardware/equipment for design tasks."""@en ;
dcterms:source "https://sfia-online.org/en/skillcode/9/GRDN"^^xsd:anyURI .

skills:HCEV a sfia:Skill , skos:Concept ; 
 skos:inScheme skillcs: ;
    skos:prefLabel "User experience design"@en ;
    skos:notation "HCEV" ;
    sfia:definedAtLevel sfialevels:HCEV_2,
        sfialevels:HCEV_3,
        sfialevels:HCEV_4,
        sfialevels:HCEV_5,
        sfialevels:HCEV_6 ;
    sfia:skillCategory categories:user_centred_design ;
     skos:definition "Producing design concepts and prototypes for user interactions and experiences of a product, system or service."@en ;
    skos:scopeNote """This skill is inclusive of a full range of user tasks not just digital tasks. The skill can be applied in various contexts, such as, but not limited to customer experience, products, services, applications, devices, learning experience and employee experience.
Activities may include, but are not limited to:

understanding and addressing design goals, usability and accessibility requirements
using an iterative design process to enhance user satisfaction by improving usability and accessibility 
designing digital and offline tasks, interactions and interfaces
refining designs based on user experience evaluation 
communicating the design to those responsible for design, development and implementation of products, systems and services
creating design artefacts such as sketches, ideas, storyboards, static wireframes, dynamic and workable prototypes
developing alternative design and evaluating advantages, disadvantages, constraints and trade-offs
considering and integrating appropriate visual design and branding elements into user experience design."""@en ;
dcterms:source "https://sfia-online.org/en/skillcode/9/HCEV"^^xsd:anyURI .

skills:HPCC a sfia:Skill , skos:Concept ; 
 skos:inScheme skillcs: ;
    skos:prefLabel "High-performance computing"@en ;
    skos:notation "HPCC" ;
    sfia:definedAtLevel sfialevels:HPCC_4,
        sfialevels:HPCC_5,
        sfialevels:HPCC_6,
        sfialevels:HPCC_7 ;
    sfia:skillCategory categories:computational_science ;
     skos:definition "Using advanced computer systems and special programming techniques to solve complex computational problems."@en ;
    skos:scopeNote """High-performance computing (HPC) is the use of super computers and parallel processing techniques for solving complex computational problems. HPC technology focuses on developing parallel processing algorithms and systems.
High-performance computing is typically used for solving advanced problems and performing research activities through computer modelling, simulation and analysis. Activities may include, but are not limited to:

designing and optimising parallel algorithms
managing and maintaining HPC infrastructures
developing software for HPC environments
conducting performance analysis and optimisation of HPC applications
collaborating with researchers to translate scientific problems into HPC solutions.

HPC technology is implemented in a variety of disciplines including, but not limited to:

biosciences and molecular modelling
geographical data
oil and gas exploration
climate modelling and weather forecasting
physical simulations
cryptanalysis.

The terms high-performance computing and supercomputing are sometimes used interchangeably."""@en ;
dcterms:source "https://sfia-online.org/en/skillcode/9/HPCC"^^xsd:anyURI .

skills:HSIN a sfia:Skill , skos:Concept ; 
 skos:inScheme skillcs: ;
    skos:prefLabel "Systems installation and removal"@en ;
    skos:notation "HSIN" ;
    sfia:definedAtLevel sfialevels:HSIN_1,
        sfialevels:HSIN_2,
        sfialevels:HSIN_3,
        sfialevels:HSIN_4,
        sfialevels:HSIN_5 ;
    sfia:skillCategory categories:technology_management ;
     skos:definition "Installing and testing, or decommissioning and removing, systems or system components."@en ;
    skos:scopeNote """Systems or systems components may include, but are not limited to, hardware, software, cabling, wiring and monitoring equipment.
Activities may include, but are not limited to:

developing and following plans and instructions in accordance with agreed standards
adhering to established safety, security and quality standards
testing of hardware and software components, resolution of malfunctions and recording of results
documenting the details of hardware and software installed so that configuration management records can be updated
safe disconnection, decommissioning and removal of systems or system components."""@en ;
dcterms:source "https://sfia-online.org/en/skillcode/9/HSIN"^^xsd:anyURI .

skills:HWDE a sfia:Skill , skos:Concept ; 
 skos:inScheme skillcs: ;
    skos:prefLabel "Hardware design"@en ;
    skos:notation "HWDE" ;
    sfia:definedAtLevel sfialevels:HWDE_2,
        sfialevels:HWDE_3,
        sfialevels:HWDE_4,
        sfialevels:HWDE_5,
        sfialevels:HWDE_6 ;
    sfia:skillCategory categories:systems_development ;
     skos:definition "Specifying and designing hardware systems and components to meet defined requirements by following agreed design principles and standards."@en ;
    skos:scopeNote """The scope encompasses a wide range of hardware systems and components, including but not limited to processors, specialised computing units, embedded systems, control systems and various sensor and actuator devices. The hardware design should factor in integration needs with IT infrastructures, networking environments, as well as systems architectures such as cloud service models, edge computing and cyber-physical systems.
Activities may include, but are not limited to:

defining how hardware components fit into the system architecture and integrate with software, firmware and other systems
selecting, designing, specifying, integrating and prototyping hardware components and subsystems
considering target environments, performance, security, safety, reliability, sustainability and compatibility requirements
adhering to industry standards including compatibility, safety, security, reliability and sustainability."""@en ;
dcterms:source "https://sfia-online.org/en/skillcode/9/HWDE"^^xsd:anyURI .

skills:IAMT a sfia:Skill , skos:Concept ; 
 skos:inScheme skillcs: ;
    skos:prefLabel "Identity and access management"@en ;
    skos:notation "IAMT" ;
    sfia:definedAtLevel sfialevels:IAMT_1,
        sfialevels:IAMT_2,
        sfialevels:IAMT_3,
        sfialevels:IAMT_4,
        sfialevels:IAMT_5,
        sfialevels:IAMT_6 ;
    sfia:skillCategory categories:security_services ;
     skos:definition "Manages identity verification and access permissions within organisational systems and environments."@en ;
    skos:scopeNote """Activities may include, but are not limited to:

implementing identity and access management (IAM) frameworks in line with organisational goals and compliance with regulations like GDPR, HIPAA, or SOX
streamlining user authentication with single sign-on solutions and enhancing security with multi-factor authentication
managing user access rights from onboarding to offboarding, including integration with cloud services, enterprise applications and directory services like LDAP or Active Directory
using role-based and attribute-based access controls to manage user privileges and access, aligning with organisational roles and attributes
implementing privileged access management tools for secure monitoring and control of critical asset access
handling incident responses related to access issues, like unauthorised access or identity theft
regularly auditing access to maintain security and compliance
conducting identity governance and administration to enforce policies, managing digital identities including user accounts, groups and roles."""@en ;
dcterms:source "https://sfia-online.org/en/skillcode/9/IAMT"^^xsd:anyURI .

skills:ICPM a sfia:Skill , skos:Concept ; 
 skos:inScheme skillcs: ;
    skos:prefLabel "Content publishing"@en ;
    skos:notation "ICPM" ;
    sfia:definedAtLevel sfialevels:ICPM_1,
        sfialevels:ICPM_2,
        sfialevels:ICPM_3,
        sfialevels:ICPM_4,
        sfialevels:ICPM_5,
        sfialevels:ICPM_6 ;
    sfia:skillCategory categories:content_management ;
     skos:definition "Managing processes to collect, assemble and publish content across various channels to meet organisational and audience needs."@en ;
    skos:scopeNote """Information content may be in structured, unstructured or semi-structured forms.
Activities may include, but are not limited to:

understanding the requirements of the organisation and the target audience
evaluating different publishing methods and options, and their costs, features and benefits, including open source and proprietary options
developing and implementing a framework for content publishing, including preferred media, overall information structure and rules for formatting content
identifying, briefing and collaborating with content creators
converting content into a format suitable for publication
delivering content to the user at the point of need
managing copyright, data protection and other legal issues associated with publishing and re-using published information and data
ensuring published material is in a form accessible to all potential users, including those with disabilities
coordinating content across different platforms and ensuring consistent content presence across multiple platforms
publishing new content or archiving outdated material."""@en ;
dcterms:source "https://sfia-online.org/en/skillcode/9/ICPM"^^xsd:anyURI .

skills:IFDN a sfia:Skill , skos:Concept ; 
 skos:inScheme skillcs: ;
    skos:prefLabel "Infrastructure design"@en ;
    skos:notation "IFDN" ;
    sfia:definedAtLevel sfialevels:IFDN_2,
        sfialevels:IFDN_3,
        sfialevels:IFDN_4,
        sfialevels:IFDN_5,
        sfialevels:IFDN_6 ;
    sfia:skillCategory categories:systems_development ;
     skos:definition "Designing technology infrastructure to meet business requirements, ensuring scalability, reliability, security and alignment with strategic objectives."@en ;
    skos:scopeNote """Technology infrastructure encompasses a wide range of components including, but not limited to: physical devices, virtual resources, cloud services, infrastructure-related software, middleware, network services and data storage solutions.
The skill involves defining the components and services that make up the technology environment, their connections, interrelationships and operating parameters, which together ensure infrastructure solutions support current and future business needs.
Activities may include, but are not limited to:

developing detailed infrastructure design specifications and diagrams
ensuring compatibility and integration between different infrastructure components
designing infrastructure for scalability, performance, reliability and security from the outset
ensuring designs adhere to industry standards, regulatory requirements and security protocols
collaborating with stakeholders to align infrastructure design with business objectives
maintaining comprehensive documentation of the design process and decisions
integrating cloud services into the infrastructure design."""@en ;
dcterms:source "https://sfia-online.org/en/skillcode/9/IFDN"^^xsd:anyURI .

skills:INAS a sfia:Skill , skos:Concept ; 
 skos:inScheme skillcs: ;
    skos:prefLabel "Information assurance"@en ;
    skos:notation "INAS" ;
    sfia:definedAtLevel sfialevels:INAS_2,
        sfialevels:INAS_3,
        sfialevels:INAS_4,
        sfialevels:INAS_5,
        sfialevels:INAS_6,
        sfialevels:INAS_7 ;
    sfia:skillCategory categories:security_and_privacy ;
     skos:definition "Protecting against and managing risks related to the use, storage and transmission of data and information systems."@en ;
    skos:scopeNote """Activities include, but are not limited to:

management of risk in a pragmatic and cost-effective manner to ensure stakeholder confidence
formal system certification and accreditation
assessing the effectiveness of cryptographic controls
technical assessment and evaluation to determine control effectiveness.

Information and data are typically protected by following five principles:

availability - ensuring authorised users can easily access the information they need
integrity - protecting information from unauthorised modification, retrieval or deletion
authenticity - validating the identity of users and devices
confidentiality - restricting access to authorised users only
non-repudiation - preventing possible denial that an action occurred by ensuring data is true to its origin."""@en ;
dcterms:source "https://sfia-online.org/en/skillcode/9/INAS"^^xsd:anyURI .

skills:INCA a sfia:Skill , skos:Concept ; 
 skos:inScheme skillcs: ;
    skos:prefLabel "Content design and authoring"@en ;
    skos:notation "INCA" ;
    sfia:definedAtLevel sfialevels:INCA_1,
        sfialevels:INCA_2,
        sfialevels:INCA_3,
        sfialevels:INCA_4,
        sfialevels:INCA_5,
        sfialevels:INCA_6 ;
    sfia:skillCategory categories:content_management ;
     skos:definition "Planning, designing and creating content that meets user-centred and organisational needs, encompassing textual information, graphical content and multimedia elements."@en ;
    skos:scopeNote """Content design and authoring encompasses a wide range of content types to meet user-centred and organisational needs. This includes textual information, graphical content and multimedia elements. Specific content types, include but are not limited to: website and mobile app content, user interface text, chatbot scripts, interactive content, social media content, email marketing, blog posts, online advertising copy and video scripts.
Activities may include, but are not limited to:

understanding the requirements of the intended audience
collaborating with stakeholders and audience representatives to refine content needs
applying tools and technologies to enhance content creation efficiency and quality
implementing user-centred principles in content design, authoring and presentation
considering information architecture, including how content is presented, identified and searched for
managing the content design and authoring process
coordinating with editorial and publication processes
gathering source information and creating draft content
identifying and integrating appropriate illustrations, graphics and multimedia elements
understanding and applying copyright rules and related legal issues
creating and using guidelines for clear, concise and accurate information presentation
designing content collections across multiple media, including digital services and marketing materials."""@en ;
dcterms:source "https://sfia-online.org/en/skillcode/9/INCA"^^xsd:anyURI .

skills:INOV a sfia:Skill , skos:Concept ; 
 skos:inScheme skillcs: ;
    skos:prefLabel "Innovation management"@en ;
    skos:notation "INOV" ;
    sfia:definedAtLevel sfialevels:INOV_5,
        sfialevels:INOV_6,
        sfialevels:INOV_7 ;
    sfia:skillCategory categories:strategy_and_planning ;
     skos:definition "Identifying, prioritising, incubating and exploiting opportunities provided by information, communication and digital technologies."@en ;
    skos:scopeNote """This skill focuses on a systematic, organisational approach to innovation. It is not describing personal behaviours, such as creativity.
Activities may include, but are not limited to:

developing and implementing processes, tools and infrastructures to support innovation
implementing innovation practices to support iterative/agile working
facilitating internal and external communities, employees, commercial partners, customers, users and other stakeholders in the innovation process
providing a framework for governance, monitoring and reporting on the innovation process
building a culture of experimentation and calculated risk-taking
adopting strategies to incorporate external ideas and technologies to enhance and accelerate the organisation's innovation efforts
using data analytics to drive evidence-based innovation.
developing metrics to measure innovation impact and return on investment."""@en ;
dcterms:source "https://sfia-online.org/en/skillcode/9/INOV"^^xsd:anyURI .

skills:INVA a sfia:Skill , skos:Concept ; 
 skos:inScheme skillcs: ;
    skos:prefLabel "Investment appraisal"@en ;
    skos:notation "INVA" ;
    sfia:definedAtLevel sfialevels:INVA_4,
        sfialevels:INVA_5,
        sfialevels:INVA_6 ;
    sfia:skillCategory categories:financial_and_value_management ;
     skos:definition "Assessing the attractiveness of possible investments or projects."@en ;
    skos:scopeNote """Activities may include, but are not limited to:

selecting and using appropriate techniques to compare financial investments and returns
using recognised investment appraisal techniques to compare investment and returns include payback period, accounting rate of return, discounted cash flow (net present value and internal rate of return)
collecting data using appropriate top-down or bottom-up approaches
including other factors into the appraisal approach, such as legal considerations, environmental or social impact, operational benefits and risk
developing scoring methods to allow for subjective benefits or dis-benefits and to aggregate the results of multiple appraisal methods to help compare options
documenting and presenting the results of investment appraisals
establishing investment appraisal as a tool for selecting projects/initiatives for further investigation
identifying possible sources of funding and the impact on the investment appraisal."""@en ;
dcterms:source "https://sfia-online.org/en/skillcode/9/INVA"^^xsd:anyURI .

skills:IRMG a sfia:Skill , skos:Concept ; 
 skos:inScheme skillcs: ;
    skos:prefLabel "Information management"@en ;
    skos:notation "IRMG" ;
    sfia:definedAtLevel sfialevels:IRMG_3,
        sfialevels:IRMG_4,
        sfialevels:IRMG_5,
        sfialevels:IRMG_6,
        sfialevels:IRMG_7 ;
    sfia:skillCategory categories:strategy_and_planning ;
     skos:definition "Enabling the effective management and use of information assets."@en ;
    skos:scopeNote """Information assets represent information deemed valuable by an organisation and may be held in many forms including, but not limited to: digital documents, printed material, microform, e-mail, chats and websites. Information may be structured or unstructured and may be created by internal or external sources.
Specific laws and regulations may require organisations to maintain records of certain business activities and transactions for a minimum period.
Activities may include, but are not limited to:

identifying, classifying, processing information that is used to support decision-making, business processes and digital services
developing innovative ways of managing the information assets of the organisation
governance of how information is used to support decision-making, business processes and digital services
ensuring information can be discovered and delivered in line with organisational policies and practices
developing and promoting strategies and policies for the design of information architectures, structures and taxonomies
implementing systems of cataloguing, metadata, indexing and classification standards and methods used to organise information"""@en ;
dcterms:source "https://sfia-online.org/en/skillcode/9/IRMG"^^xsd:anyURI .

skills:ISCO a sfia:Skill , skos:Concept ; 
 skos:inScheme skillcs: ;
    skos:prefLabel "Information systems coordination"@en ;
    skos:notation "ISCO" ;
    sfia:definedAtLevel sfialevels:ISCO_6,
        sfialevels:ISCO_7 ;
    sfia:skillCategory categories:strategy_and_planning ;
     skos:definition "Coordinating information and technology strategies where the adoption of a common approach would benefit the organisation."@en ;
    skos:scopeNote """This skill is typically applied in large organisations with devolved information, data, technology, digital, cybersecurity functions or in collaborative enterprises of independent organisations.
Activities may include, but are not limited to:

developing and implementing strategies for coordinated deployment across multiple business units, such as, standardising hardware procurement, aligning software licensing and unifying cloud adoption approaches
facilitating communication and collaboration between autonomous units
identifying opportunities for shared services and integration
coordinating enterprise-wide cybersecurity strategies and practices
aligning initiatives with overall business objectives
promoting standardisation of processes and technologies where beneficial
managing cross-functional projects and initiatives
evaluating and recommending enterprise-wide solutions
developing governance frameworks for coordinated management of digital, data and technology."""@en ;
dcterms:source "https://sfia-online.org/en/skillcode/9/ISCO"^^xsd:anyURI .

skills:ITCM a sfia:Skill , skos:Concept ; 
 skos:inScheme skillcs: ;
    skos:prefLabel "Contract management"@en ;
    skos:notation "ITCM" ;
    sfia:definedAtLevel sfialevels:ITCM_2,
        sfialevels:ITCM_3,
        sfialevels:ITCM_4,
        sfialevels:ITCM_5,
        sfialevels:ITCM_6,
        sfialevels:ITCM_7 ;
    sfia:skillCategory categories:stakeholder_management ;
     skos:definition "Managing and operating formal contracts, addressing supplier and client needs in product and service provision."@en ;
    skos:scopeNote """Activities may include, but are not limited to:

overseeing contracts from initiation and negotiation to renewal or termination
ensuring effective communication and collaboration with internal teams, suppliers and clients
maintaining alignment with laws, regulations and organisational policies
evaluating contract performance against agreed metrics and key performance indicators (KPIs)
managing contract variations and adjustments in response to evolving business needs or market conditions
assessing and mitigating risks associated with contractual agreements
integrating sustainability and ethical considerations into contract management
using contract management software and tools for improved efficiency and accuracy
incorporating contract management practices tailored to cloud-based services."""@en ;
dcterms:source "https://sfia-online.org/en/skillcode/9/ITCM"^^xsd:anyURI .

skills:ITMG a sfia:Skill , skos:Concept ; 
 skos:inScheme skillcs: ;
    skos:prefLabel "Technology service management"@en ;
    skos:notation "ITMG" ;
    sfia:definedAtLevel sfialevels:ITMG_5,
        sfialevels:ITMG_6,
        sfialevels:ITMG_7 ;
    sfia:skillCategory categories:technology_management ;
     skos:definition "Managing the provision of technology-based services to meet defined organisational needs."@en ;
    skos:scopeNote """Technology-based services may include, but are not limited to, IT infrastructure, audio-visual services, end-user computing, enterprise applications, facilities, communications services and industrial control systems.
Activities may include, but are not limited to:

approving, preparing, planning and managing new or changed services
managing the performance of systems and services in terms of their contribution to business outcomes, financial costs and sustainability
end-to-end management of services, whether delivered internally or sourced externally
integrating internal and external services as well as delivery options leveraging multiple service delivery capabilities
developing and implementing continual service improvement plans to ensure the technology services adequately support changing needs."""@en ;
dcterms:source "https://sfia-online.org/en/skillcode/9/ITMG"^^xsd:anyURI .

skills:ITOP a sfia:Skill , skos:Concept ; 
 skos:inScheme skillcs: ;
    skos:prefLabel "Infrastructure operations"@en ;
    skos:notation "ITOP" ;
    sfia:definedAtLevel sfialevels:ITOP_1,
        sfialevels:ITOP_2,
        sfialevels:ITOP_3,
        sfialevels:ITOP_4,
        sfialevels:ITOP_5 ;
    sfia:skillCategory categories:technology_management ;
     skos:definition "Provisioning, deploying, configuring, operating and optimising technology infrastructure across physical, virtual and cloud-based environments."@en ;
    skos:scopeNote """Technology infrastructure encompasses a wide range of components including, but not limited to, physical devices, virtual resources, cloud services, infrastructure-related software, middleware, network services and data storage solutions.
Infrastructure operations also involves implementing automation, cybersecurity measures and the adoption of cloud technologies to enhance efficiency, security and agility.
These components may be on-premises, outsourced to third parties, or provisioned through cloud services.
Activities may include, but are not limited to:

provisioning and adapting infrastructure components to meet the evolving needs of users and service providers
managing virtual, cloud and hybrid/multi-cloud environments
automating tasks through scripting, coding, orchestration tools and infrastructure as code (IaC) practices
ensuring infrastructure security through regular updates, patch management and adherence to cybersecurity policies and established industry practices
monitoring infrastructure performance and its impact on efficiency, performance, security posture and sustainability
collaborating with development teams (DevOps) 
using containerisation technologies to enhance application deployment and scalability."""@en ;
dcterms:source "https://sfia-online.org/en/skillcode/9/ITOP"^^xsd:anyURI .

skills:ITSP a sfia:Skill , skos:Concept ; 
 skos:inScheme skillcs: ;
    skos:prefLabel "Strategic planning"@en ;
    skos:notation "ITSP" ;
    sfia:definedAtLevel sfialevels:ITSP_4,
        sfialevels:ITSP_5,
        sfialevels:ITSP_6,
        sfialevels:ITSP_7 ;
    sfia:skillCategory categories:strategy_and_planning ;
     skos:definition "Creating and maintaining organisational-level strategies to align overall business plans, actions and resources with high-level business objectives."@en ;
    skos:scopeNote """This skill is primarily focused on enterprise-wide strategic planning and management, rather than developing strategies for specific technical or functional areas. For senior managers or individuals working on their own technical or functional strategies, this skill may be too broad and high-level. Instead, they may require more specific skills related to their particular domain or area of expertise.
Activities may include, but are not limited to:

conducting environmental analyses to inform strategy development
collaborating with stakeholders to formulate and implement strategies and action plans
using data analytics and digital tools to support strategic decision-making and monitor progress
ensuring agility and flexibility in strategy execution to adapt to changing business needs
communicating and embedding strategic management through objectives, accountabilities and progress monitoring
continuously reviewing and iterating strategic plans to maintain alignment with business goals."""@en ;
dcterms:source "https://sfia-online.org/en/skillcode/9/ITSP"^^xsd:anyURI .

skills:JADN a sfia:Skill , skos:Concept ; 
 skos:inScheme skillcs: ;
    skos:prefLabel "Job analysis and design"@en ;
    skos:notation "JADN" ;
    sfia:definedAtLevel sfialevels:JADN_3,
        sfialevels:JADN_4,
        sfialevels:JADN_5 ;
    sfia:skillCategory categories:change_planning ;
     skos:definition "Planning, analysing and designing job roles and structures to align with organisational requirements, goals and culture."@en ;
    skos:scopeNote """Activities may include, but are not limited to:

gathering information and insights for current and future job requirements through methods such as surveys, interviews, workforce analytics and reviewing existing job documentation
conducting task analysis to break down jobs into component roles and responsibilities, skills and competencies
analysing workflow processes to design jobs that optimise efficiency, employee engagement and job satisfaction
designing roles that support rapid team reconfiguration, upskilling and evolving in response to changing organisational needs and market demands
creating or updating job architectures, job descriptions and specifications based on comprehensive analysis, organisational requirements and skills-based frameworks
integrating new technologies, processes, or operational needs into job design, including the consideration of artificial intelligence and digital tools
developing career pathways that align with professional development opportunities and organisational needs to aid staff retention.

The scope of job analysis and design can range from single roles to multi-layered organisational structures."""@en ;
dcterms:source "https://sfia-online.org/en/skillcode/9/JADN"^^xsd:anyURI .

skills:KNOW a sfia:Skill , skos:Concept ; 
 skos:inScheme skillcs: ;
    skos:prefLabel "Knowledge management"@en ;
    skos:notation "KNOW" ;
    sfia:definedAtLevel sfialevels:KNOW_2,
        sfialevels:KNOW_3,
        sfialevels:KNOW_4,
        sfialevels:KNOW_5,
        sfialevels:KNOW_6,
        sfialevels:KNOW_7 ;
    sfia:skillCategory categories:content_management ;
     skos:definition "Systematically capturing, developing and leveraging vital knowledge to create value and enhance organisational performance."@en ;
    skos:scopeNote """Knowledge management aims to improve performance, support decision-making and mitigate risks. 
Activities may include, but are not limited to:

systematically capturing, sharing, developing and exploiting the collective knowledge of the organisation
tailoring knowledge management practices to fit organisational needs and culture
developing a supportive and collaborative knowledge-sharing culture, integrating both human and technological aspects
providing access to informal, tacit knowledge as well as formal, documented, explicit knowledge
facilitating internal and external collaboration and communications
establishing and supporting communities of practice
capturing, organising and developing information, knowledge and stories from employees, customers and external partners
external benchmarking."""@en ;
dcterms:source "https://sfia-online.org/en/skillcode/9/KNOW"^^xsd:anyURI .

skills:LEDA a sfia:Skill , skos:Concept ; 
 skos:inScheme skillcs: ;
    skos:prefLabel "Competency assessment"@en ;
    skos:notation "LEDA" ;
    sfia:definedAtLevel sfialevels:LEDA_2,
        sfialevels:LEDA_3,
        sfialevels:LEDA_4,
        sfialevels:LEDA_5,
        sfialevels:LEDA_6 ;
    sfia:skillCategory categories:skills_management ;
     skos:definition "Assessing knowledge, skills, competency and behaviours by any means, whether formal or informal, against frameworks such as SFIA."@en ;
    skos:scopeNote """Competency assessment is a specialised practice for evaluating skills and competencies, distinct from performance appraisals and general capability understanding. Unlike performance reviews which focus on job performance and contributions, competency assessment objectively measures technical and professional capabilities.
Assessments may be conducted in various contexts, including: recruitment, career progression, professional development planning, or accreditation/certification.
Activities may include, but are not limited to:

evaluating and selecting assessment options
adopting or adapting assessment methods, tools and techniques
considering the context of the assessment and how the results of the assessment will be used
aligning assessments with ethical, legal and regulatory requirements. 

Ethical, legal and regulatory requirements are essential for ensuring the integrity of assessments and protecting personal data."""@en ;
dcterms:source "https://sfia-online.org/en/skillcode/9/LEDA"^^xsd:anyURI .

skills:MEAS a sfia:Skill , skos:Concept ; 
 skos:inScheme skillcs: ;
    skos:prefLabel "Measurement"@en ;
    skos:notation "MEAS" ;
    sfia:definedAtLevel sfialevels:MEAS_2,
        sfialevels:MEAS_3,
        sfialevels:MEAS_4,
        sfialevels:MEAS_5,
        sfialevels:MEAS_6 ;
    sfia:skillCategory categories:financial_and_value_management ;
     skos:definition "Developing and operating a measurement capability to support agreed organisational information needs."@en ;
    skos:scopeNote """Measurement can be applied to organisations, projects, processes and work products.
Activities may include, but are not limited to:

planning, implementation and control of activities to measure attributes of processes, products and services
using measures to assess performance and progress and provide indications and insights to actual or potential problems, issues and risks
identifying requirements for measurement
implementing measurement to support iterative/agile working practices
selecting measures and measurement scales, setting target values and thresholds
establishing data collection and analysis methods, including automation
real-time and near-real-time measurement.

The measurement skill has diverse applications across industries, including customer experience, IT systems and services, marketing, supply chain, software development, finance, healthcare and project management."""@en ;
dcterms:source "https://sfia-online.org/en/skillcode/9/MEAS"^^xsd:anyURI .

skills:METL a sfia:Skill , skos:Concept ; 
 skos:inScheme skillcs: ;
    skos:prefLabel "Methods and tools"@en ;
    skos:notation "METL" ;
    sfia:definedAtLevel sfialevels:METL_2,
        sfialevels:METL_3,
        sfialevels:METL_4,
        sfialevels:METL_5,
        sfialevels:METL_6 ;
    sfia:skillCategory categories:advice_and_guidance ;
     skos:definition "Leads the adoption, management and optimisation of methods and tools, ensuring effective use and alignment with organisational objectives."@en ;
    skos:scopeNote """There is a wide range of methods and tools supporting areas such as, but not limited to, planning, development, testing, operation, management and maintenance of systems.
The focus is on ensuring these methods and tools are not just available but are appropriately managed, refined and applied across the organisation to enhance efficiency, quality and consistency.
Activities may include, but are not limited to:

assessing, selecting and implementing methods and tools
stewardship of methods and tools to enable effective use by others
measuring, tailoring, improving and automating the use of methods and tools
developing and maintaining documentation and user guides for methods and tools
providing guidance, support and training for the adoption of new methods and tools
evaluating the effectiveness of implemented methods and tools
staying informed about industry developments related to methods and tools
aligning methods and tools with organisational standards and good practices."""@en ;
dcterms:source "https://sfia-online.org/en/skillcode/9/METL"^^xsd:anyURI .

skills:MKCM a sfia:Skill , skos:Concept ; 
 skos:inScheme skillcs: ;
    skos:prefLabel "Marketing campaign management"@en ;
    skos:notation "MKCM" ;
    sfia:definedAtLevel sfialevels:MKCM_3,
        sfialevels:MKCM_4,
        sfialevels:MKCM_5 ;
    sfia:skillCategory categories:marketing ;
     skos:definition "Executing, monitoring and optimising marketing campaigns across various channels to engage target audiences and achieve desired outcomes."@en ;
    skos:scopeNote """Activities may include, but are not limited to:

developing campaign strategies and selecting appropriate channels and tools
writing creative briefs and evaluating creative concepts
collaborating with internal teams and external agencies to develop compelling marketing content
implementing and monitoring multi-channel marketing campaigns
selecting appropriate tools and channels to reach target audiences
developing and distributing marketing content and materials
organising and participating in marketing events and initiatives
analysing campaign performance and optimising for better results."""@en ;
dcterms:source "https://sfia-online.org/en/skillcode/9/MKCM"^^xsd:anyURI .

skills:MKTG a sfia:Skill , skos:Concept ; 
 skos:inScheme skillcs: ;
    skos:prefLabel "Marketing management"@en ;
    skos:notation "MKTG" ;
    sfia:definedAtLevel sfialevels:MKTG_4,
        sfialevels:MKTG_5,
        sfialevels:MKTG_6,
        sfialevels:MKTG_7 ;
    sfia:skillCategory categories:marketing ;
     skos:definition "Developing, implementing and managing marketing strategies and plans to achieve organisational objectives and drive business growth."@en ;
    skos:scopeNote """Activities may include, but are not limited to:

defining marketing strategy, goals and target customers
creating and executing comprehensive marketing plans
managing marketing budgets and resources
aligning marketing activities with business objectives
measuring and analysing marketing effectiveness and return on investment (ROI)
supporting business development and growth initiatives
evaluating and optimising marketing activities
developing creative solutions to brand and business challenges
adapting strategies based on market insights and performance data
collaborating with stakeholders to inform and execute strategies."""@en ;
dcterms:source "https://sfia-online.org/en/skillcode/9/MKTG"^^xsd:anyURI .

skills:MLNG a sfia:Skill , skos:Concept ; 
 skos:inScheme skillcs: ;
    skos:prefLabel "Machine learning"@en ;
    skos:notation "MLNG" ;
    sfia:definedAtLevel sfialevels:MLNG_2,
        sfialevels:MLNG_3,
        sfialevels:MLNG_4,
        sfialevels:MLNG_5,
        sfialevels:MLNG_6 ;
    sfia:skillCategory categories:data_and_analytics ;
     skos:definition "Developing systems that learn from data and experience, improving performance, accuracy and adaptability in dynamic environments."@en ;
    skos:scopeNote """Activities may include, but are not limited to:

assessing the suitability of machine learning for business problems
selecting and applying appropriate machine learning techniques, algorithms and tools to solve business problems
preparing data for machine learning, including cleansing, transformation and feature engineering
designing, training, optimising and retraining models using supervised, unsupervised or reinforcement learning
managing MLOps for model deployment, monitoring and lifecycle management
evaluating models for performance, robustness, fairness and bias, and selecting metrics to assess outcomes
diagnosing and resolving issues before and after deployment
anticipating organisational implications, including ethics, bias, privacy, sustainability and data protection
establishing traceability for outcomes produced by machine learning systems
implementing continuous learning mechanisms to ensure models adapt to new data and changing environments, including real-time adaptation to new inputs and evolving conditions."""@en ;
dcterms:source "https://sfia-online.org/en/skillcode/9/MLNG"^^xsd:anyURI .

skills:MRCH a sfia:Skill , skos:Concept ; 
 skos:inScheme skillcs: ;
    skos:prefLabel "Market research"@en ;
    skos:notation "MRCH" ;
    sfia:definedAtLevel sfialevels:MRCH_3,
        sfialevels:MRCH_4,
        sfialevels:MRCH_5,
        sfialevels:MRCH_6 ;
    sfia:skillCategory categories:marketing ;
     skos:definition "Gathering, analysing and interpreting data about markets, customers and competitors to inform business decisions and strategies."@en ;
    skos:scopeNote """Market research involves systematically collecting, analysing and interpreting data from various sources to understand market trends, customer needs and preferences and competitive landscapes. This skill applies to both qualitative and quantitative research methods.
Activities may include, but are not limited to:

designing and conducting market research studies using surveys, focus groups, interviews and other methods
analysing market data to identify trends, opportunities and challenges
segmenting markets and identifying target customers based on research findings
monitoring competitor activities and analysing their strategies and performance
communicating research findings and recommendations to stakeholders to inform decision-making and strategy development."""@en ;
dcterms:source "https://sfia-online.org/en/skillcode/9/MRCH"^^xsd:anyURI .

skills:NFTS a sfia:Skill , skos:Concept ; 
 skos:inScheme skillcs: ;
    skos:prefLabel "Non-functional testing"@en ;
    skos:notation "NFTS" ;
    sfia:definedAtLevel sfialevels:NFTS_1,
        sfialevels:NFTS_2,
        sfialevels:NFTS_3,
        sfialevels:NFTS_4,
        sfialevels:NFTS_5,
        sfialevels:NFTS_6 ;
    sfia:skillCategory categories:systems_development ;
     skos:definition "Assessing systems and services to evaluate performance, security, scalability and other non-functional qualities against requirements or expected standards."@en ;
    skos:scopeNote """Non-functional testing assesses the behaviour of technology, system components, configurations and packages, ensuring they work together to support the system's operation. It focuses on identifying and mitigating risks related to system qualities and characteristics, such as performance, security, backup and recovery, availability, scalability, reliability, maintainability, monitoring, resource efficiency and compliance with technical standards.
Activities may include, but are not limited to:

collaborating with stakeholders to clarify non-functional requirements and expectations
setting up test environments that mirror production conditions, simulating real-world usage
preparing and managing test data to accurately represent necessary variety and volumes
designing and executing stress, load, security and other non-functional tests
troubleshooting issues during testing, coordinating with technical teams to resolve problems
participating in reviews to refine non-functional requirements, identifying risks and suggesting enhancements
analysing results to assess system performance, security and other key qualities, providing insights for improvement
promoting a shift-left approach by integrating non-functional testing early in the lifecycle for early issue detection
adapting testing strategies to suit various development methodologies
developing and maintaining automated tests, monitoring systems and frameworks to continuously assess system quality and performance
ensuring compliance with industry standards, regulations and recognised good practices."""@en ;
dcterms:source "https://sfia-online.org/en/skillcode/9/NFTS"^^xsd:anyURI .

skills:NTAS a sfia:Skill , skos:Concept ; 
 skos:inScheme skillcs: ;
    skos:prefLabel "Network support"@en ;
    skos:notation "NTAS" ;
    sfia:definedAtLevel sfialevels:NTAS_1,
        sfialevels:NTAS_2,
        sfialevels:NTAS_3,
        sfialevels:NTAS_4,
        sfialevels:NTAS_5 ;
    sfia:skillCategory categories:technology_management ;
     skos:definition "Providing maintenance and support services for communications networks."@en ;
    skos:scopeNote """Activities may include, but are not limited to:

monitoring network performance, investigating issues, troubleshooting and testing network devices
implementing and managing network security measures, including access control, authentication, encryption and intrusion detection/prevention
configuring and maintaining network solutions across physical, virtual and cloud environments
automating network support tasks using scripting, automation tools and orchestration platforms
creating and maintaining network documentation, including diagrams, configuration files and procedures
providing technical support, advice and guidance to users and collaborating with others to resolve network issues
analysing network performance, generating reports and presenting findings and recommendations to stakeholders
collaborating with others to ensure seamless integration and operation across all environments."""@en ;
dcterms:source "https://sfia-online.org/en/skillcode/9/NTAS"^^xsd:anyURI .

skills:NTDS a sfia:Skill , skos:Concept ; 
 skos:inScheme skillcs: ;
    skos:prefLabel "Network design"@en ;
    skos:notation "NTDS" ;
    sfia:definedAtLevel sfialevels:NTDS_2,
        sfialevels:NTDS_3,
        sfialevels:NTDS_4,
        sfialevels:NTDS_5,
        sfialevels:NTDS_6 ;
    sfia:skillCategory categories:systems_development ;
     skos:definition "Designing communication networks to meet business requirements, ensuring scalability, reliability, security and alignment with strategic objectives."@en ;
    skos:scopeNote """Network design covers all aspects of the communications infrastructure, including, but not limited to: networks that are wired or wireless, digital or analogue, virtual or physical, local area, wide area, mobile/cellular and any other defined protocols and scales of operation. In the cloud context, network design also includes designing virtual network topologies, hybrid cloud connectivity and leveraging cloud-native networking services to ensure scalability, security and performance. 
Activities may include, but are not limited to:

analysing business requirements and translating them into network design specifications
designing network topologies, security measures and connectivity solutions for various environments
defining network configurations and policies using code
planning for network scalability, redundancy and high availability, including in cloud-based networks
defining network infrastructure as code to enable automation and streamline provisioning and management
designing disaster recovery and business continuity solutions to ensure network resilience and minimise downtime
collaborating with stakeholders to ensure network designs align with business objectives and industry standards."""@en ;
dcterms:source "https://sfia-online.org/en/skillcode/9/NTDS"^^xsd:anyURI .

skills:NUAN a sfia:Skill , skos:Concept ; 
 skos:inScheme skillcs: ;
    skos:prefLabel "Numerical analysis"@en ;
    skos:notation "NUAN" ;
    sfia:definedAtLevel sfialevels:NUAN_4,
        sfialevels:NUAN_5,
        sfialevels:NUAN_6,
        sfialevels:NUAN_7 ;
    sfia:skillCategory categories:computational_science ;
     skos:definition "Creating, analysing, implementing, testing and improving algorithms for numerically solving mathematical problems."@en ;
    skos:scopeNote """Numerical analysis is the area of mathematics and computer science that creates, analyses and implements algorithms for numerically solving mathematical problems. Numerical analysis is required for applications including, but not limited to:

simulations of physical systems
machine learning
data analytics 

Numerical analysis is concerned with:

floating-point arithmetic and the resulting accumulation of rounding errors (integer arithmetic which has different considerations)
consideration of the numerical stability, condition numbers, accuracy, computational complexity and usability of algorithms that solve mathematical problems.

Activities may include, but are not limited to:

developing and implementing numerical algorithms
analysing and optimising the efficiency of numerical methods
evaluating and improving the accuracy of computational results
collaborating with domain experts to apply numerical solutions to real-world problems
documenting and communicating complex numerical concepts to non-specialists."""@en ;
dcterms:source "https://sfia-online.org/en/skillcode/9/NUAN"^^xsd:anyURI .

skills:OCDV a sfia:Skill , skos:Concept ; 
 skos:inScheme skillcs: ;
    skos:prefLabel "Organisational capability development"@en ;
    skos:notation "OCDV" ;
    sfia:definedAtLevel sfialevels:OCDV_5,
        sfialevels:OCDV_6,
        sfialevels:OCDV_7 ;
    sfia:skillCategory categories:change_planning ;
     skos:definition "Providing leadership, advice and implementation support to assess organisational capabilities and to identify, prioritise and implement improvements."@en ;
    skos:scopeNote """Activities may include, but are not limited to:

selecting, adopting and integrating appropriate industry frameworks and models to guide improvements
using capability maturity assessments, metrics, process definition and process management
building repeatable and reliable capabilities through a process of trial, feedback, learning and continual evolution
developing appropriate techniques, tools and enhanced skills
designing and delivering integrated people, process and technology solutions to deliver improved organisational performance in line with strategic plans and objectives
identifying organisational priorities for enhancing performance, satisfying new business opportunities or responding to external drivers.

The scope of improvement is typically organisation-wide but may also be highly focused on areas such as, but not limited to, business agility, software development, systems development, project delivery, service integration and management, service delivery, information and cyber-security."""@en ;
dcterms:source "https://sfia-online.org/en/skillcode/9/OCDV"^^xsd:anyURI .

skills:OCEN a sfia:Skill , skos:Concept ; 
 skos:inScheme skillcs: ;
    skos:prefLabel "Organisational change enablement"@en ;
    skos:notation "OCEN" ;
    sfia:definedAtLevel sfialevels:OCEN_4,
        sfialevels:OCEN_5,
        sfialevels:OCEN_6 ;
    sfia:skillCategory categories:change_planning ;
     skos:definition "Facilitates cultural and behavioural change by enabling individuals and teams to embed new ways of working and adapt to changes."@en ;
    skos:scopeNote """Organisational change enablement is focused on the human and cultural aspects of change and supporting individuals and teams adapting to new work practices.
The key elements are: stakeholder engagement for commitment, ongoing support for embedding changes and tailored communication addressing behavioural impacts and emotional readiness.
Activities may include, but are not limited to:

facilitating engagement sessions with leaders and managers to secure commitment to change initiatives
defining communication strategies that address behavioural impacts and emotional readiness
supporting individuals and teams in adopting new ways of working, providing resources for skill and behaviour development
addressing and resolving issues during the implementation of change initiatives to ensure minimal disruption
creating and managing networks of change agents to support and drive change
advising leaders on monitoring and supporting behavioural change and addressing challenges
establishing feedback processes to analyse the impact and effectiveness of change initiatives."""@en ;
dcterms:source "https://sfia-online.org/en/skillcode/9/OCEN"^^xsd:anyURI .

skills:OCOP a sfia:Skill , skos:Concept ; 
 skos:inScheme skillcs: ;
    skos:prefLabel "Offensive cyber operations"@en ;
    skos:notation "OCOP" ;
    sfia:definedAtLevel sfialevels:OCOP_2,
        sfialevels:OCOP_3,
        sfialevels:OCOP_4,
        sfialevels:OCOP_5,
        sfialevels:OCOP_6 ;
    sfia:skillCategory categories:security_services ;
     skos:definition "Plans, executes and manages offensive cybersecurity operations, including target selection, electronic target folders and post-operation analysis."@en ;
    skos:scopeNote """Activities may include, but are not limited to:

developing and executing strategies for offensive cyber operations
selecting and profiling targets using intelligence and operational objectives
creating and maintaining electronic target folders to organise target information
coordinating and managing cyber operations, ensuring operational security
evaluating intelligence cost versus operational benefit
assessing potential collateral damage, including second and third-order effects
conducting post-operation assessments and impact analysis.
collaborating with intelligence and security teams to integrate operations with broader objectives."""@en ;
dcterms:source "https://sfia-online.org/en/skillcode/9/OCOP"^^xsd:anyURI .

skills:OFCL a sfia:Skill , skos:Concept ; 
 skos:inScheme skillcs: ;
    skos:prefLabel "Organisational facilitation"@en ;
    skos:notation "OFCL" ;
    sfia:definedAtLevel sfialevels:OFCL_4,
        sfialevels:OFCL_5,
        sfialevels:OFCL_6 ;
    sfia:skillCategory categories:people_management ;
     skos:definition "Supporting workgroups to implement principles and practices for effective teamwork across organisational boundaries and professional specialisms."@en ;
    skos:scopeNote """Activities may include, but are not limited to:

developing and implementing team principles and practices for decision-making, prioritisation and problem-solving
helping teams adopt new/contemporary working practices and behaviours including, but not limited to, specific agile methodologies, processes, tools and ceremonies
helping teams plan and prioritise their workload based on their capacity and track record of working
removing barriers or impediments to teams achieving their mission and objectives
providing guidance and suggestions to support team members in adopting self-management and cross-functional working
reviewing team effectiveness, identifying what went well, what could be improved, and what might be added or removed from their working practices.

Workgroups may be focused on project, product or process management or may be focused on specific problems or deliverables.
Workshop facilitation tools and techniques form part of applying this skill but are not sufficient. This skill describes a broader set of responsibilities."""@en ;
dcterms:source "https://sfia-online.org/en/skillcode/9/OFCL"^^xsd:anyURI .

skills:ORDI a sfia:Skill , skos:Concept ; 
 skos:inScheme skillcs: ;
    skos:prefLabel "Organisation design and implementation"@en ;
    skos:notation "ORDI" ;
    sfia:definedAtLevel sfialevels:ORDI_3,
        sfialevels:ORDI_4,
        sfialevels:ORDI_5,
        sfialevels:ORDI_6,
        sfialevels:ORDI_7 ;
    sfia:skillCategory categories:change_planning ;
     skos:definition "Planning, designing and implementing an integrated organisation structure and culture."@en ;
    skos:scopeNote """Activities may include, but are not limited to:

facilitating changes needed to adapt to evolving technologies, societal shifts, new operating models and business processes
defining and embedding key cultural attributes to enhance organisational performance
designing and implementing new organisational structures, reporting lines and key parameters such as spans of control to align with strategic goals and improve adaptability
aligning organisational design with business strategy and objectives, including digital transformation initiatives
analysing skills gaps and developing strategies to address them, including upskilling and reskilling programmes
facilitating cross-functional collaboration, promoting agile and flexible structures and reducing organisational silos
applying tools such as design thinking, systems thinking, collaboration tools and data analytics in organisation design to inform decisions
implementing organisational designs to improve responsiveness and adaptability.

The scope of organisation design is broad, encompassing workplace environments, location strategies, role profiles, performance measurements, competencies, skills and the integration of new technologies."""@en ;
dcterms:source "https://sfia-online.org/en/skillcode/9/ORDI"^^xsd:anyURI .

skills:PBMG a sfia:Skill , skos:Concept ; 
 skos:inScheme skillcs: ;
    skos:prefLabel "Problem management"@en ;
    skos:notation "PBMG" ;
    sfia:definedAtLevel sfialevels:PBMG_2,
        sfialevels:PBMG_3,
        sfialevels:PBMG_4,
        sfialevels:PBMG_5 ;
    sfia:skillCategory categories:service_management ;
     skos:definition "Managing the lifecycle of all problems that have occurred or could occur in delivering a service."@en ;
    skos:scopeNote """The primary objectives of problem management are to:

proactively prevent problems and resulting incidents from happening
reactively resolve problems that have already happened
eliminate recurring incidents
minimise the impact of incidents that cannot be prevented.

Activities may include, but are not limited to:

detecting and logging problems
classifying and prioritising problems
initiating actions to resolve problems
investigating and diagnosing problems
implementing remedies to prevent future incidents
reporting on problems."""@en ;
dcterms:source "https://sfia-online.org/en/skillcode/9/PBMG"^^xsd:anyURI .

skills:PDSV a sfia:Skill , skos:Concept ; 
 skos:inScheme skillcs: ;
    skos:prefLabel "Professional development"@en ;
    skos:notation "PDSV" ;
    sfia:definedAtLevel sfialevels:PDSV_4,
        sfialevels:PDSV_5,
        sfialevels:PDSV_6 ;
    sfia:skillCategory categories:people_management ;
     skos:definition "Facilitating the professional development of individuals in line with their career goals and organisational requirements."@en ;
    skos:scopeNote """Activities may include, but are not limited to:

negotiating, reviewing, monitoring and validating each individual's professional development plans
providing professional development advice and support for individuals
identifying appropriate learning and development or career-enhancing activities
liaising with internal and external providers of learning and development
adopting a suitable framework for skills, knowledge and competencies such as SFIA
adopting or defining professional career pathways
creating accreditation and qualification approaches or adopting industry frameworks
evaluating the benefits of continual professional development activities."""@en ;
dcterms:source "https://sfia-online.org/en/skillcode/9/PDSV"^^xsd:anyURI .

skills:PEDP a sfia:Skill , skos:Concept ; 
 skos:inScheme skillcs: ;
    skos:prefLabel "Information and data compliance"@en ;
    skos:notation "PEDP" ;
    sfia:definedAtLevel sfialevels:PEDP_4,
        sfialevels:PEDP_5,
        sfialevels:PEDP_6 ;
    sfia:skillCategory categories:security_and_privacy ;
     skos:definition "Implementing and promoting compliance with information and data management legislation."@en ;
    skos:scopeNote """Includes legislation regulating the holding, use and disclosure of personal data.
Activities may include, but are not limited to:

providing expert advice on policies, procedures and governance
designing privacy-friendly products, services and systems that respect customer privacy and embed data protection
performing impact assessments, identify risks whilst enabling prudent use of data and addressing issues with products and services
responding to incidents
following legislative developments
creating risk models and frameworks
working with subject matter experts in areas such as, but not limited to, legal, public relations, learning and development, procurement, security, data management and architecture."""@en ;
dcterms:source "https://sfia-online.org/en/skillcode/9/PEDP"^^xsd:anyURI .

skills:PEMT a sfia:Skill , skos:Concept ; 
 skos:inScheme skillcs: ;
    skos:prefLabel "Performance management"@en ;
    skos:notation "PEMT" ;
    sfia:definedAtLevel sfialevels:PEMT_4,
        sfialevels:PEMT_5,
        sfialevels:PEMT_6 ;
    sfia:skillCategory categories:people_management ;
     skos:definition "Improving organisational performance by developing the performance of individuals and workgroups to meet agreed objectives with measurable results."@en ;
    skos:scopeNote """The term workgroup is used to be inclusive of different organisational structures. A workgroup is a collection of people working together on interdependent tasks to achieve shared objectives. This includes, but is not limited to, permanent/business-as-usual teams, cross-functional teams, squads or workgroups formed to deliver a specific outcome.
Activities may include, but are not limited to:

setting workgroup objectives aligned to organisational drivers
supporting individual growth to achieve objectives
forming effective teams
developing effective working relations within the workgroup
developing effective working relations with other workgroups, partners and individuals who they collaborate with to achieve workgroup objectives."""@en ;
dcterms:source "https://sfia-online.org/en/skillcode/9/PEMT"^^xsd:anyURI .

skills:PENT a sfia:Skill , skos:Concept ; 
 skos:inScheme skillcs: ;
    skos:prefLabel "Penetration testing"@en ;
    skos:notation "PENT" ;
    sfia:definedAtLevel sfialevels:PENT_2,
        sfialevels:PENT_3,
        sfialevels:PENT_4,
        sfialevels:PENT_5,
        sfialevels:PENT_6 ;
    sfia:skillCategory categories:security_services ;
     skos:definition "Testing the effectiveness of security controls by emulating the tools and techniques of likely attackers."@en ;
    skos:scopeNote """Penetration testing may be a stand-alone activity or an aspect of acceptance testing prior to an approval to operate.
Activities include, but are not limited to:

ethical hacking (using the same tools and techniques as an adversary to safely exploit security weaknesses)
demonstrating how an adversary can subvert security goals or achieve specific adversarial objectives
evaluating the effectiveness of current/planned defences or mitigation controls
assuring the security of networks, systems and applications
assessing the strength and effectiveness of cryptographic implementations
identifying insights into the business risks of various vulnerabilities
testing network, infrastructure, web and mobile applications for weaknesses
checking patch levels and configurations
social engineering."""@en ;
dcterms:source "https://sfia-online.org/en/skillcode/9/PENT"^^xsd:anyURI .

skills:PGMG a sfia:Skill , skos:Concept ; 
 skos:inScheme skillcs: ;
    skos:prefLabel "Programme management"@en ;
    skos:notation "PGMG" ;
    sfia:definedAtLevel sfialevels:PGMG_6,
        sfialevels:PGMG_7 ;
    sfia:skillCategory categories:change_implementation ;
     skos:definition "Identifying, planning and coordinating a set of related projects and activities in support of specific business strategies and objectives."@en ;
    skos:scopeNote """Activities may include, but are not limited to:

managing interdependencies in support of specific business strategies and objectives
maintaining a strategic view over the set of projects
providing the framework for implementing business initiatives, or large-scale change
implementing programme management practices to support iterative/agile working
ensuring programme activities adhere to organisational governance standards and practices
conceiving, maintaining and communicating a vision of the programme's outcomes and associated benefits
agreeing business requirements and translating requirements into operational plans
determining, monitoring and reviewing programme scope, costs, schedule and expected benefits
scheduling programme resources, inter-dependencies and programme risk."""@en ;
dcterms:source "https://sfia-online.org/en/skillcode/9/PGMG"^^xsd:anyURI .

skills:POMG a sfia:Skill , skos:Concept ; 
 skos:inScheme skillcs: ;
    skos:prefLabel "Portfolio management"@en ;
    skos:notation "POMG" ;
    sfia:definedAtLevel sfialevels:POMG_5,
        sfialevels:POMG_6,
        sfialevels:POMG_7 ;
    sfia:skillCategory categories:change_implementation ;
     skos:definition "Developing and applying a management framework to define and deliver a portfolio of programmes, projects and/or ongoing services."@en ;
    skos:scopeNote """Activities include, but are not limited to:

alignment of investment with specific business strategies and objectives
ensuring governance frameworks guide strategic investment appraisal and decision-making processes
assessment of cost, risk, inter-dependencies and impact on existing business activities
identifying issues with portfolio structure, cost, risk, inter-dependencies, impact on current business activities and the strategic benefits to be realised
implementing portfolio management practices that support iterative/agile working
measurement and objective evaluation of potential changes and the benefits to be realised
prioritisation of resource utilisation and changes to be implemented
regular review of portfolios
management of the service pipeline (proposed or in development), service catalogue (live or available for deployment) and retired services."""@en ;
dcterms:source "https://sfia-online.org/en/skillcode/9/POMG"^^xsd:anyURI .

skills:PORT a sfia:Skill , skos:Concept ; 
 skos:inScheme skillcs: ;
    skos:prefLabel "Software configuration"@en ;
    skos:notation "PORT" ;
    sfia:definedAtLevel sfialevels:PORT_2,
        sfialevels:PORT_3,
        sfialevels:PORT_4,
        sfialevels:PORT_5,
        sfialevels:PORT_6 ;
    sfia:skillCategory categories:systems_development ;
     skos:definition "Designing and deploying software product configurations into software environments or platforms."@en ;
    skos:scopeNote """This skill is typically applied to the design and deployment of configurations of large, complex software.
This includes, but is not limited to:

enterprise resource planning (ERP) and customer relationship management (CRM) software
server/mainframe operating systems
software as a service (SaaS) solutions
integration platforms/suites
tools provided by infrastructure as a service (IaaS) and platform as a service (PaaS) providers.

Activities may include, but are not limited to:

porting software configurations across different environments or platforms
refactoring complex or overlapping configurations across different software modules and capabilities
designing and implementing configurations that use architectures and services like microservices, serverless and containers
optimising configurations for performance, scalability and cost-efficiency
managing configurations across multiple environments and ensuring interoperability
applying infrastructure as code principles to automate configuration deployment and management.

Depending on requirements and the characteristics of the project or assigned work, software configuration methods and lifecycles can be predictive (plan-driven) approaches or adaptive (iterative/agile) approaches."""@en ;
dcterms:source "https://sfia-online.org/en/skillcode/9/PORT"^^xsd:anyURI .

skills:PRMG a sfia:Skill , skos:Concept ; 
 skos:inScheme skillcs: ;
    skos:prefLabel "Project management"@en ;
    skos:notation "PRMG" ;
    sfia:definedAtLevel sfialevels:PRMG_4,
        sfialevels:PRMG_5,
        sfialevels:PRMG_6,
        sfialevels:PRMG_7 ;
    sfia:skillCategory categories:change_implementation ;
     skos:definition "Delivering agreed project outcomes by aligning appropriate management techniques, collaboration, leadership and governance to specific project and organisational contexts."@en ;
    skos:scopeNote """This skill is applicable to all project management techniques and lifecycles - which can be on a continuum from predictive (plan-driven) approaches to adaptive (iterative/agile) approaches.
Activities may include, but are not limited to:

selecting techniques and lifecycle models based on the context of the project
ensuring project activities align with governance frameworks and organisational standards
establishing team structures and a collaborative working environment
communicating with stakeholders and maintaining awareness of business needs and priorities
using visual techniques for project tracking and reporting 
timeboxing and incremental deliveries 
defining deliverables, milestones and dependencies
applying change control and risk management processes
acquiring the necessary resources and skills
agreeing constraints of cost, timescales, quality and scope
reviewing experiences and learning from current and previous projects
ensuring projects are formally closed and reviewed.

An understanding of project size and complexity is helpful when applying the project management skill. Typical factors that influence project complexity include the complexity of resourcing, scale of organisational impact, use of new technologies, number of interdependences, stability of requirements, business implications and risks."""@en ;
dcterms:source "https://sfia-online.org/en/skillcode/9/PRMG"^^xsd:anyURI .

skills:PROD a sfia:Skill , skos:Concept ; 
 skos:inScheme skillcs: ;
    skos:prefLabel "Product management"@en ;
    skos:notation "PROD" ;
    sfia:definedAtLevel sfialevels:PROD_2,
        sfialevels:PROD_3,
        sfialevels:PROD_4,
        sfialevels:PROD_5,
        sfialevels:PROD_6 ;
    sfia:skillCategory categories:systems_development ;
     skos:definition "Managing and developing products or services throughout their full lifecycle, from inception through growth, maturity, and decline, to retirement."@en ;
    skos:scopeNote """Activities may include, but are not limited to:

using market and/or user research insights to inform product strategies
defining product vision, strategy and roadmaps aligned with organisational goals
developing and implementing pricing/charging strategies and tactics based on competitive analysis, cost analysis and customer insights
collaborating with cross-functional teams to develop, launch and manage products over their lifecycle
managing product lifecycle and continuously improving products based on data and feedback
monitoring product performance, market trends and competitor activities
applying product management principles to both internal and customer-facing products.

For customer-facing products (including government digital services and commercial products), focusing on measures such as customer needs, service quality, public sector objectives, revenue, profitability and cost recovery
For internal products, focusing on user needs, operational efficiency and business value
A product lifecycle typically moves from inception, growth, maturity, decline to retirement. The product development lifecycle model used will be based on the context of the work and may be selected from predictive (plan-driven) or adaptive (iterative/agile) approaches."""@en ;
dcterms:source "https://sfia-online.org/en/skillcode/9/PROD"^^xsd:anyURI .

skills:PROF a sfia:Skill , skos:Concept ; 
 skos:inScheme skillcs: ;
    skos:prefLabel "Portfolio, programme and project support"@en ;
    skos:notation "PROF" ;
    sfia:definedAtLevel sfialevels:PROF_2,
        sfialevels:PROF_3,
        sfialevels:PROF_4,
        sfialevels:PROF_5,
        sfialevels:PROF_6 ;
    sfia:skillCategory categories:change_implementation ;
     skos:definition "Providing support and guidance on portfolio, programme and project management processes, procedures, tools and techniques."@en ;
    skos:scopeNote """Activities may include, but are not limited to:

support the definition of portfolios, programmes and projects
cultivating and applying new or changed working practices across a portfolio
managing the rate at which new projects are started to fit the available capacity
advising on the development, production and maintenance of business cases time, resource, cost and exception plans
advising on the use of software tools
tracking and reporting progress and performance 
facilitating portfolio/programme/project meetings and workshops
advising and sharing knowledge on standards and how to comply."""@en ;
dcterms:source "https://sfia-online.org/en/skillcode/9/PROF"^^xsd:anyURI .

skills:PROG a sfia:Skill , skos:Concept ; 
 skos:inScheme skillcs: ;
    skos:prefLabel "Programming/software development"@en ;
    skos:notation "PROG" ;
    sfia:definedAtLevel sfialevels:PROG_2,
        sfialevels:PROG_3,
        sfialevels:PROG_4,
        sfialevels:PROG_5,
        sfialevels:PROG_6 ;
    sfia:skillCategory categories:systems_development ;
     skos:definition "Developing software components to deliver value to stakeholders."@en ;
    skos:scopeNote """Activities may include, but are not limited to:

identifying, creating and applying software development and security standards and processes
planning and designing software components
estimating time and effort required for software development
constructing, amending, and verifying software components, ensuring security is embedded
applying test-driven development and ensuring appropriate test coverage
using peer review techniques such as pair programming
documenting software components
understanding and obtaining agreement to the value of the software components to be developed
selecting appropriate development methods and lifecycles
applying recovery techniques to ensure the software being developed is not lost 
implementing appropriate change control to software development practices
resolving operational problems with software and fixing bugs

Depending on requirements and the characteristics of the project or assigned work, software development methods and lifecycles can be predictive (plan-driven) approaches or adaptive (iterative/agile) approaches."""@en ;
dcterms:source "https://sfia-online.org/en/skillcode/9/PROG"^^xsd:anyURI .

skills:PRTS a sfia:Skill , skos:Concept ; 
 skos:inScheme skillcs: ;
    skos:prefLabel "Process testing"@en ;
    skos:notation "PRTS" ;
    sfia:definedAtLevel sfialevels:PRTS_1,
        sfialevels:PRTS_2,
        sfialevels:PRTS_3,
        sfialevels:PRTS_4,
        sfialevels:PRTS_5,
        sfialevels:PRTS_6 ;
    sfia:skillCategory categories:systems_development ;
     skos:definition "Assessing documented and undocumented process flows within a product, system or service against business needs through investigation and testing."@en ;
    skos:scopeNote """Process testing focuses on ensuring systems effectively support business processes, deliver value and meet user needs.
It involves identifying and mitigating risks such as inefficient or error-prone processes, unsupported user roles, restricted user actions, system complexity, inconsistent data handling and non-compliance with business requirements.
Activities may include, but are not limited to:

collaborating with stakeholders to align testing with business requirements and objectives
designing test cases that cover entire business workflows, including business rules, alternate paths and exception scenarios
setting up test environments that simulate real-world conditions, user roles and data flows
preparing and managing test data to accurately support the scenarios being tested
executing manual and automated tests to validate workflows, ensuring systems operate correctly across scenarios
logging and reporting findings with an emphasis on business process impact, providing insights and recommendations
analysing results to identify inefficiencies and areas for system and process enhancement
promoting a shift-left approach by integrating process testing early in the lifecycle for early issue detection
developing and maintaining scalable automation frameworks
ensuring compliance with industry standards, regulations and recognised good practices."""@en ;
dcterms:source "https://sfia-online.org/en/skillcode/9/PRTS"^^xsd:anyURI .

skills:QUAS a sfia:Skill , skos:Concept ; 
 skos:inScheme skillcs: ;
    skos:prefLabel "Quality assurance"@en ;
    skos:notation "QUAS" ;
    sfia:definedAtLevel sfialevels:QUAS_2,
        sfialevels:QUAS_3,
        sfialevels:QUAS_4,
        sfialevels:QUAS_5,
        sfialevels:QUAS_6 ;
    sfia:skillCategory categories:governance__risk_and_compliance ;
     skos:definition "Assuring, through ongoing and periodic assessments and reviews, that the organisation's quality objectives are being met."@en ;
    skos:scopeNote """Quality assurance provides confidence to internal and external stakeholders that quality requirements will be fulfilled.
Quality assurance provides confidence to internal and external stakeholders that quality requirements will be fulfilled. It may relate to any area where quality standards are applied, including products, data, services and business processes.
Activities may include, but are not limited to:

planning and conducting quality assessments and quality audits
reviewing processes, products and services against defined quality criteria
identifying and reporting on quality issues and non-conformances
recommending corrective actions and improvements
verifying the implementation and effectiveness of corrective actions
promoting quality awareness throughout the organisation."""@en ;
dcterms:source "https://sfia-online.org/en/skillcode/9/QUAS"^^xsd:anyURI .

skills:QUMG a sfia:Skill , skos:Concept ; 
 skos:inScheme skillcs: ;
    skos:prefLabel "Quality management"@en ;
    skos:notation "QUMG" ;
    sfia:definedAtLevel sfialevels:QUMG_2,
        sfialevels:QUMG_3,
        sfialevels:QUMG_4,
        sfialevels:QUMG_5,
        sfialevels:QUMG_6,
        sfialevels:QUMG_7 ;
    sfia:skillCategory categories:governance__risk_and_compliance ;
     skos:definition "Defining and operating a management framework of processes and working practices to deliver the organisation's quality objectives."@en ;
    skos:scopeNote """Quality management involves defining and operating a management framework of processes and working practices to deliver the organisation's quality objectives. 
Activities may include, but are not limited to:

establishing a quality management system and promoting a quality culture
developing and maintaining quality standards and procedures
applying techniques for the monitoring and improving the quality of any aspect of a function, processes, products, services or data
providing advice on the application of appropriate quality management techniques
achieving and maintaining compliance with national and international standards and to internal policies
developing and implementing quality metrics and key performance indicators (KPIs)
facilitating continuous improvement initiatives
integrating quality management practices with other management systems (e.g., environmental, health and safety).

Internal or external standards are typically related to areas such as, but not limited to: quality, service, sustainability and security."""@en ;
dcterms:source "https://sfia-online.org/en/skillcode/9/QUMG"^^xsd:anyURI .

skills:RELM a sfia:Skill , skos:Concept ; 
 skos:inScheme skillcs: ;
    skos:prefLabel "Release management"@en ;
    skos:notation "RELM" ;
    sfia:definedAtLevel sfialevels:RELM_2,
        sfialevels:RELM_3,
        sfialevels:RELM_4,
        sfialevels:RELM_5,
        sfialevels:RELM_6 ;
    sfia:skillCategory categories:technology_management ;
     skos:definition "Managing the release of new and updated services into production, ensuring alignment with business objectives and compliance standards."@en ;
    skos:scopeNote """Activities may include, but are not limited to:

planning and scheduling releases in line with business requirements, considering the size, scope and content of each release
coordinating release activities across multiple teams and stakeholders, including third-party suppliers
managing the release lifecycle, including build, testing, deployment and post-implementation review
ensuring releases meet quality, security and compliance standards
communicating release plans, progress and outcomes to stakeholders
conducting post-release reviews and identifying areas for improvement
maintaining release processes, procedures and documentation
managing staged releases, pilot releases, blue/green releases or feature flags as appropriate."""@en ;
dcterms:source "https://sfia-online.org/en/skillcode/9/RELM"^^xsd:anyURI .

skills:REQM a sfia:Skill , skos:Concept ; 
 skos:inScheme skillcs: ;
    skos:prefLabel "Requirements definition and management"@en ;
    skos:notation "REQM" ;
    sfia:definedAtLevel sfialevels:REQM_2,
        sfialevels:REQM_3,
        sfialevels:REQM_4,
        sfialevels:REQM_5,
        sfialevels:REQM_6 ;
    sfia:skillCategory categories:change_analysis ;
     skos:definition "Managing requirements through the entire delivery and operational lifecycle."@en ;
    skos:scopeNote """Requirements may be related to software, systems, data, processes, products or services.
Activities may include, but are not limited to:

eliciting and analysing requirements, both functional and non-functional
ensuring customer requirements, priorities and acceptance criteria are accurately captured and validated
organising and prioritising requirements using techniques such as, but not limited to, product roadmaps, epics, user stories and backlogs
specifying and validating requirements, constraints and acceptance criteria to a level that enables effective development and operations of new or changed software, systems, processes, products or services
negotiating trade-offs that are acceptable to key stakeholders and within budgetary, technical, regulatory and other constraints
adopting and adapting requirements management lifecycle models.

The requirements lifecycle approach will be based on the context of the work and may be selected from predictive (plan-driven) or adaptive (iterative/agile) approaches."""@en ;
dcterms:source "https://sfia-online.org/en/skillcode/9/REQM"^^xsd:anyURI .

skills:RESC a sfia:Skill , skos:Concept ; 
 skos:inScheme skillcs: ;
    skos:prefLabel "Resourcing"@en ;
    skos:notation "RESC" ;
    sfia:definedAtLevel sfialevels:RESC_2,
        sfialevels:RESC_3,
        sfialevels:RESC_4,
        sfialevels:RESC_5,
        sfialevels:RESC_6 ;
    sfia:skillCategory categories:people_management ;
     skos:definition "Acquiring, deploying and onboarding resources."@en ;
    skos:scopeNote """Resources include, but are not limited to, salaried employees, temporary staff, consultants and contractors. Resourcing may be undertaken for departments, teams, projects, or individual roles. Resourcing should be attributed to those whose role is the specialised practice of acquiring and integrating resources into the organisation.
Activities may include, but are not limited to:

recruiting, selecting, deploying, onboarding and transitioning resources
assessing candidates using methods such as, but not limited to, interviews, assessment centres, CV/resume review, tests and exercises
ensuring compliance with relevant statutory or external regulations and codes of good practice
enhancing recruitment using workforce and process analytics
proactively building talent pipelines aligned to future strategic skills
adapting sourcing approaches to attract candidates for hard-to-fill needs
measuring the effectiveness of resourcing approaches using methods such as, but not limited to, retention analysis, media and supplier assessment, customer satisfaction and validation of selection methods."""@en ;
dcterms:source "https://sfia-online.org/en/skillcode/9/RESC"^^xsd:anyURI .

skills:RESD a sfia:Skill , skos:Concept ; 
 skos:inScheme skillcs: ;
    skos:prefLabel "Real-time/embedded systems development"@en ;
    skos:notation "RESD" ;
    sfia:definedAtLevel sfialevels:RESD_2,
        sfialevels:RESD_3,
        sfialevels:RESD_4,
        sfialevels:RESD_5,
        sfialevels:RESD_6 ;
    sfia:skillCategory categories:systems_development ;
     skos:definition "Designing and developing reliable real-time software typically within embedded systems."@en ;
    skos:scopeNote """Embedded systems provide dedicated functionality within a larger mechanical or electronic system, often with constraints related to real-time performance, safety, security, and reliability. These systems typically interface with hardware, sensors, and actuators, supporting critical operations in industrial, automotive, aerospace, medical, or robotic equipment, as well as in IoT (Internet of Things) devices and intelligent systems.
These systems usually perform essential functions and have strict requirements for integrity, reliability, safety, security, and power consumption.
Activities may include, but are not limited to:

defining non-functional system requirements such as performance, reliability, safety, and security, as well as constraints like power, cost, physical space, or response time
building in fail-safe or secure characteristics to support graceful degradation
applying specialised techniques to ensure systems meet their critical attributes
employing comprehensive methods for validation, verification, and testing
using virtual or model-based development approaches to simulate, test, and optimise systems throughout the development lifecycle
using specialised tools for real-time program and system analysis, validation, and debugging."""@en ;
dcterms:source "https://sfia-online.org/en/skillcode/9/RESD"^^xsd:anyURI .

skills:RFEN a sfia:Skill , skos:Concept ; 
 skos:inScheme skillcs: ;
    skos:prefLabel "Radio frequency engineering"@en ;
    skos:notation "RFEN" ;
    sfia:definedAtLevel sfialevels:RFEN_2,
        sfialevels:RFEN_3,
        sfialevels:RFEN_4,
        sfialevels:RFEN_5,
        sfialevels:RFEN_6 ;
    sfia:skillCategory categories:systems_development ;
     skos:definition "Designing, installing and maintaining radio frequency based devices and software."@en ;
    skos:scopeNote """Activities may include, but are not limited to:

evaluating and selecting devices and software
integrating radio frequency (RF) sub-systems into larger systems
calibrating, tuning and maintaining devices and software
receiving, transmitting and converting data between analogue and digital devices, in accordance with industry and regulatory standards
developing, integrating and configuring antennas, readers and transmitters in hardware or software forms, including software-defined radio (SDR), radio frequency identification (RFID), near field communication (NFC), Bluetooth and Wi-Fi
adhering to established safety, security and quality standards.

Applications of this skill include, but are not limited to:

wireless local area networks
wireless communication systems for voice, data and image, cellular radio systems, global positioning systems and military communications networks
navigation and sensor systems."""@en ;
dcterms:source "https://sfia-online.org/en/skillcode/9/RFEN"^^xsd:anyURI .

skills:RLMT a sfia:Skill , skos:Concept ; 
 skos:inScheme skillcs: ;
    skos:prefLabel "Stakeholder relationship management"@en ;
    skos:notation "RLMT" ;
    sfia:definedAtLevel sfialevels:RLMT_4,
        sfialevels:RLMT_5,
        sfialevels:RLMT_6,
        sfialevels:RLMT_7 ;
    sfia:skillCategory categories:stakeholder_management ;
     skos:definition "Systematically analysing, managing and influencing stakeholder relationships to achieve mutually beneficial outcomes through structured engagement."@en ;
    skos:scopeNote """Activities may include, but are not limited to:

identifying stakeholders and analysing the relationships
agreeing on mutually beneficial outcomes
managing, monitoring and improving stakeholder relationships 
determining the relationship management approach to take - including roles and responsibilities, governance, policies, processes, tools and support mechanisms
getting commitment to action through consultation and consideration of impacts
combining formal and informal communication channels to achieve the desired result
operational management of stakeholder relationships and communications.

The focus of this skill is a systematic and planned approach. This skill is not intended for general communication and developing productive working relationships. Those factors are described in SFIA's generic attributes and levels of responsibility."""@en ;
dcterms:source "https://sfia-online.org/en/skillcode/9/RLMT"^^xsd:anyURI .

skills:RMGT a sfia:Skill , skos:Concept ; 
 skos:inScheme skillcs: ;
    skos:prefLabel "Records management"@en ;
    skos:notation "RMGT" ;
    sfia:definedAtLevel sfialevels:RMGT_1,
        sfialevels:RMGT_2,
        sfialevels:RMGT_3,
        sfialevels:RMGT_4,
        sfialevels:RMGT_5 ;
    sfia:skillCategory categories:data_and_records_operations ;
     skos:definition "Planning, implementing and managing the full lifecycle of organisational records."@en ;
    skos:scopeNote """Specific laws and regulations may require organisations to maintain records of certain activities and transactions. Records are typically subject to specific lifecycle management activities that include retention, disposal requirements and potentially other controls.
Records are held in many forms including, but not limited to, digital documents, printed material, microfilm, e-mail, chats and may be generated by internal or external sources.
Activities may include, but are not limited to:

identifying, classifying, valuing, processing, storing, archiving, destroying information and records
capturing and maintaining evidence of and information about business activities and transactions in the form of records
implementing systems of cataloguing, metadata, indexing and classification standards and methods used to identify and organise records
ensuring compliance with legal obligations
management of records management systems
conducting searches for records to comply with internal or external requests"""@en ;
dcterms:source "https://sfia-online.org/en/skillcode/9/RMGT"^^xsd:anyURI .

skills:RSCH a sfia:Skill , skos:Concept ; 
 skos:inScheme skillcs: ;
    skos:prefLabel "Formal research"@en ;
    skos:notation "RSCH" ;
    sfia:definedAtLevel sfialevels:RSCH_2,
        sfialevels:RSCH_3,
        sfialevels:RSCH_4,
        sfialevels:RSCH_5,
        sfialevels:RSCH_6 ;
    sfia:skillCategory categories:strategy_and_planning ;
     skos:definition "Systematically creating new knowledge by data gathering, innovation, experimentation, evaluation and dissemination."@en ;
    skos:scopeNote """Activities may include, but are not limited to:

determining research goals and the methods by which the research will be conducted
actively participating in a community of researchers
communicating formally and informally through digital media, conferences, journals, books and seminars.

The Formal Research skill, as defined in SFIA, encompasses the systematic creation of new knowledge through rigorous methodologies, applicable across various sectors including, but not limited to, commercial research and development, academic institutions, governmental agencies, and non-profit organisations.
Because of its name, this skill can be confused with general search and investigation into a topic of interest. In most cases, general investigations are covered by responsibilities described by the SFIA generic attributes. Many of the SFIA professional skills also refer to investigation or similar activity."""@en ;
dcterms:source "https://sfia-online.org/en/skillcode/9/RSCH"^^xsd:anyURI .

skills:SALE a sfia:Skill , skos:Concept ; 
 skos:inScheme skillcs: ;
    skos:prefLabel "Selling"@en ;
    skos:notation "SALE" ;
    sfia:definedAtLevel sfialevels:SALE_3,
        sfialevels:SALE_4,
        sfialevels:SALE_5,
        sfialevels:SALE_6 ;
    sfia:skillCategory categories:sales_and_bid_management ;
     skos:definition "Finding prospective customers and working with them to identify needs, influence purchase decisions and enhance future business opportunities."@en ;
    skos:scopeNote """Activities may include, but are not limited to:

identifying, qualifying and prospecting sales leads through appropriate channels
developing customer interest by building rapport, understanding needs, and proposing solutions
preparing, executing and monitoring sales of products or services in external or internal markets
conducting value analysis, delivering presentations, and negotiating terms to close sales
collaborating with bid/proposal management teams to support sales efforts
managing and growing relationships with existing customers, including identifying upselling and cross-selling opportunities
conducting regular account reviews and needs assessments to ensure ongoing customer satisfaction."""@en ;
dcterms:source "https://sfia-online.org/en/skillcode/9/SALE"^^xsd:anyURI .

skills:SCAD a sfia:Skill , skos:Concept ; 
 skos:inScheme skillcs: ;
    skos:prefLabel "Security operations"@en ;
    skos:notation "SCAD" ;
    sfia:definedAtLevel sfialevels:SCAD_1,
        sfialevels:SCAD_2,
        sfialevels:SCAD_3,
        sfialevels:SCAD_4,
        sfialevels:SCAD_5,
        sfialevels:SCAD_6 ;
    sfia:skillCategory categories:security_services ;
     skos:definition "Manages and administers security measures, using tools and intelligence to protect assets, ensuring compliance and operational integrity."@en ;
    skos:scopeNote """Activities may include, but are not limited to:

providing advice and guidance on the implementation and enforcement of security controls across all technological environments, including on-premise, cloud-based and automated systems
using security tools such as Security Information and Event Management (SIEM), Intrusion Detection/Prevention Systems (IDS/IPS) and firewalls, alongside the use of automation to streamline security operations
acting on threat intelligence to proactively address potential security threats
conducting routine vulnerability assessments, monitoring and analysing relevant logs, alerts and events, and responding to incidents submitted via tickets or phone
performing rapid analysis and remediation of security issues
ensuring compliance with relevant legislation, adherence to security policies and maintaining standard security operating procedures
keeping accurate security records and documentation
implementing, managing and monitoring cryptographic and certificate management activities to protect data, ensure compliance and manage cryptographic keys securely
using advanced reporting techniques for comprehensive security oversight and informed decision-making."""@en ;
dcterms:source "https://sfia-online.org/en/skillcode/9/SCAD"^^xsd:anyURI .

skills:SCMG a sfia:Skill , skos:Concept ; 
 skos:inScheme skillcs: ;
    skos:prefLabel "Service catalogue management"@en ;
    skos:notation "SCMG" ;
    sfia:definedAtLevel sfialevels:SCMG_2,
        sfialevels:SCMG_3,
        sfialevels:SCMG_4,
        sfialevels:SCMG_5 ;
    sfia:skillCategory categories:service_management ;
     skos:definition "Providing a source of consistent information about available services and products to customers and users."@en ;
    skos:scopeNote """Activities may include, but are not limited to:

publishing and maintaining information about available services
tracking the list of available services as new services are introduced and current services are amended or retired
making the catalogue useful and easy to use
customising the information published for specific audiences, such as for users, for customers, for service providers
supporting discussion of standard and non-standard service offerings
enabling automation of service requests and service fulfilment where appropriate.

The information documented in the service catalogue includes, but is not limited to, service names and descriptions, features, value propositions, costs, service support levels and availability."""@en ;
dcterms:source "https://sfia-online.org/en/skillcode/9/SCMG"^^xsd:anyURI .

skills:SCMO a sfia:Skill , skos:Concept ; 
 skos:inScheme skillcs: ;
    skos:prefLabel "Scientific modelling"@en ;
    skos:notation "SCMO" ;
    sfia:definedAtLevel sfialevels:SCMO_4,
        sfialevels:SCMO_5,
        sfialevels:SCMO_6,
        sfialevels:SCMO_7 ;
    sfia:skillCategory categories:computational_science ;
     skos:definition "Applying computer simulation and other forms of computation to solve real-world problems in scientific disciplines."@en ;
    skos:scopeNote """Scientific modelling involves applying computer simulation and other forms of computation to solve real-world problems in scientific disciplines.
Activities may include, but are not limited to:

identifying relevant mathematical principles and scientific theory within a computational model
creating, testing and tuning scientific models through the application of computing
validating and interpreting computational models against the reality which the models attempt to represent
collaborating with domain experts to ensure models accurately represent scientific phenomena
communicating model results and implications to both technical and non-technical audiences
continuously refining models based on new data or scientific understanding
applying models to predict outcomes or test hypotheses in scientific research.

Scientific modelling is used across various fields, including physics, chemistry, biology, environmental science and social sciences, to simulate complex systems and processes."""@en ;
dcterms:source "https://sfia-online.org/en/skillcode/9/SCMO"^^xsd:anyURI .

skills:SCTY a sfia:Skill , skos:Concept ; 
 skos:inScheme skillcs: ;
    skos:prefLabel "Information security"@en ;
    skos:notation "SCTY" ;
    sfia:definedAtLevel sfialevels:SCTY_2,
        sfialevels:SCTY_3,
        sfialevels:SCTY_4,
        sfialevels:SCTY_5,
        sfialevels:SCTY_6,
        sfialevels:SCTY_7 ;
    sfia:skillCategory categories:security_and_privacy ;
     skos:definition "Defining and operating a framework of security controls and security management strategies."@en ;
    skos:scopeNote """Activities may include, but are not limited to:

selecting and adapting security frameworks to protect confidentiality, integrity, and availability of systems
implementing security controls, including physical, procedural, technical, and compliance measures
ensuring accountability and adherence to relevant laws and standards
embedding secure by design principles throughout the system's lifecycle, ensuring security is integrated from the earliest design stages, through development, deployment, and into operations
identifying and mitigating risks in infrastructure and applications.

Security controls include, but are not limited to:

physical controls - protecting tangible assets and physical environments
procedural or administrative controls - policies and guidelines governing organisational security practices
technical or logical controls - hardware and software measures that protect information systems
legal, regulatory or compliance controls - measures ensuring laws, regulations and industry standards.

These activities are typically performed in collaboration with specialists in other areas including, but not limited to: legal, technical infrastructure, audit, architecture and software engineering."""@en ;
dcterms:source "https://sfia-online.org/en/skillcode/9/SCTY"^^xsd:anyURI .

skills:SEAC a sfia:Skill , skos:Concept ; 
 skos:inScheme skillcs: ;
    skos:prefLabel "Service acceptance"@en ;
    skos:notation "SEAC" ;
    sfia:definedAtLevel sfialevels:SEAC_3,
        sfialevels:SEAC_4,
        sfialevels:SEAC_5,
        sfialevels:SEAC_6 ;
    sfia:skillCategory categories:service_management ;
     skos:definition "Managing the process to obtain formal confirmation that service acceptance criteria have been met."@en ;
    skos:scopeNote """Service acceptance criteria are used to ensure a service meets the defined service requirements, including functionality, operational support, performance, safety, security and quality requirements. Acceptance criteria include both utility/functional and warranty/non-functional tests.
Activities may include, but are not limited to:

defining and documenting service acceptance criteria
conducting service acceptance testing and evaluating test results against defined criteria
ensuring the service provider is ready to operate the new service when it has been deployed
providing feedback to service providers on necessary improvements
documenting and reporting on service acceptance outcomes
ensuring operational readiness for new or changed services
implementing service acceptance practices to support iterative/agile working
engaging with stakeholders to validate service readiness such as, but not limited to: external service providers, technical design, software development, DevOps and project management."""@en ;
dcterms:source "https://sfia-online.org/en/skillcode/9/SEAC"^^xsd:anyURI .

skills:SFAS a sfia:Skill , skos:Concept ; 
 skos:inScheme skillcs: ;
    skos:prefLabel "Safety assessment"@en ;
    skos:notation "SFAS" ;
    sfia:definedAtLevel sfialevels:SFAS_4,
        sfialevels:SFAS_5,
        sfialevels:SFAS_6 ;
    sfia:skillCategory categories:systems_development ;
     skos:definition "Assessing safety-related software and hardware systems to determine compliance with standards and required levels of safety integrity."@en ;
    skos:scopeNote """Activities may include, but are not limited to:

making professional judgements on software and hardware engineering approaches
assessing the suitability of design, testing and validation and verification methods
identifying and evaluating risks and how they can be reduced
establishing, maintaining and managing a safety assessment framework and practices
using techniques such as failure modes effects analysis, hazard and operability studies, component failure impact analysis, fault tree analysis, event tree analysis and criticality analysis."""@en ;
dcterms:source "https://sfia-online.org/en/skillcode/9/SFAS"^^xsd:anyURI .

skills:SFEN a sfia:Skill , skos:Concept ; 
 skos:inScheme skillcs: ;
    skos:prefLabel "Safety engineering"@en ;
    skos:notation "SFEN" ;
    sfia:definedAtLevel sfialevels:SFEN_2,
        sfialevels:SFEN_3,
        sfialevels:SFEN_4,
        sfialevels:SFEN_5,
        sfialevels:SFEN_6 ;
    sfia:skillCategory categories:systems_development ;
     skos:definition "Applying appropriate methods to assure safety during all lifecycle phases of safety-related systems developments."@en ;
    skos:scopeNote """Safety-critical systems are those in which a system failure could harm human life, other living things, physical structures, or the environment. 
Activities may include, but are not limited to:

safety hazard and risk analysis
safety requirements specification
safety-related systems architectural design
formal method design
safety validation and verification
safety case preparation
applying generic safety standards such as IEC 61508, IEC 61511 or industry-specific safety standards.

System safety is engineered and measured by safety levels based on hazard and risk analysis."""@en ;
dcterms:source "https://sfia-online.org/en/skillcode/9/SFEN"^^xsd:anyURI .

skills:SINT a sfia:Skill , skos:Concept ; 
 skos:inScheme skillcs: ;
    skos:prefLabel "Systems integration and build"@en ;
    skos:notation "SINT" ;
    sfia:definedAtLevel sfialevels:SINT_2,
        sfialevels:SINT_3,
        sfialevels:SINT_4,
        sfialevels:SINT_5,
        sfialevels:SINT_6 ;
    sfia:skillCategory categories:systems_development ;
     skos:definition "Planning, implementing and controlling activities to integrate system elements, subsystems and interfaces to create operational systems, products or services."@en ;
    skos:scopeNote """The scope of integration includes system elements, subsystems, interfaces and software components including computing, storage, networking and cloud services.
Systems integration is used to create systems for testing purposes as well as for operational use by customers and users.
Activities may include, but are not limited to:

developing organisational capabilities, processes and procedures for automation and continuous integration of build, packaging, testing, security and deployment
building and operating a continuous integration (CI) capability when required, employing version control of source code and related artefacts
ensuring security and privacy requirements are an essential part of systems integration and build
collaborating with development, testing and operations teams to streamline the integration process
testing, validation and sign off of integration to satisfy requirements, architectures and design
monitoring and controlling integration activities and recording and reporting on the results of integration
keeping stakeholders informed and providing feedback into risk management processes
developing and testing disaster recovery plans and applying incident management processes for major systems integrations."""@en ;
dcterms:source "https://sfia-online.org/en/skillcode/9/SINT"^^xsd:anyURI .

skills:SLEN a sfia:Skill , skos:Concept ; 
 skos:inScheme skillcs: ;
    skos:prefLabel "Systems and software lifecycle engineering"@en ;
    skos:notation "SLEN" ;
    sfia:definedAtLevel sfialevels:SLEN_3,
        sfialevels:SLEN_4,
        sfialevels:SLEN_5,
        sfialevels:SLEN_6,
        sfialevels:SLEN_7 ;
    sfia:skillCategory categories:systems_development ;
     skos:definition "Establishing and deploying an environment for developing, continually improving and securely operating software and systems products and services."@en ;
    skos:scopeNote """This skill involves interdisciplinary approaches to developing and operating software and systems across their entire lifecycle. Commonly associated with terms such as DevOps, DevSecOps, site reliability engineering, developer productivity engineering.
This skill extends beyond continuous improvement. It focuses on integrating technical practices and collaborative methods, automation and lifecycle processes essential for system reliability, security and operational excellence.
Activities include, but are not limited to:

establishing secure, reliable software lifecycle practices
developing a supporting framework of methods, tools, processes, procedures and skilled personnel
deploying this environment with teams responsible for developing and operating software and systems 
building repeatable, reliable capabilities through trial, feedback, learning and continual evolution
adapting practices to specific products and services
defining, controlling and improving lifecycle processes
incorporating risk management, quality, security, privacy and safety
maximising automation
establishing architecture and design principles to support lifecycle processes
focusing on mission, value and customer needs
cultivating a culture of collaboration, learning, adaptation and resilience
integrating industry frameworks to guide improvements."""@en ;
dcterms:source "https://sfia-online.org/en/skillcode/9/SLEN"^^xsd:anyURI .

skills:SLMO a sfia:Skill , skos:Concept ; 
 skos:inScheme skillcs: ;
    skos:prefLabel "Service level management"@en ;
    skos:notation "SLMO" ;
    sfia:definedAtLevel sfialevels:SLMO_2,
        sfialevels:SLMO_3,
        sfialevels:SLMO_4,
        sfialevels:SLMO_5,
        sfialevels:SLMO_6,
        sfialevels:SLMO_7 ;
    sfia:skillCategory categories:service_management ;
     skos:definition "Agreeing targets for service levels and assessing, monitoring and managing the delivery of services against the targets."@en ;
    skos:scopeNote """Activities may include, but are not limited to:

planning, implementation, control, review and audit of service provision, to meet customer business requirements
developing and managing both formal Service Level Agreements (SLAs) and less formal service expectations, depending on organisational needs and practices
negotiating, implementing and monitoring service level agreements or service expectations
managing operational facilities to provide the agreed levels of service
identifying opportunities to improve service delivery
implementing service level management practices to support cloud-based services
identifying future trends and their impact on service delivery, for example, technical, market, industrial, socioeconomic, legislative or sustainability targets."""@en ;
dcterms:source "https://sfia-online.org/en/skillcode/9/SLMO"^^xsd:anyURI .

skills:SORC a sfia:Skill , skos:Concept ; 
 skos:inScheme skillcs: ;
    skos:prefLabel "Sourcing"@en ;
    skos:notation "SORC" ;
    sfia:definedAtLevel sfialevels:SORC_2,
        sfialevels:SORC_3,
        sfialevels:SORC_4,
        sfialevels:SORC_5,
        sfialevels:SORC_6,
        sfialevels:SORC_7 ;
    sfia:skillCategory categories:stakeholder_management ;
     skos:definition "Managing, or providing advice on, the procurement or commissioning of products and services."@en ;
    skos:scopeNote """Activities may include, but are not limited to:

providing policies and standards for procurement
ensuring compliance with commercial governance, legislation and supplier-related information security requirements
implementing compliant procurement processes, taking full account of the issues and imperatives of both the commissioning and supplier sides
clarifying requirements for products and services
identifying, evaluating and selecting suppliers 
evaluating tenders
advising on build or buy criteria as part of strategic sourcing input
evaluating and purchasing cloud-based services
benchmarking supplier performance 
placing, monitoring and terminating contracts."""@en ;
dcterms:source "https://sfia-online.org/en/skillcode/9/SORC"^^xsd:anyURI .

skills:SSUP a sfia:Skill , skos:Concept ; 
 skos:inScheme skillcs: ;
    skos:prefLabel "Sales support"@en ;
    skos:notation "SSUP" ;
    sfia:definedAtLevel sfialevels:SSUP_1,
        sfialevels:SSUP_2,
        sfialevels:SSUP_3,
        sfialevels:SSUP_4,
        sfialevels:SSUP_5,
        sfialevels:SSUP_6 ;
    sfia:skillCategory categories:sales_and_bid_management ;
     skos:definition "Providing advice and support to the sales force, customers and sales partners."@en ;
    skos:scopeNote """Sales support can be delivered to a range of roles, such as, but not limited to, the sales force, sales agents, reseller/distributor staff and existing or prospective customers.
This skill includes the provision of technical advice and assistance either in support of customer development or sales activity or in fulfilment of sales obligations.
Activities may include, but are not limited to:

providing technical information about products and services
assisting in the preparation of sales proposals and presentations
conducting product demonstrations
responding to customer queries and providing solutions
supporting the sales team in understanding customer requirements
collaborating with other departments to resolve customer issues
maintaining customer relationship management (CRM) systems
assisting in post-sale support and customer onboarding."""@en ;
dcterms:source "https://sfia-online.org/en/skillcode/9/SSUP"^^xsd:anyURI .

skills:STMG a sfia:Skill , skos:Concept ; 
 skos:inScheme skillcs: ;
    skos:prefLabel "Storage management"@en ;
    skos:notation "STMG" ;
    sfia:definedAtLevel sfialevels:STMG_2,
        sfialevels:STMG_3,
        sfialevels:STMG_4,
        sfialevels:STMG_5,
        sfialevels:STMG_6 ;
    sfia:skillCategory categories:technology_management ;
     skos:definition "Provisioning, configuring and optimising on-premises and cloud-based storage solutions, ensuring data availability, security and alignment with business objectives."@en ;
    skos:scopeNote """Storage management encompasses managing various storage solutions, local or external storage such as direct access storage (DAS), network access storage (NAS), storage area networks (SAN) and cloud-based storage. 
It involves technologies and processes such as, but not limited to, virtualisation, replication, mirroring, security, compression, performance monitoring, automation and storage provisioning. 
Activities may include, but are not limited to:

backup, archiving and recovery of data
monitoring and optimising storage performance and capacity
resolving potential and actual storage-related issues
developing and maintaining tools and procedures for storage troubleshooting and analysis
evaluating, provisioning and testing new storage solutions, including cloud-based storage
managing storage in hybrid and multi-cloud environments
investigating emerging technologies for storage management
ensuring compliance with regulatory and security requirements
addressing business goals based on information value, data classification, recovery point and recovery time objectives."""@en ;
dcterms:source "https://sfia-online.org/en/skillcode/9/STMG"^^xsd:anyURI .

skills:STPL a sfia:Skill , skos:Concept ; 
 skos:inScheme skillcs: ;
    skos:prefLabel "Enterprise and business architecture"@en ;
    skos:notation "STPL" ;
    sfia:definedAtLevel sfialevels:STPL_5,
        sfialevels:STPL_6,
        sfialevels:STPL_7 ;
    sfia:skillCategory categories:strategy_and_planning ;
     skos:definition "Aligning an organisation's technology strategy with its business mission, strategy and processes and documenting this using architectural models."@en ;
    skos:scopeNote """Enterprise architecture is typically considered across four domains: business, data, applications and infrastructure technologies. It may also include information security or legal and regulatory compliance.
Activities may include, but are not limited to:

translating business strategies and objectives into an operating model
assessing current capabilities and identifying required changes to achieve objectives
developing and maintaining roadmaps to guide the transition from the current state to the future state
describing the interrelationships between people, organisation, services, processes, data, information, technology and the external environment
creating, iterating and maintaining architectural models and views that embody key principles for the organisation's future state and evolution
implementing enterprise architecture working practices to support and enable iterative/agile working
interpreting business goals and drivers
documenting and communicating constraints, standards and guiding principles necessary to define, assure and govern the required evolution
using architectural models and processes to facilitate changes in the organisation's structure, business processes, information or data, business systems and infrastructure
describing where and why the enterprise will benefit from cloud-based services."""@en ;
dcterms:source "https://sfia-online.org/en/skillcode/9/STPL"^^xsd:anyURI .

skills:SUBF a sfia:Skill , skos:Concept ; 
 skos:inScheme skillcs: ;
    skos:prefLabel "Subject formation"@en ;
    skos:notation "SUBF" ;
    sfia:definedAtLevel sfialevels:SUBF_4,
        sfialevels:SUBF_5,
        sfialevels:SUBF_6,
        sfialevels:SUBF_7 ;
    sfia:skillCategory categories:skills_management ;
     skos:definition "Specifying, designing and developing curricula within a structured and systematic education environment."@en ;
    skos:scopeNote """Subject formation focuses on:

developing curricula to support the development of understanding of the principles, approaches and practices that underpin specific topics and knowledge areas 
incorporating significant emerging technologies and techniques for which current students need to be prepared. 

The scope may include curricula for formal education or for independent examination bodies.
This skill is generic and can be applied to curriculum design and development for any topic or knowledge area. In the context of the SFIA framework, this includes:

the topics and knowledge areas that support any skills described in the SFIA framework
and the application of these topics and knowledge areas to other disciplines and practices.

In the context of computing and IT curricula, the topics addressed are typically:

common digital skills needed to safely benefit from, participate in and contribute to the digital world for everyday life and for work
fundamental and more advanced aspects of specific topics and knowledge areas including emerging technologies and new applications for existing technologies
the ideas of computational thinking and the application of computational concepts to everyday life and professional working practices."""@en ;
dcterms:source "https://sfia-online.org/en/skillcode/9/SUBF"^^xsd:anyURI .

skills:SUPP a sfia:Skill , skos:Concept ; 
 skos:inScheme skillcs: ;
    skos:prefLabel "Supplier management"@en ;
    skos:notation "SUPP" ;
    sfia:definedAtLevel sfialevels:SUPP_2,
        sfialevels:SUPP_3,
        sfialevels:SUPP_4,
        sfialevels:SUPP_5,
        sfialevels:SUPP_6,
        sfialevels:SUPP_7 ;
    sfia:skillCategory categories:stakeholder_management ;
     skos:definition "Aligning the organisation's supplier performance objectives and activities with sourcing strategies and plans, balancing costs, efficiencies and service quality."@en ;
    skos:scopeNote """Activities may include, but are not limited to:

establishing working relationships based on collaboration, trust and open communication
encouraging co-innovation and service improvement with suppliers
proactively engaging with suppliers for mutual benefit to resolve operational incidents, problems, unsatisfactory performance and other sources of conflict
implementing clear escalation paths for discussing and resolving issues
managing performance and risks across multiple suppliers (internal and external) using a set of agreed metrics
ensuring compliance to legislation
commercial governance and supply chain management
managing risks associated with security, continuity and integrity of supply
incorporating supplier management practices tailored to cloud-based services
implementing policies for selection of suppliers and bench-marking supplier performance."""@en ;
dcterms:source "https://sfia-online.org/en/skillcode/9/SUPP"^^xsd:anyURI .

skills:SUST a sfia:Skill , skos:Concept ; 
 skos:inScheme skillcs: ;
    skos:prefLabel "Sustainability"@en ;
    skos:notation "SUST" ;
    sfia:definedAtLevel sfialevels:SUST_4,
        sfialevels:SUST_5,
        sfialevels:SUST_6 ;
    sfia:skillCategory categories:strategy_and_planning ;
     skos:definition "Advising and leading sustainability initiatives to reduce environmental impact and ensure compliance with relevant standards and regulations."@en ;
    skos:scopeNote """Activities may include, but are not limited to:

developing policies, standards and guidelines to minimise the environmental impact of IT operations and assets.
providing advice on sustainability regulations and standards.
establishing and monitoring sustainability metrics and benchmarks.
promoting and communicating sustainability policies and programmes.
overseeing the implementation of sustainable practices in hardware, software, networks, storage, power supply, maintenance and asset disposal."""@en ;
dcterms:source "https://sfia-online.org/en/skillcode/9/SUST"^^xsd:anyURI .

skills:SWDN a sfia:Skill , skos:Concept ; 
 skos:inScheme skillcs: ;
    skos:prefLabel "Software design"@en ;
    skos:notation "SWDN" ;
    sfia:definedAtLevel sfialevels:SWDN_2,
        sfialevels:SWDN_3,
        sfialevels:SWDN_4,
        sfialevels:SWDN_5,
        sfialevels:SWDN_6 ;
    sfia:skillCategory categories:systems_development ;
     skos:definition "Architecting and designing software to meet specified requirements, ensuring adherence to established standards and principles."@en ;
    skos:scopeNote """Activities may include, but are not limited to:

designing and architecting software applications, components, interfaces and related characteristics (including security)
designing for scalability, performance, resilience, security and privacy from the outset, aligned with cloud computing, distributed systems and data protection
applying design concepts, patterns, modelling techniques and architectural styles such as microservices, serverless and domain-driven design to develop software designs and architectures, which serve as the foundation for software construction and verification
evaluating alternative solutions and trade-offs to facilitate design decisions
considering functional and non-functional requirements such as the target environment, performance, security, scalability and integration with existing systems
adopting and adapting software design models, tools and techniques based on the context of the work, including contemporary practices such as cloud-native architectures, edge computing, cyber-physical systems and agile and iterative design practices
developing prototypes/simulations to enable informed decision-making.

Unlike programming and designing at the code level, this skill focuses on higher-level design, addressing architecture and system-wide considerations."""@en ;
dcterms:source "https://sfia-online.org/en/skillcode/9/SWDN"^^xsd:anyURI .

skills:SYSP a sfia:Skill , skos:Concept ; 
 skos:inScheme skillcs: ;
    skos:prefLabel "System software administration"@en ;
    skos:notation "SYSP" ;
    sfia:definedAtLevel sfialevels:SYSP_2,
        sfialevels:SYSP_3,
        sfialevels:SYSP_4,
        sfialevels:SYSP_5 ;
    sfia:skillCategory categories:technology_management ;
     skos:definition "Installing, managing and maintaining operating systems, data management, office automation and utility software across various infrastructure environments."@en ;
    skos:scopeNote """System software encompasses a wide range of software components that support the functioning and management of technology infrastructure, including operating systems, infrastructure software, data management products, office automation products, middleware and utility software. It may run in cloud, virtual or physical hardware environments and enables applications to run effectively.
Activities may include, but are not limited to:

monitoring and optimising the performance of system software
developing and maintaining diagnostic tools and procedures for system software troubleshooting and performance analysis
resolving service problems with system software components
evaluating, provisioning and testing new system software, including cloud based solutions 
reviewing system software updates and upgrades
provisioning and testing system software updates and configurations
adhering to established safety, security and quality standards
managing system software in hybrid and multi-cloud environments."""@en ;
dcterms:source "https://sfia-online.org/en/skillcode/9/SYSP"^^xsd:anyURI .

skills:TEAC a sfia:Skill , skos:Concept ; 
 skos:inScheme skillcs: ;
    skos:prefLabel "Teaching"@en ;
    skos:notation "TEAC" ;
    sfia:definedAtLevel sfialevels:TEAC_2,
        sfialevels:TEAC_3,
        sfialevels:TEAC_4,
        sfialevels:TEAC_5,
        sfialevels:TEAC_6,
        sfialevels:TEAC_7 ;
    sfia:skillCategory categories:skills_management ;
     skos:definition "Delivering and assessing curricula in a structured and systematic education environment."@en ;
    skos:scopeNote """Teaching focuses on:

developing an understanding of the principles, approaches and practices that underpin a specified topic or knowledge area
the methods, techniques and practice of teaching (pedagogy).

This skill is generic and can be applied to the teaching of any topic or knowledge area. In the context of the SFIA framework, this includes:

the topics and knowledge areas supporting any of the skills described in the SFIA framework
and the application of these topics and knowledge areas to other disciplines and practices.

In the context of computing and IT curricula, the topics addressed are typically:

common digital skills needed to safely benefit from, participate in and contribute to the digital world for everyday life and work
fundamental and more advanced aspects of specific topics and knowledge areas including emerging technologies and new applications for existing technologies
the ideas of computational thinking and the application of computational concepts to everyday life and professional working practices."""@en ;
dcterms:source "https://sfia-online.org/en/skillcode/9/TEAC"^^xsd:anyURI .

skills:TECH a sfia:Skill , skos:Concept ; 
 skos:inScheme skillcs: ;
    skos:prefLabel "Specialist advice"@en ;
    skos:notation "TECH" ;
    sfia:definedAtLevel sfialevels:TECH_4,
        sfialevels:TECH_5,
        sfialevels:TECH_6 ;
    sfia:skillCategory categories:advice_and_guidance ;
     skos:definition "Providing authoritative, professional advice and direction in a specialist area."@en ;
    skos:scopeNote """This skill entails developing and using specialist knowledge to offer authoritative advice and direction, distinct from general guidance or troubleshooting.
Professional advice is the provision of expert, objective and evidence-based recommendations, guidance and solutions to address specific challenges or opportunities, drawing upon the advisor's in-depth knowledge, skills and experience. 
Expertise may cover a particular aspect of information or communications technology, digital practices, methodologies, or application areas and can extend to applying knowledge from other disciplines, such as legal, finance, public relations, ethics or human resources, to technology-related topics.
Activities include, but are not limited to:

research and analysis to stay current with the latest developments in the specialist area
providing subject matter expert advice and recommendations based on thorough understanding of the subject
collaborating with other specialists to ensure comprehensive and cohesive advice
clearly communicating complex information to non-experts
creating guidelines, standards and recommended practices related to the specialist area
providing mentorship and guidance to support the development of specialist knowledge within the organisation."""@en ;
dcterms:source "https://sfia-online.org/en/skillcode/9/TECH"^^xsd:anyURI .

skills:TEST a sfia:Skill , skos:Concept ; 
 skos:inScheme skillcs: ;
    skos:prefLabel "Functional testing"@en ;
    skos:notation "TEST" ;
    sfia:definedAtLevel sfialevels:TEST_1,
        sfialevels:TEST_2,
        sfialevels:TEST_3,
        sfialevels:TEST_4,
        sfialevels:TEST_5,
        sfialevels:TEST_6 ;
    sfia:skillCategory categories:systems_development ;
     skos:definition "Assessing specified or unspecified functional requirements and characteristics of products, systems and services through investigation and testing."@en ;
    skos:scopeNote """Functional testing verifies that systems, components and interfaces deliver specific functionality, operate as intended and meet user expectations. Risk-based test planning and execution is a key aspect, focusing on identifying and mitigating risks such as functionality errors, integration failures, edge case defects, data inconsistencies and non-compliance with requirements.
Activities may include, but are not limited to:

collaborating with stakeholders to align testing with business requirements and objectives
designing and adapting test cases based on requirements, including various scenarios, boundary values and edge cases
preparing data and configuring environments to simulate realistic use cases
executing tests to verify actual results align with expected outcomes
logging defects with detailed reproduction steps, prioritising issues and providing feedback for improvements
analysing results to identify patterns, assess quality and suggest system/testing enhancements
promoting a shift-left approach by integrating functional testing early in the lifecycle for early issue detection
managing, executing and automating tests, including regression and smoke tests, to improve efficiency and coverage
developing and maintaining scalable, reliable automated tests and frameworks to validate critical functionality and ensure continuous quality
ensuring compliance with industry standards, regulations and recognised good practices."""@en ;
dcterms:source "https://sfia-online.org/en/skillcode/9/TEST"^^xsd:anyURI .

skills:THIN a sfia:Skill , skos:Concept ; 
 skos:inScheme skillcs: ;
    skos:prefLabel "Threat intelligence"@en ;
    skos:notation "THIN" ;
    sfia:definedAtLevel sfialevels:THIN_2,
        sfialevels:THIN_3,
        sfialevels:THIN_4,
        sfialevels:THIN_5,
        sfialevels:THIN_6 ;
    sfia:skillCategory categories:security_and_privacy ;
     skos:definition "Developing and sharing actionable insights on current and potential security threats to the success or integrity of an organisation."@en ;
    skos:scopeNote """Activities may include, but are not limited to:

gathering data from a variety of open or proprietary intelligence sources
processing and classifying threat data to make it useful and actionable by others
packaging the data for use by consumers of the information
enabling the use of the data automatically by security tools
providing threat intelligence to help others mitigate vulnerabilities or to respond to security incidents
collaborating with internal teams and external partners to enhance threat detection capabilities
analysing trends in cyber threats to predict future attack vectors
developing threat intelligence frameworks and methodologies."""@en ;
dcterms:source "https://sfia-online.org/en/skillcode/9/THIN"^^xsd:anyURI .

skills:TMCR a sfia:Skill , skos:Concept ; 
 skos:inScheme skillcs: ;
    skos:prefLabel "Learning design and development"@en ;
    skos:notation "TMCR" ;
    sfia:definedAtLevel sfialevels:TMCR_2,
        sfialevels:TMCR_3,
        sfialevels:TMCR_4,
        sfialevels:TMCR_5 ;
    sfia:skillCategory categories:skills_management ;
     skos:definition "Designing and developing resources to transfer knowledge, develop skills and change behaviours."@en ;
    skos:scopeNote """Includes instructional design, content development, configuration and testing of learning environments, and use of appropriate current technologies such as audio, video, simulation and assessment.
Scope includes learning and development activities for the workplace, for all levels of education and blended models such as apprenticeships and work placements.
Activities may include, but are not limited to:

specifying, designing, creating, packaging and maintaining materials and resources
assimilating information from existing sources
selecting and presenting material in a form suitable to the intended purpose and audience
securing third-party accreditation
creating simulated data and replicating external systems, interfaces, and assessment systems to support simulated learning environments."""@en ;
dcterms:source "https://sfia-online.org/en/skillcode/9/TMCR"^^xsd:anyURI .

skills:UNAN a sfia:Skill , skos:Concept ; 
 skos:inScheme skillcs: ;
    skos:prefLabel "User experience analysis"@en ;
    skos:notation "UNAN" ;
    sfia:definedAtLevel sfialevels:UNAN_2,
        sfialevels:UNAN_3,
        sfialevels:UNAN_4,
        sfialevels:UNAN_5 ;
    sfia:skillCategory categories:user_centred_design ;
     skos:definition "Understanding the context of use for systems, products and services and specifying user experience requirements and design goals."@en ;
    skos:scopeNote """This skill is inclusive of a full range of user tasks not just digital tasks. The skill can be applied in various contexts, such as: customer experience, products, services, applications, devices, learning experience and employee experience.
Activities may include, but are not limited to:

identifying, analysing, clarifying and communicating the context in which the product or service will be used
describing users' goals, tasks and the environment within which the systems, products, services or devices will be used
creating and describing personas to represent key user segments
developing user stories or requirements to describe features or capabilities 
agreeing user experience design goals
analysing and prioritising user experience needs with stakeholders
understanding and specifying user experience and user accessibility requirements for all potential users."""@en ;
dcterms:source "https://sfia-online.org/en/skillcode/9/UNAN"^^xsd:anyURI .

skills:URCH a sfia:Skill , skos:Concept ; 
 skos:inScheme skillcs: ;
    skos:prefLabel "User research"@en ;
    skos:notation "URCH" ;
    sfia:definedAtLevel sfialevels:URCH_2,
        sfialevels:URCH_3,
        sfialevels:URCH_4,
        sfialevels:URCH_5,
        sfialevels:URCH_6 ;
    sfia:skillCategory categories:user_centred_design ;
     skos:definition "Identifying users' behaviours, needs and motivations using observational research methods."@en ;
    skos:scopeNote """This skill is inclusive of a full range of user tasks not just digital tasks. The skill can be applied in various contexts, such as, but not limited to customer experience, products, services, applications, devices, learning experience and employee experience.
User research has a different set of responsibilities to academic research or user requirements elicitation. User research incorporates significant involvement of users to generate deep understanding and uncover new opportunities for systems, products, services or devices. 
Activities may include, but are not limited to: 

using ethnography, observation techniques, task analysis and other methodologies that incorporate both the social and technological context
quantifying different user populations and their needs
identifying target users and segments to maximise the chances of design success for systems, products, services or devices
analysing and synthesising research data to generate actionable insights
communicating research findings effectively to various stakeholders
including a range of users in research activities to capture the diversity of users' behaviours, needs and motivations."""@en ;
dcterms:source "https://sfia-online.org/en/skillcode/9/URCH"^^xsd:anyURI .

skills:USEV a sfia:Skill , skos:Concept ; 
 skos:inScheme skillcs: ;
    skos:prefLabel "User experience evaluation"@en ;
    skos:notation "USEV" ;
    sfia:definedAtLevel sfialevels:USEV_2,
        sfialevels:USEV_3,
        sfialevels:USEV_4,
        sfialevels:USEV_5,
        sfialevels:USEV_6 ;
    sfia:skillCategory categories:user_centred_design ;
     skos:definition "Validating systems, products or services against user experience goals, metrics and targets."@en ;
    skos:scopeNote """This skill is inclusive of a full range of user tasks not just digital tasks. The skill can be applied in various contexts, such as, but not limited to customer experience, products, services, applications, devices, learning experience and employee experience.
Evaluation is typically part of an iterative user experience design process and contributes to the improvement of the product or service. An evaluation can also be the starting point if an existing system, product or service is to be replaced or improved. Methods include user trials, expert review, survey and analysis.
Activities may include, but are not limited to:

providing assurance that user stories or requirements have been met and required practice has been followed to address accessibility, usability, security, health and safety
applying a range of qualitative and quantitative evaluation techniques
selecting from lightweight/rapid techniques or more thorough and resource-intensive approaches
selecting appropriate use of formative or summative evaluations
facilitating both moderated and unmoderated tests."""@en ;
dcterms:source "https://sfia-online.org/en/skillcode/9/USEV"^^xsd:anyURI .

skills:USUP a sfia:Skill , skos:Concept ; 
 skos:inScheme skillcs: ;
    skos:prefLabel "Incident management"@en ;
    skos:notation "USUP" ;
    sfia:definedAtLevel sfialevels:USUP_1,
        sfialevels:USUP_2,
        sfialevels:USUP_3,
        sfialevels:USUP_4,
        sfialevels:USUP_5,
        sfialevels:USUP_6 ;
    sfia:skillCategory categories:service_management ;
     skos:definition "Coordinating responses to a diverse range of incidents to minimise negative impacts and quickly restore services."@en ;
    skos:scopeNote """Activities may include, but are not limited to:

designing and implementing different processes and procedures for different categories of incidents including, but not limited to, major incidents, information or cybersecurity incidents, complex incidents and low impact incidents
establishing incident response teams or security incident response teams
enhancing preparedness through regular testing, training, simulations and development of incident response plans and playbooks
restoring service to users as quickly as possible, prioritising service continuity over permanent solutions
managing unplanned interruptions to a service or reductions in service quality
routing requests for help to appropriate functions for resolution
monitoring resolution activity
ensuring compliance with regulations and data privacy requirements 
using automation and data-driven tools for earlier and faster incident detection and resolution
informing users, customers and key stakeholders of progress towards service restoration.

Incidents can impact areas such as business operations, information and cyber security, IT systems, services, employees, customers, or other vital business functions.
Different roles or groups may be needed to diagnose and resolve incidents. These can include users, subject matter experts, service desk staff, support teams, suppliers, and partners. Although they participate in the incident management process, they do not necessarily require incident management skills."""@en ;
dcterms:source "https://sfia-online.org/en/skillcode/9/USUP"^^xsd:anyURI .

skills:VISL a sfia:Skill , skos:Concept ; 
 skos:inScheme skillcs: ;
    skos:prefLabel "Data visualisation"@en ;
    skos:notation "VISL" ;
    sfia:definedAtLevel sfialevels:VISL_2,
        sfialevels:VISL_3,
        sfialevels:VISL_4,
        sfialevels:VISL_5 ;
    sfia:skillCategory categories:data_and_analytics ;
     skos:definition "Facilitating understanding of data by displaying concepts, ideas and facts using graphical representations."@en ;
    skos:scopeNote """Activities may include, but are not limited to:

condensing and encapsulating data characteristics, making it easier to surface opportunities, identify risks, analyse trends and drive effective decision-making
presenting findings and data insights in creative ways to facilitate the understanding of data across a range of technical and non-technical audiences
developing narratives and storytelling around data to enhance understanding and support decision-making.

The skill is typically put into practice by using specialist analytics tools. Specialisation in this skill implies a requirement to use more than just standard office software to create graphical representations of simple data."""@en ;
dcterms:source "https://sfia-online.org/en/skillcode/9/VISL"^^xsd:anyURI .

skills:VUAS a sfia:Skill , skos:Concept ; 
 skos:inScheme skillcs: ;
    skos:prefLabel "Vulnerability assessment"@en ;
    skos:notation "VUAS" ;
    sfia:definedAtLevel sfialevels:VUAS_2,
        sfialevels:VUAS_3,
        sfialevels:VUAS_4,
        sfialevels:VUAS_5 ;
    sfia:skillCategory categories:security_services ;
     skos:definition "Identifying and classifying security vulnerabilities in networks, systems and applications and mitigating or eliminating their impact."@en ;
    skos:scopeNote """Activities may include, but are not limited to:

cataloguing and classifying information and technology resources (assets and capabilities) to support vulnerability assessment
assigning quantifiable value, rank order and importance to information and technology resources
identifying and analysing the vulnerabilities of each resource, manually or using automated tools and information sources
prioritising, scoring and ranking the risk associated with vulnerabilities
business impact assessment
mitigating or eliminating the vulnerabilities.

Vulnerability assessment tools include web application scanners, protocol scanners and network scanners."""@en ;
dcterms:source "https://sfia-online.org/en/skillcode/9/VUAS"^^xsd:anyURI .

skills:VURE a sfia:Skill , skos:Concept ; 
 skos:inScheme skillcs: ;
    skos:prefLabel "Vulnerability research"@en ;
    skos:notation "VURE" ;
    sfia:definedAtLevel sfialevels:VURE_2,
        sfialevels:VURE_3,
        sfialevels:VURE_4,
        sfialevels:VURE_5,
        sfialevels:VURE_6 ;
    sfia:skillCategory categories:security_and_privacy ;
     skos:definition "Conducting applied research to discover, evaluate and mitigate new or unknown security vulnerabilities and weaknesses."@en ;
    skos:scopeNote """A security vulnerability is a weakness, flaw or error found within a security system that has the potential to be leveraged by an external agent to compromise a secure system.
Activities may include, but are not limited to:

researching new threats, attack vectors, risks and potential solutions
researching new or emerging cryptographic vulnerabilities 
reverse engineering hardware or software 
applying tools such as disassemblers, debuggers and fuzzers 
analysing embedded devices
developing techniques and tools to analyse and expose vulnerabilities
designing new vulnerability discovery techniques
sharing mitigation techniques with relevant stakeholders."""@en ;
dcterms:source "https://sfia-online.org/en/skillcode/9/VURE"^^xsd:anyURI .

skills:WFPL a sfia:Skill , skos:Concept ; 
 skos:inScheme skillcs: ;
    skos:prefLabel "Workforce planning"@en ;
    skos:notation "WFPL" ;
    sfia:definedAtLevel sfialevels:WFPL_4,
        sfialevels:WFPL_5,
        sfialevels:WFPL_6 ;
    sfia:skillCategory categories:people_management ;
     skos:definition "Strategically projecting the demand for people and skills and proactively planning the workforce supply to meet organisational needs."@en ;
    skos:scopeNote """Workforce planning typically takes an enterprise-wide view, assessing capabilities across the organisation rather than just a single team. The scope is more strategic than tactical resource allocation to projects or operational work schedules.
Activities may include, but are not limited to:

assessing the current state of the workforce
assessing organisation-wide data over extended time periods to discover multi-year trends
identifying critical capabilities needed to compete and meet strategic goals, not just immediate resource allocation gaps
identifying the workforce required for current and future activities 
adopting or developing a skills and capabilities framework
developing plans to close gaps between current state and future state using actions such as, but not limited to: external recruitment, internal development, re-skilling, sourcing external partners, organisational design or outplacement 
influencing organisational policies and practices to align recruitment, learning, promotion, and recognition and reward to support the development of an inclusive and diverse workforce 
adhering to relevant regulations and ethical standards concerning employment practices and organisational policies, including requirements related to layoffs and restructuring."""@en ;
dcterms:source "https://sfia-online.org/en/skillcode/9/WFPL"^^xsd:anyURI .

sfialevels:ACIN_2 a sfia:SkillLevel ;
    skos:notation "ACIN_2" ;
    sfia:level lor:2 ;
    sfia:skillLevelDescription """Assists with basic accessibility testing and gathering information for accessibility reviews. 
Supports team members in executing predefined accessibility tests. 
Documents test results and contributes to accessibility audit reports."""@en .

sfialevels:ACIN_3 a sfia:SkillLevel ;
    skos:notation "ACIN_3" ;
    sfia:level lor:3 ;
    sfia:skillLevelDescription """Analyses accessibility requirements and technical information. 
Designs and executes accessibility tests under direction. Reports findings in a structured way and makes initial recommendations for compliance. 
Supports accessibility reviews and audits.
Escalates complex issues to senior colleagues."""@en .

sfialevels:ACIN_4 a sfia:SkillLevel ;
    skos:notation "ACIN_4" ;
    sfia:level lor:4 ;
    sfia:skillLevelDescription """Engages with stakeholders to explain accessibility factors. Influences designs to improve accessibility. 
Provides detailed accessibility analysis to inform decisions throughout the product or service lifecycle.
Plans and manages accessibility testing to meet agreed standards. 
Evaluates compliance with accessibility regulations. Assesses risks based on test outcomes."""@en .

sfialevels:ACIN_5 a sfia:SkillLevel ;
    skos:notation "ACIN_5" ;
    sfia:level lor:5 ;
    sfia:skillLevelDescription """Leads accessibility governance and assurance activities. 
Interprets complex systems to identify opportunities for improved accessibility. Provides expert advice to drive accessibility compliance across products, services and projects. 
Defines organisational accessibility testing approaches, aligned with regulations and standards. 
Promotes awareness of accessibility and inclusion principles."""@en .

sfialevels:ACIN_6 a sfia:SkillLevel ;
    skos:notation "ACIN_6" ;
    sfia:level lor:6 ;
    sfia:skillLevelDescription """Sets the organisation's strategic direction for accessibility and inclusion in products and services. 
Defines and oversees governance processes to ensure compliance. Leads the development of accessibility policies, standards and guidelines. 
Engages with industry bodies and experts to develop and implement good working practices.
Drives a culture of proactive accessibility consideration in design and development. Ensures adequate resources and skills for accessibility assurance."""@en .

sfialevels:ADEV_2 a sfia:SkillLevel ;
    skos:notation "ADEV_2" ;
    sfia:level lor:2 ;
    sfia:skillLevelDescription """Assists in the creation of basic visual and audio components for animations under routine supervision. 
Follows established procedures and guidelines and contributes to the development of simple animations using standard tools. 
Helps create and maintain documentation."""@en .

sfialevels:ADEV_3 a sfia:SkillLevel ;
    skos:notation "ADEV_3" ;
    sfia:level lor:3 ;
    sfia:skillLevelDescription """Builds visual and audio components using animation software. 
Uses design tools to evolve rapid prototypes of interactive systems and user interfaces.
Uses visual design tools and organic modelling techniques to create and animate virtual characters within a game or system design."""@en .

sfialevels:ADEV_4 a sfia:SkillLevel ;
    skos:notation "ADEV_4" ;
    sfia:level lor:4 ;
    sfia:skillLevelDescription """Builds visual and audio components and integrates them into the system structure.
Uses design tools to evolve rapid prototypes and assess the viability of design concepts for interactive systems and user interfaces. 
Uses complex visual design tools and organic modelling techniques to create and animate virtual characters within a game or system design."""@en .

sfialevels:ADEV_5 a sfia:SkillLevel ;
    skos:notation "ADEV_5" ;
    sfia:level lor:5 ;
    sfia:skillLevelDescription """Manages iterations of level design and storytelling, documenting the overall flow and architecture of a game or similar system. 
Develops conceptual structures into design blueprints to create high-level structures and runtime architectures for websites and virtual environments.
Oversees the integration of animations with game logic, physics and artificial intelligence systems."""@en .

sfialevels:ADEV_6 a sfia:SkillLevel ;
    skos:notation "ADEV_6" ;
    sfia:level lor:6 ;
    sfia:skillLevelDescription """Provides overall creative direction in the conception and design of animation products such as games and simulations.
Establishes animation development strategies, pipelines and quality assurance processes. 
Adapts or develops new methods and organisational capabilities and drives adoption of, and adherence to, policies and standards."""@en .

sfialevels:ADMN_1 a sfia:SkillLevel ;
    skos:notation "ADMN_1" ;
    sfia:level lor:1 ;
    sfia:skillLevelDescription """Performs routine administrative tasks in a structured environment. 
Follows clear procedures. Uses common office software and equipment. 
Organises and maintains information following agreed procedures.
Assists with basic coordination activities."""@en .

sfialevels:ADMN_2 a sfia:SkillLevel ;
    skos:notation "ADMN_2" ;
    sfia:level lor:2 ;
    sfia:skillLevelDescription """Assists with administrative tasks for a team. 
Maintains systems for organising information and documents. 
Coordinates team activities and acts as a point of contact for internal and external contacts.
Uses relevant digital tools and platforms."""@en .

sfialevels:ADMN_3 a sfia:SkillLevel ;
    skos:notation "ADMN_3" ;
    sfia:level lor:3 ;
    sfia:skillLevelDescription """Provides administrative support function to teams and meetings.
Takes an active part in team discussions. 
Sets up and maintains systems for organising information and documents. Compiles and distributes reports. 
Provides guidance on administrative software, procedures, processes, tools and techniques."""@en .

sfialevels:ADMN_4 a sfia:SkillLevel ;
    skos:notation "ADMN_4" ;
    sfia:level lor:4 ;
    sfia:skillLevelDescription """Assists the teams and managers in ensuring they have the information and resources needed to support ongoing processes. 
Assists in planning for meetings. Liaises and organises across functions. 
Sets up and provides detailed guidance on software, procedures, processes, tools and techniques for administration and workplace productivity.
Contributes to the development and maintenance of organisational policies, procedures and documentation."""@en .

sfialevels:ADMN_5 a sfia:SkillLevel ;
    skos:notation "ADMN_5" ;
    sfia:level lor:5 ;
    sfia:skillLevelDescription """Manages the delivery of business administration services. 
Manages and prioritises the schedules and communication of senior managers and leadership teams to ensure efficient use of time and resources.
Handles sensitive, confidential information. 
Ensures managers have the information and resources needed to support ongoing processes and changes in processes."""@en .

sfialevels:ADMN_6 a sfia:SkillLevel ;
    skos:notation "ADMN_6" ;
    sfia:level lor:6 ;
    sfia:skillLevelDescription """Leads and coordinates strategic initiatives working across departmental or functional boundaries. 
Designs, plans and coordinates high-level meetings and events, ensuring alignment with strategic objectives and desired outcomes.
Provides direction and receives progress updates from members of an executive team. Meets collectively or individually with members of a leadership management team to follow up on action points, issues and risks. Reports on progress and resolves issues. 
Manages highly sensitive and confidential issues and information."""@en .

sfialevels:AIDE_3 a sfia:SkillLevel ;
    skos:notation "AIDE_3" ;
    sfia:level lor:3 ;
    sfia:skillLevelDescription """Supports ethical reviews and conducts basic impact assessments under direction. 
Gathers and analyses information for assessments. Reports on ethical issues and compliance with guidance from others. Documents findings from audits and reviews. 
Assists with documentation and communication of ethical policies.  
Supports others in responding to incidents."""@en .

sfialevels:AIDE_4 a sfia:SkillLevel ;
    skos:notation "AIDE_4" ;
    sfia:level lor:4 ;
    sfia:skillLevelDescription """Engages stakeholders to communicate ethical considerations and influence design decisions. 
Conducts detailed impact assessments and makes recommendations. Manages ethical reviews to ensure compliance with standards. 
Evaluates risks and proposes measures to address ethical concerns. Leads discussions with stakeholders on ethical issues. 
Designs and executes ethical impact assessments. Prepares reports based on audit findings."""@en .

sfialevels:AIDE_5 a sfia:SkillLevel ;
    skos:notation "AIDE_5" ;
    sfia:level lor:5 ;
    sfia:skillLevelDescription """Provides expert advice to integrate ethics into AI and data projects and programmes. 
Oversees governance and assurance activities. Reviews and approves impact assessments and audits. 
Promotes awareness of ethical principles and their application across the organisation. 
Contributes to the development of policy, standards and guidelines related to AI and data ethics."""@en .

sfialevels:AIDE_6 a sfia:SkillLevel ;
    skos:notation "AIDE_6" ;
    sfia:level lor:6 ;
    sfia:skillLevelDescription """Sets direction for ethics in AI and data initiatives. Defines governance processes to ensure compliance with ethical standards. 
Engages with industry bodies and experts to develop and drive industry recommended practices. 
Develops and implements strategic ethical frameworks. Leads high-level reviews and decision-making processes. 
Allocates resources to support the organisation's commitment to ethical practices. Ensures the organisation has resources and skills for ethical assurance."""@en .

sfialevels:ANCC_2 a sfia:SkillLevel ;
    skos:notation "ANCC_2" ;
    sfia:level lor:2 ;
    sfia:skillLevelDescription """Accurately assigns classifications/labels to low complexity information under supervision. 
Understands and applies relevant classification/labelling systems, standards and guidelines. 
Participates in quality assurance activities such as peer review or supervisor checks."""@en .

sfialevels:ANCC_3 a sfia:SkillLevel ;
    skos:notation "ANCC_3" ;
    sfia:level lor:3 ;
    sfia:skillLevelDescription """Independently assigns accurate classifications/labels to a broad range of information. 
Interprets complex information and chooses appropriate classifications/labels. 
Participates in team quality improvement initiatives. 
Advises and guides others on classification/labelling practices."""@en .

sfialevels:ANCC_4 a sfia:SkillLevel ;
    skos:notation "ANCC_4" ;
    sfia:level lor:4 ;
    sfia:skillLevelDescription """Assigns classifications/labels to highly complex information. 
Performs quality assurance checks on the work of others. Investigates and corrects complex classification/labelling errors. 
Delivers training to team members. 
Contributes to the development of classification/labelling processes and guidelines."""@en .

sfialevels:ANCC_5 a sfia:SkillLevel ;
    skos:notation "ANCC_5" ;
    sfia:level lor:5 ;
    sfia:skillLevelDescription """Leads team quality assurance and training for information classification/labelling. 
Develops and implements audit methodologies for assessing classification and labelling accuracy and consistency.
Collaborates with subject matter experts to improve source information quality. Analyses and reports on classification/labelling quality. 
Contributes to organisational information classification/labelling strategy."""@en .

sfialevels:ANCC_6 a sfia:SkillLevel ;
    skos:notation "ANCC_6" ;
    sfia:level lor:6 ;
    sfia:skillLevelDescription """Sets organisational information classification/labelling standards, policies and procedures. 
Designs and oversees quality audit programmes. 
Leads strategic interventions to improve information classification/labelling. 
Engages with industry bodies and collaborates to define and improve standards and working practices."""@en .

sfialevels:ARCH_4 a sfia:SkillLevel ;
    skos:notation "ARCH_4" ;
    sfia:level lor:4 ;
    sfia:skillLevelDescription """Contributes to the development of solution architectures in specific business, infrastructure or functional areas. 
Identifies and evaluates alternative architectures and the trade-offs in cost, performance and scalability. Determines and documents architecturally significant decisions. 
Produces specifications of cloud-based or on-premises components, tiers and interfaces, for translation into detailed designs using selected services and products. 
Supports projects or change initiatives through the preparation of technical plans and application of design principles. Aligns solutions with enterprise and solution architecture standards (including security)."""@en .

sfialevels:ARCH_5 a sfia:SkillLevel ;
    skos:notation "ARCH_5" ;
    sfia:level lor:5 ;
    sfia:skillLevelDescription """Leads the development of solution architectures in specific business, infrastructure or functional areas. 
Leads the preparation of technical plans and ensures appropriate technical resources are made available. Ensures appropriate tools and methods are available, understood and employed in architecture development.
Provides technical guidance and governance on solution development and integration. Evaluates requests for changes and deviations from specifications and recommends actions.
Ensures relevant technical strategies, policies, standards and practices (including security and cost management) are applied correctly."""@en .

sfialevels:ARCH_6 a sfia:SkillLevel ;
    skos:notation "ARCH_6" ;
    sfia:level lor:6 ;
    sfia:skillLevelDescription """Leads the development of architectures for complex solutions ensuring consistency with agreed requirements. 
Establishes policies, principles and practices for the selection of solution architecture components. 
Manages trade-offs and balances functional, service quality, cost efficiency and systems management requirements within a significant area of the organisation. Communicates proposed decisions to stakeholders.
Coordinates and manages the target architecture across multiple projects or initiatives.  Maintains a stable, viable architecture and ensures consistency of design and adherence to appropriate standards across multiple projects or initiatives."""@en .

sfialevels:ASMG_2 a sfia:SkillLevel ;
    skos:notation "ASMG_2" ;
    sfia:level lor:2 ;
    sfia:skillLevelDescription """Uses agreed procedures to create and maintain an accurate register of assets. 
Performs activities related to the administration of assets. 
Produces routine reports to assist asset management activities and decision-making."""@en .

sfialevels:ASMG_3 a sfia:SkillLevel ;
    skos:notation "ASMG_3" ;
    sfia:level lor:3 ;
    sfia:skillLevelDescription """Applies tools, techniques and processes to create and maintain an accurate asset register. 
Produces reports and analysis to support asset management activities and aid decision-making."""@en .

sfialevels:ASMG_4 a sfia:SkillLevel ;
    skos:notation "ASMG_4" ;
    sfia:level lor:4 ;
    sfia:skillLevelDescription """Controls assets in one or more significant areas ensuring administration of full lifecycle of assets is carried out. 
Produces and analyses registers and histories of authorised assets and verifies that all of these assets are in a known state and location. 
Acts to highlight and resolve potential instances of unauthorised assets."""@en .

sfialevels:ASMG_5 a sfia:SkillLevel ;
    skos:notation "ASMG_5" ;
    sfia:level lor:5 ;
    sfia:skillLevelDescription """Manages and maintains the service compliance of  IT and service assets in line with business and regulatory requirements. 
Identifies, assesses and communicates associated risks. 
Ensures asset controllers, infrastructure teams and the business co-ordinate and optimise value, maintain control and maintain appropriate legal compliance."""@en .

sfialevels:ASMG_6 a sfia:SkillLevel ;
    skos:notation "ASMG_6" ;
    sfia:level lor:6 ;
    sfia:skillLevelDescription """Sets the strategy for asset management across the organisation. 
Communicates the policy, governance, scope and roles involved in asset management. 
Promotes awareness of and commitment to the role of asset management in the continuing economic and effective provision of services. Provides information and advice on complex asset management issues.
Initiates impact assessment arising from decisions to obtain, change or continue the possession or use of an asset, system or service."""@en .

sfialevels:ASUP_2 a sfia:SkillLevel ;
    skos:notation "ASUP_2" ;
    sfia:level lor:2 ;
    sfia:skillLevelDescription """Assists with specified maintenance procedures. 
Assists in the investigation and resolution of issues relating to applications."""@en .

sfialevels:ASUP_3 a sfia:SkillLevel ;
    skos:notation "ASUP_3" ;
    sfia:level lor:3 ;
    sfia:skillLevelDescription """Follows agreed procedures to identify and resolve issues with applications. 
Uses application management software and tools to collect agreed performance statistics. 
Carries out agreed applications maintenance tasks."""@en .

sfialevels:ASUP_4 a sfia:SkillLevel ;
    skos:notation "ASUP_4" ;
    sfia:level lor:4 ;
    sfia:skillLevelDescription """Maintains application support processes and checks that all requests for support are dealt with according to agreed procedures. 
Uses application management software and tools to investigate issues, collect performance statistics and create reports."""@en .

sfialevels:ASUP_5 a sfia:SkillLevel ;
    skos:notation "ASUP_5" ;
    sfia:level lor:5 ;
    sfia:skillLevelDescription """Ensures all requests for support are dealt with according to set standards and procedures. 
Drafts and maintains procedures and documentation for applications support, incorporating security considerations.
Manages application enhancements to improve business performance. 
Advises on application security, licensing, upgrades, backups and disaster recovery needs."""@en .

sfialevels:AUDT_2 a sfia:SkillLevel ;
    skos:notation "AUDT_2" ;
    sfia:level lor:2 ;
    sfia:skillLevelDescription """Assists in collecting evidence and conducting audit activities under routine supervision. 
Maintains documentation and audit trails. 
Helps identify and report issues and discrepancies."""@en .

sfialevels:AUDT_3 a sfia:SkillLevel ;
    skos:notation "AUDT_3" ;
    sfia:level lor:3 ;
    sfia:skillLevelDescription """Adopts a structured approach to executing and documenting audit fieldwork, following agreed standards. 
Maintains integrity of records to support and satisfy audit trails.
Identifies typical risk indicators and explains prevention measures."""@en .

sfialevels:AUDT_4 a sfia:SkillLevel ;
    skos:notation "AUDT_4" ;
    sfia:level lor:4 ;
    sfia:skillLevelDescription """Contributes to planning and executing of risk-based audit of existing and planned processes, products, systems and services.
Identifies and documents risks in detail.
Identifies the root cause of issues during an audit and communicates these effectively as risk insights.
Collates evidence regarding the interpretation and implementation of control measures. Prepares and communicates reports to stakeholders, providing a factual basis for findings."""@en .

sfialevels:AUDT_5 a sfia:SkillLevel ;
    skos:notation "AUDT_5" ;
    sfia:level lor:5 ;
    sfia:skillLevelDescription """Plans, organises and conducts audits of complex domains areas, cross-functional areas and across the supply chain.
Confirms the scope and objectives of specific audit activities with management. Aligns with the scope of the audit programme and organisational policies.
Determines appropriate methods of investigation to achieve the audit objectives. Presents audit findings to management describing the effectiveness and efficiency of control mechanisms.
Provides general and specific audit advice. Collaborates with professionals in related specialisms to develop and integrate findings."""@en .

sfialevels:AUDT_6 a sfia:SkillLevel ;
    skos:notation "AUDT_6" ;
    sfia:level lor:6 ;
    sfia:skillLevelDescription """Leads and manages complex audits and programmes of audit activity.
Obtains and manages appropriate specialist expertise to contribute highly specialised technical knowledge and experience.
Develops organisational policies, standards and guidelines for the conduct of audits. Ensures the objectivity and impartiality of the audit process.
Identifies areas of risk and specifies audit programmes. Ensures audit coverage is sufficient to provide the business with assurance of adequacy and integrity. Authorises the issue of formal reports to management on the effectiveness and efficiency of control mechanisms."""@en .

sfialevels:AUDT_7 a sfia:SkillLevel ;
    skos:notation "AUDT_7" ;
    sfia:level lor:7 ;
    sfia:skillLevelDescription """Directs the definition and implementation of the organisation's audit function, and oversees its communication to stakeholders.
Defines audit strategy, plans audit cycles and ensures appropriate coverage across the organisation. Ensures the audit function adds value. Liaises with stakeholders to ensure audit coverage is relevant and understood.
Directs use of risk analysis to identify areas for review. Ensures appropriate resources are available to deliver organisational requirements for audits.
Reports to the most senior level on findings, relevance and recommendations for improvement of audit activity."""@en .

sfialevels:AVMT_3 a sfia:SkillLevel ;
    skos:notation "AVMT_3" ;
    sfia:level lor:3 ;
    sfia:skillLevelDescription """Performs defined availability management tasks, such as routine monitoring and data collection.
Tests disaster recovery procedures under direction and contributes to the documentation of recovery plans.
Assists with the operation of availability management tools and processes.
Monitors service components against agreed performance standards and reports any deviations."""@en .

sfialevels:AVMT_4 a sfia:SkillLevel ;
    skos:notation "AVMT_4" ;
    sfia:level lor:4 ;
    sfia:skillLevelDescription """Analyses service and component availability, reliability, maintainability and serviceability. 
Contributes to the availability management process and its operation. 
Monitors and maintains services and components to ensure ongoing compliance with agreed performance targets and service levels.
Implements disaster recovery arrangements and documents recovery procedures. Conducts testing of recovery procedures."""@en .

sfialevels:AVMT_5 a sfia:SkillLevel ;
    skos:notation "AVMT_5" ;
    sfia:level lor:5 ;
    sfia:skillLevelDescription """Provides advice and guidance on the planning, design and improvement of service and component availability. 
Investigates all breaches of availability targets and service non-availability and initiates remedial activities. 
Develops plans for disaster recovery together with supporting processes. 
Manages the testing of disaster recovery plans."""@en .

sfialevels:AVMT_6 a sfia:SkillLevel ;
    skos:notation "AVMT_6" ;
    sfia:level lor:6 ;
    sfia:skillLevelDescription """Sets policy and develops strategies, plans and processes to ensure services deliver agreed levels of availability. 
Develops and implements new availability tools and techniques."""@en .

sfialevels:BENM_3 a sfia:SkillLevel ;
    skos:notation "BENM_3" ;
    sfia:level lor:3 ;
    sfia:skillLevelDescription """Supports the identification and tracking of benefits for projects and programmes.  
Collects data to measure benefits realisation."""@en .

sfialevels:BENM_4 a sfia:SkillLevel ;
    skos:notation "BENM_4" ;
    sfia:level lor:4 ;
    sfia:skillLevelDescription """Contributes to the development and implementation of benefits management plans for projects and programmes. 
Engages with stakeholders to identify and quantify benefits and to establish metrics and mechanisms for tracking benefits realisation. 
Monitors and reports on progress towards benefits realisation. 
Identifies risks and issues that may impact benefits delivery and escalates as appropriate. Supports the embedding of benefits management practices across the organisation."""@en .

sfialevels:BENM_5 a sfia:SkillLevel ;
    skos:notation "BENM_5" ;
    sfia:level lor:5 ;
    sfia:skillLevelDescription """Leads activities required in the realisation of the benefits of each part of the change programme. 
Identifies specific metrics and mechanisms to measure benefits and plans to activate these mechanisms at the required time. Monitors benefits against what was predicted in the business case. 
Ensures all participants are engaged throughout the change programme and fully prepared to exploit the new operational business environment. 
Supports operational managers to ensure all plans, work packages and deliverables are aligned with the expected benefits."""@en .

sfialevels:BENM_6 a sfia:SkillLevel ;
    skos:notation "BENM_6" ;
    sfia:level lor:6 ;
    sfia:skillLevelDescription """Works with operational managers to ensure maximum improvements are made as groups of projects deliver their products into operational use. 
Communicates the change programme vision to staff at all levels of the business and keeps a focus on business objectives. 
Maintains the business case for funding the programme and confirms continuing business viability of the programme at regular intervals."""@en .

sfialevels:BIDM_3 a sfia:SkillLevel ;
    skos:notation "BIDM_3" ;
    sfia:level lor:3 ;
    sfia:skillLevelDescription """Supports the development of proposals by engaging in document analysis and internal review. 
Understands and analyses bid documents and requirements, preparing initial response drafts that align with the organisation's capabilities and stakeholder needs. 
Communicates with internal stakeholders to gather necessary information and clarify proposal requirements. 
Ensures proposal responses meet basic compliance standards and align with the specified requirements and organisational capabilities."""@en .

sfialevels:BIDM_4 a sfia:SkillLevel ;
    skos:notation "BIDM_4" ;
    sfia:level lor:4 ;
    sfia:skillLevelDescription """Leads the creation of small to medium proposals, integrating technical analysis and broader context. 
Coordinates team efforts, shapes the proposal structure and addresses financial aspects including budgeting and pricing strategies. 
Identifies and manages proposal risks, ensuring timely compliance with stakeholder expectations. 
Engages with stakeholders and shapes proposal structure and content based on in-depth discussions and feedback."""@en .

sfialevels:BIDM_5 a sfia:SkillLevel ;
    skos:notation "BIDM_5" ;
    sfia:level lor:5 ;
    sfia:skillLevelDescription """Leads the formulation and execution of significant proposals, managing the process from initial evaluation to final submission. 
Oversees significant proposals, aligning them with organisational strategies and managing the process from inception to submission. 
Collaborates with high-level stakeholders, negotiates with key stakeholders and secures advantageous partnerships. 
Refines and optimises the proposal development process for efficiency and effectiveness."""@en .

sfialevels:BIDM_6 a sfia:SkillLevel ;
    skos:notation "BIDM_6" ;
    sfia:level lor:6 ;
    sfia:skillLevelDescription """Directs major proposal initiatives, devising engagement strategies and promoting excellence in proposal practices throughout the organisation. 
Influences organisational policies and strategies in proposal management, setting standards and expectations."""@en .

sfialevels:BINT_2 a sfia:SkillLevel ;
    skos:notation "BINT_2" ;
    sfia:level lor:2 ;
    sfia:skillLevelDescription """Assists with the creation of regular business intelligence reports using standard tools. 
Supports data preparation from existing sources."""@en .

sfialevels:BINT_3 a sfia:SkillLevel ;
    skos:notation "BINT_3" ;
    sfia:level lor:3 ;
    sfia:skillLevelDescription """Sources and prepares data for analysis and performs standard business intelligence analysis activities. 
Checks the integrity and validity of data sources. Creates and delivers standard reports in accordance with stakeholder needs and conforming to agreed standards. 
Investigates the need for new or revised business intelligence analysis.  
Contributes to the recommendation of improvements. Engages with stakeholders under direction."""@en .

sfialevels:BINT_4 a sfia:SkillLevel ;
    skos:notation "BINT_4" ;
    sfia:level lor:4 ;
    sfia:skillLevelDescription """Supports business intelligence needs of specific management or governance processes or operational areas. 
Investigates the need for business intelligence reporting and analysis where there is some complexity and ambiguity. 
Selects and applies non-standard business intelligence tools and techniques to provide insights and aid decision-making. Selects, acquires and integrates data for analysis and verifies the data's quality and integrity.
Identifies opportunities to digitise and streamline operational data handling and optimise business intelligence capabilities."""@en .

sfialevels:BINT_5 a sfia:SkillLevel ;
    skos:notation "BINT_5" ;
    sfia:level lor:5 ;
    sfia:skillLevelDescription """Plans and manages business intelligence activities. 
Ensures business intelligence processes, procedures and practices are robust, efficient and fit for purpose, focusing on automation, key controls and data quality. Advises on the available standards, procedures, methods, tools and techniques.
Manages reviews of the benefits and value of business intelligence techniques and tools and recommends improvements. 
Contributes to the development of analytics policies, standards and guidelines."""@en .

sfialevels:BPRE_2 a sfia:SkillLevel ;
    skos:notation "BPRE_2" ;
    sfia:level lor:2 ;
    sfia:skillLevelDescription """Assists in gathering data and documenting current business processes under routine supervision. 
Participates in process mapping exercises and helps identify areas for potential improvement.
Assists in creating process documentation.
Supports the implementation of minor process changes and improvements."""@en .

sfialevels:BPRE_3 a sfia:SkillLevel ;
    skos:notation "BPRE_3" ;
    sfia:level lor:3 ;
    sfia:skillLevelDescription """Applies standard techniques to analyse existing business processes and identifies opportunities for improvement.  
Collaborates with stakeholders to ensure process changes align with business objectives. Proposes and implements process improvements that enhance efficiency, effectiveness and quality. 
Develops and maintains process documentation. 
Supports the adoption of new technologies and tools to enable process automation and optimisation."""@en .

sfialevels:BPRE_4 a sfia:SkillLevel ;
    skos:notation "BPRE_4" ;
    sfia:level lor:4 ;
    sfia:skillLevelDescription """Analyses and designs business processes to identify alternative solutions to improve efficiency, effectiveness and exploit new technologies and automation.
Develops graphical models of business processes to facilitate understanding and decision-making.
Recommends implementation approaches for process improvement initiatives."""@en .

sfialevels:BPRE_5 a sfia:SkillLevel ;
    skos:notation "BPRE_5" ;
    sfia:level lor:5 ;
    sfia:skillLevelDescription """Manages the execution of business process improvements. 
Assesses the feasibility of business process changes and recommends alternative approaches. 
Selects, tailors and implements methods and tools for improving business processes at programme, project or team level. 
Contributes to the definition of organisational policies, standards and guidelines for business process improvement."""@en .

sfialevels:BPRE_6 a sfia:SkillLevel ;
    skos:notation "BPRE_6" ;
    sfia:level lor:6 ;
    sfia:skillLevelDescription """Plans and leads strategic, large and complex business process improvement activities aligned with automation, or exploiting existing or new technologies.
Develops organisational policies, standards and guidelines for business process improvement. 
Leads the introduction of techniques, methodologies and tools to meet business requirements, ensuring consistency across all user groups.
Leads the development of organisational capabilities for business process improvement and ensures adoption and adherence to policies and standards."""@en .

sfialevels:BPRE_7 a sfia:SkillLevel ;
    skos:notation "BPRE_7" ;
    sfia:level lor:7 ;
    sfia:skillLevelDescription """Directs the identification, evaluation and adoption of new or existing technologies to improve business processes. 
Aligns business strategies, enterprise transformation and technology strategies. 
Embeds strategic business process improvement into the governance and leadership of the organisation. 
Directs the creation and review of a cross-functional, enterprise-wide approach and culture for embracing business process management."""@en .

sfialevels:BPTS_2 a sfia:SkillLevel ;
    skos:notation "BPTS_2" ;
    sfia:level lor:2 ;
    sfia:skillLevelDescription """Assists in planning and preparing acceptance tests for systems, products, business processes or services.
Assists in collecting feedback from acceptance testing."""@en .

sfialevels:BPTS_3 a sfia:SkillLevel ;
    skos:notation "BPTS_3" ;
    sfia:level lor:3 ;
    sfia:skillLevelDescription """Follows agreed standards and techniques to devise test cases and scenarios based on pre-defined acceptance criteria. 
Analyses and reports on test activities, results, issues and risks."""@en .

sfialevels:BPTS_4 a sfia:SkillLevel ;
    skos:notation "BPTS_4" ;
    sfia:level lor:4 ;
    sfia:skillLevelDescription """Develops acceptance criteria related to functional and non-functional requirements, business processes, features, user stories and business rules. 
Designs and specifies test cases and scenarios to test that systems, products and services fulfil the acceptance criteria and deliver the predicted business benefits. 
Collaborates with project colleagues and stakeholders involved in the analysis, development and operation of products, systems or services to ensure accuracy and comprehensive test coverage. 
Analyses and reports on test activities, results, issues and risks including the work of others."""@en .

sfialevels:BPTS_5 a sfia:SkillLevel ;
    skos:notation "BPTS_5" ;
    sfia:level lor:5 ;
    sfia:skillLevelDescription """Plans and manages user acceptance testing activity.
Specifies the testing environment. Manages the creation of test cases and scenarios, ensuring they reflect realistic operational conditions and coverage needs. 
Ensures entry and exit criteria are set and met before user acceptance testing starts or ends. Specifies required user resources. Ensures users receive appropriate training and support.
Ensures tests and results are documented, analysed and reported, highlighting issues and risks to stakeholders. Provides authoritative advice on acceptance testing planning and execution."""@en .

sfialevels:BPTS_6 a sfia:SkillLevel ;
    skos:notation "BPTS_6" ;
    sfia:level lor:6 ;
    sfia:skillLevelDescription """Leads the organisation's approach to user acceptance testing.
Engages senior stakeholders to secure organisational commitment and resources for effective acceptance testing. 
Integrates entry and exit criteria into user acceptance testing planning and execution. Provides input on required resources, including skills and availability, for user acceptance testing activities. Reports on any significant risks and issues, recommending actions as needed. 
Develops organisational policies, standards and guidelines for acceptance testing. Develops acceptance testing capabilities and methods for the organisation."""@en .

sfialevels:BRMG_4 a sfia:SkillLevel ;
    skos:notation "BRMG_4" ;
    sfia:level lor:4 ;
    sfia:skillLevelDescription """Contributes to the development and implementation of brand identity elements and guidelines. 
Supports brand research and analysis. 
Ensures consistent application of brand standards across assigned projects. 
Monitors brand performance metrics and reports on key findings."""@en .

sfialevels:BRMG_5 a sfia:SkillLevel ;
    skos:notation "BRMG_5" ;
    sfia:level lor:5 ;
    sfia:skillLevelDescription """Leads the development and execution of brand strategies and plans. 
Defines brand positioning, values and value proposition. Applies principles of brand architecture to manage brand portfolio. 
Conducts in-depth brand performance analysis and provides strategic recommendations. 
Uses creative approaches to differentiate the brand. Collaborates with internal and external stakeholders to align brand initiatives with business objectives."""@en .

sfialevels:BRMG_6 a sfia:SkillLevel ;
    skos:notation "BRMG_6" ;
    sfia:level lor:6 ;
    sfia:skillLevelDescription """Establishes the overall brand vision, strategy and governance for the organisation. 
Oversees brand research, analysis and strategic planning. 
Evaluates brand performance and equity, making decisions to enhance brand value and organisational outcomes. Ensures alignment of brand strategy with organisational goals and market dynamics. 
Governs the application of visual identity and distinctive brand assets across the organisation."""@en .

sfialevels:BSMO_2 a sfia:SkillLevel ;
    skos:notation "BSMO_2" ;
    sfia:level lor:2 ;
    sfia:skillLevelDescription """Assists in creating models for simple, well-defined business scenarios under guidance. 
Uses established techniques, as directed, to model simple subject areas with clearly-defined boundaries.
Supports more complex modelling activities under the guidance of others by organising information and helping to apply relevant techniques."""@en .

sfialevels:BSMO_3 a sfia:SkillLevel ;
    skos:notation "BSMO_3" ;
    sfia:level lor:3 ;
    sfia:skillLevelDescription """Produces models for straightforward business scenarios with clear boundaries, selecting suitable techniques to meet assigned objectives. 
Engages with subject matter experts to ensure models are accurate and meet business requirements. Applies established techniques to meet objectives, modelling business processes, roles and data.
Collaborates with stakeholders to address issues and ensure models provide clarity and insight. 
Tests models and makes improvements as needed, ensuring accuracy and relevance to the business context."""@en .

sfialevels:BSMO_4 a sfia:SkillLevel ;
    skos:notation "BSMO_4" ;
    sfia:level lor:4 ;
    sfia:skillLevelDescription """Develops models for complex and ambiguous business scenarios. 
Selects appropriate techniques and approaches to ensure models capture the necessary business elements. Independently plans modelling activities, ensuring alignment with business objectives.
Collaborates with operational stakeholders to validate and refine models based on feedback, and to gain agreement on modelling results and their implications. 
Advises stakeholders interpreting and applying models for decision-making and business improvements."""@en .

sfialevels:BSMO_5 a sfia:SkillLevel ;
    skos:notation "BSMO_5" ;
    sfia:level lor:5 ;
    sfia:skillLevelDescription """Manages the development of models that support strategic business objectives.
Works on complex and ambiguous scenarios, applying advanced techniques and methods. Creates bespoke models for non-standard contexts and ensures their alignment with overall business strategy.
Ensures the quality of business modelling work. 
Engages and collaborates with a wide range of stakeholders providing guidance on selecting and applying appropriate modelling techniques. Influences decision-making by presenting models that highlight key business insights."""@en .

sfialevels:BSMO_6 a sfia:SkillLevel ;
    skos:notation "BSMO_6" ;
    sfia:level lor:6 ;
    sfia:skillLevelDescription """Defines organisational standards for business modelling, ensuring models align with strategic business objectives. 
Oversees the creation and maintenance of models across multiple functions and departments, ensuring they are used effectively.
Leads organisation-wide initiatives to improve business modelling, introducing new techniques where necessary. 
Engages with senior stakeholders to gain agreement on strategic models and the decisions they inform."""@en .

sfialevels:BUDF_2 a sfia:SkillLevel ;
    skos:notation "BUDF_2" ;
    sfia:level lor:2 ;
    sfia:skillLevelDescription """Assists in gathering financial data and preparing basic budget templates under supervision. 
Supports the budgeting and forecasting process by completing assigned tasks."""@en .

sfialevels:BUDF_3 a sfia:SkillLevel ;
    skos:notation "BUDF_3" ;
    sfia:level lor:3 ;
    sfia:skillLevelDescription """Performs specified tasks in the budgeting and forecasting process, including data analysis and report preparation, using standard methods. 
Identifies and resolves routine budgeting and forecasting issues. 
Communicates budget and forecast information to relevant stakeholders."""@en .

sfialevels:BUDF_4 a sfia:SkillLevel ;
    skos:notation "BUDF_4" ;
    sfia:level lor:4 ;
    sfia:skillLevelDescription """Contributes to the development of budgets and forecasts for specific areas of responsibility.
Gathers and analyses financial data and prepares budget templates and reports.
Supports stakeholder communication and collaboration in the budgeting and forecasting process."""@en .

sfialevels:BUDF_5 a sfia:SkillLevel ;
    skos:notation "BUDF_5" ;
    sfia:level lor:5 ;
    sfia:skillLevelDescription """Leads the development of budgets and forecasts for a department or function.
Provides authoritative advice and guidance on budgeting and forecasting practices. Selects and applies appropriate budgeting and forecasting methodologies and tools.
Incorporates scenario planning, sensitivity analysis and risk assessment into the budgeting and forecasting process.
Collaborates with stakeholders to align budgets and forecasts with organisational objectives and business metrics."""@en .

sfialevels:BUDF_6 a sfia:SkillLevel ;
    skos:notation "BUDF_6" ;
    sfia:level lor:6 ;
    sfia:skillLevelDescription """Develops and implements budgeting and forecasting strategies, policies and processes aligned with overall organisational objectives and business metrics. 
Drives the adoption of good working practices across the organisation.
Oversees the development of complex financial models and scenario analyses to support strategic decision-making. Provides insights and recommendations to optimise investments and resource allocation.
Collaborates with senior leaders to ensure budgets and forecasts support long-term organisational goals and drive value creation. Sets the vision and direction for budgeting and forecasting practices."""@en .

sfialevels:BURM_2 a sfia:SkillLevel ;
    skos:notation "BURM_2" ;
    sfia:level lor:2 ;
    sfia:skillLevelDescription """Assists in collecting and reporting data to support risk management activities under routine supervision. 
Helps create and maintain documentation of risks and risk management activities. 
Helps identify and report issues and discrepancies."""@en .

sfialevels:BURM_3 a sfia:SkillLevel ;
    skos:notation "BURM_3" ;
    sfia:level lor:3 ;
    sfia:skillLevelDescription """Undertakes basic risk management activities. 
Maintains documentation of risks, threats, vulnerabilities and mitigation actions."""@en .

sfialevels:BURM_4 a sfia:SkillLevel ;
    skos:notation "BURM_4" ;
    sfia:level lor:4 ;
    sfia:skillLevelDescription """Carries out risk management activities within a specific function, technical area or project of medium complexity. 
Identifies risks and vulnerabilities, assesses their impact and probability, develops mitigation strategies and reports to the business. 
Involves specialists and domain experts as necessary."""@en .

sfialevels:BURM_5 a sfia:SkillLevel ;
    skos:notation "BURM_5" ;
    sfia:level lor:5 ;
    sfia:skillLevelDescription """Plans and implements complex and substantial risk management activities within a specific function, technical area, project or programme. 
Establishes consistent risk management processes and reporting mechanisms aligned with governance frameworks.
Engages specialists and domain experts as necessary. 
Advises on the organisation's approach to risk management."""@en .

sfialevels:BURM_6 a sfia:SkillLevel ;
    skos:notation "BURM_6" ;
    sfia:level lor:6 ;
    sfia:skillLevelDescription """Plans and manages the implementation of organisation-wide risk management processes, integrating tools and techniques aligned with governance frameworks.
Considers organisation-wide risk and mitigation activities within the context of business risk as a whole and the organisation's appetite for risk.
Provides leadership on risk management, ensuring practices support strategic decision-making and compliance with organisational policies."""@en .

sfialevels:BURM_7 a sfia:SkillLevel ;
    skos:notation "BURM_7" ;
    sfia:level lor:7 ;
    sfia:skillLevelDescription """Establishes the organisation's risk management strategy, defining and communicating the risk appetite in alignment with governance and strategic objectives.
Defines and communicates the organisation's appetite for risk. 
Provides resources to implement the organisation's risk strategy. 
Delegates authority for detailed planning and execution of risk management activities across the organisation."""@en .

sfialevels:BUSA_2 a sfia:SkillLevel ;
    skos:notation "BUSA_2" ;
    sfia:level lor:2 ;
    sfia:skillLevelDescription """Assists in investigating business situations to help identify and analyse problems and opportunities, under routine supervision. 
Helps collect and organise data and information to support recommendations."""@en .

sfialevels:BUSA_3 a sfia:SkillLevel ;
    skos:notation "BUSA_3" ;
    sfia:level lor:3 ;
    sfia:skillLevelDescription """Investigates straightforward business situations to identify and analyse problems and opportunities. 
Contributes to the recommendation of improvements. 
Follows agreed standards and techniques to investigate, analyse and document business situations. 
Engages with stakeholders under direction."""@en .

sfialevels:BUSA_4 a sfia:SkillLevel ;
    skos:notation "BUSA_4" ;
    sfia:level lor:4 ;
    sfia:skillLevelDescription """Investigates business situations where there is some complexity and ambiguity. 
Adopts holistic view to identify and analyse problems and opportunities. 
Contributes to the selection of the approach and techniques to be used for business situation analysis. 
Conducts root cause analysis and identifies recommendations for improvements. Engages and collaborates with operational stakeholders."""@en .

sfialevels:BUSA_5 a sfia:SkillLevel ;
    skos:notation "BUSA_5" ;
    sfia:level lor:5 ;
    sfia:skillLevelDescription """Plans, manages and investigates business situation analysis where there is significant ambiguity and complexity. 
Advises on the approach and techniques to be used for business situation analysis. Ensures holistic view adopted to identify and analyse wide-ranging problems and opportunities. 
Engages and collaborates with a wide range of stakeholders, including those at the management level. Gains agreement from stakeholders to conclusions and recommendations. 
Contributes to definition of organisational standards and guidelines for business situation analysis."""@en .

sfialevels:BUSA_6 a sfia:SkillLevel ;
    skos:notation "BUSA_6" ;
    sfia:level lor:6 ;
    sfia:skillLevelDescription """Initiates and leads business situation analysis where there is extensive ambiguity, complexity and potentially significant organisational impacts. 
Establishes and promotes the need for holistic business situation analysis prior to change programme initiation. 
Engages with stakeholders at executive level and advises on recommended change initiatives. 
Defines organisational policies, standards and techniques for business situation analysis."""@en .

sfialevels:CELO_3 a sfia:SkillLevel ;
    skos:notation "CELO_3" ;
    sfia:level lor:3 ;
    sfia:skillLevelDescription """Assists in implementing customer engagement and loyalty initiatives. 
Uses marketing technologies for customer engagement tasks. Sets up campaigns in lifecycle management tools.
Collects and analyses customer data to support personalised communications. 
Monitors and reports on customer engagement metrics."""@en .

sfialevels:CELO_4 a sfia:SkillLevel ;
    skos:notation "CELO_4" ;
    sfia:level lor:4 ;
    sfia:skillLevelDescription """Develops and executes customer engagement and loyalty initiatives. 
Creates and manages loyalty programmes. 
Analyses customer data to inform targeted communications and experiences. Develops customer segmentation approaches.
Applies appropriate marketing technologies to support initiatives. Measures and reports on the effectiveness of engagement and loyalty efforts."""@en .

sfialevels:CELO_5 a sfia:SkillLevel ;
    skos:notation "CELO_5" ;
    sfia:level lor:5 ;
    sfia:skillLevelDescription """Leads the development and implementation of comprehensive customer engagement and loyalty plans. 
Oversees the creation and management of loyalty programmes and initiatives. Develops comprehensive plans for customer communications across all lifecycle stages.
Uses advanced analytics to optimise personalised customer experiences. Provides recommendations based on customer engagement and loyalty insights.
Collaborates with cross-functional teams to improve customer retention and satisfaction. Evaluates and recommends marketing technologies for customer engagement."""@en .

sfialevels:CELO_6 a sfia:SkillLevel ;
    skos:notation "CELO_6" ;
    sfia:level lor:6 ;
    sfia:skillLevelDescription """Defines organisational vision and strategy for customer engagement and loyalty. 
Drives innovation in loyalty programme development and implementation. Aligns customer engagement strategies with overall business objectives. 
Leads the assessment and adoption of advanced marketing technologies. Directs the development of customer journeys and database management strategies. 
Ensures integration of customer engagement initiatives across all business functions."""@en .

sfialevels:CEXP_2 a sfia:SkillLevel ;
    skos:notation "CEXP_2" ;
    sfia:level lor:2 ;
    sfia:skillLevelDescription """Assists in the creation of customer journey maps and identifies key touchpoints for improvement.
Follows established procedures to document customer feedback and support the implementation of minor improvements."""@en .

sfialevels:CEXP_3 a sfia:SkillLevel ;
    skos:notation "CEXP_3" ;
    sfia:level lor:3 ;
    sfia:skillLevelDescription """Analyses research to gather detailed insights into customer needs and preferences. 
Uses appropriate tools and methods for data collection. Participates in the design and optimisation of customer journeys. 
Collaborates with team members to implement customer experience improvements. 
Documents findings and supports the analysis process."""@en .

sfialevels:CEXP_4 a sfia:SkillLevel ;
    skos:notation "CEXP_4" ;
    sfia:level lor:4 ;
    sfia:skillLevelDescription """Uses customer research findings to gain a comprehensive understanding of customer needs and expectations.
Enables the creation of visual representations of customer journeys to enhance cross-functional collaboration. Designs and refines customer journeys, working with cross-functional teams to enhance touchpoints and interactions. 
Develops and implements designs to improve customer experience. Recommends and applies appropriate technologies and segmentation insights to enhance customer experiences.
Monitors metrics and feedback to assess effectiveness and drive continuous improvement."""@en .

sfialevels:CEXP_5 a sfia:SkillLevel ;
    skos:notation "CEXP_5" ;
    sfia:level lor:5 ;
    sfia:skillLevelDescription """Plans and oversees customer experience initiatives. 
Ensures alignment with business goals and customer expectations.
Establishes frameworks for monitoring and measuring customer experience. Uses data-driven insights to guide improvements.
Ensures customer experience designs leverage customer insights and emerging technologies for personalised experiences. Works with senior stakeholders to develop and implement customer experience strategies. Drives collaboration across teams to ensure a consistent experience."""@en .

sfialevels:CEXP_6 a sfia:SkillLevel ;
    skos:notation "CEXP_6" ;
    sfia:level lor:6 ;
    sfia:skillLevelDescription """Champions customer experience at an organisational level. 
Leads strategic initiatives to enhance customer experience, including the evaluation and adoption of innovative technologies and approaches. Aligns efforts with business objectives and customer needs.
Monitors industry trends and innovations in customer experience. 
Develops policies and standards to guide customer experience practices. Ensures adoption of good practices and continuous improvement within the organisation."""@en .

sfialevels:CFMG_2 a sfia:SkillLevel ;
    skos:notation "CFMG_2" ;
    sfia:level lor:2 ;
    sfia:skillLevelDescription """Applies tools, techniques and processes to administer, track, log, report on and correct configuration items, components and changes. 
Assists with audits to check the accuracy of the information and undertakes any necessary corrective action under direction."""@en .

sfialevels:CFMG_3 a sfia:SkillLevel ;
    skos:notation "CFMG_3" ;
    sfia:level lor:3 ;
    sfia:skillLevelDescription """Applies tools, techniques and processes to track, log and correct information related to configuration items. 
Verifies and approves changes to protect assets and components from unauthorised change, diversion and inappropriate use. 
Supports user compliance with identification standards for object types, environments, processes, lifecycles, documentation, versions, formats, baselines, releases and templates. 
Performs audits to check the accuracy of the information and undertakes any necessary corrective action under direction."""@en .

sfialevels:CFMG_4 a sfia:SkillLevel ;
    skos:notation "CFMG_4" ;
    sfia:level lor:4 ;
    sfia:skillLevelDescription """Proposes and agrees the configuration items (CIs) to be uniquely identified with naming conventions. 
Puts in place operational processes for secure configuration, classification and management of CIs and for verifying and auditing  configuration records. 
Develops, configures and maintains tools (including automation) to identify, track, log and maintain accurate, complete and current information. 
Reports on the status of configuration management. Identifies problems and issues and recommend corrective actions."""@en .

sfialevels:CFMG_5 a sfia:SkillLevel ;
    skos:notation "CFMG_5" ;
    sfia:level lor:5 ;
    sfia:skillLevelDescription """Plans the capture and management of CIs and related information. 
Agrees scope of configuration management processes and the configuration items (CIs) and related information to be controlled. 
Identifies, evaluates and manages the adoption of appropriate tools, techniques and processes (including automation) for configuration management. 
Contributes to the development of configuration management strategies, policies, standards and guidelines."""@en .

sfialevels:CFMG_6 a sfia:SkillLevel ;
    skos:notation "CFMG_6" ;
    sfia:level lor:6 ;
    sfia:skillLevelDescription """Develops configuration management strategies, policies, standards and guidelines. 
Champions the importance and value of configuration management and develops new methods and organisational capabilities (including automation) for configuration management. 
Provides resources to drive adoption of, and adherence to, policies and standards. 
Measures and monitors adherence to standards and ensures consistent execution of the process across the organisation."""@en .

sfialevels:CHMG_2 a sfia:SkillLevel ;
    skos:notation "CHMG_2" ;
    sfia:level lor:2 ;
    sfia:skillLevelDescription """Administers, tracks, logs, reports on change requests, using appropriate tools, techniques and processes.
Provides assistance to implement standard low-risk changes, in accordance with defined change control procedures."""@en .

sfialevels:CHMG_3 a sfia:SkillLevel ;
    skos:notation "CHMG_3" ;
    sfia:level lor:3 ;
    sfia:skillLevelDescription """Develops, documents and implements changes based on requests for change. 
Applies change control processes and procedures. 
Applies tools, techniques and processes to manage and report on change requests."""@en .

sfialevels:CHMG_4 a sfia:SkillLevel ;
    skos:notation "CHMG_4" ;
    sfia:level lor:4 ;
    sfia:skillLevelDescription """Assesses, analyses, develops, documents and implements changes based on requests for change. 
Ensures operational processes and procedures are in place for effective change control. 
Develops, configures and maintains tools to manage and report on the lifecycle of change requests.  
Identifies problems and issues and recommend corrective actions."""@en .

sfialevels:CHMG_5 a sfia:SkillLevel ;
    skos:notation "CHMG_5" ;
    sfia:level lor:5 ;
    sfia:skillLevelDescription """Leads the assessment, analysis, development, documentation and implementation of changes.
Develops implementation plans for complex requests for change. 
Reviews proposed implementations and evaluates the risks to the integrity of the product and service environment. Ensures appropriate change approval is applied to changes. 
Reviews the effectiveness of change implementation.  Identifies, evaluates and manages the adoption of appropriate tools, techniques and processes for change control."""@en .

sfialevels:CHMG_6 a sfia:SkillLevel ;
    skos:notation "CHMG_6" ;
    sfia:level lor:6 ;
    sfia:skillLevelDescription """Sets the organisation's policy for the management of change in live services and test environments.
Ensures effective control and treatment of risk. 
Leads the development of new and improved practices for change control. 
Measures and monitors adherence to standards and ensures consistent execution of the process across the organisation."""@en .

sfialevels:CIPM_2 a sfia:SkillLevel ;
    skos:notation "CIPM_2" ;
    sfia:level lor:2 ;
    sfia:skillLevelDescription """Assists with organisational change management tasks under routine supervision.
Supports the collection and analysis of data related to change readiness and impact.
Helps document and communicate change management plans and activities."""@en .

sfialevels:CIPM_3 a sfia:SkillLevel ;
    skos:notation "CIPM_3" ;
    sfia:level lor:3 ;
    sfia:skillLevelDescription """Follows standard techniques to investigate and analyse the size, nature and impact of changes to operational activities. 
Contributes to change management plans and actions, focusing on the procedural execution of change. 
Supports implementation and engages with stakeholders under direction."""@en .

sfialevels:CIPM_4 a sfia:SkillLevel ;
    skos:notation "CIPM_4" ;
    sfia:level lor:4 ;
    sfia:skillLevelDescription """Conducts readiness assessments to assess the size, nature and impact of organisational change. 
Defines tactics to use considering the challenges to be addressed. Provides guidance and makes suggestions to support individuals responsible for operational implementation of change management activities.
Gathers feedback to analyse the impact and effectiveness of the change management activities being deployed. Takes corrective action as required.
Develops and communicates tailored change management plans. Establishes and builds relationships with the project sponsors and key stakeholders."""@en .

sfialevels:CIPM_5 a sfia:SkillLevel ;
    skos:notation "CIPM_5" ;
    sfia:level lor:5 ;
    sfia:skillLevelDescription """Develops the change management approach and a change management plan in collaboration with sponsors, users and project teams. 
Creates and implements action plans to ensure readiness for change before going live. Acquires change management resources and develops their capabilities to deliver the required changes.
Gathers feedback to allow timely improvements to the change management plan and approach. Assesses risks and takes preventative action. 
Develops and communicates tailored change management plans for senior stakeholder groups. Provides guidance to support change sponsors."""@en .

sfialevels:CIPM_6 a sfia:SkillLevel ;
    skos:notation "CIPM_6" ;
    sfia:level lor:6 ;
    sfia:skillLevelDescription """Defines and communicates the approach for change management for a significant part of the organisation. 
Initiates, plans and leads strategic, large and complex change management initiatives. Provides guidance to change leaders, emphasising the technical and procedural aspects of change.
Establishes feedback processes and leads analyses of change management successes.  
Enables continual improvements to change management methodology, tools and training necessary to enhance the maturity across the organisation."""@en .

sfialevels:CNSL_4 a sfia:SkillLevel ;
    skos:notation "CNSL_4" ;
    sfia:level lor:4 ;
    sfia:skillLevelDescription """Takes responsibility for specific elements of a consulting engagement within a defined scope.
Collaborates with clients as part of formal or informal consultancy engagements. Understands client requirements by collecting data and delivering analysis. 
Ensures proposed solutions are correctly understood and effectively applied.
Supports the broader consultancy engagement by contributing insights and assisting with problem-solving, always within the established boundaries of responsibility."""@en .

sfialevels:CNSL_5 a sfia:SkillLevel ;
    skos:notation "CNSL_5" ;
    sfia:level lor:5 ;
    sfia:skillLevelDescription """Takes full responsibility for understanding client requirements including data collection, analysis and resolving issues.
Manages the scope and delivery of consultancy engagements to meet agreed objectives. Identifies, evaluates and recommends options. 
Collaborates with, and facilitates, stakeholder groups, as part of formal or informal consultancy agreements. Seeks to fully address client needs and implements solutions if required. 
Enhances the capabilities and effectiveness of clients by ensuring proposed solutions are fully understood and appropriately exploited."""@en .

sfialevels:CNSL_6 a sfia:SkillLevel ;
    skos:notation "CNSL_6" ;
    sfia:level lor:6 ;
    sfia:skillLevelDescription """Leads and manages the provision of consultancy services and/or a team of consultants. 
Provides expert advice and guidance in own areas of expertise to both consultants and clients.
Engages with clients at a strategic level, establishing consultancy agreements or contracts and maintaining long-term relationships. Manages the completion of engagements, ensuring strategic alignment with client needs and overseeing the transition from consultancy delivery to operational adoption. 
Oversees the development and delivery of consultancy services within the agreed strategic framework."""@en .

sfialevels:CNSL_7 a sfia:SkillLevel ;
    skos:notation "CNSL_7" ;
    sfia:level lor:7 ;
    sfia:skillLevelDescription """Directs the strategic direction and operations of a significant consultancy practice. 
Engages with key stakeholders at the highest levels to ensure consultancy services drive strategic outcomes. 
Manages overall client relationships and the development of long-term consultancy partnerships, maintaining high standards of service delivery and ethical practice.
Oversees practice development, proposals, sales, account management and the delivery of consultancy services across diverse topics."""@en .

sfialevels:COMG_2 a sfia:SkillLevel ;
    skos:notation "COMG_2" ;
    sfia:level lor:2 ;
    sfia:skillLevelDescription """Assists in gathering cost data and preparing basic cost reports under supervision. 
Supports the cost management process by completing assigned tasks and seeking guidance when needed."""@en .

sfialevels:COMG_3 a sfia:SkillLevel ;
    skos:notation "COMG_3" ;
    sfia:level lor:3 ;
    sfia:skillLevelDescription """Applies standard cost management techniques and processes to monitor and report on costs within a specific area of responsibility.
Identifies and escalates cost variances and supports the implementation of cost-saving initiatives. Collaborates with stakeholders to gather cost data and provide reports."""@en .

sfialevels:COMG_4 a sfia:SkillLevel ;
    skos:notation "COMG_4" ;
    sfia:level lor:4 ;
    sfia:skillLevelDescription """Develops and implements cost management processes and procedures for a department or function.
Monitors actual performance against budget and identifies variances.
Analyses costs, identifies trends and recommends corrective actions.
Provides guidance and advice on cost management techniques and tools."""@en .

sfialevels:COMG_5 a sfia:SkillLevel ;
    skos:notation "COMG_5" ;
    sfia:level lor:5 ;
    sfia:skillLevelDescription """Leads the development and implementation of cost management strategies, policies and procedures for a significant area of the organisation.
Provides authoritative advice and guidance on cost optimisation techniques and recognised good practices. Oversees the development of complex cost models and reporting frameworks.
Presents cost management insights to senior stakeholders and facilitates data-driven decision-making. Promotes a culture of cost consciousness and continuous improvement."""@en .

sfialevels:COMG_6 a sfia:SkillLevel ;
    skos:notation "COMG_6" ;
    sfia:level lor:6 ;
    sfia:skillLevelDescription """Defines and leads the organisation's overall approach to cost management, aligning it with strategic objectives and financial goals.
Develops and implements enterprise-wide cost management policies, standards and processes. Collaborates with senior leaders to identify and drive cost optimisation initiatives.
Provides strategic insights and recommendations to optimise cost performance and drive long-term value creation. Sets the vision and direction for cost management across the organisation."""@en .

sfialevels:COPL_2 a sfia:SkillLevel ;
    skos:notation "COPL_2" ;
    sfia:level lor:2 ;
    sfia:skillLevelDescription """Maintains records of all related testing and training and ensures the availability of all documentation.
Records the actions taken and the consequences following an incident or live testing of a continuity plan for a lessons-learned report."""@en .

sfialevels:COPL_3 a sfia:SkillLevel ;
    skos:notation "COPL_3" ;
    sfia:level lor:3 ;
    sfia:skillLevelDescription """Applies a structured approach to develop and document the detail for a continuity plan. 
Maintains documentation of business continuity and disaster recovery plans. 
Supports the development of a test plan and implementation of continuity management exercises."""@en .

sfialevels:COPL_4 a sfia:SkillLevel ;
    skos:notation "COPL_4" ;
    sfia:level lor:4 ;
    sfia:skillLevelDescription """Contributes to the development of continuity management plans. 
Identifies information and communication systems that support critical business processes. 
Coordinates the business impact analysis and the assessment of risks.  
Coordinates the planning, designing and testing of contingency plans."""@en .

sfialevels:COPL_5 a sfia:SkillLevel ;
    skos:notation "COPL_5" ;
    sfia:level lor:5 ;
    sfia:skillLevelDescription """Manages the development, implementation and testing of continuity management plans.  
Manages the relationship with individuals and teams who have authority for critical business processes and supporting systems. 
Evaluates the critical risks and identifies priority areas for improvement. 
Tests continuity management plans and procedures to ensure they address exposure to risk and that agreed levels of continuity can be maintained."""@en .

sfialevels:COPL_6 a sfia:SkillLevel ;
    skos:notation "COPL_6" ;
    sfia:level lor:6 ;
    sfia:skillLevelDescription """Sets the strategy for continuity management across the organisation. 
Secures organisational commitment, funding and resources for continuity management. 
Leads continuity management exercises. 
Communicates the policy, governance, scope and roles involved in continuity management. Has defined authority and accountability for the actions and decisions for continuity management"""@en .

sfialevels:CPMG_2 a sfia:SkillLevel ;
    skos:notation "CPMG_2" ;
    sfia:level lor:2 ;
    sfia:skillLevelDescription """Assists in monitoring service component capacity and performance under routine guidance and supervision.
Collects and reports data on resource utilisation and capacity metrics. 
Supports the implementation of capacity management procedures and practices."""@en .

sfialevels:CPMG_3 a sfia:SkillLevel ;
    skos:notation "CPMG_3" ;
    sfia:level lor:3 ;
    sfia:skillLevelDescription """Monitors service component capacity and performance, identifying potential issues and escalating as necessary. 
Applies standard procedures to manage demand and capacity. 
Participates in capacity modelling and forecasting activities, providing input and recommendations. 
Supports the implementation of capacity management tools and techniques."""@en .

sfialevels:CPMG_4 a sfia:SkillLevel ;
    skos:notation "CPMG_4" ;
    sfia:level lor:4 ;
    sfia:skillLevelDescription """Monitors service component capacity and initiates actions to resolve any shortfalls according to agreed procedures. 
Applies techniques to control the demand upon a particular resource or service. 
Contributes to capacity modelling and planning using data-driven insights.
Supports the design of service component capacity."""@en .

sfialevels:CPMG_5 a sfia:SkillLevel ;
    skos:notation "CPMG_5" ;
    sfia:level lor:5 ;
    sfia:skillLevelDescription """Manages capacity modelling and forecasting activities, using data-driven insights.
Proactively reviews information in conjunction with service level agreements to identify any capacity issues and specifies any required changes. Provides advice to support the design of service components, including designing in flexible and scalable capacity. 
Works with business representatives to agree and implement short- and medium-term modifications to capacity. 
Drafts and maintains standards and procedures for service component capacity management. Ensures the correct implementation of standards and procedures."""@en .

sfialevels:CPMG_6 a sfia:SkillLevel ;
    skos:notation "CPMG_6" ;
    sfia:level lor:6 ;
    sfia:skillLevelDescription """Leads the development and implementation of policy and strategies for capacity and performance management to meet business needs. 
Leads capacity modelling and forecasting over the organisation's planning or budgeting cycle using data-driven insights. Considers external factors and industry trends.
Ensures policies and standards for capacity management are fit for purpose, current and correctly implemented. Drives continuous improvement in capacity management practices, focusing on cost-effectiveness and resource optimisation.
Reviews new business proposals and provides specialist advice on capacity issues."""@en .

sfialevels:CRIM_2 a sfia:SkillLevel ;
    skos:notation "CRIM_2" ;
    sfia:level lor:2 ;
    sfia:skillLevelDescription """Assists in cybercrime investigations under routine supervision. 
Supports the collection of evidence related to cybercrime investigations. 
Participates in monitoring suspicious activities.
Helps maintain evidence integrity and assists in preliminary interviews. Follows established protocols and guidelines."""@en .

sfialevels:CRIM_3 a sfia:SkillLevel ;
    skos:notation "CRIM_3" ;
    sfia:level lor:3 ;
    sfia:skillLevelDescription """Conducts cybercrime investigations using standard procedures. 
Collects and preserves various forms of evidence in cybercrime cases. Assesses credibility and checks for compliance with relevant investigative standards. 
Analyses basic cyber threats and incidents, and prepares investigative reports. Identifies incidents that may have legal implications. 
Conducts interviews and assists in interrogations."""@en .

sfialevels:CRIM_4 a sfia:SkillLevel ;
    skos:notation "CRIM_4" ;
    sfia:level lor:4 ;
    sfia:skillLevelDescription """Oversees mid-level investigations, coordinating evidence collection and forensic analyses.
Assesses target vulnerabilities and operational impacts of cyber incidents.
Provides comprehensive reports and expert analysis for stakeholders. 
Conducts interviews and interrogations, identifying potential legal implications and collaborating with legal professionals."""@en .

sfialevels:CRIM_5 a sfia:SkillLevel ;
    skos:notation "CRIM_5" ;
    sfia:level lor:5 ;
    sfia:skillLevelDescription """Manages complex cybercrime investigations, overseeing all stages from detection to resolution. 
Evaluates incidents involving advanced threats or significant breaches. 
Develops and implements procedures for evidence handling and documentation. Collaborates with legal teams to ensure evidence supports potential legal proceedings. 
Leads the development of response strategies, assessing vulnerabilities and operational capabilities. Oversees the implementation of tools and automation to enhance investigative processes."""@en .

sfialevels:CRIM_6 a sfia:SkillLevel ;
    skos:notation "CRIM_6" ;
    sfia:level lor:6 ;
    sfia:skillLevelDescription """Defines the organisational strategy for cybercrime investigations.
Establishes policies and standards for handling various forms of evidence in cybercrime cases, including the adoption and integration of tools and automation to improve efficiency and accuracy.
Oversees high-risk or sensitive investigations, managing cross-disciplinary teams. Conducts high-level interviews and interrogations, providing strategic insights on cybersecurity threats and vulnerabilities.
Engages with external stakeholders, including regulatory bodies and legal entities, to ensure compliance with legal and ethical standards."""@en .

sfialevels:CSMG_1 a sfia:SkillLevel ;
    skos:notation "CSMG_1" ;
    sfia:level lor:1 ;
    sfia:skillLevelDescription """Receives and handles routine customer inquiries and requests, following established procedures.
Accurately records customer interactions and maintains relevant records.
Escalates complex issues to appropriate team members or departments."""@en .

sfialevels:CSMG_2 a sfia:SkillLevel ;
    skos:notation "CSMG_2" ;
    sfia:level lor:2 ;
    sfia:skillLevelDescription """Responds to common customer service requests, providing information to enable fulfilment or resolution.
Allocates unresolved calls, requests, or issues to appropriate functions.
Contributes to the maintenance of customer service knowledge bases and documentation.
Assists in monitoring customer satisfaction metrics."""@en .

sfialevels:CSMG_3 a sfia:SkillLevel ;
    skos:notation "CSMG_3" ;
    sfia:level lor:3 ;
    sfia:skillLevelDescription """Acts as a routine contact point for customers, handling a wide range of inquiries and service requests.
Performs initial investigation and diagnosis of customer issues, resolving them where possible or escalating as needed.
Contributes to the development of service standards and procedures.
Assists in analysing service performance data and identifying areas for improvement."""@en .

sfialevels:CSMG_4 a sfia:SkillLevel ;
    skos:notation "CSMG_4" ;
    sfia:level lor:4 ;
    sfia:skillLevelDescription """Monitors service delivery across multiple channels and analyses performance data.
Contributes to the development and implementation of service standards and procedures. Provides technical and procedural guidance to team members.
Identifies trends in customer inquiries and service issues, recommending process improvements.
Collaborates with other departments to enhance the overall customer experience."""@en .

sfialevels:CSMG_5 a sfia:SkillLevel ;
    skos:notation "CSMG_5" ;
    sfia:level lor:5 ;
    sfia:skillLevelDescription """Manages day-to-day operations of the customer service function, including resource planning and work allocation.
Develops and implements service standards, policies and procedures. Analyses service metrics and customer feedback to drive continuous improvement initiatives.
Ensures the service catalogue is comprehensive, up-to-date and aligned with organisational goals.
Develops approaches to enhance customer satisfaction."""@en .

sfialevels:CSMG_6 a sfia:SkillLevel ;
    skos:notation "CSMG_6" ;
    sfia:level lor:6 ;
    sfia:skillLevelDescription """Shapes the strategic direction for customer service across the organisation.
Defines service channels, service levels, standards and the monitoring process for customer service or service desk staff. Champions the service culture required to deliver organisational outcomes.
Leads the development and implementation of organisational frameworks for complaints, service standards and operational agreements.
Takes responsibility for business continuity and legal, regulatory and contractual compliance."""@en .

sfialevels:CSOP_2 a sfia:SkillLevel ;
    skos:notation "CSOP_2" ;
    sfia:level lor:2 ;
    sfia:skillLevelDescription """Processes applications for certification. 
Logs complaints.
Assists with the preparation and organisation of credential materials.
Supports the creation and maintenance of credentials or certificates and helps resolve routine problems during the certification lifecycle."""@en .

sfialevels:CSOP_3 a sfia:SkillLevel ;
    skos:notation "CSOP_3" ;
    sfia:level lor:3 ;
    sfia:skillLevelDescription """Issues certifications or credentials and maintains and retains certification records. 
Maintains information on the certification scheme and a general description of the certification process. 
Designs, creates, develops, customises and maintains credentials or certificates. 
Responds to public information requests. Analyses and acts on complaints or issues."""@en .

sfialevels:CSOP_4 a sfia:SkillLevel ;
    skos:notation "CSOP_4" ;
    sfia:level lor:4 ;
    sfia:skillLevelDescription """Documents instructions for all personnel involved in certification, including legally enforceable agreements with any third parties involved in the process. 
Identifies threats to impartiality by analysing, mitigating or eliminating potential conflict of interests arising from certification activities. 
Implements the procedures for certification of individuals for the delivery of training. 
Determines the merits of complaints and any remedial actions required."""@en .

sfialevels:CSOP_5 a sfia:SkillLevel ;
    skos:notation "CSOP_5" ;
    sfia:level lor:5 ;
    sfia:skillLevelDescription """Defines a certification or accreditation scheme, including organisation structure, duties, responsibilities and authorities. 
Determines necessary competence to perform certification functions. Designs and implements the examiner or assessor selection and approval process. 
Monitors performance and judgements, and agrees corrective actions. Plans and provides adequate premises, equipment and resources. 
Documents policies and procedures for maintenance and release of information, including consideration of any legal agreements for confidentiality."""@en .

sfialevels:CSOP_6 a sfia:SkillLevel ;
    skos:notation "CSOP_6" ;
    sfia:level lor:6 ;
    sfia:skillLevelDescription """Sets policies and standards for the operation of a certification scheme, including segregation of duties and addressing impartiality. 
Develops and maintains a description of the code of ethics and professional practices required. 
Aligns certification schemes with relevant external standards, frameworks such as SFIA and established industry practices. 
Obtains approval from accreditation scheme owners or governance bodies."""@en .

sfialevels:DAAN_2 a sfia:SkillLevel ;
    skos:notation "DAAN_2" ;
    sfia:level lor:2 ;
    sfia:skillLevelDescription """Assists in data preparation and analysis activities under direction. 
Processes and validates data to support analytics. 
Generates standard reports and insights using established tools and methods."""@en .

sfialevels:DAAN_3 a sfia:SkillLevel ;
    skos:notation "DAAN_3" ;
    sfia:level lor:3 ;
    sfia:skillLevelDescription """Supports data analytics by gathering and preparing data from multiple sources. 
Applies analytical and statistical methods and software tools to analyse data and develop reports. 
Assists in identifying trends, patterns and insights that inform business decisions. 
Collaborates with team members to refine analysis techniques and maintain data quality."""@en .

sfialevels:DAAN_4 a sfia:SkillLevel ;
    skos:notation "DAAN_4" ;
    sfia:level lor:4 ;
    sfia:skillLevelDescription """Conducts end-to-end data analysis, defining data requirements and ensuring data integrity. 
Applies advanced analytical and statistical techniques to extract meaningful insights and develop predictive models.
Communicates complex findings to stakeholders in an understandable manner. 
Contributes to the development of data analytics processes and standards. Identifies opportunities for improving data analytics practices."""@en .

sfialevels:DAAN_5 a sfia:SkillLevel ;
    skos:notation "DAAN_5" ;
    sfia:level lor:5 ;
    sfia:skillLevelDescription """Manages data analytics activities, establishing frameworks and methodologies aligned with business objectives and data governance policies. 
Leads the implementation of data analytics solutions. Translates business needs into analytics requirements and identifies data-driven solutions. 
Guides the selection and application of advanced analytical techniques. 
Communicates insights and recommendations to senior stakeholders, influencing strategic decisions."""@en .

sfialevels:DAAN_6 a sfia:SkillLevel ;
    skos:notation "DAAN_6" ;
    sfia:level lor:6 ;
    sfia:skillLevelDescription """Develops organisational strategies and roadmaps for data analytics. 
Sets policies, standards and recommended practices for the use of data and data analytical techniques.
Leads initiatives to build data analytics capabilities and develop a data-driven culture.
Oversees the delivery of analytics projects and programmes. Promotes the ethical use of data and data analytics."""@en .

sfialevels:DAAN_7 a sfia:SkillLevel ;
    skos:notation "DAAN_7" ;
    sfia:level lor:7 ;
    sfia:skillLevelDescription """Directs the creation and review of a cross-functional, enterprise-wide approach and culture for generating value from data analytics and data science. 
Drives the identification, evaluation and adoption of data analytics and data science capabilities to transform organisational performance. Leads the provision of the organisation's data analytics and data science capabilities.
Ensures the strategic application of data analytics and data science is embedded in the governance and leadership of the organisation. 
Aligns business strategies, enterprise transformation and data analytics and data science strategies."""@en .

sfialevels:DATM_2 a sfia:SkillLevel ;
    skos:notation "DATM_2" ;
    sfia:level lor:2 ;
    sfia:skillLevelDescription """Assists in implementing data management activities under close guidance and supervision.
Helps create and maintain documentation of data management activities. 
Helps identify and report issues and discrepancies."""@en .

sfialevels:DATM_3 a sfia:SkillLevel ;
    skos:notation "DATM_3" ;
    sfia:level lor:3 ;
    sfia:skillLevelDescription """Implements standard data management practices based on detailed organisational requirements.
Monitors and maintains data quality through regular reviews and validation checks.    
Communicates the details of data management procedures to others, helping with their understanding and compliance."""@en .

sfialevels:DATM_4 a sfia:SkillLevel ;
    skos:notation "DATM_4" ;
    sfia:level lor:4 ;
    sfia:skillLevelDescription """Devises and implements data governance and master data management processes for specific subsets of data. 
Assesses the integrity of data from multiple sources. 
Advises on transformation of data between formats or media. Maintains and implements data handling procedures. 
Enables data availability, integrity and searchability through formal data and metadata structures and protection measures."""@en .

sfialevels:DATM_5 a sfia:SkillLevel ;
    skos:notation "DATM_5" ;
    sfia:level lor:5 ;
    sfia:skillLevelDescription """Devises and implements data governance and master data management processes. 
Derives data management structures and metadata to support consistent data retrieval, integration, analysis, pattern recognition and interpretation across the organisation.
Independently validates external information from multiple sources.  Plans effective data storage, sharing and publishing practices within the organisation.
Identifies and addresses issues preventing optimal use of information assets. Provides expert advice to maximise data asset value, ensuring data quality and compliance."""@en .

sfialevels:DATM_6 a sfia:SkillLevel ;
    skos:notation "DATM_6" ;
    sfia:level lor:6 ;
    sfia:skillLevelDescription """Leads the strategic direction for data management and data governance, establishing policies and frameworks that align with business and regulatory requirements. Derives an overall strategy of master data management that supports the development and secure operation of data and digital services. 
Creates organisational policies, standards and guidelines for data management, ensuring ethical principles are applied.
Plans, establishes and manages processes for regular and consistent access to external data sources, ensuring their validation and integration."""@en .

sfialevels:DATS_2 a sfia:SkillLevel ;
    skos:notation "DATS_2" ;
    sfia:level lor:2 ;
    sfia:skillLevelDescription """Under routine supervision, applies specified data science techniques to data.
Analyses and reports findings and addresses simple issues, using algorithms included within standard software frameworks and tools."""@en .

sfialevels:DATS_3 a sfia:SkillLevel ;
    skos:notation "DATS_3" ;
    sfia:level lor:3 ;
    sfia:skillLevelDescription """Applies standard data science techniques to new problems and datasets using specialised programming techniques.
Identifies and selects appropriate data sources and prepares data to be used by data science models.
Evaluates the outcomes and performance of data science models. Identifies and implements opportunities to train and improve models and the data they use. 
Publishes and reports on model outputs to meet customer needs and conform to agreed standards."""@en .

sfialevels:DATS_4 a sfia:SkillLevel ;
    skos:notation "DATS_4" ;
    sfia:level lor:4 ;
    sfia:skillLevelDescription """Investigates problems and datasets to assess the usefulness of data science solutions. 
Applies diverse data science techniques and specialised programming languages. Understands and applies rules and guidelines specific to the industry and business, and anticipates risks and other implications of modelling.
Selects, acquires and integrates data for analysis. Formulates hypotheses and evaluates data science models. Advises on the effectiveness of specific techniques based on analysis findings and research. 
Contributes to the development, evaluation, monitoring and deployment of data science solutions."""@en .

sfialevels:DATS_5 a sfia:SkillLevel ;
    skos:notation "DATS_5" ;
    sfia:level lor:5 ;
    sfia:skillLevelDescription """Plans, coordinates and drives all stages of the development of data science solutions. 
Provides expert advice to evaluate the problems to be solved and the need for data science solutions. Identifies and justifies what data sources to use or acquire. 
Specifies and applies appropriate data science techniques and specialised programming languages.
Critically reviews the benefits and value of data science techniques and tools and recommends improvements. Contributes to developing policy, standards and guidelines for developing, evaluating, monitoring and deploying data science solutions."""@en .

sfialevels:DATS_6 a sfia:SkillLevel ;
    skos:notation "DATS_6" ;
    sfia:level lor:6 ;
    sfia:skillLevelDescription """Champions and leads the introduction and use of data science to drive innovation and business value. 
Develops and drives adoption of and adherence to organisational policies, standards, guidelines and methods for data science.
Sets direction and leads in the introduction and use of data science techniques, methodologies and tools. Leads the development of organisational capabilities for data science. 
Plans and leads strategic, large and complex data science initiatives to generate insights, create value and drive decision-making."""@en .

sfialevels:DBAD_2 a sfia:SkillLevel ;
    skos:notation "DBAD_2" ;
    sfia:level lor:2 ;
    sfia:skillLevelDescription """Executes operational procedures, runs automation scripts and performs routine maintenance and monitoring of databases.
Adjusts automation tasks as instructed to meet operational standards for databases.
Reports on database performance, addresses issues directly when possible, or escalates to others for resolution."""@en .

sfialevels:DBAD_3 a sfia:SkillLevel ;
    skos:notation "DBAD_3" ;
    sfia:level lor:3 ;
    sfia:skillLevelDescription """Provisions, installs, configures and ensures the maintenance and reliability of databases.
Monitors databases for load, performance and security events. Reports metrics and resolves operational issues.
Executes standard operational procedures, including database backups and restorations.
Automates routine database administration tasks to specifications using standard scripts and tools."""@en .

sfialevels:DBAD_4 a sfia:SkillLevel ;
    skos:notation "DBAD_4" ;
    sfia:level lor:4 ;
    sfia:skillLevelDescription """Applies technical expertise to maintain and optimise databases, executing updates and employing automation tools. Configures tools and/or creates scripts to automate database tasks.
Maintains operational procedures and checks that they are followed, including compliance with security policies. Uses database management tools to monitor load and performance statistics. 
Investigates and enables the resolution of database operational and security issues. Provides reports and proposals for improvement to stakeholders.
Contributes to the planning and implementation of database maintenance and updates. Implements agreed database changes and maintenance routines."""@en .

sfialevels:DBAD_5 a sfia:SkillLevel ;
    skos:notation "DBAD_5" ;
    sfia:level lor:5 ;
    sfia:skillLevelDescription """Provides technical leadership to optimise the performance of databases.
Drives the adoption of tools and automated processes for effective database management and delivery.
Oversees the planning, installation, maintenance and acceptance of new and updated database components and database-based services. Ensures alignment to service expectations, security requirements and other quality standards.
Ensures database operational procedures and documentation are current and effective, tracks and addresses operational issues and reports to stakeholders."""@en .

sfialevels:DBDS_2 a sfia:SkillLevel ;
    skos:notation "DBDS_2" ;
    sfia:level lor:2 ;
    sfia:skillLevelDescription """Assists in creating and documenting detailed database designs under routine supervision. 
Follows established procedures and guidelines. 
Helps create and maintain documentation."""@en .

sfialevels:DBDS_3 a sfia:SkillLevel ;
    skos:notation "DBDS_3" ;
    sfia:level lor:3 ;
    sfia:skillLevelDescription """Interprets installation standards to meet project needs and produces database or data warehouse component specifications. 
Develops physical database or data warehouse design elements, within set policies, to meet data requirements."""@en .

sfialevels:DBDS_4 a sfia:SkillLevel ;
    skos:notation "DBDS_4" ;
    sfia:level lor:4 ;
    sfia:skillLevelDescription """Implements physical database designs to support transactional data requirements for performance and availability. 
Develops and maintains specialist knowledge of database and data warehouse concepts, design principles, architectures, software and facilities. 
Assesses proposed changes to object/data structures and evaluates alternative options. 
Implements data warehouse designs that support business intelligence and data analytics."""@en .

sfialevels:DBDS_5 a sfia:SkillLevel ;
    skos:notation "DBDS_5" ;
    sfia:level lor:5 ;
    sfia:skillLevelDescription """Provides specialist expertise in the design characteristics of database management systems or data warehouse products/services. 
Provides expert guidance in the selection, provision and use of database and data warehouse architectures, software and facilities. 
Ensures design policies optimise transactional data systems for performance and availability while meeting the needs of business intelligence and analytics platforms."""@en .

sfialevels:DCMA_2 a sfia:SkillLevel ;
    skos:notation "DCMA_2" ;
    sfia:level lor:2 ;
    sfia:skillLevelDescription """Assists with the tasks related to granting, monitoring and reporting on physical access controls under routine supervision. 
Follows established procedures and guidelines to support the maintenance of the physical environment. 
Helps create and maintain documentation."""@en .

sfialevels:DCMA_3 a sfia:SkillLevel ;
    skos:notation "DCMA_3" ;
    sfia:level lor:3 ;
    sfia:skillLevelDescription """Monitors compliance against agreed processes and investigates, assesses and resolves incidents of non-compliance, escalating where necessary. 
Processes physical access requests, monitors access control systems and reports on access-related activities."""@en .

sfialevels:DCMA_4 a sfia:SkillLevel ;
    skos:notation "DCMA_4" ;
    sfia:level lor:4 ;
    sfia:skillLevelDescription """Uses data centre management tools to produce management information on power, cooling and space and investigate issues where necessary. 
Carries out routine audit and checks to ensure adherence to policies and procedures. 
Facilitates the implementation of mandatory electrical safety testing."""@en .

sfialevels:DCMA_5 a sfia:SkillLevel ;
    skos:notation "DCMA_5" ;
    sfia:level lor:5 ;
    sfia:skillLevelDescription """Develops and maintains the standards, processes and documentation for data centres. 
Optimises efficiency in the population of data centre space. Ensures adherence to all relevant policies and processes. 
Uses data centre management tools to plan, record and manage installed infrastructure, power, space and cooling capabilities. 
Monitors  usage and actions to meet sustainability targets."""@en .

sfialevels:DCMA_6 a sfia:SkillLevel ;
    skos:notation "DCMA_6" ;
    sfia:level lor:6 ;
    sfia:skillLevelDescription """Sets organisational policies for managing the IT estate, ensuring alignment with recognised industry practices. 
Develops strategies to forecast and fulfil future data centre space requirements.
Takes overall responsibility for adherence to health and safety regulations and electrical safety policies.
Identifies and implements recognised industry practices to align future plans with corporate sustainability targets."""@en .

sfialevels:DEMG_3 a sfia:SkillLevel ;
    skos:notation "DEMG_3" ;
    sfia:level lor:3 ;
    sfia:skillLevelDescription """Manages the routine delivery of small products or services, or specific parts of a larger product or service.
Follows delivery methodologies, tools, and quality processes. Monitors the team's adherence to these practices.
Coordinates team planning processes based on the established priorities of work items. Tracks and reports on delivery progress, risks and issues.
Supports a collaborative and productive working environment, demonstrating appropriate behaviours. Contributes to continuous improvement of delivery processes within the team."""@en .

sfialevels:DEMG_4 a sfia:SkillLevel ;
    skos:notation "DEMG_4" ;
    sfia:level lor:4 ;
    sfia:skillLevelDescription """Manages the delivery of products or services for small to medium-sized initiatives.
Applies appropriate delivery methodologies and tools. Establishes and leads delivery teams, creating a collaborative and productive working environment.
Manages the prioritisation of work items, leads iteration planning processes and ensures value is delivered incrementally throughout the delivery cycle. Communicates delivery progress, risks and issues to stakeholders.
Ensures the quality of deliverables. Participates in reviews and contributes to the continuous improvement of delivery processes within the scope of the team or initiative."""@en .

sfialevels:DEMG_5 a sfia:SkillLevel ;
    skos:notation "DEMG_5" ;
    sfia:level lor:5 ;
    sfia:skillLevelDescription """Leads delivery of products or services for large or complex initiatives.
Adapts delivery approaches based on the context and complexity of the initiative. Provides leadership and guidance to multiple delivery teams. Collaborates with stakeholders to align delivery objectives with business goals. Proactively manages risks, dependencies and changes that may impact delivery.
Ensures optimal allocation of resources and skills across teams. Monitors key delivery metrics, ensuring transparency and visibility.
Drives the continuous improvement of delivery processes and practices across the organisation."""@en .

sfialevels:DEMG_6 a sfia:SkillLevel ;
    skos:notation "DEMG_6" ;
    sfia:level lor:6 ;
    sfia:skillLevelDescription """Defines and oversees the delivery strategy for multiple products or services.
Aligns delivery strategy with organisational goals and customer needs. Ensures effective allocation of resources and budget.
Monitors and reports on performance of product and service delivery, ensuring alignment with objectives. Identifies and mitigates systemic risks and issues.
Sets the direction and standards for delivery management across the organisation. Leads the development of a culture focused on continuous improvement and customer-centricity."""@en .

sfialevels:DEMM_4 a sfia:SkillLevel ;
    skos:notation "DEMM_4" ;
    sfia:level lor:4 ;
    sfia:skillLevelDescription """Performs demand management analysis and planning activities within a specific business or operational area. 
Monitors patterns of demand and identifies insights and proposals to improve business value. 
Identifies and assesses opportunities to prioritise or improve alignment between business demand and capacity to deliver. 
Engages stakeholders to communicate insights, plans and decisions regarding business demand."""@en .

sfialevels:DEMM_5 a sfia:SkillLevel ;
    skos:notation "DEMM_5" ;
    sfia:level lor:5 ;
    sfia:skillLevelDescription """Implements demand management analysis and  planning activities. 
Provides advice to help stakeholders adopt and adhere to the agreed demand management approach. Manages the process of integrating demand management  with complementary strategic, operational and change management processes. 
Maintains a register of business requests and routes requests to the right place. Reports on the status of each request.
Reviews new business proposals and provides advice on demand issues. Works with business representatives to agree and implement short-term and medium-term modifications to demand."""@en .

sfialevels:DEMM_6 a sfia:SkillLevel ;
    skos:notation "DEMM_6" ;
    sfia:level lor:6 ;
    sfia:skillLevelDescription """Defines the approach and sets policies for discovering, analysing, planning, controlling and documenting demand for services and products. 
Organises scoping and business priority setting for strategic business changes involving business policymakers and direction setters. 
Engages with and influences senior stakeholders to improve the business value delivered from new or existing services and products. 
Leads the development of demand management capabilities. Leads the integration of demand management with complementary strategic, operational and change management processes."""@en .

sfialevels:DENG_2 a sfia:SkillLevel ;
    skos:notation "DENG_2" ;
    sfia:level lor:2 ;
    sfia:skillLevelDescription """Assists in developing and implementing data pipelines and data stores. 
Performs administrative tasks to provide data accessibility, retrievability, security and protection.
Supports the monitoring of data pipeline operations, identifying issues and escalating as needed. 
Participates in data migration and conversion tasks under routine supervision."""@en .

sfialevels:DENG_3 a sfia:SkillLevel ;
    skos:notation "DENG_3" ;
    sfia:level lor:3 ;
    sfia:skillLevelDescription """Follows standard approaches and established design patterns to create and implement simple data pipelines and data stores to acquire and prepare data. 
Applies data engineering standards and tools to create and maintain data pipelines and perform extract, transform and load (ETL) processes, incorporating security and data integrity practices.
Contributes to data migration and conversion projects, ensuring data integrity and consistency.
Conducts routine data quality checks and remediation."""@en .

sfialevels:DENG_4 a sfia:SkillLevel ;
    skos:notation "DENG_4" ;
    sfia:level lor:4 ;
    sfia:skillLevelDescription """Designs, implements and maintains complex data engineering solutions to acquire and prepare data. 
Creates and maintains data pipelines to connect data across data stores, applications and organisations.  Builds in compliance with data governance and security standards.
Supports the development of continuous integration and deployment practices.  Monitors and optimises pipeline performance and scalability. 
Conducts complex data quality checking and remediation. Leads data migration and data conversion activities."""@en .

sfialevels:DENG_5 a sfia:SkillLevel ;
    skos:notation "DENG_5" ;
    sfia:level lor:5 ;
    sfia:skillLevelDescription """Plans and drives the development of data engineering solutions, balancing functional and non-functional requirements. 
Monitors application of data standards, architectures and security, ensuring compliance and scalability.
Develops and promotes continuous integration, deployment and monitoring practices.
Contributes to organisational policies, standards and guidelines for data engineering."""@en .

sfialevels:DENG_6 a sfia:SkillLevel ;
    skos:notation "DENG_6" ;
    sfia:level lor:6 ;
    sfia:skillLevelDescription """Leads the selection and development of data engineering methods, tools and techniques. 
Develops organisational policies, standards and guidelines for the development and secure operation of data services and products. 
Ensures adherence to technical strategies and architectures. 
Plans and leads data engineering for strategic, high-impact, large and complex programmes ensuring alignment with organisational objectives and industry practices."""@en .

sfialevels:DEPL_2 a sfia:SkillLevel ;
    skos:notation "DEPL_2" ;
    sfia:level lor:2 ;
    sfia:skillLevelDescription """Assists in deploying software releases and updates under routine supervision.
Executes defined deployment processes and procedures using deployment tools and techniques.
Monitors deployed applications and reports issues. Assists in rolling back deployments when necessary."""@en .

sfialevels:DEPL_3 a sfia:SkillLevel ;
    skos:notation "DEPL_3" ;
    sfia:level lor:3 ;
    sfia:skillLevelDescription """Deploys software releases and updates to production environments.
Uses deployment tools and techniques to ensure consistent deployments. Monitors and troubleshoots deployment processes.
Performs rollbacks of deployments in case of issues or failures.
Collaborates with release management and operations teams."""@en .

sfialevels:DEPL_4 a sfia:SkillLevel ;
    skos:notation "DEPL_4" ;
    sfia:level lor:4 ;
    sfia:skillLevelDescription """Plans and executes deployments of complex software releases and updates.
Manages continuous deployment using automation tools and techniques. Develops and maintains deployment processes, procedures and scripts.
Monitors and optimises deployment processes for efficiency and reliability. Ensures the availability, performance and security of deployed applications.
Collaborates with cross-functional teams."""@en .

sfialevels:DEPL_5 a sfia:SkillLevel ;
    skos:notation "DEPL_5" ;
    sfia:level lor:5 ;
    sfia:skillLevelDescription """Designs and implements deployment approaches, processes and automation tools for the organisation.
Oversees the deployment of critical and large-scale software. Ensures deployment processes align with organisational standards and recommended practices.
Continuously improves deployment processes and automation capabilities.
Defines monitoring and alert strategies for deployed applications."""@en .

sfialevels:DEPL_6 a sfia:SkillLevel ;
    skos:notation "DEPL_6" ;
    sfia:level lor:6 ;
    sfia:skillLevelDescription """Defines organisational deployment strategies, policies and standards.
Aligns deployment practices with overall operations and service delivery goals.
Ensures the availability of resources and tools for effective deployment.
Drives the adoption of new deployment techniques and technologies. Collaborates with senior stakeholders to ensure deployments meet business strategies and objectives."""@en .

sfialevels:DESN_2 a sfia:SkillLevel ;
    skos:notation "DESN_2" ;
    sfia:level lor:2 ;
    sfia:skillLevelDescription """Assists in the creation and documentation of system design elements under routine supervision. 
Follows established procedures and guidelines. 
Helps create and maintain documentation."""@en .

sfialevels:DESN_3 a sfia:SkillLevel ;
    skos:notation "DESN_3" ;
    sfia:level lor:3 ;
    sfia:skillLevelDescription """Follows standard approaches and established design patterns to create new designs for simple systems or system components.
Identifies and resolves minor design issues. 
Identifies alternative design options and seeks guidance when deviating from established design patterns."""@en .

sfialevels:DESN_4 a sfia:SkillLevel ;
    skos:notation "DESN_4" ;
    sfia:level lor:4 ;
    sfia:skillLevelDescription """Designs system components using appropriate modelling techniques following agreed architectures, design standards, patterns and methodology. 
Identifies and evaluates alternative design options and trade-offs. Creates multiple design views to address the concerns of the different stakeholders and to handle functional and non-functional requirements. 
Models, simulates or prototypes the behaviour of proposed system components to enable approval by stakeholders. 
Produces detailed design specifications to form the basis for the construction of systems. Reviews, verifies and improves own designs against specifications."""@en .

sfialevels:DESN_5 a sfia:SkillLevel ;
    skos:notation "DESN_5" ;
    sfia:level lor:5 ;
    sfia:skillLevelDescription """Designs large or complex systems and undertakes impact analysis on major design options and trade-offs. 
Ensures the system design balances functional and non-functional requirements. 
Reviews systems designs and ensures appropriate methods, tools and techniques are applied effectively. Makes recommendations and assesses and manages associated risks. 
Adopts and adapts system design methods, tools and techniques. Contributes to development of system design policies, standards and selection of architecture components."""@en .

sfialevels:DESN_6 a sfia:SkillLevel ;
    skos:notation "DESN_6" ;
    sfia:level lor:6 ;
    sfia:skillLevelDescription """Develops and drives adoption of and adherence to organisational policies, standards, guidelines and methods for system design. 
Champions the importance and value of system design principles and the selection of appropriate systems design lifecycle models. 
Leads system design activities for strategic, large and complex systems development programmes. Develops effective implementation strategies consistent with specified requirements, architectures and constraints of performance and feasibility. 
Develops system design requiring the introduction of new technologies or new uses for existing technologies."""@en .

sfialevels:DGFS_2 a sfia:SkillLevel ;
    skos:notation "DGFS_2" ;
    sfia:level lor:2 ;
    sfia:skillLevelDescription """Assists with digital forensic investigations under routine supervision. 
Supports the recovery of damaged, deleted or hidden data from digital devices.
Helps collect and preserve digital information and evidence according to established protocols."""@en .

sfialevels:DGFS_3 a sfia:SkillLevel ;
    skos:notation "DGFS_3" ;
    sfia:level lor:3 ;
    sfia:skillLevelDescription """Applies standard forensic tools and techniques to examine digital devices. 
Recovers and analyses damaged, deleted or hidden data from various digital sources and devices. 
Maintains the integrity of digital evidence and ensures its collection adheres to legal admissibility standards."""@en .

sfialevels:DGFS_4 a sfia:SkillLevel ;
    skos:notation "DGFS_4" ;
    sfia:level lor:4 ;
    sfia:skillLevelDescription """Designs and executes complex digital forensic examinations. 
Specifies requirements for specialised forensic tools and resources. Provides guidance on advanced data recovery techniques and artefact analysis. 
Processes and analyses digital evidence in line with organisational policies and industry standards. Develops procedures for handling emerging technologies in forensic contexts.
Contributes to forensic reports detailing technical findings."""@en .

sfialevels:DGFS_5 a sfia:SkillLevel ;
    skos:notation "DGFS_5" ;
    sfia:level lor:5 ;
    sfia:skillLevelDescription """Leads investigations to correctly gather, analyse and present findings, including digital evidence, to both business and legal audiences.
Collates conclusions and recommendations and presents forensic findings to stakeholders.
Plans and manages digital forensics activities within the organisation. Provides expert advice on digital forensics.
Contributes to the development of digital forensics policies, standards and guidelines. Evaluates and selects digital forensics tools and techniques."""@en .

sfialevels:DGFS_6 a sfia:SkillLevel ;
    skos:notation "DGFS_6" ;
    sfia:level lor:6 ;
    sfia:skillLevelDescription """Plans and leads the organisation's approach to digital forensics.
Sets policies, standards and guidelines for how the organisation conducts digital forensic investigations.
Leads and manages high risk, large or wide-ranging digital forensics investigations engaging additional specialists if required.
Authorises the release of formal forensic reports. Engages with external stakeholders on forensic matters."""@en .

sfialevels:DIGM_2 a sfia:SkillLevel ;
    skos:notation "DIGM_2" ;
    sfia:level lor:2 ;
    sfia:skillLevelDescription """Performs basic digital marketing tasks under routine supervision. 
Assists in the implementation of digital marketing campaigns across various platforms. 
Collects and organises basic performance data from digital marketing activities. 
Contributes to the creation and distribution of digital marketing content following established guidelines."""@en .

sfialevels:DIGM_3 a sfia:SkillLevel ;
    skos:notation "DIGM_3" ;
    sfia:level lor:3 ;
    sfia:skillLevelDescription """Implements digital marketing activities across multiple channels. 
Monitors campaign performance and makes basic optimisations. 
Assists in the development of digital marketing content. Follows procedures to comply with regulatory requirements and platform policies.
Contributes to the analysis of marketing metrics and prepares reports. Supports the planning and execution of marketing performance improvement initiatives."""@en .

sfialevels:DIGM_4 a sfia:SkillLevel ;
    skos:notation "DIGM_4" ;
    sfia:level lor:4 ;
    sfia:skillLevelDescription """Plans and executes digital marketing activities across various platforms. 
Analyses detailed marketing data to derive insights and improve campaign performance. Recommends and implements improvements to digital marketing activities based on performance data.
Manages relationships with digital marketing vendors and platform representatives. 
Leads the implementation of marketing automation processes. Applies organisational guidelines and uses appropriate tools to ensure digital marketing activities adhere to relevant regulations and platform policies."""@en .

sfialevels:DIGM_5 a sfia:SkillLevel ;
    skos:notation "DIGM_5" ;
    sfia:level lor:5 ;
    sfia:skillLevelDescription """Leads the development and implementation of comprehensive digital marketing plans. 
Oversees the integration with broader marketing and business objectives. Manages budgets and resources for digital marketing initiatives. 
Provides guidance on recognised good practices for digital marketing and emerging trends to stakeholders across the organisation. Evaluates and recommends new digital marketing technologies and approaches. Establishes and maintains strategic relationships with digital marketing vendors and platform representatives. 
Develops standards and procedures for compliant digital marketing practices."""@en .

sfialevels:DLMG_4 a sfia:SkillLevel ;
    skos:notation "DLMG_4" ;
    sfia:level lor:4 ;
    sfia:skillLevelDescription """Contributes to the planning and management of systems development work.
Adopts and applies appropriate systems development methods, tools and techniques in line with agreed standards. 
Engages with stakeholders to ensure systems development deliverables meet requirements and quality expectations. Manages risks and issues related to systems development activities, escalating as needed. 
Contributes to the continuous improvement of systems development processes and practices."""@en .

sfialevels:DLMG_5 a sfia:SkillLevel ;
    skos:notation "DLMG_5" ;
    sfia:level lor:5 ;
    sfia:skillLevelDescription """Plans and drives systems development work to deliver the organisation's objectives and plans. 
Selects, adopts and adapts appropriate systems development methods, tools and techniques. Ensures stakeholders are aware of required resources and that they are made available. Facilitates availability and optimum utilisation of resources. 
Monitors and reports on the progress of development projects. Ensures projects are carried out in accordance with agreed architectures, standards, methods and tools and addresses security and privacy requirements. 
Develops roadmaps to communicate future development activity."""@en .

sfialevels:DLMG_6 a sfia:SkillLevel ;
    skos:notation "DLMG_6" ;
    sfia:level lor:6 ;
    sfia:skillLevelDescription """Sets policy and drives adherence to standards for systems development. 
Leads activities to make security and privacy integral to systems development. 
Identifies and manages the resources necessary for all stages of systems development projects. 
Ensures technical, financial and quality targets are met."""@en .

sfialevels:DLMG_7 a sfia:SkillLevel ;
    skos:notation "DLMG_7" ;
    sfia:level lor:7 ;
    sfia:skillLevelDescription """Directs the definition, implementation and continual improvement of the organisation's systems development management framework. 
Aligns systems development to business strategies and objectives and with emerging technology and digital opportunities. Maintains an overview of the contribution of systems development programmes to organisational success.
Authorises the structure of systems development functions and platforms. 
Sets strategy for resource management within systems development and authorises the allocation of resources for systems development programmes."""@en .

sfialevels:DTAN_2 a sfia:SkillLevel ;
    skos:notation "DTAN_2" ;
    sfia:level lor:2 ;
    sfia:skillLevelDescription """Establishes, modifies or maintains simple data structures and associated components. 
Uses specific data modelling and design techniques under guidance."""@en .

sfialevels:DTAN_3 a sfia:SkillLevel ;
    skos:notation "DTAN_3" ;
    sfia:level lor:3 ;
    sfia:skillLevelDescription """Applies standard data modelling and design techniques based upon a detailed understanding of organisational requirements. 
Establishes, modifies and maintains data structures and associated components. 
Communicates and explain the details of data structures and components to others."""@en .

sfialevels:DTAN_4 a sfia:SkillLevel ;
    skos:notation "DTAN_4" ;
    sfia:level lor:4 ;
    sfia:skillLevelDescription """Investigates enterprise data requirements where there is some complexity and ambiguity.  
Plans data modelling and design activities, selecting appropriate techniques and levels of detail to meet objectives. 
Provides advice and guidance to others using the data structures and associated components."""@en .

sfialevels:DTAN_5 a sfia:SkillLevel ;
    skos:notation "DTAN_5" ;
    sfia:level lor:5 ;
    sfia:skillLevelDescription """Sets standards for data modelling and design tools and techniques, advises on their application and ensures compliance. 
Manages the investigation of enterprise data requirements based on a detailed understanding of information requirements. 
Coordinates the application of analysis, design and modelling techniques to establish, modify or maintain data structures and their associated components. 
Manages the iteration, review and maintenance of data requirements and data models."""@en .

sfialevels:EEXP_4 a sfia:SkillLevel ;
    skos:notation "EEXP_4" ;
    sfia:level lor:4 ;
    sfia:skillLevelDescription """Supports assigned co-workers by providing guidance on areas such as organisational contacts, communication channels, processes, job expectations and manager relations.
Helps individuals navigate areas of uncertainty, offering practical advice and connecting them with the appropriate resources when needed."""@en .

sfialevels:EEXP_5 a sfia:SkillLevel ;
    skos:notation "EEXP_5" ;
    sfia:level lor:5 ;
    sfia:skillLevelDescription """Implements working practices that motivate employees and support their health and wellbeing. 
Provides guidance to individuals on long-term development goals and career opportunities, considering an individual's strengths and preferences. 
Communicates business direction, policy and purpose where these may drive or affect employee engagement. Ensures clear communication of delegated tasks and provides sufficient autonomy to motivate and empower individuals.
Maintains awareness of the physical and emotional welfare of employees, and provides counselling when required."""@en .

sfialevels:EEXP_6 a sfia:SkillLevel ;
    skos:notation "EEXP_6" ;
    sfia:level lor:6 ;
    sfia:skillLevelDescription """Leads on the implementation of organisational strategies for employee engagement.
Ensures managers provide a productive working environment that motivates employees and supports their health and wellbeing. 
Initiates productive working practices for remote, virtual and onsite working and ensures the availability of support for employees. 
Communicates and promotes policies for employee health and wellbeing."""@en .

sfialevels:EMRG_4 a sfia:SkillLevel ;
    skos:notation "EMRG_4" ;
    sfia:level lor:4 ;
    sfia:skillLevelDescription """Supports monitoring of the external environment and assessment of emerging technologies. 
Contributes to the creation of reports, technology roadmapping and the sharing of knowledge and insights."""@en .

sfialevels:EMRG_5 a sfia:SkillLevel ;
    skos:notation "EMRG_5" ;
    sfia:level lor:5 ;
    sfia:skillLevelDescription """Monitors the external environment to gather intelligence on emerging technologies. 
Assesses and documents the impacts, threats and opportunities to the organisation. 
Creates reports and technology roadmaps and shares knowledge and insights with others."""@en .

sfialevels:EMRG_6 a sfia:SkillLevel ;
    skos:notation "EMRG_6" ;
    sfia:level lor:6 ;
    sfia:skillLevelDescription """Plans and leads the identification and assessment of emerging technologies and the evaluation of potential impacts, threats and opportunities.
Creates technology roadmaps that align organisational plans with emerging technology solutions. Engages with, and influences, relevant stakeholders to obtain organisational commitment to technology roadmaps. 
Develops organisational guidelines for monitoring emerging technologies. 
Collaborates with internal and external parties to facilitate intelligence gathering."""@en .

sfialevels:ETDL_2 a sfia:SkillLevel ;
    skos:notation "ETDL_2" ;
    sfia:level lor:2 ;
    sfia:skillLevelDescription """Performs a range of learning activities under direction to support the delivery of learning objectives. 
Assists in the preparation of learning environments. 
Observes learners performing practical activities and work, providing assistance with routine enquiries and escalating where needed."""@en .

sfialevels:ETDL_3 a sfia:SkillLevel ;
    skos:notation "ETDL_3" ;
    sfia:level lor:3 ;
    sfia:skillLevelDescription """Delivers learning activities to various audiences using prepared materials aligned with established learning objectives. 
Follows established guidelines to prepare the learning environment. Assists in developing and maintaining relevant examples and case studies.
Uses a range of delivery techniques to develop learner skills and knowledge. 
Observes learners performing practical activities and work. Advises and assists where necessary. Provides detailed instruction where necessary and responds to questions, seeking advice in exceptional conditions beyond own experience."""@en .

sfialevels:ETDL_4 a sfia:SkillLevel ;
    skos:notation "ETDL_4" ;
    sfia:level lor:4 ;
    sfia:skillLevelDescription """Prepares and delivers learning activities tailored to various audiences and specific learning objectives.
Contributes to the design and selection of appropriate environments. Uses a broad range of learning delivery techniques to build learner skills and knowledge. Develops and updates examples and case study materials.
Observes and evaluates learner performance, offering guidance and tailored instruction. 
Adjusts delivery approaches and materials to enhance learner experience, responding to specialised queries and ensuring objectives are met."""@en .

sfialevels:ETDL_5 a sfia:SkillLevel ;
    skos:notation "ETDL_5" ;
    sfia:level lor:5 ;
    sfia:skillLevelDescription """Manages the delivery of programmes of learning to ensure learning objectives are met. 
Plans and schedules the delivery of learning activities. Leads the design and selection of appropriate environments to support and enhance the learning experience. Customises learning activities incorporating relevant scenarios and case studies. 
Delivers learning activities to specialist audiences requiring the application of advanced technical and professional principles to unpredictable situations. Advises others in learning delivery techniques and options.
Evaluates and monitors the performance of learning delivery activities."""@en .

sfialevels:ETMG_2 a sfia:SkillLevel ;
    skos:notation "ETMG_2" ;
    sfia:level lor:2 ;
    sfia:skillLevelDescription """Supports learning and development activities under routine supervision. 
Assists in maintaining training records and documenting learning and development activities. 
Helps organise learning events and track attendance."""@en .

sfialevels:ETMG_3 a sfia:SkillLevel ;
    skos:notation "ETMG_3" ;
    sfia:level lor:3 ;
    sfia:skillLevelDescription """Contributes to the maintenance of training records and the catalogue of learning and development resources.
Supports the organisation of learning events by helping to coordinate logistics, schedules, and communication with attendees.
Supports the collection and organisation of data on learning and development activities to assist in evaluating their effectiveness."""@en .

sfialevels:ETMG_4 a sfia:SkillLevel ;
    skos:notation "ETMG_4" ;
    sfia:level lor:4 ;
    sfia:skillLevelDescription """Contributes to the development and maintenance of a catalogue of learning and development resources. 
Uses data to analyse and evaluate the effectiveness of learning/educational activities. 
Books and organises learning events. 
Updates and controls training records, including attainment of certificates and accreditations."""@en .

sfialevels:ETMG_5 a sfia:SkillLevel ;
    skos:notation "ETMG_5" ;
    sfia:level lor:5 ;
    sfia:skillLevelDescription """Manages the provision of learning and development, ensuring optimum use of resources. 
Maintains, publicises and promotes a catalogue of learning and development activities. Ensures courses are up to date and accredited (when required). 
Arranges facilities and schedules with learning and development providers as appropriate. 
Uses data to assess and improve the effectiveness of learning or educational activities."""@en .

sfialevels:ETMG_6 a sfia:SkillLevel ;
    skos:notation "ETMG_6" ;
    sfia:level lor:6 ;
    sfia:skillLevelDescription """Determines the learning and development programme and delivery mechanisms needed to grow staff skills in line with business needs.
Identifies appropriate accreditation and qualification paths applicable to individuals within the organisation.
Evaluates learning outcomes. 
Manages the development and provision of all learning, taking account of the strategic aims of the employing organisation."""@en .

sfialevels:ETMG_7 a sfia:SkillLevel ;
    skos:notation "ETMG_7" ;
    sfia:level lor:7 ;
    sfia:skillLevelDescription """Directs the development and implementation of a learning and development strategy for the organisation aligned to business needs. 
Leads the provision of learning and development expertise, guidance and systems needed to execute strategic and operational plans. 
Secures organisational resources to execute the learning and development strategy. 
Identifies opportunities for strategic relationships with suppliers and partners."""@en .

sfialevels:FEAS_2 a sfia:SkillLevel ;
    skos:notation "FEAS_2" ;
    sfia:level lor:2 ;
    sfia:skillLevelDescription """Assists in feasibility assessment tasks under routine supervision. 
Helps gather information required for feasibility assessments. 
Supports the identification and documentation of options for business change."""@en .

sfialevels:FEAS_3 a sfia:SkillLevel ;
    skos:notation "FEAS_3" ;
    sfia:level lor:3 ;
    sfia:skillLevelDescription """Supports option identification and feasibility assessment.
Selects and employs standard techniques to get the information required for feasibility assessment. 
Supports identification of tangible costs and benefits, and development of business cases."""@en .

sfialevels:FEAS_4 a sfia:SkillLevel ;
    skos:notation "FEAS_4" ;
    sfia:level lor:4 ;
    sfia:skillLevelDescription """Selects relevant feasibility assessment approaches and techniques. 
Identifies the range of possible options. Undertakes short-listing of options and feasibility assessment. 
Engages with internal and external stakeholders to get the information required for feasibility assessment. 
Supports preparation of business cases including cost/benefit, impact and risk analysis for each option."""@en .

sfialevels:FEAS_5 a sfia:SkillLevel ;
    skos:notation "FEAS_5" ;
    sfia:level lor:5 ;
    sfia:skillLevelDescription """Manages investigative work to enable feasibility assessments. 
Collaborates with stakeholders and specialists to get the information required for feasibility assessment. 
Advises on the selection of feasibility assessment approaches and techniques relevant to the business situation and options. 
Prepares business cases, including cost/benefit, impact and risk analysis for each option."""@en .

sfialevels:FEAS_6 a sfia:SkillLevel ;
    skos:notation "FEAS_6" ;
    sfia:level lor:6 ;
    sfia:skillLevelDescription """Establishes an organisational framework and standards for feasibility assessment and business case development. 
Directs and leads feasibility assessments for initiatives that will have a significant impact on the organisation. 
Engages with senior stakeholders to clarify the strategic context for investment options. Directs and leads the selection of feasibility assessment approaches and techniques that are relevant to the business situation and options. 
Presents feasibility assessments and business cases to senior stakeholders and supports decision-making regarding investment options."""@en .

sfialevels:FIAN_2 a sfia:SkillLevel ;
    skos:notation "FIAN_2" ;
    sfia:level lor:2 ;
    sfia:skillLevelDescription """Assists in collecting and organising financial data and preparing basic reports under supervision. 
Supports the financial analysis process by completing assigned tasks and seeking guidance when needed."""@en .

sfialevels:FIAN_3 a sfia:SkillLevel ;
    skos:notation "FIAN_3" ;
    sfia:level lor:3 ;
    sfia:skillLevelDescription """Applies established financial analysis techniques and processes to carry out specific tasks such as detailed data analysis, report generation and interpretation of financial metrics. 
Contributes to the development of actionable insights for decision-making.
Communicates financial analysis findings to relevant stakeholders."""@en .

sfialevels:FIAN_4 a sfia:SkillLevel ;
    skos:notation "FIAN_4" ;
    sfia:level lor:4 ;
    sfia:skillLevelDescription """Performs financial analysis for specific areas, using standard techniques and tools. 
Prepares reports and provides insights to support decision-making. Conducts cost-benefit analyses and supports stakeholder collaboration in the cost management process. 
Collaborates with stakeholders to understand requirements and deliver relevant analysis. 
Supports the development and maintenance of financial models."""@en .

sfialevels:FIAN_5 a sfia:SkillLevel ;
    skos:notation "FIAN_5" ;
    sfia:level lor:5 ;
    sfia:skillLevelDescription """Leads financial analysis activities for a department or function, applying advanced techniques and tools. Develops and maintains complex financial models.
Conducts scenario planning and sensitivity analysis to support decision-making. Provides authoritative advice and guidance on recommended financial analysis practices.
Presents findings and recommendations to senior stakeholders, linking financial performance to business outcomes. Collaborates with stakeholders to align analysis with organisational objectives."""@en .

sfialevels:FIAN_6 a sfia:SkillLevel ;
    skos:notation "FIAN_6" ;
    sfia:level lor:6 ;
    sfia:skillLevelDescription """Defines and leads the organisation's approach to financial analysis, aligning it with strategic objectives and business value creation.
Develops and implements enterprise-wide financial analysis policies, standards and processes. Drives a culture of data-driven decision-making and continuous improvement in financial management.
Provides strategic insights and recommendations based on comprehensive financial analysis, linking performance to business strategy."""@en .

sfialevels:FMIT_4 a sfia:SkillLevel ;
    skos:notation "FMIT_4" ;
    sfia:level lor:4 ;
    sfia:skillLevelDescription """Monitors and maintains financial records to ensure compliance and audit requirements are met.
Provides general support in financial planning and budgeting by compiling and reporting on financial data.
Supports decision-making by collating and summarising financial information at a high level.
Collaborates with business units to gather financial data and understand operational needs."""@en .

sfialevels:FMIT_5 a sfia:SkillLevel ;
    skos:notation "FMIT_5" ;
    sfia:level lor:5 ;
    sfia:skillLevelDescription """Provides general advice and guidance on financial planning, budgeting and accounting using recognised practices and standards.
Develops high-level financial plans and forecasts to guide organisational strategies and plans.
Monitors expenditure to ensure alignment with budgetary goals.
Contributes to financial control frameworks and supports strategic decision-making by summarising expenditure trends and variances."""@en .

sfialevels:FMIT_6 a sfia:SkillLevel ;
    skos:notation "FMIT_6" ;
    sfia:level lor:6 ;
    sfia:skillLevelDescription """Develops organisational policies, standards and guidelines for financial management to support strategic business goals.
Promotes financial governance and drives adherence to financial policies and standards. Collaborates with senior leaders and business unit heads to ensure financial strategies support overall business objectives.
Oversees the setting and management of financial budgets and targets at a strategic level.
Leads high-level reviews of financial performance and implements improvements to align budget usage with organisational priorities."""@en .

sfialevels:GOVN_6 a sfia:SkillLevel ;
    skos:notation "GOVN_6" ;
    sfia:level lor:6 ;
    sfia:skillLevelDescription """Implements the governance framework to enable governance activity to be conducted. 
Within a defined area of accountability, determines the requirements for appropriate governance reflecting the organisation's values, ethics, risk appetite and wider governance frameworks. Communicates delegated authority, benefits, opportunities, costs and risks. 
Leads reviews of governance practices with appropriate and sufficient independence from management activity. 
Acts as the organisation's contact for relevant regulatory authorities and ensures proper relationships between the organisation and external stakeholders."""@en .

sfialevels:GOVN_7 a sfia:SkillLevel ;
    skos:notation "GOVN_7" ;
    sfia:level lor:7 ;
    sfia:skillLevelDescription """Directs the definition, implementation and monitoring of the governance framework to meet organisational obligations under regulation, law, or contracts. 
Provides leadership, direction and oversight for governance activities.  Integrates risk management into frameworks, aligning with strategic objectives and risk appetite.
Secures resources required to execute activities to achieve the organisation's governance goals with effective transparency. 
Provides assurance to stakeholders that the organisation can deliver its obligations with an agreed balance of benefits, opportunities, costs and risks."""@en .

sfialevels:GRDN_1 a sfia:SkillLevel ;
    skos:notation "GRDN_1" ;
    sfia:level lor:1 ;
    sfia:skillLevelDescription """Creates simple visual elements under supervision. 
Applies basic design principles. Uses design software to produce simple graphics. Supports the maintenance of design assets and libraries. 
Participates in design reviews and incorporates feedback. 
Helps with routine tasks such as resizing images, preparing files for print or digital use and organising design assets."""@en .

sfialevels:GRDN_2 a sfia:SkillLevel ;
    skos:notation "GRDN_2" ;
    sfia:level lor:2 ;
    sfia:skillLevelDescription """Assists the creation of visual elements and layouts for digital and print media under routine supervision. 
Applies design principles to produce consistent and effective visuals. Uses design software to create and edit graphics, preparing mock-ups and prototypes. Conforms to brand guidelines and assignment specifications. 
Responds to feedback and research findings to revise designs. 
Participates in research activities to inform design decisions and understand user needs."""@en .

sfialevels:GRDN_3 a sfia:SkillLevel ;
    skos:notation "GRDN_3" ;
    sfia:level lor:3 ;
    sfia:skillLevelDescription """Designs visual concepts and layouts for a range of media. 
Works with stakeholders to understand design requirements. 
Produces high-quality graphics and visual elements using design software. Develops prototypes and iterates based on feedback. Applies brand guidelines and assignment specifications. 
Contributes to the development of design standards and recognised good practices."""@en .

sfialevels:GRDN_4 a sfia:SkillLevel ;
    skos:notation "GRDN_4" ;
    sfia:level lor:4 ;
    sfia:skillLevelDescription """Designs visual concepts and comprehensive designs for complex assignments.
Engages with clients and stakeholders to elicit and document design requirements and goals. Manages design assignments from concept to final delivery. 
Creates detailed design mock-ups and interactive prototypes. Reviews and approves design work, ensuring alignment with brand standards and evidence-based practices. 
Develops and implements design processes, guidelines and recognised good practices to enhance design quality and effectiveness."""@en .

sfialevels:GRDN_5 a sfia:SkillLevel ;
    skos:notation "GRDN_5" ;
    sfia:level lor:5 ;
    sfia:skillLevelDescription """Manages graphic design activities for the organisation, ensuring designs are research-driven and aligned with business objectives. 
Oversees multiple design initiatives, ensuring high-quality, consistent output. Engages with senior stakeholders to align design goals with business objectives and user needs. 
Develops research-informed visual solutions to strengthen brand identity and user experience. 
Leads the creation and adoption of design standards, processes and recognised good practices. Provides authoritative advice on visual design trends and evidence-based practices, ensuring designs meet all required specifications and brand guidelines."""@en .

sfialevels:HCEV_2 a sfia:SkillLevel ;
    skos:notation "HCEV_2" ;
    sfia:level lor:2 ;
    sfia:skillLevelDescription """Assists in creating user experience elements under routine supervision. 
Follows established procedures and guidelines. 
Helps create and maintain documentation."""@en .

sfialevels:HCEV_3 a sfia:SkillLevel ;
    skos:notation "HCEV_3" ;
    sfia:level lor:3 ;
    sfia:skillLevelDescription """Applies standard techniques and tools for designing user interactions with and experiences of selected system, product or service components. 
Reviews design goals and agreed security, usability and accessibility requirements. Creates design artefacts to communicate ideas. 
Contributes to overall user experience design as part of a team.
Assists in evaluating design options and trade-offs. Considers and applies visual design and branding guidelines consistently when appropriate."""@en .

sfialevels:HCEV_4 a sfia:SkillLevel ;
    skos:notation "HCEV_4" ;
    sfia:level lor:4 ;
    sfia:skillLevelDescription """Selects appropriate tools, methods and design patterns to design user interactions with and experiences of a product, system or service.
Translates concepts into outputs and prototypes for user feedback and evaluation.
Evaluates alternative design options and recommends designs taking into account performance, security, usability and accessibility requirements. 
Considers and integrates appropriate visual design and branding elements in user experience designs."""@en .

sfialevels:HCEV_5 a sfia:SkillLevel ;
    skos:notation "HCEV_5" ;
    sfia:level lor:5 ;
    sfia:skillLevelDescription """Plans and drives user experience design activities.
Provides expert advice and guidance to support the adoption of agreed approaches. Determines the approaches to be used to design user experiences. 
Uses iterative approaches to incorporate user feedback or evaluation rapidly into designs. 
Ensures appropriate consideration and integration of visual design and branding elements into user experience design."""@en .

sfialevels:HCEV_6 a sfia:SkillLevel ;
    skos:notation "HCEV_6" ;
    sfia:level lor:6 ;
    sfia:skillLevelDescription """Obtains organisational commitment to strategies to deliver required user experience, usability, accessibility and security. 
Defines organisational policies, standards and techniques for user experience design. 
Plans and leads user experience design activities for strategic, large or complex programmes.
Promotes the value of user-centred design across the organisation."""@en .

sfialevels:HPCC_4 a sfia:SkillLevel ;
    skos:notation "HPCC_4" ;
    sfia:level lor:4 ;
    sfia:skillLevelDescription """Develops moderately complex solutions that use high-performance computing environments to address real-world problems. 
Applies a range of high-performance computing techniques with sensitivity to the limitations of the techniques. Uses input and feedback from experts as appropriate. 
Analyses the complexity, scalability and performance of algorithms, including massively parallel implementations, and makes or recommends improvements."""@en .

sfialevels:HPCC_5 a sfia:SkillLevel ;
    skos:notation "HPCC_5" ;
    sfia:level lor:5 ;
    sfia:skillLevelDescription """Creates, tests and improves complex high-performance computing solutions to address real-world problems. 
Collaborates with stakeholders to ensure high-performance computing solutions are effective at addressing their problems. 
Guides development teams in the appropriate and effective use of high-performance computing resources"""@en .

sfialevels:HPCC_6 a sfia:SkillLevel ;
    skos:notation "HPCC_6" ;
    sfia:level lor:6 ;
    sfia:skillLevelDescription """Initiates the creation, testing, improvement and application of algorithms that solve real-world problems in high-performance computing environments. 
Sets standards and strategies for the use of high-performance computing. 
Leads the implementation of organisational capabilities to ensure appropriate, consistent and effective usage of high-performance computing."""@en .

sfialevels:HPCC_7 a sfia:SkillLevel ;
    skos:notation "HPCC_7" ;
    sfia:level lor:7 ;
    sfia:skillLevelDescription """Directs the creation and review of a cross-functional, enterprise-wide approach and culture for high-performance computing.
Leads the development of the organisation's high-performance computing capabilities and champions its use in solving real-world problems."""@en .

sfialevels:HSIN_1 a sfia:SkillLevel ;
    skos:notation "HSIN_1" ;
    sfia:level lor:1 ;
    sfia:skillLevelDescription """Follows agreed procedures to perform simple installations, replace consumable items and check the correct working of installations. 
Documents and reports on work done."""@en .

sfialevels:HSIN_2 a sfia:SkillLevel ;
    skos:notation "HSIN_2" ;
    sfia:level lor:2 ;
    sfia:skillLevelDescription """Installs or removes system components using supplied installation instructions and tools.  
Conducts standard tests and contributes to investigations of problems and faults.
Confirms the correct working of installations. 
Documents results in accordance with agreed procedures."""@en .

sfialevels:HSIN_3 a sfia:SkillLevel ;
    skos:notation "HSIN_3" ;
    sfia:level lor:3 ;
    sfia:skillLevelDescription """Installs or removes hardware and/or software, using supplied installation instructions and tools, including handover to the client. 
Uses standard procedures and diagnostic tools to test installations, correct problems, and document results. 
Records details of all components that have been installed and removed. Assists users and follows agreed procedures for further help or escalation.
Contributes to the development of installation procedures and standards."""@en .

sfialevels:HSIN_4 a sfia:SkillLevel ;
    skos:notation "HSIN_4" ;
    sfia:level lor:4 ;
    sfia:skillLevelDescription """Undertakes or supervises complex installations and de-installations of systems or components, including handover to the client. 
Develops procedures and standards for installation and handover to maintain and improve the installation service. 
Schedules installation work around client priorities and resource availability.  
Ensures adherence to established safety and quality procedures."""@en .

sfialevels:HSIN_5 a sfia:SkillLevel ;
    skos:notation "HSIN_5" ;
    sfia:level lor:5 ;
    sfia:skillLevelDescription """Takes responsibility for installation and/or decommissioning projects. 
Provides effective team leadership, including information flow to and from the customer during project work. 
Develops and implements quality plans and method statements. 
Monitors the effectiveness of installations and ensures appropriate recommendations for change are made."""@en .

sfialevels:HWDE_2 a sfia:SkillLevel ;
    skos:notation "HWDE_2" ;
    sfia:level lor:2 ;
    sfia:skillLevelDescription """Assists in designing simple hardware components or subsystems under guidance.
Follows established design principles, patterns and methodologies as directed. Participates in translating logical designs into physical implementations.
Tests hardware components or subsystems against provided specifications and documents results. Contributes to the documentation of hardware designs using required standards, methods and tools.
Seeks guidance and support for deviations from standard practices or when facing unfamiliar scenarios."""@en .

sfialevels:HWDE_3 a sfia:SkillLevel ;
    skos:notation "HWDE_3" ;
    sfia:level lor:3 ;
    sfia:skillLevelDescription """Follows selected standard approaches and design patterns to design simple hardware components. 
Seeks guidance when deviating from established design patterns. Takes account of target environment, performance, security, safety, reliability and sustainability requirements.
Translates logical designs into physical designs. Tests the performance of prototypes and production output against specification.
Submits hardware designs for approval. Documents all work using required standards, methods and tools."""@en .

sfialevels:HWDE_4 a sfia:SkillLevel ;
    skos:notation "HWDE_4" ;
    sfia:level lor:4 ;
    sfia:skillLevelDescription """Designs hardware components, taking account of target environment, performance, security, safety, reliability and sustainability requirements. 
Translates logical designs into physical designs and delivers technical prototypes of proposed components for approval and production. 
Designs the tests to measure the performance of prototypes and production output against specification and inform iterative development."""@en .

sfialevels:HWDE_5 a sfia:SkillLevel ;
    skos:notation "HWDE_5" ;
    sfia:level lor:5 ;
    sfia:skillLevelDescription """Specifies and designs complex hardware components/systems. 
Selects appropriate design standards, methods and tools, consistent with agreed policies and ensures they are applied effectively. 
Undertakes impact analysis on major design options. Assesses and manages associated risks. Ensures hardware designs balance functional, quality, safety, security, systems management, reliability and sustainability requirements. 
Reviews designs created by others to ensure selection of appropriate technology, efficient use of resources and effective integration of multiple systems and technology. Contributes to policy for selection of components."""@en .

sfialevels:HWDE_6 a sfia:SkillLevel ;
    skos:notation "HWDE_6" ;
    sfia:level lor:6 ;
    sfia:skillLevelDescription """Provides overall direction and leadership in the hardware design practice within an organisation. 
Influences industry-based models for the development of new technology and  components. 
Develops effective procurement strategies, consistent with business needs. 
Develops, drives adoption and ensures adherence to organisational policies, strategies and standards for hardware design."""@en .

sfialevels:IAMT_1 a sfia:SkillLevel ;
    skos:notation "IAMT_1" ;
    sfia:level lor:1 ;
    sfia:skillLevelDescription """Performs basic identity and access management tasks, including user account lifecycle management, under supervision.
Maintains accurate records and follows established identity and access management protocols."""@en .

sfialevels:IAMT_2 a sfia:SkillLevel ;
    skos:notation "IAMT_2" ;
    sfia:level lor:2 ;
    sfia:skillLevelDescription """Provides assistance for identity and access management operations, including automated role allocation and access control management.
Engages in user identity lifecycle management, including account creation and deletion.
Facilitates operation of identity and access management tools and self-service portals."""@en .

sfialevels:IAMT_3 a sfia:SkillLevel ;
    skos:notation "IAMT_3" ;
    sfia:level lor:3 ;
    sfia:skillLevelDescription """Administers standard identity and access management services, implementing policies and resolving related issues. 
Manages monitoring, audits and logging for identity and access management systems. Investigates minor security breaches in accordance with established procedures related to identity and access management.
Assists users in defining their access rights and privileges. Designs and implements simple identity and access management solutions, enhancing user access security. Contributes to the enhancement and optimisation of existing identity and access management processes and systems."""@en .

sfialevels:IAMT_4 a sfia:SkillLevel ;
    skos:notation "IAMT_4" ;
    sfia:level lor:4 ;
    sfia:skillLevelDescription """Designs and implements complex identity and access management solutions, focusing on automated access control and role allocation. 
Oversees the integration of identity and access management services with new technologies.
Provides specialised support for complex identity and access management operations and supports implementation of policies and standards.
Collaborates with stakeholders to align identity and access management with business objectives and emerging security trends."""@en .

sfialevels:IAMT_5 a sfia:SkillLevel ;
    skos:notation "IAMT_5" ;
    sfia:level lor:5 ;
    sfia:skillLevelDescription """Offers authoritative advice on identity and access management, ensuring services align with and support evolving business needs and security protocols.
Manages large-scale identity and access management initiatives and oversees the integration of identity and access management services with new technologies, enhancing security and operational efficiency.
Leads operational planning for identity and access management, anticipating future trends and preparing the organisation for scalable growth.
Ensures compliance of identity and access management systems and oversees advanced monitoring and audit processes."""@en .

sfialevels:IAMT_6 a sfia:SkillLevel ;
    skos:notation "IAMT_6" ;
    sfia:level lor:6 ;
    sfia:skillLevelDescription """Shapes and defines organisation-wide identity and access management policies, ensuring alignment with business strategies and security requirements.
Champions good practices, advocating for robust and innovative identity and access management solutions across the organisation.
Influences and guides organisational governance, integrating emerging technologies and regulatory compliance into identity and access management strategies.
Reviews and advises on identity and access management aspects and implications of new business initiatives."""@en .

sfialevels:ICPM_1 a sfia:SkillLevel ;
    skos:notation "ICPM_1" ;
    sfia:level lor:1 ;
    sfia:skillLevelDescription """Contributes, under instruction, to publication support activities. 
Supports the collation of data. 
Uses established publishing processes and procedures following appropriate guidelines."""@en .

sfialevels:ICPM_2 a sfia:SkillLevel ;
    skos:notation "ICPM_2" ;
    sfia:level lor:2 ;
    sfia:skillLevelDescription """Uses technical publication concepts, tools, and methods to publish content following agreed procedures and guidelines. 
Prepares and formats content to meet the needs of the target audience and platform.
Obtains and analyses usage data and presents it effectively. 
Applies principles of usability and accessibility to published information."""@en .

sfialevels:ICPM_3 a sfia:SkillLevel ;
    skos:notation "ICPM_3" ;
    sfia:level lor:3 ;
    sfia:skillLevelDescription """Coordinates content management processes and procedures to meet the needs of users. 
Uses content publishing systems to manage published content across different channels. 
Assists in identifying and working with content creators.
Considers all legal issues related to publishing."""@en .

sfialevels:ICPM_4 a sfia:SkillLevel ;
    skos:notation "ICPM_4" ;
    sfia:level lor:4 ;
    sfia:skillLevelDescription """Applies organisational guidelines and uses appropriate tools and techniques to provide publishing interfaces to new or existing platforms and applications. 
Maintains and updates content management processes and practices to meet the needs of users. Selects appropriate channels through which content should be published. 
Collaborates with and provides guidance to content creators. Provides advice to users and content authors to leverage the features of the relevant channels and tools used. 
Identifies the legal implications associated with publishing."""@en .

sfialevels:ICPM_5 a sfia:SkillLevel ;
    skos:notation "ICPM_5" ;
    sfia:level lor:5 ;
    sfia:skillLevelDescription """Plans and manages content publishing activities and assignments. 
Develops standards, processes and practices for consistent content publishing across one or more platforms/channels. Advises on the approach and techniques to be used for content publishing. 
Advises on approaches for content publishing and creator collaborations. Assures design of the overall content structure and style. 
Ensures publication processes comply with agreed policies and strategies and legal requirements."""@en .

sfialevels:ICPM_6 a sfia:SkillLevel ;
    skos:notation "ICPM_6" ;
    sfia:level lor:6 ;
    sfia:skillLevelDescription """Obtains organisational commitment and resources to ensure the appropriate quality of material published by or on behalf of the organisation. 
Defines organisational policies, standards, processes and practices for content publishing, including creator partnerships. 
Plans and leads content publishing activities for strategic, large and complex programmes. 
Ensures policies are implemented and any legal issues related to publishing are adequately managed."""@en .

sfialevels:IFDN_2 a sfia:SkillLevel ;
    skos:notation "IFDN_2" ;
    sfia:level lor:2 ;
    sfia:skillLevelDescription """Assists in developing preliminary infrastructure design specifications under routine supervision. 
Uses established standards and security protocols to contribute to infrastructure design activities. 
Helps draft design documents and diagrams. Documents design-related issues."""@en .

sfialevels:IFDN_3 a sfia:SkillLevel ;
    skos:notation "IFDN_3" ;
    sfia:level lor:3 ;
    sfia:skillLevelDescription """Performs varied infrastructure design tasks, including complex and non-routine assignments, using standard methods. 
Develops design specifications and diagrams for infrastructure components, integrating hardware, software, network elements, and cloud services, and addressing security requirements.
Collaborates with others to align infrastructure design with organisational objectives and resolve design issues. 
Suggests improvements to enhance infrastructure performance and reliability."""@en .

sfialevels:IFDN_4 a sfia:SkillLevel ;
    skos:notation "IFDN_4" ;
    sfia:level lor:4 ;
    sfia:skillLevelDescription """Leads the design of complex infrastructure systems to deliver comprehensive design solutions. 
Develops detailed architectural frameworks and ensures integration of all infrastructure components, including cloud services.
Provides guidance on recommended practices and design standards. Reviews and validates design specifications and documentation. 
Checks that designs are scalable, reliable and secure, aligning with business and technical requirements."""@en .

sfialevels:IFDN_5 a sfia:SkillLevel ;
    skos:notation "IFDN_5" ;
    sfia:level lor:5 ;
    sfia:skillLevelDescription """Manages the design of infrastructure from analysis to execution and evaluation. 
Accountable for achieving design objectives and ensuring alignment with organisational goals and the effective integration of infrastructure components and systems. Provides authoritative guidance on design practices and methodologies.
Evaluates new technologies and their applicability to the organisation's needs. Develops and enforces design standards and recommended practices, ensuring consistent and high-quality design outcomes."""@en .

sfialevels:IFDN_6 a sfia:SkillLevel ;
    skos:notation "IFDN_6" ;
    sfia:level lor:6 ;
    sfia:skillLevelDescription """Develops and drives adoption of and adherence to organisational policies, standards, guidelines and methods for infrastructure design.
Collaborates with senior stakeholders to align design projects with organisational objectives. 
Provides strategic oversight and guidance, ensuring infrastructure designs are forward-looking, scalable and secure. 
Accountable for the overall success of infrastructure design initiatives."""@en .

sfialevels:INAS_2 a sfia:SkillLevel ;
    skos:notation "INAS_2" ;
    sfia:level lor:2 ;
    sfia:skillLevelDescription """Assists with information assurance activities under routine supervision.
Helps perform basic risk assessments and supports the implementation of information assurance measures.
Assists in maintaining records and documentation related to information assurance."""@en .

sfialevels:INAS_3 a sfia:SkillLevel ;
    skos:notation "INAS_3" ;
    sfia:level lor:3 ;
    sfia:skillLevelDescription """Follows standard approaches for the technical assessment of information systems against information assurance policies and business objectives. 
Makes routine accreditation decisions. Recognises decisions that are beyond their scope and responsibility level and escalates according.
Reviews and performs risk assessments and risk treatment plans. Identifies typical risk indicators and explains prevention measures.
Maintains integrity of records to support and justify decisions."""@en .

sfialevels:INAS_4 a sfia:SkillLevel ;
    skos:notation "INAS_4" ;
    sfia:level lor:4 ;
    sfia:skillLevelDescription """Performs technical assessments and/or accreditation of complex or higher-risk information systems. 
Identifies risk mitigation measures required in addition to the standard organisation or domain measures. 
Establishes the requirement for accreditation evidence from delivery partners and communicates accreditation requirements to stakeholders.  
Contributes to planning and organisation of information assurance and accreditation activities. Contributes to development of and implementation of information assurance processes."""@en .

sfialevels:INAS_5 a sfia:SkillLevel ;
    skos:notation "INAS_5" ;
    sfia:level lor:5 ;
    sfia:skillLevelDescription """Interprets information assurance and security policies and applies these to manage risks. 
Provides advice and guidance to ensure adoption of and adherence to information assurance architectures, strategies, policies, standards and guidelines. 
Plans, organises and conducts information assurance and accreditation of complex domains areas, cross-functional areas and across the supply chain. 
Contributes to the development of policies, standards and guidelines."""@en .

sfialevels:INAS_6 a sfia:SkillLevel ;
    skos:notation "INAS_6" ;
    sfia:level lor:6 ;
    sfia:skillLevelDescription """Develops information assurance policy, standards and guidelines. 
Contributes to the development of organisational strategies that address the evolving business risk and information control requirements. 
Drives adoption of and adherence to policies and standards. Ensures architectural principles are followed, requirements are defined and rigorous security testing is applied. Ensures accreditation processes support and enable organisational objectives.
Monitors environmental and market trends and assesses any impact on organisational strategies, benefits and risks."""@en .

sfialevels:INAS_7 a sfia:SkillLevel ;
    skos:notation "INAS_7" ;
    sfia:level lor:7 ;
    sfia:skillLevelDescription """Directs the creation and review of an enterprise information assurance strategy to support the strategic requirements of the business.
Ensures compliance between business strategies and information assurance by setting strategies, policies, standards and practices. 
Leads the provision of information assurance expertise, advice and guidance across all of the organisation's information and information systems."""@en .

sfialevels:INCA_1 a sfia:SkillLevel ;
    skos:notation "INCA_1" ;
    sfia:level lor:1 ;
    sfia:skillLevelDescription """Contributes, under instruction, to the generation of content and the configuration of content items and files. 
Executes pre-planned testing activities under supervision and records findings."""@en .

sfialevels:INCA_2 a sfia:SkillLevel ;
    skos:notation "INCA_2" ;
    sfia:level lor:2 ;
    sfia:skillLevelDescription """Works with colleagues and stakeholders to understand audience needs and to assimilate source material. 
Creates draft content to meet the requirements of the audience as clearly, simply and quickly as possible. 
Applies guidelines and standards to moderate content from others, escalating where appropriate."""@en .

sfialevels:INCA_3 a sfia:SkillLevel ;
    skos:notation "INCA_3" ;
    sfia:level lor:3 ;
    sfia:skillLevelDescription """Produces information artefacts that are accurate, current, relevant and easily understood by the intended audience. 
Clarifies detailed content requirements with clients and representatives of the intended audience. 
Designs, creates, controls and evaluates moderately complex subject matter. 
Makes informed decisions about the best way to present information to an audience. Applies moderation and editing processes to content supplied by others."""@en .

sfialevels:INCA_4 a sfia:SkillLevel ;
    skos:notation "INCA_4" ;
    sfia:level lor:4 ;
    sfia:skillLevelDescription """Designs the content and appearance of complex information artefacts. 
Controls, monitors and evaluates content to ensure quality, consistency and accessibility of messages and optimal use of chosen media. Understands and manages risks associated with publishing content.
Moderates content and ensures content can be re-purposed appropriately. 
Reviews work of others and takes responsibility for ensuring appropriate publication."""@en .

sfialevels:INCA_5 a sfia:SkillLevel ;
    skos:notation "INCA_5" ;
    sfia:level lor:5 ;
    sfia:skillLevelDescription """Provides overall editorial control across the team or teams of content designers and authors. 
Advises on appropriate content formats and mediums. 
Develops and maintains content plans showing how the identified audience needs will be met. 
Oversees the review and approval of materials to enable requirements to be satisfied."""@en .

sfialevels:INCA_6 a sfia:SkillLevel ;
    skos:notation "INCA_6" ;
    sfia:level lor:6 ;
    sfia:skillLevelDescription """Obtains organisational commitment to policies, standards and strategies to create required content. 
Specifies design standards and methods to meet organisational objectives for content creation. 
Plans and leads content creation for strategic, large and complex programmes."""@en .

sfialevels:INOV_5 a sfia:SkillLevel ;
    skos:notation "INOV_5" ;
    sfia:level lor:5 ;
    sfia:skillLevelDescription """Manages the innovation pipeline and executes innovation processes. 
Develops and adapts innovation tools, processes and infrastructures to drive the process of innovation. Identifies resources and capabilities needed to support innovation. 
Encourages and motivates innovation communities, teams and individuals to share creative ideas and learn from failures. 
Manages and facilitates the communication and open flow of creative ideas between interested parties and the set-up of innovation networks and communities."""@en .

sfialevels:INOV_6 a sfia:SkillLevel ;
    skos:notation "INOV_6" ;
    sfia:level lor:6 ;
    sfia:skillLevelDescription """Obtains organisational commitment to innovation. 
Develops organisational capabilities to drive innovation. 
Leads and plans the development of innovation capabilities and implementation of innovation processes, tools and frameworks. 
Leads the communication and an open flow of creative ideas between interested parties and the set-up of innovation networks and communities."""@en .

sfialevels:INOV_7 a sfia:SkillLevel ;
    skos:notation "INOV_7" ;
    sfia:level lor:7 ;
    sfia:skillLevelDescription """Leads development of a culture that encourages innovation, risk-taking and collaboration. 
Embeds innovation processes throughout business units and links strategy execution with innovation. 
Aligns organisational and individual objectives, measures and rewards with innovation."""@en .

sfialevels:INVA_4 a sfia:SkillLevel ;
    skos:notation "INVA_4" ;
    sfia:level lor:4 ;
    sfia:skillLevelDescription """Develops and documents investment appraisals for a range of different projects. 
Identifies suitable appraisal techniques based on the characteristics of a project. 
Collects the information required to create an investment appraisal in collaboration with internal and external stakeholders. Presents findings of investment appraisals to selected stakeholders. 
Refines and maintains investment appraisals."""@en .

sfialevels:INVA_5 a sfia:SkillLevel ;
    skos:notation "INVA_5" ;
    sfia:level lor:5 ;
    sfia:skillLevelDescription """Advises on investment appraisal approaches and tailors organisational standards to the context of portfolios/programmes.  
Leads investment appraisal activities for simple portfolios and programmes and complex projects."""@en .

sfialevels:INVA_6 a sfia:SkillLevel ;
    skos:notation "INVA_6" ;
    sfia:level lor:6 ;
    sfia:skillLevelDescription """Develops organisational policies, standards and guidelines for investment appraisals. 
Leads activities to establish consistent appraisal across the component projects and programmes within a portfolio. 
Reviews investment appraisals for high-value initiatives to assure their quality. 
Leads investment appraisal activities for complex programmes of work and portfolios."""@en .

sfialevels:IRMG_3 a sfia:SkillLevel ;
    skos:notation "IRMG_3" ;
    sfia:level lor:3 ;
    sfia:skillLevelDescription """Supports teams and individuals to identify and organise information assets and repositories in line with policy and practices.
Conducts routine searches for non-sensitive information needed to support organisational decision making.
Supports users to find and access information resources based on their requirements and approved access."""@en .

sfialevels:IRMG_4 a sfia:SkillLevel ;
    skos:notation "IRMG_4" ;
    sfia:level lor:4 ;
    sfia:skillLevelDescription """Enables the organisation to organise, control and discover information assets.
Supports the organisation to identify, catalogue and categorise information types and information repositories in line with information management strategies and practices.
Enables users to find information through appropriate use of metadata and search tools.
Provides advice and guidance to enable good information management practices to be adopted across the organisation."""@en .

sfialevels:IRMG_5 a sfia:SkillLevel ;
    skos:notation "IRMG_5" ;
    sfia:level lor:5 ;
    sfia:skillLevelDescription """Ensures implementation of information and records management policies and standard practice.  Communicates the benefits and value of information management. 
Plans effective information storage, sharing and publishing within the organisation. Develops organisational taxonomy for information assets. 
Provides expert advice and guidance to enable the organisation to get maximum value from its information assets. 
Assesses issues that might prevent the organisation from making maximum use of its information assets. Contributes to the development of policy, standards and procedures for compliance with relevant legislation."""@en .

sfialevels:IRMG_6 a sfia:SkillLevel ;
    skos:notation "IRMG_6" ;
    sfia:level lor:6 ;
    sfia:skillLevelDescription """Leads and plans activities to communicate and implement information management strategies and policies.  
Develops organisational policies, standards and guidelines for information management. 
Ensures the information required to support the organisation is defined. Creates information management processes.  
Coordinates internal and externally sourced information resources to meet specific business objectives."""@en .

sfialevels:IRMG_7 a sfia:SkillLevel ;
    skos:notation "IRMG_7" ;
    sfia:level lor:7 ;
    sfia:skillLevelDescription """Establishes and communicates the organisation's information management strategy. 
Specifies at a strategic level the information needed to support the business strategy and business functions.  
Directs information resources to create value for stakeholders. 
Accountable for compliance with regulations, standards and codes of good practice relating to all aspects of information management."""@en .

sfialevels:ISCO_6 a sfia:SkillLevel ;
    skos:notation "ISCO_6" ;
    sfia:level lor:6 ;
    sfia:skillLevelDescription """Maintains awareness of the global needs of the organisation. 
Promotes the benefits that a common approach to technology deployment will bring to the entire organisation.
Coordinates and collaborates with others on the promotion, acquisition, development and implementation of information systems and services."""@en .

sfialevels:ISCO_7 a sfia:SkillLevel ;
    skos:notation "ISCO_7" ;
    sfia:level lor:7 ;
    sfia:skillLevelDescription """Establishes the organisation's strategy for managing information and communicates the policies, standards, procedures and methods necessary to implement the strategy. 
Coordinates all aspects of management of the lifecycle of information systems. 
Represents the interests of the entire organisation to general management and external bodies on matters relating to information strategy."""@en .

sfialevels:ITCM_2 a sfia:SkillLevel ;
    skos:notation "ITCM_2" ;
    sfia:level lor:2 ;
    sfia:skillLevelDescription """Assists in collecting contract performance data. 
Produces standard reports on contract performance under routine supervision."""@en .

sfialevels:ITCM_3 a sfia:SkillLevel ;
    skos:notation "ITCM_3" ;
    sfia:level lor:3 ;
    sfia:skillLevelDescription """Acts as a routine contact point between the organisation and counterparties concerning contract management. 
Supports the collection of contract performance data. Creates standard reports on contract performance."""@en .

sfialevels:ITCM_4 a sfia:SkillLevel ;
    skos:notation "ITCM_4" ;
    sfia:level lor:4 ;
    sfia:skillLevelDescription """Sources and collects contract performance data (such as pricing and supply chain costs), and monitors performance against key performance indicators. 
Monitors progress against business objectives specified in the business case. Proactively manages risk and reward mechanisms in the contract. 
Identifies and reports under-performance and develops opportunities for improvement. Monitors compliance with terms and conditions and takes appropriate steps to address non-compliance. 
Identifies where change is required and plans for variations. Ensures, in consultation with stakeholders, that change management protocols are implemented."""@en .

sfialevels:ITCM_5 a sfia:SkillLevel ;
    skos:notation "ITCM_5" ;
    sfia:level lor:5 ;
    sfia:skillLevelDescription """Oversees and measures the fulfilment of contractual obligations. 
Uses key performance indicators to monitor and challenge performance and identify opportunities for continual improvement. Develops strategies to address under-performance and compliance failures, including the application of contract terms. 
Identifies where changes are required, evaluates the impact, and advises stakeholders about the implications and consequences. Negotiates variations and seeks appropriate authorisation. 
Actively supports and engages with experts and stakeholders to ensure continual improvements are identified through review and benchmarking processes. Develops and implements change management protocols."""@en .

sfialevels:ITCM_6 a sfia:SkillLevel ;
    skos:notation "ITCM_6" ;
    sfia:level lor:6 ;
    sfia:skillLevelDescription """Negotiates and resolves contractual issues, including failure to meet contractual obligations. 
Promotes change control processes and leads variation negotiations when necessary. Champions continual improvement programmes, jointly developing strategies and incentives to enhance performance. Undertakes comprehensive financial evaluations. 
Ensures due diligence and legal vetting underpin all procurement processes, affirming risk assessment and compliance in contractual engagements. Ensures lessons learned from reviews are documented and promoted to all stakeholders. 
Leads the advancement and application of effective contract management practices within a specific business domain or category."""@en .

sfialevels:ITCM_7 a sfia:SkillLevel ;
    skos:notation "ITCM_7" ;
    sfia:level lor:7 ;
    sfia:skillLevelDescription """Leads the strategic direction and governance of contract management processes across the organisation. Advises executive leadership on contract management risks and strategies.
Implements contract management strategies aligned with organisational goals and market dynamics, including oversight of significant contracts and associated legal risks. Acts as the escalation point for major disputes. 
Promotes operational excellence in contract management, driving supply chain contracting improvements and innovation. 
Establishes strategic partnerships, aligning organisational and supplier goals. Represents the organisation in key negotiations, ensuring strategic, compliant outcomes."""@en .

sfialevels:ITMG_5 a sfia:SkillLevel ;
    skos:notation "ITMG_5" ;
    sfia:level lor:5 ;
    sfia:skillLevelDescription """Takes responsibility for managing the design, procurement, installation, upgrading, operation, control, maintenance and effective use of specific technology services.
Leads service delivery, ensuring agreed service levels, security requirements and other quality standards are met. Ensures adherence to relevant policies and procedures.
Ensures processes, procedures and practices are aligned across teams and providers to operate effectively and efficiently. 
Monitors technology services performance. Provides appropriate status and other reports to managers and senior users."""@en .

sfialevels:ITMG_6 a sfia:SkillLevel ;
    skos:notation "ITMG_6" ;
    sfia:level lor:6 ;
    sfia:skillLevelDescription """Manages and allocates resources for budgeting, estimating, planning, developing and delivering a portfolio of technology services and systems. 
Engages and influences stakeholders to ensure services are developed and managed to meet agreed service levels, security requirements and quality standards. 
Plans and implements processes, procedures, tools and practices for monitoring and managing the performance of technology services. 
Aligns the contribution of specified systems and services with organisational and financial goals. Recommends sourcing options, whether in-house, outsourced, or a combination, ensuring optimal service delivery."""@en .

sfialevels:ITMG_7 a sfia:SkillLevel ;
    skos:notation "ITMG_7" ;
    sfia:level lor:7 ;
    sfia:skillLevelDescription """Sets the strategic direction for managing the technology services portfolio, ensuring alignment with organisational strategies, objectives and emerging opportunities. 
Promotes and assesses technology's potential to drive change, evaluating feasibility and impact.
Authorises the establishment and integration of new or modified service delivery capabilities, balancing in-house and outsourced options. Oversees resource allocation for planning, developing and delivering technical services and products.
Maintains a strategic overview of how technology services contribute to organisational success."""@en .

sfialevels:ITOP_1 a sfia:SkillLevel ;
    skos:notation "ITOP_1" ;
    sfia:level lor:1 ;
    sfia:skillLevelDescription """Supports routine infrastructure tasks and basic troubleshooting under close supervision.
Monitors infrastructure health and reports on component status to support operational continuity."""@en .

sfialevels:ITOP_2 a sfia:SkillLevel ;
    skos:notation "ITOP_2" ;
    sfia:level lor:2 ;
    sfia:skillLevelDescription """Executes operational procedures, runs automation scripts and performs routine maintenance, installation and monitoring of infrastructure components. 
Adjusts automation tasks as instructed to meet operational standards.
Reports on infrastructure performance and security events, addressing issues directly when possible or escalating them to others for resolution."""@en .

sfialevels:ITOP_3 a sfia:SkillLevel ;
    skos:notation "ITOP_3" ;
    sfia:level lor:3 ;
    sfia:skillLevelDescription """Provisions, deploys and configures infrastructure services and components.
Monitors infrastructure for load, performance and security events. Reports metrics and resolves operational issues.
Executes standard operational procedures, including backups and restorations. 
Carries out agreed system software maintenance tasks. Automates routine system administration tasks to specifications using standard tools and basic scripting."""@en .

sfialevels:ITOP_4 a sfia:SkillLevel ;
    skos:notation "ITOP_4" ;
    sfia:level lor:4 ;
    sfia:skillLevelDescription """Applies technical expertise to maintain and optimise technology infrastructure, executing updates and employing automation tools. Configures tools and/or creates scripts to automate infrastructure tasks. 
Maintains operational procedures and checks that they are followed, including adherence to security policies. Uses infrastructure management tools to monitor load, performance, and security metrics.
Investigates and enables the resolution of operational and security-related issues. Provides reports and proposals for improvement to stakeholders.
Contributes to the planning and implementation of infrastructure maintenance and updates. Implements agreed infrastructure changes and maintenance routines."""@en .

sfialevels:ITOP_5 a sfia:SkillLevel ;
    skos:notation "ITOP_5" ;
    sfia:level lor:5 ;
    sfia:skillLevelDescription """Provides technical leadership to optimise the performance of the technology infrastructure. 
Drives the adoption of tools and automated processes for effective operational management and delivery.
Oversees the planning, installation, maintenance and acceptance of new and updated infrastructure components and infrastructure-based services. Aligns to service expectations, security requirements and other quality standards. 
Ensures operational procedures and documentation are current and effective, tracks and addresses operational issues and reports to stakeholders."""@en .

sfialevels:ITSP_4 a sfia:SkillLevel ;
    skos:notation "ITSP_4" ;
    sfia:level lor:4 ;
    sfia:skillLevelDescription """Contributes to the collection and analysis of information to support strategy development. 
Assists in the preparation of reports and insights for strategic planning.
Supports the communication of strategic plans and related change initiatives to relevant stakeholders. 
Helps monitor progress against strategic objectives and provides feedback."""@en .

sfialevels:ITSP_5 a sfia:SkillLevel ;
    skos:notation "ITSP_5" ;
    sfia:level lor:5 ;
    sfia:skillLevelDescription """Collates information and creates reports and insights to support strategy management processes.
Ensures all stakeholders are aware of the strategic management approach and timetables. Provides support and guidance to help stakeholders adhere to the approach.
Develops and communicates plans to drive forward the strategy and related change planning.
Contributes to the development of policies, standards and guidelines for strategy development and planning."""@en .

sfialevels:ITSP_6 a sfia:SkillLevel ;
    skos:notation "ITSP_6" ;
    sfia:level lor:6 ;
    sfia:skillLevelDescription """Sets policies, standards and guidelines for how the organisation conducts strategy development and planning.
Leads and manages the creation or review of a strategy that meets the requirements of the business. 
Develops, communicates, implements and reviews the processes which embed strategic management in the operational management of the organisation."""@en .

sfialevels:ITSP_7 a sfia:SkillLevel ;
    skos:notation "ITSP_7" ;
    sfia:level lor:7 ;
    sfia:skillLevelDescription """Leads the definition, implementation and communication of the organisation's strategic management framework. 
Directs the creation and review of a strategy and plans to support the strategic requirements of the business."""@en .

sfialevels:JADN_3 a sfia:SkillLevel ;
    skos:notation "JADN_3" ;
    sfia:level lor:3 ;
    sfia:skillLevelDescription """Gathers data regarding job roles and responsibilities from various sources. 
Assists in mapping tasks and competencies using established skills-based frameworks. Contributes to the creation of preliminary job descriptions and performance metrics. 
Works under direction to align job roles with organisational strategies, workplace practices and evolving requirements. 
Provides support in the assessment of job changes and their impact on workflows and employee satisfaction. Participates in the process of revising job documentation to reflect updated role definitions and responsibilities."""@en .

sfialevels:JADN_4 a sfia:SkillLevel ;
    skos:notation "JADN_4" ;
    sfia:level lor:4 ;
    sfia:skillLevelDescription """Performs detailed job analyses, breaking down roles using data-driven insights. 
Creates or revises job descriptions with consideration of required skills, competencies and organisational culture. 
Evaluates the impact of job role changes on workflows, employee engagement and overall workplace practices. 
Provides insights into aligning job roles with emerging organisational needs, including technology integration and adaptive strategies. Collaborates with stakeholders to ensure job designs are effective, responsive to changing business needs and aligned with skills-based approaches."""@en .

sfialevels:JADN_5 a sfia:SkillLevel ;
    skos:notation "JADN_5" ;
    sfia:level lor:5 ;
    sfia:skillLevelDescription """Leads job architecture and design initiatives, ensuring alignment with organisational strategies and evolving workplace practices. 
Develops comprehensive role definitions that encompass necessary skills, competencies and alignment with the organisation's culture and goals.
Assesses and suggests modifications to existing roles to improve effectiveness and address new challenges. 
Provides authoritative advice on the adaptation of job architecture and job design to reflect changes in organisational strategy, technology, workplace practices and skills-based approaches."""@en .

sfialevels:KNOW_2 a sfia:SkillLevel ;
    skos:notation "KNOW_2" ;
    sfia:level lor:2 ;
    sfia:skillLevelDescription """Maintains a knowledge management database. 
Leverages knowledge of a specialism to capture and classify content, taking expert advice when required."""@en .

sfialevels:KNOW_3 a sfia:SkillLevel ;
    skos:notation "KNOW_3" ;
    sfia:level lor:3 ;
    sfia:skillLevelDescription """Maintains knowledge management systems and content to meet business needs.
Supports others to enable them to complete knowledge management activities and form knowledge management habits. Supports changes to work practices to enable capture and use of knowledge.
Reports on the progress of knowledge management activities. 
Configures and develops knowledge management systems and standards."""@en .

sfialevels:KNOW_4 a sfia:SkillLevel ;
    skos:notation "KNOW_4" ;
    sfia:level lor:4 ;
    sfia:skillLevelDescription """Organises knowledge assets and oversees the lifecycle of identifying, capturing, classifying, storing and maintaining assets. 
Facilitates sharing, collaboration and communication of knowledge. Implements specific knowledge management initiatives.
Monitors the  use and impact of knowledge. 
Interrogates existing knowledge content to identify issues, risks and opportunities."""@en .

sfialevels:KNOW_5 a sfia:SkillLevel ;
    skos:notation "KNOW_5" ;
    sfia:level lor:5 ;
    sfia:skillLevelDescription """Develops and implements knowledge management processes, practices and behaviours. 
Provides advice, guidance and support to help people to adopt and embed knowledge management. Contributes to the definition of policies, standards and guidelines for knowledge management.
Evaluates and selects knowledge management methods and tools. Promotes collaborative technologies, processes and behaviours to facilitate sharing of ideas and work-knowledge. 
Shares ideas and examples of existing practices. Implements knowledge management at programme, project and team level."""@en .

sfialevels:KNOW_6 a sfia:SkillLevel ;
    skos:notation "KNOW_6" ;
    sfia:level lor:6 ;
    sfia:skillLevelDescription """Develops organisational policies, standards and guidelines for knowledge management. 
Champions and leads in the development of an organisational knowledge management approach. Shares different approaches for knowledge sharing across communities of practice, business units and networks.
Promotes knowledge-sharing through operational business processes and systems. Monitors and evaluates knowledge-sharing initiatives. 
Manages reviews of the benefits and value of knowledge management. Identifies and recommends improvements."""@en .

sfialevels:KNOW_7 a sfia:SkillLevel ;
    skos:notation "KNOW_7" ;
    sfia:level lor:7 ;
    sfia:skillLevelDescription """Develops an organisation-wide knowledge management strategy and leads the creation of a knowledge management culture. 
Embeds knowledge management across business units and develops strategic knowledge management capabilities. 
Reinforces the importance of knowledge sharing by aligning individual and organisational objectives and rewards. 
Identifies opportunities for strategic relationships or partnerships with customers, suppliers and partners."""@en .

sfialevels:LEDA_2 a sfia:SkillLevel ;
    skos:notation "LEDA_2" ;
    sfia:level lor:2 ;
    sfia:skillLevelDescription """Assists in the administration of competency assessments using standard tools and procedures under routine supervision. 
Supports the collection and organisation of assessment data and results using specified methods and tools. 
Helps create and maintain documentation."""@en .

sfialevels:LEDA_3 a sfia:SkillLevel ;
    skos:notation "LEDA_3" ;
    sfia:level lor:3 ;
    sfia:skillLevelDescription """Performs routine assessments of knowledge, skills, competencies, or behaviours using specified tools and methods. 
Supports the collection, organisation, and review of assessment data to maintain accurate records."""@en .

sfialevels:LEDA_4 a sfia:SkillLevel ;
    skos:notation "LEDA_4" ;
    sfia:level lor:4 ;
    sfia:skillLevelDescription """Performs routine and non-routine assessments of knowledge, skill, competency or behaviour using specified methods. 
Provides advice and guidance to support the adoption of assessment methods and tools. 
Moderates assessments conducted by other assessors. 
Reviews and improves usage and application of assessment methods and tools."""@en .

sfialevels:LEDA_5 a sfia:SkillLevel ;
    skos:notation "LEDA_5" ;
    sfia:level lor:5 ;
    sfia:skillLevelDescription """Provides advice and guidance on selecting, adopting and adapting assessment methods, tools and techniques. 
Plans assessments based on the context of the assessment and how assessment results will be used. 
Manages execution of assessments to ensure they deliver the required outcomes with acceptable quality. Monitors and moderates reviews performed by other assessors. 
Manages reviews of the benefits and value of assessment methods and tools. Identifies and recommends improvements to assessment methods and tools."""@en .

sfialevels:LEDA_6 a sfia:SkillLevel ;
    skos:notation "LEDA_6" ;
    sfia:level lor:6 ;
    sfia:skillLevelDescription """Champions the importance and value of assessment and appropriate assessment methods, tools and techniques. 
Develops organisational policies, standards and guidelines for assessments. 
Leads in the introduction and use of assessment methodologies and tools.  Establishes an assessment practice and pool of assessors within the organisation. 
Establishes quality assurance to ensure internal and/or external consistency and reliability of assessment outcomes. Ensures the quality of assessments across different user groups."""@en .

sfialevels:MEAS_2 a sfia:SkillLevel ;
    skos:notation "MEAS_2" ;
    sfia:level lor:2 ;
    sfia:skillLevelDescription """Assists in the collection and maintenance of data for measurement purposes under routine supervision.
Uses standard procedures for measuring attributes of processes, products and services. 
Helps generate and distribute measurement reports."""@en .

sfialevels:MEAS_3 a sfia:SkillLevel ;
    skos:notation "MEAS_3" ;
    sfia:level lor:3 ;
    sfia:skillLevelDescription """Applies standard techniques to support the specification of measures and the collection and maintenance of data for measurement. 
Generates, produces and distributes reports. 
Uses measurement tools for routine analysis of data. 
Identifies and implements improvements to data collection methods."""@en .

sfialevels:MEAS_4 a sfia:SkillLevel ;
    skos:notation "MEAS_4" ;
    sfia:level lor:4 ;
    sfia:skillLevelDescription """Identifies and prioritises appropriate measures, scales and targets. 
Supports projects, functions or teams in the development of measurement methods. 
Specifies base and derived measures which support agreed information needs. Specifies how to collect and store the data for each required measure. Provides guidance on collection of data. 
Designs reports and reporting formats."""@en .

sfialevels:MEAS_5 a sfia:SkillLevel ;
    skos:notation "MEAS_5" ;
    sfia:level lor:5 ;
    sfia:skillLevelDescription """Establishes measurement objectives and the scope of measurement for functions, teams and projects. 
Plans and implements improvements to measurement capability. Provides advice and guidance for effective use of measures and measurement.  
Selects measures appropriate to the context and organisational objectives. Reviews data collection and storage mechanisms to support measurement.
Contributes to organisational policies, standards and guidelines for measurement."""@en .

sfialevels:MEAS_6 a sfia:SkillLevel ;
    skos:notation "MEAS_6" ;
    sfia:level lor:6 ;
    sfia:skillLevelDescription """Leads the development of organisational capabilities for measurement (including automation). 
Creates the measurement framework and aligns measurement objectives with business objectives. 
Develops organisational policies, standards and guidelines for measurement. 
Provides resources to ensure adoption and adherence to policies and standards."""@en .

sfialevels:METL_2 a sfia:SkillLevel ;
    skos:notation "METL_2" ;
    sfia:level lor:2 ;
    sfia:skillLevelDescription """Provide routine support using agreed guidelines on the use of well-established methods and tools. 
Assists in configuring and maintaining methods and tools under routine supervision. 
Supports the creation and updating of documentation related to methods and tools."""@en .

sfialevels:METL_3 a sfia:SkillLevel ;
    skos:notation "METL_3" ;
    sfia:level lor:3 ;
    sfia:skillLevelDescription """Provides support on the use of existing methods and tools. 
Configures and maintains methods and tools within a known context. 
Creates and updates the documentation of methods and tools.
Identifies and resolves basic issues related to tool usage."""@en .

sfialevels:METL_4 a sfia:SkillLevel ;
    skos:notation "METL_4" ;
    sfia:level lor:4 ;
    sfia:skillLevelDescription """Engages with stakeholders to understand requirements and recommends appropriate solutions. 
Provides advice and guidance to support the adoption of methods and tools and adherence to policies and standards. 
Tailors processes to meet specific needs while ensuring they align with established standards and are informed by evaluations of methods and tools.
Reviews and improves usage and application of methods and tools."""@en .

sfialevels:METL_5 a sfia:SkillLevel ;
    skos:notation "METL_5" ;
    sfia:level lor:5 ;
    sfia:skillLevelDescription """Provides authoritative advice and leadership to promote adoption of methods and tools and adherence to policies and standards. 
Evaluates and selects appropriate methods and tools in line with agreed policies and standards. Contributes to organisational policies, standards and guidelines for methods and tools.
Implements methods and tools at programme, project and team levels including selection and tailoring in line with agreed standards. 
Manages reviews of the benefits and value of methods and tools. Identifies and recommends improvements that support broader organisational goals."""@en .

sfialevels:METL_6 a sfia:SkillLevel ;
    skos:notation "METL_6" ;
    sfia:level lor:6 ;
    sfia:skillLevelDescription """Develops organisational policies, standards and guidelines for methods and tools. 
Sets direction and leads in the introduction and use of techniques, methodologies and tools, to meet business requirements. 
Leads the development of organisational capabilities for methods and tools to ensure consistent adoption and adherence to policies and standards.
Secures organisational commitment and resources to methods and tools. Drives continuous improvement and innovation in methods and tools."""@en .

sfialevels:MKCM_3 a sfia:SkillLevel ;
    skos:notation "MKCM_3" ;
    sfia:level lor:3 ;
    sfia:skillLevelDescription """Assists in the execution of marketing campaigns. 
Uses selected tools and channels to engage target audiences. 
Monitors campaign performance and collects data for analysis. 
Participates in marketing events and initiatives."""@en .

sfialevels:MKCM_4 a sfia:SkillLevel ;
    skos:notation "MKCM_4" ;
    sfia:level lor:4 ;
    sfia:skillLevelDescription """Plans and executes marketing campaigns across multiple channels. 
Selects appropriate tools and platforms to reach desired audiences. 
Creates and distributes engaging marketing content and materials. Writes campaign briefs and contributes to creative evaluation.
Analyses campaign performance and makes recommendations for optimisation."""@en .

sfialevels:MKCM_5 a sfia:SkillLevel ;
    skos:notation "MKCM_5" ;
    sfia:level lor:5 ;
    sfia:skillLevelDescription """Develops and oversees complex, multi-channel marketing campaign strategies. 
Selects optimal channels, tools and creative partners. Leads creative briefings and evaluates concepts.
Manages stakeholders and ensures brand consistency.
Monitors campaign performance and adjusts tactics as needed. Analyses campaign results and reports on key metrics and outcomes."""@en .

sfialevels:MKTG_4 a sfia:SkillLevel ;
    skos:notation "MKTG_4" ;
    sfia:level lor:4 ;
    sfia:skillLevelDescription """Contributes to the development and execution of marketing plans. 
Applies recognised good practices to analyse marketing effectiveness and ROI. 
Assists in defining target customers and brand positioning. Implements solutions to marketing challenges within established guidelines. Collaborates with team members to execute marketing activities."""@en .

sfialevels:MKTG_5 a sfia:SkillLevel ;
    skos:notation "MKTG_5" ;
    sfia:level lor:5 ;
    sfia:skillLevelDescription """Develops and manages comprehensive marketing plans aligned with business objectives. 
Implements strategies to maximise marketing effectiveness given organisational goals. Leads the definition of target customers and brand positioning.
Analyses complex data to inform marketing decisions. Creates innovative solutions to marketing challenges. 
Coordinates with other teams to execute integrated marketing approaches."""@en .

sfialevels:MKTG_6 a sfia:SkillLevel ;
    skos:notation "MKTG_6" ;
    sfia:level lor:6 ;
    sfia:skillLevelDescription """Defines and oversees the execution of  marketing strategies to achieve organisational goals. 
Ensures alignment of marketing plans with business objectives and market insights. Evaluates and optimises marketing effectiveness and budget allocation to drive outcomes.
Identifies and addresses current and future marketing capability needs. 
Collaborates with senior leadership to integrate marketing strategies with organisational vision."""@en .

sfialevels:MKTG_7 a sfia:SkillLevel ;
    skos:notation "MKTG_7" ;
    sfia:level lor:7 ;
    sfia:skillLevelDescription """Leads the creation of long-term marketing strategies aligned with organisational vision. 
Directs the marketing function, ensuring integration of marketing plans with business goals. Oversees the evaluation and optimisation of marketing activities, ensuring maximum impact and efficiency. 
Provides strategic advice to senior leadership on marketing trends and opportunities. 
Promotes a culture of creativity and continuous improvement within the marketing team. Ensures the marketing function adapts to changing market conditions and business needs."""@en .

sfialevels:MLNG_2 a sfia:SkillLevel ;
    skos:notation "MLNG_2" ;
    sfia:level lor:2 ;
    sfia:skillLevelDescription """Assists in data preparation, model training and evaluation tasks under routine supervision. 
Uses standard machine learning frameworks and tools to develop basic models for well-defined problems. 
Documents results and contributes to maintaining machine learning solutions."""@en .

sfialevels:MLNG_3 a sfia:SkillLevel ;
    skos:notation "MLNG_3" ;
    sfia:level lor:3 ;
    sfia:skillLevelDescription """Applies established machine learning techniques and algorithms to solve business problems. 
Selects and prepares data for model training and evaluation. 
Trains, optimises and validates machine learning models using standard tools and frameworks. 
Deploys models into production and monitors their performance. Communicates results and limitations to stakeholders."""@en .

sfialevels:MLNG_4 a sfia:SkillLevel ;
    skos:notation "MLNG_4" ;
    sfia:level lor:4 ;
    sfia:skillLevelDescription """Assesses the suitability of machine learning and designs and develops solutions for a range of business problems.
Selects and applies appropriate techniques and algorithms based on data characteristics and business requirements. Provides guidance to others.
Engineers features and optimises model performance. Implements algorithms and contributes to development, evaluation, monitoring and deployment. Applies industry-specific rules and guidelines, anticipating risks and implications.
Collaborates with cross-functional teams to integrate machine learning models into production systems. Conducts in-depth performance analysis and troubleshoots issues."""@en .

sfialevels:MLNG_5 a sfia:SkillLevel ;
    skos:notation "MLNG_5" ;
    sfia:level lor:5 ;
    sfia:skillLevelDescription """Leads the development and implementation of machine learning solutions for complex, high-impact business problems.
Architects end-to-end machine learning pipelines and systems, incorporating MLOps practices. Evaluates and selects tools, frameworks and infrastructure for machine learning projects. 
Establishes practices and standards for machine learning development and operations. Provides expert advice and guidance on machine learning techniques and applications.
Collaborates with stakeholders to align machine learning initiatives with organisational goals."""@en .

sfialevels:MLNG_6 a sfia:SkillLevel ;
    skos:notation "MLNG_6" ;
    sfia:level lor:6 ;
    sfia:skillLevelDescription """Sets the strategic direction and roadmap for machine learning adoption and innovation within the organisation. 
Establishes governance frameworks and recommended protocols for responsible, ethical and sustainable development and use of machine learning. 
Leads the development of organisational capabilities, policies, standards and guidelines in machine learning. 
Collaborates with senior stakeholders to identify high-impact opportunities for machine learning and drives their implementation. Follows research and industry trends and integrates them into organisational practices."""@en .

sfialevels:MRCH_3 a sfia:SkillLevel ;
    skos:notation "MRCH_3" ;
    sfia:level lor:3 ;
    sfia:skillLevelDescription """Assists in the design and execution of market research studies. 
Collects and analyses data using standard methods and tools. 
Contributes to the preparation of research reports and presentations."""@en .

sfialevels:MRCH_4 a sfia:SkillLevel ;
    skos:notation "MRCH_4" ;
    sfia:level lor:4 ;
    sfia:skillLevelDescription """Designs and conducts market research studies independently. 
Analyses market data to identify trends, opportunities and challenges. 
Segments markets and identifies target customers based on research findings. 
Prepares research reports and presentations to communicate findings and recommendations."""@en .

sfialevels:MRCH_5 a sfia:SkillLevel ;
    skos:notation "MRCH_5" ;
    sfia:level lor:5 ;
    sfia:skillLevelDescription """Leads the design and execution of complex market research studies. 
Analyses and synthesises market data from multiple sources to generate insights and recommendations. 
Presents research findings and strategic recommendations to stakeholders. Advises stakeholders on the implications of research findings for business strategy and decision-making. 
Contributes to the development of organisational market research methods and standards."""@en .

sfialevels:MRCH_6 a sfia:SkillLevel ;
    skos:notation "MRCH_6" ;
    sfia:level lor:6 ;
    sfia:skillLevelDescription """Sets the overall direction and strategy for market research in the organisation. 
Develops organisational policies, standards and guidelines for market research. Ensures market research capabilities and resources are aligned with business needs and objectives. 
Communicates high-level market insights and strategic implications to senior leadership and stakeholders. 
Collaborates with internal and external partners to influence organisational strategy and drive the effective use of market research in decision-making and strategy development."""@en .

sfialevels:NFTS_1 a sfia:SkillLevel ;
    skos:notation "NFTS_1" ;
    sfia:level lor:1 ;
    sfia:skillLevelDescription """Executes given non-functional test scripts under supervision, focusing on system qualities and characteristics such as performance.
Sets up basic test environments and uses standard tools to execute prescribed tests.
Records results and reports issues."""@en .

sfialevels:NFTS_2 a sfia:SkillLevel ;
    skos:notation "NFTS_2" ;
    sfia:level lor:2 ;
    sfia:skillLevelDescription """Assists in designing non-functional test cases and creating test scripts. 
Supports the preparation of test data for non-functional testing under supervision. Configures test environments. Executes both manual and automated non-functional testing.
Implements appropriate test tools based on given non-functional requirements or specifications. Defines test conditions for given non-functional requirements. 
Analyses and reports on test activities, results, issues and risks."""@en .

sfialevels:NFTS_3 a sfia:SkillLevel ;
    skos:notation "NFTS_3" ;
    sfia:level lor:3 ;
    sfia:skillLevelDescription """Designs non-functional test cases and scripts, mapping to pre-set criteria for system qualities and characteristics.
Prepares and manages test data to reflect real-world scenarios. Configures test environments, collaborates with stakeholders to clarify requirements and automates repeatable tests. 
Participates in requirement reviews to refine comprehensive test plans. Undertakes exploratory tests to investigate unusual behaviours. 
Executes tests, troubleshooting issues as they arise. Analyses and reports on test activities, providing thorough coverage of non-functional attributes."""@en .

sfialevels:NFTS_4 a sfia:SkillLevel ;
    skos:notation "NFTS_4" ;
    sfia:level lor:4 ;
    sfia:skillLevelDescription """Selects suitable non-functional testing approaches, considering system criticality and complexity. 
Develops, automates and executes test plans for end-to-end system attributes. Configures and manages complex, test environments, ensuring alignment with production conditions. 
Applies risk-based strategies to prioritise test efforts and collaborates across teams to ensure comprehensive automated test coverage. Troubleshoots issues in real-time, ensuring prompt resolution. 
Analyses and reports on test activities, results and risks, including the work of others."""@en .

sfialevels:NFTS_5 a sfia:SkillLevel ;
    skos:notation "NFTS_5" ;
    sfia:level lor:5 ;
    sfia:skillLevelDescription """Plans and drives non-functional testing across all stages, ensuring alignment with requirements and prioritising risk-based strategies. 
Provides expert advice on non-functional  methods, tools and frameworks. Leads the setup and maintenance of advanced test environments. 
Monitors the application of testing standards, ensuring they reflect real-world conditions. Troubleshoots and resolves complex issues, working closely with stakeholders.
Leads efforts to improve the efficiency and reliability of non-functional testing. Identifies improvements and contributes to organisational policies, standards and guidelines for non-functional testing."""@en .

sfialevels:NFTS_6 a sfia:SkillLevel ;
    skos:notation "NFTS_6" ;
    sfia:level lor:6 ;
    sfia:skillLevelDescription """Develops organisational policies, standards and guidelines for non-functional testing, ensuring they align with business strategy and incorporate a risk-based approach.
Plans and leads strategic, complex testing activities, ensuring they align with overall system quality goals. Manages risks and opportunities, coordinating with other types of testing.
Develops organisational capabilities to address complex quality validation challenges. Drives continuous automation and improvements in test environments.
Promotes a culture of quality in non-functional testing, driving adherence to organisational standards and proactive risk mitigation."""@en .

sfialevels:NTAS_1 a sfia:SkillLevel ;
    skos:notation "NTAS_1" ;
    sfia:level lor:1 ;
    sfia:skillLevelDescription """Supports routine network tasks under close supervision. 
Monitors basic network health and reports on the status of network components. 
Assists with straightforward troubleshooting and follows established procedures to maintain operational continuity. 
Escalates issues as necessary to higher levels of support"""@en .

sfialevels:NTAS_2 a sfia:SkillLevel ;
    skos:notation "NTAS_2" ;
    sfia:level lor:2 ;
    sfia:skillLevelDescription """Assists in the operational configuration of network components and the investigation and resolution of network problems.
Assists in the implementation of basic scripting and automation tools to streamline network support tasks.
Assists with specified maintenance procedures and follows established safety, security and quality standards.
Provides first-line support and guidance to network users, escalating issues as necessary."""@en .

sfialevels:NTAS_3 a sfia:SkillLevel ;
    skos:notation "NTAS_3" ;
    sfia:level lor:3 ;
    sfia:skillLevelDescription """Executes agreed network maintenance tasks and specified operational configuration of network components.
Identifies and diagnoses network problems/faults using the required troubleshooting tools and network management software, including addressing security-related issues.
Implements and maintains scripts, automation tools and orchestration platforms to optimise network support processes.
Collects performance and traffic statistics and collaborates with others to ensure network effectiveness and resolve issues"""@en .

sfialevels:NTAS_4 a sfia:SkillLevel ;
    skos:notation "NTAS_4" ;
    sfia:level lor:4 ;
    sfia:skillLevelDescription """Applies technical expertise to maintain and optimise network infrastructure, executing updates and employing automation tools. 
Uses network management tools to monitor load, performance, and security statistics. Investigates and enables the resolution of network-related operational and security issues.  Configures tools and/or creates scripts to automate network tasks. 
Maintains operational procedures and checks that they are followed. Provides reports and proposals for improvement to stakeholders.
Contributes to the planning and implementation of network maintenance, updates, and security enhancements. Implements agreed network changes and maintenance routines."""@en .

sfialevels:NTAS_5 a sfia:SkillLevel ;
    skos:notation "NTAS_5" ;
    sfia:level lor:5 ;
    sfia:skillLevelDescription """Leads network operations to optimise performance. 
Oversees planning, installation, maintenance, and acceptance of network components and services, aligning with service expectations, standards, and security requirements.
Ensures network support requests are handled according to set standards and procedures.
Drives the adoption of tools and processes for effective operational management and delivery, ensuring security considerations are addressed. Maintains procedures and documentation. Investigates and resolves complex network problems. Tracks operational issues and reports to stakeholders."""@en .

sfialevels:NTDS_2 a sfia:SkillLevel ;
    skos:notation "NTDS_2" ;
    sfia:level lor:2 ;
    sfia:skillLevelDescription """Assists with defining configurations for networks and network components under routine supervision. 
Follows established network architectures, standards, and security protocols.
Assists in documenting network configurations and producing detailed network specifications under guidance, incorporating relevant security aspects."""@en .

sfialevels:NTDS_3 a sfia:SkillLevel ;
    skos:notation "NTDS_3" ;
    sfia:level lor:3 ;
    sfia:skillLevelDescription """Specifies the technical configurations and components required for a small network or a network segment in a more complex infrastructure.
Follows organisational architectures, standards, and security guidelines."""@en .

sfialevels:NTDS_4 a sfia:SkillLevel ;
    skos:notation "NTDS_4" ;
    sfia:level lor:4 ;
    sfia:skillLevelDescription """Designs specific network components using agreed architectures, design standards, patterns and methodology.
Translates logical designs into physical designs that meet specified operational parameters for capacity and performance.
Reviews and verifies network designs against non-functional requirements, including validation and error correction procedures, access, security and audit controls.
Contributes to the development of recovery routines and contingency procedures. Contributes to alternative network architectures, networking topologies and design options."""@en .

sfialevels:NTDS_5 a sfia:SkillLevel ;
    skos:notation "NTDS_5" ;
    sfia:level lor:5 ;
    sfia:skillLevelDescription """Produces, or approves network providers', network architectures, topologies and configuration databases for own area of responsibility.
Specifies design parameters for network connectivity, capacity, speed, interfacing, security and access, in line with business requirements.
Assesses network-related risks and specifies recovery routines and contingency procedures.
Creates multiple design views to address the different stakeholders' concerns and to handle both functional and non-functional requirements."""@en .

sfialevels:NTDS_6 a sfia:SkillLevel ;
    skos:notation "NTDS_6" ;
    sfia:level lor:6 ;
    sfia:skillLevelDescription """Takes responsibility for major aspects of network specification, standards, technologies and overall network design models within the organisation.
Produces network design policies, principles and criteria covering connectivity, capacity, interfacing, security, resilience, recovery and access.
Develops and drives adoption of and adherence to organisational policies, standards, guidelines and methods for network design."""@en .

sfialevels:NUAN_4 a sfia:SkillLevel ;
    skos:notation "NUAN_4" ;
    sfia:level lor:4 ;
    sfia:skillLevelDescription """Creates moderately complex algorithms using a range of mathematical techniques and with sensitivity to the limitations of the techniques. 
Uses sophisticated scientific computing and visualisation environments. 
Assesses the stability, accuracy and efficiency of algorithms and makes or recommends improvements to them. 
Iterates and improves models using feedback from experts as appropriate."""@en .

sfialevels:NUAN_5 a sfia:SkillLevel ;
    skos:notation "NUAN_5" ;
    sfia:level lor:5 ;
    sfia:skillLevelDescription """Creates, tests and improves complex algorithms that numerically solve real-world problems. 
Develops mathematical and computational techniques to assist with numerical analysis. 
Communicates limitations such as uncertainty and systematic errors. 
Reviews algorithms for their conformance to design and performance standards."""@en .

sfialevels:NUAN_6 a sfia:SkillLevel ;
    skos:notation "NUAN_6" ;
    sfia:level lor:6 ;
    sfia:skillLevelDescription """Initiates the creation, testing, improvement and application of numerical algorithms that solve real-world mathematical problems. 
Sets standards and strategies for the application of numerical analysis. 
Leads the implementation of numerical analyses capabilities to ensure appropriate, consistent and effective usage across the organisation."""@en .

sfialevels:NUAN_7 a sfia:SkillLevel ;
    skos:notation "NUAN_7" ;
    sfia:level lor:7 ;
    sfia:skillLevelDescription """Directs the creation and review of a cross-functional, enterprise-wide approach and culture for numerical analysis. 
Leads the development of the organisation's numerical analysis capabilities and champions its use in solving real-world problems."""@en .

sfialevels:OCDV_5 a sfia:SkillLevel ;
    skos:notation "OCDV_5" ;
    sfia:level lor:5 ;
    sfia:skillLevelDescription """Contributes to identifying new areas of capability improvement within the organisation which may be enhancements to skills, technology or processes. 
Develops and maintains a detailed knowledge of capability improvement approaches and techniques and selects appropriate approaches for the organisation. 
Conducts capability improvement assignments, such as maturity or performance assessments, to identify strengths and weaknesses. Selects and prioritises improvement opportunities, generates buy-in and plans improvement activities justified by measurable organisational benefits. 
Offers support, guidance, advice and suggestions to help continual improvement activities."""@en .

sfialevels:OCDV_6 a sfia:SkillLevel ;
    skos:notation "OCDV_6" ;
    sfia:level lor:6 ;
    sfia:skillLevelDescription """Seeks out, identifies, proposes and initiates capability improvement activities within the organisation. 
Leads substantial improvement programmes. Plans and manages the evaluation or assessment of organisational capabilities. Selects frameworks, approaches and techniques for use. 
Takes action to exploit opportunities to deliver measurable, beneficial impacts upon operational effectiveness. Devises solutions and leads change initiatives, including communication, transition and implementation activities. 
Monitors international, national and sector trends to establish the needed capability."""@en .

sfialevels:OCDV_7 a sfia:SkillLevel ;
    skos:notation "OCDV_7" ;
    sfia:level lor:7 ;
    sfia:skillLevelDescription """Represents and leads organisational capability improvement at the highest level. 
Determines the need for strategic organisation-level capability improvement to satisfy the organisation's strategic goals and long-term objectives.
Liaises with the organisation's functions to establish requirements and identifies, proposes, initiates and leads significant organisational capability improvement programmes.
Manages the quality and appropriateness of the work performed and delivers measurable business benefits. Adopts and/or modifies existing capability improvement approaches as necessary."""@en .

sfialevels:OCEN_4 a sfia:SkillLevel ;
    skos:notation "OCEN_4" ;
    sfia:level lor:4 ;
    sfia:skillLevelDescription """Supports teams in adopting new practices, providing ongoing resources and guidance. 
Facilitates a safe environment for exploring challenges related to change. 
Assists with engagement sessions to secure leadership commitment, focusing on the behavioural aspects of change.
Addresses issues that arise during implementation, ensuring minimal disruption."""@en .

sfialevels:OCEN_5 a sfia:SkillLevel ;
    skos:notation "OCEN_5" ;
    sfia:level lor:5 ;
    sfia:skillLevelDescription """Develops and implements cultural change plans across teams, ensuring alignment with long-term success. 
Coordinates cross-functional teams to support the adoption of new behaviours. Communicates how changes align with business goals and long-term success, focusing on emotional and behavioural impacts. Supports leaders and employees in exploring challenges associated with adopting new practices. 
Enables employees to develop the necessary skills and behaviours for sustained change."""@en .

sfialevels:OCEN_6 a sfia:SkillLevel ;
    skos:notation "OCEN_6" ;
    sfia:level lor:6 ;
    sfia:skillLevelDescription """Champions new ways of working that align with strategic opportunities. 
Influences and engages with senior executives to gain their support for change initiatives. 
Guides the development of strategies and roadmaps to drive long-term behavioural change.  Reviews progress, addresses challenges and ensures the sustainability of change initiatives.
Provides guidance to change leaders, focusing on the human aspects of organisational change."""@en .

sfialevels:OCOP_2 a sfia:SkillLevel ;
    skos:notation "OCOP_2" ;
    sfia:level lor:2 ;
    sfia:skillLevelDescription """Supports offensive cyber operations under supervision. 
Assists in creating electronic target folders based on provided intelligence. 
Participates in basic operational tasks, following established security protocols.
Assists in documenting operations and outcomes, contributing to post-operation reviews."""@en .

sfialevels:OCOP_3 a sfia:SkillLevel ;
    skos:notation "OCOP_3" ;
    sfia:level lor:3 ;
    sfia:skillLevelDescription """Carries out specific tasks within offensive cyber operations, aligning operational tasks with broader objectives.
Supports the creation and maintenance of electronic target folders, gathering and verifying target information. 
Assists in the execution of operations, maintaining operational security. 
Prepares detailed reports and participates in post-operation analysis."""@en .

sfialevels:OCOP_4 a sfia:SkillLevel ;
    skos:notation "OCOP_4" ;
    sfia:level lor:4 ;
    sfia:skillLevelDescription """Responsible for the execution of offensive cyber operations, including detailed planning and target selection. 
Manages the development and updating of electronic target folders, ensuring accuracy and comprehensiveness. Coordinates operational teams, adapting actions based on real-time intelligence. 
Ensures compliance with legal and ethical standards during operations. Evaluates collateral damage from targeting activities, including potential second and third-order effects.
Conducts post-operation analyses, assessing impact and recommending improvements."""@en .

sfialevels:OCOP_5 a sfia:SkillLevel ;
    skos:notation "OCOP_5" ;
    sfia:level lor:5 ;
    sfia:skillLevelDescription """Leads complex and high-risk offensive cyber operations, overseeing planning, execution and analysis. 
Integrates intelligence with operational planning, aligning all actions with organisational objectives. Evaluates the intelligence cost against the operational benefit of engaging targets. Assesses potential collateral damage, including second and third-order effects. 
Manages the creation and tactical use of electronic target folders, coordinating with external entities as necessary. 
Develops policies and standards for offensive operations, ensuring legal and ethical compliance. Provides expert guidance on offensive capabilities and operational tactics."""@en .

sfialevels:OCOP_6 a sfia:SkillLevel ;
    skos:notation "OCOP_6" ;
    sfia:level lor:6 ;
    sfia:skillLevelDescription """Sets the strategic direction and policies for offensive cyber operations within the organisation. 
Leads the development and deployment of advanced operational techniques and capabilities. Oversees critical and sensitive operations, ensuring alignment with national or organisational security goals. 
Collaborates with senior leadership and external entities on offensive operations. Evaluates intelligence cost versus operational benefit at a strategic level. Assesses and mitigates potential collateral damage.
Evaluates and refines the effectiveness of offensive operations, providing recommendations for future initiatives."""@en .

sfialevels:OFCL_4 a sfia:SkillLevel ;
    skos:notation "OFCL_4" ;
    sfia:level lor:4 ;
    sfia:skillLevelDescription """Facilitates a series of group activities or workshops in situations of complexity and ambiguity and competing stakeholder needs.
Designs a structured sequence of meetings, events or workshops to solve complex problems.
Understands required outcomes and outputs from teams and facilitates the team to deliver these.
Helps to improve team processes and performance in meetings, events or workshops."""@en .

sfialevels:OFCL_5 a sfia:SkillLevel ;
    skos:notation "OFCL_5" ;
    sfia:level lor:5 ;
    sfia:skillLevelDescription """Facilitates workgroups to deliver defined goals and outcomes. 
Provides support, guidance and suggestions to workgroups and teams to learn collaborative problem solving and improve their team performance.  Creates shared responsibilities and sustainable agreements with the team.
Implements and improves agreed team principles, practices, processes & ceremonies.
Recognises and works with the strengths and constraints of team dynamics."""@en .

sfialevels:OFCL_6 a sfia:SkillLevel ;
    skos:notation "OFCL_6" ;
    sfia:level lor:6 ;
    sfia:skillLevelDescription """Facilitates cross-functional leadership teams to deliver organisational goals and outcomes.
Designs repeatable, systematic or ad hoc team processes for decision-making, prioritisation and problem-solving at the highest level. Guides leadership teams in developing shared responsibilities and making decisions that enable sustainable agreements.
Asks questions and raises awareness of leadership team performance. Provides suggestions to encourage teams to learn and improve how they work together.
Champions the development of self-organising workgroups across the organisation."""@en .

sfialevels:ORDI_3 a sfia:SkillLevel ;
    skos:notation "ORDI_3" ;
    sfia:level lor:3 ;
    sfia:skillLevelDescription """Assists in designing team structures and workflows under guidance, following standard modelling techniques and tools.
Helps develop visual representations of organisational models to aid understanding. Assists in preparing and updating organisational charts, role descriptions and other documentation.
Supports evaluation of design options by gathering and analysing data. Participates in creating design views to address stakeholder concerns and perspectives."""@en .

sfialevels:ORDI_4 a sfia:SkillLevel ;
    skos:notation "ORDI_4" ;
    sfia:level lor:4 ;
    sfia:skillLevelDescription """Designs team structures and workflows using modelling techniques, following agreed architectures, design standards and methodologies. 
Develops visual representations of organisational models and structures to facilitate understanding and decision-making. Supports the identification and evaluation of alternative design options and trade-offs.
Creates multiple design views to address the concerns of different stakeholders and to present different perspectives. Develops representations of team dynamics and workflows to aid stakeholder understanding and approval.
Reviews and refines designs to ensure they meet specifications."""@en .

sfialevels:ORDI_5 a sfia:SkillLevel ;
    skos:notation "ORDI_5" ;
    sfia:level lor:5 ;
    sfia:skillLevelDescription """Leads the design and implementation of organisational structures for significant teams, departments or divisions.
Conducts impact analyses on major design options and trade-offs to inform strategic decision-making.
Aligns existing organisational structures, roles, jobs and career paths to new processes and strategies. Ensures that the organisational design balances organisational performance and cultural requirements.
Reviews organisational designs and ensures that appropriate methods, tools and techniques are applied effectively. Contributes to development of organisational design policies, processes and standards."""@en .

sfialevels:ORDI_6 a sfia:SkillLevel ;
    skos:notation "ORDI_6" ;
    sfia:level lor:6 ;
    sfia:skillLevelDescription """Champions the value of new ways of working to address internal and external opportunities and threats. 
Sets direction and leads in selecting and using organisation design techniques, methodologies and tools. 
Plans and leads organisation design activities, identifies alternatives, assesses feasibility and recommends solutions. Identifies major changes affecting the organisation and mobilises resources to implement changes. 
Initiates the definition of new organisation boundaries and creates future organisation design. Outlines performance measurement objectives and the high-level implementation approach."""@en .

sfialevels:ORDI_7 a sfia:SkillLevel ;
    skos:notation "ORDI_7" ;
    sfia:level lor:7 ;
    sfia:skillLevelDescription """Establishes and communicates the need and rationale for organisational structure and culture change. 
Secures organisational commitment and resources needed for organisational and culture change. 
Leads organisational change by removing obstacles, advocating and lobbying for change at the highest levels. 
Puts in place mechanisms to reinforce and embed organisational and culture change. Acts as a role model for desired behaviours and sets consistent standards and expectations."""@en .

sfialevels:PBMG_2 a sfia:SkillLevel ;
    skos:notation "PBMG_2" ;
    sfia:level lor:2 ;
    sfia:skillLevelDescription """Assists with problem management tasks under routine supervision.
Helps document problems and maintain relevant records.
Assists in detecting, logging, classifying, and prioritising problems in systems, processes, and services."""@en .

sfialevels:PBMG_3 a sfia:SkillLevel ;
    skos:notation "PBMG_3" ;
    sfia:level lor:3 ;
    sfia:skillLevelDescription """Investigates problems in systems, processes and services. 
Contributes to the implementation of agreed remedies and preventative measures."""@en .

sfialevels:PBMG_4 a sfia:SkillLevel ;
    skos:notation "PBMG_4" ;
    sfia:level lor:4 ;
    sfia:skillLevelDescription """Initiates and monitors actions to investigate and resolve problems in systems, processes and services.
Determines problem fixes and remedies. 
Collaborates with others to implement agreed remedies and preventative measures.
Supports analysis of patterns and trends to improve problem management processes."""@en .

sfialevels:PBMG_5 a sfia:SkillLevel ;
    skos:notation "PBMG_5" ;
    sfia:level lor:5 ;
    sfia:skillLevelDescription """Ensures appropriate action is taken to anticipate, investigate and resolve problems in systems and services. 
Ensures problems are fully documented within the relevant reporting systems. 
Enables development of problem solutions. Coordinates the implementation of agreed remedies and preventative measures.
Analyses patterns and trends and improves problem management processes."""@en .

sfialevels:PDSV_4 a sfia:SkillLevel ;
    skos:notation "PDSV_4" ;
    sfia:level lor:4 ;
    sfia:skillLevelDescription """Assists practitioners with creating personal development plans. 
Advises on suitable development activities such as specific learning or experience to be gained. 
Monitors practitioners' continuing professional development records. 
Ensures achievements and enhanced capabilities are recorded and referenced to personal and organisational objectives."""@en .

sfialevels:PDSV_5 a sfia:SkillLevel ;
    skos:notation "PDSV_5" ;
    sfia:level lor:5 ;
    sfia:skillLevelDescription """Determines development needs for a professional practice area. 
Aligns development activities with organisational priorities, learning and development strategies and career pathways. 
Guides practitioners in creating development plans. Advises and supports assigned practitioners, ensuring alignment with professional development plans and career opportunities. 
Ensures practitioners record evidence of continuing professional development. Contributes to practitioners' performance appraisals, when required."""@en .

sfialevels:PDSV_6 a sfia:SkillLevel ;
    skos:notation "PDSV_6" ;
    sfia:level lor:6 ;
    sfia:skillLevelDescription """Develops and defines a professional development framework for one or more professional disciplines. 
Determines and maintains organisational development needs in line with business needs and strategic direction. Generates development strategies to achieve required change. 
Develops and leads communities of practice, including defining career pathways. 
Defines the approach to identifying suitable individuals to provide career advice and support.  Monitors progress and evaluates business benefits achieved from continual professional development."""@en .

sfialevels:PEDP_4 a sfia:SkillLevel ;
    skos:notation "PEDP_4" ;
    sfia:level lor:4 ;
    sfia:skillLevelDescription """Supports the implementation of policy, standards and guidelines related to information and data legislation and compliance requirements.
Monitors the implementation of effective controls for internal delegation, audit and control relating to information management.
Reports on the consolidated status of information controls to inform effective decision-making.
Identifies risks around the use of information  and data that is subject to specific legislation. Recommends remediation actions as required."""@en .

sfialevels:PEDP_5 a sfia:SkillLevel ;
    skos:notation "PEDP_5" ;
    sfia:level lor:5 ;
    sfia:skillLevelDescription """Contributes to policies, standards and guidelines for information and data compliance. 
Provides authoritative advice on implementing compliance controls in products, services and systems. 
Investigates breaches and recommends control improvements.  Maintains an inventory of legislated data, conducts risk assessments and specifies necessary changes. 
Ensures formal requests and complaints are handled following procedures. Prepares and submits reports to relevant authorities, ensuring all compliance requirements are met."""@en .

sfialevels:PEDP_6 a sfia:SkillLevel ;
    skos:notation "PEDP_6" ;
    sfia:level lor:6 ;
    sfia:skillLevelDescription """Develops strategies for compliance with information and data legislation. 
Ensures that the policy and standards for compliance with information and data legislation are fit for purpose, current and correctly implemented. 
Acts as the organisation's contact for the regulatory authorities. 
Operates as a focus for information and data legislation for the organisation, working with specialists to provide authoritative advice and guidance."""@en .

sfialevels:PEMT_4 a sfia:SkillLevel ;
    skos:notation "PEMT_4" ;
    sfia:level lor:4 ;
    sfia:skillLevelDescription """Provides operational direction, support and guidance to assigned colleagues. 
Allocates routine tasks or project work, in line with team objectives and individual capabilities. Monitors quality and performance against agreed criteria to make learning recommendations or to escalate concerns. 
Coaches colleagues in developing target skills and capabilities in line with team and personal goals.  
Facilitates effective working relationships between team members."""@en .

sfialevels:PEMT_5 a sfia:SkillLevel ;
    skos:notation "PEMT_5" ;
    sfia:level lor:5 ;
    sfia:skillLevelDescription """Forms, maintains and leads workgroups and individuals to achieve organisational objectives. 
Delegates objectives and responsibilities, including people management tasks. Sets quality, performance and capability targets aligned with organisational goals. 
Monitors performance and working relationships and provides feedback to address individual issues. Encourages skill development in line with team and personal goals. Adjusts workload, targets and team capacity to support individual growth. 
Actively participates in formal processes such as recruitment, reward, promotion and disciplinary procedures."""@en .

sfialevels:PEMT_6 a sfia:SkillLevel ;
    skos:notation "PEMT_6" ;
    sfia:level lor:6 ;
    sfia:skillLevelDescription """Determines and delegates people management and functional management objectives and responsibilities. 
Creates and sets the direction for multiple workgroups to achieve strategic organisational objectives. Sets strategy for quality and performance measurement in line with organisational goals. 
Provides a work environment and resources that allow individuals and workgroups to perform their tasks efficiently. 
Leads the implementation of formal organisational processes such as recruitment, reward, promotion and disciplinary procedures."""@en .

sfialevels:PENT_2 a sfia:SkillLevel ;
    skos:notation "PENT_2" ;
    sfia:level lor:2 ;
    sfia:skillLevelDescription """Assists with penetration testing tasks under routine supervision.
Supports the execution of standard penetration tests on systems, networks and applications.
Helps document and report on test results, findings and potential security risks."""@en .

sfialevels:PENT_3 a sfia:SkillLevel ;
    skos:notation "PENT_3" ;
    sfia:level lor:3 ;
    sfia:skillLevelDescription """Follows standard approaches to design and execute penetration testing activities.
Researches and investigates attack techniques and recommends ways to defend against them. 
Analyses and reports on penetration testing activities, results, issues and risks."""@en .

sfialevels:PENT_4 a sfia:SkillLevel ;
    skos:notation "PENT_4" ;
    sfia:level lor:4 ;
    sfia:skillLevelDescription """Selects appropriate testing approaches using in-depth technical analysis of risks and typical vulnerabilities. 
Produces test scripts, materials and test packs and tests new and existing networks, systems or applications. Provides advice on penetration testing to support others.
Records and analyses actions and results and modifies tests if necessary. 
Provides reports on progress, anomalies, risks and issues associated with the overall project."""@en .

sfialevels:PENT_5 a sfia:SkillLevel ;
    skos:notation "PENT_5" ;
    sfia:level lor:5 ;
    sfia:skillLevelDescription """Plans and drives penetration testing within a defined area of business activity. 
Delivers objective insights into the existence of vulnerabilities, the effectiveness of defences and mitigating controls. 
Takes responsibility for the integrity of testing activities and coordinates the execution of these activities. Provides authoritative advice and guidance on all aspects of penetration testing. 
Identifies needs and implements new approaches for penetration testing. Contributes to security testing standards."""@en .

sfialevels:PENT_6 a sfia:SkillLevel ;
    skos:notation "PENT_6" ;
    sfia:level lor:6 ;
    sfia:skillLevelDescription """Determines penetration testing policy and owns the supporting processes. 
Manages all penetration testing activities within the organisation. Assesses and advises on the practicality of testing process alternatives. 
Establishes capability for continual improvement and invention in penetration testing and leads the implementation of new approaches. 
Assesses suppliers' development and testing capabilities. Manages client relationships with respect to penetration testing."""@en .

sfialevels:PGMG_6 a sfia:SkillLevel ;
    skos:notation "PGMG_6" ;
    sfia:level lor:6 ;
    sfia:skillLevelDescription """Plans, directs and co-ordinates activities to manage and implement a programme from initiation to final transition into operational, business-as-usual management. 
Plans, schedules, monitors and reports on programme-related activities. Establishes and maintains appropriate and effective governance and risk management frameworks. 
Ensures comprehensive reporting and communication policies are in place and followed. Maintains an awareness of current technical developments that may provide opportunities to the programmes. 
Ensures programmes are managed to realise agreed business benefits within agreed timescales."""@en .

sfialevels:PGMG_7 a sfia:SkillLevel ;
    skos:notation "PGMG_7" ;
    sfia:level lor:7 ;
    sfia:skillLevelDescription """Sets organisational strategy governing programme management, including the application of appropriate methodologies. 
Plans, directs and co-ordinates activities to manage and implement complex programmes from initiation to full integration with operational, business-as-usual management. Aligns programme objectives with business goals and authorises related projects and activities. 
Plans, schedules, monitors and reports on programme activities, supported by comprehensive reporting and communication strategies.
Ensures governance and risk management frameworks are in place to support strategic decision-making and programme execution."""@en .

sfialevels:POMG_5 a sfia:SkillLevel ;
    skos:notation "POMG_5" ;
    sfia:level lor:5 ;
    sfia:skillLevelDescription """Ensures programme/project leads and/or service owners adhere to the agreed portfolio management and governance frameworks.
Explains what information is needed and ensures they provide this information to agreed targets of timelines and accuracy. 
Produces reports as appropriate for portfolio governance, including making recommendations for changes to the portfolio."""@en .

sfialevels:POMG_6 a sfia:SkillLevel ;
    skos:notation "POMG_6" ;
    sfia:level lor:6 ;
    sfia:skillLevelDescription """Engages and influences senior managers to ensure the portfolio will deliver the agreed business objectives. 
Leads the definition, planning, scheduling and monitoring of portfolio activities, ensuring alignment with governance standards. 
Ensures each portfolio component contributes to the overall objectives. Identifies and addresses portfolio-related issues, recommending and monitoring corrective actions. 
Collects and summarises portfolio measures, reporting on status and ensuring compliance with governance frameworks."""@en .

sfialevels:POMG_7 a sfia:SkillLevel ;
    skos:notation "POMG_7" ;
    sfia:level lor:7 ;
    sfia:skillLevelDescription """Authorises the structure of portfolios and aligns the portfolio with strategies, objectives, governance frameworks and emerging opportunities. 
Leads the definition, implementation and review of the organisation's portfolio management framework.  Sets parameters for the prioritisation of resources and the changes to be implemented. 
Recommends and implements corrective action by engaging and influencing senior management. 
Leads the on-going monitoring and review of portfolios for impact on current business activities and the strategic benefits to be realised. Implements portfolio governance arrangements and effective reporting."""@en .

sfialevels:PORT_2 a sfia:SkillLevel ;
    skos:notation "PORT_2" ;
    sfia:level lor:2 ;
    sfia:skillLevelDescription """Assists with software configuration tasks.
Supports the setup and customisation of software environments and platforms.
Helps document and report on configuration changes and deployments.
Reviews own work."""@en .

sfialevels:PORT_3 a sfia:SkillLevel ;
    skos:notation "PORT_3" ;
    sfia:level lor:3 ;
    sfia:skillLevelDescription """Designs, verifies, documents, amends and refactors moderately complex software configurations for deployment. 
Applies agreed standards and tools, to achieve a well-engineered result. 
Collaborates in reviews of work with others as appropriate."""@en .

sfialevels:PORT_4 a sfia:SkillLevel ;
    skos:notation "PORT_4" ;
    sfia:level lor:4 ;
    sfia:skillLevelDescription """Designs, verifies, documents, amends and refactors complex software configurations for deployment. 
Contributes to the selection of the software configuration methods, tools and techniques.
Applies agreed standards and tools, to achieve well-engineered outcomes. 
Participates in reviews of own work and leads reviews of colleagues' work."""@en .

sfialevels:PORT_5 a sfia:SkillLevel ;
    skos:notation "PORT_5" ;
    sfia:level lor:5 ;
    sfia:skillLevelDescription """Takes technical responsibility across all stages and iterations of configuration development and deployment. 
Plans and drives software configuration activities. Adopts and adapts appropriate software configuration methods, tools and techniques. 
Measures and monitors the application of standards for configuration design and deployment including software security. 
Contributes to the development of organisational policies, standards and guidelines for software configuration design and deployment."""@en .

sfialevels:PORT_6 a sfia:SkillLevel ;
    skos:notation "PORT_6" ;
    sfia:level lor:6 ;
    sfia:skillLevelDescription """Develops organisational policies, standards and guidelines for software configuration design, deployment and refactoring. 
Plans and leads software configuration and deployment activities for strategic, large and complex deployment projects. 
Develops new methods and organisational capabilities and drives adoption of and adherence to policies and standards."""@en .

sfialevels:PRMG_4 a sfia:SkillLevel ;
    skos:notation "PRMG_4" ;
    sfia:level lor:4 ;
    sfia:skillLevelDescription """Defines, documents and executes small projects or sub-projects. 
Works independently or with a small team, actively participating in all project phases. Applies appropriate project management methods and tools. Identifies, assesses and manages risks effectively.  
Prepares realistic project plans ((including scope, schedule, quality, risk and communication plans), ensuring stakeholder involvement and alignment with organisational governance standards. 
Tracks activities against the project schedule, managing stakeholder involvement as appropriate. Monitors costs, times, quality and resources used. Takes action where these exceed agreed tolerances."""@en .

sfialevels:PRMG_5 a sfia:SkillLevel ;
    skos:notation "PRMG_5" ;
    sfia:level lor:5 ;
    sfia:skillLevelDescription """Takes full responsibility for the definition, approach, facilitation and satisfactory completion of medium-scale projects. 
Provides effective leadership to the project team, adopting suitable project management methods and tools. Manages change control processes and assesses risks, ensuring projects align with governance frameworks and business priorities.
Communicates regularly with stakeholders, ensuring project deliverables meet agreed standards, budgets and timelines. Ensures project and product quality reviews occur on schedule and according to procedure. 
Proactively monitors performance metrics, implementing preventive and corrective actions as needed."""@en .

sfialevels:PRMG_6 a sfia:SkillLevel ;
    skos:notation "PRMG_6" ;
    sfia:level lor:6 ;
    sfia:skillLevelDescription """Takes full responsibility for the definition, documentation and successful completion of complex projects. 
Adopts and adapts project management methods and tools suited to the project's needs. Ensures effective monitoring and control of resources, budgets and timelines. 
Integrates robust risk management within governance frameworks to align decisions with the organisation's risk appetite and standards. 
Manages expectations of key stakeholders, ensuring all activities align with organisational goals, deliver agreed outcomes and provide business value."""@en .

sfialevels:PRMG_7 a sfia:SkillLevel ;
    skos:notation "PRMG_7" ;
    sfia:level lor:7 ;
    sfia:skillLevelDescription """Sets organisational strategy governing the direction and conduct of project management, ensuring projects align with strategic objectives and governance frameworks. 
Authorises the management of large-scale projects.  Leads project planning, scheduling, controlling and reporting activities for strategic, high impact, high risk projects. 
Oversees the selection and application of project methodologies. Directs the approach to risk management for projects, ensuring risks and issues are managed in line with organisational policies. 
Ensures projects deliver their intended benefits and contribute to long-term goals."""@en .

sfialevels:PROD_2 a sfia:SkillLevel ;
    skos:notation "PROD_2" ;
    sfia:level lor:2 ;
    sfia:skillLevelDescription """Assists with product management tasks under routine supervision. 
Helps create and curate content to support product usage.
Assists in monitoring results and feedback from product activities.
Supports problem resolution by collecting and reporting on feedback and usage data."""@en .

sfialevels:PROD_3 a sfia:SkillLevel ;
    skos:notation "PROD_3" ;
    sfia:level lor:3 ;
    sfia:skillLevelDescription """Creates and curates various content to support the adoption and usage of products or services. 
Monitors results and feedback from product campaigns. 
Applies standard techniques and tools to carry out analysis and performance monitoring activities for specified products. 
Supports problem resolution, resolves issues and acts on feedback for products in use."""@en .

sfialevels:PROD_4 a sfia:SkillLevel ;
    skos:notation "PROD_4" ;
    sfia:level lor:4 ;
    sfia:skillLevelDescription """Manages one or more lower-value products or services. 
Prioritises product requirements and develops product roadmaps. Owns the product backlog. Manages elements of the product lifecycle to meet customer/user needs and achieve financial or other targets. 
Uses insights from market and/or user research, feedback, expert opinion and usage data to understand needs and opportunities. 
Facilitates uptake of products by developing content, supporting and evaluating campaigns and monitoring product performance. Rolls out product trials and product launches."""@en .

sfialevels:PROD_5 a sfia:SkillLevel ;
    skos:notation "PROD_5" ;
    sfia:level lor:5 ;
    sfia:skillLevelDescription """Manages the full product lifecycle to meet customer/user needs and achieve targets. 
Selects and adapts appropriate product development methods, tools and techniques. 
Uses insights from market and/or user research, feedback and usage data to understand needs and opportunities. Develops product propositions and determines positioning and variants for different segments. Prioritises requirements and develops product roadmaps. 
Coordinates customer testing, product launches and supports communications and training. Adapts products based on changing customer/user needs and creates retirement and transition plans."""@en .

sfialevels:PROD_6 a sfia:SkillLevel ;
    skos:notation "PROD_6" ;
    sfia:level lor:6 ;
    sfia:skillLevelDescription """Oversees the organisation's product and services portfolio and the delivery of customer value and/or user satisfaction. 
Creates the product lifecycle management framework for internal and external customers and users. Champions the value of product management principles and appropriate product development models. 
Aligns the product management objectives with business objectives and authorises the selection and planning of all product management activities. 
Initiates the creation of new products and services. Identifies how developing new products or adapting existing products can create new opportunities."""@en .

sfialevels:PROF_2 a sfia:SkillLevel ;
    skos:notation "PROF_2" ;
    sfia:level lor:2 ;
    sfia:skillLevelDescription """Assists with the compilation of reports for projects, programmes, or portfolios. 
Maintains programme and project files from supplied actual and forecast data.
Works under supervision to support the administrative needs of project teams, contributing to routine project activities."""@en .

sfialevels:PROF_3 a sfia:SkillLevel ;
    skos:notation "PROF_3" ;
    sfia:level lor:3 ;
    sfia:skillLevelDescription """Provides foundational support for projects, programmes, or portfolios. 
Assists with planning, scheduling, tracking and reporting using established tools and processes. Follows recommended solutions to ensure accurate documentation and communication of project progress. 
Collaborates closely with project teams and stakeholders, gathering updates and information to maintain project records and ensure alignment with project objectives.
Participates in project boards, assurance teams and quality review meetings when necessary."""@en .

sfialevels:PROF_4 a sfia:SkillLevel ;
    skos:notation "PROF_4" ;
    sfia:level lor:4 ;
    sfia:skillLevelDescription """Supports programme or project control boards, project assurance teams and quality review meetings.
Takes responsibility for the provision of support services to projects. Uses project control solutions for planning, scheduling and tracking. Sets up and provides guidance on project management software, procedures, processes, tools and techniques.
Provides basic guidance on project proposals. May provide views across projects on topics such as risk, quality, finance, or configuration management.
Works closely with project boards and review meetings, contributing actively to discussions and decisions."""@en .

sfialevels:PROF_5 a sfia:SkillLevel ;
    skos:notation "PROF_5" ;
    sfia:level lor:5 ;
    sfia:skillLevelDescription """Takes responsibility for the provision of portfolio, programme and project support. 
Advises on the available standards, procedures, methods, tools and techniques. 
Evaluates project and/or programme performance and recommends changes where necessary. 
Contributes to reviews and audits of project and programme management to ensure conformance to standards."""@en .

sfialevels:PROF_6 a sfia:SkillLevel ;
    skos:notation "PROF_6" ;
    sfia:level lor:6 ;
    sfia:skillLevelDescription """Leads implementation and delivery of portfolio, programme and project office services. 
Defines the approach/policy and sets standards for the support provided for managing and monitoring portfolios, programmes, and projects. 
Manages resources to ensure delivery of effective services/resources in line with current and planned demand. 
Reviews and improves the delivery portfolio, programme and project office services."""@en .

sfialevels:PROG_2 a sfia:SkillLevel ;
    skos:notation "PROG_2" ;
    sfia:level lor:2 ;
    sfia:skillLevelDescription """Designs, codes, verifies, tests, documents, amends and refactors simple programs/scripts. 
Applies agreed standards, tools and basic security practices to achieve a well-engineered result.
Reviews own work."""@en .

sfialevels:PROG_3 a sfia:SkillLevel ;
    skos:notation "PROG_3" ;
    sfia:level lor:3 ;
    sfia:skillLevelDescription """Designs, codes, verifies, tests, documents, amends and refactors moderately complex programs/scripts. 
Applies agreed standards, tools and security measures to achieve a well-engineered result.
Monitors and reports on progress. Identifies issues related to software development activities. Proposes practical solutions to resolve issues.
Collaborates in reviews of work with others as appropriate."""@en .

sfialevels:PROG_4 a sfia:SkillLevel ;
    skos:notation "PROG_4" ;
    sfia:level lor:4 ;
    sfia:skillLevelDescription """Designs, codes, verifies, tests, documents, amends and refactors complex programs/scripts and integration software services. 
Contributes to the selection of the software development methods, tools, techniques, and security practices.
Applies agreed standards, tools, and security measures to achieve well-engineered outcomes.
Participates in reviews of own work and leads reviews of colleagues' work."""@en .

sfialevels:PROG_5 a sfia:SkillLevel ;
    skos:notation "PROG_5" ;
    sfia:level lor:5 ;
    sfia:skillLevelDescription """Takes technical responsibility across all stages and iterations of software development. 
Plans and drives software construction activities. Adopts and adapts appropriate software development methods, tools and techniques. 
Measures and monitors applications of project/team standards for software construction, including software security. 
Contributes to the development of organisational policies, standards and guidelines for software development."""@en .

sfialevels:PROG_6 a sfia:SkillLevel ;
    skos:notation "PROG_6" ;
    sfia:level lor:6 ;
    sfia:skillLevelDescription """Develops organisational policies, standards and guidelines for software construction and refactoring. 
Plans and leads software construction activities for strategic, large and complex development projects. 
Adapts or develops new methods and organisational capabilities and drives adoption of, and adherence to, policies and standards."""@en .

sfialevels:PRTS_1 a sfia:SkillLevel ;
    skos:notation "PRTS_1" ;
    sfia:level lor:1 ;
    sfia:skillLevelDescription """Executes given process test scripts under supervision to verify business workflows and user journeys. 
Configures basic test environments to simulate business processes.
Uses standard testing tools for process validation, records results and reports issues."""@en .

sfialevels:PRTS_2 a sfia:SkillLevel ;
    skos:notation "PRTS_2" ;
    sfia:level lor:2 ;
    sfia:skillLevelDescription """Designs test cases and scripts to validate key business scenarios and workflows.
Supports the preparation and management of test data under supervision to align with business processes Configures test environments to reflect real-world business processes.
Executes and records manual and automated process tests in line with test plans.
Analyses and reports on test activities, identifying issues and risks related to business process validation."""@en .

sfialevels:PRTS_3 a sfia:SkillLevel ;
    skos:notation "PRTS_3" ;
    sfia:level lor:3 ;
    sfia:skillLevelDescription """Designs process test cases and scripts that cover end-to-end business scenarios. 
Actively participates in requirement and design reviews to refine test plans. Prepares and manages test data that accurately mirrors business processes. 
Configures test environments, executes tests and addresses issues as they arise. Undertakes structured exploratory testing to assess alternative business flows. 
Automates repeatable tests for efficiency. Analyses and reports on outcomes, focusing on impacts to business processes."""@en .

sfialevels:PRTS_4 a sfia:SkillLevel ;
    skos:notation "PRTS_4" ;
    sfia:level lor:4 ;
    sfia:skillLevelDescription """Selects and applies appropriate testing approaches based on business criticality, risk and process complexity. 
Develops, automates and executes detailed test plans focusing on end-to-end process validation. Ensures automated test environments accurately simulate real business processes and workflows. 
Collaborates closely with stakeholders to refine business requirements and ensure full coverage. Identifies and mitigates risks throughout the testing process and addresses issues.
Provides detailed analysis and reports on the impact of test results on business operations, including work done by others."""@en .

sfialevels:PRTS_5 a sfia:SkillLevel ;
    skos:notation "PRTS_5" ;
    sfia:level lor:5 ;
    sfia:skillLevelDescription """Leads process testing activities across all stages of development, ensuring alignment with business objectives and prioritising key workflows based on risk.
Ensures test environments are robust and reflective of actual business operations.
Provides expert advice on process testing, ensuring tests are effective and align with business needs.
Leads efforts to improve the efficiency and reliability of process testing. Identifies gaps and risks and contributes to the development of policies and standards that support comprehensive and risk-based process testing."""@en .

sfialevels:PRTS_6 a sfia:SkillLevel ;
    skos:notation "PRTS_6" ;
    sfia:level lor:6 ;
    sfia:skillLevelDescription """Develops organisational policies, standards and guidelines for process testing, ensuring they align with business strategy and incorporate a risk-based approach.
Plans and leads large-scale process testing initiatives, focusing on validating complex and critical processes.
Leads efforts to optimise and innovate process testing methodologies, integrating them with overall business goals and risk management strategies.
Promotes a culture of quality in process testing, driving adherence to organisational standards and proactive risk mitigation."""@en .

sfialevels:QUAS_2 a sfia:SkillLevel ;
    skos:notation "QUAS_2" ;
    sfia:level lor:2 ;
    sfia:skillLevelDescription """Assists with quality assurance tasks under routine supervision.
Supports the collection of data and evidence related to quality assurance. 
Assists in reviewing records to ensure compliance with quality standards.
Helps identify and report quality issues and discrepancies."""@en .

sfialevels:QUAS_3 a sfia:SkillLevel ;
    skos:notation "QUAS_3" ;
    sfia:level lor:3 ;
    sfia:skillLevelDescription """Contributes to the collection of evidence and the conduct of formal audits or reviews of activities.
Examines records for evidence that appropriate testing and other quality control activities have taken place. 
Determines compliance with organisational directives, standards and procedures and identifies non-compliances, non-conformances and abnormal occurrences."""@en .

sfialevels:QUAS_4 a sfia:SkillLevel ;
    skos:notation "QUAS_4" ;
    sfia:level lor:4 ;
    sfia:skillLevelDescription """Plans, organises and conducts assessment activity and determines whether appropriate quality control has been applied.
Conducts formal assessments or reviews for given domain areas, suppliers or parts of the supply chain. Collates, collects and examines records, analyses the evidence and drafts all or part of formal compliance reports.
Determines the risks associated with findings and non-compliance and proposes corrective actions.
Provides advice and guidance in the use of organisational standards."""@en .

sfialevels:QUAS_5 a sfia:SkillLevel ;
    skos:notation "QUAS_5" ;
    sfia:level lor:5 ;
    sfia:skillLevelDescription """Plans, organises and conducts formal reviews and assessments of complex domains areas, cross-functional areas and across the supply chain.
Evaluates, appraises and identifies non-compliances with organisational standards and determines the underlying reasons for non-compliance.
Prepares and reports on assessment findings and associated risks. Ensures appropriate owners for corrective actions are identified. Identifies opportunities to improve organisational control mechanisms.
Oversees the assurance activities of others, providing advice and expertise to support assurance activity."""@en .

sfialevels:QUAS_6 a sfia:SkillLevel ;
    skos:notation "QUAS_6" ;
    sfia:level lor:6 ;
    sfia:skillLevelDescription """Leads, develops and is accountable for an organisational approach and commitment to quality assurance.
Ensures quality assurance processes and activities are robust and reliable, and appropriately tailored to the organisation's quality objectives. Plans and resources the organisational quality assurance activities, using internal or third-party resources.
Considers the implications of emerging technology, approaches, trends, regulations and legislation.
Monitors and reports on quality assurance activities, levels of compliance and improvement opportunities."""@en .

sfialevels:QUMG_2 a sfia:SkillLevel ;
    skos:notation "QUMG_2" ;
    sfia:level lor:2 ;
    sfia:skillLevelDescription """Assists with quality management tasks under routine supervision.
Supports the development, maintenance and distribution of quality standards.
Helps document and track updates to quality management processes and standards."""@en .

sfialevels:QUMG_3 a sfia:SkillLevel ;
    skos:notation "QUMG_3" ;
    sfia:level lor:3 ;
    sfia:skillLevelDescription """Uses appropriate methods and a systematic approach to developing, maintaining, controlling and distributing quality and environmental standards. 
Makes technical changes to and controls the updates and distribution of quality standards. 
Distributes new and revised standards."""@en .

sfialevels:QUMG_4 a sfia:SkillLevel ;
    skos:notation "QUMG_4" ;
    sfia:level lor:4 ;
    sfia:skillLevelDescription """Assists in the development of new or improved practices and organisational processes or standards. 
Assists projects, functions or teams in planning the quality management for their area of responsibility. 
Facilitates localised improvements to the quality system or services."""@en .

sfialevels:QUMG_5 a sfia:SkillLevel ;
    skos:notation "QUMG_5" ;
    sfia:level lor:5 ;
    sfia:skillLevelDescription """Ensures projects, teams and functions have appropriate practices in place and are meeting required organisational quality levels. 
Advises on the application of appropriate quality management techniques and standards. 
Determines areas where existing processes should change after analysing audit findings. Facilitates improvements to processes by changing approaches and working practices, typically using recognised models. 
Takes responsibility for controlling updating and distributing organisational standards."""@en .

sfialevels:QUMG_6 a sfia:SkillLevel ;
    skos:notation "QUMG_6" ;
    sfia:level lor:6 ;
    sfia:skillLevelDescription """Achieves and maintains compliance against national and international standards, as appropriate. 
Prioritises areas for quality improvement by considering strategy, business objectives and results from internal and external audits. Initiates the application of appropriate quality management techniques in these areas. 
Initiates improvements to processes by changing approaches and working practices, typically using recognised models. 
Identifies and plans systematic corrective action to reduce errors and improve the quality of the systems and services."""@en .

sfialevels:QUMG_7 a sfia:SkillLevel ;
    skos:notation "QUMG_7" ;
    sfia:level lor:7 ;
    sfia:skillLevelDescription """Determines the quality strategy and secures commitment from executive leadership. 
Develops policies for approval and adoption by organisational management. Ensures adequate technology, procedures and resources are in place to support the quality system. 
Plans and monitors the performance of the quality management system and the internal quality audit schedule. 
Determines the extent to which quality policies and quality systems meet organisational needs and reviews as necessary."""@en .

sfialevels:RELM_2 a sfia:SkillLevel ;
    skos:notation "RELM_2" ;
    sfia:level lor:2 ;
    sfia:skillLevelDescription """Assists with release management tasks under routine supervision.
Supports the collection of data and information for release planning and scheduling.
Assists in the preparation of release materials and resources. Helps document and maintain records of release activities.
Participates in basic testing and quality assurance tasks and issue resolution."""@en .

sfialevels:RELM_3 a sfia:SkillLevel ;
    skos:notation "RELM_3" ;
    sfia:level lor:3 ;
    sfia:skillLevelDescription """Supports the planning and scheduling of releases.
Coordinates release activities with relevant teams. Follows defined release processes and procedures.
Participates in testing and quality assurance activities to ensure releases meet standards. Identifies and resolves issues related to the release process.
Documents and reports on release outcomes and communicates findings to stakeholders."""@en .

sfialevels:RELM_4 a sfia:SkillLevel ;
    skos:notation "RELM_4" ;
    sfia:level lor:4 ;
    sfia:skillLevelDescription """Plans and schedules releases in line with business requirements and objectives.
Coordinates release activities across multiple teams and stakeholders. Manages the release lifecycle, ensuring timely and quality deliverables.
Ensures releases meet defined quality, security and compliance standards.
Communicates release plans, progress and outcomes to stakeholders. Conducts post-release reviews and identifies areas for improvement."""@en .

sfialevels:RELM_5 a sfia:SkillLevel ;
    skos:notation "RELM_5" ;
    sfia:level lor:5 ;
    sfia:skillLevelDescription """Develops and maintains release approaches, processes and automation tools.
Oversees the planning and scheduling of complex, large-scale releases. Coordinates release activities across multiple projects and programmes.
Ensures release processes and procedures are applied and that releases can be rolled back as needed. 
Communicates release approaches and outcomes. Conducts post-release analysis and drives continuous improvement."""@en .

sfialevels:RELM_6 a sfia:SkillLevel ;
    skos:notation "RELM_6" ;
    sfia:level lor:6 ;
    sfia:skillLevelDescription """Defines organisational release management strategies, policies and standards.
Aligns release management with overall business strategies and objectives. Ensures the availability of resources and tools for effective release management.
Communicates release strategies and outcomes to stakeholders.
Drives the adoption of new release management techniques and technologies."""@en .

sfialevels:REQM_2 a sfia:SkillLevel ;
    skos:notation "REQM_2" ;
    sfia:level lor:2 ;
    sfia:skillLevelDescription """Uses standard techniques to elicit, specify and document requirements for simple subject areas with clearly-defined boundaries. 
Assists in the definition and management of requirements.  
Assists in the creation of a requirements baseline/backlog.
Assists in investigating and applying changes to requirements."""@en .

sfialevels:REQM_3 a sfia:SkillLevel ;
    skos:notation "REQM_3" ;
    sfia:level lor:3 ;
    sfia:skillLevelDescription """Defines and manages scoping, requirements definition and prioritisation activities for small-scale changes and assists with more complex change initiatives.
Follows agreed standards and applies appropriate techniques to elicit and document detailed requirements. Provides constructive challenge to stakeholders as required. Reviews requirements for errors and omissions. 
Prioritises requirements and documents traceability to source. 
Provides input to the requirements baseline/backlog. Investigates, manages and applies requests for changes to requirements, in line with change management policy."""@en .

sfialevels:REQM_4 a sfia:SkillLevel ;
    skos:notation "REQM_4" ;
    sfia:level lor:4 ;
    sfia:skillLevelDescription """Defines and manages scoping, requirements definition and prioritisation activities for initiatives of medium size and complexity. 
Contributes to selecting the requirements approach. 
Facilitates input from stakeholders, provides constructive challenge and enables effective prioritisation of requirements. 
Establishes requirements baselines or backlogs, obtains appropriate agreement to requirements and ensures traceability to source."""@en .

sfialevels:REQM_5 a sfia:SkillLevel ;
    skos:notation "REQM_5" ;
    sfia:level lor:5 ;
    sfia:skillLevelDescription """Plans and drives scoping, requirements definition and prioritisation activities for large, complex initiatives. 
Selects, adopts and adapts appropriate requirements definition and management methods, tools and techniques. Contributes to the development of organisational methods and standards for requirements management.
Obtains input and agreement to requirements from a diverse range of stakeholders. Negotiates with stakeholders to manage competing priorities and conflicts. 
Establishes requirements baselines or backlogs. Ensures changes to requirements are investigated and managed."""@en .

sfialevels:REQM_6 a sfia:SkillLevel ;
    skos:notation "REQM_6" ;
    sfia:level lor:6 ;
    sfia:skillLevelDescription """Champions the importance and value of requirements management principles and selecting effective requirements management lifecycle models. 
Develops organisational policies, standards and guidelines for requirements definition and management. 
Plans and leads scoping, requirements definition and priority setting for complex, strategic programmes.
Drives adoption of, and adherence to, policies and standards. Develops new methods and organisational capabilities for requirements management."""@en .

sfialevels:RESC_2 a sfia:SkillLevel ;
    skos:notation "RESC_2" ;
    sfia:level lor:2 ;
    sfia:skillLevelDescription """Assists with resourcing tasks under routine supervision.
Helps with recruiting and onboarding new employees.
Supports the documentation and tracking of resourcing activities."""@en .

sfialevels:RESC_3 a sfia:SkillLevel ;
    skos:notation "RESC_3" ;
    sfia:level lor:3 ;
    sfia:skillLevelDescription """Supports managers and teams in resourcing and recruitment activities. 
Uses recommended tools for planning, scheduling and tracking resourcing activity. 
Provides guidance on resource management and recruitment software, procedures, processes, tools and techniques."""@en .

sfialevels:RESC_4 a sfia:SkillLevel ;
    skos:notation "RESC_4" ;
    sfia:level lor:4 ;
    sfia:skillLevelDescription """Facilitates and supports the execution of resourcing activities in collaboration with managers and teams.
Analyses resource requests to determine tasks, skills and effort required. Creates and communicates open positions internally and externally. Conducts interviews and assessments using a planned format and structure.
Implements internal resource allocation matching skills to tasks. Contributes to transitioning of resources, complying with relevant statutory or external regulations and codes of practice."""@en .

sfialevels:RESC_5 a sfia:SkillLevel ;
    skos:notation "RESC_5" ;
    sfia:level lor:5 ;
    sfia:skillLevelDescription """Plans and manages the acquisition and deployment of resources to meet specific needs and ongoing demand.
Defines and manages the implementation of resourcing processes and tools. Advises on available options and customises resourcing approach to meet requirements. Adheres to standards, statutory or external regulations and codes of practice and ensures compliance. 
Engages with external parties in support of resourcing plans.
Measures effectiveness of resourcing processes and implements improvements."""@en .

sfialevels:RESC_6 a sfia:SkillLevel ;
    skos:notation "RESC_6" ;
    sfia:level lor:6 ;
    sfia:skillLevelDescription """Defines resourcing approach for a significant part of the organisation in line with workforce plans and strategic business goals.
Communicates resourcing approach and obtains organisational commitment. Advises on standards, regulations and codes of practice and ensures compliance.
Maintains a strong external network and supplier framework to support sourcing and acquiring resources.
Leads development of plans and budget to ensure the organisation has appropriately skilled resources to meet organisational objectives and commitments. Reviews the ongoing success and effectiveness of resource management processes."""@en .

sfialevels:RESD_2 a sfia:SkillLevel ;
    skos:notation "RESD_2" ;
    sfia:level lor:2 ;
    sfia:skillLevelDescription """Designs, builds and tests simple real-time/embedded components as part of an overall larger systems design. 
Uses appropriate programming languages to drive simple sensors and actuators. 
Applies specialised tools for real-time program analysis and system debugging."""@en .

sfialevels:RESD_3 a sfia:SkillLevel ;
    skos:notation "RESD_3" ;
    sfia:level lor:3 ;
    sfia:skillLevelDescription """Designs, builds and integrates medium-complexity real-time/embedded components as part of an overall larger systems design. 
Follows agreed standards and uses specialised tools for system analysis and optimisation.
Drives specialist hardware, typically sensors and actuators, and optimises component code for performance. 
Applies a range of approaches to the verification and testing of real-time components."""@en .

sfialevels:RESD_4 a sfia:SkillLevel ;
    skos:notation "RESD_4" ;
    sfia:level lor:4 ;
    sfia:skillLevelDescription """Designs, builds and integrates complex real-time/embedded components and sub-systems.
Designs physical layouts that reflect the connection between system components to test and optimise performance. 
Builds system prototypes and simulations to aid development and enable debugging, testing and troubleshooting of embedded software. 
Applies a range of approaches to the validation, verification, and testing of real-time components and sub-systems, using a variety of specialist tools for system analysis and optimisation."""@en .

sfialevels:RESD_5 a sfia:SkillLevel ;
    skos:notation "RESD_5" ;
    sfia:level lor:5 ;
    sfia:skillLevelDescription """Designs and develops real-time/embedded architectures and systems to meet agreed system requirements.
Plans and manages the development of complex real-time/embedded systems and selects the approaches and techniques to be used. 
Analyses design options and trade-offs between hardware and software, makes recommendations and assesses and manages associated risks. Ensures effective validation, verification and testing is undertaken throughout development.
Oversees the integration of multiple sub-systems into the overall system."""@en .

sfialevels:RESD_6 a sfia:SkillLevel ;
    skos:notation "RESD_6" ;
    sfia:level lor:6 ;
    sfia:skillLevelDescription """Provides overall direction and leadership in the development of real-time/embedded systems. 
Develops organisational policies, standards and guidelines for real-time/embedded systems architectures and designs. 
Plans and leads strategic, large and complex real-time/embedded system developments.  Identifies opportunities to exploit new technologies and improve existing technologies and practices.  
Drives adherence to technical strategies, systems architectures and the implementation of risk-based verification, validation and testing. Develops effective implementation and procurement strategies."""@en .

sfialevels:RFEN_2 a sfia:SkillLevel ;
    skos:notation "RFEN_2" ;
    sfia:level lor:2 ;
    sfia:skillLevelDescription """Assists with setting up, tuning and functional checks of radio frequency devices and software. 
Resolves faults down to line replaceable unit level or escalates according to given procedures. 
Carries out user confidence checks and escalates faults according to given procedures. 
Integrates RF devices with software applications using static configurations."""@en .

sfialevels:RFEN_3 a sfia:SkillLevel ;
    skos:notation "RFEN_3" ;
    sfia:level lor:3 ;
    sfia:skillLevelDescription """Deploys, sets up, tunes and calibrates RF devices and software following maintenance schedules and using appropriate tools and test equipment. 
Incorporates hardware/firmware modifications. Interprets automatic fault/performance indications and resolves faults down to discrete component level or escalates according to given procedures. 
Implements communication protocols between system elements in accordance with defined standards. 
Integrates RF devices with software applications, incorporating dynamic reconfiguration of elements under software control to optimise their operational performance."""@en .

sfialevels:RFEN_4 a sfia:SkillLevel ;
    skos:notation "RFEN_4" ;
    sfia:level lor:4 ;
    sfia:skillLevelDescription """Investigates and resolves system-wide fault conditions using a wide range of diagnostic tools and techniques. 
Reconfigures equipment to circumvent temporary outages. Specifies, selects and integrates RF devices in a system. 
Defines internal communication protocols for transmission over the available frequencies. 
Reconfigures devices and software to optimise performance."""@en .

sfialevels:RFEN_5 a sfia:SkillLevel ;
    skos:notation "RFEN_5" ;
    sfia:level lor:5 ;
    sfia:skillLevelDescription """Monitors system performance, recommends equipment modifications and changes to operating procedures, servicing methods and schedules. 
Develops maintenance schedules and procedures. Approves equipment upgrades and modifications. 
Reviews industry and national standards on relevant RF protocols and regulations. 
Measures and evaluates the effectiveness of RF devices and software."""@en .

sfialevels:RFEN_6 a sfia:SkillLevel ;
    skos:notation "RFEN_6" ;
    sfia:level lor:6 ;
    sfia:skillLevelDescription """Provides overall direction and leadership for the use of RF based devices and software. 
Specifies requirements for radio frequency equipment performance and sets maintenance policy. 
Identifies opportunities to exploit new technologies and improve existing technologies and practices.
Develops effective implementation and procurement strategies."""@en .

sfialevels:RLMT_4 a sfia:SkillLevel ;
    skos:notation "RLMT_4" ;
    sfia:level lor:4 ;
    sfia:skillLevelDescription """Deals with problems and issues, managing resolutions, corrective actions, lessons learned and the collection and dissemination of relevant information. 
Implements stakeholder engagement/communications plans.  Collects and uses feedback from customers and stakeholders to help measure the effectiveness of stakeholder management. 
Helps develop and enhance customer and stakeholder relationships."""@en .

sfialevels:RLMT_5 a sfia:SkillLevel ;
    skos:notation "RLMT_5" ;
    sfia:level lor:5 ;
    sfia:skillLevelDescription """Identifies the communications and relationship needs of stakeholder groups. Translates communications/stakeholder engagement strategies into specific activities and deliverables. 
Facilitates open communication and discussion between stakeholders. 
Acts as a single point of contact by developing, maintaining and working to stakeholder engagement strategies and plans.  Provides informed feedback to assess and promote understanding. 
Facilitates business decision-making processes. Captures and disseminates technical and business information."""@en .

sfialevels:RLMT_6 a sfia:SkillLevel ;
    skos:notation "RLMT_6" ;
    sfia:level lor:6 ;
    sfia:skillLevelDescription """Leads the development of comprehensive stakeholder management strategies and plans. 
Establishes and builds long-term, strategic relationships with key stakeholders to support service delivery and change initiatives. 
Acts as a principal point of contact, ensuring effective communication and alignment. Negotiates and ensures agreements meet stakeholder needs.
Oversees the monitoring of stakeholder relationships, capturing lessons learned and providing feedback. Leads initiatives to enhance communication and relationships, promoting collaboration and understanding between all parties."""@en .

sfialevels:RLMT_7 a sfia:SkillLevel ;
    skos:notation "RLMT_7" ;
    sfia:level lor:7 ;
    sfia:skillLevelDescription """Determines the strategic approach to understanding stakeholder objectives and requirements. 
Works with all interested parties to identify stakeholders and establish effective relationships. Establishes and promotes the overall vision for how stakeholder objectives are met and determines organisational roles and alignment. 
Actively manages relationships with the most senior stakeholders and is the ultimate escalation point for issue resolution."""@en .

sfialevels:RMGT_1 a sfia:SkillLevel ;
    skos:notation "RMGT_1" ;
    sfia:level lor:1 ;
    sfia:skillLevelDescription """Follows detailed guidance to acknowledge receipt of records, including the capture of essential metadata.
Delivers digital and physical records in line with agreed procedures."""@en .

sfialevels:RMGT_2 a sfia:SkillLevel ;
    skos:notation "RMGT_2" ;
    sfia:level lor:2 ;
    sfia:skillLevelDescription """Assists in the collection, delivery and retention of records. 
Identifies and applies appropriate metadata.
Uses established methods to transform records between formats or media, following organisational policies and procedures. Identifies and reports potential risks or issues related to information handling and security.
Performs administrative tasks to maintain accessibility, retrievability, integrity, security and protection of records."""@en .

sfialevels:RMGT_3 a sfia:SkillLevel ;
    skos:notation "RMGT_3" ;
    sfia:level lor:3 ;
    sfia:skillLevelDescription """Maintains key metadata for records, including ownership and category information.
Configures routine controls to restrict record operations to approved actions only. Conducts routine searches for records required to support authorised requests. Supports users in finding and accessing records.
Uses ethical and reliable methods to transform data between formats or media, following organisational policies and being aware of potential issues when handling information.
Transforms data between formats or media using ethical and reliable methods. Follows organisational policies and actively identifies potential risks in information handling."""@en .

sfialevels:RMGT_4 a sfia:SkillLevel ;
    skos:notation "RMGT_4" ;
    sfia:level lor:4 ;
    sfia:skillLevelDescription """Supports the implementation of records management policies and practices including the approved disposal of records.
Conducts complex or sensitive searches for records to address authorised requests.
Monitors and reports on the implementation of effective controls for records management including metadata and access controls. Recommends remediation actions as required.
Provides advice and guidance to enable appropriate records management practices to be adopted across the organisation."""@en .

sfialevels:RMGT_5 a sfia:SkillLevel ;
    skos:notation "RMGT_5" ;
    sfia:level lor:5 ;
    sfia:skillLevelDescription """Ensures implementation of records management policies covering all aspects of retention and disposal.
Manages access controls for records, including authorising access and approving the release of potentially sensitive information. Conducts and oversees complex record searches, seeking legal guidance when necessary.
Reviews new change proposals and provides specialist advice on records management. Assesses and manages records-related risks.
Contributes to the development of policy, standards and procedures for compliance with records-related legislation."""@en .

sfialevels:RSCH_2 a sfia:SkillLevel ;
    skos:notation "RSCH_2" ;
    sfia:level lor:2 ;
    sfia:skillLevelDescription """Within given research goals, assists in selection and review of credible and reliable resources. 
Searches for relevant material using specialised websites and sources, reads relevant articles to update knowledge of the relevant field. 
Reports on work carried out and may contribute sections of publication-quality material. 
Curates, under guidance, a personal collection of relevant material."""@en .

sfialevels:RSCH_3 a sfia:SkillLevel ;
    skos:notation "RSCH_3" ;
    sfia:level lor:3 ;
    sfia:skillLevelDescription """Within given research goals, builds on and refines appropriate outline ideas for research, including evaluation, development, demonstration and implementation. 
Applies standard methods to collect and analyse quantitative and qualitative data. Creates research reports to communicate research methodology, findings and conclusions. 
Contributes sections of publication-quality material. 
Uses available resources to update knowledge of any relevant field and curates a personal collection of relevant material. Participates in research communities."""@en .

sfialevels:RSCH_4 a sfia:SkillLevel ;
    skos:notation "RSCH_4" ;
    sfia:level lor:4 ;
    sfia:skillLevelDescription """Builds on and refines appropriate outline ideas for the evaluation, development, demonstration and implementation of research. 
Contributes to research goals and funding proposals. Collects and analyses qualitative and quantitative data as required. 
Contributes to research plans and identifies appropriate opportunities for publication and dissemination of research findings. Makes an active contribution to research communities.
Presents papers at conferences, contributes significant sections of publication-quality material and presents reports to clients."""@en .

sfialevels:RSCH_5 a sfia:SkillLevel ;
    skos:notation "RSCH_5" ;
    sfia:level lor:5 ;
    sfia:skillLevelDescription """Agrees research goals and methods and performs projects to generate original ideas. 
Attracts and manages external research funding. Maintains a strong external network within own area of specialism. 
Provides advice on performing research. Selects and adapts data collection tools and techniques.  Develops, reviews and constructively criticises the research and ideas of others. Shares demonstrations of research findings.
Takes part in professional activities outside own employing organisation. Presents papers at significant conferences, writes articles for specialist journals and presents reports to key stakeholders."""@en .

sfialevels:RSCH_6 a sfia:SkillLevel ;
    skos:notation "RSCH_6" ;
    sfia:level lor:6 ;
    sfia:skillLevelDescription """Develops the organisation's research policy and supervises the work of research functions. 
Promotes activities externally, attracts and manages significant portfolios of research funding. 
Sets research goals and authorises research proposals. Leads strategic and/or interdisciplinary research projects. Maintains a strong external network reaching beyond own immediate area of specialism. 
Takes a leading part in professional activities outside own employing organisation. Presents keynote papers at major conferences, writes articles for high impact journals and presents reports to major clients."""@en .

sfialevels:SALE_3 a sfia:SkillLevel ;
    skos:notation "SALE_3" ;
    sfia:level lor:3 ;
    sfia:skillLevelDescription """Identifies new leads and prospects and communicates them to the sales manager. 
Responds to assigned sales leads. Assists in maintaining relationships with existing customers and identifies potential opportunities for additional sales or services.
Applies agreed standards and tools to perform simple sales tasks or support complex sales processes. 
Monitors and reports on assigned sales quota, performance, customer satisfaction, market intelligence and competitors."""@en .

sfialevels:SALE_4 a sfia:SkillLevel ;
    skos:notation "SALE_4" ;
    sfia:level lor:4 ;
    sfia:skillLevelDescription """Identifies and qualifies new sales leads and prospects with a view to developing a pipeline of potential opportunities. 
Manages existing sales leads. 
Collects and uses information to achieve sales objectives. 
Understands customers and their needs, and develops and enhances customer relationships before, during and after the conclusion of agreements/contracts. Identifies opportunities for upselling and cross-selling within the existing customer base."""@en .

sfialevels:SALE_5 a sfia:SkillLevel ;
    skos:notation "SALE_5" ;
    sfia:level lor:5 ;
    sfia:skillLevelDescription """Designs and implements sales strategies and works with senior management to implement sales plans. 
Develops and maintains effective customer relationships at executive levels and qualifies new sales leads. Collaborates with bid teams to align sales strategies.
Agrees and signs contracts. Maintains customer contact during and after sales to pre-empt issues and identify opportunities. Develops strategies for account growth and retention. Implements initiatives to ensure long-term value and loyalty.
Plans, monitors and controls sales teams. Contributes to the development of sales teams and product/service development."""@en .

sfialevels:SALE_6 a sfia:SkillLevel ;
    skos:notation "SALE_6" ;
    sfia:level lor:6 ;
    sfia:skillLevelDescription """Oversees the organisation's sales activities to align with business objectives.
Approves sales proposals and targets. Develops sales policy and strategy, and contributes to the marketing strategy. Works with bid management to ensure sales strategies are effectively represented in major proposals.
Negotiates with senior customer representatives on technical and contractual issues. Agrees and signs contracts.
Collaborates on evolving services, products, systems and contracts to meet future customer needs. Implements strategies for lifetime customer value and partnerships. Oversees key account management programmes."""@en .

sfialevels:SCAD_1 a sfia:SkillLevel ;
    skos:notation "SCAD_1" ;
    sfia:level lor:1 ;
    sfia:skillLevelDescription """Performs simple security administration tasks. 
Maintains relevant records and documentation, contributing to overall data integrity."""@en .

sfialevels:SCAD_2 a sfia:SkillLevel ;
    skos:notation "SCAD_2" ;
    sfia:level lor:2 ;
    sfia:skillLevelDescription """Receives and responds to routine requests for security support. Maintains records and effectively communicates actions taken.
Assists in the investigation and resolution of issues relating to security systems using basic diagnostic tools and techniques.
Documents incident and event information and generates reports on exceptions and security events. Contributes to management reporting processes."""@en .

sfialevels:SCAD_3 a sfia:SkillLevel ;
    skos:notation "SCAD_3" ;
    sfia:level lor:3 ;
    sfia:skillLevelDescription """Investigates minor security breaches using established procedures, incorporating analytical tools and techniques.
Performs non-standard operational security tasks adapting to evolving technologies and threat landscapes.
Addresses and resolves a variety of security events to maintain system integrity and operational continuity."""@en .

sfialevels:SCAD_4 a sfia:SkillLevel ;
    skos:notation "SCAD_4" ;
    sfia:level lor:4 ;
    sfia:skillLevelDescription """Maintains and optimises operational security processes. Checks that all requests for support are dealt with according to established protocols, including for cloud-based and automated systems.
Provides advice on implementing and managing physical, procedural and technical security encompassing both physical and digital assets.
Investigates security breaches in accordance with established procedures using advanced tools and techniques and recommends necessary corrective actions. 
Enables effective implementation of recommended security measures and monitors their performance."""@en .

sfialevels:SCAD_5 a sfia:SkillLevel ;
    skos:notation "SCAD_5" ;
    sfia:level lor:5 ;
    sfia:skillLevelDescription """Oversees security operations procedures, ensuring adherence and effectiveness, including cloud security practices and automated threat responses.
Reviews actual or potential security breaches and vulnerabilities and ensures they are promptly and thoroughly investigated. Recommends actions and appropriate control improvements.
Ensures the integrity and completeness of security records, ensuring timely support and adherence to established procedures.
Contributes to the creation and maintenance of security policies, standards and procedures integrating new compliance requirements and technology advances."""@en .

sfialevels:SCAD_6 a sfia:SkillLevel ;
    skos:notation "SCAD_6" ;
    sfia:level lor:6 ;
    sfia:skillLevelDescription """Develops comprehensive policies, standards, processes and guidelines for organisational security across the entire digital landscape.
Ensures the ongoing relevance and effective implementation of security policies and standards, adapting to emerging technologies and threats.
Reviews and advises on security aspects of new business initiatives considering implications in the evolving digital landscape.
Leads strategic planning for security operations, integrating advanced threat intelligence and automation to enhance organisational resilience."""@en .

sfialevels:SCMG_2 a sfia:SkillLevel ;
    skos:notation "SCMG_2" ;
    sfia:level lor:2 ;
    sfia:skillLevelDescription """Assists with service catalogue management tasks under routine supervision.
Supports the collection and updating of service and product information.
Helps maintain the accuracy and relevance of the service catalogue."""@en .

sfialevels:SCMG_3 a sfia:SkillLevel ;
    skos:notation "SCMG_3" ;
    sfia:level lor:3 ;
    sfia:skillLevelDescription """Collates information needed to populate the service catalogue. 
Edits and maintains service and product descriptions and keeps the list of available services up to date. 
Acts as a contact point, receiving and handling routine updates to the service catalogue. 
Identifies opportunities to improve service catalogue management processes."""@en .

sfialevels:SCMG_4 a sfia:SkillLevel ;
    skos:notation "SCMG_4" ;
    sfia:level lor:4 ;
    sfia:skillLevelDescription """Contributes to the design and implementation of a service catalogue.
Enables automation of service requests and order fulfilment. 
Provides advice and guidance on the information to be included in the service catalogue. 
Contributes to reviews and improvement of the catalogue and of service catalogue management processes."""@en .

sfialevels:SCMG_5 a sfia:SkillLevel ;
    skos:notation "SCMG_5" ;
    sfia:level lor:5 ;
    sfia:skillLevelDescription """Manages the creation and maintenance of a catalogue of services. 
Ensures the service catalogue is complete and current. Works with service owners to ensure consistency and accuracy of the service catalogue entries. 
Completes regular reviews of the catalogue with stakeholders to ensure relevance to business needs and requirements. 
Manages the service catalogue management processes."""@en .

sfialevels:SCMO_4 a sfia:SkillLevel ;
    skos:notation "SCMO_4" ;
    sfia:level lor:4 ;
    sfia:skillLevelDescription """Analyses the real-world problem, then selects appropriate physical and mathematical models to approximate the phenomena under investigation. 
Applies relevant mathematical techniques to simulate the problem. 
Conducts quality and performance assessments on computational model outputs and makes improvements to the models. 
Provides advice and guidance to the users of these models."""@en .

sfialevels:SCMO_5 a sfia:SkillLevel ;
    skos:notation "SCMO_5" ;
    sfia:level lor:5 ;
    sfia:skillLevelDescription """Investigates real-world problems to assess whether existing scientific models provide effective solutions.
Creates new mathematical representations of the underlying science that can be implemented in a computational model. Applies advanced programming techniques to implement scientific models and apply these for problem-solving. 
Analyses the functioning of existing computational models to improve accuracy and performance. 
Communicates limitations such as uncertainty and systematic errors. Ensures appropriate usage of computational models."""@en .

sfialevels:SCMO_6 a sfia:SkillLevel ;
    skos:notation "SCMO_6" ;
    sfia:level lor:6 ;
    sfia:skillLevelDescription """Initiates the creation, testing, improvement and application of mathematical model frameworks representing real-world systems and scientific theories. 
Sets standards and approaches for the application of scientific modelling. 
Oversees the representation of science and mathematics principles and theories in models to ensure appropriate, consistent and effective usage. 
Develops or introduces new mathematical techniques where necessary."""@en .

sfialevels:SCMO_7 a sfia:SkillLevel ;
    skos:notation "SCMO_7" ;
    sfia:level lor:7 ;
    sfia:skillLevelDescription """Directs the creation and review of a cross-functional, enterprise-wide approach and culture for scientific modelling. 
Leads the development of the organisation's scientific modelling capabilities and champions its use in solving real-world problems."""@en .

sfialevels:SCTY_2 a sfia:SkillLevel ;
    skos:notation "SCTY_2" ;
    sfia:level lor:2 ;
    sfia:skillLevelDescription """Assists with implementing and monitoring security policies and protocols across different systems.
Contributes to identifying and addressing potential risks in security governance and compliance.
Supports the analysis of documented security incidents, escalating where appropriate.
Assists in the review of access controls and permissions, ensuring adherence to security policies."""@en .

sfialevels:SCTY_3 a sfia:SkillLevel ;
    skos:notation "SCTY_3" ;
    sfia:level lor:3 ;
    sfia:skillLevelDescription """Applies and maintains specific security controls as required by organisational policy and local risk assessments.
Communicates security risks and issues to business managers and others. Performs basic risk assessments for small information systems. 
Contributes to the identification of risks that arise from potential technical solution architectures. Suggests alternate solutions or countermeasures to mitigate risks. Defines secure systems configurations in compliance with intended architectures.
Supports investigation of suspected attacks and security breaches."""@en .

sfialevels:SCTY_4 a sfia:SkillLevel ;
    skos:notation "SCTY_4" ;
    sfia:level lor:4 ;
    sfia:skillLevelDescription """Provides guidance on the application and operation of elementary physical, procedural and technical security controls. 
Explains the purpose of security controls and performs security risk and business impact analysis for medium complexity information systems. 
Identifies risks that arise from potential technical solution architectures. Designs alternate solutions or countermeasures and ensures they manage identified risks. 
Investigates suspected attacks and supports security incident management."""@en .

sfialevels:SCTY_5 a sfia:SkillLevel ;
    skos:notation "SCTY_5" ;
    sfia:level lor:5 ;
    sfia:skillLevelDescription """Provides advice and guidance on security strategies to manage identified risks and ensure adoption and adherence to standards. 
Contributes to development of information security policy, standards and guidelines. 
Obtains and acts on vulnerability information and conducts security risk assessments, business impact analysis and accreditation on complex information systems. Investigates major breaches of security and recommends appropriate control improvements. 
Develops new architectures that manage the risks posed by new technologies and business practices."""@en .

sfialevels:SCTY_6 a sfia:SkillLevel ;
    skos:notation "SCTY_6" ;
    sfia:level lor:6 ;
    sfia:skillLevelDescription """Develops and communicates corporate information security policy, standards and guidelines.  
Ensures architectural principles are applied during design to reduce risk. Drives adoption and adherence to policy, standards and guidelines. 
Contributes to the development of organisational strategies that address information control requirements. Identifies and monitors environmental and market trends and proactively assesses impact on business strategies, benefits and risks. 
Leads the provision of authoritative advice and guidance on the requirements for security controls in collaboration with subject matter experts."""@en .

sfialevels:SCTY_7 a sfia:SkillLevel ;
    skos:notation "SCTY_7" ;
    sfia:level lor:7 ;
    sfia:skillLevelDescription """Directs the development, implementation, delivery and support of an enterprise information security strategy aligned with the business strategy. 
Ensures compliance between business strategies and information security. 
Leads the provision of information security expertise, guidance and systems needed to execute strategic and operational plans.
Secures organisational resources to execute the information security strategy."""@en .

sfialevels:SEAC_3 a sfia:SkillLevel ;
    skos:notation "SEAC_3" ;
    sfia:level lor:3 ;
    sfia:skillLevelDescription """Applies standard service acceptance criteria and participates in service acceptance testing. 
Collaborates with delivery teams to ensure service deliverables meet the required standards. 
Documents and communicates the outcomes of service acceptance activities. 
Identifies and reports issues or non-conformances, assisting with their resolution."""@en .

sfialevels:SEAC_4 a sfia:SkillLevel ;
    skos:notation "SEAC_4" ;
    sfia:level lor:4 ;
    sfia:skillLevelDescription """Engages with delivery teams to confirm that products developed meet the service acceptance criteria and are to the required standard. 
Assesses risks related to service acceptance and suggests actions to address identified risks. 
Facilitates the communication of acceptance criteria across teams to maintain alignment and consistency throughout the process.
Provides input into change control processes."""@en .

sfialevels:SEAC_5 a sfia:SkillLevel ;
    skos:notation "SEAC_5" ;
    sfia:level lor:5 ;
    sfia:skillLevelDescription """Engages with delivery teams to ensure correct products are produced in a timely fashion. 
Leads the assessment of complex or critical service deliverables, ensuring they meet both current and future operational needs. Leads comprehensive risk evaluations identifying and prioritising risks that may impact service readiness. 
Provides authoritative advice on service acceptance practices. Provides recommendations for enhancing service readiness and improving service acceptance processes.
Evaluates the quality of project outputs against agreed service acceptance criteria."""@en .

sfialevels:SEAC_6 a sfia:SkillLevel ;
    skos:notation "SEAC_6" ;
    sfia:level lor:6 ;
    sfia:skillLevelDescription """Develops the organisation's approach for service acceptance, owns the transition process and defines the acceptance criteria for service transitions.
Ensures risk management activities are aligned with the organisation's broader risk management framework. Promotes and monitors project quality outputs to ensure they are fit for purpose and fit for use within operational services. 
Actively engages with stakeholders to promote awareness and compliance with service transition quality plans and processes. 
Agrees the service acceptance criteria with delivery teams."""@en .

sfialevels:SFAS_4 a sfia:SkillLevel ;
    skos:notation "SFAS_4" ;
    sfia:level lor:4 ;
    sfia:skillLevelDescription """Collects safety assurance evidence using appropriate methods and tools. 
Undertakes all work in accordance with agreed safety, technical and quality standards."""@en .

sfialevels:SFAS_5 a sfia:SkillLevel ;
    skos:notation "SFAS_5" ;
    sfia:level lor:5 ;
    sfia:skillLevelDescription """Undertakes safety analyses using agreed techniques to verify or validate that safety requirements are implemented. 
Participates in system safety assessments.
Creates safety assessment reports and recommends and defines how a system's safety requirements can be satisfied."""@en .

sfialevels:SFAS_6 a sfia:SkillLevel ;
    skos:notation "SFAS_6" ;
    sfia:level lor:6 ;
    sfia:skillLevelDescription """Champions and promotes safety practices in the organisation. 
Leads safety assessments according to organisational safety policies and standards.
Defines and implements organisational policies and standards for system safety assessment.
Assures compliance with defined standards and policies and oversees overall safety lifecycle assessment activities."""@en .

sfialevels:SFEN_2 a sfia:SkillLevel ;
    skos:notation "SFEN_2" ;
    sfia:level lor:2 ;
    sfia:skillLevelDescription """Assists with safety engineering tasks under routine supervision.
Supports the documentation of hazard and risk analysis activities.
Helps collect safety assurance evidence using agreed methods and procedures."""@en .

sfialevels:SFEN_3 a sfia:SkillLevel ;
    skos:notation "SFEN_3" ;
    sfia:level lor:3 ;
    sfia:skillLevelDescription """Contributes to hazard and risk analysis during system development and implementation using agreed methods and procedures. 
Documents the results of hazard and risk analysis activities.
Contributes to the collection of safety assurance evidence using appropriate methods and tools. 
Undertakes all work in accordance with agreed safety, technical and quality standards."""@en .

sfialevels:SFEN_4 a sfia:SkillLevel ;
    skos:notation "SFEN_4" ;
    sfia:level lor:4 ;
    sfia:skillLevelDescription """Contributes to identifying, analysing and documenting hazards and safety risks using agreed methods and procedures.
Contributes to the specification of safety requirements. 
Analyses and documents safety validation results during system development and implementation.
Contributes to developing and maintaining project safety assurance plans. Gathers safety assurance evidence for safety case preparation."""@en .

sfialevels:SFEN_5 a sfia:SkillLevel ;
    skos:notation "SFEN_5" ;
    sfia:level lor:5 ;
    sfia:skillLevelDescription """Identifies and analyses hazards and contributes to identifying and evaluating risk reduction measures, ensuring these are adequately documented. 
Specifies safety-related systems architectures for defined safety levels. 
Develops and maintains project safety assurance plans. Monitors implementation and compliance. Ensures safety assurance evidence is gathered for safety case preparation.
Works with system architects, designers and developers to assure safety requirements implementation."""@en .

sfialevels:SFEN_6 a sfia:SkillLevel ;
    skos:notation "SFEN_6" ;
    sfia:level lor:6 ;
    sfia:skillLevelDescription """Takes full responsibility for hazard analysis and risk evaluation, safety-related systems architectural design and safety compliance planning.
Leads the definition and allocation of safety requirements for the system, according to the system's nature and required safety level.  
Takes responsibility for the safety-related aspects of multiple complex or high safety integrity level projects."""@en .

sfialevels:SINT_2 a sfia:SkillLevel ;
    skos:notation "SINT_2" ;
    sfia:level lor:2 ;
    sfia:skillLevelDescription """Produces builds from system components using appropriate build automation tools and processes.
Conducts tests as defined in an integration test specification and records the details of any failures.
Analyses and reports on integration test activities and results. Identifies and reports issues and risks."""@en .

sfialevels:SINT_3 a sfia:SkillLevel ;
    skos:notation "SINT_3" ;
    sfia:level lor:3 ;
    sfia:skillLevelDescription """Defines the modules and components and dependencies needed for an integration build and produces a build definition. Accepts completed modules and components, checking that they meet defined criteria.
Produces builds from system components for loading onto target environments. 
Configures the hardware, software and infrastructure environment as required by the system being integrated. 
Produces integration test specifications, conducts tests and records and reports on outcomes. Diagnoses faults and documents the results of tests. Produces system integration reports."""@en .

sfialevels:SINT_4 a sfia:SkillLevel ;
    skos:notation "SINT_4" ;
    sfia:level lor:4 ;
    sfia:skillLevelDescription """Provides technical expertise to enable the configuration of system components and equipment for systems testing.
Collaborates with technical teams to develop and agree system integration plans and report on progress. Defines complex/new integration builds. Ensures integration test environments are correctly configured.
Designs, performs and reports results of tests of the integration build. Identifies and documents system integration components for recording in the configuration management system.
Recommends and implements improvements to processes and tools."""@en .

sfialevels:SINT_5 a sfia:SkillLevel ;
    skos:notation "SINT_5" ;
    sfia:level lor:5 ;
    sfia:skillLevelDescription """Plans and drives activities to develop organisational systems integration and build capabilities including automation and continuous integration.
Identifies, evaluates and manages the adoption of tools, techniques and processes to create a robust integration framework. Provides authoritative advice and guidance on any aspect of systems integration.
Leads integration work in line with the agreed system and service design. Assesses risks and takes preventative action. Measures and monitors applications of standards.
Contributes to the development of organisational policies, standards and guidelines for systems integration."""@en .

sfialevels:SINT_6 a sfia:SkillLevel ;
    skos:notation "SINT_6" ;
    sfia:level lor:6 ;
    sfia:skillLevelDescription """Leads the development of organisational systems integration and build capabilities including automation and continuous integration.
Develops organisational policies, standards and guidelines for systems integration and build.
Provides resources to ensure systems integration and build can operate effectively and ensures adoption and adherence to policies and standards."""@en .

sfialevels:SLEN_3 a sfia:SkillLevel ;
    skos:notation "SLEN_3" ;
    sfia:level lor:3 ;
    sfia:skillLevelDescription """Provides support for implementing systems and software lifecycle practices by applying established methods and procedures. 
Supports automation and continuous integration processes under direction. 
Monitors and reports on the effectiveness of lifecycle management activities. 
Contributes to the documentation and maintenance of lifecycle tools and practices."""@en .

sfialevels:SLEN_4 a sfia:SkillLevel ;
    skos:notation "SLEN_4" ;
    sfia:level lor:4 ;
    sfia:skillLevelDescription """Elicits requirements for systems and software lifecycle working practices and automation.
Prepares design options for the working environment of methods, procedures, techniques, tools and people. 
Selects systems and software lifecycle working practices for software components and micro-services. 
Deploys automation to achieve well-engineered and secure outcomes."""@en .

sfialevels:SLEN_5 a sfia:SkillLevel ;
    skos:notation "SLEN_5" ;
    sfia:level lor:5 ;
    sfia:skillLevelDescription """Collaborates with those responsible for ongoing systems and software lifecycle management to select, adopt and adapt working practices.
Supports deployment of the working environment for systems and software lifecycle working practices.
Provides effective feedback to encourage development of the individuals and teams responsible for systems and software lifecycle working practices. Provides guidance and makes suggestions to support continual improvement and learning approach.
Contributes to identifying new domains within the organisation where systems and software lifecycle working practices can be deployed."""@en .

sfialevels:SLEN_6 a sfia:SkillLevel ;
    skos:notation "SLEN_6" ;
    sfia:level lor:6 ;
    sfia:skillLevelDescription """Obtains organisational commitment to strategies to deliver systems and software lifecycle working practices to achieve business objectives. 
Works with others to integrate organisational policies, standards and techniques across the full software and systems lifecycle. 
Develops and deploys the working environment supporting systems and software lifecycle practices for strategic, large and complex products and services. 
Leads activities to manage risks associated with systems and software lifecycle working practices. Plans and manages the evaluation or assessment of systems and software lifecycle working practices"""@en .

sfialevels:SLEN_7 a sfia:SkillLevel ;
    skos:notation "SLEN_7" ;
    sfia:level lor:7 ;
    sfia:skillLevelDescription """Represents and leads systems and software lifecycle working practices at the highest level in the organisation.
Identifies opportunities for innovation in systems and software lifecycle working practices to achieve organisational goals and objectives. 
Leads the essential cultural and environmental changes and communicates the benefits to all stakeholders. 
Oversees the quality of the work performed and delivers measurable business benefits."""@en .

sfialevels:SLMO_2 a sfia:SkillLevel ;
    skos:notation "SLMO_2" ;
    sfia:level lor:2 ;
    sfia:skillLevelDescription """Monitors and logs the actual service provided. 
Compares delivered service to service level agreements, identifying any deviations or areas for improvement."""@en .

sfialevels:SLMO_3 a sfia:SkillLevel ;
    skos:notation "SLMO_3" ;
    sfia:level lor:3 ;
    sfia:skillLevelDescription """Monitors service delivery performance metrics. 
Liaises with stakeholders to help them plan for a deterioration in service and/or breaches of service level agreements."""@en .

sfialevels:SLMO_4 a sfia:SkillLevel ;
    skos:notation "SLMO_4" ;
    sfia:level lor:4 ;
    sfia:skillLevelDescription """Performs defined tasks to monitor service delivery against service level agreements and maintains records of relevant information. 
Analyses service delivery performance to identify actions required to maintain or improve levels of service.
Initiates and reports on actions to maintain or improve levels of service."""@en .

sfialevels:SLMO_5 a sfia:SkillLevel ;
    skos:notation "SLMO_5" ;
    sfia:level lor:5 ;
    sfia:skillLevelDescription """Ensures service delivery meets agreed service levels. 
Negotiates service level requirements and agreed service levels with customers. 
Diagnoses service delivery problems and initiates actions to maintain or improve levels of service. 
Establishes and maintains operational methods, procedures and facilities and reviews them regularly for effectiveness and efficiency."""@en .

sfialevels:SLMO_6 a sfia:SkillLevel ;
    skos:notation "SLMO_6" ;
    sfia:level lor:6 ;
    sfia:skillLevelDescription """Ensures service delivery is monitored effectively and that identified actions to maintain or improve levels of service are implemented. 
Ensures service level agreements are complete and cost-effective across the catalogue of available services. Ensures operational methods, procedures, facilities and tools are established, reviewed and maintained. Prepares proposals to meet forecast changes in the levels or types of services.
Reviews service delivery to ensure agreed targets are met. 
Negotiates with relevant parties in respect of disruptions and major amendments to the provision of services."""@en .

sfialevels:SLMO_7 a sfia:SkillLevel ;
    skos:notation "SLMO_7" ;
    sfia:level lor:7 ;
    sfia:skillLevelDescription """Sets strategies for service delivery that support the strategic needs of the client organisation. 
Authorises allocation of resources for monitoring service delivery arrangements. 
Develops relationships with customers at the highest level to identify potential areas of mutual commercial interest for future development. 
Maintains an overview of the contribution of service delivery arrangements to organisational success. Provides leadership within the industry on the identification of future trends."""@en .

sfialevels:SORC_2 a sfia:SkillLevel ;
    skos:notation "SORC_2" ;
    sfia:level lor:2 ;
    sfia:skillLevelDescription """Assists in the preparation of pre-qualification questionnaires and tender invitations in response to business cases. 
Assembles relevant  information for tenders. 
Produces detailed evaluation criteria for simple tender criteria. 
Assists in the evaluation of tenders."""@en .

sfialevels:SORC_3 a sfia:SkillLevel ;
    skos:notation "SORC_3" ;
    sfia:level lor:3 ;
    sfia:skillLevelDescription """Prepares pre-qualification questionnaires and tender invitations in response to business cases. 
Recognises the difference between open source and proprietary systems options. 
Applies standard procedures and tools to produce detailed evaluation criteria for complex tenders and to evaluate tenders."""@en .

sfialevels:SORC_4 a sfia:SkillLevel ;
    skos:notation "SORC_4" ;
    sfia:level lor:4 ;
    sfia:skillLevelDescription """Reviews business cases (requirements, potential benefits and options) and determines appropriate procurement routes. 
Using market knowledge to inform specifications, ensures detailed pre-qualification questionnaires and tender invitations are prepared. 
Collects and collates data to support collaboration and negotiates terms and conditions to reflect the scale of requirements and encourage optimal performance. 
Evaluates tenders based on specification and evaluation criteria, prepares acceptance documentation and advises on contracts and service level agreements."""@en .

sfialevels:SORC_5 a sfia:SkillLevel ;
    skos:notation "SORC_5" ;
    sfia:level lor:5 ;
    sfia:skillLevelDescription """Plans and manages procurement activities. 
Manages tender, evaluation and acquisition processes. Researches suppliers and markets, and maintains a broad understanding of the commercial environment, to inform and develop commercial strategies and sourcing plans. 
Advises on the business case for alternative sourcing models. Advises on policy and procedures covering tendering, the selection of suppliers and procurement. 
Negotiates with potential partners and suppliers, developing acceptance criteria and procedures. Drafts and places contracts."""@en .

sfialevels:SORC_6 a sfia:SkillLevel ;
    skos:notation "SORC_6" ;
    sfia:level lor:6 ;
    sfia:skillLevelDescription """Develops policy and procedures for sourcing and procurement activities. 
Establishes procurement strategies, standards, methods, processes and good practices that ensure compliance with legislation, regulation and information security requirements.
Leads the procurement process, from clarifying requirements through to placing, monitoring and terminating contracts. Conducts complex negotiations and sets parameters for routine negotiations. Ensures terms and conditions align with organisational requirements, current legislation and policy.
Identifies external partners, engaging with professionals in related disciplines as appropriate."""@en .

sfialevels:SORC_7 a sfia:SkillLevel ;
    skos:notation "SORC_7" ;
    sfia:level lor:7 ;
    sfia:skillLevelDescription """Shapes and leads the organisation's overarching sourcing and procurement strategies, ensuring alignment with the global business vision and long-term objectives.
Assumes full accountability for all sourcing and procurement activities, guiding the organisation's sourcing vision and strategic procurement decisions.
Strategically develops, deploys and continually assesses procurement processes to align with dynamic market conditions and organisational goals.
Leads high-level negotiations for major, organisation-defining contracts, setting negotiation frameworks and strategies that significantly impact the organisation's market position and success."""@en .

sfialevels:SSUP_1 a sfia:SkillLevel ;
    skos:notation "SSUP_1" ;
    sfia:level lor:1 ;
    sfia:skillLevelDescription """Communicates effectively with customers to provide basic information about products and services.
Seeks assistance from colleagues for the resolution of more complex customer service queries and complaints. 
Uses sales support systems to retrieve and enter data."""@en .

sfialevels:SSUP_2 a sfia:SkillLevel ;
    skos:notation "SSUP_2" ;
    sfia:level lor:2 ;
    sfia:skillLevelDescription """Communicates effectively with customers by telephone and in person. 
Assists in providing customer service, including technical advice and guidance on the successful use of products and services. 
Assists in devising solutions to customer requirements and solves straightforward problems."""@en .

sfialevels:SSUP_3 a sfia:SkillLevel ;
    skos:notation "SSUP_3" ;
    sfia:level lor:3 ;
    sfia:skillLevelDescription """Helps customers to clarify their requirements and documents the conclusions reached. 
Contributes to preparing and supporting bids and sales proposals. 
Provides customer service, including technical advice and guidance on the successful use of complex products and services."""@en .

sfialevels:SSUP_4 a sfia:SkillLevel ;
    skos:notation "SSUP_4" ;
    sfia:level lor:4 ;
    sfia:skillLevelDescription """Works closely with the sales team to help prospects to clarify their requirements. 
Devises solutions and assesses their feasibility and practicality. 
Demonstrates technical feasibility using physical or simulation models. Resolves technical problems.
Produces estimates of cost and risk and initial project plans to inform sales proposals."""@en .

sfialevels:SSUP_5 a sfia:SkillLevel ;
    skos:notation "SSUP_5" ;
    sfia:level lor:5 ;
    sfia:skillLevelDescription """Works closely with the sales team to ensure customers are assisted and advised appropriately. 
Ensures reliable cost, effort and risk estimates and project plans are produced. 
Manages all sales support activities, taking full responsibility for the technical content of bids and sales proposals. 
Establishes metrics to provide data on performance and support continual improvement of sales support activities."""@en .

sfialevels:SSUP_6 a sfia:SkillLevel ;
    skos:notation "SSUP_6" ;
    sfia:level lor:6 ;
    sfia:skillLevelDescription """Leads the organisation's sales-related customer service activities to ensure they are aligned with corporate objectives and policy. 
Approves proposals and initiates the implementation of development activity in customer services and systems."""@en .

sfialevels:STMG_2 a sfia:SkillLevel ;
    skos:notation "STMG_2" ;
    sfia:level lor:2 ;
    sfia:skillLevelDescription """Assists with storage management tasks such as provisioning.
Supports the setup and configuration of storage systems, incorporating standard security practices.
Helps monitor storage performance and capacity, and documents storage utilisation."""@en .

sfialevels:STMG_3 a sfia:SkillLevel ;
    skos:notation "STMG_3" ;
    sfia:level lor:3 ;
    sfia:skillLevelDescription """Executes routine storage management tasks following established procedures and using standard tools.
Implements documented configurations for allocation of storage, installation and maintenance of secure storage systems using the agreed operational procedures.
Identifies operational problems, including security-related issues, and contributes to their resolution.
Uses standard management and reporting tools to collect and report on storage utilisation, performance and backup statistics."""@en .

sfialevels:STMG_4 a sfia:SkillLevel ;
    skos:notation "STMG_4" ;
    sfia:level lor:4 ;
    sfia:skillLevelDescription """Prepares and maintains operational procedures for storage management. 
Monitors capacity, performance, availability and other operational metrics. Takes appropriate action to ensure corrective and proactive maintenance of storage and backup systems to protect and secure business information. 
Creates reports and proposals for improvement. 
Contributes to the planning and implementation of new installations and scheduled maintenance and changes of existing systems."""@en .

sfialevels:STMG_5 a sfia:SkillLevel ;
    skos:notation "STMG_5" ;
    sfia:level lor:5 ;
    sfia:skillLevelDescription """Develops standards and guidelines for implementing data protection and disaster recovery functionality for all business applications and business data. 
Provides authoritative advice and guidance to implement and improve storage management.  
Manages storage and backup systems to provide agreed service levels. 
Creates, improves and supports storage management services with optimal utilisation of storage resources, ensuring security, availability and integrity of data."""@en .

sfialevels:STMG_6 a sfia:SkillLevel ;
    skos:notation "STMG_6" ;
    sfia:level lor:6 ;
    sfia:skillLevelDescription """Develops organisational policies, standards and guidelines for storage management.
Develops strategies for managing storage and data based on the level of criticality of the information. 
Ensures compliance with regulatory and security requirements. 
Aligns investments in storage management with business goals and data management policies."""@en .

sfialevels:STPL_5 a sfia:SkillLevel ;
    skos:notation "STPL_5" ;
    sfia:level lor:5 ;
    sfia:skillLevelDescription """Develops models and plans to drive the execution of the business strategy, taking advantage of opportunities to improve business performance. 
Contributes to creating and reviewing a systems capability strategy which meets the business's strategic requirements. 
Creates and maintains roadmaps to guide the execution of business strategy and capability improvements.
Determines requirements and specifies effective business processes, through improvements in technology, information or data practices, organisation, roles, procedures and equipment."""@en .

sfialevels:STPL_6 a sfia:SkillLevel ;
    skos:notation "STPL_6" ;
    sfia:level lor:6 ;
    sfia:skillLevelDescription """Develops enterprise-wide architecture and processes to embed strategic change management within the organisation. 
Leads the creation and review of a systems capability strategy aligned with business requirements. Develops roadmaps for enterprise architecture and initiatives, ensuring stakeholder buy-in. 
Captures and prioritises market and environmental trends, business strategies and objectives, identifying alternative strategies.  Develops business cases for approval, funding and prioritisation of high-level initiatives.
Sets strategies, policies, standards and practices to ensure compliance between business strategies, technology strategies and enterprise transformation activities."""@en .

sfialevels:STPL_7 a sfia:SkillLevel ;
    skos:notation "STPL_7" ;
    sfia:level lor:7 ;
    sfia:skillLevelDescription """Directs the development of enterprise-wide architecture and processes to embed the strategic application of change in the management of the organisation. 
Directs the creation and review of an enterprise capability strategy to support the strategic requirements of the business. Oversees the creation and implementation of roadmaps to guide long-term enterprise transformation and strategic alignment.
Identifies the business benefits of alternative strategies.
Ensures compliance between business strategies, enterprise transformation activities and technology directions, setting strategies, policies, standards and practices."""@en .

sfialevels:SUBF_4 a sfia:SkillLevel ;
    skos:notation "SUBF_4" ;
    sfia:level lor:4 ;
    sfia:skillLevelDescription "Contributes to curriculum development by selecting or specifying curriculum content or assessment approaches for one or more specialist areas."@en .

sfialevels:SUBF_5 a sfia:SkillLevel ;
    skos:notation "SUBF_5" ;
    sfia:level lor:5 ;
    sfia:skillLevelDescription "Contributes to the specification and development of curricula and assessment in an educational context or for an independent examination body."@en .

sfialevels:SUBF_6 a sfia:SkillLevel ;
    skos:notation "SUBF_6" ;
    sfia:level lor:6 ;
    sfia:skillLevelDescription """Leads the specification and development of curricula and assessment in an educational context or for an independent examination body. 
Contributes to the development of a strategy for curriculum evolution. 
Ensures relevant current domain research is represented in the curricula."""@en .

sfialevels:SUBF_7 a sfia:SkillLevel ;
    skos:notation "SUBF_7" ;
    sfia:level lor:7 ;
    sfia:skillLevelDescription """Authorises the curriculum and assessment strategies for a broad range of curricula or learning pathways.
Directs the definition, implementation and monitoring of curricula to satisfy relevant statutory and professional benchmarks and frameworks.
Develops strategies for the evolution of curricula over time. Incorporates emerging domain and pedagogical themes into plans for future curricula."""@en .

sfialevels:SUPP_2 a sfia:SkillLevel ;
    skos:notation "SUPP_2" ;
    sfia:level lor:2 ;
    sfia:skillLevelDescription """Assists in the collection and reporting of supplier performance data.
Assists with the routine day-to-day communication between the organisation and suppliers."""@en .

sfialevels:SUPP_3 a sfia:SkillLevel ;
    skos:notation "SUPP_3" ;
    sfia:level lor:3 ;
    sfia:skillLevelDescription """Acts as the routine contact point between the organisation and suppliers.
Supports resolution of supplier-related incidents, problems, or unsatisfactory performance.
Collects and reports on supplier performance data."""@en .

sfialevels:SUPP_4 a sfia:SkillLevel ;
    skos:notation "SUPP_4" ;
    sfia:level lor:4 ;
    sfia:skillLevelDescription """Collects supplier performance data and investigates problems. 
Monitors and reports on supplier performance, customer satisfaction, adherence to security requirements and market intelligence. Validates that suppliers' performance is in accordance with contract terms. 
Engages proactively and collaboratively with suppliers to resolve incidents, problems, or unsatisfactory performance. 
Implements supplier management-related service improvement initiatives and programmes."""@en .

sfialevels:SUPP_5 a sfia:SkillLevel ;
    skos:notation "SUPP_5" ;
    sfia:level lor:5 ;
    sfia:skillLevelDescription """Manages suppliers to meet key performance indicators and agreed targets. 
Manages the operational relationships between suppliers and ensures potential disputes or conflicts  are raised and resolved. 
Performs bench-marking and makes use of supplier performance data to ensure performance is adequately monitored and regularly reviewed. Use suppliers' expertise to support and inform development roadmaps.
Manages implementation of supplier service improvement actions. Identifies constraints and opportunities when negotiating or renegotiating contracts."""@en .

sfialevels:SUPP_6 a sfia:SkillLevel ;
    skos:notation "SUPP_6" ;
    sfia:level lor:6 ;
    sfia:skillLevelDescription """Develops organisational policies, standards and guidelines to ensure effective supplier management across the integrated supply chain. 
Defines the approach for commercial communications and the management of relationships with suppliers. Establishes a positive and effective working environment with suppliers for mutual benefit. 
Ensures resources and tools are in place to conduct bench-marking. Reviews supplier analysis and assesses effectiveness across the supply chain. 
Manages risks and assures the quality of the services delivered by suppliers."""@en .

sfialevels:SUPP_7 a sfia:SkillLevel ;
    skos:notation "SUPP_7" ;
    sfia:level lor:7 ;
    sfia:skillLevelDescription """Determines overall supplier management strategy, embracing effective management and operational relationships at all levels. 
Leads collaborative supplier partnerships. Aligns supplier performance and relationship management with business objectives and sourcing strategies.
Establishes frameworks for supplier governance and service monitoring.
Ensures commercial value from contracts and represents the organisation in significant supplier disputes."""@en .

sfialevels:SUST_4 a sfia:SkillLevel ;
    skos:notation "SUST_4" ;
    sfia:level lor:4 ;
    sfia:skillLevelDescription """Assesses and reports on how different tactical decisions affect sustainability. 
Evaluates factors and risks (political, legislative, technological, economic, social) that impact on operational processes and strategic direction.
Evaluates and reports on the implementation of sustainability measures in specific areas."""@en .

sfialevels:SUST_5 a sfia:SkillLevel ;
    skos:notation "SUST_5" ;
    sfia:level lor:5 ;
    sfia:skillLevelDescription """Provides expert advice and guidance on planning, designing and implementing sustainability solutions. 
Evaluates and selects sustainability methods, tools and practices to be used in line with agreed policies and standards. 
Identifies and recommends improvements to the organisation's approach to sustainability."""@en .

sfialevels:SUST_6 a sfia:SkillLevel ;
    skos:notation "SUST_6" ;
    sfia:level lor:6 ;
    sfia:skillLevelDescription """Develops and promotes organisational strategies, policies, standards and guidelines for sustainability. 
Leads the introduction and use of sustainability techniques, methodologies and tools."""@en .

sfialevels:SWDN_2 a sfia:SkillLevel ;
    skos:notation "SWDN_2" ;
    sfia:level lor:2 ;
    sfia:skillLevelDescription """Creates and documents detailed designs for simple software applications or components. 
Applies agreed modelling techniques, standards, patterns and tools. 
Contributes to the design of components of larger software systems, ensuring alignment with overall design requirements, including security.
Reviews own work."""@en .

sfialevels:SWDN_3 a sfia:SkillLevel ;
    skos:notation "SWDN_3" ;
    sfia:level lor:3 ;
    sfia:skillLevelDescription """Undertakes complete design of moderately complex software applications or components.
Applies agreed standards, guidelines, patterns and tools. Assists as part of a team in the design of components of larger software systems. Specifies user and/or system interfaces. 
Creates multiple design views to address the different stakeholders' concerns and to handle functional and non-functional requirements, considering all relevant factors, including security. Assists in the evaluation of options and trade-offs. 
Collaborates in reviews of work with others as appropriate."""@en .

sfialevels:SWDN_4 a sfia:SkillLevel ;
    skos:notation "SWDN_4" ;
    sfia:level lor:4 ;
    sfia:skillLevelDescription """Designs and architects complex software applications, components and modules.
Uses appropriate modelling techniques in line with agreed software design standards, guidelines, patterns and methodologies. Produces and communicates multiple design views to address stakeholder concerns and meet both functional and non-functional requirements including security.
Identifies, evaluates and recommends design alternatives and trade-offs. Models, simulates or prototypes proposed software behaviours to secure stakeholder approval and facilitate effective software construction.  
Reviews, verifies and enhances own designs against specifications and leads reviews of others' designs."""@en .

sfialevels:SWDN_5 a sfia:SkillLevel ;
    skos:notation "SWDN_5" ;
    sfia:level lor:5 ;
    sfia:skillLevelDescription """Specifies, designs and architects large or complex software applications, components and modules. 
Adopts and adapts software design methods, tools and techniques. Undertakes impact analysis on major design options, makes recommendations and assesses and manages associated risks. Specifies prototypes/simulations to enable informed decision-making. 
Evaluates software designs to ensure adherence to standards and identifies corrective action. Ensures the software design balances functional, quality, security and systems management requirements. 
Contributes to the development of organisational software design and architecture policies and standards."""@en .

sfialevels:SWDN_6 a sfia:SkillLevel ;
    skos:notation "SWDN_6" ;
    sfia:level lor:6 ;
    sfia:skillLevelDescription """Leads the selection and development of software design and architectural methods, tools and techniques. 
Defines and maintains architectural principles, patterns and frameworks to guide software design and development across the organisation.
Ensures adherence to technical strategies and systems architectures (including security)."""@en .

sfialevels:SYSP_2 a sfia:SkillLevel ;
    skos:notation "SYSP_2" ;
    sfia:level lor:2 ;
    sfia:skillLevelDescription """Assists with system software administration tasks under routine supervision.
Supports the installation and configuration of system software.
Helps monitor system performance and resource usage.
Assists in documenting system software settings and updates."""@en .

sfialevels:SYSP_3 a sfia:SkillLevel ;
    skos:notation "SYSP_3" ;
    sfia:level lor:3 ;
    sfia:skillLevelDescription """Monitors operational systems for resource usage and failure rates, to inform and facilitate system software tuning.
Applies system software settings to optimise performance, enabling maximum throughput and efficient resource utilisation.
Installs and tests new versions of system software. 
Assists in creating software implementation procedures, including  fallback contingency plans."""@en .

sfialevels:SYSP_4 a sfia:SkillLevel ;
    skos:notation "SYSP_4" ;
    sfia:level lor:4 ;
    sfia:skillLevelDescription """Monitors system software metrics and adjusts configurations for optimum availability and performance.
Applies technical expertise to investigates and resolve complex system software issues, requesting action from supplier if required. 
Analyses system software updates and determines which ones require actions. 
Develops comprehensive software implementation procedures with robust contingency plans."""@en .

sfialevels:SYSP_5 a sfia:SkillLevel ;
    skos:notation "SYSP_5" ;
    sfia:level lor:5 ;
    sfia:skillLevelDescription """Ensures system software is provisioned and configured to support the achievement of service objectives. 
Develops and maintains diagnostic tools and processes for troubleshooting and performance analysis. 
Evaluates new system software and recommends adoption if appropriate. Plans the provisioning and testing of new versions of system software. 
Ensures operational procedures and diagnostics for system software are current, accessible and well understood. Investigates and coordinates the resolution of potential and actual service problems."""@en .

sfialevels:TEAC_2 a sfia:SkillLevel ;
    skos:notation "TEAC_2" ;
    sfia:level lor:2 ;
    sfia:skillLevelDescription """Contributes to the delivery of aspects of computing and IT curricula in a formal educational context. 
Applies good practice in learning content design, development and delivery.
Assesses student performance in aspects of a curriculum area, providing support to enhance student understanding as needed."""@en .

sfialevels:TEAC_3 a sfia:SkillLevel ;
    skos:notation "TEAC_3" ;
    sfia:level lor:3 ;
    sfia:skillLevelDescription """Delivers the majority of a curriculum. 
Applies good practice in learning content design, development and delivery. Maintains awareness of relevant pedagogical and domain research.
Assesses student performance across a curriculum. Provides feedback and support to help students improve their understanding."""@en .

sfialevels:TEAC_4 a sfia:SkillLevel ;
    skos:notation "TEAC_4" ;
    sfia:level lor:4 ;
    sfia:skillLevelDescription """Delivers a curriculum. 
Applies good practice supported by pedagogical research to learning content design, development and delivery. 
Assesses student performance and reviews cohort performance. Advises and assists students to enable the achievement of learning objectives."""@en .

sfialevels:TEAC_5 a sfia:SkillLevel ;
    skos:notation "TEAC_5" ;
    sfia:level lor:5 ;
    sfia:skillLevelDescription """Leads the teaching and assessment of a curriculum or learning pathway.  
Implements enhancement strategies for teaching and assessment. Reviews pedagogical research and practices relevant to topics in the curricula. Applies good teaching practices in learning content design, development and delivery.
Contributes to the development and implementation of specialist teaching practices needed by the curriculum.  
Evaluates and monitors student achievements and the effectiveness of teaching activities across the curriculum.  Advises on the use of appropriate pedagogies and assessment approaches."""@en .

sfialevels:TEAC_6 a sfia:SkillLevel ;
    skos:notation "TEAC_6" ;
    sfia:level lor:6 ;
    sfia:skillLevelDescription """Leads the teaching, assessment and enhancement of a range of curricula or learning pathways.
Reviews and critically evaluates pedagogical research and practices relevant to the curricula. Develops and leads the introduction of advanced or specialist teaching practices. 
Leads and supports others in the development of good practice in learning content design, development and delivery. 
Monitors, evaluates and reports the performance of teaching and assessment activities within their areas of responsibility."""@en .

sfialevels:TEAC_7 a sfia:SkillLevel ;
    skos:notation "TEAC_7" ;
    sfia:level lor:7 ;
    sfia:skillLevelDescription """Authorises teaching, assessment and enhancement strategies for a broad range of curricula or learning pathways.
Directs the definition, implementation and monitoring of teaching to satisfy relevant statutory and professional benchmarks and frameworks.
Secures resources to deliver the organisation's teaching commitments.
Monitors and evaluates relevant domain and pedagogical research to identify and implement improvements to the delivery of the curricula."""@en .

sfialevels:TECH_4 a sfia:SkillLevel ;
    skos:notation "TECH_4" ;
    sfia:level lor:4 ;
    sfia:skillLevelDescription """Provides detailed and specific advice to support the organisation's planning and operations, typically related to the immediate area of responsibility.
Actively maintains recognised expert level knowledge in one or more identifiable specialisms. 
Recognises and identifies the boundaries of their own specialist knowledge. 
Where appropriate, collaborates with other specialists to ensure advice given is professionally sound and appropriate to the organisation's needs."""@en .

sfialevels:TECH_5 a sfia:SkillLevel ;
    skos:notation "TECH_5" ;
    sfia:level lor:5 ;
    sfia:skillLevelDescription """Provides professional advice that informs operational leadership and influences the translation of strategy into operations in their specialist area.
Oversees the provision of specialist advice by others. Consolidates expertise from multiple sources, including third-party experts, to provide coherent and professionally sound advice to further organisational objectives.
Supports and promotes the development and sharing of specialist knowledge within the organisation."""@en .

sfialevels:TECH_6 a sfia:SkillLevel ;
    skos:notation "TECH_6" ;
    sfia:level lor:6 ;
    sfia:skillLevelDescription """Leads and promotes the development and application of specialist knowledge across the organisation, delivering professional advice that shapes direction and high-level decisions.
Maintains a network of recognised experts (inside and/or outside the organisation) who can deliver expert advice in relevant areas. 
Actively influences professional development planning across a significant part of the organisation to further the development of appropriate expertise and provision of high-quality professional advice."""@en .

sfialevels:TEST_1 a sfia:SkillLevel ;
    skos:notation "TEST_1" ;
    sfia:level lor:1 ;
    sfia:skillLevelDescription """Executes given manual functional test scripts under supervision to verify basic software capabilities.
Configures test environments, uses basic automated tools for functionality verification, records results and reports issues."""@en .

sfialevels:TEST_2 a sfia:SkillLevel ;
    skos:notation "TEST_2" ;
    sfia:level lor:2 ;
    sfia:skillLevelDescription """Assists in designing functional test cases and creating test scripts. 
Supports the preparation of test data for functional testing under supervision.
Configures test environments to reflect realistic use cases.
Executes and records manual and automated functional tests, analysing results and reporting on findings, issues and risks."""@en .

sfialevels:TEST_3 a sfia:SkillLevel ;
    skos:notation "TEST_3" ;
    sfia:level lor:3 ;
    sfia:skillLevelDescription """Designs detailed functional test cases and scripts, covering various scenarios and boundary values.
Actively participates in requirement and design reviews, refining test plans based on insights gained. 
Undertakes structured exploratory testing to investigate and verify functionality. 
Prepares test data, configures environments and automates repeatable tests. Executes tests, logs defects with detailed information and analyses results to assess system functionality."""@en .

sfialevels:TEST_4 a sfia:SkillLevel ;
    skos:notation "TEST_4" ;
    sfia:level lor:4 ;
    sfia:skillLevelDescription """Selects appropriate functional testing approaches, considering risk, criticality and complexity. 
Develops, automates and executes comprehensive test plans and cases. 
Configures environments to mirror real-world usage, collaborates with stakeholders to refine requirements and manages scalable automated testing frameworks. 
Identifies and mitigates risks during testing, provides detailed analysis and reports on functional test activities and results, including work done by others."""@en .

sfialevels:TEST_5 a sfia:SkillLevel ;
    skos:notation "TEST_5" ;
    sfia:level lor:5 ;
    sfia:skillLevelDescription """Leads functional testing efforts across all development stages, ensuring alignment with functional requirements and focusing on risk-based prioritisation.
Provides authoritative advice on testing methods, tools and frameworks.
Monitors and improves test coverage, collaborates with teams to address challenges and ensures compliance with standards.
Leads efforts to improve the efficiency and reliability of functional testing. Identifies improvements and contributes to organisational policies, standards and guidelines for functional testing."""@en .

sfialevels:TEST_6 a sfia:SkillLevel ;
    skos:notation "TEST_6" ;
    sfia:level lor:6 ;
    sfia:skillLevelDescription """Develops organisational policies, standards and guidelines for functional testing, ensuring they align with business strategy and incorporate a risk-based approach.
Plans and leads complex testing initiatives, ensuring alignment with strategic objectives and incorporating a risk-based approach.
Manages risks and opportunities, coordinates with other testing activities and drives improvements in functional testing capabilities.
Promotes a culture of quality in functional testing, driving adherence to organisational standards and proactive risk mitigation."""@en .

sfialevels:THIN_2 a sfia:SkillLevel ;
    skos:notation "THIN_2" ;
    sfia:level lor:2 ;
    sfia:skillLevelDescription """Contributes to routine threat intelligence gathering tasks. 
Monitors and detects potential security threats and escalates in accordance with relevant procedures and standards."""@en .

sfialevels:THIN_3 a sfia:SkillLevel ;
    skos:notation "THIN_3" ;
    sfia:level lor:3 ;
    sfia:skillLevelDescription """Performs routine threat intelligence gathering tasks. 
Transforms collected information into a data format that can be used for operational security activities.
Cleans and converts quantitative information into consistent formats."""@en .

sfialevels:THIN_4 a sfia:SkillLevel ;
    skos:notation "THIN_4" ;
    sfia:level lor:4 ;
    sfia:skillLevelDescription """Collates and analyses information for threat intelligence requirements from a variety of sources.
Contributes to reviewing, ranking and categorising qualitative threat intelligence information. 
Creates threat intelligence reports. 
Evaluates the value, usefulness and impact of threat intelligence sources."""@en .

sfialevels:THIN_5 a sfia:SkillLevel ;
    skos:notation "THIN_5" ;
    sfia:level lor:5 ;
    sfia:skillLevelDescription """Plans and manages threat intelligence activities. 
Identifies the most impactful threat categories and types of information that can help defend against them. Reviews, ranks and categorises qualitative threat intelligence information.
Provides expert advice on threat intelligence activities. 
Leads the production and editing of threat intelligence reports that enhance the intelligence production workflow. Distributes information and obtains feedback about the value, usefulness and impact of the data."""@en .

sfialevels:THIN_6 a sfia:SkillLevel ;
    skos:notation "THIN_6" ;
    sfia:level lor:6 ;
    sfia:skillLevelDescription """Sets direction, plans and leads the organisation's approach to threat intelligence, including the use of suppliers.
Identifies requirements for threat intelligence based on the assets to be protected and the types of intelligence that can help protect those assets. 
Engages with and influences relevant stakeholders to communicate results of research and the required response. 
Ensures quality and accuracy of threat intelligence information. Reviews threat intelligence capabilities."""@en .

sfialevels:TMCR_2 a sfia:SkillLevel ;
    skos:notation "TMCR_2" ;
    sfia:level lor:2 ;
    sfia:skillLevelDescription """Assists with learning design and development tasks under routine supervision.
Supports the creation and maintenance of learning materials and resources.
Helps document and organise learning content and environments."""@en .

sfialevels:TMCR_3 a sfia:SkillLevel ;
    skos:notation "TMCR_3" ;
    sfia:level lor:3 ;
    sfia:skillLevelDescription """Designs, creates, customises and maintains learning materials and resources to deliver agreed outcomes, and meet accreditation requirements when appropriate. 
Contributes to the design, configuration and testing of learning environments."""@en .

sfialevels:TMCR_4 a sfia:SkillLevel ;
    skos:notation "TMCR_4" ;
    sfia:level lor:4 ;
    sfia:skillLevelDescription """Specifies the content and structure of learning and development materials. 
Takes responsibility for design, creation, packaging and maintenance. Manages development to deliver agreed outcomes. 
Where required, designs, configures and tests learning environments. 
Secures external accreditations as appropriate."""@en .

sfialevels:TMCR_5 a sfia:SkillLevel ;
    skos:notation "TMCR_5" ;
    sfia:level lor:5 ;
    sfia:skillLevelDescription """Specifies solutions for use in learning and development programmes in the workplace or in compulsory, further or higher education.
Commissions the development of learning materials, allocates resources to learning teams and defines learning outcomes. 
Leads learning programmes, recommends and specifies learning interventions for design, development and deployment according to agreed learning outcomes."""@en .

sfialevels:UNAN_2 a sfia:SkillLevel ;
    skos:notation "UNAN_2" ;
    sfia:level lor:2 ;
    sfia:skillLevelDescription """Assists with user experience analysis tasks under routine supervision.
Supports the collection and documentation of user requirements.
Helps organise and structure user experience data for analysis."""@en .

sfialevels:UNAN_3 a sfia:SkillLevel ;
    skos:notation "UNAN_3" ;
    sfia:level lor:3 ;
    sfia:skillLevelDescription """Applies standard techniques and tools for developing user stories and eliciting user experience requirements. 
Organises and structures user experience analysis. 
Works with stakeholders to prioritise requirements and resolve conflicts."""@en .

sfialevels:UNAN_4 a sfia:SkillLevel ;
    skos:notation "UNAN_4" ;
    sfia:level lor:4 ;
    sfia:skillLevelDescription """Selects appropriate techniques and tools to develop user stories and elicit user experience requirements in complex situations. 
Identifies and describes the design goals for systems, products, services and devices. 
Identifies the roles of affected stakeholder groups. Resolves potential conflicts between differing user requirements. 
Specifies measurable criteria for the required usability and accessibility of systems, products, services and devices."""@en .

sfialevels:UNAN_5 a sfia:SkillLevel ;
    skos:notation "UNAN_5" ;
    sfia:level lor:5 ;
    sfia:skillLevelDescription """Determines the approaches to be used for user experience analysis. 
Plans and manages user experience and accessibility analysis activities. 
Provides expert advice and guidance to support the adoption and adaptation of agreed approaches.  
Develops user experience tools, techniques and standards as part of the organisation's framework for user-centred design"""@en .

sfialevels:URCH_2 a sfia:SkillLevel ;
    skos:notation "URCH_2" ;
    sfia:level lor:2 ;
    sfia:skillLevelDescription """Assists with user research tasks under routine supervision.
Supports the collection and documentation of user research.
Helps organise and share the outcomes of user research activities.
Participates in basic user-centred design activities as directed."""@en .

sfialevels:URCH_3 a sfia:SkillLevel ;
    skos:notation "URCH_3" ;
    sfia:level lor:3 ;
    sfia:skillLevelDescription """Applies standard methods to support user research initiatives.
Engages effectively with users and customer representatives to generate high-quality research. 
Documents and shares the outcomes of user research.
Contributes to research design and analysis tasks under guidance."""@en .

sfialevels:URCH_4 a sfia:SkillLevel ;
    skos:notation "URCH_4" ;
    sfia:level lor:4 ;
    sfia:skillLevelDescription """Conducts generative research for the development of systems, products, services or devices. 
Plans own user research activities. Facilitates input from users and stakeholders. 
Identifies appropriate user research methods for specific questions and contexts. 
Collects and analyses user research data. Supports synthesis of research and the creation of insights, reports and presentations."""@en .

sfialevels:URCH_5 a sfia:SkillLevel ;
    skos:notation "URCH_5" ;
    sfia:level lor:5 ;
    sfia:skillLevelDescription """Plans and drives user research activities providing expert advice and guidance to support the adoption of agreed approaches. 
Selects and implements appropriate methods for engaging users in generative research activities.
Leads the collection and analysis of user research data. Synthesises research, develops insights and presents conclusions to inform decision-making and drive actions. 
Leads complex user research initiatives and identifies emerging user needs and trends. Contributes to the development of organisational methods and standards for user research."""@en .

sfialevels:URCH_6 a sfia:SkillLevel ;
    skos:notation "URCH_6" ;
    sfia:level lor:6 ;
    sfia:skillLevelDescription """Sets the overall vision and direction for user research activities.
Champions user-centred design and secures organisational commitment to the significant involvement of users in research. 
Develops organisational policies, standards and guidelines for user research. 
Develops or sources organisational resources and capabilities to facilitate the adoption and exploitation of user research. Collaborates with internal and external partners to facilitate effective user research."""@en .

sfialevels:USEV_2 a sfia:SkillLevel ;
    skos:notation "USEV_2" ;
    sfia:level lor:2 ;
    sfia:skillLevelDescription """Assists in preparing and operating the environment, facilities and tools needed to evaluate systems, products, services or devices. 
Assists in the collection of feedback on prototypes and designs from users and others."""@en .

sfialevels:USEV_3 a sfia:SkillLevel ;
    skos:notation "USEV_3" ;
    sfia:level lor:3 ;
    sfia:skillLevelDescription """Evaluates design options and prototypes to obtain user feedback on requirements of developing systems, products, services or devices.
Tests the usability and accessibility of components and alternative designs. Administers a range of evaluations, recording data and feedback. Analyses evaluation data and recommends actions. Identifies areas for future user research.
Checks systems, products, services or devices for adherence to applicable standards, guidelines, style guides and legislation. 
Evaluates the usability of existing or competitor systems to provide benchmark values and as input to design."""@en .

sfialevels:USEV_4 a sfia:SkillLevel ;
    skos:notation "USEV_4" ;
    sfia:level lor:4 ;
    sfia:skillLevelDescription """Selects appropriate tools and techniques to evaluate user experiences of systems, products,  services or devices.
Validates that security, usability and accessibility requirements have been met. 
Checks operational systems, products, services or devices for changes in usability and accessibility needs. 
Interprets and presents results of evaluations, prioritises issues and reports on remedial actions. Collates input for future user research."""@en .

sfialevels:USEV_5 a sfia:SkillLevel ;
    skos:notation "USEV_5" ;
    sfia:level lor:5 ;
    sfia:skillLevelDescription """Manages user experience evaluation of systems, products, services or devices.
Assures that the security, usability and accessibility requirements are met and required practices have been followed.
Advises on what to evaluate, type of evaluation to use and the extent of user involvement required. Works iteratively with design teams to ensure feedback from the evaluation is understood and acted upon. 
Advises on the achievement of required usability and accessibility levels of specific designs or prototypes. Prioritises input for future user research."""@en .

sfialevels:USEV_6 a sfia:SkillLevel ;
    skos:notation "USEV_6" ;
    sfia:level lor:6 ;
    sfia:skillLevelDescription """Champions high standards in user interaction with the organisation's systems, products and services including involvement of users in evaluation activities. 
Specifies standards and methods for security, usability and accessibility and ensure this is addressed in future designs. 
Develops or sources resources and capabilities to conduct effective user experience evaluation, including specialist user-centred facilities and communities of users. Leads the provision of input and resources for future user research.
Collaborates with internal and external partners to facilitate an effective evaluation of systems, products and services."""@en .

sfialevels:USUP_1 a sfia:SkillLevel ;
    skos:notation "USUP_1" ;
    sfia:level lor:1 ;
    sfia:skillLevelDescription """Follows agreed procedures to identify, register and categorise incidents.
Uses provided tools and technologies to support the incident management process.
Collects information as instructed to assist in incident resolution and allocates incidents as directed.
Assists in monitoring incident queues and escalates issues according to procedures."""@en .

sfialevels:USUP_2 a sfia:SkillLevel ;
    skos:notation "USUP_2" ;
    sfia:level lor:2 ;
    sfia:skillLevelDescription """Provides first line investigation and gathers information to enable incident resolution and allocate incidents. 
Gathers information to enable incident resolution and allocates incidents according to established procedures. Escalates incidents as necessary. 
Advises relevant people of actions taken. Communicates with users and stakeholders to provide updates on incident status. 
Assists in maintaining records and documentation related to incidents."""@en .

sfialevels:USUP_3 a sfia:SkillLevel ;
    skos:notation "USUP_3" ;
    sfia:level lor:3 ;
    sfia:skillLevelDescription """Prioritises and diagnoses incidents applying agreed procedures and tools.
Investigates causes of incidents and seeks resolution. 
Escalates unresolved incidents to higher levels or specialist teams. Coordinates with stakeholders to ensure timely resolution.
Facilitates recovery, following resolution of incidents. Documents, communicates outcomes and closes resolved incidents."""@en .

sfialevels:USUP_4 a sfia:SkillLevel ;
    skos:notation "USUP_4" ;
    sfia:level lor:4 ;
    sfia:skillLevelDescription """Monitors and manages incident queues to ensure incidents are handled according to procedures and service levels. 
Contributes to developing, testing and improving incident management procedures. Uses analytics tools to track trends.
Ensures resolved incidents are properly documented and closed. 
Supports team members in the correct use of the incident process."""@en .

sfialevels:USUP_5 a sfia:SkillLevel ;
    skos:notation "USUP_5" ;
    sfia:level lor:5 ;
    sfia:skillLevelDescription """Responsible for the operation of the incident management process. 
Manages incident communications, ensuring al parties are aware of incidents and their role in the process. 
Leads the review of major incidents and informs service owners of outcomes. Ensures incident resolution within service targets. Analyses metrics and reports on the performance of the incident management process. 
Develops, maintains and tests incident management policy and procedures. Ensures compliance with regulatory requirements."""@en .

sfialevels:USUP_6 a sfia:SkillLevel ;
    skos:notation "USUP_6" ;
    sfia:level lor:6 ;
    sfia:skillLevelDescription """Shapes and directs the organisation's incident management strategy. Establishes policies and standards for incident management aligned with organisational goals.
Provides leadership during major incidents, coordinating cross-functional teams and external partners. Makes high-level decisions to minimise impact and ensure swift recovery.
Leads the development of organisational capabilities for incident management.
Promotes organisational collaboration and ensures that incident management processes are understood and adopted across the organisation."""@en .

sfialevels:VISL_2 a sfia:SkillLevel ;
    skos:notation "VISL_2" ;
    sfia:level lor:2 ;
    sfia:skillLevelDescription """Creates standard data visuals using established products, tools and techniques, under routine supervision.
Assists in updating and refining existing data visualisations to maintain effective representation of concepts, ideas and facts."""@en .

sfialevels:VISL_3 a sfia:SkillLevel ;
    skos:notation "VISL_3" ;
    sfia:level lor:3 ;
    sfia:skillLevelDescription """Uses visualisation products, as guided, to design and create data visuals. 
Selects appropriate visualisation techniques from the options available. 
Engages with the target user to prototype and refine specified visualisations.
Assists in developing narratives around data sets to support understanding and decision-making."""@en .

sfialevels:VISL_4 a sfia:SkillLevel ;
    skos:notation "VISL_4" ;
    sfia:level lor:4 ;
    sfia:skillLevelDescription """Applies a variety of visualisation techniques and designs the content and appearance of data visuals. 
Operationalises and automates activities for efficient and timely production of data visuals. 
Selects appropriate visualisation approaches from a range of applicable options. Develops narratives around data sets to guide decision-making processes and enhance understanding of key insights.
Contributes to exploration and experimentation in data visualisation."""@en .

sfialevels:VISL_5 a sfia:SkillLevel ;
    skos:notation "VISL_5" ;
    sfia:level lor:5 ;
    sfia:skillLevelDescription """Leads exploration of new approaches for data visualisation. Establishes the purpose and parameters of the data visualisation. 
Oversees the use of data visualisation tools and techniques. Communicates results using appropriate methods for the target audience.
Advises on the use of data visualisation approaches for different purposes and contexts to satisfy requirements.  Develops plans to meet user needs.
Collaborates with stakeholders to identify key insights and create compelling narratives that effectively communicate the story behind the data to drive decision-making processes."""@en .

sfialevels:VUAS_2 a sfia:SkillLevel ;
    skos:notation "VUAS_2" ;
    sfia:level lor:2 ;
    sfia:skillLevelDescription """Undertakes low-complexity routine vulnerability assessments using automated and semi-automated tools. 
Escalates issues where appropriate.
Contributes to documenting the scope and evaluating the results of vulnerability assessments."""@en .

sfialevels:VUAS_3 a sfia:SkillLevel ;
    skos:notation "VUAS_3" ;
    sfia:level lor:3 ;
    sfia:skillLevelDescription """Follows standard approaches to perform basic vulnerability assessments for small information systems. 
Supports creation of  catalogues of information and technology assets for vulnerability assessment."""@en .

sfialevels:VUAS_4 a sfia:SkillLevel ;
    skos:notation "VUAS_4" ;
    sfia:level lor:4 ;
    sfia:skillLevelDescription """Collates and analyses catalogues of information and technology assets for vulnerability assessment. 
Performs vulnerability assessments and business impact analysis for medium complexity information systems. 
Contributes to selection and deployment of vulnerability assessment tools and techniques."""@en .

sfialevels:VUAS_5 a sfia:SkillLevel ;
    skos:notation "VUAS_5" ;
    sfia:level lor:5 ;
    sfia:skillLevelDescription """Plans and manages vulnerability assessment activities within the organisation.
Evaluates, selects and reviews vulnerability assessment tools and techniques.
Provides expert advice and guidance to support the adoption of agreed approaches.
Obtains and acts on vulnerability information and conducts security risk assessments, business impact analysis and accreditation on complex information systems."""@en .

sfialevels:VURE_2 a sfia:SkillLevel ;
    skos:notation "VURE_2" ;
    sfia:level lor:2 ;
    sfia:skillLevelDescription """Assists with vulnerability research tasks under routine supervision.
Helps document and report findings from vulnerability research activities."""@en .

sfialevels:VURE_3 a sfia:SkillLevel ;
    skos:notation "VURE_3" ;
    sfia:level lor:3 ;
    sfia:skillLevelDescription """Applies standard techniques and tools for vulnerability research. 
Uses available resources to update knowledge of relevant specialism. 
Participates in research communities. 
Analyses and reports on activities and results."""@en .

sfialevels:VURE_4 a sfia:SkillLevel ;
    skos:notation "VURE_4" ;
    sfia:level lor:4 ;
    sfia:skillLevelDescription """Designs and executes complex vulnerability research activities. 
Specifies requirements for environment, data, resources and tools to perform assessments. 
Reviews test results and modifies tests if necessary. Creates reports to communicate methodology, findings and conclusions. Advises on deception methods by exploiting identified patterns. 
Makes an active contribution to research communities."""@en .

sfialevels:VURE_5 a sfia:SkillLevel ;
    skos:notation "VURE_5" ;
    sfia:level lor:5 ;
    sfia:skillLevelDescription """Plans and manages vulnerability research activities. 
Maintains a strong external network for vulnerability research. Gathers information on new and emerging threats and vulnerabilities. 
Assesses and documents the impacts and threats to the organisation. Creates reports and shares knowledge and insights with stakeholders. 
Provides expert advice and guidance to support the adoption of tools and techniques for vulnerability research. Contributes to the development of organisational policies, standards and guidelines for vulnerability research and assessment."""@en .

sfialevels:VURE_6 a sfia:SkillLevel ;
    skos:notation "VURE_6" ;
    sfia:level lor:6 ;
    sfia:skillLevelDescription """Plans and leads the organisation's approach to vulnerability research.
Identifies new and emerging threats and vulnerabilities. Maintains a strong external network. Takes a leading part in external-facing professional activities to facilitate information gathering and set the scope of research work. 
Engages with and influences relevant stakeholders to communicate results of research and the required response. 
Develops organisational policies and guidelines for monitoring emerging threats and vulnerabilities."""@en .

sfialevels:WFPL_4 a sfia:SkillLevel ;
    skos:notation "WFPL_4" ;
    sfia:level lor:4 ;
    sfia:skillLevelDescription """Gathers, maintains and analyses organisation-wide workforce capability data.
Performs gap analysis to identify workforce strengths and shortfalls with reference to business strategy and specific future needs. 
Contributes to the development of organisation-wide workforce plans to meet current and future demand. 
Coordinates and schedules ongoing workforce planning activities. Assists in maintaining a skills and capability inventory."""@en .

sfialevels:WFPL_5 a sfia:SkillLevel ;
    skos:notation "WFPL_5" ;
    sfia:level lor:5 ;
    sfia:skillLevelDescription """Leads the development of workforce plans to ensure the availability of appropriately skilled resources to meet organisational objectives and commitments.
Contributes to the development of the strategic workforce planning approach. Oversees and reviews the implementation of workforce plans. 
Develops current-state assessment of workforce skills, capabilities and potential. Forecasts future workforce demand for skills based on broad organisation-wide plans and external factors. 
Maintains a skills and capability inventory and identifies options for closing gaps."""@en .

sfialevels:WFPL_6 a sfia:SkillLevel ;
    skos:notation "WFPL_6" ;
    sfia:level lor:6 ;
    sfia:skillLevelDescription """Defines an integrated strategic workforce planning approach connecting organisational business goals to future skill needs.
Communicates the workforce planning approach and obtains organisational commitment. Selects frameworks to be used for the organisation's skills and capability inventory. 
Interprets business strategy to direct workforce demand forecasting (skills and numbers) for the organisation. Monitors the external environment in relation to supply and emerging trends. 
Influences people management policies and practices to align with workforce plans. Integrates with resourcing strategies and plans. Monitors execution of workforce plans."""@en .

categories:advice_and_guidance a sfia:Category ;
    skos:broader categories:strategy_and_architecture ;
    skos:inScheme sfia:CategoryScheme ;
    skos:prefLabel "Advice and guidance"@en .

categories:computational_science a sfia:Category ;
    skos:broader categories:development_and_implementation ;
    skos:inScheme sfia:CategoryScheme ;
    skos:prefLabel "Computational science"@en .

categories:data_and_records_operations a sfia:Category ;
    skos:broader categories:delivery_and_operation ;
    skos:inScheme sfia:CategoryScheme ;
    skos:prefLabel "Data and records operations"@en .

categories:people_and_skills a sfia:Category ;
    skos:inScheme sfia:CategoryScheme ;
    skos:prefLabel "People and skills"@en .

categories:sales_and_bid_management a sfia:Category ;
    skos:broader categories:relationships_and_engagement ;
    skos:inScheme sfia:CategoryScheme ;
    skos:prefLabel "Sales and bid management"@en .

categories:change_and_transformation a sfia:Category ;
    skos:inScheme sfia:CategoryScheme ;
    skos:prefLabel "Change and transformation"@en .

categories:content_management a sfia:Category ;
    skos:broader categories:development_and_implementation ;
    skos:inScheme sfia:CategoryScheme ;
    skos:prefLabel "Content management"@en .

categories:relationships_and_engagement a sfia:Category ;
    skos:inScheme sfia:CategoryScheme ;
    skos:prefLabel "Relationships and engagement"@en .

categories:change_analysis a sfia:Category ;
    skos:broader categories:change_and_transformation ;
    skos:inScheme sfia:CategoryScheme ;
    skos:prefLabel "Change analysis"@en .

categories:change_implementation a sfia:Category ;
    skos:broader categories:change_and_transformation ;
    skos:inScheme sfia:CategoryScheme ;
    skos:prefLabel "Change implementation"@en .

categories:delivery_and_operation a sfia:Category ;
    skos:inScheme sfia:CategoryScheme ;
    skos:prefLabel "Delivery and operation"@en .

categories:security_and_privacy a sfia:Category ;
    skos:broader categories:strategy_and_architecture ;
    skos:inScheme sfia:CategoryScheme ;
    skos:prefLabel "Security and privacy"@en .

categories:change_planning a sfia:Category ;
    skos:broader categories:change_and_transformation ;
    skos:inScheme sfia:CategoryScheme ;
    skos:prefLabel "Change planning"@en .

categories:development_and_implementation a sfia:Category ;
    skos:inScheme sfia:CategoryScheme ;
    skos:prefLabel "Development and implementation"@en .

categories:governance__risk_and_compliance a sfia:Category ;
    skos:broader categories:strategy_and_architecture ;
    skos:inScheme sfia:CategoryScheme ;
    skos:prefLabel "Governance, risk and compliance"@en .

categories:marketing a sfia:Category ;
    skos:broader categories:relationships_and_engagement ;
    skos:inScheme sfia:CategoryScheme ;
    skos:prefLabel "Marketing"@en .

categories:people_management a sfia:Category ;
    skos:broader categories:people_and_skills ;
    skos:inScheme sfia:CategoryScheme ;
    skos:prefLabel "People management"@en .

categories:stakeholder_management a sfia:Category ;
    skos:broader categories:relationships_and_engagement ;
    skos:inScheme sfia:CategoryScheme ;
    skos:prefLabel "Stakeholder management"@en .

categories:strategy_and_architecture a sfia:Category ;
    skos:inScheme sfia:CategoryScheme ;
    skos:prefLabel "Strategy and architecture"@en .

categories:user_centred_design a sfia:Category ;
    skos:broader categories:development_and_implementation ;
    skos:inScheme sfia:CategoryScheme ;
    skos:prefLabel "User centred design"@en .

categories:security_services a sfia:Category ;
    skos:broader categories:delivery_and_operation ;
    skos:inScheme sfia:CategoryScheme ;
    skos:prefLabel "Security services"@en .

categories:skills_management a sfia:Category ;
    skos:broader categories:people_and_skills ;
    skos:inScheme sfia:CategoryScheme ;
    skos:prefLabel "Skills management"@en .

categories:financial_and_value_management a sfia:Category ;
    skos:broader categories:strategy_and_architecture ;
    skos:inScheme sfia:CategoryScheme ;
    skos:prefLabel "Financial and value management"@en .

categories:data_and_analytics a sfia:Category ;
    skos:broader categories:development_and_implementation ;
    skos:inScheme sfia:CategoryScheme ;
    skos:prefLabel "Data and analytics"@en .

categories:strategy_and_planning a sfia:Category ;
    skos:broader categories:strategy_and_architecture ;
    skos:inScheme sfia:CategoryScheme ;
    skos:prefLabel "Strategy and planning"@en .

categories:service_management a sfia:Category ;
    skos:broader categories:delivery_and_operation ;
    skos:inScheme sfia:CategoryScheme ;
    skos:prefLabel "Service management"@en .

categories:technology_management a sfia:Category ;
    skos:broader categories:delivery_and_operation ;
    skos:inScheme sfia:CategoryScheme ;
    skos:prefLabel "Technology management"@en .

categories:systems_development a sfia:Category ;
    skos:broader categories:development_and_implementation ;
    skos:inScheme sfia:CategoryScheme ;
    skos:prefLabel "Systems development"@en .

sfia:CategoryScheme a skos:ConceptScheme ;
    dcterms:creator sfiaorg: ;
    dcterms:publisher jsa: ;
    skos:prefLabel "Scheme for the Skills' Categories"@en ;
    skos:definition "Scheme for the Skills' Categories"@en ;
    rdfs:label "Scheme for the Skills' Categories"@en ;
    skos:hasTopConcept categories:change_and_transformation,
        categories:delivery_and_operation,
        categories:development_and_implementation,
        categories:people_and_skills,
        categories:relationships_and_engagement,
        categories:strategy_and_architecture
.


lorcs: a skos:ConceptScheme ;
    skos:prefLabel "Scheme for the Levels of Responsibility"@en ;
    skos:definition "SFIA's seven levels of responsibility not only support career progression but also provide a foundation for mapping other frameworks and organisational structures to the SFIA framework. The generic attributes make these levels suitable as the basis for core competencies, mapping structures, and career development stages."@en ;
    schema:citation "https://sfia-online.org/en/sfia-9/responsibilities"^^xsd:anyURI ;
    dcterms:creator sfiaorg: ;
    dcterms:publisher jsa: ;
    skos:hasTopConcept 
        lor:1 , lor:2 , lor:3 , lor:4 , lor:5 , lor:6 , lor:7 
.

# lor

lor:1 a sfia:Level , skos:Concept ;
    skos:inScheme lorcs: ;
    skos:topConceptOf lorcs: ;
    skos:prefLabel "Follow"@en ;
    skos:definition "Works under close supervision"@en ;
    skos:notation "1" ;
    attributes:ADAP "Accepts change and is open to new ways of working."@en ;
    attributes:AUTO "Follows instructions and works under close direction. Receives specific instructions and guidance, has work closely reviewed."@en ;
    attributes:COLL "Works mostly on their own tasks and interacts with their immediate team only. Develops an understanding of how their work supports others."@en ;
    attributes:COMM "Communicates with immediate team to understand and deliver on their assigned tasks. Observes, listens, and with encouragement, asks questions to seek information or clarify instructions."@en ;
    attributes:COMP "Performs routine activities in a structured environment."@en ;
    attributes:CRTY "Participates in the generation of new ideas when prompted."@en ;
    attributes:DECM """Uses little discretion in attending to enquiries.  
Is expected to seek guidance in unexpected situations."""@en ;
    attributes:DIGI "Has basic digital skills to learn and use applications, processes and tools for their role."@en ;
    attributes:IMPM "Identifies opportunities for improvement in own tasks. Suggests basic enhancements when prompted."@en ;
    attributes:INFL "When required, contributes to team discussions with immediate colleagues."@en ;
    attributes:KNGE "Applies basic knowledge to perform routine, well-defined, predictable role-specific tasks."@en ;
    attributes:LADV "Applies newly acquired knowledge to develop  skills for their role. Contributes to identifying own development opportunities."@en ;
    attributes:LEAD "Proactively increases their understanding of their work tasks and responsibilities."@en ;
    attributes:PLAN "Confirms required steps for individual tasks."@en ;
    attributes:PROB "Works towards understanding the issue and seeks assistance in resolving unexpected problems."@en ;
    attributes:SCPE "Develops an understanding of the rules and expectations of their role and the organisation."@en ;
    sfia:levelEssence "Essence of the level: Performs routine tasks under close supervision, follows instructions, and requires guidance to complete their work. Learns and applies basic skills and knowledge."@en ;
    sfia:levelGuidingPhrase "Follow"@en ;
dcterms:source "https://sfia-online.org/en/lor/9/1"^^xsd:anyURI .

lor:2 a sfia:Level , skos:Concept ;
    skos:inScheme lorcs: ;
    skos:topConceptOf lorcs: ;
    skos:prefLabel "Assist"@en ;
    skos:definition "Works under routine supervision"@en ;
    skos:notation "2" ;
    attributes:ADAP """Adjusts to different team dynamics and work requirements.
Participates in team adaptation processes."""@en ;
    attributes:AUTO "Works under routine direction. Receives instructions and guidance, has work regularly reviewed."@en ;
    attributes:COLL "Understands the need to collaborate with their team and considers user/customer needs."@en ;
    attributes:COMM """Communicates familiar information with immediate team and stakeholders directly related to their role.
Listens to gain understanding and asks relevant questions to clarify or seek further information."""@en ;
    attributes:COMP "Performs a range of work activities in varied environments."@en ;
    attributes:CRTY "Applies creative thinking to suggest new ways to approach a task and solve problems."@en ;
    attributes:DECM """Uses limited discretion in resolving issues or enquiries.
Decides when to seek guidance in unexpected situations."""@en ;
    attributes:DIGI "Has sufficient digital skills for their role; understands and uses appropriate methods, tools, applications and processes."@en ;
    attributes:IMPM """Proposes ideas to improve own work area.

Implements agreed changes to assigned work tasks."""@en ;
    attributes:INFL "Is expected to contribute to team discussions with immediate team members. Works alongside team members, contributing to team decisions. When the role requires, interacts with people outside their team, including internal colleagues and external contacts."@en ;
    attributes:KNGE "Applies knowledge of common workplace tasks and practices to support team activities under guidance."@en ;
    attributes:LADV """Absorbs and applies new information to tasks.
Recognises personal skills and knowledge gaps and seeks learning opportunities to address them."""@en ;
    attributes:LEAD "Takes ownership to develop their work experience."@en ;
    attributes:PLAN "Plans own work within short time horizons in an organised way."@en ;
    attributes:PROB "Investigates and resolves routine issues."@en ;
    attributes:SCPE "Has a good understanding of their role and the organisation's rules and expectations."@en ;
    sfia:levelEssence "Essence of the level: Provides assistance to others, works under routine supervision, and uses their discretion to address routine problems. Actively learns through training and on-the-job experiences."@en ;
    sfia:levelGuidingPhrase "Assist"@en ;
dcterms:source "https://sfia-online.org/en/lor/9/2"^^xsd:anyURI .

lor:3 a sfia:Level , skos:Concept ;
    skos:inScheme lorcs: ;
    skos:topConceptOf lorcs: ;
    skos:prefLabel "Apply"@en ;
    skos:definition "Works under general supervision"@en ;
    skos:notation "3" ;
    attributes:ADAP "Adapts and is responsive to change and shows initiative in adopting new methods or technologies."@en ;
    attributes:AUTO "Works under general direction to complete assigned tasks. Receives guidance and has work reviewed at agreed milestones. When required, delegates routine tasks to others within own team."@en ;
    attributes:COLL "Understands and collaborates on the analysis of user/customer needs and represents this in their work."@en ;
    attributes:COMM """Communicates with team and stakeholders inside and outside the organisation clearly explaining and presenting information.
Contributes to a range of work-related conversations and listens to others to gain an understanding and asks probing questions relevant to their role."""@en ;
    attributes:COMP "Performs a range of work, sometimes complex and non-routine, in varied environments."@en ;
    attributes:CRTY "Applies and contributes to creative thinking techniques to contribute new ideas for their own work and for team activities."@en ;
    attributes:DECM """Uses discretion in identifying and responding to complex issues related to own assignments. 
Determines when issues should be escalated to a higher level."""@en ;
    attributes:DIGI """Explores and applies relevant digital tools and skills for their role.
Understands and effectively applies appropriate methods, tools, applications and processes."""@en ;
    attributes:IMPM """Identifies and implements improvements in own work area.
Contributes to team-level process enhancements."""@en ;
    attributes:INFL "Works with and influences team decisions. Has a transactional level of contact with people outside their team, including internal colleagues and external contacts."@en ;
    attributes:KNGE "Applies knowledge of a range of role-specific practices to complete tasks within defined boundaries and has an appreciation of how this knowledge applies to the wider business context."@en ;
    attributes:LADV """Absorbs and applies new information effectively with the ability to share learnings with colleagues.
Takes the initiative in identifying and negotiating their own appropriate development opportunities."""@en ;
    attributes:LEAD "Provides basic guidance and support to less experienced team members as needed."@en ;
    attributes:PLAN "Organises and keeps track of own work (and others where needed) to meet agreed timescales."@en ;
    attributes:PROB "Applies a methodical approach to investigate and evaluate options to resolve routine and moderately complex issues."@en ;
    attributes:SCPE "Applies appropriate professionalism and working practices and knowledge to work."@en ;
    sfia:levelEssence "Essence of the level: Performs varied tasks, sometimes complex and non-routine, using standard methods and procedures. Works under general direction, exercises discretion, and manages own work within deadlines. Proactively enhances skills and impact in the workplace."@en ;
    sfia:levelGuidingPhrase "Apply"@en ;
dcterms:source "https://sfia-online.org/en/lor/9/3"^^xsd:anyURI .

lor:4 a sfia:Level , skos:Concept ;
    skos:inScheme lorcs: ;
    skos:topConceptOf lorcs: ;
    skos:prefLabel "Enable"@en ;
    skos:definition "Works autonomously"@en ;
    skos:notation "4" ;
    attributes:ADAP "Enables others to adapt and change in response to challenges and changes in the work environment."@en ;
    attributes:AUTO "Works under general direction within a clear framework of accountability. Exercises considerable personal responsibility and autonomy. When required, plans, schedules, and delegates work to others, typically within own team."@en ;
    attributes:COLL """Facilitates collaboration between stakeholders who share common objectives.  
Engages with and contributes to the work of cross-functional teams to ensure that user/customer needs are being met throughout the deliverable/scope of work."""@en ;
    attributes:COMM """Communicates with both technical and non-technical audiences including team and stakeholders inside and outside the organisation.
As required, takes the lead in explaining complex concepts to support decision making.
Listens and asks insightful questions to identify different perspectives to clarify and confirm understanding."""@en ;
    attributes:COMP "Work includes a broad range of complex technical or professional activities in varied contexts."@en ;
    attributes:CRTY "Applies, facilitates and develops creative thinking concepts and finds alternative ways to approach team outcomes."@en ;
    attributes:DECM """Uses judgment and substantial discretion in identifying and responding to complex issues and assignments related to projects and team objectives.
Escalates when scope is impacted."""@en ;
    attributes:DIGI """Maximises the capabilities of applications for their role and evaluates and supports the use of new technologies and digital tools.
Selects appropriately from, and assesses the impact of change to applicable standards, methods, tools, applications and processes relevant to own specialism."""@en ;
    attributes:IMPM """Encourages and supports team discussions on improvement initiatives.

Implements procedural changes within a defined scope of work."""@en ;
    attributes:INFL "Influences projects and team objectives. Has a tactical level of contact with people outside their team, including internal colleagues and external contacts."@en ;
    attributes:KNGE "Applies knowledge across different areas in their field, integrating this knowledge to perform complex and diverse tasks. Applies a working knowledge of the organisation's domain."@en ;
    attributes:LADV """Rapidly absorbs and critically assesses new information and applies it effectively.
Maintains an understanding of emerging practices and their application and takes responsibility for driving own and team members' development opportunities."""@en ;
    attributes:LEAD """Leads, supports or guides team members.
Develops solutions for complex work activities related to assignments.
Demonstrates an understanding of risk factors in their work.
Contributes specialist expertise to requirements definition in support of proposals."""@en ;
    attributes:PLAN "Plans, schedules and monitors work to meet given personal and/or team objectives and processes, demonstrating an analytical approach to meet time and quality targets."@en ;
    attributes:PROB "Investigates the cause and impact, evaluates options and resolves a broad range of complex issues."@en ;
    attributes:SCPE "Adapts and applies applicable standards, recognising their importance in achieving team outcomes."@en ;
    sfia:levelEssence "Essence of the level: Performs diverse complex activities, supports and guides others, delegates tasks when appropriate, works autonomously under general direction, and contributes expertise to deliver team objectives."@en ;
    sfia:levelGuidingPhrase "Enable"@en ;
dcterms:source "https://sfia-online.org/en/lor/9/4"^^xsd:anyURI .

lor:5 a sfia:Level , skos:Concept ;
    skos:inScheme lorcs: ;
    skos:topConceptOf lorcs: ;
    skos:prefLabel "Ensure/Advise"@en ;
    skos:definition "Provides authoritative guidance"@en ;
    skos:notation "5" ;
    attributes:ADAP """Leads adaptations to changing business environments.
Guides teams through transitions, maintaining focus on organisational objectives."""@en ;
    attributes:AUTO "Works under broad direction. Work is self-initiated, consistent with agreed operational and budgetary requirements for meeting allocated technical and/or group objectives. Defines tasks and delegates work to teams and individuals within area of responsibility."@en ;
    attributes:COLL """Facilitates collaboration between stakeholders who have diverse objectives.
Ensures collaborative ways of working throughout all stages of work to meet user/customer needs.
Builds effective relationships across the organisation and with customers, suppliers and partners."""@en ;
    attributes:COMM """Communicates clearly with impact, articulating complex information and ideas to broad audiences with different viewpoints.
Leads and encourages conversations to share ideas and build consensus on actions to be taken."""@en ;
    attributes:COMP "Performs an extensive range of complex technical and/or professional work activities, requiring the application of fundamental principles in a range of unpredictable contexts."@en ;
    attributes:CRTY "Creatively applies innovative thinking and design practices in identifying solutions that will deliver value for the benefit of the customer/stakeholder."@en ;
    attributes:DECM """Uses judgement to make informed decisions on actions to achieve organisational outcomes such as meeting targets, deadlines, and budget.
Raises issues when objectives are at risk."""@en ;
    attributes:DIGI """Recognises and evaluates the organisational impact of new technologies and digital services.
Implements new and effective practices.
Advises on available standards, methods, tools, applications and processes relevant to group specialism(s) and can make appropriate choices from alternatives."""@en ;
    attributes:IMPM """Identifies and evaluates potential improvements to products, practices, or services.
Leads implementation of enhancements within own area of responsibility.
Assesses effectiveness of implemented changes."""@en ;
    attributes:INFL "Influences critical decisions in their domain. Has operational level contact impacting execution and implementation with internal colleagues and external contacts. Has significant influence over the allocation and management of resources required to deliver projects."@en ;
    attributes:KNGE "Applies knowledge to interpret complex situations and offer authoritative advice. Applies in-depth expertise in specific fields, with a broader understanding across industry/business."@en ;
    attributes:LADV """Uses their skills and knowledge to help establish the standards that others in the organisation will apply.
Takes the initiative to develop a wider breadth of knowledge across industry and/or business and identify and manage development opportunities in area of responsibility."""@en ;
    attributes:LEAD """Provides leadership at an operational level.
Implements and executes policies aligned to strategic plans.
Assesses and evaluates risk.
Takes all requirements into account when considering proposals."""@en ;
    attributes:PLAN "Analyses, designs, plans, establishes milestones, and executes and evaluates work to time, cost and quality targets."@en ;
    attributes:PROB "Investigates complex issues to identify the root causes and impacts, assesses a range of solutions, and makes informed decisions on the best course of action, often in collaboration with other experts."@en ;
    attributes:SCPE "Contributes proactively to the implementation of professional working practices and helps promote a supportive organisational culture."@en ;
    sfia:levelEssence "Essence of the level: Provides authoritative guidance in their field and works under broad direction. Accountable for delivering significant work outcomes, from analysis through execution to evaluation."@en ;
    sfia:levelGuidingPhrase "Ensure, advise"@en ;
dcterms:source "https://sfia-online.org/en/lor/9/5"^^xsd:anyURI .

lor:6 a sfia:Level , skos:Concept ;
    skos:inScheme lorcs: ;
    skos:topConceptOf lorcs: ;
    skos:prefLabel "Initiate/Influence"@en ;
    skos:definition "Has organizational influence"@en ;
    skos:notation "6" ;
    attributes:ADAP "Drives organisational adaptability by initiating and leading significant changes. Influences change management strategies at an organisational level."@en ;
    attributes:AUTO "Guides high level decisions and strategies within the organisation's overall policies and objectives. Has defined authority and accountability for actions and decisions within a significant area of work, including technical, financial and quality aspects. Delegates responsibility for operational objectives."@en ;
    attributes:COLL """Leads collaboration with a diverse range of stakeholders across competing objectives within the organisation.
Builds strong, influential connections with key internal and external contacts at senior management/technical leader level"""@en ;
    attributes:COMM """Communicates with credibility at all levels across the organisation to broad audiences with divergent objectives.
Explains complex information and ideas clearly, influencing the strategic direction.
Promotes information sharing across the organisation."""@en ;
    attributes:COMP "Performs highly complex work activities covering technical, financial and quality aspects."@en ;
    attributes:CRTY "Creatively applies a wide range of new ideas and effective management techniques to achieve results that align with organisational strategy."@en ;
    attributes:DECM """Uses judgement to make decisions that initiate the achievement of agreed strategic objectives including financial performance.
Escalates when broader strategic direction is impacted."""@en ;
    attributes:DIGI """Leads the enhancement of the organisation's digital capabilities.
Identifies and endorses opportunities to adopt new technologies and digital services.
Leads digital governance and compliance with relevant legislation and the need for products and services."""@en ;
    attributes:IMPM """Drives improvement initiatives that have a significant impact on the organisation.
Aligns improvement strategies with organisational objectives.
Engages stakeholders in improvement processes."""@en ;
    attributes:INFL "Influences the formation of strategy and the execution of business plans. Has a significant management level of contact with internal colleagues and external contacts. Has organisational leadership and influence over the appointment and management of resources related to the implementation of strategic initiatives."@en ;
    attributes:KNGE "Applies broad business knowledge to enable strategic leadership and decision-making across various domains."@en ;
    attributes:LADV """Promotes the application of knowledge to support strategic imperatives.
Actively develops their strategic and technical leadership skills and leads the development of skills in their area of accountability."""@en ;
    attributes:LEAD """Provides leadership at an organisational level.
Contributes to the development and implementation of policy and strategy.
Understands and communicates industry developments, and the role and impact of technology.
Manages and mitigates organisational risk. 
Balances the requirements of proposals with the broader needs of the organisation."""@en ;
    attributes:PLAN "Initiates and influences strategic objectives and assigns responsibilities."@en ;
    attributes:PROB "Anticipates and leads in addressing problems and opportunities that may impact organisational objectives, establishing a strategic approach and allocating resources."@en ;
    attributes:SCPE "Takes a leading role in promoting and ensuring appropriate culture and working practices, including the provision of equal access and opportunity to people with diverse abilities."@en ;
    sfia:levelEssence "Essence of the level: Has significant organisational influence, makes high-level decisions, shapes policies, demonstrates leadership, promotes organisational collaboration, and accepts accountability in key areas."@en ;
    sfia:levelGuidingPhrase "Initiate, influence"@en ;
dcterms:source "https://sfia-online.org/en/lor/9/6"^^xsd:anyURI .

lor:7 a sfia:Level , skos:Concept ;
    skos:inScheme lorcs: ;
    skos:topConceptOf lorcs: ;
    skos:prefLabel "Set Strategy"@en ;
    skos:definition "Determines vision and strategy"@en ;
    skos:notation "7" ;
    attributes:ADAP """Champions organisational agility and resilience.
Embeds adaptability into organisational culture and strategic planning."""@en ;
    attributes:AUTO "Defines and leads the organisation's vision and strategy within over-arching business objectives. Is fully accountable for actions taken and decisions made, both by self and others to whom responsibilities have been assigned. Delegates authority and responsibility for strategic business objectives."@en ;
    attributes:COLL """Drives collaboration, engaging with leadership stakeholders ensuring alignment to corporate vision and strategy. 
Builds strong, influential relationships with customers, partners and industry leaders."""@en ;
    attributes:COMM """Communicates to audiences at all levels within own organisation and engages with industry.
Presents compelling arguments and ideas authoritatively and convincingly to achieve business objectives."""@en ;
    attributes:COMP "Performs extensive strategic leadership in delivering business value through vision, governance and executive management."@en ;
    attributes:CRTY "Champions creativity and innovation in driving strategy development to enable business opportunities."@en ;
    attributes:DECM """Uses judgement in making decisions critical to the organisational strategic direction and success.
Escalates when business executive management input is required through established governance structures."""@en ;
    attributes:DIGI """Leads the development of the organisation's digital culture and the transformational vision.
Advances capability and/or exploitation of technology within one or more organisations through a deep understanding of the industry and the implications of emerging technologies.
Accountable for assessing how laws and regulations impact organisational objectives and its use of digital, data and technology capabilities."""@en ;
    attributes:IMPM """Defines and communicates the organisational approach to continuous improvement.
Cultivates a culture of ongoing enhancement.
Evaluates the impact of improvement initiatives on organisational success."""@en ;
    attributes:INFL "Directs, influences and inspires the strategic direction and development of the organisation. Has an extensive leadership level of contact with internal colleagues and external contacts. Authorises the appointment of required resources."@en ;
    attributes:KNGE "Applies strategic and broad-based knowledge to shape organisational strategy, anticipate future industry trends, and prepare the organisation to adapt and lead."@en ;
    attributes:LADV """Inspires a learning culture to align with business objectives.
Maintains strategic insight into contemporary and emerging industry landscapes.
Ensures the organisation develops and mobilises the full range of required skills and capabilities."""@en ;
    attributes:LEAD """Leads strategic management.
Applies the highest level of leadership to the formulation and implementation of strategy.
Communicates the potential impact of emerging practices and technologies on organisations and individuals and assesses the risks of using or not using such practices and technologies. 
Establishes governance to address business risk.
Ensures proposals align with the strategic direction of the organisation."""@en ;
    attributes:PLAN "Plans and leads at the highest level of authority over all aspects of a significant area of work."@en ;
    attributes:PROB "Manages inter-relationships between impacted parties and strategic imperatives, recognising the broader business context and drawing accurate conclusions when resolving problems."@en ;
    attributes:SCPE "Provides clear direction and strategic leadership for embedding compliance, organisational culture, and working practices, and actively promotes diversity and inclusivity."@en ;
    sfia:levelEssence "Essence of the level: Operates at the highest organisational level, determines overall organisational vision and strategy, and assumes accountability for overall success."@en ;
    sfia:levelGuidingPhrase "Set strategy, inspire, mobilise"@en ;
dcterms:source "https://sfia-online.org/en/lor/9/7"^^xsd:anyURI .


# owl axioms
sfia:Skill a owl:Class ;
owl:equivalentClass esco:Skill ;
    rdfs:label "Skill"@en .

esco:Skill a owl:Class ;
owl:equivalentClass sfia:Skill ;
    rdfs:label "Skill"@en .

sfia:SkillLevel a owl:Class ;
    rdfs:label "Skill Level"@en .

sfia:Category rdfs:subClassOf skos:Concept ;
    skos:prefLabel "Category"@en .

sfia:Level a owl:Class ;
    rdfs:label "Level of Responsibility"@en .