@prefix dcterms: <http://purl.org/dc/terms/> .
@prefix dewr: <https://linked.data.gov.au/org/dewr> .
@prefix jsa: <https://linked.data.gov.au/org/jsa> .
@prefix nsto: <https://test.linked.data.gov.au/def/nst/ontology#> .
@prefix nstst: <https://test.linked.data.gov.au/def/skillTransfer/> .
@prefix nststcs: <https://test.linked.data.gov.au/def/skillTransfer> .
@prefix owl: <http://www.w3.org/2002/07/owl#> .
@prefix schema: <https://schema.org/> .
@prefix skos: <http://www.w3.org/2004/02/skos/core#> .
@prefix xsd: <http://www.w3.org/2001/XMLSchema#> .

jsa:
a schema:Organization ;
schema:name "Jobs and Skills Australia"@en ;
schema:url "https://wwww.jobsandskills.gov.au"^^xsd:anyURI
.

dewr:
a schema:Organization ;
schema:name "Department of Employment and Work Relations"@en ;
schema:url "https://wwww.dewr.gov.au"^^xsd:anyURI
.

nststcs: a skos:ConceptScheme ;
dcterms:created "2026-02-05"^^xsd:date ;
dcterms:modified "2026-02-05"^^xsd:date ;
owl:versionIRI <https://test.linked.data.gov.au/def/skillTransfer/0.0.1> ;
skos:prefLabel "Skill Transferability"@en ;
skos:definition "Transferability of skills"@en ;
skos:creator jsa: ;
skos:publisher dewr: ;
skos:hasTopConcept 
  nstst:UNI ,
  nstst:BRD ,
  nstst:SEC ,
  nstst:OCC
.

nstst:UNI a skos:Concept ;
skos:inScheme nststcs: ;
skos:topConceptOf nststcs: ;
skos:definition "Foundational skills applicable across all occupations and industries"@en ;
skos:prefLabel "Universal"@en
.

nstst:BRD a skos:Concept ;
skos:inScheme nststcs: ;
skos:topConceptOf nststcs: ;
skos:definition "Specialist skills transferable across multiple industries"@en ;
skos:prefLabel "Broad/Cross-Sector"@en
.

nstst:SEC a skos:Concept ;
skos:inScheme nststcs: ;
skos:topConceptOf nststcs: ;
skos:definition "Skills relevant within a specific sector or closely related industries"@en ;
skos:prefLabel "Sector-Specific"@en
.

nstst:OCC a skos:Concept ;
skos:inScheme nststcs: ;
skos:topConceptOf nststcs: ;
skos:definition "Highly specialized skills unique to particular occupation or role"@en ;
skos:prefLabel "Occupation-Specific"@en
.
