@prefix dcterms: <http://purl.org/dc/terms/> .
@prefix dewr: <https://linked.data.gov.au/org/dewr> .
@prefix jsa: <https://linked.data.gov.au/org/jsa> .
@prefix nsto: <https://test.linked.data.gov.au/def/nst/ontology#> .
@prefix nstsn: <https://test.linked.data.gov.au/def/skillNature/> .
@prefix nstsncs: <https://test.linked.data.gov.au/def/skillNature> .
@prefix owl: <http://www.w3.org/2002/07/owl#> .
@prefix schema: <https://schema.org/> .
@prefix skos: <http://www.w3.org/2004/02/skos/core#> .
@prefix xsd: <http://www.w3.org/2001/XMLSchema#> .

jsa:
a schema:Organization ;
schema:name "Jobs and Skills Australia"@en ;
schema:url "https://wwww.jobsandskills.gov.au"^^xsd:anyURI
.

dewr:
a schema:Organization ;
schema:name "Department of Employment and Work Relations"@en ;
schema:url "https://wwww.dewr.gov.au"^^xsd:anyURI
.

nstsncs: a skos:ConceptScheme ;
dcterms:created "2026-02-05"^^xsd:date ;
dcterms:modified "2026-02-05"^^xsd:date ;
owl:versionIRI <https://test.linked.data.gov.au/def/skillNature/0.0.1> ;
skos:prefLabel "Skill Nature"@en ;
skos:definition "Nature of skills"@en ;
skos:creator jsa: ;
skos:publisher dewr: ;
skos:hasTopConcept 
  nstsn:TEC ,
  nstsn:COG ,
  nstsn:SOC ,
  nstsn:SLF ,
  nstsn:FND ,
  nstsn:REG
.

nstsn:TEC a skos:Concept ;
skos:inScheme nstsncs: ;
skos:topConceptOf nstsncs: ;
skos:definition "Practical, industry-specific skills for operating tools, equipment, and technical systems"@en ;
skos:prefLabel "Technical/Procedural"@en
.

nstsn:COG a skos:Concept ;
skos:inScheme nstsncs: ;
skos:topConceptOf nstsncs: ;
skos:definition "Skills for analysis, reasoning, problem-solving, and informed decision-making"@en ;
skos:prefLabel "Cognitive/Analytical"@en
.

nstsn:SOC a skos:Concept ;
skos:inScheme nstsncs: ;
skos:topConceptOf nstsncs: ;
skos:definition "Skills for collaboration, communication, and managing interpersonal relationships"@en ;
skos:prefLabel "Social/Interpersonal"@en
.

nstsn:SLF a skos:Concept ;
skos:inScheme nstsncs: ;
skos:topConceptOf nstsncs: ;
skos:definition "Capabilities for self-organisation, adaptability, and maintaining professional conduct"@en ;
skos:prefLabel "Self-Management"@en
.

nstsn:FND a skos:Concept ;
skos:inScheme nstsncs: ;
skos:topConceptOf nstsncs: ;
skos:definition "Essential skills in literacy, numeracy, and basic digital fluency"@en ;
skos:prefLabel "Foundational/Core"@en
.

nstsn:REG a skos:Concept ;
skos:inScheme nstsncs: ;
skos:topConceptOf nstsncs: ;
skos:definition "Skills ensuring safety, ethical practice, and compliance with standards"@en ;
skos:prefLabel "Regulatory/Compliance"@en
.
