@prefix dcterms: <http://purl.org/dc/terms/> .
@prefix dewr: <https://linked.data.gov.au/org/dewr> .
@prefix jsa: <https://linked.data.gov.au/org/jsa> .
@prefix nsto: <https://test.linked.data.gov.au/def/nst/ontology#> .
@prefix nstslrnctx: <https://test.linked.data.gov.au/def/skilllearnctx/> .
@prefix nstslrnctxcs: <https://test.linked.data.gov.au/def/skilllearnctx> .
@prefix owl: <http://www.w3.org/2002/07/owl#> .
@prefix schema: <https://schema.org/> .
@prefix skos: <http://www.w3.org/2004/02/skos/core#> .
@prefix xsd: <http://www.w3.org/2001/XMLSchema#> .

jsa:
a schema:Organization ;
schema:name "Jobs and Skills Australia"@en ;
schema:url "https://wwww.jobsandskills.gov.au"^^xsd:anyURI
.

dewr:
a schema:Organization ;
schema:name "Department of Employment and Work Relations"@en ;
schema:url "https://wwww.dewr.gov.au"^^xsd:anyURI
.

nstslrnctxcs: a skos:ConceptScheme ;
dcterms:created "2026-02-05"^^xsd:date ;
dcterms:modified "2026-02-13"^^xsd:date ;
owl:versionIRI <https://test.linked.data.gov.au/def/nstslrnctx/0.0.1> ;
skos:prefLabel "Skill Learning Context"@en ;
skos:definition "Classification defining typical environment for skill development"@en ;
skos:creator jsa: ;
skos:publisher dewr: ;
skos:hasTopConcept 
  nstslrnctx:THE ,
  nstslrnctx:PRA ,
  nstslrnctx:WRK ,
  nstslrnctx:HYB ,
  nstslrnctx:DIG
.

nstslrnctx:THE a skos:Concept ;
skos:inScheme nstslrnctxcs: ;
skos:topConceptOf nstslrnctxcs: ;
skos:definition "Learning focused on theoretical concepts in academic settings"@en ;
skos:prefLabel "Theoretical/Academic"@en
.

nstslrnctx:PRA a skos:Concept ;
skos:inScheme nstslrnctxcs: ;
skos:topConceptOf nstslrnctxcs: ;
skos:definition "Learning through hands-on practice in workshops, labs, or simulations"@en ;
skos:prefLabel "Practical/Hands-on"@en
.

nstslrnctx:WRK a skos:Concept ;
skos:inScheme nstslrnctxcs: ;
skos:topConceptOf nstslrnctxcs: ;
skos:definition "Learning through real-world workplace experience"@en ;
skos:prefLabel "Workplace/On-the-Job"@en
.

nstslrnctx:HYB a skos:Concept ;
skos:inScheme nstslrnctxcs: ;
skos:topConceptOf nstslrnctxcs: ;
skos:definition "Combining theoretical instruction with practical application"@en ;
skos:prefLabel "Hybrid/Blended"@en
.

nstslrnctx:DIG a skos:Concept ;
skos:inScheme nstslrnctxcs: ;
skos:topConceptOf nstslrnctxcs: ;
skos:definition "Learning via digital platforms and self-paced study"@en ;
skos:prefLabel "Digital/Self-Paced"@en
.

