@prefix dcterms: <http://purl.org/dc/terms/> .
@prefix dewr: <https://linked.data.gov.au/org/dewr> .
@prefix jsa: <https://linked.data.gov.au/org/jsa> .
@prefix nsto: <https://test.linked.data.gov.au/def/nst/ontology#> .
@prefix nstsfutread: <https://test.linked.data.gov.au/def/skillfutread/> .
@prefix nstsfutreadcs: <https://test.linked.data.gov.au/def/skillfutread> .
@prefix owl: <http://www.w3.org/2002/07/owl#> .
@prefix schema: <https://schema.org/> .
@prefix skos: <http://www.w3.org/2004/02/skos/core#> .
@prefix xsd: <http://www.w3.org/2001/XMLSchema#> .

jsa:
a schema:Organization ;
schema:name "Jobs and Skills Australia"@en ;
schema:url "https://wwww.jobsandskills.gov.au"^^xsd:anyURI
.

dewr:
a schema:Organization ;
schema:name "Department of Employment and Work Relations"@en ;
schema:url "https://wwww.dewr.gov.au"^^xsd:anyURI
.

nstsfutreadcs: a skos:ConceptScheme ;
dcterms:created "2026-02-05"^^xsd:date ;
dcterms:modified "2026-02-13"^^xsd:date ;
owl:versionIRI <https://test.linked.data.gov.au/def/nstsfutread/0.0.1> ;
skos:prefLabel "Skill Future Readiness"@en ;
skos:definition "Classification indicating skill's resilience to automation and future demand"@en ;
skos:creator jsa: ;
skos:publisher dewr: ;
skos:hasTopConcept 
  nstsfutread:HUM ,
  nstsfutread:COL ,
  nstsfutread:AUG ,
  nstsfutread:AUT ,
  nstsfutread:EMG
.

nstsfutread:HUM a skos:Concept ;
skos:inScheme nstsfutreadcs: ;
skos:topConceptOf nstsfutreadcs: ;
skos:definition "Skills requiring human judgment, empathy, creativity; resistant to automation"@en ;
skos:prefLabel "Uniquely Human"@en
.

nstsfutread:COL a skos:Concept ;
skos:inScheme nstsfutreadcs: ;
skos:topConceptOf nstsfutreadcs: ;
skos:definition "Skills augmented by AI, requiring human oversight"@en ;
skos:prefLabel "Human-AI Collaborative"@en
.

nstsfutread:AUG a skos:Concept ;
skos:inScheme nstsfutreadcs: ;
skos:topConceptOf nstsfutreadcs: ;
skos:definition "Skills where AI boosts efficiency but human expertise essential"@en ;
skos:prefLabel "AI-Augmentable"@en
.

nstsfutread:AUT a skos:Concept ;
skos:inScheme nstsfutreadcs: ;
skos:topConceptOf nstsfutreadcs: ;
skos:definition "Routine tasks highly susceptible to automation"@en ;
skos:prefLabel "Automatable"@en
.

nstsfutread:EMG a skos:Concept ;
skos:inScheme nstsfutreadcs: ;
skos:topConceptOf nstsfutreadcs: ;
skos:definition "Skills in rapidly growing areas driven by emerging technologies"@en ;
skos:prefLabel "Emerging"@en
.

