PREFIX skillctx:    <https://example.com/skillctx/>
PREFIX skillctxcs:  <https://example.com/skillctxcs>
PREFIX dcterms:     <http://purl.org/dc/terms/> 
PREFIX dewr:        <https://linked.data.gov.au/org/dewr>
PREFIX jsa:         <https://linked.data.gov.au/org/jsa>
PREFIX nst:         <https://test.linked.data.gov.au/def/nst>
PREFIX owl:         <http://www.w3.org/2002/07/owl#>
PREFIX rdfs:        <http://www.w3.org/2000/01/rdf-schema#>
PREFIX ror:         <https://ror.org/>
PREFIX schema:      <https://schema.org/>
PREFIX skos:        <http://www.w3.org/2004/02/skos/core#>
PREFIX xsd:         <http://www.w3.org/2001/XMLSchema#>

dewr:
a schema:Organization ;
schema:name "Jobs and Skills Australia"@en ;
schema:alternateName "JSA"@en ;
schema:url "https://www.jobsandskills.gov.au"^^xsd:anyURI
.

jsa:
a schema:Organization ;
schema:name "Jobs and Skills Australia"@en ;
schema:alternateName "JSA"@en ;
schema:url "https://www.jobsandskills.gov.au"^^xsd:anyURI
.

skillctxcs: a skos:ConceptScheme ;
dcterms:creator jsa: ;
dcterms:publisher dewr: ;
skos:PrefLabel "Skill context"@en ;
skos:Definition "Indicates the educational context  of the skill and whether taught/learnt in theory or practice: theoretical, practical or hybrid"@en ;
skos:hasTopConcept skillctx:hybrid , skillctx:practial , skillcxt:theoretical
.

skillctx:hybrid a skos:Concept ;
skos:prefLabel: "Hybrid"@en ;
skos:definition: "Skills requiring BOTH theoretical understanding AND practical application"@en ;
skos:inScheme skillctxcs: ;
skos:topConceptOf skillctxcs: 
.

skillctx:practial a skos:Concept ;
skos:prefLabel: "Practical"@en ;
skos:definition: "Skills focused on hands-on application, implementation, and doing"@en ;
skos:inScheme skillctxcs: ;
skos:topConceptOf skillctxcs: 
.

skillctx:theoretical a skos:Concept ;
skos:prefLabel: "Theoretical"@en ;
skos:definition: "Skills focused on understanding concepts, principles, and knowledge without direct application"@en ;
skos:inScheme skillctxcs: ;
skos:topConceptOf skillctxcs: 
.
